<?xml version="1.0"?>
<rdf:RDF xmlns="http://www.oasis-open.org/ciq_xnl#"
     xml:base="http://www.oasis-open.org/ciq_xnl"
     xmlns:rdf="http://www.w3.org/1999/02/22-rdf-syntax-ns#"
     xmlns:owl="http://www.w3.org/2002/07/owl#"
     xmlns:xml="http://www.w3.org/XML/1998/namespace"
     xmlns:ciq_xnl="http://www.oasis-open.org/ciq_xnl#"
     xmlns:xsd="http://www.w3.org/2001/XMLSchema#"
     xmlns:rdfs="http://www.w3.org/2000/01/rdf-schema#">
    <owl:Ontology rdf:about="http://www.oasis-open.org/ciq_xnl">
        <owl:imports rdf:resource="http://www.oasis-open.org/ciq_common"/>
        <rdfs:label>OASIS Customer Information Quality (CIQ) eXtensible Naming Language (xNL) Ontology</rdfs:label>
        <rdfs:comment>This ontology provides a vocabulary and representation of the OASIS Customer Information Quality (CIQ) eXtensible Naming Language (xNL) Specification V3.0.

Copyright (c) 2014, DaedaFusion, LLC.  All rights reserved.</rdfs:comment>
        <owl:versionInfo rdf:datatype="http://www.w3.org/2001/XMLSchema#string">1.0.0-001</owl:versionInfo>
    </owl:Ontology>
    




    <!-- 
    ///////////////////////////////////////////////////////////////////////////////////////
    //
    // Object Properties
    //
    ///////////////////////////////////////////////////////////////////////////////////////
     -->

    


    <!-- http://www.oasis-open.org/ciq_xnl#nameDetails -->

    <owl:ObjectProperty rdf:about="http://www.oasis-open.org/ciq_xnl#nameDetails">
        <rdfs:range>
            <owl:Class>
                <owl:unionOf rdf:parseType="Collection">
                    <rdf:Description rdf:about="http://www.oasis-open.org/ciq_xnl#OrganizationName"/>
                    <rdf:Description rdf:about="http://www.oasis-open.org/ciq_xnl#PersonName"/>
                </owl:unionOf>
            </owl:Class>
        </rdfs:range>
        <rdfs:comment>Specifies details about the names associated with the party</rdfs:comment>
        <rdfs:isDefinedBy rdf:resource="http://www.oasis-open.org/ciq_xnl"/>
        <rdfs:label>Name Details</rdfs:label>
    </owl:ObjectProperty>
    


    <!-- http://www.oasis-open.org/ciq_xnl#organizationName.subdivision -->

    <owl:ObjectProperty rdf:about="http://www.oasis-open.org/ciq_xnl#organizationName.subdivision">
        <rdfs:range rdf:resource="http://www.oasis-open.org/ciq_xnl#Subdivison"/>
        <rdfs:comment>Specifies a sub-division of the organization</rdfs:comment>
        <rdfs:label>Organization Sub-Division</rdfs:label>
    </owl:ObjectProperty>
    


    <!-- http://www.oasis-open.org/ciq_xnl#otherNames -->

    <owl:ObjectProperty rdf:about="http://www.oasis-open.org/ciq_xnl#otherNames">
        <rdfs:comment>Specifies any other additional names that are not directly used to identify or call the individual, such as names of ancestors, saints, etc.</rdfs:comment>
        <rdfs:label>Other Name</rdfs:label>
    </owl:ObjectProperty>
    


    <!-- http://www.oasis-open.org/ciq_xnl#personName.MaidenName -->

    <owl:ObjectProperty rdf:about="http://www.oasis-open.org/ciq_xnl#personName.MaidenName">
        <rdfs:comment>Specifies the name of the individual before marriage.</rdfs:comment>
        <rdfs:label>Maiden Name</rdfs:label>
    </owl:ObjectProperty>
    


    <!-- http://www.oasis-open.org/ciq_xnl#personName.aliases -->

    <owl:ObjectProperty rdf:about="http://www.oasis-open.org/ciq_xnl#personName.aliases">
        <rdfs:comment>Specifies other names by which the person is know.</rdfs:comment>
        <rdfs:label>Aliases</rdfs:label>
    </owl:ObjectProperty>
    


    <!-- http://www.oasis-open.org/ciq_xnl#personName.birthName -->

    <owl:ObjectProperty rdf:about="http://www.oasis-open.org/ciq_xnl#personName.birthName">
        <rdfs:comment>Specifies the name given to an individual at birth, but later changed (common in some cultures).</rdfs:comment>
        <rdfs:label>Name at Birth</rdfs:label>
    </owl:ObjectProperty>
    


    <!-- http://www.oasis-open.org/ciq_xnl#personName.commonUse -->

    <owl:ObjectProperty rdf:about="http://www.oasis-open.org/ciq_xnl#personName.commonUse">
        <rdfs:comment>Specifies the name that is comonly used by others, e.g., a simplied form of the official name.</rdfs:comment>
        <rdfs:label>person name.Common use</rdfs:label>
    </owl:ObjectProperty>
    


    <!-- http://www.oasis-open.org/ciq_xnl#personName.formerName -->

    <owl:ObjectProperty rdf:about="http://www.oasis-open.org/ciq_xnl#personName.formerName">
        <rdfs:comment>Specifies the former name of the individual</rdfs:comment>
        <rdfs:label>Former Name</rdfs:label>
    </owl:ObjectProperty>
    


    <!-- http://www.oasis-open.org/ciq_xnl#personName.knownAs -->

    <owl:ObjectProperty rdf:about="http://www.oasis-open.org/ciq_xnl#personName.knownAs">
        <rdfs:comment>Specifies names that the person is also known as</rdfs:comment>
        <rdfs:label>Known As</rdfs:label>
    </owl:ObjectProperty>
    


    <!-- http://www.oasis-open.org/ciq_xnl#personName.legalName -->

    <owl:ObjectProperty rdf:about="http://www.oasis-open.org/ciq_xnl#personName.legalName">
        <rdfs:comment>Specifies the individual&apos;s legal name</rdfs:comment>
        <rdfs:label>Legal Name</rdfs:label>
    </owl:ObjectProperty>
    


    <!-- http://www.oasis-open.org/ciq_xnl#personName.officialName -->

    <owl:ObjectProperty rdf:about="http://www.oasis-open.org/ciq_xnl#personName.officialName">
        <rdfs:comment>Specifies the official name of the person, e.g., as in the passport, incorporation certificate, etc.</rdfs:comment>
        <rdfs:label>Official Name</rdfs:label>
    </owl:ObjectProperty>
    


    <!-- http://www.oasis-open.org/ciq_xnl#personName.unofficialName -->

    <owl:ObjectProperty rdf:about="http://www.oasis-open.org/ciq_xnl#personName.unofficialName">
        <rdfs:comment>Specifies an unofficial name that the individual is known to go by.</rdfs:comment>
        <rdfs:label>Unofficial Name</rdfs:label>
    </owl:ObjectProperty>
    


    <!-- 
    ///////////////////////////////////////////////////////////////////////////////////////
    //
    // Data properties
    //
    ///////////////////////////////////////////////////////////////////////////////////////
     -->

    


    <!-- http://www.oasis-open.org/ciq_xnl#jointNameConnector -->

    <owl:DatatypeProperty rdf:about="http://www.oasis-open.org/ciq_xnl#jointNameConnector">
        <rdfs:range rdf:resource="http://www.w3.org/2001/XMLSchema#string"/>
        <rdfs:comment>Specifies the connector used to join more than one person name.  Example: Mr. Hunt AND Mrs Clark, where AND is the joint name connector.  If there is more than 2 names, then all names are connected using the this connector in the natural order.</rdfs:comment>
        <rdfs:label>Joint Name Connector</rdfs:label>
    </owl:DatatypeProperty>
    


    <!-- http://www.oasis-open.org/ciq_xnl#nameLine -->

    <owl:DatatypeProperty rdf:about="http://www.oasis-open.org/ciq_xnl#nameLine">
        <rdfs:range rdf:resource="http://www.w3.org/2001/XMLSchema#string"/>
        <rdfs:comment>Specifies a name as a free-form text.  Use this when the type of the entity (person or organization) is unknown or is not broken down into individual elements (e.g., unstructured, unparsed) or is beyond the provided types.  The name represented may be formatted in the righ order or may not be as it is not parsed/broken into atomic fields</rdfs:comment>
        <rdfs:label>Name</rdfs:label>
    </owl:DatatypeProperty>
    


    <!-- http://www.oasis-open.org/ciq_xnl#nameLineType -->

    <owl:DatatypeProperty rdf:about="http://www.oasis-open.org/ciq_xnl#nameLineType">
        <rdfs:range rdf:resource="http://www.w3.org/2001/XMLSchema#string"/>
        <rdfs:comment>Specifies what the free form name line means.  For example, the type could be &quot;Unknown&quot;</rdfs:comment>
        <rdfs:label>Name Line Type</rdfs:label>
    </owl:DatatypeProperty>
    


    <!-- http://www.oasis-open.org/ciq_xnl#organizationIdType -->

    <owl:DatatypeProperty rdf:about="http://www.oasis-open.org/ciq_xnl#organizationIdType">
        <rdfs:range rdf:resource="http://www.w3.org/2001/XMLSchema#string"/>
        <rdfs:comment>Specifies the type of an organization ID</rdfs:comment>
        <rdfs:label>Organization ID Type</rdfs:label>
    </owl:DatatypeProperty>
    


    <!-- http://www.oasis-open.org/ciq_xnl#organizationName.branch -->

    <owl:DatatypeProperty rdf:about="http://www.oasis-open.org/ciq_xnl#organizationName.branch">
        <rdfs:range rdf:resource="http://www.w3.org/2001/XMLSchema#string"/>
        <rdfs:comment>Specifies the name of a branch within an organization</rdfs:comment>
        <rdfs:label>Organization Branch Name</rdfs:label>
    </owl:DatatypeProperty>
    


    <!-- http://www.oasis-open.org/ciq_xnl#organizationName.businessUnit -->

    <owl:DatatypeProperty rdf:about="http://www.oasis-open.org/ciq_xnl#organizationName.businessUnit">
        <rdfs:range rdf:resource="http://www.w3.org/2001/XMLSchema#string"/>
        <rdfs:comment>Specifies the name of a business unit within an organization</rdfs:comment>
        <rdfs:label>Organization Business Unit Name</rdfs:label>
    </owl:DatatypeProperty>
    


    <!-- http://www.oasis-open.org/ciq_xnl#organizationName.department -->

    <owl:DatatypeProperty rdf:about="http://www.oasis-open.org/ciq_xnl#organizationName.department">
        <rdfs:range rdf:resource="http://www.w3.org/2001/XMLSchema#string"/>
        <rdfs:comment>Specifies the name of the department within an organization.</rdfs:comment>
        <rdfs:label>Organization Department Name</rdfs:label>
    </owl:DatatypeProperty>
    


    <!-- http://www.oasis-open.org/ciq_xnl#organizationName.division -->

    <owl:DatatypeProperty rdf:about="http://www.oasis-open.org/ciq_xnl#organizationName.division">
        <rdfs:range rdf:resource="http://www.w3.org/2001/XMLSchema#string"/>
        <rdfs:comment>Specifies the name of the division within an organization.</rdfs:comment>
        <rdfs:label>Organization Division</rdfs:label>
    </owl:DatatypeProperty>
    


    <!-- http://www.oasis-open.org/ciq_xnl#organizationName.fullName -->

    <owl:DatatypeProperty rdf:about="http://www.oasis-open.org/ciq_xnl#organizationName.fullName">
        <rdfs:range rdf:resource="http://www.w3.org/2001/XMLSchema#string"/>
        <rdfs:comment>Specifies the full name of an organization, including its name, propriety type, liability type, etc.(e.g., Sakthisoft Pty. Ltd)</rdfs:comment>
        <rdfs:label>Full Name</rdfs:label>
    </owl:DatatypeProperty>
    


    <!-- http://www.oasis-open.org/ciq_xnl#organizationName.nameOnly -->

    <owl:DatatypeProperty rdf:about="http://www.oasis-open.org/ciq_xnl#organizationName.nameOnly">
        <rdfs:range rdf:resource="http://www.w3.org/2001/XMLSchema#string"/>
        <rdfs:comment>Specifies just the name of the organization.  For example, in &quot;Sakthisoft Pty. Ltd&quot;, &quot;Pty. Ltd&quot; is the legal entity for the organization name &quot;Sakthisoft&quot;</rdfs:comment>
        <rdfs:label>Organization Name</rdfs:label>
    </owl:DatatypeProperty>
    


    <!-- http://www.oasis-open.org/ciq_xnl#organizationName.orgType -->

    <owl:DatatypeProperty rdf:about="http://www.oasis-open.org/ciq_xnl#organizationName.orgType">
        <rdfs:range rdf:resource="http://www.w3.org/2001/XMLSchema#string"/>
        <rdfs:comment>Specifies the type of the organization.  &quot;Pty. Ltd&quot; in Sakthisoft Pty.Ltd, where &quot;Sakthisoft&quot; is the name of the organisation, &quot;Inc&quot; in ABC Inc, where &quot;ABC&quot; is organisation name.</rdfs:comment>
        <rdfs:label>organization name.org type</rdfs:label>
    </owl:DatatypeProperty>
    


    <!-- http://www.oasis-open.org/ciq_xnl#organizationName.school -->

    <owl:DatatypeProperty rdf:about="http://www.oasis-open.org/ciq_xnl#organizationName.school">
        <rdfs:range rdf:resource="http://www.w3.org/2001/XMLSchema#string"/>
        <rdfs:comment>Specifies the name of a school within an organization</rdfs:comment>
        <rdfs:label>Organization School Name</rdfs:label>
    </owl:DatatypeProperty>
    


    <!-- http://www.oasis-open.org/ciq_xnl#organizationName.section -->

    <owl:DatatypeProperty rdf:about="http://www.oasis-open.org/ciq_xnl#organizationName.section">
        <rdfs:range rdf:resource="http://www.w3.org/2001/XMLSchema#string"/>
        <rdfs:comment>Specifies the name of a section within an organization.</rdfs:comment>
        <rdfs:label>Organization Section Name</rdfs:label>
    </owl:DatatypeProperty>
    


    <!-- http://www.oasis-open.org/ciq_xnl#organizationNameType -->

    <owl:DatatypeProperty rdf:about="http://www.oasis-open.org/ciq_xnl#organizationNameType">
        <rdfs:range rdf:resource="http://www.w3.org/2001/XMLSchema#string"/>
        <rdfs:comment>Specifies just the type of an organization without its name. For example, in &quot;Sakthisoft Pty. Ltd&quot;, &quot;Pty. Ltd&quot; is the legal entity  or type for the organization name &quot;Sakthisoft&quot;, &quot;Inc.&quot; in &quot;ABC, Inc.&quot; &quot;Inc.&quot; is the type and &quot;ABC&quot; is the organization name</rdfs:comment>
        <rdfs:label>Type</rdfs:label>
    </owl:DatatypeProperty>
    


    <!-- http://www.oasis-open.org/ciq_xnl#organizationNameUsage -->

    <owl:DatatypeProperty rdf:about="http://www.oasis-open.org/ciq_xnl#organizationNameUsage">
        <rdfs:range rdf:resource="http://www.w3.org/2001/XMLSchema#string"/>
        <rdfs:comment>Specifies how an organization&apos;s name can be used and for what purposes.   It provides an indication of which name is a set of names to select for a given purpose. (e..g, used for legal purposes)</rdfs:comment>
        <rdfs:label>Organization Name Usage</rdfs:label>
    </owl:DatatypeProperty>
    


    <!-- http://www.oasis-open.org/ciq_xnl#partyName -->

    <owl:DatatypeProperty rdf:about="http://www.oasis-open.org/ciq_xnl#partyName">
        <rdfs:range rdf:resource="http://www.w3.org/2001/XMLSchema#string"/>
        <rdfs:comment>Specifies the name of a party when it is unknown whether the party is an person or an organziation.</rdfs:comment>
        <rdfs:label>Name of Party</rdfs:label>
    </owl:DatatypeProperty>
    


    <!-- http://www.oasis-open.org/ciq_xnl#partyName.jointNameConnector -->

    <owl:DatatypeProperty rdf:about="http://www.oasis-open.org/ciq_xnl#partyName.jointNameConnector">
       <rdfs:range rdf:resource="http://www.w3.org/2001/XMLSchema#string"/>
        <rdfs:comment>Specifies the connector used to join more than one person name.

E xample: Mr Hunt AND Mrs Clark, where AND is the JointNameConnector.  The flow is from the preceding to the following. If there is more than 2 names then all names are connected using this connector in the natural order.</rdfs:comment>
        <rdfs:label>party name.Joint name connector</rdfs:label>
    </owl:DatatypeProperty>
    


    <!-- http://www.oasis-open.org/ciq_xnl#partyNameId -->

    <owl:DatatypeProperty rdf:about="http://www.oasis-open.org/ciq_xnl#partyNameId">
        <rdfs:range rdf:resource="http://www.w3.org/2001/XMLSchema#string"/>
        <rdfs:comment>Specifies a unique identifier for a party</rdfs:comment>
        <rdfs:label>Party Name ID</rdfs:label>
    </owl:DatatypeProperty>
    


    <!-- http://www.oasis-open.org/ciq_xnl#partyNameType -->

    <owl:DatatypeProperty rdf:about="http://www.oasis-open.org/ciq_xnl#partyNameType">
       <rdfs:range rdf:resource="http://www.w3.org/2001/XMLSchema#string"/>
        <rdfs:comment>Specifies the type of a Party Name ID</rdfs:comment>
        <rdfs:label>Party Name ID Type</rdfs:label>
    </owl:DatatypeProperty>
    


    <!-- http://www.oasis-open.org/ciq_xnl#partyNameUsage -->

    <owl:DatatypeProperty rdf:about="http://www.oasis-open.org/ciq_xnl#partyNameUsage">
        <rdfs:range rdf:resource="http://www.w3.org/2001/XMLSchema#string"/>
        <rdfs:comment>Specifies how a party&apos;s name can be used and for what purposes (e.g., data exchange, contact, update, create).</rdfs:comment>
        <rdfs:label>Party Name Usage</rdfs:label>
    </owl:DatatypeProperty>
    


    <!-- http://www.oasis-open.org/ciq_xnl#personId -->

    <owl:DatatypeProperty rdf:about="http://www.oasis-open.org/ciq_xnl#personId">
        <rdfs:range rdf:resource="http://www.w3.org/2001/XMLSchema#string"/>
        <rdfs:comment>Specifies a unique identifier of a person</rdfs:comment>
        <rdfs:label>Person ID</rdfs:label>
    </owl:DatatypeProperty>
    


    <!-- http://www.oasis-open.org/ciq_xnl#personIdType -->

    <owl:DatatypeProperty rdf:about="http://www.oasis-open.org/ciq_xnl#personIdType">
        <rdfs:range rdf:resource="http://www.w3.org/2001/XMLSchema#string"/>
        <rdfs:comment>Specifies a type of person ID</rdfs:comment>
        <rdfs:label>Person ID Type</rdfs:label>
    </owl:DatatypeProperty>
    


    <!-- http://www.oasis-open.org/ciq_xnl#personName.credentials -->

    <owl:DatatypeProperty rdf:about="http://www.oasis-open.org/ciq_xnl#personName.credentials">
        <rdfs:range rdf:resource="http://www.w3.org/2001/XMLSchema#string"/>
        <rdfs:comment>Specifies an educational degree or credentials (e.g., PhD)</rdfs:comment>
        <rdfs:label>Credentials</rdfs:label>
    </owl:DatatypeProperty>
    


    <!-- http://www.oasis-open.org/ciq_xnl#personName.firstName -->

    <owl:DatatypeProperty rdf:about="http://www.oasis-open.org/ciq_xnl#personName.firstName">
        <rdfs:range rdf:resource="http://www.w3.org/2001/XMLSchema#string"/>
        <rdfs:comment>Specifies the most important name element by which this particular individual is identified in the group (e.g., John, Sam, Brian for Anglo-Saxon cultures)</rdfs:comment>
        <rdfs:label>First Name</rdfs:label>
    </owl:DatatypeProperty>
    


    <!-- http://www.oasis-open.org/ciq_xnl#personName.generationIdentifier -->

    <owl:DatatypeProperty rdf:about="http://www.oasis-open.org/ciq_xnl#personName.generationIdentifier">
        <rdfs:range rdf:resource="http://www.w3.org/2001/XMLSchema#string"/>
        <rdfs:comment>Specifies a generational identifier (e.g., Jr, Sr, 2nd, IV, etc.)</rdfs:comment>
        <rdfs:label>Generation Identifier</rdfs:label>
    </owl:DatatypeProperty>
    


    <!-- http://www.oasis-open.org/ciq_xnl#personName.lastName -->

    <owl:DatatypeProperty rdf:about="http://www.oasis-open.org/ciq_xnl#personName.lastName">
        <rdfs:range rdf:resource="http://www.w3.org/2001/XMLSchema#string"/>
        <rdfs:comment>Specifies the name elemnt that identifies the group the individual belongs to and is identified by, such as last name, surname, family name, etc.</rdfs:comment>
        <rdfs:label>Last Name</rdfs:label>
    </owl:DatatypeProperty>
    


    <!-- http://www.oasis-open.org/ciq_xnl#personName.middleName -->

    <owl:DatatypeProperty rdf:about="http://www.oasis-open.org/ciq_xnl#personName.middleName">
        <rdfs:range rdf:resource="http://www.w3.org/2001/XMLSchema#string"/>
        <rdfs:comment>Specifies the name element related to additional identification of the individual, such names are parents or places</rdfs:comment>
        <rdfs:label>Middle Name</rdfs:label>
    </owl:DatatypeProperty>
    


    <!-- http://www.oasis-open.org/ciq_xnl#personName.nickname -->

    <owl:DatatypeProperty rdf:about="http://www.oasis-open.org/ciq_xnl#personName.nickname">
        <rdfs:range rdf:resource="http://www.w3.org/2001/XMLSchema#string"/>
        <rdfs:comment>Specifies a simple nick name that is commonly used as part of the name (e.g., a fancy kick-boxer can be commonly known as Bill &quot;Storm&quot; Bababoons, where &quot;Storm&quot; is obviously an alias)</rdfs:comment>
        <rdfs:label>Nickname</rdfs:label>
    </owl:DatatypeProperty>
    


    <!-- http://www.oasis-open.org/ciq_xnl#personName.otherName -->

    <owl:DatatypeProperty rdf:about="http://www.oasis-open.org/ciq_xnl#personName.otherName">
        <rdfs:range rdf:resource="http://www.w3.org/2001/XMLSchema#string"/>
        <rdfs:comment>Specifies any other additional names that are not directly used to identify or call the individual, such as names of ancestors, saints, etc.</rdfs:comment>
        <rdfs:isDefinedBy rdf:resource="http://www.oasis-open.org/ciq_xnl"/>
        <rdfs:label>Other Name</rdfs:label>
    </owl:DatatypeProperty>
    


    <!-- http://www.oasis-open.org/ciq_xnl#personName.petName -->

    <owl:DatatypeProperty rdf:about="http://www.oasis-open.org/ciq_xnl#personName.petName">
        <rdfs:range rdf:resource="http://www.w3.org/2001/XMLSchema#string"/>
        <rdfs:comment>Specifies a &quot;pet name&quot; by which the person is known to individuals that have a close relationship with the person.</rdfs:comment>
        <rdfs:label>Pet Name</rdfs:label>
    </owl:DatatypeProperty>
    


    <!-- http://www.oasis-open.org/ciq_xnl#personName.precedingTitle -->

    <owl:DatatypeProperty rdf:about="http://www.oasis-open.org/ciq_xnl#personName.precedingTitle">
        <rdfs:range rdf:resource="http://www.w3.org/2001/XMLSchema#string"/>
        <rdfs:comment>Specifies the preceding title of a person (e.g., His Excellency, Honorable, etc.)</rdfs:comment>
        <rdfs:label>Preceding Title</rdfs:label>
    </owl:DatatypeProperty>
    


    <!-- http://www.oasis-open.org/ciq_xnl#personName.preferredName -->

    <owl:DatatypeProperty rdf:about="http://www.oasis-open.org/ciq_xnl#personName.preferredName">
        <rdfs:range rdf:resource="http://www.w3.org/2001/XMLSchema#string"/>
        <rdfs:comment>Specifies the name that the individual prefers to be called by, e.g., &quot;Jim&quot; instead of &quot;James&quot;, &quot;Bill&quot; instead of &quot;William&quot;</rdfs:comment>
        <rdfs:label>Preferred Name</rdfs:label>
    </owl:DatatypeProperty>
    


    <!-- http://www.oasis-open.org/ciq_xnl#personName.title -->

    <owl:DatatypeProperty rdf:about="http://www.oasis-open.org/ciq_xnl#personName.title">
        <rdfs:range rdf:resource="http://www.w3.org/2001/XMLSchema#string"/>
        <rdfs:comment>Specifies a title of some sorts, such as Mr, Miss, Ms (marriage status), or eduction such as Professor, Phd, Dr, etc.</rdfs:comment>
        <rdfs:label>Title</rdfs:label>
    </owl:DatatypeProperty>
    


    <!-- http://www.oasis-open.org/ciq_xnl#personNameType -->

    <owl:DatatypeProperty rdf:about="http://www.oasis-open.org/ciq_xnl#personNameType">
        <rdfs:range rdf:resource="http://www.w3.org/2001/XMLSchema#string"/>
        <rdfs:comment>Specifies common types of person names</rdfs:comment>
        <rdfs:label>Person Name Type</rdfs:label>
    </owl:DatatypeProperty>
    


    <!-- http://www.oasis-open.org/ciq_xnl#personNameUsage -->

    <owl:DatatypeProperty rdf:about="http://www.oasis-open.org/ciq_xnl#personNameUsage">
        <rdfs:range rdf:resource="http://www.w3.org/2001/XMLSchema#string"/>
        <rdfs:comment>Specifies how a person&apos;s name can be used and for what purposes.  It provides an indication of which name is a set of names to select for a given purpose. (e..g, used for legal purposes)</rdfs:comment>
        <rdfs:label>Person Name Usage</rdfs:label>
    </owl:DatatypeProperty>
    


    <!-- http://www.oasis-open.org/ciq_xnl#subDivisionType -->

    <owl:DatatypeProperty rdf:about="http://www.oasis-open.org/ciq_xnl#subDivisionType">
      <rdfs:range rdf:resource="http://www.w3.org/2001/XMLSchema#string"/>
        <rdfs:comment>Specifies a type of subdivision of an organization</rdfs:comment>
        <rdfs:label>Subdivision Type</rdfs:label>
    </owl:DatatypeProperty>
    


    <!-- http://www.oasis-open.org/ciq_xnl#subdivision.branchName -->

    <owl:DatatypeProperty rdf:about="http://www.oasis-open.org/ciq_xnl#subdivision.branchName">
        <rdfs:range rdf:resource="http://www.w3.org/2001/XMLSchema#string"/>
        <rdfs:comment>Specifies the branch name of an organization&apos;s subdivision</rdfs:comment>
        <rdfs:isDefinedBy rdf:resource="http://www.oasis-open.org/ciq_xnl"/>
        <rdfs:label>SubDivision Branch Name</rdfs:label>
    </owl:DatatypeProperty>
    


    <!-- http://www.oasis-open.org/ciq_xnl#subdivision.businessUnitName -->

    <owl:DatatypeProperty rdf:about="http://www.oasis-open.org/ciq_xnl#subdivision.businessUnitName">
        <rdfs:range rdf:resource="http://www.w3.org/2001/XMLSchema#string"/>
        <rdfs:comment>Specifies the business unit name of an organization&apos;s subdivision</rdfs:comment>
        <rdfs:isDefinedBy rdf:resource="http://www.oasis-open.org/ciq_xnl"/>
        <rdfs:label>subdivision.business unit name</rdfs:label>
    </owl:DatatypeProperty>
    


    <!-- http://www.oasis-open.org/ciq_xnl#subdivision.departmentName -->

    <owl:DatatypeProperty rdf:about="http://www.oasis-open.org/ciq_xnl#subdivision.departmentName">
        <rdfs:range rdf:resource="http://www.w3.org/2001/XMLSchema#string"/>
        <rdfs:comment>Specifies the department name of an organization&apos;s subdivision</rdfs:comment>
        <rdfs:isDefinedBy rdf:resource="http://www.oasis-open.org/ciq_xnl"/>
        <rdfs:label>subdivision.department name</rdfs:label>
    </owl:DatatypeProperty>
    


    <!-- http://www.oasis-open.org/ciq_xnl#subdivision.divisionName -->

    <owl:DatatypeProperty rdf:about="http://www.oasis-open.org/ciq_xnl#subdivision.divisionName">
        <rdfs:range rdf:resource="http://www.w3.org/2001/XMLSchema#string"/>
        <rdfs:comment>Specifies the division name of an organization&apos;s subdivision</rdfs:comment>
        <rdfs:isDefinedBy rdf:resource="http://www.oasis-open.org/ciq_xnl"/>
        <rdfs:label>subdivision.division name</rdfs:label>
    </owl:DatatypeProperty>
    


    <!-- http://www.oasis-open.org/ciq_xnl#subdivision.schoolName -->

    <owl:DatatypeProperty rdf:about="http://www.oasis-open.org/ciq_xnl#subdivision.schoolName">
        <rdfs:range rdf:resource="http://www.w3.org/2001/XMLSchema#string"/>
        <rdfs:comment>Specifies the school name of an organization&apos;s subdivision</rdfs:comment>
        <rdfs:isDefinedBy rdf:resource="http://www.oasis-open.org/ciq_xnl"/>
        <rdfs:label>subdivision.school name</rdfs:label>
    </owl:DatatypeProperty>
    


    <!-- http://www.oasis-open.org/ciq_xnl#subdivision.sectionName -->

    <owl:DatatypeProperty rdf:about="http://www.oasis-open.org/ciq_xnl#subdivision.sectionName">
        <rdfs:range rdf:resource="http://www.w3.org/2001/XMLSchema#string"/>
        <rdfs:comment>Specifies the section name of an organization&apos;s subdivision</rdfs:comment>
        <rdfs:isDefinedBy rdf:resource="http://www.oasis-open.org/ciq_xnl"/>
        <rdfs:label>subdivision.section name</rdfs:label>
    </owl:DatatypeProperty>
    


    <!-- http://www.oasis-open.org/ciq_xnl#subdivisionName -->

    <owl:DatatypeProperty rdf:about="http://www.oasis-open.org/ciq_xnl#subdivisionName">
        <rdfs:range rdf:resource="http://www.w3.org/2001/XMLSchema#string"/>
        <rdfs:comment>Specifies the name of a subdivision of an organziation (e.g. department, branch, division, section)</rdfs:comment>
        <rdfs:label>Subdivision name</rdfs:label>
    </owl:DatatypeProperty>
    


    <!-- 
    ///////////////////////////////////////////////////////////////////////////////////////
    //
    // Classes
    //
    ///////////////////////////////////////////////////////////////////////////////////////
     -->

    


    <!-- http://www.oasis-open.org/ciq_xnl#Branch -->

    <owl:Class rdf:about="http://www.oasis-open.org/ciq_xnl#Branch">
        <rdfs:subClassOf rdf:resource="http://www.oasis-open.org/ciq_xnl#Subdivison"/>
        <rdfs:comment>Defines a branch of an organization</rdfs:comment>
        <rdfs:isDefinedBy rdf:resource="http://www.oasis-open.org/ciq_xnl"/>
        <rdfs:label>Branch</rdfs:label>
    </owl:Class>
    


    <!-- http://www.oasis-open.org/ciq_xnl#BusinessUnit -->

    <owl:Class rdf:about="http://www.oasis-open.org/ciq_xnl#BusinessUnit">
        <rdfs:subClassOf rdf:resource="http://www.oasis-open.org/ciq_xnl#Subdivison"/>
        <rdfs:comment>Defines a business unit of an organization</rdfs:comment>
        <rdfs:isDefinedBy rdf:resource="http://www.oasis-open.org/ciq_xnl"/>
        <rdfs:label>Business Unit</rdfs:label>
    </owl:Class>
    


    <!-- http://www.oasis-open.org/ciq_xnl#Department -->

    <owl:Class rdf:about="http://www.oasis-open.org/ciq_xnl#Department">
        <rdfs:subClassOf rdf:resource="http://www.oasis-open.org/ciq_xnl#Subdivison"/>
        <rdfs:comment>Defines a department of an organization</rdfs:comment>
        <rdfs:isDefinedBy rdf:resource="http://www.oasis-open.org/ciq_xnl"/>
        <rdfs:label>Department</rdfs:label>
    </owl:Class>
    


    <!-- http://www.oasis-open.org/ciq_xnl#Division -->

    <owl:Class rdf:about="http://www.oasis-open.org/ciq_xnl#Division">
        <rdfs:subClassOf rdf:resource="http://www.oasis-open.org/ciq_xnl#Subdivison"/>
        <rdfs:comment>Defines a division of an organization</rdfs:comment>
        <rdfs:isDefinedBy rdf:resource="http://www.oasis-open.org/ciq_xnl"/>
        <rdfs:label>Division</rdfs:label>
    </owl:Class>
    


    <!-- http://www.oasis-open.org/ciq_xnl#NameDetails -->

    <owl:Class rdf:about="http://www.oasis-open.org/ciq_xnl#NameDetails">
        <rdfs:comment>Specifies details about the party&apos;s name</rdfs:comment>
        <rdfs:isDefinedBy rdf:resource="http://www.oasis-open.org/ciq_xnl"/>
        <rdfs:label>Name details</rdfs:label>
    </owl:Class>
    


    <!-- http://www.oasis-open.org/ciq_xnl#OrganizationName -->

    <owl:Class rdf:about="http://www.oasis-open.org/ciq_xnl#OrganizationName">
        <rdfs:subClassOf rdf:resource="http://www.oasis-open.org/ciq_xnl#NameDetails"/>
        <rdfs:subClassOf>
            <owl:Restriction>
                <owl:onProperty rdf:resource="http://www.oasis-open.org/ciq_xnl#organizationName.fullName"/>
                <owl:someValuesFrom rdf:resource="http://www.w3.org/2000/01/rdf-schema#Literal"/>
            </owl:Restriction>
        </rdfs:subClassOf>
        <rdfs:subClassOf>
            <owl:Restriction>
                <owl:onProperty rdf:resource="http://www.oasis-open.org/ciq_xnl#organizationNameType"/>
                <owl:someValuesFrom rdf:resource="http://www.w3.org/2000/01/rdf-schema#Literal"/>
            </owl:Restriction>
        </rdfs:subClassOf>
        <rdfs:comment>Characterizes details about an organization&apos;s name</rdfs:comment>
        <rdfs:isDefinedBy rdf:resource="http://www.oasis-open.org/ciq_xnl"/>
        <rdfs:label>Organization Name</rdfs:label>
    </owl:Class>
    


    <!-- http://www.oasis-open.org/ciq_xnl#PersonName -->

    <owl:Class rdf:about="http://www.oasis-open.org/ciq_xnl#PersonName">
        <rdfs:subClassOf rdf:resource="http://www.oasis-open.org/ciq_xnl#NameDetails"/>
        <rdfs:subClassOf>
            <owl:Restriction>
                <owl:onProperty rdf:resource="http://www.oasis-open.org/ciq_xnl#personId"/>
                <owl:someValuesFrom rdf:resource="http://www.w3.org/2000/01/rdf-schema#Literal"/>
            </owl:Restriction>
        </rdfs:subClassOf>
        <rdfs:subClassOf>
            <owl:Restriction>
                <owl:onProperty rdf:resource="http://www.oasis-open.org/ciq_xnl#personName.firstName"/>
                <owl:someValuesFrom rdf:resource="http://www.w3.org/2000/01/rdf-schema#Literal"/>
            </owl:Restriction>
        </rdfs:subClassOf>
        <rdfs:subClassOf>
            <owl:Restriction>
                <owl:onProperty rdf:resource="http://www.oasis-open.org/ciq_xnl#personName.lastName"/>
                <owl:someValuesFrom rdf:resource="http://www.w3.org/2000/01/rdf-schema#Literal"/>
            </owl:Restriction>
        </rdfs:subClassOf>
        <rdfs:subClassOf>
            <owl:Restriction>
                <owl:onProperty rdf:resource="http://www.oasis-open.org/ciq_xnl#personName.middleName"/>
                <owl:someValuesFrom rdf:resource="http://www.w3.org/2000/01/rdf-schema#Literal"/>
            </owl:Restriction>
        </rdfs:subClassOf>
        <rdfs:subClassOf>
            <owl:Restriction>
                <owl:onProperty rdf:resource="http://www.oasis-open.org/ciq_xnl#personName.nickname"/>
                <owl:someValuesFrom rdf:resource="http://www.w3.org/2000/01/rdf-schema#Literal"/>
            </owl:Restriction>
        </rdfs:subClassOf>
        <rdfs:subClassOf>
            <owl:Restriction>
                <owl:onProperty rdf:resource="http://www.oasis-open.org/ciq_xnl#personName.precedingTitle"/>
                <owl:someValuesFrom rdf:resource="http://www.w3.org/2000/01/rdf-schema#Literal"/>
            </owl:Restriction>
        </rdfs:subClassOf>
        <rdfs:subClassOf>
            <owl:Restriction>
                <owl:onProperty rdf:resource="http://www.oasis-open.org/ciq_xnl#personName.title"/>
                <owl:someValuesFrom rdf:resource="http://www.w3.org/2000/01/rdf-schema#Literal"/>
            </owl:Restriction>
        </rdfs:subClassOf>
        <rdfs:subClassOf>
            <owl:Restriction>
                <owl:onProperty rdf:resource="http://www.oasis-open.org/ciq_xnl#personNameType"/>
                <owl:someValuesFrom rdf:resource="http://www.w3.org/2000/01/rdf-schema#Literal"/>
            </owl:Restriction>
        </rdfs:subClassOf>
        <rdfs:comment>Characterizes details about a person&apos;s name</rdfs:comment>
        <rdfs:isDefinedBy rdf:resource="http://www.oasis-open.org/ciq_xnl"/>
        <rdfs:label>Person name</rdfs:label>
    </owl:Class>
    


    <!-- http://www.oasis-open.org/ciq_xnl#School -->

    <owl:Class rdf:about="http://www.oasis-open.org/ciq_xnl#School">
        <rdfs:subClassOf rdf:resource="http://www.oasis-open.org/ciq_xnl#Subdivison"/>
        <rdfs:comment>Defines a school of an organization</rdfs:comment>
        <rdfs:isDefinedBy rdf:resource="http://www.oasis-open.org/ciq_xnl"/>
        <rdfs:label>School</rdfs:label>
    </owl:Class>
    


    <!-- http://www.oasis-open.org/ciq_xnl#Section -->

    <owl:Class rdf:about="http://www.oasis-open.org/ciq_xnl#Section">
        <rdfs:subClassOf rdf:resource="http://www.oasis-open.org/ciq_xnl#Subdivison"/>
        <rdfs:comment>Defines a section of an organization</rdfs:comment>
        <rdfs:isDefinedBy rdf:resource="http://www.oasis-open.org/ciq_xnl"/>
        <rdfs:label>Section</rdfs:label>
    </owl:Class>
    


    <!-- http://www.oasis-open.org/ciq_xnl#Subdivison -->

    <owl:Class rdf:about="http://www.oasis-open.org/ciq_xnl#Subdivison">
        <rdfs:comment>Characterizes a subdivision of an organization</rdfs:comment>
        <rdfs:isDefinedBy rdf:resource="http://www.oasis-open.org/ciq_xnl"/>
        <rdfs:label>Subdivision</rdfs:label>
    </owl:Class>
</rdf:RDF>



<!-- Generated by the OWL API (version 4.2.6.20160910-2108) https://github.com/owlcs/owlapi -->

