<?xml version="1.0"?>
<rdf:RDF xmlns="http://www.oasis-open.org/ciq_common#"
     xml:base="http://www.oasis-open.org/ciq_common"
     xmlns:rdf="http://www.w3.org/1999/02/22-rdf-syntax-ns#"
     xmlns:owl="http://www.w3.org/2002/07/owl#"
     xmlns:xml="http://www.w3.org/XML/1998/namespace"
     xmlns:ciqct="http://www.oasis-open.org/ciq_common#"
     xmlns:xsd="http://www.w3.org/2001/XMLSchema#"
     xmlns:rdfs="http://www.w3.org/2000/01/rdf-schema#">
    <owl:Ontology rdf:about="http://www.oasis-open.org/ciq_common">
        <rdfs:label>OASIS Customer Information Quality (CIQ) Common Types Ontology</rdfs:label>
        <owl:versionInfo rdf:datatype="http://www.w3.org/2001/XMLSchema#string">1.0.0-001</owl:versionInfo>
        <rdfs:comment>This ontology provides a vocabulary and representation of the OASIS Customer Information Quality (CIQ) Specification V3.0 commonly used types in the name, address, and party ontologies.

Copyright (c) 2014, DaedaFusion, LLC.  All rights reserved.</rdfs:comment>
    </owl:Ontology>
    


    <!-- 
    ///////////////////////////////////////////////////////////////////////////////////////
    //
    // Data properties
    //
    ///////////////////////////////////////////////////////////////////////////////////////
     -->

    


    <!-- http://www.oasis-open.org/ciq_common#abbreviation -->

    <owl:DatatypeProperty rdf:about="http://www.oasis-open.org/ciq_common#abbreviation">
        <rdfs:range rdf:resource="http://www.w3.org/2001/XMLSchema#boolean"/>
        <rdfs:comment>Specifies that the entry has been abbreviated</rdfs:comment>
        <rdfs:label>Abbreviation</rdfs:label>
    </owl:DatatypeProperty>
    


    <!-- http://www.oasis-open.org/ciq_common#dataQuality.reliabilityLevel -->

    <owl:DatatypeProperty rdf:about="http://www.oasis-open.org/ciq_common#dataQuality.reliabilityLevel">
       <rdfs:range rdf:resource="http://www.w3.org/2001/XMLSchema#string"/>
        <rdfs:comment>Specifes values to indicate the level of reliability of the data</rdfs:comment>
        <rdfs:label>Data Quality Type</rdfs:label>
    </owl:DatatypeProperty>
    


    <!-- http://www.oasis-open.org/ciq_common#dataQuality.validFromDateTime -->

    <owl:DatatypeProperty rdf:about="http://www.oasis-open.org/ciq_common#dataQuality.validFromDateTime">
        <rdfs:range rdf:resource="http://www.w3.org/2001/XMLSchema#dateTime"/>
        <rdfs:comment>Specifies the date the data quality is valid from</rdfs:comment>
        <rdfs:label>Valid From</rdfs:label>
    </owl:DatatypeProperty>
    


    <!-- http://www.oasis-open.org/ciq_common#dataQuality.validToDateTime -->

    <owl:DatatypeProperty rdf:about="http://www.oasis-open.org/ciq_common#dataQuality.validToDateTime">
        <rdfs:range rdf:resource="http://www.w3.org/2001/XMLSchema#dateTime"/>
        <rdfs:comment>Specifies the date the data quality is valid to</rdfs:comment>
        <rdfs:label>Valid To</rdfs:label>
    </owl:DatatypeProperty>
    


    <!-- http://www.oasis-open.org/ciq_common#id -->

    <owl:DatatypeProperty rdf:about="http://www.oasis-open.org/ciq_common#id">
        <rdfs:range rdf:resource="http://www.w3.org/2001/XMLSchema#string"/>
        <rdfs:comment>Specifies a globally unique identifier for this definition</rdfs:comment>
        <rdfs:label>Globally Unique Identifier</rdfs:label>
    </owl:DatatypeProperty>
    


    <!-- http://www.oasis-open.org/ciq_common#languageCode -->

    <owl:DatatypeProperty rdf:about="http://www.oasis-open.org/ciq_common#languageCode">
        <rdfs:range rdf:resource="http://www.w3.org/2001/XMLSchema#language"/>
        <rdfs:comment>Specifies the language used (name of human language, e.g. en, en-US)</rdfs:comment>
        <rdfs:label>Language Code</rdfs:label>
    </owl:DatatypeProperty>
    


    <!-- http://www.oasis-open.org/ciq_common#parentId -->

    <owl:DatatypeProperty rdf:about="http://www.oasis-open.org/ciq_common#parentId">
        <rdfs:range rdf:resource="http://www.w3.org/2001/XMLSchema#string"/>
        <rdfs:comment>Specifies the identifier associate with an object&apos;s parent</rdfs:comment>
        <rdfs:isDefinedBy rdf:resource="http://www.oasis-open.org/ciq_common"/>
        <rdfs:label>Parent Id</rdfs:label>
    </owl:DatatypeProperty>
    


    <!-- http://www.oasis-open.org/ciq_common#status -->

    <owl:DatatypeProperty rdf:about="http://www.oasis-open.org/ciq_common#status">
        <rdfs:range rdf:resource="http://www.w3.org/2001/XMLSchema#string"/>
        <rdfs:comment>Specifies the status of the entity. e.g. Old, Current, Inactive, Active, etc</rdfs:comment>
        <rdfs:label>Status</rdfs:label>
    </owl:DatatypeProperty>
    


    <!-- http://www.oasis-open.org/ciq_common#textLine -->

    <owl:DatatypeProperty rdf:about="http://www.oasis-open.org/ciq_common#textLine">
        <rdfs:range rdf:resource="http://www.w3.org/2001/XMLSchema#string"/>
        <rdfs:comment>Specifies a line of text</rdfs:comment>
        <rdfs:label>Text Line</rdfs:label>
    </owl:DatatypeProperty>
    


    <!-- http://www.oasis-open.org/ciq_common#textLineOrdinality -->

    <owl:DatatypeProperty rdf:about="http://www.oasis-open.org/ciq_common#textLineOrdinality">
        <rdfs:range rdf:resource="http://www.w3.org/2001/XMLSchema#positiveInteger"/>
        <rdfs:comment>Specifies the ordinality (e.g., 1,2, or 3) of this text line</rdfs:comment>
        <rdfs:label>Ordinality</rdfs:label>
    </owl:DatatypeProperty>
    


    <!-- http://www.oasis-open.org/ciq_common#validFromDateTime -->

    <owl:DatatypeProperty rdf:about="http://www.oasis-open.org/ciq_common#validFromDateTime">
        <rdfs:range rdf:resource="http://www.w3.org/2001/XMLSchema#dateTime"/>
        <rdfs:comment>Specifies the date from which data is valid.  Could be start date, issue date, validity start date, etc</rdfs:comment>
        <rdfs:label>Date Valid From</rdfs:label>
    </owl:DatatypeProperty>
    


    <!-- http://www.oasis-open.org/ciq_common#validToDateTime -->

    <owl:DatatypeProperty rdf:about="http://www.oasis-open.org/ciq_common#validToDateTime">
        <rdfs:range rdf:resource="http://www.w3.org/2001/XMLSchema#dateTime"/>
        <rdfs:comment>Specifies date to which the data is valid.  Could be end date, expiry date, validity end date, etc</rdfs:comment>
        <rdfs:label>Date Valid To</rdfs:label>
    </owl:DatatypeProperty>
</rdf:RDF>



<!-- Generated by the OWL API (version 4.2.6.20160910-2108) https://github.com/owlcs/owlapi -->

