<?xml version="1.0"?>
<rdf:RDF xmlns="http://www.oasis-open.org/ciq_xal#"
     xml:base="http://www.oasis-open.org/ciq_xal"
     xmlns:geo="http://www.w3.org/2003/01/geo/wgs84_pos#"
     xmlns:ciq_xal="http://www.oasis-open.org/ciq_xal#"
     xmlns:rdf="http://www.w3.org/1999/02/22-rdf-syntax-ns#"
     xmlns:owl="http://www.w3.org/2002/07/owl#"
     xmlns:xml="http://www.w3.org/XML/1998/namespace"
     xmlns:xsd="http://www.w3.org/2001/XMLSchema#"
     xmlns:rdfs="http://www.w3.org/2000/01/rdf-schema#"
     xmlns:foaf="http://xmlns.com/foaf/0.1/"
     xmlns:dc="http://purl.org/dc/elements/1.1/">
    <owl:Ontology rdf:about="http://www.oasis-open.org/ciq_xal">
        <owl:imports rdf:resource="http://www.oasis-open.org/ciq_common"/>
        <owl:imports rdf:resource="http://www.oasis-open.org/ciq_currency"/>
        <rdfs:comment>This ontology provides a vocabulary and representation of the OASIS Customer Information Quality (CIQ) eXtensible Address Language (xAL) Specification V3.0.

Copyright (c) 2014, DaedaFusion, LLC.  All rights reserved.</rdfs:comment>
        <rdfs:label>OASIS Customer Information Quality (CIQ) eXtensible Address Language (xAL) Ontology</rdfs:label>
        <owl:versionInfo rdf:datatype="http://www.w3.org/2001/XMLSchema#string">1.0.0-001</owl:versionInfo>
    </owl:Ontology>
    


    <!-- 
    ///////////////////////////////////////////////////////////////////////////////////////
    //
    // Annotation properties
    //
    ///////////////////////////////////////////////////////////////////////////////////////
     -->

    


    <!-- http://purl.org/dc/elements/1.1/date -->

    <owl:AnnotationProperty rdf:about="http://purl.org/dc/elements/1.1/date"/>
    


    <!-- http://purl.org/dc/elements/1.1/description -->

    <owl:AnnotationProperty rdf:about="http://purl.org/dc/elements/1.1/description"/>
    


    <!-- http://purl.org/dc/elements/1.1/title -->

    <owl:AnnotationProperty rdf:about="http://purl.org/dc/elements/1.1/title"/>
    


    <!-- http://www.w3.org/2001/XMLSchema#base64Binary -->

    <owl:AnnotationProperty rdf:about="http://www.w3.org/2001/XMLSchema#base64Binary"/>
    


    <!-- http://www.w3.org/2002/07/owl#cardinality -->

    <owl:AnnotationProperty rdf:about="http://www.w3.org/2002/07/owl#cardinality"/>
    


    <!-- http://www.w3.org/2002/07/owl#maxCardinality -->

    <owl:AnnotationProperty rdf:about="http://www.w3.org/2002/07/owl#maxCardinality"/>
    


    <!-- http://www.w3.org/2003/01/geo/wgs84_pos#alt -->

    <owl:AnnotationProperty rdf:about="http://www.w3.org/2003/01/geo/wgs84_pos#alt">
        <rdfs:comment>The WGS84 altitude of a SpatialThing (decimal meters 
above the local reference ellipsoid).</rdfs:comment>
        <rdfs:label>altitude</rdfs:label>
    </owl:AnnotationProperty>
    


    <!-- http://www.w3.org/2003/01/geo/wgs84_pos#lat -->

    <owl:AnnotationProperty rdf:about="http://www.w3.org/2003/01/geo/wgs84_pos#lat">
        <rdfs:comment>The WGS84 latitude of a SpatialThing (decimal degrees).</rdfs:comment>
        <rdfs:label>latitude</rdfs:label>
    </owl:AnnotationProperty>
    


    <!-- http://www.w3.org/2003/01/geo/wgs84_pos#location -->

    <owl:AnnotationProperty rdf:about="http://www.w3.org/2003/01/geo/wgs84_pos#location">
        <rdfs:subPropertyOf rdf:resource="http://xmlns.com/foaf/0.1/based_near"/>
        <rdfs:range rdf:resource="http://www.w3.org/2003/01/geo/wgs84_pos#SpatialThing"/>
    </owl:AnnotationProperty>
    


    <!-- http://www.w3.org/2003/01/geo/wgs84_pos#long -->

    <owl:AnnotationProperty rdf:about="http://www.w3.org/2003/01/geo/wgs84_pos#long">
        <rdfs:comment>The WGS84 longitude of a SpatialThing (decimal degrees).</rdfs:comment>
        <rdfs:label>longitude</rdfs:label>
    </owl:AnnotationProperty>
    


    <!-- http://xmlns.com/foaf/0.1/based_near -->

    <owl:AnnotationProperty rdf:about="http://xmlns.com/foaf/0.1/based_near"/>
    


    <!-- 
    ///////////////////////////////////////////////////////////////////////////////////////
    //
    // Datatypes
    //
    ///////////////////////////////////////////////////////////////////////////////////////
     -->

    


    <!-- http://www.w3.org/2001/XMLSchema#date -->

    <rdfs:Datatype rdf:about="http://www.w3.org/2001/XMLSchema#date"/>
    


    <!-- 
    ///////////////////////////////////////////////////////////////////////////////////////
    //
    // Object Properties
    //
    ///////////////////////////////////////////////////////////////////////////////////////
     -->

    


    <!-- http://www.oasis-open.org/ciq_xal#administrativeArea -->

    <owl:ObjectProperty rdf:about="http://www.oasis-open.org/ciq_xal#administrativeArea">
        <rdfs:range rdf:resource="http://www.oasis-open.org/ciq_xal#AdministrativeArea"/>
        <rdfs:comment>Specifies the first-order administrative area for a country</rdfs:comment>
        <rdfs:isDefinedBy rdf:resource="http://www.oasis-open.org/ciq_xal"/>
        <rdfs:label>Administrative Area</rdfs:label>
    </owl:ObjectProperty>
    


    <!-- http://www.oasis-open.org/ciq_xal#capital -->

    <owl:ObjectProperty rdf:about="http://www.oasis-open.org/ciq_xal#capital">
        <rdfs:range rdf:resource="http://www.oasis-open.org/ciq_xal#Locality"/>
        <rdfs:comment>Specifies the capital of the country</rdfs:comment>
        <rdfs:isDefinedBy rdf:resource="http://www.oasis-open.org/ciq_xal"/>
        <rdfs:label>Capital</rdfs:label>
    </owl:ObjectProperty>
    


    <!-- http://www.oasis-open.org/ciq_xal#continent -->

    <owl:ObjectProperty rdf:about="http://www.oasis-open.org/ciq_xal#continent">
        <rdfs:range rdf:resource="http://www.oasis-open.org/ciq_xal#Continent"/>
        <rdfs:comment>Specifies a reference to the continent in which the country resides.</rdfs:comment>
        <rdfs:isDefinedBy rdf:resource="http://www.oasis-open.org/ciq_xal"/>
        <rdfs:label>Continent</rdfs:label>
    </owl:ObjectProperty>
    


    <!-- http://www.oasis-open.org/ciq_xal#country -->

    <owl:ObjectProperty rdf:about="http://www.oasis-open.org/ciq_xal#country">
        <rdfs:range rdf:resource="http://www.oasis-open.org/ciq_xal#Country"/>
        <rdfs:comment>Specifies the country associated with the address</rdfs:comment>
        <rdfs:label>Country</rdfs:label>
    </owl:ObjectProperty>
    


    <!-- http://www.oasis-open.org/ciq_xal#currency -->

    <owl:ObjectProperty rdf:about="http://www.oasis-open.org/ciq_xal#currency">
        <rdfs:range rdf:resource="http://www.oasis-open.org/ciq_currency#Currency"/>
        <rdfs:comment>Specifies the national currency of the country</rdfs:comment>
        <rdfs:isDefinedBy rdf:resource="http://www.oasis-open.org/ciq_xal"/>
        <rdfs:label>Currency</rdfs:label>
    </owl:ObjectProperty>
    


    <!-- http://www.oasis-open.org/ciq_xal#locality -->

    <owl:ObjectProperty rdf:about="http://www.oasis-open.org/ciq_xal#locality">
        <rdfs:range rdf:resource="http://www.oasis-open.org/ciq_xal#Locality"/>
        <rdfs:comment>Specifies the details of Locality which is a named densely populated area  (a place) such as town, village, suburb, etc. A locality composes of many individual addresses.</rdfs:comment>
        <rdfs:label>Locality</rdfs:label>
    </owl:ObjectProperty>
    


    <!-- http://www.oasis-open.org/ciq_xal#neighbors -->

    <owl:ObjectProperty rdf:about="http://www.oasis-open.org/ciq_xal#neighbors">
        <rdfs:range rdf:resource="http://www.oasis-open.org/ciq_xal#Country"/>
        <rdfs:comment>Specifies the countries that neighbor the country</rdfs:comment>
        <rdfs:isDefinedBy rdf:resource="http://www.oasis-open.org/ciq_xal"/>
        <rdfs:label>neighbors</rdfs:label>
    </owl:ObjectProperty>
    


    <!-- http://www.oasis-open.org/ciq_xal#parentAdminArea1 -->

    <owl:ObjectProperty rdf:about="http://www.oasis-open.org/ciq_xal#parentAdminArea1">
        <rdfs:range rdf:resource="http://www.oasis-open.org/ciq_xal#AdministrativeArea"/>
        <rdfs:comment>Specifies a reference to the first-order administrative division of a country, such as a state in the United States, that is parent to the entity.</rdfs:comment>
        <rdfs:isDefinedBy rdf:resource="http://www.oasis-open.org/ciq_xal"/>
        <rdfs:label>Parent First-Order Administrative Division</rdfs:label>
    </owl:ObjectProperty>
    


    <!-- http://www.oasis-open.org/ciq_xal#parentAdminArea2 -->

    <owl:ObjectProperty rdf:about="http://www.oasis-open.org/ciq_xal#parentAdminArea2">
        <rdfs:range rdf:resource="http://www.oasis-open.org/ciq_xal#AdministrativeArea"/>
        <rdfs:comment>Specifies a reference to a subdivision of a first-order administrative division of a country that is parent to the entity.</rdfs:comment>
        <rdfs:isDefinedBy rdf:resource="http://www.oasis-open.org/ciq_xal"/>
        <rdfs:label>Parent Second-Order Administrative Division</rdfs:label>
    </owl:ObjectProperty>
    


    <!-- http://www.oasis-open.org/ciq_xal#parentAdminArea3 -->

    <owl:ObjectProperty rdf:about="http://www.oasis-open.org/ciq_xal#parentAdminArea3">
        <rdfs:range rdf:resource="http://www.oasis-open.org/ciq_xal#AdministrativeArea"/>
        <rdfs:comment>Specifies a reference to a subdivision of a second-order administrative division of a country that is parent to the entity.</rdfs:comment>
        <rdfs:isDefinedBy rdf:resource="http://www.oasis-open.org/ciq_xal"/>
        <rdfs:label>Parent Third-Order Administrative Division</rdfs:label>
    </owl:ObjectProperty>
    


    <!-- http://www.oasis-open.org/ciq_xal#parentAdminArea4 -->

    <owl:ObjectProperty rdf:about="http://www.oasis-open.org/ciq_xal#parentAdminArea4">
        <rdfs:range rdf:resource="http://www.oasis-open.org/ciq_xal#AdministrativeArea"/>
        <rdfs:comment>Specifies a reference to a subdivision of a third-order administrative division of a country that is parent to the entity.</rdfs:comment>
        <rdfs:isDefinedBy rdf:resource="http://www.oasis-open.org/ciq_xal"/>
        <rdfs:label>Parent Fourth-Order Administrative Division</rdfs:label>
    </owl:ObjectProperty>
    


    <!-- http://www.oasis-open.org/ciq_xal#parentCountry -->

    <owl:ObjectProperty rdf:about="http://www.oasis-open.org/ciq_xal#parentCountry">
        <rdfs:range rdf:resource="http://www.oasis-open.org/ciq_xal#Country"/>
        <rdfs:comment>Specifies a reference to the country in to which the entity belongs.</rdfs:comment>
        <rdfs:isDefinedBy rdf:resource="http://www.oasis-open.org/ciq_xal"/>
        <rdfs:label>Parent Country</rdfs:label>
    </owl:ObjectProperty>
    


    <!-- http://www.oasis-open.org/ciq_xal#postOffice -->

    <owl:ObjectProperty rdf:about="http://www.oasis-open.org/ciq_xal#postOffice">
        <rdfs:range rdf:resource="http://www.oasis-open.org/ciq_xal#PostOffice"/>
        <rdfs:comment>Specifies a delivery point/installation where all mails are delivered and the post man/delivery service picks up the mails and delivers it to the recipients through a delivery mode.</rdfs:comment>
        <rdfs:label>Post Office</rdfs:label>
    </owl:ObjectProperty>
    


    <!-- http://www.oasis-open.org/ciq_xal#postalDelliveryPoint -->

    <owl:ObjectProperty rdf:about="http://www.oasis-open.org/ciq_xal#postalDelliveryPoint">
        <rdfs:range rdf:resource="http://www.oasis-open.org/ciq_xal#PostalDeliveryPoint"/>
        <rdfs:comment>Specifies where the mail is dropped off for recipients to pick them up directly. E.g. POBox, Private Bag,  pigeon hole, free mail numbers, etc.</rdfs:comment>
        <rdfs:label>Postal Delivery Point</rdfs:label>
    </owl:ObjectProperty>
    


    <!-- http://www.oasis-open.org/ciq_xal#postcode -->

    <owl:ObjectProperty rdf:about="http://www.oasis-open.org/ciq_xal#postcode">
        <rdfs:range rdf:resource="http://www.oasis-open.org/ciq_xal#Postcode"/>
        <rdfs:comment>Specifies the post code.  Note that not all countries have post codes</rdfs:comment>
        <rdfs:label>Post Code</rdfs:label>
    </owl:ObjectProperty>
    


    <!-- http://www.oasis-open.org/ciq_xal#premises -->

    <owl:ObjectProperty rdf:about="http://www.oasis-open.org/ciq_xal#premises">
        <rdfs:range rdf:resource="http://www.oasis-open.org/ciq_xal#Premises"/>
        <rdfs:comment>Specifies the Premises (could be building(s), site, loaction, property, premise, place) which is a landmark place which has a main address such as large mail user (e.g. Airport, Hospital, University) or could be a building (e.g. apartment, house)  or a building or complex of buildings (e.g. an apartment complex or shopping centre) or even a vacant land (e.g. LOT).</rdfs:comment>
        <rdfs:label>Premises</rdfs:label>
    </owl:ObjectProperty>
    


    <!-- http://www.oasis-open.org/ciq_xal#ruralDelivery -->

    <owl:ObjectProperty rdf:about="http://www.oasis-open.org/ciq_xal#ruralDelivery">
        <rdfs:range rdf:resource="http://www.oasis-open.org/ciq_xal#RuralDelivery"/>
        <rdfs:comment>Specifies the postal-specific delivery identifier for remote communities. Note that not all countries have RuralDelivery</rdfs:comment>
        <rdfs:label>Rural Delivery</rdfs:label>
    </owl:ObjectProperty>
    


    <!-- http://www.oasis-open.org/ciq_xal#subAdministrativeArea -->

    <owl:ObjectProperty rdf:about="http://www.oasis-open.org/ciq_xal#subAdministrativeArea">
        <rdfs:range rdf:resource="http://www.oasis-open.org/ciq_xal#AdministrativeArea"/>
        <rdfs:comment>Specifies the second-order administrative division of the area. Note that not all countries have a subadministrative area</rdfs:comment>
        <rdfs:label>SubAdmininstrative Area</rdfs:label>
    </owl:ObjectProperty>
    


    <!-- http://www.oasis-open.org/ciq_xal#subLocality -->

    <owl:ObjectProperty rdf:about="http://www.oasis-open.org/ciq_xal#subLocality">
        <rdfs:comment>Specifies a locality that is smaller and is contained within the boundaries of its parent locality. Note that not all localities have sub locality. For example, many areas within a locality where each area is a sub locality</rdfs:comment>
        <rdfs:label>SubLocality</rdfs:label>
    </owl:ObjectProperty>
    


    <!-- http://www.oasis-open.org/ciq_xal#subPremises -->

    <owl:ObjectProperty rdf:about="http://www.oasis-open.org/ciq_xal#subPremises">
        <rdfs:range rdf:resource="http://www.oasis-open.org/ciq_xal#SubPremises"/>
        <rdfs:comment>Specifies sub-premises.   Examples of sub-premises are apartments and suites in buildings, shops in malls, etc.  or sub-addresses in a land mark place such as airports, military bases, hospitals, etc. Some countries have blocks within blocks</rdfs:comment>
        <rdfs:label>SubPremises</rdfs:label>
    </owl:ObjectProperty>
    


    <!-- http://www.oasis-open.org/ciq_xal#subThoroughfare -->

    <owl:ObjectProperty rdf:about="http://www.oasis-open.org/ciq_xal#subThoroughfare">
        <rdfs:range rdf:resource="http://www.oasis-open.org/ciq_xal#Thoroughfare"/>
        <rdfs:comment>Specifies another thoroughfare that is required to uniquely identify the location, such as an access route, intersection, corner, adjacent, boundary, etc</rdfs:comment>
        <rdfs:label>Subthoroughfare</rdfs:label>
    </owl:ObjectProperty>
    


    <!-- http://www.oasis-open.org/ciq_xal#thoroughfare -->

    <owl:ObjectProperty rdf:about="http://www.oasis-open.org/ciq_xal#thoroughfare">
        <rdfs:range rdf:resource="http://www.oasis-open.org/ciq_xal#Thoroughfare"/>
        <rdfs:comment>Specifies the details of the Access route along which buildings/lot/land are located, such as street, road, channel, crescent, avenue, etc.</rdfs:comment>
        <rdfs:label>Thoroughfare</rdfs:label>
    </owl:ObjectProperty>
    


    <!-- http://www.w3.org/2003/01/geo/wgs84_pos#location -->

    <owl:ObjectProperty rdf:about="http://www.w3.org/2003/01/geo/wgs84_pos#location"/>
    


    <!-- 
    ///////////////////////////////////////////////////////////////////////////////////////
    //
    // Data properties
    //
    ///////////////////////////////////////////////////////////////////////////////////////
     -->

    


    <!-- http://www.oasis-open.org/ciq_xal#addressID -->

    <owl:DatatypeProperty rdf:about="http://www.oasis-open.org/ciq_xal#addressID">
        <rdfs:range rdf:resource="http://www.w3.org/2001/XMLSchema#string"/>
        <rdfs:comment>Specifies a unique address identifier such as postal delivery idetifier assigned to the address by local postal authority, e.g. DPID in Australia.</rdfs:comment>
        <rdfs:label>Address ID</rdfs:label>
    </owl:DatatypeProperty>
    


    <!-- http://www.oasis-open.org/ciq_xal#addressIDType -->

    <owl:DatatypeProperty rdf:about="http://www.oasis-open.org/ciq_xal#addressIDType">
        <rdfs:range rdf:resource="http://www.w3.org/2001/XMLSchema#string"/>
        <rdfs:comment>Type of address ID used. e.g. DPID, etc</rdfs:comment>
        <rdfs:label>Address ID Type</rdfs:label>
    </owl:DatatypeProperty>
    


    <!-- http://www.oasis-open.org/ciq_xal#addressKeyRef -->

    <owl:DatatypeProperty rdf:about="http://www.oasis-open.org/ciq_xal#addressKeyRef">
        <rdfs:comment>Specifies a reference attribute Key of Address.</rdfs:comment>
        <rdfs:label>Address Key Reference</rdfs:label>
    </owl:DatatypeProperty>
    


    <!-- http://www.oasis-open.org/ciq_xal#addressType -->

    <owl:DatatypeProperty rdf:about="http://www.oasis-open.org/ciq_xal#addressType">
        <rdfs:range>
            <rdfs:Datatype>
                <owl:oneOf>
                    <rdf:Description>
                        <rdf:type rdf:resource="http://www.w3.org/1999/02/22-rdf-syntax-ns#List"/>
                        <rdf:first rdf:datatype="http://www.w3.org/2001/XMLSchema#string">Airport</rdf:first>
                        <rdf:rest>
                            <rdf:Description>
                                <rdf:type rdf:resource="http://www.w3.org/1999/02/22-rdf-syntax-ns#List"/>
                                <rdf:first rdf:datatype="http://www.w3.org/2001/XMLSchema#string">Business</rdf:first>
                                <rdf:rest>
                                    <rdf:Description>
                                        <rdf:type rdf:resource="http://www.w3.org/1999/02/22-rdf-syntax-ns#List"/>
                                        <rdf:first rdf:datatype="http://www.w3.org/2001/XMLSchema#string">CaravanPark</rdf:first>
                                        <rdf:rest>
                                            <rdf:Description>
                                                <rdf:type rdf:resource="http://www.w3.org/1999/02/22-rdf-syntax-ns#List"/>
                                                <rdf:first rdf:datatype="http://www.w3.org/2001/XMLSchema#string">CommercialPark</rdf:first>
                                                <rdf:rest>
                                                    <rdf:Description>
                                                        <rdf:type rdf:resource="http://www.w3.org/1999/02/22-rdf-syntax-ns#List"/>
                                                        <rdf:first rdf:datatype="http://www.w3.org/2001/XMLSchema#string">CommunityDevelopment</rdf:first>
                                                        <rdf:rest>
                                                            <rdf:Description>
                                                                <rdf:type rdf:resource="http://www.w3.org/1999/02/22-rdf-syntax-ns#List"/>
                                                                <rdf:first rdf:datatype="http://www.w3.org/2001/XMLSchema#string">EducationalInstitution</rdf:first>
                                                                <rdf:rest>
                                                                    <rdf:Description>
                                                                        <rdf:type rdf:resource="http://www.w3.org/1999/02/22-rdf-syntax-ns#List"/>
                                                                        <rdf:first rdf:datatype="http://www.w3.org/2001/XMLSchema#string">Entertainment</rdf:first>
                                                                        <rdf:rest>
                                                                            <rdf:Description>
                                                                                <rdf:type rdf:resource="http://www.w3.org/1999/02/22-rdf-syntax-ns#List"/>
                                                                                <rdf:first rdf:datatype="http://www.w3.org/2001/XMLSchema#string">Hospital</rdf:first>
                                                                                <rdf:rest>
                                                                                    <rdf:Description>
                                                                                        <rdf:type rdf:resource="http://www.w3.org/1999/02/22-rdf-syntax-ns#List"/>
                                                                                        <rdf:first rdf:datatype="http://www.w3.org/2001/XMLSchema#string">Location</rdf:first>
                                                                                        <rdf:rest>
                                                                                            <rdf:Description>
                                                                                                <rdf:type rdf:resource="http://www.w3.org/1999/02/22-rdf-syntax-ns#List"/>
                                                                                                <rdf:first rdf:datatype="http://www.w3.org/2001/XMLSchema#string">Marina</rdf:first>
                                                                                                <rdf:rest>
                                                                                                    <rdf:Description>
                                                                                                        <rdf:type rdf:resource="http://www.w3.org/1999/02/22-rdf-syntax-ns#List"/>
                                                                                                        <rdf:first rdf:datatype="http://www.w3.org/2001/XMLSchema#string">MilitaryBase</rdf:first>
                                                                                                        <rdf:rest>
                                                                                                            <rdf:Description>
                                                                                                                <rdf:type rdf:resource="http://www.w3.org/1999/02/22-rdf-syntax-ns#List"/>
                                                                                                                <rdf:first rdf:datatype="http://www.w3.org/2001/XMLSchema#string">OverseasMilitary</rdf:first>
                                                                                                                <rdf:rest>
                                                                                                                    <rdf:Description>
                                                                                                                        <rdf:type rdf:resource="http://www.w3.org/1999/02/22-rdf-syntax-ns#List"/>
                                                                                                                        <rdf:first rdf:datatype="http://www.w3.org/2001/XMLSchema#string">Port</rdf:first>
                                                                                                                        <rdf:rest>
                                                                                                                            <rdf:Description>
                                                                                                                                <rdf:type rdf:resource="http://www.w3.org/1999/02/22-rdf-syntax-ns#List"/>
                                                                                                                                <rdf:first rdf:datatype="http://www.w3.org/2001/XMLSchema#string">Primary</rdf:first>
                                                                                                                                <rdf:rest>
                                                                                                                                    <rdf:Description>
                                                                                                                                        <rdf:type rdf:resource="http://www.w3.org/1999/02/22-rdf-syntax-ns#List"/>
                                                                                                                                        <rdf:first rdf:datatype="http://www.w3.org/2001/XMLSchema#string">RecreationalPark</rdf:first>
                                                                                                                                        <rdf:rest>
                                                                                                                                            <rdf:Description>
                                                                                                                                                <rdf:type rdf:resource="http://www.w3.org/1999/02/22-rdf-syntax-ns#List"/>
                                                                                                                                                <rdf:first rdf:datatype="http://www.w3.org/2001/XMLSchema#string">Resort</rdf:first>
                                                                                                                                                <rdf:rest>
                                                                                                                                                    <rdf:Description>
                                                                                                                                                        <rdf:type rdf:resource="http://www.w3.org/1999/02/22-rdf-syntax-ns#List"/>
                                                                                                                                                        <rdf:first rdf:datatype="http://www.w3.org/2001/XMLSchema#string">RetirementVillage</rdf:first>
                                                                                                                                                        <rdf:rest>
                                                                                                                                                            <rdf:Description>
                                                                                                                                                                <rdf:type rdf:resource="http://www.w3.org/1999/02/22-rdf-syntax-ns#List"/>
                                                                                                                                                                <rdf:first rdf:datatype="http://www.w3.org/2001/XMLSchema#string">Rural</rdf:first>
                                                                                                                                                                <rdf:rest>
                                                                                                                                                                    <rdf:Description>
                                                                                                                                                                        <rdf:type rdf:resource="http://www.w3.org/1999/02/22-rdf-syntax-ns#List"/>
                                                                                                                                                                        <rdf:first rdf:datatype="http://www.w3.org/2001/XMLSchema#string">Secondary</rdf:first>
                                                                                                                                                                        <rdf:rest>
                                                                                                                                                                            <rdf:Description>
                                                                                                                                                                                <rdf:type rdf:resource="http://www.w3.org/1999/02/22-rdf-syntax-ns#List"/>
                                                                                                                                                                                <rdf:first rdf:datatype="http://www.w3.org/2001/XMLSchema#string">ShoppingCentre</rdf:first>
                                                                                                                                                                                <rdf:rest>
                                                                                                                                                                                    <rdf:Description>
                                                                                                                                                                                        <rdf:type rdf:resource="http://www.w3.org/1999/02/22-rdf-syntax-ns#List"/>
                                                                                                                                                                                        <rdf:first rdf:datatype="http://www.w3.org/2001/XMLSchema#string">SportingCentre</rdf:first>
                                                                                                                                                                                        <rdf:rest>
                                                                                                                                                                                            <rdf:Description>
                                                                                                                                                                                                <rdf:type rdf:resource="http://www.w3.org/1999/02/22-rdf-syntax-ns#List"/>
                                                                                                                                                                                                <rdf:first rdf:datatype="http://www.w3.org/2001/XMLSchema#string">Urban</rdf:first>
                                                                                                                                                                                                <rdf:rest rdf:resource="http://www.w3.org/1999/02/22-rdf-syntax-ns#nil"/>
                                                                                                                                                                                            </rdf:Description>
                                                                                                                                                                                        </rdf:rest>
                                                                                                                                                                                    </rdf:Description>
                                                                                                                                                                                </rdf:rest>
                                                                                                                                                                            </rdf:Description>
                                                                                                                                                                        </rdf:rest>
                                                                                                                                                                    </rdf:Description>
                                                                                                                                                                </rdf:rest>
                                                                                                                                                            </rdf:Description>
                                                                                                                                                        </rdf:rest>
                                                                                                                                                    </rdf:Description>
                                                                                                                                                </rdf:rest>
                                                                                                                                            </rdf:Description>
                                                                                                                                        </rdf:rest>
                                                                                                                                    </rdf:Description>
                                                                                                                                </rdf:rest>
                                                                                                                            </rdf:Description>
                                                                                                                        </rdf:rest>
                                                                                                                    </rdf:Description>
                                                                                                                </rdf:rest>
                                                                                                            </rdf:Description>
                                                                                                        </rdf:rest>
                                                                                                    </rdf:Description>
                                                                                                </rdf:rest>
                                                                                            </rdf:Description>
                                                                                        </rdf:rest>
                                                                                    </rdf:Description>
                                                                                </rdf:rest>
                                                                            </rdf:Description>
                                                                        </rdf:rest>
                                                                    </rdf:Description>
                                                                </rdf:rest>
                                                            </rdf:Description>
                                                        </rdf:rest>
                                                    </rdf:Description>
                                                </rdf:rest>
                                            </rdf:Description>
                                        </rdf:rest>
                                    </rdf:Description>
                                </rdf:rest>
                            </rdf:Description>
                        </rdf:rest>
                    </rdf:Description>
                </owl:oneOf>
            </rdfs:Datatype>
        </rdfs:range>
        <rdfs:comment>Specifies the type of address.</rdfs:comment>
        <rdfs:label>Address Type</rdfs:label>
    </owl:DatatypeProperty>
    


    <!-- http://www.oasis-open.org/ciq_xal#addressUsage -->

    <owl:DatatypeProperty rdf:about="http://www.oasis-open.org/ciq_xal#addressUsage">
        <rdfs:range>
            <rdfs:Datatype>
                <owl:oneOf>
                    <rdf:Description>
                        <rdf:type rdf:resource="http://www.w3.org/1999/02/22-rdf-syntax-ns#List"/>
                        <rdf:first rdf:datatype="http://www.w3.org/2001/XMLSchema#string">Billing</rdf:first>
                        <rdf:rest>
                            <rdf:Description>
                                <rdf:type rdf:resource="http://www.w3.org/1999/02/22-rdf-syntax-ns#List"/>
                                <rdf:first rdf:datatype="http://www.w3.org/2001/XMLSchema#string">Business</rdf:first>
                                <rdf:rest>
                                    <rdf:Description>
                                        <rdf:type rdf:resource="http://www.w3.org/1999/02/22-rdf-syntax-ns#List"/>
                                        <rdf:first rdf:datatype="http://www.w3.org/2001/XMLSchema#string">Communication</rdf:first>
                                        <rdf:rest>
                                            <rdf:Description>
                                                <rdf:type rdf:resource="http://www.w3.org/1999/02/22-rdf-syntax-ns#List"/>
                                                <rdf:first rdf:datatype="http://www.w3.org/2001/XMLSchema#string">Contact</rdf:first>
                                                <rdf:rest>
                                                    <rdf:Description>
                                                        <rdf:type rdf:resource="http://www.w3.org/1999/02/22-rdf-syntax-ns#List"/>
                                                        <rdf:first rdf:datatype="http://www.w3.org/2001/XMLSchema#string">Mailing</rdf:first>
                                                        <rdf:rest>
                                                            <rdf:Description>
                                                                <rdf:type rdf:resource="http://www.w3.org/1999/02/22-rdf-syntax-ns#List"/>
                                                                <rdf:first rdf:datatype="http://www.w3.org/2001/XMLSchema#string">Personal</rdf:first>
                                                                <rdf:rest>
                                                                    <rdf:Description>
                                                                        <rdf:type rdf:resource="http://www.w3.org/1999/02/22-rdf-syntax-ns#List"/>
                                                                        <rdf:first rdf:datatype="http://www.w3.org/2001/XMLSchema#string">Postal</rdf:first>
                                                                        <rdf:rest>
                                                                            <rdf:Description>
                                                                                <rdf:type rdf:resource="http://www.w3.org/1999/02/22-rdf-syntax-ns#List"/>
                                                                                <rdf:first rdf:datatype="http://www.w3.org/2001/XMLSchema#string">Residential</rdf:first>
                                                                                <rdf:rest rdf:resource="http://www.w3.org/1999/02/22-rdf-syntax-ns#nil"/>
                                                                            </rdf:Description>
                                                                        </rdf:rest>
                                                                    </rdf:Description>
                                                                </rdf:rest>
                                                            </rdf:Description>
                                                        </rdf:rest>
                                                    </rdf:Description>
                                                </rdf:rest>
                                            </rdf:Description>
                                        </rdf:rest>
                                    </rdf:Description>
                                </rdf:rest>
                            </rdf:Description>
                        </rdf:rest>
                    </rdf:Description>
                </owl:oneOf>
            </rdfs:Datatype>
        </rdfs:range>
        <rdfs:comment>Specifies the purpose the address is used for. E.g.  Postal, residential, business,  exchange, update, create, delete, etc</rdfs:comment>
        <rdfs:label>Address Usage</rdfs:label>
    </owl:DatatypeProperty>
    


    <!-- http://www.oasis-open.org/ciq_xal#adminAreaName -->

    <owl:DatatypeProperty rdf:about="http://www.oasis-open.org/ciq_xal#adminAreaName">
        <rdfs:range rdf:resource="http://www.w3.org/2001/XMLSchema#string"/>
        <rdfs:comment>Specifies the name of the Administrative Area entity</rdfs:comment>
        <rdfs:label>Administrative Area Name</rdfs:label>
    </owl:DatatypeProperty>
    


    <!-- http://www.oasis-open.org/ciq_xal#adminAreaNameCode -->

    <owl:DatatypeProperty rdf:about="http://www.oasis-open.org/ciq_xal#adminAreaNameCode">
        <rdfs:range rdf:resource="http://www.w3.org/2001/XMLSchema#string"/>
        <rdfs:comment>Specifies name of the administrative area represented as a code. e.g. &quot;CO&quot; for COLORADO</rdfs:comment>
        <rdfs:label>Name Code</rdfs:label>
    </owl:DatatypeProperty>
    


    <!-- http://www.oasis-open.org/ciq_xal#adminAreaNameCodeType -->

    <owl:DatatypeProperty rdf:about="http://www.oasis-open.org/ciq_xal#adminAreaNameCodeType">
        <rdfs:range>
            <rdfs:Datatype>
                <owl:oneOf>
                    <rdf:Description>
                        <rdf:type rdf:resource="http://www.w3.org/1999/02/22-rdf-syntax-ns#List"/>
                        <rdf:first rdf:datatype="http://www.w3.org/2001/XMLSchema#string">ISO 3166 Numeric</rdf:first>
                        <rdf:rest>
                            <rdf:Description>
                                <rdf:type rdf:resource="http://www.w3.org/1999/02/22-rdf-syntax-ns#List"/>
                                <rdf:first rdf:datatype="http://www.w3.org/2001/XMLSchema#string">ISO 3166 alpha-2</rdf:first>
                                <rdf:rest>
                                    <rdf:Description>
                                        <rdf:type rdf:resource="http://www.w3.org/1999/02/22-rdf-syntax-ns#List"/>
                                        <rdf:first rdf:datatype="http://www.w3.org/2001/XMLSchema#string">ISO 3166 alpha-3</rdf:first>
                                        <rdf:rest>
                                            <rdf:Description>
                                                <rdf:type rdf:resource="http://www.w3.org/1999/02/22-rdf-syntax-ns#List"/>
                                                <rdf:first rdf:datatype="http://www.w3.org/2001/XMLSchema#string">ISO 3166 alpha-4</rdf:first>
                                                <rdf:rest rdf:resource="http://www.w3.org/1999/02/22-rdf-syntax-ns#nil"/>
                                            </rdf:Description>
                                        </rdf:rest>
                                    </rdf:Description>
                                </rdf:rest>
                            </rdf:Description>
                        </rdf:rest>
                    </rdf:Description>
                </owl:oneOf>
            </rdfs:Datatype>
        </rdfs:range>
        <rdfs:comment>Specifies the type of the name code, which defines its format</rdfs:comment>
        <rdfs:label>Name Code Type</rdfs:label>
    </owl:DatatypeProperty>
    


    <!-- http://www.oasis-open.org/ciq_xal#adminAreaType -->

    <owl:DatatypeProperty rdf:about="http://www.oasis-open.org/ciq_xal#adminAreaType">
        <rdfs:range rdf:resource="http://www.w3.org/2001/XMLSchema#string"/>
        <rdfs:comment>Specifies the type of the administrative area</rdfs:comment>
        <rdfs:label>Administrative Area Type</rdfs:label>
    </owl:DatatypeProperty>
    


    <!-- http://www.oasis-open.org/ciq_xal#alternateName -->

    <owl:DatatypeProperty rdf:about="http://www.oasis-open.org/ciq_xal#alternateName">
        <rdfs:range rdf:resource="http://www.w3.org/2001/XMLSchema#string"/>
        <rdfs:comment>Specifies an alternative name for the entity</rdfs:comment>
        <rdfs:isDefinedBy rdf:resource="http://www.oasis-open.org/ciq_xal"/>
        <rdfs:label>Alternate Names</rdfs:label>
    </owl:DatatypeProperty>
    


    <!-- http://www.oasis-open.org/ciq_xal#area -->

    <owl:DatatypeProperty rdf:about="http://www.oasis-open.org/ciq_xal#area">
        <rdfs:range rdf:resource="http://www.w3.org/2001/XMLSchema#positiveInteger"/>
        <rdfs:comment>Specifies the area of the country in square kilometers</rdfs:comment>
        <rdfs:isDefinedBy rdf:resource="http://www.oasis-open.org/ciq_xal"/>
        <rdfs:label>Area</rdfs:label>
    </owl:DatatypeProperty>
    


    <!-- http://www.oasis-open.org/ciq_xal#asciiName -->

    <owl:DatatypeProperty rdf:about="http://www.oasis-open.org/ciq_xal#asciiName">
        <rdfs:range rdf:resource="http://www.w3.org/2001/XMLSchema#string"/>
        <rdfs:comment>Specifies the ASCII name of the entity</rdfs:comment>
        <rdfs:isDefinedBy rdf:resource="http://www.oasis-open.org/ciq_xal"/>
        <rdfs:label>ASCII  Name</rdfs:label>
    </owl:DatatypeProperty>
    


    <!-- http://www.oasis-open.org/ciq_xal#callingCodes -->

    <owl:DatatypeProperty rdf:about="http://www.oasis-open.org/ciq_xal#callingCodes">
        <rdfs:range rdf:resource="http://www.w3.org/2001/XMLSchema#string"/>
        <rdfs:comment>Specifies the calling code for the country</rdfs:comment>
        <rdfs:isDefinedBy rdf:resource="http://www.oasis-open.org/ciq_xal"/>
        <rdfs:label>Calling Codes</rdfs:label>
    </owl:DatatypeProperty>
    


    <!-- http://www.oasis-open.org/ciq_xal#continentCode -->

    <owl:DatatypeProperty rdf:about="http://www.oasis-open.org/ciq_xal#continentCode">
        <rdfs:range rdf:resource="http://www.w3.org/2001/XMLSchema#string"/>
        <rdfs:comment>Specifies the 2-character continent code</rdfs:comment>
        <rdfs:isDefinedBy rdf:resource="http://www.oasis-open.org/ciq_xal"/>
        <rdfs:label>Continent Code</rdfs:label>
    </owl:DatatypeProperty>
    


    <!-- http://www.oasis-open.org/ciq_xal#continentName -->

    <owl:DatatypeProperty rdf:about="http://www.oasis-open.org/ciq_xal#continentName">
        <rdfs:range rdf:resource="http://www.w3.org/2001/XMLSchema#string"/>
        <rdfs:comment>Specifies the name of the continent</rdfs:comment>
        <rdfs:isDefinedBy rdf:resource="http://www.oasis-open.org/ciq_xal"/>
        <rdfs:label>Continent Name</rdfs:label>
    </owl:DatatypeProperty>
    


    <!-- http://www.oasis-open.org/ciq_xal#countryFlagImage -->

    <owl:DatatypeProperty rdf:about="http://www.oasis-open.org/ciq_xal#countryFlagImage">
        <rdfs:range rdf:resource="http://www.w3.org/2001/XMLSchema#base64Binary"/>
        <rdfs:comment>Specifies the image of the flag of the country based64 encoded</rdfs:comment>
        <rdfs:isDefinedBy rdf:resource="http://www.oasis-open.org/ciq_xal"/>
        <rdfs:label>Country Flag</rdfs:label>
    </owl:DatatypeProperty>
    


    <!-- http://www.oasis-open.org/ciq_xal#countryFlagRef -->

    <owl:DatatypeProperty rdf:about="http://www.oasis-open.org/ciq_xal#countryFlagRef">
        <rdfs:range rdf:resource="http://www.w3.org/2001/XMLSchema#anyURI"/>
        <rdfs:comment>Specifies a reference to the flag of the country</rdfs:comment>
        <rdfs:isDefinedBy rdf:resource="http://www.oasis-open.org/ciq_xal"/>
        <rdfs:label>Country Flag Reference</rdfs:label>
    </owl:DatatypeProperty>
    


    <!-- http://www.oasis-open.org/ciq_xal#countryName -->

    <owl:DatatypeProperty rdf:about="http://www.oasis-open.org/ciq_xal#countryName">
        <rdfs:range rdf:resource="http://www.w3.org/2001/XMLSchema#string"/>
        <rdfs:comment>Specifies the name of the country</rdfs:comment>
        <rdfs:label>Country</rdfs:label>
    </owl:DatatypeProperty>
    


    <!-- http://www.oasis-open.org/ciq_xal#countryNameType -->

    <owl:DatatypeProperty rdf:about="http://www.oasis-open.org/ciq_xal#countryNameType">
        <rdfs:range>
            <rdfs:Datatype>
                <owl:oneOf>
                    <rdf:Description>
                        <rdf:type rdf:resource="http://www.w3.org/1999/02/22-rdf-syntax-ns#List"/>
                        <rdf:first rdf:datatype="http://www.w3.org/2001/XMLSchema#string">Name</rdf:first>
                        <rdf:rest>
                            <rdf:Description>
                                <rdf:type rdf:resource="http://www.w3.org/1999/02/22-rdf-syntax-ns#List"/>
                                <rdf:first rdf:datatype="http://www.w3.org/2001/XMLSchema#string">Type</rdf:first>
                                <rdf:rest rdf:resource="http://www.w3.org/1999/02/22-rdf-syntax-ns#nil"/>
                            </rdf:Description>
                        </rdf:rest>
                    </rdf:Description>
                </owl:oneOf>
            </rdfs:Datatype>
        </rdfs:range>
        <rdfs:comment>Specifes the type of name for the country.</rdfs:comment>
        <rdfs:label>Country Name Type</rdfs:label>
    </owl:DatatypeProperty>
    


    <!-- http://www.oasis-open.org/ciq_xal#deliveryMode -->

    <owl:DatatypeProperty rdf:about="http://www.oasis-open.org/ciq_xal#deliveryMode">
        <rdfs:range rdf:resource="http://www.w3.org/2001/XMLSchema#string"/>
        <rdfs:comment>Specifies the mode of delivery of address. For example: rural route, normal delivery, post office box, etc.</rdfs:comment>
        <rdfs:label>Delivery Mode</rdfs:label>
    </owl:DatatypeProperty>
    


    <!-- http://www.oasis-open.org/ciq_xal#digitalElevationModel -->

    <owl:DatatypeProperty rdf:about="http://www.oasis-open.org/ciq_xal#digitalElevationModel">
        <rdfs:range rdf:resource="http://www.w3.org/2001/XMLSchema#string"/>
        <rdfs:comment>Specifies the Digital Elevation Model, stm3 or gtopo30, average elevation of 3&apos;&apos;x3&apos;&apos; (ca 90mx90m) or 30&apos;&apos;x30&apos;&apos; (ca 900mx900m) area in meters, integer. srtm processed by cgiar/ciat.</rdfs:comment>
        <rdfs:isDefinedBy rdf:resource="http://www.oasis-open.org/ciq_xal"/>
        <rdfs:label>Digital Elevation Mode</rdfs:label>
    </owl:DatatypeProperty>
    


    <!-- http://www.oasis-open.org/ciq_xal#direction -->

    <owl:DatatypeProperty rdf:about="http://www.oasis-open.org/ciq_xal#direction">
        <rdfs:range>
            <rdfs:Datatype>
                <owl:oneOf>
                    <rdf:Description>
                        <rdf:type rdf:resource="http://www.w3.org/1999/02/22-rdf-syntax-ns#List"/>
                        <rdf:first rdf:datatype="http://www.w3.org/2001/XMLSchema#string">East</rdf:first>
                        <rdf:rest>
                            <rdf:Description>
                                <rdf:type rdf:resource="http://www.w3.org/1999/02/22-rdf-syntax-ns#List"/>
                                <rdf:first rdf:datatype="http://www.w3.org/2001/XMLSchema#string">North</rdf:first>
                                <rdf:rest>
                                    <rdf:Description>
                                        <rdf:type rdf:resource="http://www.w3.org/1999/02/22-rdf-syntax-ns#List"/>
                                        <rdf:first rdf:datatype="http://www.w3.org/2001/XMLSchema#string">South</rdf:first>
                                        <rdf:rest>
                                            <rdf:Description>
                                                <rdf:type rdf:resource="http://www.w3.org/1999/02/22-rdf-syntax-ns#List"/>
                                                <rdf:first rdf:datatype="http://www.w3.org/2001/XMLSchema#string">West</rdf:first>
                                                <rdf:rest rdf:resource="http://www.w3.org/1999/02/22-rdf-syntax-ns#nil"/>
                                            </rdf:Description>
                                        </rdf:rest>
                                    </rdf:Description>
                                </rdf:rest>
                            </rdf:Description>
                        </rdf:rest>
                    </rdf:Description>
                </owl:oneOf>
            </rdfs:Datatype>
        </rdfs:range>
        <rdfs:comment>Specifies the direction of latitude measurement offset from the equator</rdfs:comment>
        <rdfs:label>Direction</rdfs:label>
    </owl:DatatypeProperty>
    


    <!-- http://www.oasis-open.org/ciq_xal#featureInfo -->

    <owl:DatatypeProperty rdf:about="http://www.oasis-open.org/ciq_xal#featureInfo">
        <rdfs:range rdf:resource="http://www.w3.org/2001/XMLSchema#string"/>
        <rdfs:comment>Specifies the Geonams Feature Class and Feature Code in the format {featureClass}.{featureCode}</rdfs:comment>
        <rdfs:isDefinedBy rdf:resource="http://www.oasis-open.org/ciq_xal"/>
        <rdfs:label>Geonames Feature Class and Code</rdfs:label>
    </owl:DatatypeProperty>
    


    <!-- http://www.oasis-open.org/ciq_xal#fipsCountryCode -->

    <owl:DatatypeProperty rdf:about="http://www.oasis-open.org/ciq_xal#fipsCountryCode">
        <rdfs:range rdf:resource="http://www.w3.org/2001/XMLSchema#string"/>
        <rdfs:comment>Specifies the country code per Federal Information Processing Standards (FIPS) 10-4</rdfs:comment>
        <rdfs:isDefinedBy rdf:resource="http://www.oasis-open.org/ciq_xal"/>
        <rdfs:label>FIPS 10-4 Country Code</rdfs:label>
    </owl:DatatypeProperty>
    


    <!-- http://www.oasis-open.org/ciq_xal#freeTextAddress -->

    <owl:DatatypeProperty rdf:about="http://www.oasis-open.org/ciq_xal#freeTextAddress">
        <rdfs:range rdf:resource="http://www.w3.org/2001/XMLSchema#string"/>
        <rdfs:comment>Specifies a container for free text address elements where address elements are not parsed.</rdfs:comment>
        <rdfs:label>Free Text Address</rdfs:label>
    </owl:DatatypeProperty>
    


    <!-- http://www.oasis-open.org/ciq_xal#geoCoordinates.datum -->

    <owl:DatatypeProperty rdf:about="http://www.oasis-open.org/ciq_xal#geoCoordinates.datum">
        <rdfs:range rdf:resource="http://www.w3.org/2001/XMLSchema#string"/>
        <rdfs:comment>Specifies the datum within with the measurement was taken</rdfs:comment>
        <rdfs:isDefinedBy rdf:resource="http://www.oasis-open.org/ciq_xal"/>
        <rdfs:label>Geo Coordinates Datum</rdfs:label>
    </owl:DatatypeProperty>
    


    <!-- http://www.oasis-open.org/ciq_xal#geoCoordinates.datumCodeType -->

    <owl:DatatypeProperty rdf:about="http://www.oasis-open.org/ciq_xal#geoCoordinates.datumCodeType">
        <rdfs:range rdf:resource="http://www.w3.org/2001/XMLSchema#string"/>
        <rdfs:comment>Specifies the type of the datum code (e.g., EPSG, WGS-84).</rdfs:comment>
        <rdfs:isDefinedBy rdf:resource="http://www.oasis-open.org/ciq_xal"/>
        <rdfs:label>Geo Coordinates Datum Code Type</rdfs:label>
    </owl:DatatypeProperty>
    


    <!-- http://www.oasis-open.org/ciq_xal#geoCoordinates.meridian -->

    <owl:DatatypeProperty rdf:about="http://www.oasis-open.org/ciq_xal#geoCoordinates.meridian">
        <rdfs:range rdf:resource="http://www.w3.org/2001/XMLSchema#string"/>
        <rdfs:comment>Specifies the meridian code that specifies the position of the meridian.</rdfs:comment>
        <rdfs:isDefinedBy rdf:resource="http://www.oasis-open.org/ciq_xal"/>
        <rdfs:label>Geo Coordinates Meridian</rdfs:label>
    </owl:DatatypeProperty>
    


    <!-- http://www.oasis-open.org/ciq_xal#geoCoordinates.meridianCodeType -->

    <owl:DatatypeProperty rdf:about="http://www.oasis-open.org/ciq_xal#geoCoordinates.meridianCodeType">
        <rdfs:range rdf:resource="http://www.w3.org/2001/XMLSchema#string"/>
        <rdfs:comment>Specifies the type of meridian code utilized (e.g., EPSG, GeoTIFF)</rdfs:comment>
        <rdfs:isDefinedBy rdf:resource="http://www.oasis-open.org/ciq_xal"/>
        <rdfs:label>Geo Coordinates Meridian Code Type</rdfs:label>
    </owl:DatatypeProperty>
    


    <!-- http://www.oasis-open.org/ciq_xal#geoCoordinates.projection -->

    <owl:DatatypeProperty rdf:about="http://www.oasis-open.org/ciq_xal#geoCoordinates.projection">
        <rdfs:range rdf:resource="http://www.w3.org/2001/XMLSchema#string"/>
        <rdfs:comment>Specifies the projection within which the measurement was taken.</rdfs:comment>
        <rdfs:isDefinedBy rdf:resource="http://www.oasis-open.org/ciq_xal"/>
        <rdfs:label>Geo Coordinates Projection</rdfs:label>
    </owl:DatatypeProperty>
    


    <!-- http://www.oasis-open.org/ciq_xal#geoCoordinates.projectionCodeType -->

    <owl:DatatypeProperty rdf:about="http://www.oasis-open.org/ciq_xal#geoCoordinates.projectionCodeType">
        <rdfs:range rdf:resource="http://www.w3.org/2001/XMLSchema#string"/>
        <rdfs:comment>Specifies the type of the projection code utilizes (e.g., EPSG)</rdfs:comment>
        <rdfs:isDefinedBy rdf:resource="http://www.oasis-open.org/ciq_xal"/>
        <rdfs:label>Geo Coordinates Projection Code Type</rdfs:label>
    </owl:DatatypeProperty>
    


    <!-- http://www.oasis-open.org/ciq_xal#geonameId -->

    <owl:DatatypeProperty rdf:about="http://www.oasis-open.org/ciq_xal#geonameId">
        <rdfs:range rdf:resource="http://www.w3.org/2001/XMLSchema#integer"/>
        <rdfs:comment>Specifies the geoname identifier for the country</rdfs:comment>
        <rdfs:isDefinedBy rdf:resource="http://www.oasis-open.org/ciq_xal"/>
        <rdfs:label>Geoname Id</rdfs:label>
    </owl:DatatypeProperty>
    


    <!-- http://www.oasis-open.org/ciq_xal#identifierExtension -->

    <owl:DatatypeProperty rdf:about="http://www.oasis-open.org/ciq_xal#identifierExtension">
        <rdfs:range rdf:resource="http://www.w3.org/2001/XMLSchema#string"/>
        <rdfs:comment>Specifies that the value is an extension number of some identifier, e.g. 01 in Private Bag 2330-01, where the main number of the private bag is 2330, 12345-1223 in post code where 1223 is the extension</rdfs:comment>
        <rdfs:label>Extension</rdfs:label>
    </owl:DatatypeProperty>
    


    <!-- http://www.oasis-open.org/ciq_xal#identifierName -->

    <owl:DatatypeProperty rdf:about="http://www.oasis-open.org/ciq_xal#identifierName">
        <rdfs:range rdf:resource="http://www.w3.org/2001/XMLSchema#string"/>
        <rdfs:comment>Specifies the identifier name.  Applicable to mail box office names such as PO BOX, GPO BOX, MAIL BAG NO., etc.</rdfs:comment>
        <rdfs:label>Name</rdfs:label>
    </owl:DatatypeProperty>
    


    <!-- http://www.oasis-open.org/ciq_xal#identifierNumber -->

    <owl:DatatypeProperty rdf:about="http://www.oasis-open.org/ciq_xal#identifierNumber">
        <rdfs:range rdf:resource="http://www.w3.org/2001/XMLSchema#string"/>
        <rdfs:comment>Specifies that the value is number, e.g. 2020 in PoBox 2020. The actual value can be alpha-numeric.</rdfs:comment>
        <rdfs:label>Number</rdfs:label>
    </owl:DatatypeProperty>
    


    <!-- http://www.oasis-open.org/ciq_xal#identifierPrefix -->

    <owl:DatatypeProperty rdf:about="http://www.oasis-open.org/ciq_xal#identifierPrefix">
        <rdfs:range rdf:resource="http://www.w3.org/2001/XMLSchema#string"/>
        <rdfs:comment>Specifes that the element contains some value that is important, but not exactly the number itself. E.g. PoBox can be a prefix in PoBox 2020, street no. A-15, where A is the prefix and 15 is the number</rdfs:comment>
        <rdfs:label>Prefix</rdfs:label>
    </owl:DatatypeProperty>
    


    <!-- http://www.oasis-open.org/ciq_xal#identifierRangeFrom -->

    <owl:DatatypeProperty rdf:about="http://www.oasis-open.org/ciq_xal#identifierRangeFrom">
        <rdfs:range rdf:resource="http://www.w3.org/2001/XMLSchema#string"/>
        <rdfs:comment>Specifies that the element contains the lower value of a range, e.g. 25 in 25-37</rdfs:comment>
        <rdfs:label>Range From</rdfs:label>
    </owl:DatatypeProperty>
    


    <!-- http://www.oasis-open.org/ciq_xal#identifierRangeTo -->

    <owl:DatatypeProperty rdf:about="http://www.oasis-open.org/ciq_xal#identifierRangeTo">
        <rdfs:range rdf:resource="http://www.w3.org/2001/XMLSchema#string"/>
        <rdfs:comment>Specifies that the element contains the top value of a range, e.g. 25 in 25-37</rdfs:comment>
        <rdfs:label>Range To</rdfs:label>
    </owl:DatatypeProperty>
    


    <!-- http://www.oasis-open.org/ciq_xal#identifierSeparator -->

    <owl:DatatypeProperty rdf:about="http://www.oasis-open.org/ciq_xal#identifierSeparator">
        <rdfs:range rdf:resource="http://www.w3.org/2001/XMLSchema#string"/>
        <rdfs:comment>Specifies that the value is a separator that is expected to be preserved. Examples are / - #, as in 15-A where &quot;-&quot; is the separator</rdfs:comment>
        <rdfs:label>Separator</rdfs:label>
    </owl:DatatypeProperty>
    


    <!-- http://www.oasis-open.org/ciq_xal#identifierSuffix -->

    <owl:DatatypeProperty rdf:about="http://www.oasis-open.org/ciq_xal#identifierSuffix">
        <rdfs:range rdf:resource="http://www.w3.org/2001/XMLSchema#string"/>
        <rdfs:comment>Specifies that the element contains some value that is important, but not exactly the number itself. E.g. &apos;bis&apos; in &apos;45 bis&apos;</rdfs:comment>
        <rdfs:label>Suffix</rdfs:label>
    </owl:DatatypeProperty>
    


    <!-- http://www.oasis-open.org/ciq_xal#internalThoroughfare -->

    <owl:DatatypeProperty rdf:about="http://www.oasis-open.org/ciq_xal#internalThoroughfare">
        <rdfs:range rdf:resource="http://www.w3.org/2001/XMLSchema#string"/>
        <rdfs:comment>Specifies the roads and streets within boundaries of larger complexes/premises such as hospitals, airports, etc.</rdfs:comment>
        <rdfs:label>Internal Thoroughfare</rdfs:label>
    </owl:DatatypeProperty>
    


    <!-- http://www.oasis-open.org/ciq_xal#internetTLD -->

    <owl:DatatypeProperty rdf:about="http://www.oasis-open.org/ciq_xal#internetTLD">
        <rdfs:range rdf:resource="http://www.w3.org/2001/XMLSchema#string"/>
        <rdfs:comment>Specifies the Internet Top-Level Domain (TLD) for the country</rdfs:comment>
        <rdfs:isDefinedBy rdf:resource="http://www.oasis-open.org/ciq_xal"/>
        <rdfs:label>Internet TLD</rdfs:label>
    </owl:DatatypeProperty>
    


    <!-- http://www.oasis-open.org/ciq_xal#iso2CountryCode -->

    <owl:DatatypeProperty rdf:about="http://www.oasis-open.org/ciq_xal#iso2CountryCode">
        <rdfs:range rdf:resource="http://www.w3.org/2001/XMLSchema#string"/>
        <rdfs:comment>Specifies the 2-character country code per ISO 3166-1 alpha-2</rdfs:comment>
        <rdfs:isDefinedBy rdf:resource="http://www.oasis-open.org/ciq_xal"/>
        <rdfs:label>ISO 3166-1 alpha-2 Country Code</rdfs:label>
    </owl:DatatypeProperty>
    


    <!-- http://www.oasis-open.org/ciq_xal#iso3CountryCode -->

    <owl:DatatypeProperty rdf:about="http://www.oasis-open.org/ciq_xal#iso3CountryCode">
        <rdfs:range rdf:resource="http://www.w3.org/2001/XMLSchema#string"/>
        <rdfs:comment>Specifies the 3-character country code per ISO 3166-1 alpha-3</rdfs:comment>
        <rdfs:isDefinedBy rdf:resource="http://www.oasis-open.org/ciq_xal"/>
        <rdfs:label>ISO 3166-1 alpha-3  Country Code</rdfs:label>
    </owl:DatatypeProperty>
    


    <!-- http://www.oasis-open.org/ciq_xal#iso4CountryCode -->

    <owl:DatatypeProperty rdf:about="http://www.oasis-open.org/ciq_xal#iso4CountryCode">
        <rdfs:range rdf:resource="http://www.w3.org/2001/XMLSchema#string"/>
        <rdfs:comment>Specifies the 4-character country code per ISO 3166-1 alpha-4</rdfs:comment>
        <rdfs:isDefinedBy rdf:resource="http://www.oasis-open.org/ciq_xal"/>
        <rdfs:label>ISO 3166-1 alpha-4  Country Code</rdfs:label>
    </owl:DatatypeProperty>
    


    <!-- http://www.oasis-open.org/ciq_xal#isoNumericCountryCode -->

    <owl:DatatypeProperty rdf:about="http://www.oasis-open.org/ciq_xal#isoNumericCountryCode">
        <rdfs:range rdf:resource="http://www.w3.org/2001/XMLSchema#integer"/>
        <rdfs:comment>Specifies the 3-digit country code per ISO 3166-1 numeric</rdfs:comment>
        <rdfs:label>ISO 3166-1 numeric  Country Code</rdfs:label>
    </owl:DatatypeProperty>
    


    <!-- http://www.oasis-open.org/ciq_xal#languages -->

    <owl:DatatypeProperty rdf:about="http://www.oasis-open.org/ciq_xal#languages">
        <rdfs:range rdf:resource="http://www.w3.org/2001/XMLSchema#string"/>
        <rdfs:comment>Specifies the languages spoken in a country ordered by the number of speakers.

The language code is a &apos;locale&apos; where any two-letter primary-tag is an ISO-639 language abbreviation and any two-letter initial subtag is an ISO-3166 country code.</rdfs:comment>
        <rdfs:isDefinedBy rdf:resource="http://www.oasis-open.org/ciq_xal"/>
        <rdfs:label>Languages</rdfs:label>
    </owl:DatatypeProperty>
    


    <!-- http://www.oasis-open.org/ciq_xal#lastModifiedDate -->

    <owl:DatatypeProperty rdf:about="http://www.oasis-open.org/ciq_xal#lastModifiedDate">
        <rdfs:range rdf:resource="http://www.w3.org/2001/XMLSchema#date"/>
        <rdfs:comment>Specifies the date last modified</rdfs:comment>
        <rdfs:isDefinedBy rdf:resource="http://www.oasis-open.org/ciq_xal"/>
        <rdfs:label>Date Last Modified</rdfs:label>
    </owl:DatatypeProperty>
    


    <!-- http://www.oasis-open.org/ciq_xal#localityName -->

    <owl:DatatypeProperty rdf:about="http://www.oasis-open.org/ciq_xal#localityName">
        <rdfs:range rdf:resource="http://www.w3.org/2001/XMLSchema#string"/>
        <rdfs:comment>Specifies the name of the locality entity</rdfs:comment>
        <rdfs:isDefinedBy rdf:resource="http://www.oasis-open.org/ciq_xal"/>
        <rdfs:label>Locality Name</rdfs:label>
    </owl:DatatypeProperty>
    


    <!-- http://www.oasis-open.org/ciq_xal#localityNameCode -->

    <owl:DatatypeProperty rdf:about="http://www.oasis-open.org/ciq_xal#localityNameCode">
        <rdfs:range rdf:resource="http://www.w3.org/2001/XMLSchema#string"/>
        <rdfs:comment>Specifies name of the locality represented as a code.</rdfs:comment>
        <rdfs:isDefinedBy rdf:resource="http://www.oasis-open.org/ciq_xal"/>
        <rdfs:label>Locality Name Code</rdfs:label>
    </owl:DatatypeProperty>
    


    <!-- http://www.oasis-open.org/ciq_xal#localityNameCodeType -->

    <owl:DatatypeProperty rdf:about="http://www.oasis-open.org/ciq_xal#localityNameCodeType">
        <rdfs:range rdf:resource="http://www.w3.org/2001/XMLSchema#string"/>
        <rdfs:comment>Specifies the type of the name code, which defines its format</rdfs:comment>
        <rdfs:isDefinedBy rdf:resource="http://www.oasis-open.org/ciq_xal"/>
        <rdfs:label>Locality Name Code Type</rdfs:label>
    </owl:DatatypeProperty>
    


    <!-- http://www.oasis-open.org/ciq_xal#localityType -->

    <owl:DatatypeProperty rdf:about="http://www.oasis-open.org/ciq_xal#localityType">
        <rdfs:range rdf:resource="http://www.w3.org/2001/XMLSchema#string"/>
        <rdfs:comment>Specifies the type of locality. e.g. suburb, area, zone, village, etc</rdfs:comment>
        <rdfs:label>Locality Type</rdfs:label>
    </owl:DatatypeProperty>
    


    <!-- http://www.oasis-open.org/ciq_xal#memberOfOECD -->

    <owl:DatatypeProperty rdf:about="http://www.oasis-open.org/ciq_xal#memberOfOECD">
        <rdfs:range rdf:resource="http://www.w3.org/2001/XMLSchema#boolean"/>
        <rdfs:comment>Specifies whether the country is a member of the Organization for Economic Co-Operation and Development (OECD).</rdfs:comment>
        <rdfs:isDefinedBy rdf:resource="http://www.oasis-open.org/ciq_xal"/>
        <rdfs:label>Member of OECD</rdfs:label>
    </owl:DatatypeProperty>
    


    <!-- http://www.oasis-open.org/ciq_xal#population -->

    <owl:DatatypeProperty rdf:about="http://www.oasis-open.org/ciq_xal#population">
        <rdfs:range rdf:resource="http://www.w3.org/2001/XMLSchema#positiveInteger"/>
        <rdfs:comment>Specifies the population of the entity.</rdfs:comment>
        <rdfs:isDefinedBy rdf:resource="http://www.oasis-open.org/ciq_xal"/>
        <rdfs:label>Population</rdfs:label>
    </owl:DatatypeProperty>
    


    <!-- http://www.oasis-open.org/ciq_xal#postOfficeName -->

    <owl:DatatypeProperty rdf:about="http://www.oasis-open.org/ciq_xal#postOfficeName">
        <rdfs:range rdf:resource="http://www.w3.org/2001/XMLSchema#string"/>
        <rdfs:comment>Specifies the full combined name of the Post Office</rdfs:comment>
        <rdfs:label>Post Office Name</rdfs:label>
    </owl:DatatypeProperty>
    


    <!-- http://www.oasis-open.org/ciq_xal#postOfficeType -->

    <owl:DatatypeProperty rdf:about="http://www.oasis-open.org/ciq_xal#postOfficeType">
        <rdfs:range rdf:resource="http://www.w3.org/2001/XMLSchema#string"/>
        <rdfs:comment>Specifies the type of postal delivery office from where the mail will be distributed to the final delivery point by a delivery mode.  Example: Post Office, Mail Collection Centre, Letter Carrier Depot,  Station, etc.</rdfs:comment>
        <rdfs:label>Post Office Type</rdfs:label>
    </owl:DatatypeProperty>
    


    <!-- http://www.oasis-open.org/ciq_xal#postalCode -->

    <owl:DatatypeProperty rdf:about="http://www.oasis-open.org/ciq_xal#postalCode">
        <rdfs:range rdf:resource="http://www.w3.org/2001/XMLSchema#string"/>
        <rdfs:comment>Specifies a postal code for the entity. An entity may have more than one postal code, depending upon its size.</rdfs:comment>
        <rdfs:isDefinedBy rdf:resource="http://www.oasis-open.org/ciq_xal"/>
        <rdfs:label>Postal Code</rdfs:label>
    </owl:DatatypeProperty>
    


    <!-- http://www.oasis-open.org/ciq_xal#postalCodeFormat -->

    <owl:DatatypeProperty rdf:about="http://www.oasis-open.org/ciq_xal#postalCodeFormat">
        <rdfs:range rdf:resource="http://www.w3.org/2001/XMLSchema#string"/>
        <rdfs:comment>Specifies the format of the postal code for the country</rdfs:comment>
        <rdfs:isDefinedBy rdf:resource="http://www.oasis-open.org/ciq_xal"/>
        <rdfs:label>Postal Code Format</rdfs:label>
    </owl:DatatypeProperty>
    


    <!-- http://www.oasis-open.org/ciq_xal#postalDeliveryPointName -->

    <owl:DatatypeProperty rdf:about="http://www.oasis-open.org/ciq_xal#postalDeliveryPointName">
        <rdfs:range rdf:resource="http://www.w3.org/2001/XMLSchema#string"/>
        <rdfs:comment>Specifies the full combined name of the Postal Delivery Point</rdfs:comment>
        <rdfs:label>Postal Delivery Point Name</rdfs:label>
    </owl:DatatypeProperty>
    


    <!-- http://www.oasis-open.org/ciq_xal#postalDeliveryPointType -->

    <owl:DatatypeProperty rdf:about="http://www.oasis-open.org/ciq_xal#postalDeliveryPointType">
        <rdfs:range>
            <rdfs:Datatype>
                <owl:oneOf>
                    <rdf:Description>
                        <rdf:type rdf:resource="http://www.w3.org/1999/02/22-rdf-syntax-ns#List"/>
                        <rdf:first rdf:datatype="http://www.w3.org/2001/XMLSchema#string">GPOBox</rdf:first>
                        <rdf:rest>
                            <rdf:Description>
                                <rdf:type rdf:resource="http://www.w3.org/1999/02/22-rdf-syntax-ns#List"/>
                                <rdf:first rdf:datatype="http://www.w3.org/2001/XMLSchema#string">LockedBag</rdf:first>
                                <rdf:rest>
                                    <rdf:Description>
                                        <rdf:type rdf:resource="http://www.w3.org/1999/02/22-rdf-syntax-ns#List"/>
                                        <rdf:first rdf:datatype="http://www.w3.org/2001/XMLSchema#string">MailStop</rdf:first>
                                        <rdf:rest>
                                            <rdf:Description>
                                                <rdf:type rdf:resource="http://www.w3.org/1999/02/22-rdf-syntax-ns#List"/>
                                                <rdf:first rdf:datatype="http://www.w3.org/2001/XMLSchema#string">POBox</rdf:first>
                                                <rdf:rest>
                                                    <rdf:Description>
                                                        <rdf:type rdf:resource="http://www.w3.org/1999/02/22-rdf-syntax-ns#List"/>
                                                        <rdf:first rdf:datatype="http://www.w3.org/2001/XMLSchema#string">PigonHole</rdf:first>
                                                        <rdf:rest>
                                                            <rdf:Description>
                                                                <rdf:type rdf:resource="http://www.w3.org/1999/02/22-rdf-syntax-ns#List"/>
                                                                <rdf:first rdf:datatype="http://www.w3.org/2001/XMLSchema#string">PrivateBag</rdf:first>
                                                                <rdf:rest rdf:resource="http://www.w3.org/1999/02/22-rdf-syntax-ns#nil"/>
                                                            </rdf:Description>
                                                        </rdf:rest>
                                                    </rdf:Description>
                                                </rdf:rest>
                                            </rdf:Description>
                                        </rdf:rest>
                                    </rdf:Description>
                                </rdf:rest>
                            </rdf:Description>
                        </rdf:rest>
                    </rdf:Description>
                </owl:oneOf>
            </rdfs:Datatype>
        </rdfs:range>
        <rdfs:comment>Specifies the type of the postal delivery point</rdfs:comment>
        <rdfs:label>Postal Delivery Point Type</rdfs:label>
    </owl:DatatypeProperty>
    


    <!-- http://www.oasis-open.org/ciq_xal#postcodeIdentifier -->

    <owl:DatatypeProperty rdf:about="http://www.oasis-open.org/ciq_xal#postcodeIdentifier">
        <rdfs:range rdf:resource="http://www.w3.org/2001/XMLSchema#string"/>
        <rdfs:comment>Specifies the full combined name of the postcode.  The postcode is formatted according to country-specific rules. Example: SW3 0A8-1A, 600074, 2067. This element can also be used to define the semantics of what each code in the post code means</rdfs:comment>
        <rdfs:label>Postcode Identifier</rdfs:label>
    </owl:DatatypeProperty>
    


    <!-- http://www.oasis-open.org/ciq_xal#postdirection -->

    <owl:DatatypeProperty rdf:about="http://www.oasis-open.org/ciq_xal#postdirection">
        <rdfs:range rdf:resource="http://www.w3.org/2001/XMLSchema#string"/>
        <rdfs:comment>Specifies the direction as a suffix, such as Archer Street North, where &quot;North&quot; is PostDirection.</rdfs:comment>
        <rdfs:isDefinedBy rdf:resource="http://www.oasis-open.org/ciq_xal"/>
        <rdfs:label>Post-Direction</rdfs:label>
    </owl:DatatypeProperty>
    


    <!-- http://www.oasis-open.org/ciq_xal#predirection -->

    <owl:DatatypeProperty rdf:about="http://www.oasis-open.org/ciq_xal#predirection">
        <rdfs:range rdf:resource="http://www.w3.org/2001/XMLSchema#string"/>
        <rdfs:comment>Specifies the direction as a prefix, such as North Archer Street, where &quot;North&quot; is PreDirection. {@en-US}</rdfs:comment>
        <rdfs:isDefinedBy rdf:resource="http://www.oasis-open.org/ciq_xal"/>
        <rdfs:label>Pre-Direction</rdfs:label>
    </owl:DatatypeProperty>
    


    <!-- http://www.oasis-open.org/ciq_xal#premisesLocation -->

    <owl:DatatypeProperty rdf:about="http://www.oasis-open.org/ciq_xal#premisesLocation">
        <rdfs:range rdf:resource="http://www.w3.org/2001/XMLSchema#string"/>
        <rdfs:comment>Specifies where in the building/landmark the premises is located, e.g. lobby, ground floor, penthouse, or where in a larger complex (e.g. airport) the address is located.</rdfs:comment>
        <rdfs:label>Premises Location</rdfs:label>
    </owl:DatatypeProperty>
    


    <!-- http://www.oasis-open.org/ciq_xal#premisesName -->

    <owl:DatatypeProperty rdf:about="http://www.oasis-open.org/ciq_xal#premisesName">
        <rdfs:range rdf:resource="http://www.w3.org/2001/XMLSchema#string"/>
        <rdfs:comment>Specifies the full combined name of the premises</rdfs:comment>
        <rdfs:label>Premises Name</rdfs:label>
    </owl:DatatypeProperty>
    


    <!-- http://www.oasis-open.org/ciq_xal#premisesNumber -->

    <owl:DatatypeProperty rdf:about="http://www.oasis-open.org/ciq_xal#premisesNumber">
        <rdfs:range rdf:resource="http://www.w3.org/2001/XMLSchema#string"/>
        <rdfs:comment>Specifies data associated with the number of the premises. E.g.House 15, number range, number suffix.

When range is specified, the beginning of the range should be specified as the value of the rangeFrom property, the end of the range should be specified as the value of the rangeTo poperty, and the character(s) used to separate the beginning and ending of the range should be specified as the value of the separator property</rdfs:comment>
        <rdfs:label>Premises Number</rdfs:label>
    </owl:DatatypeProperty>
    


    <!-- http://www.oasis-open.org/ciq_xal#premisesType -->

    <owl:DatatypeProperty rdf:about="http://www.oasis-open.org/ciq_xal#premisesType">
        <rdfs:range>
            <rdfs:Datatype>
                <owl:oneOf>
                    <rdf:Description>
                        <rdf:type rdf:resource="http://www.w3.org/1999/02/22-rdf-syntax-ns#List"/>
                        <rdf:first rdf:datatype="http://www.w3.org/2001/XMLSchema#string">Airport</rdf:first>
                        <rdf:rest>
                            <rdf:Description>
                                <rdf:type rdf:resource="http://www.w3.org/1999/02/22-rdf-syntax-ns#List"/>
                                <rdf:first rdf:datatype="http://www.w3.org/2001/XMLSchema#string">Area</rdf:first>
                                <rdf:rest>
                                    <rdf:Description>
                                        <rdf:type rdf:resource="http://www.w3.org/1999/02/22-rdf-syntax-ns#List"/>
                                        <rdf:first rdf:datatype="http://www.w3.org/2001/XMLSchema#string">Building</rdf:first>
                                        <rdf:rest>
                                            <rdf:Description>
                                                <rdf:type rdf:resource="http://www.w3.org/1999/02/22-rdf-syntax-ns#List"/>
                                                <rdf:first rdf:datatype="http://www.w3.org/2001/XMLSchema#string">Farm</rdf:first>
                                                <rdf:rest>
                                                    <rdf:Description>
                                                        <rdf:type rdf:resource="http://www.w3.org/1999/02/22-rdf-syntax-ns#List"/>
                                                        <rdf:first rdf:datatype="http://www.w3.org/2001/XMLSchema#string">Hospital</rdf:first>
                                                        <rdf:rest>
                                                            <rdf:Description>
                                                                <rdf:type rdf:resource="http://www.w3.org/1999/02/22-rdf-syntax-ns#List"/>
                                                                <rdf:first rdf:datatype="http://www.w3.org/2001/XMLSchema#string">House</rdf:first>
                                                                <rdf:rest>
                                                                    <rdf:Description>
                                                                        <rdf:type rdf:resource="http://www.w3.org/1999/02/22-rdf-syntax-ns#List"/>
                                                                        <rdf:first rdf:datatype="http://www.w3.org/2001/XMLSchema#string">Landmark</rdf:first>
                                                                        <rdf:rest>
                                                                            <rdf:Description>
                                                                                <rdf:type rdf:resource="http://www.w3.org/1999/02/22-rdf-syntax-ns#List"/>
                                                                                <rdf:first rdf:datatype="http://www.w3.org/2001/XMLSchema#string">LargeMailUser</rdf:first>
                                                                                <rdf:rest>
                                                                                    <rdf:Description>
                                                                                        <rdf:type rdf:resource="http://www.w3.org/1999/02/22-rdf-syntax-ns#List"/>
                                                                                        <rdf:first rdf:datatype="http://www.w3.org/2001/XMLSchema#string">Lot</rdf:first>
                                                                                        <rdf:rest>
                                                                                            <rdf:Description>
                                                                                                <rdf:type rdf:resource="http://www.w3.org/1999/02/22-rdf-syntax-ns#List"/>
                                                                                                <rdf:first rdf:datatype="http://www.w3.org/2001/XMLSchema#string">RailwayStation</rdf:first>
                                                                                                <rdf:rest>
                                                                                                    <rdf:Description>
                                                                                                        <rdf:type rdf:resource="http://www.w3.org/1999/02/22-rdf-syntax-ns#List"/>
                                                                                                        <rdf:first rdf:datatype="http://www.w3.org/2001/XMLSchema#string">ShoppingComplex</rdf:first>
                                                                                                        <rdf:rest>
                                                                                                            <rdf:Description>
                                                                                                                <rdf:type rdf:resource="http://www.w3.org/1999/02/22-rdf-syntax-ns#List"/>
                                                                                                                <rdf:first rdf:datatype="http://www.w3.org/2001/XMLSchema#string">Unit</rdf:first>
                                                                                                                <rdf:rest>
                                                                                                                    <rdf:Description>
                                                                                                                        <rdf:type rdf:resource="http://www.w3.org/1999/02/22-rdf-syntax-ns#List"/>
                                                                                                                        <rdf:first rdf:datatype="http://www.w3.org/2001/XMLSchema#string">University</rdf:first>
                                                                                                                        <rdf:rest rdf:resource="http://www.w3.org/1999/02/22-rdf-syntax-ns#nil"/>
                                                                                                                    </rdf:Description>
                                                                                                                </rdf:rest>
                                                                                                            </rdf:Description>
                                                                                                        </rdf:rest>
                                                                                                    </rdf:Description>
                                                                                                </rdf:rest>
                                                                                            </rdf:Description>
                                                                                        </rdf:rest>
                                                                                    </rdf:Description>
                                                                                </rdf:rest>
                                                                            </rdf:Description>
                                                                        </rdf:rest>
                                                                    </rdf:Description>
                                                                </rdf:rest>
                                                            </rdf:Description>
                                                        </rdf:rest>
                                                    </rdf:Description>
                                                </rdf:rest>
                                            </rdf:Description>
                                        </rdf:rest>
                                    </rdf:Description>
                                </rdf:rest>
                            </rdf:Description>
                        </rdf:rest>
                    </rdf:Description>
                </owl:oneOf>
            </rdfs:Datatype>
        </rdfs:range>
        <rdfs:comment>Specifies the types of Premises</rdfs:comment>
        <rdfs:label>Premises Type</rdfs:label>
    </owl:DatatypeProperty>
    


    <!-- http://www.oasis-open.org/ciq_xal#premisesTypeCode -->

    <owl:DatatypeProperty rdf:about="http://www.oasis-open.org/ciq_xal#premisesTypeCode">
        <rdfs:range rdf:resource="http://www.w3.org/2001/XMLSchema#string"/>
        <rdfs:comment>Specifies the type of code use for Premises</rdfs:comment>
        <rdfs:label>Premise Type Code</rdfs:label>
    </owl:DatatypeProperty>
    


    <!-- http://www.oasis-open.org/ciq_xal#range -->

    <owl:DatatypeProperty rdf:about="http://www.oasis-open.org/ciq_xal#range">
        <rdfs:range rdf:resource="http://www.w3.org/2001/XMLSchema#string"/>
        <rdfs:comment>Specifies that the value is a range, e.g. 25-37. 

When range is specified, the beginning of the range should be specified as the value of the rangeFrom property, the end of the range should be specified as the value of the rangeTo poperty, and the character(s) used to separate the beginning and ending of the range should be specified as the value of the separator property</rdfs:comment>
        <rdfs:label>Range</rdfs:label>
    </owl:DatatypeProperty>
    


    <!-- http://www.oasis-open.org/ciq_xal#referenceLocation -->

    <owl:DatatypeProperty rdf:about="http://www.oasis-open.org/ciq_xal#referenceLocation">
        <rdfs:range rdf:resource="http://www.w3.org/2001/XMLSchema#string"/>
        <rdfs:comment>Specifies the reference location information in support of the area. e.g. Territory of France</rdfs:comment>
        <rdfs:label>Reference Location</rdfs:label>
    </owl:DatatypeProperty>
    


    <!-- http://www.oasis-open.org/ciq_xal#ruralDeliveryName -->

    <owl:DatatypeProperty rdf:about="http://www.oasis-open.org/ciq_xal#ruralDeliveryName">
        <rdfs:range rdf:resource="http://www.w3.org/2001/XMLSchema#string"/>
        <rdfs:comment>Specifies the full combined name of the rural delivery</rdfs:comment>
        <rdfs:label>Rural Delivery Name</rdfs:label>
    </owl:DatatypeProperty>
    


    <!-- http://www.oasis-open.org/ciq_xal#ruralDeliveryType -->

    <owl:DatatypeProperty rdf:about="http://www.oasis-open.org/ciq_xal#ruralDeliveryType">
        <rdfs:range>
            <rdfs:Datatype>
                <owl:oneOf>
                    <rdf:Description>
                        <rdf:type rdf:resource="http://www.w3.org/1999/02/22-rdf-syntax-ns#List"/>
                        <rdf:first rdf:datatype="http://www.w3.org/2001/XMLSchema#string">Air</rdf:first>
                        <rdf:rest>
                            <rdf:Description>
                                <rdf:type rdf:resource="http://www.w3.org/1999/02/22-rdf-syntax-ns#List"/>
                                <rdf:first rdf:datatype="http://www.w3.org/2001/XMLSchema#string">Dirt</rdf:first>
                                <rdf:rest>
                                    <rdf:Description>
                                        <rdf:type rdf:resource="http://www.w3.org/1999/02/22-rdf-syntax-ns#List"/>
                                        <rdf:first rdf:datatype="http://www.w3.org/2001/XMLSchema#string">Road</rdf:first>
                                        <rdf:rest>
                                            <rdf:Description>
                                                <rdf:type rdf:resource="http://www.w3.org/1999/02/22-rdf-syntax-ns#List"/>
                                                <rdf:first rdf:datatype="http://www.w3.org/2001/XMLSchema#string">Water</rdf:first>
                                                <rdf:rest rdf:resource="http://www.w3.org/1999/02/22-rdf-syntax-ns#nil"/>
                                            </rdf:Description>
                                        </rdf:rest>
                                    </rdf:Description>
                                </rdf:rest>
                            </rdf:Description>
                        </rdf:rest>
                    </rdf:Description>
                </owl:oneOf>
            </rdfs:Datatype>
        </rdfs:range>
        <rdfs:comment>Specifies the type of rural delivery. For some addresses, delivery to rural areas happens via water, air or road</rdfs:comment>
        <rdfs:label>Rural Delivery Type</rdfs:label>
    </owl:DatatypeProperty>
    


    <!-- http://www.oasis-open.org/ciq_xal#subAdministrativeAreaType -->

    <owl:DatatypeProperty rdf:about="http://www.oasis-open.org/ciq_xal#subAdministrativeAreaType">
        <rdfs:range>
            <rdfs:Datatype>
                <owl:oneOf>
                    <rdf:Description>
                        <rdf:type rdf:resource="http://www.w3.org/1999/02/22-rdf-syntax-ns#List"/>
                        <rdf:first rdf:datatype="http://www.w3.org/2001/XMLSchema#string">County</rdf:first>
                        <rdf:rest>
                            <rdf:Description>
                                <rdf:type rdf:resource="http://www.w3.org/1999/02/22-rdf-syntax-ns#List"/>
                                <rdf:first rdf:datatype="http://www.w3.org/2001/XMLSchema#string">District</rdf:first>
                                <rdf:rest>
                                    <rdf:Description>
                                        <rdf:type rdf:resource="http://www.w3.org/1999/02/22-rdf-syntax-ns#List"/>
                                        <rdf:first rdf:datatype="http://www.w3.org/2001/XMLSchema#string">Province</rdf:first>
                                        <rdf:rest>
                                            <rdf:Description>
                                                <rdf:type rdf:resource="http://www.w3.org/1999/02/22-rdf-syntax-ns#List"/>
                                                <rdf:first rdf:datatype="http://www.w3.org/2001/XMLSchema#string">Region</rdf:first>
                                                <rdf:rest rdf:resource="http://www.w3.org/1999/02/22-rdf-syntax-ns#nil"/>
                                            </rdf:Description>
                                        </rdf:rest>
                                    </rdf:Description>
                                </rdf:rest>
                            </rdf:Description>
                        </rdf:rest>
                    </rdf:Description>
                </owl:oneOf>
            </rdfs:Datatype>
        </rdfs:range>
        <rdfs:comment>Specifes the type of sub administrative area</rdfs:comment>
        <rdfs:label>Subadminstrative Area Type</rdfs:label>
    </owl:DatatypeProperty>
    


    <!-- http://www.oasis-open.org/ciq_xal#subLocalityName -->

    <owl:DatatypeProperty rdf:about="http://www.oasis-open.org/ciq_xal#subLocalityName">
        <rdfs:range rdf:resource="http://www.w3.org/2001/XMLSchema#string"/>
        <rdfs:comment>Specifies the name of the sub-locality</rdfs:comment>
        <rdfs:label>Sub-Locality Name</rdfs:label>
    </owl:DatatypeProperty>
    


    <!-- http://www.oasis-open.org/ciq_xal#subLocalityNameCode -->

    <owl:DatatypeProperty rdf:about="http://www.oasis-open.org/ciq_xal#subLocalityNameCode">
        <rdfs:range rdf:resource="http://www.w3.org/2001/XMLSchema#string"/>
        <rdfs:comment>Specifies the name of locality represented as a code</rdfs:comment>
        <rdfs:label>Sublocality Name Code</rdfs:label>
    </owl:DatatypeProperty>
    


    <!-- http://www.oasis-open.org/ciq_xal#subPremisesConnector -->

    <owl:DatatypeProperty rdf:about="http://www.oasis-open.org/ciq_xal#subPremisesConnector">
        <rdfs:range rdf:resource="http://www.w3.org/2001/XMLSchema#string"/>
        <rdfs:comment>Specifies a description that is required to logically connect the 2 premises</rdfs:comment>
        <rdfs:label>Sub-Premises Connector</rdfs:label>
    </owl:DatatypeProperty>
    


    <!-- http://www.oasis-open.org/ciq_xal#subPremisesName -->

    <owl:DatatypeProperty rdf:about="http://www.oasis-open.org/ciq_xal#subPremisesName">
        <rdfs:range rdf:resource="http://www.w3.org/2001/XMLSchema#string"/>
        <rdfs:comment>Specifies the name of the sub-premises</rdfs:comment>
        <rdfs:label>Sub-Premises Name</rdfs:label>
    </owl:DatatypeProperty>
    


    <!-- http://www.oasis-open.org/ciq_xal#subPremisesType -->

    <owl:DatatypeProperty rdf:about="http://www.oasis-open.org/ciq_xal#subPremisesType">
        <rdfs:range>
            <rdfs:Datatype>
                <owl:oneOf>
                    <rdf:Description>
                        <rdf:type rdf:resource="http://www.w3.org/1999/02/22-rdf-syntax-ns#List"/>
                        <rdf:first rdf:datatype="http://www.w3.org/2001/XMLSchema#string">Apartment</rdf:first>
                        <rdf:rest>
                            <rdf:Description>
                                <rdf:type rdf:resource="http://www.w3.org/1999/02/22-rdf-syntax-ns#List"/>
                                <rdf:first rdf:datatype="http://www.w3.org/2001/XMLSchema#string">Office</rdf:first>
                                <rdf:rest>
                                    <rdf:Description>
                                        <rdf:type rdf:resource="http://www.w3.org/1999/02/22-rdf-syntax-ns#List"/>
                                        <rdf:first rdf:datatype="http://www.w3.org/2001/XMLSchema#string">Room</rdf:first>
                                        <rdf:rest>
                                            <rdf:Description>
                                                <rdf:type rdf:resource="http://www.w3.org/1999/02/22-rdf-syntax-ns#List"/>
                                                <rdf:first rdf:datatype="http://www.w3.org/2001/XMLSchema#string">Shop</rdf:first>
                                                <rdf:rest>
                                                    <rdf:Description>
                                                        <rdf:type rdf:resource="http://www.w3.org/1999/02/22-rdf-syntax-ns#List"/>
                                                        <rdf:first rdf:datatype="http://www.w3.org/2001/XMLSchema#string">Suite</rdf:first>
                                                        <rdf:rest>
                                                            <rdf:Description>
                                                                <rdf:type rdf:resource="http://www.w3.org/1999/02/22-rdf-syntax-ns#List"/>
                                                                <rdf:first rdf:datatype="http://www.w3.org/2001/XMLSchema#string">Unit</rdf:first>
                                                                <rdf:rest rdf:resource="http://www.w3.org/1999/02/22-rdf-syntax-ns#nil"/>
                                                            </rdf:Description>
                                                        </rdf:rest>
                                                    </rdf:Description>
                                                </rdf:rest>
                                            </rdf:Description>
                                        </rdf:rest>
                                    </rdf:Description>
                                </rdf:rest>
                            </rdf:Description>
                        </rdf:rest>
                    </rdf:Description>
                </owl:oneOf>
            </rdfs:Datatype>
        </rdfs:range>
        <rdfs:comment>Speicfies a type of sub-premises</rdfs:comment>
        <rdfs:label>Sub-Premises Type</rdfs:label>
    </owl:DatatypeProperty>
    


    <!-- http://www.oasis-open.org/ciq_xal#subPremisesTypeCode -->

    <owl:DatatypeProperty rdf:about="http://www.oasis-open.org/ciq_xal#subPremisesTypeCode">
        <rdfs:range rdf:resource="http://www.w3.org/2001/XMLSchema#string"/>
        <rdfs:comment>Specifies the type of code used for sub-premises</rdfs:comment>
        <rdfs:label>Sub-Premises Type Code</rdfs:label>
    </owl:DatatypeProperty>
    


    <!-- http://www.oasis-open.org/ciq_xal#subjectToEUSavingsDirective -->

    <owl:DatatypeProperty rdf:about="http://www.oasis-open.org/ciq_xal#subjectToEUSavingsDirective">
        <rdfs:range rdf:resource="http://www.w3.org/2001/XMLSchema#boolean"/>
        <rdfs:comment>Specifies whether the country is subject to the European Union Savings Directive</rdfs:comment>
        <rdfs:isDefinedBy rdf:resource="http://www.oasis-open.org/ciq_xal"/>
        <rdfs:label>Subject to EU Savings Directive</rdfs:label>
    </owl:DatatypeProperty>
    


    <!-- http://www.oasis-open.org/ciq_xal#subjectToVAT -->

    <owl:DatatypeProperty rdf:about="http://www.oasis-open.org/ciq_xal#subjectToVAT">
        <rdfs:range rdf:resource="http://www.w3.org/2001/XMLSchema#boolean"/>
        <rdfs:comment>Specifies whether the country is subject to the European Union&apos;s Value Added Tax (VAT)</rdfs:comment>
        <rdfs:isDefinedBy rdf:resource="http://www.oasis-open.org/ciq_xal"/>
        <rdfs:label>Subject to VAT</rdfs:label>
    </owl:DatatypeProperty>
    


    <!-- http://www.oasis-open.org/ciq_xal#sublocalityType -->

    <owl:DatatypeProperty rdf:about="http://www.oasis-open.org/ciq_xal#sublocalityType">
        <rdfs:range>
            <rdfs:Datatype>
                <owl:oneOf>
                    <rdf:Description>
                        <rdf:type rdf:resource="http://www.w3.org/1999/02/22-rdf-syntax-ns#List"/>
                        <rdf:first rdf:datatype="http://www.w3.org/2001/XMLSchema#string">Municipality</rdf:first>
                        <rdf:rest>
                            <rdf:Description>
                                <rdf:type rdf:resource="http://www.w3.org/1999/02/22-rdf-syntax-ns#List"/>
                                <rdf:first rdf:datatype="http://www.w3.org/2001/XMLSchema#string">Village</rdf:first>
                                <rdf:rest rdf:resource="http://www.w3.org/1999/02/22-rdf-syntax-ns#nil"/>
                            </rdf:Description>
                        </rdf:rest>
                    </rdf:Description>
                </owl:oneOf>
            </rdfs:Datatype>
        </rdfs:range>
        <rdfs:comment>Specifies the type of sublocality</rdfs:comment>
        <rdfs:label>Sublocality Type</rdfs:label>
    </owl:DatatypeProperty>
    


    <!-- http://www.oasis-open.org/ciq_xal#supportingInfo -->

    <owl:DatatypeProperty rdf:about="http://www.oasis-open.org/ciq_xal#supportingInfo">
        <rdfs:range rdf:resource="http://www.w3.org/2001/XMLSchema#string"/>
        <rdfs:comment>Specifies other supporting information</rdfs:comment>
        <rdfs:label>Supporting Information</rdfs:label>
    </owl:DatatypeProperty>
    


    <!-- http://www.oasis-open.org/ciq_xal#thoroughfareConnector -->

    <owl:DatatypeProperty rdf:about="http://www.oasis-open.org/ciq_xal#thoroughfareConnector">
        <rdfs:range rdf:resource="http://www.w3.org/2001/XMLSchema#string"/>
        <rdfs:comment>Specifies a value such as &quot;CORNER OF&quot; or &quot;VIA&quot; that can be used to connect more than one street name in order to identify the location.</rdfs:comment>
        <rdfs:isDefinedBy rdf:resource="http://www.oasis-open.org/ciq_xal"/>
        <rdfs:label>Thoroughfare Connector</rdfs:label>
    </owl:DatatypeProperty>
    


    <!-- http://www.oasis-open.org/ciq_xal#thoroughfareName -->

    <owl:DatatypeProperty rdf:about="http://www.oasis-open.org/ciq_xal#thoroughfareName">
        <rdfs:range rdf:resource="http://www.w3.org/2001/XMLSchema#string"/>
        <rdfs:comment>Specifies the fully combiined name of the thoroughfare. e.g. Full thoroughfare name or part of it, type of thoroughfare, old name, new name, reference data in support of the thoroughfare</rdfs:comment>
        <rdfs:label>Thoroughfare Name</rdfs:label>
    </owl:DatatypeProperty>
    


    <!-- http://www.oasis-open.org/ciq_xal#thoroughfareNumber -->

    <owl:DatatypeProperty rdf:about="http://www.oasis-open.org/ciq_xal#thoroughfareNumber">
        <rdfs:range rdf:resource="http://www.w3.org/2001/XMLSchema#string"/>
        <rdfs:comment>Specifies the data associated with the number of the thoroughfare. E.g. 39 in 39 Baker Street, street range, street suffix</rdfs:comment>
        <rdfs:label>Thoroughfare Number</rdfs:label>
    </owl:DatatypeProperty>
    


    <!-- http://www.oasis-open.org/ciq_xal#thoroughfareType -->

    <owl:DatatypeProperty rdf:about="http://www.oasis-open.org/ciq_xal#thoroughfareType">
        <rdfs:range>
            <rdfs:Datatype>
                <owl:oneOf>
                    <rdf:Description>
                        <rdf:type rdf:resource="http://www.w3.org/1999/02/22-rdf-syntax-ns#List"/>
                        <rdf:first rdf:datatype="http://www.w3.org/2001/XMLSchema#string">AVENUE</rdf:first>
                        <rdf:rest>
                            <rdf:Description>
                                <rdf:type rdf:resource="http://www.w3.org/1999/02/22-rdf-syntax-ns#List"/>
                                <rdf:first rdf:datatype="http://www.w3.org/2001/XMLSchema#string">COURT</rdf:first>
                                <rdf:rest>
                                    <rdf:Description>
                                        <rdf:type rdf:resource="http://www.w3.org/1999/02/22-rdf-syntax-ns#List"/>
                                        <rdf:first rdf:datatype="http://www.w3.org/2001/XMLSchema#string">ROAD</rdf:first>
                                        <rdf:rest>
                                            <rdf:Description>
                                                <rdf:type rdf:resource="http://www.w3.org/1999/02/22-rdf-syntax-ns#List"/>
                                                <rdf:first rdf:datatype="http://www.w3.org/2001/XMLSchema#string">STREET</rdf:first>
                                                <rdf:rest rdf:resource="http://www.w3.org/1999/02/22-rdf-syntax-ns#nil"/>
                                            </rdf:Description>
                                        </rdf:rest>
                                    </rdf:Description>
                                </rdf:rest>
                            </rdf:Description>
                        </rdf:rest>
                    </rdf:Description>
                </owl:oneOf>
            </rdfs:Datatype>
        </rdfs:range>
        <rdfs:comment>Specifies the type of thoroughfare. eg. primary road, secondary road, road branch (e.g. Lane 14), road sub branch (e.g. Alley 21), adjourning street, cross street, closest street, etc</rdfs:comment>
        <rdfs:label>Thoroughfare Type</rdfs:label>
    </owl:DatatypeProperty>
    


    <!-- http://www.oasis-open.org/ciq_xal#thoroughfareTypeCode -->

    <owl:DatatypeProperty rdf:about="http://www.oasis-open.org/ciq_xal#thoroughfareTypeCode">
        <rdfs:range rdf:resource="http://www.w3.org/2001/XMLSchema#string"/>
        <rdfs:comment>Sspecifies the type of code use for thoroughfare</rdfs:comment>
        <rdfs:label>Thoroughfare Type Code</rdfs:label>
    </owl:DatatypeProperty>
    


    <!-- http://www.oasis-open.org/ciq_xal#timezoneId -->

    <owl:DatatypeProperty rdf:about="http://www.oasis-open.org/ciq_xal#timezoneId">
        <rdfs:range rdf:resource="http://www.w3.org/2001/XMLSchema#string"/>
        <rdfs:comment>Specifies the IANA timezone identifier</rdfs:comment>
        <rdfs:isDefinedBy rdf:resource="http://www.oasis-open.org/ciq_xal"/>
        <rdfs:label>Timezone Identifier</rdfs:label>
    </owl:DatatypeProperty>
    


    <!-- 
    ///////////////////////////////////////////////////////////////////////////////////////
    //
    // Classes
    //
    ///////////////////////////////////////////////////////////////////////////////////////
     -->

    


    <!-- http://www.oasis-open.org/ciq_currency#Currency -->

    <owl:Class rdf:about="http://www.oasis-open.org/ciq_currency#Currency"/>
    


    <!-- http://www.oasis-open.org/ciq_xal#Address -->

    <owl:Class rdf:about="http://www.oasis-open.org/ciq_xal#Address">
        <rdfs:subClassOf>
            <owl:Restriction>
                <owl:onProperty rdf:resource="http://www.oasis-open.org/ciq_xal#administrativeArea"/>
                <owl:someValuesFrom rdf:resource="http://www.w3.org/2002/07/owl#Thing"/>
            </owl:Restriction>
        </rdfs:subClassOf>
        <rdfs:subClassOf>
            <owl:Restriction>
                <owl:onProperty rdf:resource="http://www.oasis-open.org/ciq_xal#country"/>
                <owl:someValuesFrom rdf:resource="http://www.w3.org/2002/07/owl#Thing"/>
            </owl:Restriction>
        </rdfs:subClassOf>
        <rdfs:subClassOf>
            <owl:Restriction>
                <owl:onProperty rdf:resource="http://www.oasis-open.org/ciq_xal#locality"/>
                <owl:someValuesFrom rdf:resource="http://www.w3.org/2002/07/owl#Thing"/>
            </owl:Restriction>
        </rdfs:subClassOf>
        <rdfs:subClassOf>
            <owl:Restriction>
                <owl:onProperty rdf:resource="http://www.oasis-open.org/ciq_xal#postOffice"/>
                <owl:someValuesFrom rdf:resource="http://www.w3.org/2002/07/owl#Thing"/>
            </owl:Restriction>
        </rdfs:subClassOf>
        <rdfs:subClassOf>
            <owl:Restriction>
                <owl:onProperty rdf:resource="http://www.oasis-open.org/ciq_xal#postalDelliveryPoint"/>
                <owl:someValuesFrom rdf:resource="http://www.w3.org/2002/07/owl#Thing"/>
            </owl:Restriction>
        </rdfs:subClassOf>
        <rdfs:subClassOf>
            <owl:Restriction>
                <owl:onProperty rdf:resource="http://www.oasis-open.org/ciq_xal#postcode"/>
                <owl:someValuesFrom rdf:resource="http://www.w3.org/2002/07/owl#Thing"/>
            </owl:Restriction>
        </rdfs:subClassOf>
        <rdfs:subClassOf>
            <owl:Restriction>
                <owl:onProperty rdf:resource="http://www.oasis-open.org/ciq_xal#premises"/>
                <owl:someValuesFrom rdf:resource="http://www.w3.org/2002/07/owl#Thing"/>
            </owl:Restriction>
        </rdfs:subClassOf>
        <rdfs:subClassOf>
            <owl:Restriction>
                <owl:onProperty rdf:resource="http://www.oasis-open.org/ciq_xal#ruralDelivery"/>
                <owl:someValuesFrom rdf:resource="http://www.w3.org/2002/07/owl#Thing"/>
            </owl:Restriction>
        </rdfs:subClassOf>
        <rdfs:subClassOf>
            <owl:Restriction>
                <owl:onProperty rdf:resource="http://www.oasis-open.org/ciq_xal#subAdministrativeArea"/>
                <owl:someValuesFrom rdf:resource="http://www.w3.org/2002/07/owl#Thing"/>
            </owl:Restriction>
        </rdfs:subClassOf>
        <rdfs:subClassOf>
            <owl:Restriction>
                <owl:onProperty rdf:resource="http://www.oasis-open.org/ciq_xal#subLocality"/>
                <owl:someValuesFrom rdf:resource="http://www.w3.org/2002/07/owl#Thing"/>
            </owl:Restriction>
        </rdfs:subClassOf>
        <rdfs:subClassOf>
            <owl:Restriction>
                <owl:onProperty rdf:resource="http://www.oasis-open.org/ciq_xal#thoroughfare"/>
                <owl:someValuesFrom rdf:resource="http://www.w3.org/2002/07/owl#Thing"/>
            </owl:Restriction>
        </rdfs:subClassOf>
        <rdfs:subClassOf>
            <owl:Restriction>
                <owl:onProperty rdf:resource="http://www.oasis-open.org/ciq_xal#addressType"/>
                <owl:someValuesFrom rdf:resource="http://www.w3.org/2000/01/rdf-schema#Literal"/>
            </owl:Restriction>
        </rdfs:subClassOf>
        <rdfs:subClassOf>
            <owl:Restriction>
                <owl:onProperty rdf:resource="http://www.oasis-open.org/ciq_xal#addressUsage"/>
                <owl:someValuesFrom rdf:resource="http://www.w3.org/2000/01/rdf-schema#Literal"/>
            </owl:Restriction>
        </rdfs:subClassOf>
        <rdfs:subClassOf>
            <owl:Restriction>
                <owl:onProperty rdf:resource="http://www.oasis-open.org/ciq_xal#deliveryMode"/>
                <owl:someValuesFrom rdf:resource="http://www.w3.org/2000/01/rdf-schema#Literal"/>
            </owl:Restriction>
        </rdfs:subClassOf>
        <rdfs:subClassOf>
            <owl:Restriction>
                <owl:onProperty rdf:resource="http://www.oasis-open.org/ciq_xal#freeTextAddress"/>
                <owl:someValuesFrom rdf:resource="http://www.w3.org/2000/01/rdf-schema#Literal"/>
            </owl:Restriction>
        </rdfs:subClassOf>
        <rdfs:subClassOf>
            <owl:Restriction>
                <owl:onProperty rdf:resource="http://www.oasis-open.org/ciq_xal#geoCoordinates.datum"/>
                <owl:someValuesFrom rdf:resource="http://www.w3.org/2000/01/rdf-schema#Literal"/>
            </owl:Restriction>
        </rdfs:subClassOf>
        <rdfs:subClassOf>
            <owl:Restriction>
                <owl:onProperty rdf:resource="http://www.oasis-open.org/ciq_xal#geoCoordinates.datumCodeType"/>
                <owl:someValuesFrom rdf:resource="http://www.w3.org/2000/01/rdf-schema#Literal"/>
            </owl:Restriction>
        </rdfs:subClassOf>
        <rdfs:subClassOf>
            <owl:Restriction>
                <owl:onProperty rdf:resource="http://www.oasis-open.org/ciq_xal#geoCoordinates.meridian"/>
                <owl:someValuesFrom rdf:resource="http://www.w3.org/2000/01/rdf-schema#Literal"/>
            </owl:Restriction>
        </rdfs:subClassOf>
        <rdfs:subClassOf>
            <owl:Restriction>
                <owl:onProperty rdf:resource="http://www.oasis-open.org/ciq_xal#geoCoordinates.meridianCodeType"/>
                <owl:someValuesFrom rdf:resource="http://www.w3.org/2000/01/rdf-schema#Literal"/>
            </owl:Restriction>
        </rdfs:subClassOf>
        <rdfs:subClassOf>
            <owl:Restriction>
                <owl:onProperty rdf:resource="http://www.oasis-open.org/ciq_xal#geoCoordinates.projection"/>
                <owl:someValuesFrom rdf:resource="http://www.w3.org/2000/01/rdf-schema#Literal"/>
            </owl:Restriction>
        </rdfs:subClassOf>
        <rdfs:subClassOf>
            <owl:Restriction>
                <owl:onProperty rdf:resource="http://www.oasis-open.org/ciq_xal#geoCoordinates.projectionCodeType"/>
                <owl:someValuesFrom rdf:resource="http://www.w3.org/2000/01/rdf-schema#Literal"/>
            </owl:Restriction>
        </rdfs:subClassOf>
        <rdfs:comment>Defines an address with geocode details</rdfs:comment>
        <rdfs:isDefinedBy rdf:resource="http://www.oasis-open.org/ciq_xal"/>
        <rdfs:label>Address</rdfs:label>
    </owl:Class>
    


    <!-- http://www.oasis-open.org/ciq_xal#AdministrativeArea -->

    <owl:Class rdf:about="http://www.oasis-open.org/ciq_xal#AdministrativeArea">
        <rdfs:subClassOf>
            <owl:Restriction>
                <owl:onProperty rdf:resource="http://www.oasis-open.org/ciq_xal#parentAdminArea1"/>
                <owl:someValuesFrom rdf:resource="http://www.w3.org/2002/07/owl#Thing"/>
            </owl:Restriction>
        </rdfs:subClassOf>
        <rdfs:subClassOf>
            <owl:Restriction>
                <owl:onProperty rdf:resource="http://www.oasis-open.org/ciq_xal#parentAdminArea2"/>
                <owl:someValuesFrom rdf:resource="http://www.w3.org/2002/07/owl#Thing"/>
            </owl:Restriction>
        </rdfs:subClassOf>
        <rdfs:subClassOf>
            <owl:Restriction>
                <owl:onProperty rdf:resource="http://www.oasis-open.org/ciq_xal#parentAdminArea3"/>
                <owl:someValuesFrom rdf:resource="http://www.w3.org/2002/07/owl#Thing"/>
            </owl:Restriction>
        </rdfs:subClassOf>
        <rdfs:subClassOf>
            <owl:Restriction>
                <owl:onProperty rdf:resource="http://www.oasis-open.org/ciq_xal#parentAdminArea4"/>
                <owl:someValuesFrom rdf:resource="http://www.w3.org/2002/07/owl#Thing"/>
            </owl:Restriction>
        </rdfs:subClassOf>
        <rdfs:subClassOf>
            <owl:Restriction>
                <owl:onProperty rdf:resource="http://www.oasis-open.org/ciq_xal#parentCountry"/>
                <owl:someValuesFrom rdf:resource="http://www.w3.org/2002/07/owl#Thing"/>
            </owl:Restriction>
        </rdfs:subClassOf>
        <rdfs:subClassOf>
            <owl:Restriction>
                <owl:onProperty rdf:resource="http://www.oasis-open.org/ciq_xal#adminAreaName"/>
                <owl:someValuesFrom rdf:resource="http://www.w3.org/2000/01/rdf-schema#Literal"/>
            </owl:Restriction>
        </rdfs:subClassOf>
        <rdfs:subClassOf>
            <owl:Restriction>
                <owl:onProperty rdf:resource="http://www.oasis-open.org/ciq_xal#adminAreaNameCodeType"/>
                <owl:someValuesFrom rdf:resource="http://www.w3.org/2000/01/rdf-schema#Literal"/>
            </owl:Restriction>
        </rdfs:subClassOf>
        <rdfs:subClassOf>
            <owl:Restriction>
                <owl:onProperty rdf:resource="http://www.oasis-open.org/ciq_xal#adminAreaType"/>
                <owl:someValuesFrom rdf:resource="http://www.w3.org/2000/01/rdf-schema#Literal"/>
            </owl:Restriction>
        </rdfs:subClassOf>
        <rdfs:subClassOf>
            <owl:Restriction>
                <owl:onProperty rdf:resource="http://www.oasis-open.org/ciq_xal#asciiName"/>
                <owl:someValuesFrom rdf:resource="http://www.w3.org/2000/01/rdf-schema#Literal"/>
            </owl:Restriction>
        </rdfs:subClassOf>
        <rdfs:subClassOf>
            <owl:Restriction>
                <owl:onProperty rdf:resource="http://www.oasis-open.org/ciq_xal#digitalElevationModel"/>
                <owl:someValuesFrom rdf:resource="http://www.w3.org/2000/01/rdf-schema#Literal"/>
            </owl:Restriction>
        </rdfs:subClassOf>
        <rdfs:subClassOf>
            <owl:Restriction>
                <owl:onProperty rdf:resource="http://www.oasis-open.org/ciq_xal#featureInfo"/>
                <owl:someValuesFrom rdf:resource="http://www.w3.org/2000/01/rdf-schema#Literal"/>
            </owl:Restriction>
        </rdfs:subClassOf>
        <rdfs:subClassOf>
            <owl:Restriction>
                <owl:onProperty rdf:resource="http://www.oasis-open.org/ciq_xal#geonameId"/>
                <owl:someValuesFrom rdf:resource="http://www.w3.org/2000/01/rdf-schema#Literal"/>
            </owl:Restriction>
        </rdfs:subClassOf>
        <rdfs:subClassOf>
            <owl:Restriction>
                <owl:onProperty rdf:resource="http://www.oasis-open.org/ciq_xal#lastModifiedDate"/>
                <owl:someValuesFrom rdf:resource="http://www.w3.org/2000/01/rdf-schema#Literal"/>
            </owl:Restriction>
        </rdfs:subClassOf>
        <rdfs:subClassOf>
            <owl:Restriction>
                <owl:onProperty rdf:resource="http://www.oasis-open.org/ciq_xal#population"/>
                <owl:someValuesFrom rdf:resource="http://www.w3.org/2000/01/rdf-schema#Literal"/>
            </owl:Restriction>
        </rdfs:subClassOf>
        <rdfs:subClassOf>
            <owl:Restriction>
                <owl:onProperty rdf:resource="http://www.oasis-open.org/ciq_xal#referenceLocation"/>
                <owl:someValuesFrom rdf:resource="http://www.w3.org/2000/01/rdf-schema#Literal"/>
            </owl:Restriction>
        </rdfs:subClassOf>
        <rdfs:subClassOf>
            <owl:Restriction>
                <owl:onProperty rdf:resource="http://www.oasis-open.org/ciq_xal#timezoneId"/>
                <owl:someValuesFrom rdf:resource="http://www.w3.org/2000/01/rdf-schema#Literal"/>
            </owl:Restriction>
        </rdfs:subClassOf>
        <rdfs:comment>Defines the details of the top-level area division in the country, such as state, district, province, island, region, etc. Note that some countries do not have this</rdfs:comment>
        <rdfs:isDefinedBy rdf:resource="http://www.oasis-open.org/ciq_xal"/>
        <rdfs:label>Administrative Area</rdfs:label>
    </owl:Class>
    


    <!-- http://www.oasis-open.org/ciq_xal#Continent -->

    <owl:Class rdf:about="http://www.oasis-open.org/ciq_xal#Continent">
        <rdfs:subClassOf>
            <owl:Restriction>
                <owl:onProperty rdf:resource="http://www.oasis-open.org/ciq_xal#continentCode"/>
                <owl:someValuesFrom rdf:resource="http://www.w3.org/2000/01/rdf-schema#Literal"/>
            </owl:Restriction>
        </rdfs:subClassOf>
        <rdfs:subClassOf>
            <owl:Restriction>
                <owl:onProperty rdf:resource="http://www.oasis-open.org/ciq_xal#continentName"/>
                <owl:someValuesFrom rdf:resource="http://www.w3.org/2000/01/rdf-schema#Literal"/>
            </owl:Restriction>
        </rdfs:subClassOf>
        <rdfs:subClassOf>
            <owl:Restriction>
                <owl:onProperty rdf:resource="http://www.oasis-open.org/ciq_xal#featureInfo"/>
                <owl:someValuesFrom rdf:resource="http://www.w3.org/2000/01/rdf-schema#Literal"/>
            </owl:Restriction>
        </rdfs:subClassOf>
        <rdfs:subClassOf>
            <owl:Restriction>
                <owl:onProperty rdf:resource="http://www.oasis-open.org/ciq_xal#geonameId"/>
                <owl:someValuesFrom rdf:resource="http://www.w3.org/2000/01/rdf-schema#Literal"/>
            </owl:Restriction>
        </rdfs:subClassOf>
        <rdfs:comment>Characterizes details about a continent</rdfs:comment>
        <rdfs:isDefinedBy rdf:resource="http://www.oasis-open.org/ciq_xal"/>
        <rdfs:label>Continent</rdfs:label>
    </owl:Class>
    


    <!-- http://www.oasis-open.org/ciq_xal#Country -->

    <owl:Class rdf:about="http://www.oasis-open.org/ciq_xal#Country">
        <rdfs:subClassOf>
            <owl:Restriction>
                <owl:onProperty rdf:resource="http://www.oasis-open.org/ciq_xal#capital"/>
                <owl:someValuesFrom rdf:resource="http://www.w3.org/2002/07/owl#Thing"/>
            </owl:Restriction>
        </rdfs:subClassOf>
        <rdfs:subClassOf>
            <owl:Restriction>
                <owl:onProperty rdf:resource="http://www.oasis-open.org/ciq_xal#continent"/>
                <owl:someValuesFrom rdf:resource="http://www.w3.org/2002/07/owl#Thing"/>
            </owl:Restriction>
        </rdfs:subClassOf>
        <rdfs:subClassOf>
            <owl:Restriction>
                <owl:onProperty rdf:resource="http://www.oasis-open.org/ciq_xal#currency"/>
                <owl:someValuesFrom rdf:resource="http://www.w3.org/2002/07/owl#Thing"/>
            </owl:Restriction>
        </rdfs:subClassOf>
        <rdfs:subClassOf>
            <owl:Restriction>
                <owl:onProperty rdf:resource="http://www.oasis-open.org/ciq_xal#area"/>
                <owl:someValuesFrom rdf:resource="http://www.w3.org/2000/01/rdf-schema#Literal"/>
            </owl:Restriction>
        </rdfs:subClassOf>
        <rdfs:subClassOf>
            <owl:Restriction>
                <owl:onProperty rdf:resource="http://www.oasis-open.org/ciq_xal#asciiName"/>
                <owl:someValuesFrom rdf:resource="http://www.w3.org/2000/01/rdf-schema#Literal"/>
            </owl:Restriction>
        </rdfs:subClassOf>
        <rdfs:subClassOf>
            <owl:Restriction>
                <owl:onProperty rdf:resource="http://www.oasis-open.org/ciq_xal#callingCodes"/>
                <owl:someValuesFrom rdf:resource="http://www.w3.org/2000/01/rdf-schema#Literal"/>
            </owl:Restriction>
        </rdfs:subClassOf>
        <rdfs:subClassOf>
            <owl:Restriction>
                <owl:onProperty rdf:resource="http://www.oasis-open.org/ciq_xal#countryFlagImage"/>
                <owl:someValuesFrom rdf:resource="http://www.w3.org/2000/01/rdf-schema#Literal"/>
            </owl:Restriction>
        </rdfs:subClassOf>
        <rdfs:subClassOf>
            <owl:Restriction>
                <owl:onProperty rdf:resource="http://www.oasis-open.org/ciq_xal#countryFlagRef"/>
                <owl:someValuesFrom rdf:resource="http://www.w3.org/2000/01/rdf-schema#Literal"/>
            </owl:Restriction>
        </rdfs:subClassOf>
        <rdfs:subClassOf>
            <owl:Restriction>
                <owl:onProperty rdf:resource="http://www.oasis-open.org/ciq_xal#countryName"/>
                <owl:someValuesFrom rdf:resource="http://www.w3.org/2000/01/rdf-schema#Literal"/>
            </owl:Restriction>
        </rdfs:subClassOf>
        <rdfs:subClassOf>
            <owl:Restriction>
                <owl:onProperty rdf:resource="http://www.oasis-open.org/ciq_xal#digitalElevationModel"/>
                <owl:someValuesFrom rdf:resource="http://www.w3.org/2000/01/rdf-schema#Literal"/>
            </owl:Restriction>
        </rdfs:subClassOf>
        <rdfs:subClassOf>
            <owl:Restriction>
                <owl:onProperty rdf:resource="http://www.oasis-open.org/ciq_xal#featureInfo"/>
                <owl:someValuesFrom rdf:resource="http://www.w3.org/2000/01/rdf-schema#Literal"/>
            </owl:Restriction>
        </rdfs:subClassOf>
        <rdfs:subClassOf>
            <owl:Restriction>
                <owl:onProperty rdf:resource="http://www.oasis-open.org/ciq_xal#fipsCountryCode"/>
                <owl:someValuesFrom rdf:resource="http://www.w3.org/2000/01/rdf-schema#Literal"/>
            </owl:Restriction>
        </rdfs:subClassOf>
        <rdfs:subClassOf>
            <owl:Restriction>
                <owl:onProperty rdf:resource="http://www.oasis-open.org/ciq_xal#geonameId"/>
                <owl:someValuesFrom rdf:resource="http://www.w3.org/2000/01/rdf-schema#Literal"/>
            </owl:Restriction>
        </rdfs:subClassOf>
        <rdfs:subClassOf>
            <owl:Restriction>
                <owl:onProperty rdf:resource="http://www.oasis-open.org/ciq_xal#internetTLD"/>
                <owl:someValuesFrom rdf:resource="http://www.w3.org/2000/01/rdf-schema#Literal"/>
            </owl:Restriction>
        </rdfs:subClassOf>
        <rdfs:subClassOf>
            <owl:Restriction>
                <owl:onProperty rdf:resource="http://www.oasis-open.org/ciq_xal#iso2CountryCode"/>
                <owl:someValuesFrom rdf:resource="http://www.w3.org/2000/01/rdf-schema#Literal"/>
            </owl:Restriction>
        </rdfs:subClassOf>
        <rdfs:subClassOf>
            <owl:Restriction>
                <owl:onProperty rdf:resource="http://www.oasis-open.org/ciq_xal#iso3CountryCode"/>
                <owl:someValuesFrom rdf:resource="http://www.w3.org/2000/01/rdf-schema#Literal"/>
            </owl:Restriction>
        </rdfs:subClassOf>
        <rdfs:subClassOf>
            <owl:Restriction>
                <owl:onProperty rdf:resource="http://www.oasis-open.org/ciq_xal#iso4CountryCode"/>
                <owl:someValuesFrom rdf:resource="http://www.w3.org/2000/01/rdf-schema#Literal"/>
            </owl:Restriction>
        </rdfs:subClassOf>
        <rdfs:subClassOf>
            <owl:Restriction>
                <owl:onProperty rdf:resource="http://www.oasis-open.org/ciq_xal#isoNumericCountryCode"/>
                <owl:someValuesFrom rdf:resource="http://www.w3.org/2000/01/rdf-schema#Literal"/>
            </owl:Restriction>
        </rdfs:subClassOf>
        <rdfs:subClassOf>
            <owl:Restriction>
                <owl:onProperty rdf:resource="http://www.oasis-open.org/ciq_xal#lastModifiedDate"/>
                <owl:someValuesFrom rdf:resource="http://www.w3.org/2000/01/rdf-schema#Literal"/>
            </owl:Restriction>
        </rdfs:subClassOf>
        <rdfs:subClassOf>
            <owl:Restriction>
                <owl:onProperty rdf:resource="http://www.oasis-open.org/ciq_xal#memberOfOECD"/>
                <owl:someValuesFrom rdf:resource="http://www.w3.org/2000/01/rdf-schema#Literal"/>
            </owl:Restriction>
        </rdfs:subClassOf>
        <rdfs:subClassOf>
            <owl:Restriction>
                <owl:onProperty rdf:resource="http://www.oasis-open.org/ciq_xal#postalCodeFormat"/>
                <owl:someValuesFrom rdf:resource="http://www.w3.org/2000/01/rdf-schema#Literal"/>
            </owl:Restriction>
        </rdfs:subClassOf>
        <rdfs:subClassOf>
            <owl:Restriction>
                <owl:onProperty rdf:resource="http://www.oasis-open.org/ciq_xal#subjectToEUSavingsDirective"/>
                <owl:someValuesFrom rdf:resource="http://www.w3.org/2000/01/rdf-schema#Literal"/>
            </owl:Restriction>
        </rdfs:subClassOf>
        <rdfs:subClassOf>
            <owl:Restriction>
                <owl:onProperty rdf:resource="http://www.oasis-open.org/ciq_xal#subjectToVAT"/>
                <owl:someValuesFrom rdf:resource="http://www.w3.org/2000/01/rdf-schema#Literal"/>
            </owl:Restriction>
        </rdfs:subClassOf>
        <rdfs:comment>Defines details about a country</rdfs:comment>
        <rdfs:isDefinedBy rdf:resource="http://www.oasis-open.org/ciq_xal"/>
        <rdfs:label>Country</rdfs:label>
    </owl:Class>
    


    <!-- http://www.oasis-open.org/ciq_xal#Locality -->

    <owl:Class rdf:about="http://www.oasis-open.org/ciq_xal#Locality">
        <rdfs:subClassOf>
            <owl:Restriction>
                <owl:onProperty rdf:resource="http://www.oasis-open.org/ciq_xal#parentAdminArea1"/>
                <owl:someValuesFrom rdf:resource="http://www.w3.org/2002/07/owl#Thing"/>
            </owl:Restriction>
        </rdfs:subClassOf>
        <rdfs:subClassOf>
            <owl:Restriction>
                <owl:onProperty rdf:resource="http://www.oasis-open.org/ciq_xal#parentAdminArea2"/>
                <owl:someValuesFrom rdf:resource="http://www.w3.org/2002/07/owl#Thing"/>
            </owl:Restriction>
        </rdfs:subClassOf>
        <rdfs:subClassOf>
            <owl:Restriction>
                <owl:onProperty rdf:resource="http://www.oasis-open.org/ciq_xal#parentAdminArea3"/>
                <owl:someValuesFrom rdf:resource="http://www.w3.org/2002/07/owl#Thing"/>
            </owl:Restriction>
        </rdfs:subClassOf>
        <rdfs:subClassOf>
            <owl:Restriction>
                <owl:onProperty rdf:resource="http://www.oasis-open.org/ciq_xal#parentAdminArea4"/>
                <owl:someValuesFrom rdf:resource="http://www.w3.org/2002/07/owl#Thing"/>
            </owl:Restriction>
        </rdfs:subClassOf>
        <rdfs:subClassOf>
            <owl:Restriction>
                <owl:onProperty rdf:resource="http://www.oasis-open.org/ciq_xal#parentCountry"/>
                <owl:someValuesFrom rdf:resource="http://www.w3.org/2002/07/owl#Thing"/>
            </owl:Restriction>
        </rdfs:subClassOf>
        <rdfs:subClassOf>
            <owl:Restriction>
                <owl:onProperty rdf:resource="http://www.oasis-open.org/ciq_xal#asciiName"/>
                <owl:someValuesFrom rdf:resource="http://www.w3.org/2000/01/rdf-schema#Literal"/>
            </owl:Restriction>
        </rdfs:subClassOf>
        <rdfs:subClassOf>
            <owl:Restriction>
                <owl:onProperty rdf:resource="http://www.oasis-open.org/ciq_xal#digitalElevationModel"/>
                <owl:someValuesFrom rdf:resource="http://www.w3.org/2000/01/rdf-schema#Literal"/>
            </owl:Restriction>
        </rdfs:subClassOf>
        <rdfs:subClassOf>
            <owl:Restriction>
                <owl:onProperty rdf:resource="http://www.oasis-open.org/ciq_xal#featureInfo"/>
                <owl:someValuesFrom rdf:resource="http://www.w3.org/2000/01/rdf-schema#Literal"/>
            </owl:Restriction>
        </rdfs:subClassOf>
        <rdfs:subClassOf>
            <owl:Restriction>
                <owl:onProperty rdf:resource="http://www.oasis-open.org/ciq_xal#geonameId"/>
                <owl:someValuesFrom rdf:resource="http://www.w3.org/2000/01/rdf-schema#Literal"/>
            </owl:Restriction>
        </rdfs:subClassOf>
        <rdfs:subClassOf>
            <owl:Restriction>
                <owl:onProperty rdf:resource="http://www.oasis-open.org/ciq_xal#lastModifiedDate"/>
                <owl:someValuesFrom rdf:resource="http://www.w3.org/2000/01/rdf-schema#Literal"/>
            </owl:Restriction>
        </rdfs:subClassOf>
        <rdfs:subClassOf>
            <owl:Restriction>
                <owl:onProperty rdf:resource="http://www.oasis-open.org/ciq_xal#localityName"/>
                <owl:someValuesFrom rdf:resource="http://www.w3.org/2000/01/rdf-schema#Literal"/>
            </owl:Restriction>
        </rdfs:subClassOf>
        <rdfs:subClassOf>
            <owl:Restriction>
                <owl:onProperty rdf:resource="http://www.oasis-open.org/ciq_xal#localityNameCode"/>
                <owl:someValuesFrom rdf:resource="http://www.w3.org/2000/01/rdf-schema#Literal"/>
            </owl:Restriction>
        </rdfs:subClassOf>
        <rdfs:subClassOf>
            <owl:Restriction>
                <owl:onProperty rdf:resource="http://www.oasis-open.org/ciq_xal#localityNameCodeType"/>
                <owl:someValuesFrom rdf:resource="http://www.w3.org/2000/01/rdf-schema#Literal"/>
            </owl:Restriction>
        </rdfs:subClassOf>
        <rdfs:subClassOf>
            <owl:Restriction>
                <owl:onProperty rdf:resource="http://www.oasis-open.org/ciq_xal#localityType"/>
                <owl:someValuesFrom rdf:resource="http://www.w3.org/2000/01/rdf-schema#Literal"/>
            </owl:Restriction>
        </rdfs:subClassOf>
        <rdfs:subClassOf>
            <owl:Restriction>
                <owl:onProperty rdf:resource="http://www.oasis-open.org/ciq_xal#population"/>
                <owl:someValuesFrom rdf:resource="http://www.w3.org/2000/01/rdf-schema#Literal"/>
            </owl:Restriction>
        </rdfs:subClassOf>
        <rdfs:subClassOf>
            <owl:Restriction>
                <owl:onProperty rdf:resource="http://www.oasis-open.org/ciq_xal#referenceLocation"/>
                <owl:someValuesFrom rdf:resource="http://www.w3.org/2000/01/rdf-schema#Literal"/>
            </owl:Restriction>
        </rdfs:subClassOf>
        <rdfs:subClassOf>
            <owl:Restriction>
                <owl:onProperty rdf:resource="http://www.oasis-open.org/ciq_xal#timezoneId"/>
                <owl:someValuesFrom rdf:resource="http://www.w3.org/2000/01/rdf-schema#Literal"/>
            </owl:Restriction>
        </rdfs:subClassOf>
        <rdfs:comment>Defines the details of Locality which is a named densely populated area  (a place) such as town, village, suburb, etc. A locality composes of many individual addresses.  Many localities exist in an administrative area or a sub adminisrative area. A locality can also have sub localities. For example, a municipality locality can have many villages associated with it which are sub localities. Example: Tamil Nadu State, Erode District, Bhavani Taluk, Paruvachi Village is a valid address in India. Tamil Nadu is the Administrative Area, Erode is the sub admin area, Bhavani is the locality, and Paruvachi is the sub locality</rdfs:comment>
        <rdfs:isDefinedBy rdf:resource="http://www.oasis-open.org/ciq_xal"/>
        <rdfs:label>Locality</rdfs:label>
    </owl:Class>
    


    <!-- http://www.oasis-open.org/ciq_xal#PostOffice -->

    <owl:Class rdf:about="http://www.oasis-open.org/ciq_xal#PostOffice">
        <rdfs:subClassOf>
            <owl:Restriction>
                <owl:onProperty rdf:resource="http://www.oasis-open.org/ciq_xal#identifierExtension"/>
                <owl:someValuesFrom rdf:resource="http://www.w3.org/2000/01/rdf-schema#Literal"/>
            </owl:Restriction>
        </rdfs:subClassOf>
        <rdfs:subClassOf>
            <owl:Restriction>
                <owl:onProperty rdf:resource="http://www.oasis-open.org/ciq_xal#identifierPrefix"/>
                <owl:someValuesFrom rdf:resource="http://www.w3.org/2000/01/rdf-schema#Literal"/>
            </owl:Restriction>
        </rdfs:subClassOf>
        <rdfs:subClassOf>
            <owl:Restriction>
                <owl:onProperty rdf:resource="http://www.oasis-open.org/ciq_xal#identifierRangeFrom"/>
                <owl:someValuesFrom rdf:resource="http://www.w3.org/2000/01/rdf-schema#Literal"/>
            </owl:Restriction>
        </rdfs:subClassOf>
        <rdfs:subClassOf>
            <owl:Restriction>
                <owl:onProperty rdf:resource="http://www.oasis-open.org/ciq_xal#identifierRangeTo"/>
                <owl:someValuesFrom rdf:resource="http://www.w3.org/2000/01/rdf-schema#Literal"/>
            </owl:Restriction>
        </rdfs:subClassOf>
        <rdfs:subClassOf>
            <owl:Restriction>
                <owl:onProperty rdf:resource="http://www.oasis-open.org/ciq_xal#identifierSeparator"/>
                <owl:someValuesFrom rdf:resource="http://www.w3.org/2000/01/rdf-schema#Literal"/>
            </owl:Restriction>
        </rdfs:subClassOf>
        <rdfs:subClassOf>
            <owl:Restriction>
                <owl:onProperty rdf:resource="http://www.oasis-open.org/ciq_xal#identifierSuffix"/>
                <owl:someValuesFrom rdf:resource="http://www.w3.org/2000/01/rdf-schema#Literal"/>
            </owl:Restriction>
        </rdfs:subClassOf>
        <rdfs:subClassOf>
            <owl:Restriction>
                <owl:onProperty rdf:resource="http://www.oasis-open.org/ciq_xal#postOfficeName"/>
                <owl:someValuesFrom rdf:resource="http://www.w3.org/2000/01/rdf-schema#Literal"/>
            </owl:Restriction>
        </rdfs:subClassOf>
        <rdfs:subClassOf>
            <owl:Restriction>
                <owl:onProperty rdf:resource="http://www.oasis-open.org/ciq_xal#postOfficeType"/>
                <owl:someValuesFrom rdf:resource="http://www.w3.org/2000/01/rdf-schema#Literal"/>
            </owl:Restriction>
        </rdfs:subClassOf>
        <rdfs:comment>Defines a delivery point/installation where all mails are delivered and the post man/delivery service picks up the mails and delivers it to the recipients through a delivery mode. Examples are a rural post office where post is delivered, a post office containing post office boxes/personal mail boxes. Note that not all countries have PostOffice. Can be used to represent overseas military addresses also along with PostalDeliveryPoint element</rdfs:comment>
        <rdfs:isDefinedBy rdf:resource="http://www.oasis-open.org/ciq_xal"/>
        <rdfs:label>Post Office</rdfs:label>
    </owl:Class>
    


    <!-- http://www.oasis-open.org/ciq_xal#PostalDeliveryPoint -->

    <owl:Class rdf:about="http://www.oasis-open.org/ciq_xal#PostalDeliveryPoint">
        <rdfs:subClassOf>
            <owl:Restriction>
                <owl:onProperty rdf:resource="http://www.oasis-open.org/ciq_xal#identifierExtension"/>
                <owl:someValuesFrom rdf:resource="http://www.w3.org/2000/01/rdf-schema#Literal"/>
            </owl:Restriction>
        </rdfs:subClassOf>
        <rdfs:subClassOf>
            <owl:Restriction>
                <owl:onProperty rdf:resource="http://www.oasis-open.org/ciq_xal#identifierPrefix"/>
                <owl:someValuesFrom rdf:resource="http://www.w3.org/2000/01/rdf-schema#Literal"/>
            </owl:Restriction>
        </rdfs:subClassOf>
        <rdfs:subClassOf>
            <owl:Restriction>
                <owl:onProperty rdf:resource="http://www.oasis-open.org/ciq_xal#identifierRangeFrom"/>
                <owl:someValuesFrom rdf:resource="http://www.w3.org/2000/01/rdf-schema#Literal"/>
            </owl:Restriction>
        </rdfs:subClassOf>
        <rdfs:subClassOf>
            <owl:Restriction>
                <owl:onProperty rdf:resource="http://www.oasis-open.org/ciq_xal#identifierRangeTo"/>
                <owl:someValuesFrom rdf:resource="http://www.w3.org/2000/01/rdf-schema#Literal"/>
            </owl:Restriction>
        </rdfs:subClassOf>
        <rdfs:subClassOf>
            <owl:Restriction>
                <owl:onProperty rdf:resource="http://www.oasis-open.org/ciq_xal#identifierSeparator"/>
                <owl:someValuesFrom rdf:resource="http://www.w3.org/2000/01/rdf-schema#Literal"/>
            </owl:Restriction>
        </rdfs:subClassOf>
        <rdfs:subClassOf>
            <owl:Restriction>
                <owl:onProperty rdf:resource="http://www.oasis-open.org/ciq_xal#identifierSuffix"/>
                <owl:someValuesFrom rdf:resource="http://www.w3.org/2000/01/rdf-schema#Literal"/>
            </owl:Restriction>
        </rdfs:subClassOf>
        <rdfs:subClassOf>
            <owl:Restriction>
                <owl:onProperty rdf:resource="http://www.oasis-open.org/ciq_xal#postalDeliveryPointName"/>
                <owl:someValuesFrom rdf:resource="http://www.w3.org/2000/01/rdf-schema#Literal"/>
            </owl:Restriction>
        </rdfs:subClassOf>
        <rdfs:subClassOf>
            <owl:Restriction>
                <owl:onProperty rdf:resource="http://www.oasis-open.org/ciq_xal#postalDeliveryPointType"/>
                <owl:someValuesFrom rdf:resource="http://www.w3.org/2000/01/rdf-schema#Literal"/>
            </owl:Restriction>
        </rdfs:subClassOf>
        <rdfs:comment>Defines a final mail delivery point where the mail is dropped off for recipients to pick them up directly. E.g. POBox, Private Bag,  pigeon hole, free mail numbers, etc.</rdfs:comment>
        <rdfs:isDefinedBy rdf:resource="http://www.oasis-open.org/ciq_xal"/>
        <rdfs:label>Postal Delivery Point</rdfs:label>
    </owl:Class>
    


    <!-- http://www.oasis-open.org/ciq_xal#Postcode -->

    <owl:Class rdf:about="http://www.oasis-open.org/ciq_xal#Postcode">
        <rdfs:subClassOf>
            <owl:Restriction>
                <owl:onProperty rdf:resource="http://www.oasis-open.org/ciq_xal#identifierExtension"/>
                <owl:someValuesFrom rdf:resource="http://www.w3.org/2000/01/rdf-schema#Literal"/>
            </owl:Restriction>
        </rdfs:subClassOf>
        <rdfs:subClassOf>
            <owl:Restriction>
                <owl:onProperty rdf:resource="http://www.oasis-open.org/ciq_xal#identifierPrefix"/>
                <owl:someValuesFrom rdf:resource="http://www.w3.org/2000/01/rdf-schema#Literal"/>
            </owl:Restriction>
        </rdfs:subClassOf>
        <rdfs:subClassOf>
            <owl:Restriction>
                <owl:onProperty rdf:resource="http://www.oasis-open.org/ciq_xal#identifierSeparator"/>
                <owl:someValuesFrom rdf:resource="http://www.w3.org/2000/01/rdf-schema#Literal"/>
            </owl:Restriction>
        </rdfs:subClassOf>
        <rdfs:subClassOf>
            <owl:Restriction>
                <owl:onProperty rdf:resource="http://www.oasis-open.org/ciq_xal#identifierSuffix"/>
                <owl:someValuesFrom rdf:resource="http://www.w3.org/2000/01/rdf-schema#Literal"/>
            </owl:Restriction>
        </rdfs:subClassOf>
        <rdfs:subClassOf>
            <owl:Restriction>
                <owl:onProperty rdf:resource="http://www.oasis-open.org/ciq_xal#postcodeIdentifier"/>
                <owl:someValuesFrom rdf:resource="http://www.w3.org/2000/01/rdf-schema#Literal"/>
            </owl:Restriction>
        </rdfs:subClassOf>
        <rdfs:comment>Define a container for a single free text or structured postcode. Note that not all countries have post codes</rdfs:comment>
        <rdfs:isDefinedBy rdf:resource="http://www.oasis-open.org/ciq_xal"/>
        <rdfs:label>Postcode</rdfs:label>
    </owl:Class>
    


    <!-- http://www.oasis-open.org/ciq_xal#Premises -->

    <owl:Class rdf:about="http://www.oasis-open.org/ciq_xal#Premises">
        <rdfs:subClassOf>
            <owl:Restriction>
                <owl:onProperty rdf:resource="http://www.oasis-open.org/ciq_xal#identifierExtension"/>
                <owl:someValuesFrom rdf:resource="http://www.w3.org/2000/01/rdf-schema#Literal"/>
            </owl:Restriction>
        </rdfs:subClassOf>
        <rdfs:subClassOf>
            <owl:Restriction>
                <owl:onProperty rdf:resource="http://www.oasis-open.org/ciq_xal#identifierNumber"/>
                <owl:someValuesFrom rdf:resource="http://www.w3.org/2000/01/rdf-schema#Literal"/>
            </owl:Restriction>
        </rdfs:subClassOf>
        <rdfs:subClassOf>
            <owl:Restriction>
                <owl:onProperty rdf:resource="http://www.oasis-open.org/ciq_xal#identifierPrefix"/>
                <owl:someValuesFrom rdf:resource="http://www.w3.org/2000/01/rdf-schema#Literal"/>
            </owl:Restriction>
        </rdfs:subClassOf>
        <rdfs:subClassOf>
            <owl:Restriction>
                <owl:onProperty rdf:resource="http://www.oasis-open.org/ciq_xal#identifierRangeFrom"/>
                <owl:someValuesFrom rdf:resource="http://www.w3.org/2000/01/rdf-schema#Literal"/>
            </owl:Restriction>
        </rdfs:subClassOf>
        <rdfs:subClassOf>
            <owl:Restriction>
                <owl:onProperty rdf:resource="http://www.oasis-open.org/ciq_xal#identifierRangeTo"/>
                <owl:someValuesFrom rdf:resource="http://www.w3.org/2000/01/rdf-schema#Literal"/>
            </owl:Restriction>
        </rdfs:subClassOf>
        <rdfs:subClassOf>
            <owl:Restriction>
                <owl:onProperty rdf:resource="http://www.oasis-open.org/ciq_xal#identifierSeparator"/>
                <owl:someValuesFrom rdf:resource="http://www.w3.org/2000/01/rdf-schema#Literal"/>
            </owl:Restriction>
        </rdfs:subClassOf>
        <rdfs:subClassOf>
            <owl:Restriction>
                <owl:onProperty rdf:resource="http://www.oasis-open.org/ciq_xal#identifierSuffix"/>
                <owl:someValuesFrom rdf:resource="http://www.w3.org/2000/01/rdf-schema#Literal"/>
            </owl:Restriction>
        </rdfs:subClassOf>
        <rdfs:subClassOf>
            <owl:Restriction>
                <owl:onProperty rdf:resource="http://www.oasis-open.org/ciq_xal#internalThoroughfare"/>
                <owl:someValuesFrom rdf:resource="http://www.w3.org/2000/01/rdf-schema#Literal"/>
            </owl:Restriction>
        </rdfs:subClassOf>
        <rdfs:subClassOf>
            <owl:Restriction>
                <owl:onProperty rdf:resource="http://www.oasis-open.org/ciq_xal#premisesLocation"/>
                <owl:someValuesFrom rdf:resource="http://www.w3.org/2000/01/rdf-schema#Literal"/>
            </owl:Restriction>
        </rdfs:subClassOf>
        <rdfs:subClassOf>
            <owl:Restriction>
                <owl:onProperty rdf:resource="http://www.oasis-open.org/ciq_xal#premisesName"/>
                <owl:someValuesFrom rdf:resource="http://www.w3.org/2000/01/rdf-schema#Literal"/>
            </owl:Restriction>
        </rdfs:subClassOf>
        <rdfs:subClassOf>
            <owl:Restriction>
                <owl:onProperty rdf:resource="http://www.oasis-open.org/ciq_xal#premisesNumber"/>
                <owl:someValuesFrom rdf:resource="http://www.w3.org/2000/01/rdf-schema#Literal"/>
            </owl:Restriction>
        </rdfs:subClassOf>
        <rdfs:subClassOf>
            <owl:Restriction>
                <owl:onProperty rdf:resource="http://www.oasis-open.org/ciq_xal#premisesType"/>
                <owl:someValuesFrom rdf:resource="http://www.w3.org/2000/01/rdf-schema#Literal"/>
            </owl:Restriction>
        </rdfs:subClassOf>
        <rdfs:subClassOf>
            <owl:Restriction>
                <owl:onProperty rdf:resource="http://www.oasis-open.org/ciq_xal#premisesTypeCode"/>
                <owl:someValuesFrom rdf:resource="http://www.w3.org/2000/01/rdf-schema#Literal"/>
            </owl:Restriction>
        </rdfs:subClassOf>
        <rdfs:subClassOf>
            <owl:Restriction>
                <owl:onProperty rdf:resource="http://www.oasis-open.org/ciq_xal#referenceLocation"/>
                <owl:someValuesFrom rdf:resource="http://www.w3.org/2000/01/rdf-schema#Literal"/>
            </owl:Restriction>
        </rdfs:subClassOf>
        <rdfs:subClassOf>
            <owl:Restriction>
                <owl:onProperty rdf:resource="http://www.oasis-open.org/ciq_xal#subPremisesConnector"/>
                <owl:someValuesFrom rdf:resource="http://www.w3.org/2000/01/rdf-schema#Literal"/>
            </owl:Restriction>
        </rdfs:subClassOf>
        <rdfs:comment>Defines the details of the Premises (could be building(s), site, loaction, property, premise, place) which is a landmark place which has a main address such as large mail user (e.g. Airport, Hospital, University) or could be a building (e.g. apartment, house)  or a building or complex of buildings (e.g. an apartment complex or shopping centre) or even a vacant land (e.g. LOT). A premises can have many sub-addresses such as apartments in a building having its own addresses or buildings within an airport having its own addresses including its own thoroughfares</rdfs:comment>
        <rdfs:isDefinedBy rdf:resource="http://www.oasis-open.org/ciq_xal"/>
        <rdfs:label>Premises</rdfs:label>
    </owl:Class>
    


    <!-- http://www.oasis-open.org/ciq_xal#RuralDelivery -->

    <owl:Class rdf:about="http://www.oasis-open.org/ciq_xal#RuralDelivery">
        <rdfs:subClassOf>
            <owl:Restriction>
                <owl:onProperty rdf:resource="http://www.oasis-open.org/ciq_xal#identifierExtension"/>
                <owl:someValuesFrom rdf:resource="http://www.w3.org/2000/01/rdf-schema#Literal"/>
            </owl:Restriction>
        </rdfs:subClassOf>
        <rdfs:subClassOf>
            <owl:Restriction>
                <owl:onProperty rdf:resource="http://www.oasis-open.org/ciq_xal#identifierPrefix"/>
                <owl:someValuesFrom rdf:resource="http://www.w3.org/2000/01/rdf-schema#Literal"/>
            </owl:Restriction>
        </rdfs:subClassOf>
        <rdfs:subClassOf>
            <owl:Restriction>
                <owl:onProperty rdf:resource="http://www.oasis-open.org/ciq_xal#identifierRangeFrom"/>
                <owl:someValuesFrom rdf:resource="http://www.w3.org/2000/01/rdf-schema#Literal"/>
            </owl:Restriction>
        </rdfs:subClassOf>
        <rdfs:subClassOf>
            <owl:Restriction>
                <owl:onProperty rdf:resource="http://www.oasis-open.org/ciq_xal#identifierRangeTo"/>
                <owl:someValuesFrom rdf:resource="http://www.w3.org/2000/01/rdf-schema#Literal"/>
            </owl:Restriction>
        </rdfs:subClassOf>
        <rdfs:subClassOf>
            <owl:Restriction>
                <owl:onProperty rdf:resource="http://www.oasis-open.org/ciq_xal#identifierSeparator"/>
                <owl:someValuesFrom rdf:resource="http://www.w3.org/2000/01/rdf-schema#Literal"/>
            </owl:Restriction>
        </rdfs:subClassOf>
        <rdfs:subClassOf>
            <owl:Restriction>
                <owl:onProperty rdf:resource="http://www.oasis-open.org/ciq_xal#identifierSuffix"/>
                <owl:someValuesFrom rdf:resource="http://www.w3.org/2000/01/rdf-schema#Literal"/>
            </owl:Restriction>
        </rdfs:subClassOf>
        <rdfs:subClassOf>
            <owl:Restriction>
                <owl:onProperty rdf:resource="http://www.oasis-open.org/ciq_xal#ruralDeliveryName"/>
                <owl:someValuesFrom rdf:resource="http://www.w3.org/2000/01/rdf-schema#Literal"/>
            </owl:Restriction>
        </rdfs:subClassOf>
        <rdfs:subClassOf>
            <owl:Restriction>
                <owl:onProperty rdf:resource="http://www.oasis-open.org/ciq_xal#ruralDeliveryType"/>
                <owl:someValuesFrom rdf:resource="http://www.w3.org/2000/01/rdf-schema#Literal"/>
            </owl:Restriction>
        </rdfs:subClassOf>
        <rdfs:comment>Defines a container for postal-specific delivery identifier for remote communities. Note that not all countries have RuralDelivery</rdfs:comment>
        <rdfs:isDefinedBy rdf:resource="http://www.oasis-open.org/ciq_xal"/>
        <rdfs:label>Rural Delivery</rdfs:label>
    </owl:Class>
    


    <!-- http://www.oasis-open.org/ciq_xal#SubPremises -->

    <owl:Class rdf:about="http://www.oasis-open.org/ciq_xal#SubPremises">
        <rdfs:subClassOf>
            <owl:Restriction>
                <owl:onProperty rdf:resource="http://www.oasis-open.org/ciq_xal#identifierExtension"/>
                <owl:someValuesFrom rdf:resource="http://www.w3.org/2000/01/rdf-schema#Literal"/>
            </owl:Restriction>
        </rdfs:subClassOf>
        <rdfs:subClassOf>
            <owl:Restriction>
                <owl:onProperty rdf:resource="http://www.oasis-open.org/ciq_xal#identifierNumber"/>
                <owl:someValuesFrom rdf:resource="http://www.w3.org/2000/01/rdf-schema#Literal"/>
            </owl:Restriction>
        </rdfs:subClassOf>
        <rdfs:subClassOf>
            <owl:Restriction>
                <owl:onProperty rdf:resource="http://www.oasis-open.org/ciq_xal#identifierPrefix"/>
                <owl:someValuesFrom rdf:resource="http://www.w3.org/2000/01/rdf-schema#Literal"/>
            </owl:Restriction>
        </rdfs:subClassOf>
        <rdfs:subClassOf>
            <owl:Restriction>
                <owl:onProperty rdf:resource="http://www.oasis-open.org/ciq_xal#identifierRangeFrom"/>
                <owl:someValuesFrom rdf:resource="http://www.w3.org/2000/01/rdf-schema#Literal"/>
            </owl:Restriction>
        </rdfs:subClassOf>
        <rdfs:subClassOf>
            <owl:Restriction>
                <owl:onProperty rdf:resource="http://www.oasis-open.org/ciq_xal#identifierRangeTo"/>
                <owl:someValuesFrom rdf:resource="http://www.w3.org/2000/01/rdf-schema#Literal"/>
            </owl:Restriction>
        </rdfs:subClassOf>
        <rdfs:subClassOf>
            <owl:Restriction>
                <owl:onProperty rdf:resource="http://www.oasis-open.org/ciq_xal#identifierSeparator"/>
                <owl:someValuesFrom rdf:resource="http://www.w3.org/2000/01/rdf-schema#Literal"/>
            </owl:Restriction>
        </rdfs:subClassOf>
        <rdfs:subClassOf>
            <owl:Restriction>
                <owl:onProperty rdf:resource="http://www.oasis-open.org/ciq_xal#identifierSuffix"/>
                <owl:someValuesFrom rdf:resource="http://www.w3.org/2000/01/rdf-schema#Literal"/>
            </owl:Restriction>
        </rdfs:subClassOf>
        <rdfs:subClassOf>
            <owl:Restriction>
                <owl:onProperty rdf:resource="http://www.oasis-open.org/ciq_xal#internalThoroughfare"/>
                <owl:someValuesFrom rdf:resource="http://www.w3.org/2000/01/rdf-schema#Literal"/>
            </owl:Restriction>
        </rdfs:subClassOf>
        <rdfs:subClassOf>
            <owl:Restriction>
                <owl:onProperty rdf:resource="http://www.oasis-open.org/ciq_xal#premisesLocation"/>
                <owl:someValuesFrom rdf:resource="http://www.w3.org/2000/01/rdf-schema#Literal"/>
            </owl:Restriction>
        </rdfs:subClassOf>
        <rdfs:subClassOf>
            <owl:Restriction>
                <owl:onProperty rdf:resource="http://www.oasis-open.org/ciq_xal#premisesName"/>
                <owl:someValuesFrom rdf:resource="http://www.w3.org/2000/01/rdf-schema#Literal"/>
            </owl:Restriction>
        </rdfs:subClassOf>
        <rdfs:subClassOf>
            <owl:Restriction>
                <owl:onProperty rdf:resource="http://www.oasis-open.org/ciq_xal#premisesNumber"/>
                <owl:someValuesFrom rdf:resource="http://www.w3.org/2000/01/rdf-schema#Literal"/>
            </owl:Restriction>
        </rdfs:subClassOf>
        <rdfs:subClassOf>
            <owl:Restriction>
                <owl:onProperty rdf:resource="http://www.oasis-open.org/ciq_xal#referenceLocation"/>
                <owl:someValuesFrom rdf:resource="http://www.w3.org/2000/01/rdf-schema#Literal"/>
            </owl:Restriction>
        </rdfs:subClassOf>
        <rdfs:subClassOf>
            <owl:Restriction>
                <owl:onProperty rdf:resource="http://www.oasis-open.org/ciq_xal#subPremisesConnector"/>
                <owl:someValuesFrom rdf:resource="http://www.w3.org/2000/01/rdf-schema#Literal"/>
            </owl:Restriction>
        </rdfs:subClassOf>
        <rdfs:subClassOf>
            <owl:Restriction>
                <owl:onProperty rdf:resource="http://www.oasis-open.org/ciq_xal#subPremisesName"/>
                <owl:someValuesFrom rdf:resource="http://www.w3.org/2000/01/rdf-schema#Literal"/>
            </owl:Restriction>
        </rdfs:subClassOf>
        <rdfs:subClassOf>
            <owl:Restriction>
                <owl:onProperty rdf:resource="http://www.oasis-open.org/ciq_xal#subPremisesType"/>
                <owl:someValuesFrom rdf:resource="http://www.w3.org/2000/01/rdf-schema#Literal"/>
            </owl:Restriction>
        </rdfs:subClassOf>
        <rdfs:subClassOf>
            <owl:Restriction>
                <owl:onProperty rdf:resource="http://www.oasis-open.org/ciq_xal#subPremisesTypeCode"/>
                <owl:someValuesFrom rdf:resource="http://www.w3.org/2000/01/rdf-schema#Literal"/>
            </owl:Restriction>
        </rdfs:subClassOf>
        <rdfs:comment>Defines sub-premises, such as apartments and suites, within buildings, shops in malls, etc.  or sub-addresses in a land mark place such as airports, military bases, hospitals, etc.  Some countries have blocks within blocks</rdfs:comment>
        <rdfs:isDefinedBy rdf:resource="http://www.oasis-open.org/ciq_xal"/>
        <rdfs:label>Sub-Premises</rdfs:label>
    </owl:Class>
    


    <!-- http://www.oasis-open.org/ciq_xal#SubThoroughfare -->

    <owl:Class rdf:about="http://www.oasis-open.org/ciq_xal#SubThoroughfare">
        <rdfs:subClassOf>
            <owl:Restriction>
                <owl:onProperty rdf:resource="http://www.oasis-open.org/ciq_xal#identifierExtension"/>
                <owl:someValuesFrom rdf:resource="http://www.w3.org/2000/01/rdf-schema#Literal"/>
            </owl:Restriction>
        </rdfs:subClassOf>
        <rdfs:subClassOf>
            <owl:Restriction>
                <owl:onProperty rdf:resource="http://www.oasis-open.org/ciq_xal#identifierPrefix"/>
                <owl:someValuesFrom rdf:resource="http://www.w3.org/2000/01/rdf-schema#Literal"/>
            </owl:Restriction>
        </rdfs:subClassOf>
        <rdfs:subClassOf>
            <owl:Restriction>
                <owl:onProperty rdf:resource="http://www.oasis-open.org/ciq_xal#identifierRangeFrom"/>
                <owl:someValuesFrom rdf:resource="http://www.w3.org/2000/01/rdf-schema#Literal"/>
            </owl:Restriction>
        </rdfs:subClassOf>
        <rdfs:subClassOf>
            <owl:Restriction>
                <owl:onProperty rdf:resource="http://www.oasis-open.org/ciq_xal#identifierRangeTo"/>
                <owl:someValuesFrom rdf:resource="http://www.w3.org/2000/01/rdf-schema#Literal"/>
            </owl:Restriction>
        </rdfs:subClassOf>
        <rdfs:subClassOf>
            <owl:Restriction>
                <owl:onProperty rdf:resource="http://www.oasis-open.org/ciq_xal#identifierSeparator"/>
                <owl:someValuesFrom rdf:resource="http://www.w3.org/2000/01/rdf-schema#Literal"/>
            </owl:Restriction>
        </rdfs:subClassOf>
        <rdfs:subClassOf>
            <owl:Restriction>
                <owl:onProperty rdf:resource="http://www.oasis-open.org/ciq_xal#identifierSuffix"/>
                <owl:someValuesFrom rdf:resource="http://www.w3.org/2000/01/rdf-schema#Literal"/>
            </owl:Restriction>
        </rdfs:subClassOf>
        <rdfs:subClassOf>
            <owl:Restriction>
                <owl:onProperty rdf:resource="http://www.oasis-open.org/ciq_xal#referenceLocation"/>
                <owl:someValuesFrom rdf:resource="http://www.w3.org/2000/01/rdf-schema#Literal"/>
            </owl:Restriction>
        </rdfs:subClassOf>
        <rdfs:subClassOf>
            <owl:Restriction>
                <owl:onProperty rdf:resource="http://www.oasis-open.org/ciq_xal#thoroughfareName"/>
                <owl:someValuesFrom rdf:resource="http://www.w3.org/2000/01/rdf-schema#Literal"/>
            </owl:Restriction>
        </rdfs:subClassOf>
        <rdfs:subClassOf>
            <owl:Restriction>
                <owl:onProperty rdf:resource="http://www.oasis-open.org/ciq_xal#thoroughfareNumber"/>
                <owl:someValuesFrom rdf:resource="http://www.w3.org/2000/01/rdf-schema#Literal"/>
            </owl:Restriction>
        </rdfs:subClassOf>
        <rdfs:subClassOf>
            <owl:Restriction>
                <owl:onProperty rdf:resource="http://www.oasis-open.org/ciq_xal#thoroughfareType"/>
                <owl:someValuesFrom rdf:resource="http://www.w3.org/2000/01/rdf-schema#Literal"/>
            </owl:Restriction>
        </rdfs:subClassOf>
        <rdfs:subClassOf>
            <owl:Restriction>
                <owl:onProperty rdf:resource="http://www.oasis-open.org/ciq_xal#thoroughfareTypeCode"/>
                <owl:someValuesFrom rdf:resource="http://www.w3.org/2000/01/rdf-schema#Literal"/>
            </owl:Restriction>
        </rdfs:subClassOf>
        <rdfs:comment>Characterizes another thoroughfare that is required to uniquely identify the location, such as an access route, intersection, corner, adjacent, boundary, etc</rdfs:comment>
        <rdfs:isDefinedBy rdf:resource="http://www.oasis-open.org/ciq_xal"/>
        <rdfs:label>Sub thoroughfare</rdfs:label>
    </owl:Class>
    


    <!-- http://www.oasis-open.org/ciq_xal#Thoroughfare -->

    <owl:Class rdf:about="http://www.oasis-open.org/ciq_xal#Thoroughfare">
        <rdfs:subClassOf>
            <owl:Restriction>
                <owl:onProperty rdf:resource="http://www.oasis-open.org/ciq_xal#subThoroughfare"/>
                <owl:someValuesFrom rdf:resource="http://www.w3.org/2002/07/owl#Thing"/>
            </owl:Restriction>
        </rdfs:subClassOf>
        <rdfs:subClassOf>
            <owl:Restriction>
                <owl:onProperty rdf:resource="http://www.oasis-open.org/ciq_xal#identifierExtension"/>
                <owl:someValuesFrom rdf:resource="http://www.w3.org/2000/01/rdf-schema#Literal"/>
            </owl:Restriction>
        </rdfs:subClassOf>
        <rdfs:subClassOf>
            <owl:Restriction>
                <owl:onProperty rdf:resource="http://www.oasis-open.org/ciq_xal#identifierPrefix"/>
                <owl:someValuesFrom rdf:resource="http://www.w3.org/2000/01/rdf-schema#Literal"/>
            </owl:Restriction>
        </rdfs:subClassOf>
        <rdfs:subClassOf>
            <owl:Restriction>
                <owl:onProperty rdf:resource="http://www.oasis-open.org/ciq_xal#identifierRangeFrom"/>
                <owl:someValuesFrom rdf:resource="http://www.w3.org/2000/01/rdf-schema#Literal"/>
            </owl:Restriction>
        </rdfs:subClassOf>
        <rdfs:subClassOf>
            <owl:Restriction>
                <owl:onProperty rdf:resource="http://www.oasis-open.org/ciq_xal#identifierRangeTo"/>
                <owl:someValuesFrom rdf:resource="http://www.w3.org/2000/01/rdf-schema#Literal"/>
            </owl:Restriction>
        </rdfs:subClassOf>
        <rdfs:subClassOf>
            <owl:Restriction>
                <owl:onProperty rdf:resource="http://www.oasis-open.org/ciq_xal#identifierSeparator"/>
                <owl:someValuesFrom rdf:resource="http://www.w3.org/2000/01/rdf-schema#Literal"/>
            </owl:Restriction>
        </rdfs:subClassOf>
        <rdfs:subClassOf>
            <owl:Restriction>
                <owl:onProperty rdf:resource="http://www.oasis-open.org/ciq_xal#postdirection"/>
                <owl:someValuesFrom rdf:resource="http://www.w3.org/2000/01/rdf-schema#Literal"/>
            </owl:Restriction>
        </rdfs:subClassOf>
        <rdfs:subClassOf>
            <owl:Restriction>
                <owl:onProperty rdf:resource="http://www.oasis-open.org/ciq_xal#predirection"/>
                <owl:someValuesFrom rdf:resource="http://www.w3.org/2000/01/rdf-schema#Literal"/>
            </owl:Restriction>
        </rdfs:subClassOf>
        <rdfs:subClassOf>
            <owl:Restriction>
                <owl:onProperty rdf:resource="http://www.oasis-open.org/ciq_xal#thoroughfareConnector"/>
                <owl:someValuesFrom rdf:resource="http://www.w3.org/2000/01/rdf-schema#Literal"/>
            </owl:Restriction>
        </rdfs:subClassOf>
        <rdfs:subClassOf>
            <owl:Restriction>
                <owl:onProperty rdf:resource="http://www.oasis-open.org/ciq_xal#thoroughfareName"/>
                <owl:someValuesFrom rdf:resource="http://www.w3.org/2000/01/rdf-schema#Literal"/>
            </owl:Restriction>
        </rdfs:subClassOf>
        <rdfs:subClassOf>
            <owl:Restriction>
                <owl:onProperty rdf:resource="http://www.oasis-open.org/ciq_xal#thoroughfareNumber"/>
                <owl:someValuesFrom rdf:resource="http://www.w3.org/2000/01/rdf-schema#Literal"/>
            </owl:Restriction>
        </rdfs:subClassOf>
        <rdfs:subClassOf>
            <owl:Restriction>
                <owl:onProperty rdf:resource="http://www.oasis-open.org/ciq_xal#thoroughfareType"/>
                <owl:someValuesFrom rdf:resource="http://www.w3.org/2000/01/rdf-schema#Literal"/>
            </owl:Restriction>
        </rdfs:subClassOf>
        <rdfs:subClassOf>
            <owl:Restriction>
                <owl:onProperty rdf:resource="http://www.oasis-open.org/ciq_xal#thoroughfareTypeCode"/>
                <owl:someValuesFrom rdf:resource="http://www.w3.org/2000/01/rdf-schema#Literal"/>
            </owl:Restriction>
        </rdfs:subClassOf>
        <rdfs:comment>Characterizes the details of the Access route along which buildings/lot/land are located, such as street, road, channel, crescent, avenue, etc. This also includes canals/banks on which houses/boat houses are located where people live</rdfs:comment>
        <rdfs:isDefinedBy rdf:resource="http://www.oasis-open.org/ciq_xal"/>
        <rdfs:label>Thoroughfare</rdfs:label>
    </owl:Class>
    


    <!-- 
    ///////////////////////////////////////////////////////////////////////////////////////
    //
    // Annotations
    //
    ///////////////////////////////////////////////////////////////////////////////////////
     -->

    <rdf:Description rdf:about="http://www.w3.org/2003/01/geo/wgs84_pos#">
        <dc:date>$Date: 2009/04/20 15:00:30 $</dc:date>
        <rdfs:label>geo</rdfs:label>
        <dc:description>A vocabulary for representing latitude, longitude and 
 altitude information in the WGS84 geodetic reference datum. 
 Version $Id: wgs84_pos.rdf,v 1.22 2009/04/20 15:00:30 timbl Exp $. See http://www.w3.org/2003/01/geo/ for more details.</dc:description>
        <rdfs:comment>
Recent changes to this namespace:
$Log: wgs84_pos.rdf,v $
Revision 1.22  2009/04/20 15:00:30  timbl
Remove the time bits which have been deal with elsewhere eg in iCal.

Revision 1.21  2009/04/20 12:52:47  timbl
try again

Revision 1.20  2009/04/20 12:42:11  timbl
Add Event (edited ages ago and never checked in), and location (following discussion http://chatlogs.planetrdf.com/swig/2009-04-20#T12-36-09)

Revision 1.19  2009/04/20 12:36:31  timbl
Add Event (edited ages ago and never checked in), and location (following discussion http://chatlogs.planetrdf.com/swig/2009-04-20#T12-36-09)

Revision 1.18  2006/02/01 22:01:04  danbri
Clarified that lat and long are decimal degrees, and that alt is decimal metres about local reference ellipsoid

Revision 1.17  2004/02/06 17:38:12  danbri
Fixed a bad commit screwup

Revision 1.15  2003/04/19 11:24:08  danbri
Fixed the typo even more.

Revision 1.14  2003/04/19 11:16:56  danbri
fixed a typo

Revision 1.13  2003/02/19 22:27:27  connolly
relaxed domain constraints on lat/long/alt from Point to SpatialThing

Revision 1.12  2003/01/12 01:41:41  danbri
Trying local copy of XSLT doc.

Revision 1.11  2003/01/12 01:20:18  danbri
added a link to morten&apos;s xslt rdfs viewer.

Revision 1.10  2003/01/11 18:56:49  danbri
Removed datatype range from lat and long properties, since they would
have required each occurance of the property to mention the datatype.

Revision 1.9  2003/01/11 11:41:31  danbri
Another typo; repaired rdfs:Property to rdf:Property x4

Revision 1.8  2003/01/11 11:05:02  danbri
Added an rdfs:range for each lat/long/alt property,
http://www.w3.org/2001/XMLSchema#float

Revision 1.7  2003/01/10 20:25:16  danbri
Longer rdfs:comment for Point, trying to be Earth-centric and neutral about
coordinate system(s) at the same time. Feedback welcomed.

Revision 1.6  2003/01/10 20:18:30  danbri
Added CVS log comments into the RDF/XML as an rdfs:comment property of the
vocabulary. Note that this is not common practice (but seems both harmless
and potentially useful).


revision 1.5
date: 2003/01/10 20:14:31;  author: danbri;  state: Exp;  lines: +16 -5
Updated schema:
Added a dc:date, added url for more info. Changed the rdfs:label of the
namespace from gp to geo. Added a class Point, set as the rdfs:domain of
each property. Added XML comment on the lat_long property suggesting that
we might not need it (based on #rdfig commentary from implementors).

revision 1.4
date: 2003/01/10 20:01:07;  author: danbri;  state: Exp;  lines: +6 -5
Fixed typo; several rdfs:about attributes are now rdf:about. Thanks to MortenF in
#rdfig for catching this error.

revision 1.3
date: 2003/01/10 11:59:03;  author: danbri;  state: Exp;  lines: +4 -3
fixed buglet in vocab, added more wgs links

revision 1.2
date: 2003/01/10 11:01:11;  author: danbri;  state: Exp;  lines: +4 -4
Removed alt from the as-a-flat-string property, and switched from
space separated to comma separated.

revision 1.1
date: 2003/01/10 10:53:23;  author: danbri;  state: Exp;
basic geo vocab

</rdfs:comment>
        <dc:title>WGS84 Geo Positioning: an RDF vocabulary</dc:title>
    </rdf:Description>
    <rdf:Description rdf:about="http://www.w3.org/2003/01/geo/wgs84_pos#lat_long">
        <rdfs:comment>A comma-separated representation of a latitude, longitude coordinate.</rdfs:comment>
        <rdfs:label>lat/long</rdfs:label>
    </rdf:Description>
    <rdf:Description rdf:about="http://www.w3.org/2003/01/geo/wgs84_pos#location">
        <rdfs:label>location</rdfs:label>
        <rdfs:comment>The relation between something and the point, 
 or other geometrical thing in space, where it is.  For example, the realtionship between
 a radio tower and a Point with a given lat and long.
 Or a relationship between a park and its outline as a closed arc of points, or a road and
 its location as a arc (a sequence of points).
 Clearly in practice there will be limit to the accuracy of any such statement, but one would expect
 an accuracy appropriate for the size of the object and uses such as mapping .
 </rdfs:comment>
    </rdf:Description>
</rdf:RDF>



<!-- Generated by the OWL API (version 4.2.6.20160910-2108) https://github.com/owlcs/owlapi -->

