<?xml version="1.0"?>
<rdf:RDF xmlns="http://cybox.mitre.org/objects/ARPCache#"
     xml:base="http://cybox.mitre.org/objects/ARPCache"
     xmlns:arpCacheObj="http://cybox.mitre.org/objects/ARPCache#"
     xmlns:rdf="http://www.w3.org/1999/02/22-rdf-syntax-ns#"
     xmlns:owl="http://www.w3.org/2002/07/owl#"
     xmlns:xml="http://www.w3.org/XML/1998/namespace"
     xmlns:xsd="http://www.w3.org/2001/XMLSchema#"
     xmlns:rdfs="http://www.w3.org/2000/01/rdf-schema#">
    <owl:Ontology rdf:about="http://cybox.mitre.org/objects/ARPCache">
        <owl:imports rdf:resource="http://cybox.mitre.org/objects/System"/>
        <owl:imports rdf:resource="http://cybox.mitre.org/cybox_core"/>
        <owl:imports rdf:resource="http://cybox.mitre.org/objects/Address"/>
        <rdfs:label>Cyber Observable eXpression (CybOX) ARP Cache Ontology</rdfs:label>
        <owl:versionInfo rdf:datatype="http://www.w3.org/2001/XMLSchema#string">2.1.0-000</owl:versionInfo>
        <rdfs:comment>This ontology provides a vocabulary and representation of a ARP Cache for the  Cyber Observable eXpression (CybOX).  

CybOX provides a common mechansim (structure and content) to convey the full range of potential cyber observable information and strives to be fully expressive, flexible, extensible, automatable, and as human-readable as possible.

The ontology is based on the CybOX ARP Cache object schema maintained by The MITRE Corporation copyright 2012-2014.  The version number of the ontology is kept in sync with the schema in order to more easily relate between the ontology and the corresponding schema version.

Copyright (c) 2014, DaedaFusion, LLC.  All rights reserved.</rdfs:comment>
    </owl:Ontology>
    


    <!-- 
    ///////////////////////////////////////////////////////////////////////////////////////
    //
    // Object Properties
    //
    ///////////////////////////////////////////////////////////////////////////////////////
     -->

    


    <!-- http://cybox.mitre.org/objects/ARPCache#arpCacheEntries -->

    <owl:ObjectProperty rdf:about="http://cybox.mitre.org/objects/ARPCache#arpCacheEntries">
        <rdfs:range rdf:resource="http://cybox.mitre.org/objects/ARPCache#ARPCacheEntry"/>
        <rdfs:comment>Specifies one or more  address resolution protocol (ARP) cache entries.</rdfs:comment>
        <rdfs:isDefinedBy rdf:resource="http://cybox.mitre.org/objects/ARPCache"/>
        <rdfs:label>ARP Cache Entries</rdfs:label>
    </owl:ObjectProperty>
    


    <!-- http://cybox.mitre.org/objects/ARPCache#ipAddress -->

    <owl:ObjectProperty rdf:about="http://cybox.mitre.org/objects/ARPCache#ipAddress">
        <rdfs:range>
            <owl:Class>
                <owl:unionOf rdf:parseType="Collection">
                    <rdf:Description rdf:about="http://cybox.mitre.org/objects/Address#IPv4Address"/>
                    <rdf:Description rdf:about="http://cybox.mitre.org/objects/Address#IPv6Address"/>
                </owl:unionOf>
            </owl:Class>
        </rdfs:range>
        <rdfs:comment>Specifies the IP address that is mapped to the physical address in the ARP cache entry.</rdfs:comment>
        <rdfs:isDefinedBy rdf:resource="http://cybox.mitre.org/objects/ARPCache"/>
        <rdfs:label>IP Address</rdfs:label>
    </owl:ObjectProperty>
    


    <!-- http://cybox.mitre.org/objects/ARPCache#networkInterface -->

    <owl:ObjectProperty rdf:about="http://cybox.mitre.org/objects/ARPCache#networkInterface">
        <rdfs:range rdf:resource="http://cybox.mitre.org/objects/System#NetworkInterface"/>
        <rdfs:comment>Specifies the network interface to which the ARP cache entry belongs.</rdfs:comment>
        <rdfs:isDefinedBy rdf:resource="http://cybox.mitre.org/objects/ARPCache"/>
        <rdfs:label>Network Interface</rdfs:label>
    </owl:ObjectProperty>
    


    <!-- http://cybox.mitre.org/objects/ARPCache#physicalAddress -->

    <owl:ObjectProperty rdf:about="http://cybox.mitre.org/objects/ARPCache#physicalAddress">
        <rdfs:range rdf:resource="http://cybox.mitre.org/objects/Address#MACAddress"/>
        <rdfs:comment>Specifies the physical (e.g. MAC-48) address that is mapped to the IP address in the ARP cache entry.</rdfs:comment>
        <rdfs:isDefinedBy rdf:resource="http://cybox.mitre.org/objects/ARPCache"/>
        <rdfs:label>Physical Address</rdfs:label>
    </owl:ObjectProperty>
    


    <!-- 
    ///////////////////////////////////////////////////////////////////////////////////////
    //
    // Data properties
    //
    ///////////////////////////////////////////////////////////////////////////////////////
     -->

    


    <!-- http://cybox.mitre.org/objects/ARPCache#arpCacheEntryType -->

    <owl:DatatypeProperty rdf:about="http://cybox.mitre.org/objects/ARPCache#arpCacheEntryType">
        <rdfs:range rdf:resource="http://www.w3.org/2001/XMLSchema#string"/>
        <rdfs:comment>Specifies the type of ARP cache entry, which typically refers to the way the entry was added to the cache.</rdfs:comment>
        <rdfs:isDefinedBy rdf:resource="http://cybox.mitre.org/objects/ARPCache"/>
        <rdfs:label>ARP Cache Entry Type</rdfs:label>
    </owl:DatatypeProperty>
    


    <!-- 
    ///////////////////////////////////////////////////////////////////////////////////////
    //
    // Classes
    //
    ///////////////////////////////////////////////////////////////////////////////////////
     -->

    


    <!-- http://cybox.mitre.org/objects/ARPCache#ARPCache -->

    <owl:Class rdf:about="http://cybox.mitre.org/objects/ARPCache#ARPCache">
        <rdfs:subClassOf rdf:resource="http://cybox.mitre.org/cybox_core#Object"/>
        <rdfs:comment>Characterize entries in a system&apos;s address resolution protocol (ARP) cache.</rdfs:comment>
        <rdfs:isDefinedBy rdf:resource="http://cybox.mitre.org/objects/ARPCache"/>
        <rdfs:label>ARPCache</rdfs:label>
    </owl:Class>
    


    <!-- http://cybox.mitre.org/objects/ARPCache#ARPCacheEntry -->

    <owl:Class rdf:about="http://cybox.mitre.org/objects/ARPCache#ARPCacheEntry">
        <rdfs:subClassOf>
            <owl:Restriction>
                <owl:onProperty rdf:resource="http://cybox.mitre.org/objects/ARPCache#ipAddress"/>
                <owl:someValuesFrom rdf:resource="http://www.w3.org/2002/07/owl#Thing"/>
            </owl:Restriction>
        </rdfs:subClassOf>
        <rdfs:subClassOf>
            <owl:Restriction>
                <owl:onProperty rdf:resource="http://cybox.mitre.org/objects/ARPCache#networkInterface"/>
                <owl:someValuesFrom rdf:resource="http://www.w3.org/2002/07/owl#Thing"/>
            </owl:Restriction>
        </rdfs:subClassOf>
        <rdfs:subClassOf>
            <owl:Restriction>
                <owl:onProperty rdf:resource="http://cybox.mitre.org/objects/ARPCache#physicalAddress"/>
                <owl:someValuesFrom rdf:resource="http://www.w3.org/2002/07/owl#Thing"/>
            </owl:Restriction>
        </rdfs:subClassOf>
        <rdfs:subClassOf>
            <owl:Restriction>
                <owl:onProperty rdf:resource="http://cybox.mitre.org/objects/ARPCache#arpCacheEntryType"/>
                <owl:someValuesFrom rdf:resource="http://www.w3.org/2000/01/rdf-schema#Literal"/>
            </owl:Restriction>
        </rdfs:subClassOf>
        <rdfs:comment>Characterize an ARP Cache Entry.</rdfs:comment>
        <rdfs:isDefinedBy rdf:resource="http://cybox.mitre.org/objects/ARPCache"/>
        <rdfs:label>ARPCache Entry</rdfs:label>
    </owl:Class>
    

</rdf:RDF>



<!-- Generated by the OWL API (version 4.2.6.20160910-2108) https://github.com/owlcs/owlapi -->

