<?xml version="1.0"?>
<rdf:RDF xmlns="http://cybox.mitre.org/objects/Code#"
     xml:base="http://cybox.mitre.org/objects/Code"
     xmlns:rdf="http://www.w3.org/1999/02/22-rdf-syntax-ns#"
     xmlns:owl="http://www.w3.org/2002/07/owl#"
     xmlns:xml="http://www.w3.org/XML/1998/namespace"
     xmlns:xsd="http://www.w3.org/2001/XMLSchema#"
     xmlns:codeObj="http://cybox.mitre.org/objects/Code#"
     xmlns:rdfs="http://www.w3.org/2000/01/rdf-schema#">
    <owl:Ontology rdf:about="http://cybox.mitre.org/objects/Code">
        <owl:imports rdf:resource="http://cpe.mitre.org/cpe"/>
        <owl:imports rdf:resource="http://cybox.mitre.org/cybox_core"/>
        <rdfs:comment>This ontology provides a vocabulary and representation of Code for the  Cyber Observable eXpression (CybOX).  

CybOX  provides a common mechansim (structure and content) to convey the full range of potential cyber observable information and strives to be fully expressive, flexible, extensible, automatable, and as human-readable as possible.

Copyright (c) 2014, DaedaFusion, LLC.  All rights reserved.</rdfs:comment>
        <rdfs:label>Cyber Observable eXpression (CybOX) Code Ontology</rdfs:label>
        <owl:versionInfo rdf:datatype="http://www.w3.org/2001/XMLSchema#string">1.0.0-000</owl:versionInfo>
    </owl:Ontology>
    


    <!-- 
    ///////////////////////////////////////////////////////////////////////////////////////
    //
    // Object Properties
    //
    ///////////////////////////////////////////////////////////////////////////////////////
     -->

    


    <!-- http://cybox.mitre.org/cyboxCommon#extractedFeature.codeSnippets -->

    <owl:ObjectProperty rdf:about="http://cybox.mitre.org/cyboxCommon#extractedFeature.codeSnippets">
        <rdfs:range rdf:resource="http://cybox.mitre.org/objects/Code#Code"/>
    </owl:ObjectProperty>
    


    <!-- http://cybox.mitre.org/objects/Code#targetedPlatforms -->

    <owl:ObjectProperty rdf:about="http://cybox.mitre.org/objects/Code#targetedPlatforms">
        <rdfs:range>
            <owl:Class>
                <owl:unionOf rdf:parseType="Collection">
                    <rdf:Description rdf:about="http://cpe.mitre.org/cpe#Platform"/>
                    <rdf:Description rdf:about="http://cybox.mitre.org/cyboxCommon#PlatformSpecification"/>
                </owl:unionOf>
            </owl:Class>
        </rdfs:range>
        <rdfs:comment>Specifies a list platforms that this code is targeted for.</rdfs:comment>
        <rdfs:isDefinedBy rdf:datatype="http://www.w3.org/2001/XMLSchema#string">&lt;http://cybox.mitre.org/objects/Code&gt;</rdfs:isDefinedBy>
        <rdfs:label>targeted platforms</rdfs:label>
    </owl:ObjectProperty>
    


    <!-- 
    ///////////////////////////////////////////////////////////////////////////////////////
    //
    // Data properties
    //
    ///////////////////////////////////////////////////////////////////////////////////////
     -->

    


    <!-- http://cybox.mitre.org/objects/Code#codeDescription -->

    <owl:DatatypeProperty rdf:about="http://cybox.mitre.org/objects/Code#codeDescription">
        <rdfs:range rdf:resource="http://www.w3.org/2001/XMLSchema#string"/>
        <rdfs:comment>Specifies a brief description of the code that is encapsulated in this field.</rdfs:comment>
        <rdfs:isDefinedBy rdf:datatype="http://www.w3.org/2001/XMLSchema#string">&lt;http://cybox.mitre.org/objects/Code&gt;</rdfs:isDefinedBy>
        <rdfs:label>Description</rdfs:label>
    </owl:DatatypeProperty>
    


    <!-- http://cybox.mitre.org/objects/Code#codeLanguage -->

    <owl:DatatypeProperty rdf:about="http://cybox.mitre.org/objects/Code#codeLanguage">
        <rdfs:range rdf:resource="http://www.w3.org/2001/XMLSchema#string"/>
        <rdfs:comment>Specifes the code language used in the code.</rdfs:comment>
        <rdfs:isDefinedBy rdf:resource="http://cybox.mitre.org/objects/Code"/>
        <rdfs:label>Code Language</rdfs:label>
    </owl:DatatypeProperty>
    


    <!-- http://cybox.mitre.org/objects/Code#codePurpose -->

    <owl:DatatypeProperty rdf:about="http://cybox.mitre.org/objects/Code#codePurpose">
        <rdfs:range rdf:resource="http://www.w3.org/2001/XMLSchema#string"/>
        <rdfs:comment>Specifies the purpose or flavor of code being characterized.</rdfs:comment>
        <rdfs:isDefinedBy rdf:resource="http://cybox.mitre.org/objects/Code"/>
        <rdfs:label>Code Purpose</rdfs:label>
    </owl:DatatypeProperty>
    


    <!-- http://cybox.mitre.org/objects/Code#codeSegment -->

    <owl:DatatypeProperty rdf:about="http://cybox.mitre.org/objects/Code#codeSegment">
        <rdfs:range rdf:resource="http://www.w3.org/2001/XMLSchema#string"/>
        <rdfs:comment>Specifies an  arbitrary code segment in unencoded (plaintext or binary) format. Code would typically be included here within a CDATA section.</rdfs:comment>
        <rdfs:isDefinedBy rdf:datatype="http://www.w3.org/2001/XMLSchema#string">&lt;http://cybox.mitre.org/objects/Code&gt;</rdfs:isDefinedBy>
        <rdfs:label>Code Segment</rdfs:label>
    </owl:DatatypeProperty>
    


    <!-- http://cybox.mitre.org/objects/Code#codeSegmentXOR -->

    <owl:DatatypeProperty rdf:about="http://cybox.mitre.org/objects/Code#codeSegmentXOR">
        <rdfs:range rdf:resource="http://www.w3.org/2001/XMLSchema#string"/>
        <rdfs:comment>Specifies a segment of code that has been XORed with a pattern in order to avoid tripping anti-virus detection.</rdfs:comment>
        <rdfs:isDefinedBy rdf:datatype="http://www.w3.org/2001/XMLSchema#string">&lt;http://cybox.mitre.org/objects/Code&gt;</rdfs:isDefinedBy>
        <rdfs:label>Code Segment XOR</rdfs:label>
    </owl:DatatypeProperty>
    


    <!-- http://cybox.mitre.org/objects/Code#codeSegmentXOR.xorPattern -->

    <owl:DatatypeProperty rdf:about="http://cybox.mitre.org/objects/Code#codeSegmentXOR.xorPattern">
        <rdfs:range rdf:resource="http://www.w3.org/2001/XMLSchema#hexBinary"/>
        <rdfs:comment>Specifies a segment of code that has been XORed with a pattern in order to avoid tripping anti-virus detection.</rdfs:comment>
        <rdfs:isDefinedBy rdf:datatype="http://www.w3.org/2001/XMLSchema#string">&lt;http://cybox.mitre.org/objects/Code&gt;</rdfs:isDefinedBy>
        <rdfs:label>XOR Pattern</rdfs:label>
    </owl:DatatypeProperty>
    


    <!-- http://cybox.mitre.org/objects/Code#codeType -->

    <owl:DatatypeProperty rdf:about="http://cybox.mitre.org/objects/Code#codeType">
        <rdfs:range rdf:resource="http://www.w3.org/2001/XMLSchema#string"/>
        <rdfs:comment>Specifies the type of code being characterized.</rdfs:comment>
        <rdfs:isDefinedBy rdf:resource="http://cybox.mitre.org/objects/Code"/>
        <rdfs:label>Type</rdfs:label>
    </owl:DatatypeProperty>
    


    <!-- http://cybox.mitre.org/objects/Code#processorFamily -->

    <owl:DatatypeProperty rdf:about="http://cybox.mitre.org/objects/Code#processorFamily">
        <rdfs:range rdf:resource="http://www.w3.org/2001/XMLSchema#string"/>
        <rdfs:comment>Specifies the class of processor that the code snippet is targeting.</rdfs:comment>
        <rdfs:isDefinedBy rdf:resource="http://cybox.mitre.org/objects/Code"/>
        <rdfs:label>Processor Family</rdfs:label>
    </owl:DatatypeProperty>
    


    <!-- http://cybox.mitre.org/objects/Code#startAddress -->

    <owl:DatatypeProperty rdf:about="http://cybox.mitre.org/objects/Code#startAddress">
        <rdfs:range rdf:resource="http://www.w3.org/2001/XMLSchema#hexBinary"/>
        <rdfs:comment>Specifies the start address of the code, if it was discovered inside a binary.</rdfs:comment>
        <rdfs:isDefinedBy rdf:datatype="http://www.w3.org/2001/XMLSchema#string">&lt;http://cybox.mitre.org/objects/Code&gt;</rdfs:isDefinedBy>
        <rdfs:label>Start Address</rdfs:label>
    </owl:DatatypeProperty>
    


    <!-- 
    ///////////////////////////////////////////////////////////////////////////////////////
    //
    // Classes
    //
    ///////////////////////////////////////////////////////////////////////////////////////
     -->

    


    <!-- http://cybox.mitre.org/objects/Code#Code -->

    <owl:Class rdf:about="http://cybox.mitre.org/objects/Code#Code">
        <rdfs:subClassOf rdf:resource="http://cybox.mitre.org/cybox_core#Object"/>
        <rdfs:subClassOf>
            <owl:Restriction>
                <owl:onProperty rdf:resource="http://cybox.mitre.org/objects/Code#codeDescription"/>
                <owl:someValuesFrom rdf:resource="http://www.w3.org/2000/01/rdf-schema#Literal"/>
            </owl:Restriction>
        </rdfs:subClassOf>
        <rdfs:subClassOf>
            <owl:Restriction>
                <owl:onProperty rdf:resource="http://cybox.mitre.org/objects/Code#codeLanguage"/>
                <owl:someValuesFrom rdf:resource="http://www.w3.org/2000/01/rdf-schema#Literal"/>
            </owl:Restriction>
        </rdfs:subClassOf>
        <rdfs:subClassOf>
            <owl:Restriction>
                <owl:onProperty rdf:resource="http://cybox.mitre.org/objects/Code#codePurpose"/>
                <owl:someValuesFrom rdf:resource="http://www.w3.org/2000/01/rdf-schema#Literal"/>
            </owl:Restriction>
        </rdfs:subClassOf>
        <rdfs:subClassOf>
            <owl:Restriction>
                <owl:onProperty rdf:resource="http://cybox.mitre.org/objects/Code#codeSegment"/>
                <owl:someValuesFrom rdf:resource="http://www.w3.org/2000/01/rdf-schema#Literal"/>
            </owl:Restriction>
        </rdfs:subClassOf>
        <rdfs:subClassOf>
            <owl:Restriction>
                <owl:onProperty rdf:resource="http://cybox.mitre.org/objects/Code#codeSegmentXOR"/>
                <owl:someValuesFrom rdf:resource="http://www.w3.org/2000/01/rdf-schema#Literal"/>
            </owl:Restriction>
        </rdfs:subClassOf>
        <rdfs:subClassOf>
            <owl:Restriction>
                <owl:onProperty rdf:resource="http://cybox.mitre.org/objects/Code#codeSegmentXOR.xorPattern"/>
                <owl:someValuesFrom rdf:resource="http://www.w3.org/2000/01/rdf-schema#Literal"/>
            </owl:Restriction>
        </rdfs:subClassOf>
        <rdfs:subClassOf>
            <owl:Restriction>
                <owl:onProperty rdf:resource="http://cybox.mitre.org/objects/Code#codeType"/>
                <owl:someValuesFrom rdf:resource="http://www.w3.org/2000/01/rdf-schema#Literal"/>
            </owl:Restriction>
        </rdfs:subClassOf>
        <rdfs:subClassOf>
            <owl:Restriction>
                <owl:onProperty rdf:resource="http://cybox.mitre.org/objects/Code#startAddress"/>
                <owl:someValuesFrom rdf:resource="http://www.w3.org/2000/01/rdf-schema#Literal"/>
            </owl:Restriction>
        </rdfs:subClassOf>
        <rdfs:comment>Characterize a body of computer code.</rdfs:comment>
        <rdfs:isDefinedBy rdf:resource="http://cybox.mitre.org/objects/Code"/>
        <rdfs:label>Code</rdfs:label>
    </owl:Class>
</rdf:RDF>



<!-- Generated by the OWL API (version 4.2.6.20160910-2108) https://github.com/owlcs/owlapi -->

