<?xml version="1.0"?>
<rdf:RDF xmlns="http://cybox.mitre.org/cybox_core#"
     xml:base="http://cybox.mitre.org/cybox_core"
     xmlns:rdf="http://www.w3.org/1999/02/22-rdf-syntax-ns#"
     xmlns:owl="http://www.w3.org/2002/07/owl#"
     xmlns:xml="http://www.w3.org/XML/1998/namespace"
     xmlns:xsd="http://www.w3.org/2001/XMLSchema#"
     xmlns:ciq_xnl="http://www.oasis-open.org/ciq_xnl#"
     xmlns:wgs84_pos="http://www.w3.org/2003/01/geo/wgs84_pos#"
     xmlns:rdfs="http://www.w3.org/2000/01/rdf-schema#"
     xmlns:cybox="http://cybox.mitre.org/cybox_core#"
	 xmlns:cyboxCommon="http://cybox.mitre.org/cyboxCommon#"
     xmlns:foaf="http://xmlns.com/foaf/0.1/"
     xmlns:dc="http://purl.org/dc/elements/1.1/">
    <owl:Ontology rdf:about="http://cybox.mitre.org/cybox_core">
        <owl:imports rdf:resource="http://www.oasis-open.org/ciq_xal"/>
        <owl:imports rdf:resource="http://cybox.mitre.org/cyboxCommon"/>
        <rdfs:label>Cyber Observable eXpression (CybOX) Core Types Ontology</rdfs:label>
        <rdfs:comment>This ontology provides a vocabulary and representation for the  Cyber Observable eXpression (CybOX)  core types.  

CybOX  provides a common mechansim (structure and content) to convey the full range of potential cyber observable information and strives to be fully expressive, flexible, extensible, automatable, and as human-readable as possible.

Copyright (c) 2014, DaedaFusion, LLC.  All rights reserved.</rdfs:comment>
        <owl:versionInfo rdf:datatype="http://www.w3.org/2001/XMLSchema#string">1.0.0-000</owl:versionInfo>
    </owl:Ontology>
    


    <!-- 
    ///////////////////////////////////////////////////////////////////////////////////////
    //
    // Annotation properties
    //
    ///////////////////////////////////////////////////////////////////////////////////////
     -->

    


    <!-- http://www.w3.org/2002/07/owl#cardinality -->

    <owl:AnnotationProperty rdf:about="http://www.w3.org/2002/07/owl#cardinality"/>
    


    <!-- http://www.w3.org/2002/07/owl#maxCardinality -->

    <owl:AnnotationProperty rdf:about="http://www.w3.org/2002/07/owl#maxCardinality"/>
    


    <!-- 
    ///////////////////////////////////////////////////////////////////////////////////////
    //
    // Object Properties
    //
    ///////////////////////////////////////////////////////////////////////////////////////
     -->

    


    <!-- http://cybox.mitre.org/cybox_core#actionArguments -->

    <owl:ObjectProperty rdf:about="http://cybox.mitre.org/cybox_core#actionArguments">
        <rdfs:range rdf:resource="http://cybox.mitre.org/cybox_core#ActionArgument"/>
        <rdfs:comment>Specifies relevant arguments/parameters for this Action.</rdfs:comment>
        <rdfs:isDefinedBy rdf:resource="http://cybox.mitre.org/cybox_core"/>
        <rdfs:label>Arguments</rdfs:label>
    </owl:ObjectProperty>
    


    <!-- http://cybox.mitre.org/cybox_core#actionPertinentObjectProperties -->

    <owl:ObjectProperty rdf:about="http://cybox.mitre.org/cybox_core#actionPertinentObjectProperties">
        <rdfs:range rdf:resource="http://cybox.mitre.org/cyboxCommon#Property"/>
        <rdfs:comment>Specifies which of the Properties of this Object are specifically pertinent to this Action.</rdfs:comment>
        <rdfs:isDefinedBy rdf:resource="http://cybox.mitre.org/cybox_core"/>
        <rdfs:label>Action Pertinent Object Properties</rdfs:label>
    </owl:ObjectProperty>
    


    <!-- http://cybox.mitre.org/cybox_core#actionPool -->

    <owl:ObjectProperty rdf:about="http://cybox.mitre.org/cybox_core#actionPool">
        <rdfs:range rdf:resource="http://cybox.mitre.org/cybox_core#Action"/>
        <rdfs:comment>Specifies the description of CybOX Actions in a space-efficient pooled manner with the actual Observable structures defined in the CybOX schema containing references to the pooled Action elements. This reduces redundancy caused when identical Actions occur multiple times within a set of defined Observables.</rdfs:comment>
        <rdfs:isDefinedBy rdf:resource="http://cybox.mitre.org/cybox_core"/>
        <rdfs:label>Action Pool</rdfs:label>
    </owl:ObjectProperty>
    


    <!-- http://cybox.mitre.org/cybox_core#actionReference -->

    <owl:ObjectProperty rdf:about="http://cybox.mitre.org/cybox_core#actionReference">
        <rdfs:range rdf:resource="http://cybox.mitre.org/cybox_core#Action"/>
        <rdfs:comment>Specifies the target of the association or relationship</rdfs:comment>
        <rdfs:isDefinedBy rdf:resource="http://cybox.mitre.org/cybox_core"/>
        <rdfs:label>Action Reference</rdfs:label>
    </owl:ObjectProperty>
    


    <!-- http://cybox.mitre.org/cybox_core#actions -->

    <owl:ObjectProperty rdf:about="http://cybox.mitre.org/cybox_core#actions">
        <rdfs:range rdf:resource="http://cybox.mitre.org/cybox_core#Action"/>
        <rdfs:comment>Specifies one or more cyber observable actions.</rdfs:comment>
        <rdfs:isDefinedBy rdf:resource="http://cybox.mitre.org/cybox_core"/>
        <rdfs:label>Actions</rdfs:label>
    </owl:ObjectProperty>
    


    <!-- http://cybox.mitre.org/cybox_core#associatedObject -->

    <owl:ObjectProperty rdf:about="http://cybox.mitre.org/cybox_core#associatedObject">
        <rdfs:range rdf:resource="http://cybox.mitre.org/cybox_core#Object"/>
        <rdfs:comment>Specifies a reference to the associated object</rdfs:comment>
        <rdfs:isDefinedBy rdf:resource="http://cybox.mitre.org/cybox_core"/>
        <rdfs:label>Associated Object</rdfs:label>
    </owl:ObjectProperty>
    


    <!-- http://cybox.mitre.org/cybox_core#associatedObjects -->

    <owl:ObjectProperty rdf:about="http://cybox.mitre.org/cybox_core#associatedObjects">
        <rdfs:range rdf:resource="http://cybox.mitre.org/cybox_core#Object"/>
        <rdfs:comment>Specifies cyber Objects relevant (either initiating or affected by) this Action.</rdfs:comment>
        <rdfs:isDefinedBy rdf:resource="http://cybox.mitre.org/cybox_core"/>
        <rdfs:label>Associated Objects</rdfs:label>
    </owl:ObjectProperty>
    


    <!-- http://cybox.mitre.org/cybox_core#definedEffect -->

    <owl:ObjectProperty rdf:about="http://cybox.mitre.org/cybox_core#definedEffect">
        <rdfs:range rdf:resource="http://cybox.mitre.org/cybox_core#DefinedEffect"/>
        <rdfs:comment>Specifies arious predefined Object Effect types (e.g. DataReadEffect, ValuesEnumeratedEffect or StateChangeEffect) that can be instantiated in its place through extension of the DefinedEffectType. This mechanism enables the specification of a broad range of types of potential complex action effects on Objects.</rdfs:comment>
        <rdfs:isDefinedBy rdf:resource="http://cybox.mitre.org/cybox_core"/>
        <rdfs:label>Defined Effect</rdfs:label>
    </owl:ObjectProperty>
    


    <!-- http://cybox.mitre.org/cybox_core#discoveryMethod -->

    <owl:ObjectProperty rdf:about="http://cybox.mitre.org/cybox_core#discoveryMethod">
        <rdfs:range rdf:resource="http://cybox.mitre.org/cyboxCommon#MeasureSource"/>
        <rdfs:comment>Specifies a descriptive specification of how this Object was observed (in the case of a Cyber Observable Object instance) or could potentially be observed (in the case of a Cyber Observable Object pattern).</rdfs:comment>
        <rdfs:isDefinedBy rdf:resource="http://cybox.mitre.org/cybox_core"/>
        <rdfs:label>Discovery Method</rdfs:label>
    </owl:ObjectProperty>
    


    <!-- http://cybox.mitre.org/cybox_core#event -->

    <owl:ObjectProperty rdf:about="http://cybox.mitre.org/cybox_core#event">
        <rdfs:range rdf:resource="http://cybox.mitre.org/cybox_core#Event"/>
        <rdfs:comment>Specifies another Event that is part of a composite Event</rdfs:comment>
        <rdfs:isDefinedBy rdf:resource="http://cybox.mitre.org/cybox_core"/>
        <rdfs:label>Event</rdfs:label>
    </owl:ObjectProperty>
    


    <!-- http://cybox.mitre.org/cybox_core#eventPool -->

    <owl:ObjectProperty rdf:about="http://cybox.mitre.org/cybox_core#eventPool">
        <rdfs:range rdf:resource="http://cybox.mitre.org/cybox_core#Event"/>
        <rdfs:comment>Specifies the description of CybOX Events in a space-efficient pooled manner with the actual Observable structures defined in the CybOX schema containing references to the pooled Event elements. This reduces redundancy caused when identical Events occur multiple times within a set of defined Observables.</rdfs:comment>
        <rdfs:isDefinedBy rdf:resource="http://cybox.mitre.org/cybox_core"/>
        <rdfs:label>Event Pool</rdfs:label>
    </owl:ObjectProperty>
    


    <!-- http://cybox.mitre.org/cybox_core#newObject -->

    <owl:ObjectProperty rdf:about="http://cybox.mitre.org/cybox_core#newObject">
        <rdfs:range rdf:resource="http://cybox.mitre.org/cybox_core#Object"/>
        <rdfs:comment>Specifies the object and its properties as they are after the state change effect occurred.</rdfs:comment>
        <rdfs:isDefinedBy rdf:resource="http://cybox.mitre.org/cybox_core"/>
        <rdfs:label>New Object</rdfs:label>
    </owl:ObjectProperty>
    


    <!-- http://cybox.mitre.org/cybox_core#objectPool -->

    <owl:ObjectProperty rdf:about="http://cybox.mitre.org/cybox_core#objectPool">
        <rdfs:range rdf:resource="http://cybox.mitre.org/cybox_core#Object"/>
        <rdfs:comment>Specifies the description of CybOX Objects in a space-efficient pooled manner with the actual Observable structures defined in the CybOX schema containing references to the pooled Object elements. This reduces redundancy caused when identical Objects occur multiple times within a set of defined Observables.</rdfs:comment>
        <rdfs:isDefinedBy rdf:resource="http://cybox.mitre.org/cybox_core"/>
        <rdfs:label>Object Pool</rdfs:label>
    </owl:ObjectProperty>
    


    <!-- http://cybox.mitre.org/cybox_core#observable -->

    <owl:ObjectProperty rdf:about="http://cybox.mitre.org/cybox_core#observable">
        <rdfs:range rdf:resource="http://cybox.mitre.org/cybox_core#Observable"/>
        <rdfs:comment>Specifies one or more Observable.</rdfs:comment>
        <rdfs:isDefinedBy rdf:resource="http://cybox.mitre.org/cybox_core"/>
        <rdfs:label>Observable</rdfs:label>
    </owl:ObjectProperty>
    


    <!-- http://cybox.mitre.org/cybox_core#observablePackageSource -->

    <owl:ObjectProperty rdf:about="http://cybox.mitre.org/cybox_core#observablePackageSource">
        <rdfs:range rdf:resource="http://cybox.mitre.org/cyboxCommon#MeasureSource"/>
        <rdfs:comment>Specifies a descriptive specification of how this package of Observables was identified and specified</rdfs:comment>
        <rdfs:isDefinedBy rdf:resource="http://cybox.mitre.org/cybox_core"/>
        <rdfs:label>Observable Package Source</rdfs:label>
    </owl:ObjectProperty>
    


    <!-- http://cybox.mitre.org/cybox_core#observableSource -->

    <owl:ObjectProperty rdf:about="http://cybox.mitre.org/cybox_core#observableSource">
        <rdfs:range rdf:resource="http://cybox.mitre.org/cyboxCommon#MeasureSource"/>
        <rdfs:comment>Specifies a descriptive specification of how this Observable was identified and specified.</rdfs:comment>
        <rdfs:isDefinedBy rdf:resource="http://cybox.mitre.org/cybox_core"/>
        <rdfs:label>Observable Source</rdfs:label>
    </owl:ObjectProperty>
    


    <!-- http://cybox.mitre.org/cybox_core#observationMethod -->

    <owl:ObjectProperty rdf:about="http://cybox.mitre.org/cybox_core#observationMethod">
        <rdfs:range rdf:resource="http://cybox.mitre.org/cyboxCommon#MeasureSource"/>
        <rdfs:comment>Specifies a descriptive specification of how this Event was observed (in the case of a Cyber Observable Event instance) or could potentially be observed (in the case of a Cyber Observable Event pattern).</rdfs:comment>
        <rdfs:isDefinedBy rdf:resource="http://cybox.mitre.org/cybox_core"/>
        <rdfs:label>Observation Method</rdfs:label>
    </owl:ObjectProperty>
    


    <!-- http://cybox.mitre.org/cybox_core#observedEntity -->

    <owl:ObjectProperty rdf:about="http://cybox.mitre.org/cybox_core#observedEntity">
        <rdfs:range>
            <owl:Class>
                <owl:unionOf rdf:parseType="Collection">
                    <rdf:Description rdf:about="http://cybox.mitre.org/cybox_core#Event"/>
                    <rdf:Description rdf:about="http://cybox.mitre.org/cybox_core#Object"/>
                    <rdf:Description rdf:about="http://cybox.mitre.org/cybox_core#ObservableComposition"/>
                </owl:unionOf>
            </owl:Class>
        </rdfs:range>
        <rdfs:comment>Specifies the observed entity as either an object, event, or a composition of observables</rdfs:comment>
        <rdfs:isDefinedBy rdf:resource="http://cybox.mitre.org/cybox_core"/>
        <rdfs:label>Observed Entity</rdfs:label>
    </owl:ObjectProperty>
    


    <!-- http://cybox.mitre.org/cybox_core#oldObject -->

    <owl:ObjectProperty rdf:about="http://cybox.mitre.org/cybox_core#oldObject">
        <rdfs:range rdf:resource="http://cybox.mitre.org/cybox_core#Object"/>
        <rdfs:comment>Specifies the object and its properties as they were before the state change effect occurred.</rdfs:comment>
        <rdfs:isDefinedBy rdf:resource="http://cybox.mitre.org/cybox_core"/>
        <rdfs:label>Old Object</rdfs:label>
    </owl:ObjectProperty>
    


    <!-- http://cybox.mitre.org/cybox_core#patternFidelity.evasionTechniques -->

    <owl:ObjectProperty rdf:about="http://cybox.mitre.org/cybox_core#patternFidelity.evasionTechniques">
        <rdfs:range rdf:resource="http://cybox.mitre.org/cybox_core#ObfuscationTechnique"/>
        <rdfs:comment>Specifies potential techniques an attacker could leverage to obfuscate the observability of this Observable.</rdfs:comment>
        <rdfs:isDefinedBy rdf:resource="http://cybox.mitre.org/cybox_core"/>
        <rdfs:label>Evasion Techniques</rdfs:label>
    </owl:ObjectProperty>
    


    <!-- http://cybox.mitre.org/cybox_core#physicalLocation -->

    <owl:ObjectProperty rdf:about="http://cybox.mitre.org/cybox_core#physicalLocation">
        <rdfs:range rdf:resource="http://www.oasis-open.org/ciq_xal#Address"/>
        <rdfs:comment>Specifies a relevant physical location.</rdfs:comment>
        <rdfs:isDefinedBy rdf:resource="http://cybox.mitre.org/cybox_core"/>
        <rdfs:label>Physical Location</rdfs:label>
    </owl:ObjectProperty>
    


    <!-- http://cybox.mitre.org/cybox_core#properties -->

    <owl:ObjectProperty rdf:about="http://cybox.mitre.org/cybox_core#properties">
        <rdfs:range rdf:resource="http://cybox.mitre.org/cyboxCommon#Property"/>
        <rdfs:comment>Specifies a set of custom Object properties that may not be defined for existing object definitions.</rdfs:comment>
        <rdfs:isDefinedBy rdf:resource="http://cybox.mitre.org/cybox_core"/>
        <rdfs:label>Properties</rdfs:label>
    </owl:ObjectProperty>
    


    <!-- http://cybox.mitre.org/cybox_core#propertyPool -->

    <owl:ObjectProperty rdf:about="http://cybox.mitre.org/cybox_core#propertyPool">
        <rdfs:range rdf:resource="http://cybox.mitre.org/cyboxCommon#Property"/>
        <rdfs:comment>Specifies the description of CybOX Properties in a space-efficient pooled manner with the actual Observable structures defined in the CybOX schema containing references to the pooled Properties elements. This reduces redundancy caused when identical Properties occur multiple times within a set of defined Observables.</rdfs:comment>
        <rdfs:isDefinedBy rdf:resource="http://cybox.mitre.org/cybox_core"/>
        <rdfs:label>Property Pool</rdfs:label>
    </owl:ObjectProperty>
    


    <!-- http://cybox.mitre.org/cybox_core#relatedObjects -->

    <owl:ObjectProperty rdf:about="http://cybox.mitre.org/cybox_core#relatedObjects">
        <rdfs:range rdf:resource="http://cybox.mitre.org/cybox_core#Object"/>
        <rdfs:comment>Specifiethe identification and/or specification of Objects with relevant relationships with this Object.</rdfs:comment>
        <rdfs:isDefinedBy rdf:resource="http://cybox.mitre.org/cybox_core"/>
        <rdfs:label>Related Objects</rdfs:label>
    </owl:ObjectProperty>
    


    <!-- http://cybox.mitre.org/cybox_core#relationships -->

    <owl:ObjectProperty rdf:about="http://cybox.mitre.org/cybox_core#relationships">
        <rdfs:range rdf:resource="http://cybox.mitre.org/cybox_core#Action"/>
        <rdfs:comment>Specifies other cyber observable actions that are related to this Action.</rdfs:comment>
        <rdfs:isDefinedBy rdf:resource="http://cybox.mitre.org/cybox_core"/>
        <rdfs:label>Relationships</rdfs:label>
    </owl:ObjectProperty>
    


    <!-- http://cybox.mitre.org/cybox_core#techniqueObservables -->

    <owl:ObjectProperty rdf:about="http://cybox.mitre.org/cybox_core#techniqueObservables">
        <rdfs:range rdf:resource="http://cybox.mitre.org/cybox_core#Observables"/>
        <rdfs:comment>Specifies potential cyber observables that could indicate the use of this particular obfuscation technique.</rdfs:comment>
        <rdfs:isDefinedBy rdf:resource="http://cybox.mitre.org/cybox_core"/>
        <rdfs:label>Technique Observables</rdfs:label>
    </owl:ObjectProperty>
    


    <!-- 
    ///////////////////////////////////////////////////////////////////////////////////////
    //
    // Data properties
    //
    ///////////////////////////////////////////////////////////////////////////////////////
     -->

    


    <!-- http://cybox.mitre.org/cybox_core#actionAliases -->

    <owl:DatatypeProperty rdf:about="http://cybox.mitre.org/cybox_core#actionAliases">
        <rdfs:range rdf:resource="http://www.w3.org/2001/XMLSchema#string"/>
        <rdfs:comment>Specifies other potentially used names for this Action.</rdfs:comment>
        <rdfs:isDefinedBy rdf:resource="http://cybox.mitre.org/cybox_core"/>
        <rdfs:label>Action Aliases</rdfs:label>
    </owl:DatatypeProperty>
    


    <!-- http://cybox.mitre.org/cybox_core#actionContext -->

    <owl:DatatypeProperty rdf:about="http://cybox.mitre.org/cybox_core#actionContext">
        <rdfs:range rdf:resource="http://www.w3.org/2001/XMLSchema#string"/>
        <rdfs:comment>Specifies a simple characterization of the broad operational context in which the Action is relevant.</rdfs:comment>
        <rdfs:isDefinedBy rdf:resource="http://cybox.mitre.org/cybox_core"/>
        <rdfs:label>action context</rdfs:label>
    </owl:DatatypeProperty>
    


    <!-- http://cybox.mitre.org/cybox_core#actionName -->

    <owl:DatatypeProperty rdf:about="http://cybox.mitre.org/cybox_core#actionName">
        <rdfs:range rdf:resource="http://www.w3.org/2001/XMLSchema#string"/>
        <rdfs:comment>Specifies the specific name of the action that was performed.</rdfs:comment>
        <rdfs:isDefinedBy rdf:resource="http://cybox.mitre.org/cybox_core"/>
        <rdfs:label>Name</rdfs:label>
    </owl:DatatypeProperty>
    


    <!-- http://cybox.mitre.org/cybox_core#actionRelationshipType -->

    <owl:DatatypeProperty rdf:about="http://cybox.mitre.org/cybox_core#actionRelationshipType">
        <rdfs:range rdf:resource="http://www.w3.org/2001/XMLSchema#string"/>
        <rdfs:comment>Specifies the kind of assocation thi Object holds for this Action.</rdfs:comment>
        <rdfs:isDefinedBy rdf:resource="http://cybox.mitre.org/cybox_core"/>
        <rdfs:label>Action Relationship Type</rdfs:label>
    </owl:DatatypeProperty>
    


    <!-- http://cybox.mitre.org/cybox_core#actionStatus -->

    <owl:DatatypeProperty rdf:about="http://cybox.mitre.org/cybox_core#actionStatus">
        <rdfs:range rdf:resource="http://www.w3.org/2001/XMLSchema#string"/>
        <rdfs:comment>Specifies the status of the action being described.</rdfs:comment>
        <rdfs:isDefinedBy rdf:resource="http://cybox.mitre.org/cybox_core"/>
        <rdfs:label>Status</rdfs:label>
    </owl:DatatypeProperty>
    


    <!-- http://cybox.mitre.org/cybox_core#actionType -->

    <owl:DatatypeProperty rdf:about="http://cybox.mitre.org/cybox_core#actionType">
        <rdfs:range rdf:resource="http://www.w3.org/2001/XMLSchema#string"/>
        <rdfs:comment>Specifies the type of the action that was performed.</rdfs:comment>
        <rdfs:isDefinedBy rdf:resource="http://cybox.mitre.org/cybox_core"/>
        <rdfs:label>Action Type</rdfs:label>
    </owl:DatatypeProperty>
    


    <!-- http://cybox.mitre.org/cybox_core#argumentName -->

    <owl:DatatypeProperty rdf:about="http://cybox.mitre.org/cybox_core#argumentName">
        <rdfs:range rdf:resource="http://www.w3.org/2001/XMLSchema#string"/>
        <rdfs:comment>Specifies thename of the specific action argument utilized.</rdfs:comment>
        <rdfs:isDefinedBy rdf:resource="http://cybox.mitre.org/cybox_core"/>
        <rdfs:label>Argument Name</rdfs:label>
    </owl:DatatypeProperty>
    


    <!-- http://cybox.mitre.org/cybox_core#argumentValue -->

    <owl:DatatypeProperty rdf:about="http://cybox.mitre.org/cybox_core#argumentValue">
        <rdfs:range rdf:resource="http://www.w3.org/2001/XMLSchema#string"/>
        <rdfs:comment>Specifies the value for this action argument/parameter.</rdfs:comment>
        <rdfs:isDefinedBy rdf:resource="http://cybox.mitre.org/cybox_core"/>
        <rdfs:label>Argument Value</rdfs:label>
    </owl:DatatypeProperty>
    


    <!-- http://cybox.mitre.org/cybox_core#associationType -->

    <owl:DatatypeProperty rdf:about="http://cybox.mitre.org/cybox_core#associationType">
        <rdfs:range rdf:resource="http://www.w3.org/2001/XMLSchema#string"/>
        <rdfs:comment>Specifies the kind of association this Object holds for this Action.</rdfs:comment>
        <rdfs:isDefinedBy rdf:resource="http://cybox.mitre.org/cybox_core"/>
        <rdfs:label>Association Type</rdfs:label>
    </owl:DatatypeProperty>
    


    <!-- http://cybox.mitre.org/cybox_core#controlCode -->

    <owl:DatatypeProperty rdf:about="http://cybox.mitre.org/cybox_core#controlCode">
        <rdfs:range rdf:resource="http://www.w3.org/2001/XMLSchema#string"/>
        <rdfs:comment>Specifies the actual control code that was sent to the object.</rdfs:comment>
        <rdfs:isDefinedBy rdf:resource="http://cybox.mitre.org/cybox_core"/>
        <rdfs:label>control code</rdfs:label>
    </owl:DatatypeProperty>
    


    <!-- http://cybox.mitre.org/cybox_core#description -->

    <owl:DatatypeProperty rdf:about="http://cybox.mitre.org/cybox_core#description">
        <rdfs:range rdf:resource="http://www.w3.org/2001/XMLSchema#string"/>
        <rdfs:comment>Specifies a structured text description of this entity.</rdfs:comment>
        <rdfs:isDefinedBy rdf:resource="http://cybox.mitre.org/cybox_core"/>
        <rdfs:label>Description</rdfs:label>
    </owl:DatatypeProperty>
    


    <!-- http://cybox.mitre.org/cybox_core#effectType -->

    <owl:DatatypeProperty rdf:about="http://cybox.mitre.org/cybox_core#effectType">
        <rdfs:range rdf:resource="http://www.w3.org/2001/XMLSchema#string"/>
        <rdfs:comment>Specifies the nature of the Defined Effect instantiated in the place of the Defined_Effect element.</rdfs:comment>
        <rdfs:isDefinedBy rdf:resource="http://cybox.mitre.org/cybox_core"/>
        <rdfs:label>Effect Type</rdfs:label>
    </owl:DatatypeProperty>
    


    <!-- http://cybox.mitre.org/cybox_core#eventType -->

    <owl:DatatypeProperty rdf:about="http://cybox.mitre.org/cybox_core#eventType">
        <rdfs:range rdf:resource="http://www.w3.org/2001/XMLSchema#string"/>
        <rdfs:comment>Specifies the  type of Event.</rdfs:comment>
        <rdfs:isDefinedBy rdf:resource="http://cybox.mitre.org/cybox_core"/>
        <rdfs:label>Event Type</rdfs:label>
    </owl:DatatypeProperty>
    


    <!-- http://cybox.mitre.org/cybox_core#frequence.trend -->

    <owl:DatatypeProperty rdf:about="http://cybox.mitre.org/cybox_core#frequence.trend">
        <rdfs:range rdf:resource="http://www.w3.org/2001/XMLSchema#string"/>
        <rdfs:comment>Specifies a targeted observation pattern of the nature of any trend in the frequency of the associated event or action. This field would be leveraged within an event or action pattern observable triggering on the matching of a specified trend in the frequency of an event or action.</rdfs:comment>
        <rdfs:isDefinedBy rdf:resource="http://cybox.mitre.org/cybox_core"/>
        <rdfs:label>Frequence Trend</rdfs:label>
    </owl:DatatypeProperty>
    


    <!-- http://cybox.mitre.org/cybox_core#frequency.rate -->

    <owl:DatatypeProperty rdf:about="http://cybox.mitre.org/cybox_core#frequency.rate">
        <rdfs:range rdf:resource="http://www.w3.org/2001/XMLSchema#float"/>
        <rdfs:comment>Specifies the rate for this defined frequency.</rdfs:comment>
        <rdfs:isDefinedBy rdf:resource="http://cybox.mitre.org/cybox_core"/>
        <rdfs:label>Frequency Rate</rdfs:label>
    </owl:DatatypeProperty>
    


    <!-- http://cybox.mitre.org/cybox_core#frequency.scale -->

    <owl:DatatypeProperty rdf:about="http://cybox.mitre.org/cybox_core#frequency.scale">
        <rdfs:range rdf:resource="http://www.w3.org/2001/XMLSchema#string"/>
        <rdfs:comment>Specifies the time scale for this defined frequency.</rdfs:comment>
        <rdfs:isDefinedBy rdf:resource="http://cybox.mitre.org/cybox_core"/>
        <rdfs:label>Frequency Scale</rdfs:label>
    </owl:DatatypeProperty>
    


    <!-- http://cybox.mitre.org/cybox_core#frequency.units -->

    <owl:DatatypeProperty rdf:about="http://cybox.mitre.org/cybox_core#frequency.units">
        <rdfs:range rdf:resource="http://www.w3.org/2001/XMLSchema#string"/>
        <rdfs:comment>Specifies  the units for this defined frequency.</rdfs:comment>
        <rdfs:isDefinedBy rdf:resource="http://cybox.mitre.org/cybox_core"/>
        <rdfs:label>Frequency Units</rdfs:label>
    </owl:DatatypeProperty>
    


    <!-- http://cybox.mitre.org/cybox_core#hasChanged -->

    <owl:DatatypeProperty rdf:about="http://cybox.mitre.org/cybox_core#hasChanged">
        <rdfs:range rdf:resource="http://www.w3.org/2001/XMLSchema#boolean"/>
        <rdfs:comment>Specifies a targeted observation pattern of whether the associated object specified has changed in some way without requiring further specific detail. This field would be leveraged within a pattern observable triggering on whether the value of an object specification has changed at all.</rdfs:comment>
        <rdfs:isDefinedBy rdf:resource="http://cybox.mitre.org/cybox_core"/>
        <rdfs:label>Has Changed</rdfs:label>
    </owl:DatatypeProperty>
    


    <!-- http://cybox.mitre.org/cybox_core#keywords -->

    <owl:DatatypeProperty rdf:about="http://cybox.mitre.org/cybox_core#keywords">
        <rdfs:range rdf:resource="http://www.w3.org/2001/XMLSchema#string"/>
        <rdfs:comment>Specifies relevant keywords for this cyber observable.</rdfs:comment>
        <rdfs:isDefinedBy rdf:resource="http://cybox.mitre.org/cybox_core"/>
        <rdfs:label>Keywords</rdfs:label>
    </owl:DatatypeProperty>
    


    <!-- http://cybox.mitre.org/cybox_core#negate -->

    <owl:DatatypeProperty rdf:about="http://cybox.mitre.org/cybox_core#negate">
        <rdfs:range rdf:resource="http://www.w3.org/2001/XMLSchema#boolean"/>
        <rdfs:comment>Specifies, when set to true, indicates the absence (rather than the presence) of the given Observable in a CybOX pattern.</rdfs:comment>
        <rdfs:isDefinedBy rdf:resource="http://cybox.mitre.org/cybox_core"/>
        <rdfs:label>Negate</rdfs:label>
    </owl:DatatypeProperty>
    


    <!-- http://cybox.mitre.org/cybox_core#objectRelationshipType -->

    <owl:DatatypeProperty rdf:about="http://cybox.mitre.org/cybox_core#objectRelationshipType">
        <rdfs:range rdf:resource="http://www.w3.org/2001/XMLSchema#string"/>
        <rdfs:comment>Specifies the nature of the relationship between this Object and the related Object.</rdfs:comment>
        <rdfs:isDefinedBy rdf:resource="http://cybox.mitre.org/cybox_core"/>
        <rdfs:label>Object Relationship</rdfs:label>
    </owl:DatatypeProperty>
    


    <!-- http://cybox.mitre.org/cybox_core#operator -->

    <owl:DatatypeProperty rdf:about="http://cybox.mitre.org/cybox_core#operator">
        <rdfs:range>
            <rdfs:Datatype>
                <owl:oneOf>
                    <rdf:Description>
                        <rdf:type rdf:resource="http://www.w3.org/1999/02/22-rdf-syntax-ns#List"/>
                        <rdf:first rdf:datatype="http://www.w3.org/2001/XMLSchema#string">AND</rdf:first>
                        <rdf:rest>
                            <rdf:Description>
                                <rdf:type rdf:resource="http://www.w3.org/1999/02/22-rdf-syntax-ns#List"/>
                                <rdf:first rdf:datatype="http://www.w3.org/2001/XMLSchema#string">OR</rdf:first>
                                <rdf:rest rdf:resource="http://www.w3.org/1999/02/22-rdf-syntax-ns#nil"/>
                            </rdf:Description>
                        </rdf:rest>
                    </rdf:Description>
                </owl:oneOf>
            </rdfs:Datatype>
        </rdfs:range>
        <rdfs:comment>Specifies the logical operators for defining interrelationships between constituent entities.</rdfs:comment>
        <rdfs:isDefinedBy rdf:resource="http://cybox.mitre.org/cybox_core"/>
        <rdfs:label>Operator</rdfs:label>
    </owl:DatatypeProperty>
    


    <!-- http://cybox.mitre.org/cybox_core#ordinalPosition -->

    <owl:DatatypeProperty rdf:about="http://cybox.mitre.org/cybox_core#ordinalPosition">
        <rdfs:range rdf:resource="http://www.w3.org/2001/XMLSchema#positiveInteger"/>
        <rdfs:comment>Specifies the ordinal position of the action with within a series of actions.</rdfs:comment>
        <rdfs:isDefinedBy rdf:resource="http://cybox.mitre.org/cybox_core"/>
        <rdfs:label>Ordinal Position</rdfs:label>
    </owl:DatatypeProperty>
    


    <!-- http://cybox.mitre.org/cybox_core#patternFidelity.easeOfEvasion -->

    <owl:DatatypeProperty rdf:about="http://cybox.mitre.org/cybox_core#patternFidelity.easeOfEvasion">
        <rdfs:range>
            <rdfs:Datatype>
                <owl:oneOf>
                    <rdf:Description>
                        <rdf:type rdf:resource="http://www.w3.org/1999/02/22-rdf-syntax-ns#List"/>
                        <rdf:first rdf:datatype="http://www.w3.org/2001/XMLSchema#string">High</rdf:first>
                        <rdf:rest>
                            <rdf:Description>
                                <rdf:type rdf:resource="http://www.w3.org/1999/02/22-rdf-syntax-ns#List"/>
                                <rdf:first rdf:datatype="http://www.w3.org/2001/XMLSchema#string">Low</rdf:first>
                                <rdf:rest>
                                    <rdf:Description>
                                        <rdf:type rdf:resource="http://www.w3.org/1999/02/22-rdf-syntax-ns#List"/>
                                        <rdf:first rdf:datatype="http://www.w3.org/2001/XMLSchema#string">Medium</rdf:first>
                                        <rdf:rest rdf:resource="http://www.w3.org/1999/02/22-rdf-syntax-ns#nil"/>
                                    </rdf:Description>
                                </rdf:rest>
                            </rdf:Description>
                        </rdf:rest>
                    </rdf:Description>
                </owl:oneOf>
            </rdfs:Datatype>
        </rdfs:range>
        <rdfs:comment>Specifies how easy it would be for an attacker to obfuscate the observability of this Observable.</rdfs:comment>
        <rdfs:isDefinedBy rdf:resource="http://cybox.mitre.org/cybox_core"/>
        <rdfs:label>pattern Fidelity Ease of Evasion</rdfs:label>
    </owl:DatatypeProperty>
    


    <!-- http://cybox.mitre.org/cybox_core#patternFidelity.noisiness -->

    <owl:DatatypeProperty rdf:about="http://cybox.mitre.org/cybox_core#patternFidelity.noisiness">
        <rdfs:range>
            <rdfs:Datatype>
                <owl:oneOf>
                    <rdf:Description>
                        <rdf:type rdf:resource="http://www.w3.org/1999/02/22-rdf-syntax-ns#List"/>
                        <rdf:first rdf:datatype="http://www.w3.org/2001/XMLSchema#string">High</rdf:first>
                        <rdf:rest>
                            <rdf:Description>
                                <rdf:type rdf:resource="http://www.w3.org/1999/02/22-rdf-syntax-ns#List"/>
                                <rdf:first rdf:datatype="http://www.w3.org/2001/XMLSchema#string">Low</rdf:first>
                                <rdf:rest>
                                    <rdf:Description>
                                        <rdf:type rdf:resource="http://www.w3.org/1999/02/22-rdf-syntax-ns#List"/>
                                        <rdf:first rdf:datatype="http://www.w3.org/2001/XMLSchema#string">Medium</rdf:first>
                                        <rdf:rest rdf:resource="http://www.w3.org/1999/02/22-rdf-syntax-ns#nil"/>
                                    </rdf:Description>
                                </rdf:rest>
                            </rdf:Description>
                        </rdf:rest>
                    </rdf:Description>
                </owl:oneOf>
            </rdfs:Datatype>
        </rdfs:range>
        <rdfs:comment>Specifies how noisy this Observable typically could be. In other words, how likely is it to generate false positives.</rdfs:comment>
        <rdfs:isDefinedBy rdf:resource="http://cybox.mitre.org/cybox_core"/>
        <rdfs:label>Pattern Fidelity Noisiness</rdfs:label>
    </owl:DatatypeProperty>
    


    <!-- http://cybox.mitre.org/cybox_core#sightingCount -->

    <owl:DatatypeProperty rdf:about="http://cybox.mitre.org/cybox_core#sightingCount">
        <rdfs:range rdf:resource="http://www.w3.org/2001/XMLSchema#positiveInteger"/>
        <rdfs:comment>Specifies how many different identical instances of the Observable may have been seen/sighted.</rdfs:comment>
        <rdfs:isDefinedBy rdf:resource="http://cybox.mitre.org/cybox_core"/>
        <rdfs:label>Sighting Count</rdfs:label>
    </owl:DatatypeProperty>
    


    <!-- http://cybox.mitre.org/cybox_core#state -->

    <owl:DatatypeProperty rdf:about="http://cybox.mitre.org/cybox_core#state">
        <rdfs:range rdf:resource="http://www.w3.org/2001/XMLSchema#string"/>
        <rdfs:comment>Specifies the description of the current state of the object, through a standardized controlled vocabulary.</rdfs:comment>
        <rdfs:isDefinedBy rdf:resource="http://cybox.mitre.org/cybox_core"/>
        <rdfs:label>State</rdfs:label>
    </owl:DatatypeProperty>
    


    <!-- http://cybox.mitre.org/cybox_core#timestamp -->

    <owl:DatatypeProperty rdf:about="http://cybox.mitre.org/cybox_core#timestamp">
        <rdfs:range rdf:resource="http://www.w3.org/2001/XMLSchema#dateTime"/>
        <rdfs:comment>Specifies the local or relative time at which the action occurred or was observed. In order to avoid ambiguity, it is strongly suggest that all timestamps in this field include a specification of the timezone if it is known.</rdfs:comment>
        <rdfs:isDefinedBy rdf:resource="http://cybox.mitre.org/cybox_core"/>
        <rdfs:label>Timestamp</rdfs:label>
    </owl:DatatypeProperty>
    


    <!-- http://cybox.mitre.org/cybox_core#timestampPrecision -->

    <owl:DatatypeProperty rdf:about="http://cybox.mitre.org/cybox_core#timestampPrecision">
        <rdfs:range rdf:resource="http://www.w3.org/2001/XMLSchema#string"/>
        <rdfs:comment>Specifies the precision of the associated timestamp value.

 If omitted, the default is &quot;second&quot;, meaning the timestamp is precise to the full field value. Digits in the timestamp that are required by the xs:dateTime datatype but are beyond the specified precision should be zeroed out.</rdfs:comment>
        <rdfs:isDefinedBy rdf:resource="http://cybox.mitre.org/cybox_core"/>
        <rdfs:label>Timestamp Precision</rdfs:label>
    </owl:DatatypeProperty>
    


    <!-- http://cybox.mitre.org/cybox_core#title -->

    <owl:DatatypeProperty rdf:about="http://cybox.mitre.org/cybox_core#title">
        <rdfs:range rdf:resource="http://www.w3.org/2001/XMLSchema#string"/>
        <rdfs:comment>Specifies a short title or description for this entity</rdfs:comment>
        <rdfs:isDefinedBy rdf:resource="http://cybox.mitre.org/cybox_core"/>
        <rdfs:label>Title</rdfs:label>
    </owl:DatatypeProperty>
    


    <!-- http://cybox.mitre.org/cybox_core#values -->

    <owl:DatatypeProperty rdf:about="http://cybox.mitre.org/cybox_core#values">
        <rdfs:range rdf:resource="http://www.w3.org/2001/XMLSchema#string"/>
        <rdfs:comment>Specifies the values that were enumerated as a result of the action on the object.</rdfs:comment>
        <rdfs:isDefinedBy rdf:resource="http://cybox.mitre.org/cybox_core"/>
        <rdfs:label>Values</rdfs:label>
    </owl:DatatypeProperty>
    


    <!-- 
    ///////////////////////////////////////////////////////////////////////////////////////
    //
    // Classes
    //
    ///////////////////////////////////////////////////////////////////////////////////////
     -->

    


    <!-- http://cybox.mitre.org/cybox_core#Action -->

    <owl:Class rdf:about="http://cybox.mitre.org/cybox_core#Action">
        <rdfs:subClassOf>
            <owl:Restriction>
                <owl:onProperty rdf:resource="http://cybox.mitre.org/cybox_core#discoveryMethod"/>
                <owl:maxCardinality rdf:datatype="http://www.w3.org/2001/XMLSchema#nonNegativeInteger">1</owl:maxCardinality>
            </owl:Restriction>
        </rdfs:subClassOf>
        <rdfs:subClassOf>
            <owl:Restriction>
                <owl:onProperty rdf:resource="http://cybox.mitre.org/cybox_core#physicalLocation"/>
                <owl:maxCardinality rdf:datatype="http://www.w3.org/2001/XMLSchema#nonNegativeInteger">1</owl:maxCardinality>
            </owl:Restriction>
        </rdfs:subClassOf>
        <rdfs:subClassOf>
            <owl:Restriction>
                <owl:onProperty rdf:resource="http://cybox.mitre.org/cybox_core#actionStatus"/>
                <owl:cardinality rdf:datatype="http://www.w3.org/2001/XMLSchema#nonNegativeInteger">1</owl:cardinality>
            </owl:Restriction>
        </rdfs:subClassOf>
        <rdfs:subClassOf>
            <owl:Restriction>
                <owl:onProperty rdf:resource="http://cybox.mitre.org/cybox_core#actionType"/>
                <owl:cardinality rdf:datatype="http://www.w3.org/2001/XMLSchema#nonNegativeInteger">1</owl:cardinality>
            </owl:Restriction>
        </rdfs:subClassOf>
        <rdfs:subClassOf>
            <owl:Restriction>
                <owl:onProperty rdf:resource="http://cybox.mitre.org/cybox_core#ordinalPosition"/>
                <owl:cardinality rdf:datatype="http://www.w3.org/2001/XMLSchema#nonNegativeInteger">1</owl:cardinality>
            </owl:Restriction>
        </rdfs:subClassOf>
        <rdfs:subClassOf>
            <owl:Restriction>
                <owl:onProperty rdf:resource="http://cybox.mitre.org/cybox_core#actionContext"/>
                <owl:maxCardinality rdf:datatype="http://www.w3.org/2001/XMLSchema#nonNegativeInteger">1</owl:maxCardinality>
            </owl:Restriction>
        </rdfs:subClassOf>
        <rdfs:subClassOf>
            <owl:Restriction>
                <owl:onProperty rdf:resource="http://cybox.mitre.org/cybox_core#actionName"/>
                <owl:maxCardinality rdf:datatype="http://www.w3.org/2001/XMLSchema#nonNegativeInteger">1</owl:maxCardinality>
            </owl:Restriction>
        </rdfs:subClassOf>
        <rdfs:subClassOf>
            <owl:Restriction>
                <owl:onProperty rdf:resource="http://cybox.mitre.org/cybox_core#actionType"/>
                <owl:maxCardinality rdf:datatype="http://www.w3.org/2001/XMLSchema#nonNegativeInteger">1</owl:maxCardinality>
            </owl:Restriction>
        </rdfs:subClassOf>
        <rdfs:subClassOf>
            <owl:Restriction>
                <owl:onProperty rdf:resource="http://cybox.mitre.org/cybox_core#frequence.trend"/>
                <owl:maxCardinality rdf:datatype="http://www.w3.org/2001/XMLSchema#nonNegativeInteger">1</owl:maxCardinality>
            </owl:Restriction>
        </rdfs:subClassOf>
        <rdfs:subClassOf>
            <owl:Restriction>
                <owl:onProperty rdf:resource="http://cybox.mitre.org/cybox_core#frequency.rate"/>
                <owl:maxCardinality rdf:datatype="http://www.w3.org/2001/XMLSchema#nonNegativeInteger">1</owl:maxCardinality>
            </owl:Restriction>
        </rdfs:subClassOf>
        <rdfs:subClassOf>
            <owl:Restriction>
                <owl:onProperty rdf:resource="http://cybox.mitre.org/cybox_core#frequency.scale"/>
                <owl:maxCardinality rdf:datatype="http://www.w3.org/2001/XMLSchema#nonNegativeInteger">1</owl:maxCardinality>
            </owl:Restriction>
        </rdfs:subClassOf>
        <rdfs:subClassOf>
            <owl:Restriction>
                <owl:onProperty rdf:resource="http://cybox.mitre.org/cybox_core#frequency.units"/>
                <owl:maxCardinality rdf:datatype="http://www.w3.org/2001/XMLSchema#nonNegativeInteger">1</owl:maxCardinality>
            </owl:Restriction>
        </rdfs:subClassOf>
        <rdfs:subClassOf>
            <owl:Restriction>
                <owl:onProperty rdf:resource="http://cybox.mitre.org/cybox_core#timestamp"/>
                <owl:maxCardinality rdf:datatype="http://www.w3.org/2001/XMLSchema#nonNegativeInteger">1</owl:maxCardinality>
            </owl:Restriction>
        </rdfs:subClassOf>
        <rdfs:subClassOf>
            <owl:Restriction>
                <owl:onProperty rdf:resource="http://cybox.mitre.org/cybox_core#timestampPrecision"/>
                <owl:maxCardinality rdf:datatype="http://www.w3.org/2001/XMLSchema#nonNegativeInteger">1</owl:maxCardinality>
            </owl:Restriction>
        </rdfs:subClassOf>
        <rdfs:comment>Characterizes a single cyber observable action.</rdfs:comment>
        <rdfs:isDefinedBy rdf:resource="http://cybox.mitre.org/cybox_core"/>
        <rdfs:label>Action</rdfs:label>
    </owl:Class>
    


    <!-- http://cybox.mitre.org/cybox_core#ActionArgument -->

    <owl:Class rdf:about="http://cybox.mitre.org/cybox_core#ActionArgument">
        <rdfs:subClassOf>
            <owl:Restriction>
                <owl:onProperty rdf:resource="http://cybox.mitre.org/cybox_core#argumentName"/>
                <owl:cardinality rdf:datatype="http://www.w3.org/2001/XMLSchema#nonNegativeInteger">1</owl:cardinality>
            </owl:Restriction>
        </rdfs:subClassOf>
        <rdfs:subClassOf>
            <owl:Restriction>
                <owl:onProperty rdf:resource="http://cybox.mitre.org/cybox_core#argumentValue"/>
                <owl:maxCardinality rdf:datatype="http://www.w3.org/2001/XMLSchema#nonNegativeInteger">1</owl:maxCardinality>
            </owl:Restriction>
        </rdfs:subClassOf>
        <rdfs:comment>Characterizes a single relevant argument/parameter for an Action.</rdfs:comment>
        <rdfs:isDefinedBy rdf:resource="http://cybox.mitre.org/cybox_core"/>
        <rdfs:label>Action Argument</rdfs:label>
    </owl:Class>
    


    <!-- http://cybox.mitre.org/cybox_core#ActionRelationshipStatement -->

    <owl:Class rdf:about="http://cybox.mitre.org/cybox_core#ActionRelationshipStatement">
        <rdfs:subClassOf rdf:resource="http://www.w3.org/1999/02/22-rdf-syntax-ns#Statement"/>
        <rdfs:subClassOf>
            <owl:Restriction>
                <owl:onProperty rdf:resource="http://cybox.mitre.org/cybox_core#actionRelationshipType"/>
                <owl:cardinality rdf:datatype="http://www.w3.org/2001/XMLSchema#nonNegativeInteger">1</owl:cardinality>
            </owl:Restriction>
        </rdfs:subClassOf>
        <rdfs:subClassOf>
            <owl:Restriction>
                <owl:onProperty rdf:resource="http://cybox.mitre.org/cybox_core#description"/>
                <owl:maxCardinality rdf:datatype="http://www.w3.org/2001/XMLSchema#nonNegativeInteger">1</owl:maxCardinality>
            </owl:Restriction>
        </rdfs:subClassOf>
        <rdfs:isDefinedBy rdf:resource="http://cybox.mitre.org/cybox_core"/>
        <rdfs:label>Action Relationship Statement</rdfs:label>
    </owl:Class>
    


    <!-- http://cybox.mitre.org/cybox_core#AssociationStatement -->

    <owl:Class rdf:about="http://cybox.mitre.org/cybox_core#AssociationStatement">
        <rdfs:subClassOf rdf:resource="http://www.w3.org/1999/02/22-rdf-syntax-ns#Statement"/>
        <rdfs:subClassOf>
            <owl:Restriction>
                <owl:onProperty rdf:resource="http://cybox.mitre.org/cybox_core#associationType"/>
                <owl:cardinality rdf:datatype="http://www.w3.org/2001/XMLSchema#nonNegativeInteger">1</owl:cardinality>
            </owl:Restriction>
        </rdfs:subClassOf>
        <rdfs:comment>Characterizes the nature of the relationship between an action and the associated objects</rdfs:comment>
        <rdfs:isDefinedBy rdf:resource="http://cybox.mitre.org/cybox_core"/>
        <rdfs:label>Association Statement</rdfs:label>
    </owl:Class>
    


    <!-- http://cybox.mitre.org/cybox_core#DataReadEffect -->

    <owl:Class rdf:about="http://cybox.mitre.org/cybox_core#DataReadEffect">
        <rdfs:subClassOf rdf:resource="http://cybox.mitre.org/cybox_core#DefinedEffect"/>
        <rdfs:comment>Characterize the effects of actions upon objects where some data is read, such as from a file or a pipe.</rdfs:comment>
        <rdfs:isDefinedBy rdf:resource="http://cybox.mitre.org/cybox_core"/>
        <rdfs:label>Data read effect</rdfs:label>
    </owl:Class>
    


    <!-- http://cybox.mitre.org/cybox_core#DataReceivedEffect -->

    <owl:Class rdf:about="http://cybox.mitre.org/cybox_core#DataReceivedEffect">
        <rdfs:subClassOf rdf:resource="http://cybox.mitre.org/cybox_core#DefinedEffect"/>
        <rdfs:comment>Characterizes the effects of actions upon objects where some data is received, such as a byte sequence on a socket.</rdfs:comment>
        <rdfs:isDefinedBy rdf:resource="http://cybox.mitre.org/cybox_core"/>
        <rdfs:label>Data Received Effect</rdfs:label>
    </owl:Class>
    


    <!-- http://cybox.mitre.org/cybox_core#DataSendEffect -->

    <owl:Class rdf:about="http://cybox.mitre.org/cybox_core#DataSendEffect">
        <rdfs:subClassOf rdf:resource="http://cybox.mitre.org/cybox_core#DefinedEffect"/>
        <rdfs:comment>Characterizes the effects of actions upon objects where some data is sent, such as a byte sequence on a socket.</rdfs:comment>
        <rdfs:isDefinedBy rdf:resource="http://cybox.mitre.org/cybox_core"/>
        <rdfs:label>Data Send Effect</rdfs:label>
    </owl:Class>
    


    <!-- http://cybox.mitre.org/cybox_core#DataWrittenEffect -->

    <owl:Class rdf:about="http://cybox.mitre.org/cybox_core#DataWrittenEffect">
        <rdfs:subClassOf rdf:resource="http://cybox.mitre.org/cybox_core#DefinedEffect"/>
        <rdfs:comment>Characterizes the effects of actions upon objects where some data is written, such as to a file or a pipe.</rdfs:comment>
        <rdfs:isDefinedBy rdf:resource="http://cybox.mitre.org/cybox_core"/>
        <rdfs:label>Data Written Effect</rdfs:label>
    </owl:Class>
    


    <!-- http://cybox.mitre.org/cybox_core#DefinedEffect -->

    <owl:Class rdf:about="http://cybox.mitre.org/cybox_core#DefinedEffect">
        <rdfs:subClassOf>
            <owl:Restriction>
                <owl:onProperty rdf:resource="http://cybox.mitre.org/cybox_core#effectType"/>
                <owl:cardinality rdf:datatype="http://www.w3.org/2001/XMLSchema#nonNegativeInteger">1</owl:cardinality>
            </owl:Restriction>
        </rdfs:subClassOf>
        <rdfs:comment>Characterizes various predefined Object Effect types (e.g. DataReadEffect, ValuesEnumeratedEffect or StateChangeEffect) that can be instantiated in its place through extension of the DefinedEffectType. This mechanism enables the specification of a broad range of types of potential complex action effects on Objects.</rdfs:comment>
        <rdfs:isDefinedBy rdf:resource="http://cybox.mitre.org/cybox_core"/>
        <rdfs:label>Defined Effect</rdfs:label>
    </owl:Class>
    


    <!-- http://cybox.mitre.org/cybox_core#Event -->

    <owl:Class rdf:about="http://cybox.mitre.org/cybox_core#Event">
        <rdfs:subClassOf>
            <owl:Restriction>
                <owl:onProperty rdf:resource="http://cybox.mitre.org/cybox_core#event"/>
                <owl:maxCardinality rdf:datatype="http://www.w3.org/2001/XMLSchema#nonNegativeInteger">1</owl:maxCardinality>
            </owl:Restriction>
        </rdfs:subClassOf>
        <rdfs:subClassOf>
            <owl:Restriction>
                <owl:onProperty rdf:resource="http://cybox.mitre.org/cybox_core#observationMethod"/>
                <owl:maxCardinality rdf:datatype="http://www.w3.org/2001/XMLSchema#nonNegativeInteger">1</owl:maxCardinality>
            </owl:Restriction>
        </rdfs:subClassOf>
        <rdfs:subClassOf>
            <owl:Restriction>
                <owl:onProperty rdf:resource="http://cybox.mitre.org/cybox_core#physicalLocation"/>
                <owl:maxCardinality rdf:datatype="http://www.w3.org/2001/XMLSchema#nonNegativeInteger">1</owl:maxCardinality>
            </owl:Restriction>
        </rdfs:subClassOf>
        <rdfs:subClassOf>
            <owl:Restriction>
                <owl:onProperty rdf:resource="http://cybox.mitre.org/cybox_core#eventType"/>
                <owl:cardinality rdf:datatype="http://www.w3.org/2001/XMLSchema#nonNegativeInteger">1</owl:cardinality>
            </owl:Restriction>
        </rdfs:subClassOf>
        <rdfs:subClassOf>
            <owl:Restriction>
                <owl:onProperty rdf:resource="http://cybox.mitre.org/cybox_core#description"/>
                <owl:maxCardinality rdf:datatype="http://www.w3.org/2001/XMLSchema#nonNegativeInteger">1</owl:maxCardinality>
            </owl:Restriction>
        </rdfs:subClassOf>
        <rdfs:subClassOf>
            <owl:Restriction>
                <owl:onProperty rdf:resource="http://cybox.mitre.org/cybox_core#frequence.trend"/>
                <owl:maxCardinality rdf:datatype="http://www.w3.org/2001/XMLSchema#nonNegativeInteger">1</owl:maxCardinality>
            </owl:Restriction>
        </rdfs:subClassOf>
        <rdfs:subClassOf>
            <owl:Restriction>
                <owl:onProperty rdf:resource="http://cybox.mitre.org/cybox_core#frequency.rate"/>
                <owl:maxCardinality rdf:datatype="http://www.w3.org/2001/XMLSchema#nonNegativeInteger">1</owl:maxCardinality>
            </owl:Restriction>
        </rdfs:subClassOf>
        <rdfs:subClassOf>
            <owl:Restriction>
                <owl:onProperty rdf:resource="http://cybox.mitre.org/cybox_core#frequency.scale"/>
                <owl:maxCardinality rdf:datatype="http://www.w3.org/2001/XMLSchema#nonNegativeInteger">1</owl:maxCardinality>
            </owl:Restriction>
        </rdfs:subClassOf>
        <rdfs:subClassOf>
            <owl:Restriction>
                <owl:onProperty rdf:resource="http://cybox.mitre.org/cybox_core#frequency.units"/>
                <owl:maxCardinality rdf:datatype="http://www.w3.org/2001/XMLSchema#nonNegativeInteger">1</owl:maxCardinality>
            </owl:Restriction>
        </rdfs:subClassOf>
        <rdfs:comment>Characterizes a complex type representing a cyber observable event that is dynamic in nature with specific action(s) taken against specific cyber relevant objects (e.g. a file is deleted, a registry key is created or an HTTP Get Request is received).</rdfs:comment>
        <rdfs:isDefinedBy rdf:resource="http://cybox.mitre.org/cybox_core"/>
        <rdfs:label>Event</rdfs:label>
    </owl:Class>
    


    <!-- http://cybox.mitre.org/cybox_core#ObfuscationTechnique -->

    <owl:Class rdf:about="http://cybox.mitre.org/cybox_core#ObfuscationTechnique">
        <rdfs:subClassOf>
            <owl:Restriction>
                <owl:onProperty rdf:resource="http://cybox.mitre.org/cybox_core#techniqueObservables"/>
                <owl:maxCardinality rdf:datatype="http://www.w3.org/2001/XMLSchema#nonNegativeInteger">1</owl:maxCardinality>
            </owl:Restriction>
        </rdfs:subClassOf>
        <rdfs:subClassOf>
            <owl:Restriction>
                <owl:onProperty rdf:resource="http://cybox.mitre.org/cybox_core#description"/>
                <owl:cardinality rdf:datatype="http://www.w3.org/2001/XMLSchema#nonNegativeInteger">1</owl:cardinality>
            </owl:Restriction>
        </rdfs:subClassOf>
        <rdfs:comment>Characterizes a single potential technique an attacker could leverage to obfuscate the observability of this Observable.</rdfs:comment>
        <rdfs:isDefinedBy rdf:resource="http://cybox.mitre.org/cybox_core"/>
        <rdfs:label>Obfuscation Technique</rdfs:label>
    </owl:Class>
    


    <!-- http://cybox.mitre.org/cybox_core#Object -->

    <owl:Class rdf:about="http://cybox.mitre.org/cybox_core#Object">
        <rdfs:subClassOf>
            <owl:Restriction>
                <owl:onProperty rdf:resource="http://cybox.mitre.org/cybox_core#definedEffect"/>
                <owl:maxCardinality rdf:datatype="http://www.w3.org/2001/XMLSchema#nonNegativeInteger">1</owl:maxCardinality>
            </owl:Restriction>
        </rdfs:subClassOf>
        <rdfs:subClassOf>
            <owl:Restriction>
                <owl:onProperty rdf:resource="http://cybox.mitre.org/cybox_core#discoveryMethod"/>
                <owl:maxCardinality rdf:datatype="http://www.w3.org/2001/XMLSchema#nonNegativeInteger">1</owl:maxCardinality>
            </owl:Restriction>
        </rdfs:subClassOf>
        <rdfs:subClassOf>
            <owl:Restriction>
                <owl:onProperty rdf:resource="http://cybox.mitre.org/cybox_core#physicalLocation"/>
                <owl:maxCardinality rdf:datatype="http://www.w3.org/2001/XMLSchema#nonNegativeInteger">1</owl:maxCardinality>
            </owl:Restriction>
        </rdfs:subClassOf>
        <rdfs:subClassOf>
            <owl:Restriction>
                <owl:onProperty rdf:resource="http://cybox.mitre.org/cyboxCommon#id"/>
                <owl:qualifiedCardinality rdf:datatype="http://www.w3.org/2001/XMLSchema#nonNegativeInteger">1</owl:qualifiedCardinality>
                <owl:onDataRange rdf:resource="http://www.w3.org/2001/XMLSchema#string"/>
            </owl:Restriction>
        </rdfs:subClassOf>
        <rdfs:subClassOf>
            <owl:Restriction>
                <owl:onProperty rdf:resource="http://cybox.mitre.org/cybox_core#description"/>
                <owl:maxCardinality rdf:datatype="http://www.w3.org/2001/XMLSchema#nonNegativeInteger">1</owl:maxCardinality>
            </owl:Restriction>
        </rdfs:subClassOf>
        <rdfs:subClassOf>
            <owl:Restriction>
                <owl:onProperty rdf:resource="http://cybox.mitre.org/cybox_core#hasChanged"/>
                <owl:maxCardinality rdf:datatype="http://www.w3.org/2001/XMLSchema#nonNegativeInteger">1</owl:maxCardinality>
            </owl:Restriction>
        </rdfs:subClassOf>
        <rdfs:subClassOf>
            <owl:Restriction>
                <owl:onProperty rdf:resource="http://cybox.mitre.org/cybox_core#state"/>
                <owl:maxCardinality rdf:datatype="http://www.w3.org/2001/XMLSchema#nonNegativeInteger">1</owl:maxCardinality>
            </owl:Restriction>
        </rdfs:subClassOf>
        <rdfs:comment>Characterizes a complex type representing the characteristics of a specific cyber-relevant object (e.g. a file, a registry key or a process).</rdfs:comment>
        <rdfs:isDefinedBy rdf:resource="http://cybox.mitre.org/cybox_core"/>
        <rdfs:label>Object</rdfs:label>
    </owl:Class>
    


    <!-- http://cybox.mitre.org/cybox_core#ObjectRelationshipStatement -->

    <owl:Class rdf:about="http://cybox.mitre.org/cybox_core#ObjectRelationshipStatement">
        <rdfs:subClassOf rdf:resource="http://www.w3.org/1999/02/22-rdf-syntax-ns#Statement"/>
        <rdfs:subClassOf>
            <owl:Restriction>
                <owl:onProperty rdf:resource="http://cybox.mitre.org/cybox_core#description"/>
                <owl:maxCardinality rdf:datatype="http://www.w3.org/2001/XMLSchema#nonNegativeInteger">1</owl:maxCardinality>
            </owl:Restriction>
        </rdfs:subClassOf>
        <rdfs:subClassOf>
            <owl:Restriction>
                <owl:onProperty rdf:resource="http://cybox.mitre.org/cybox_core#objectRelationshipType"/>
                <owl:maxCardinality rdf:datatype="http://www.w3.org/2001/XMLSchema#nonNegativeInteger">1</owl:maxCardinality>
            </owl:Restriction>
        </rdfs:subClassOf>
        <rdfs:comment>Characterizes the nature of the relationship between an Object  with this Object.</rdfs:comment>
        <rdfs:isDefinedBy rdf:resource="http://cybox.mitre.org/cybox_core"/>
    </owl:Class>
    


    <!-- http://cybox.mitre.org/cybox_core#Observable -->

    <owl:Class rdf:about="http://cybox.mitre.org/cybox_core#Observable">
        <rdfs:subClassOf>
            <owl:Restriction>
                <owl:onProperty rdf:resource="http://cybox.mitre.org/cybox_core#observedEntity"/>
                <owl:maxCardinality rdf:datatype="http://www.w3.org/2001/XMLSchema#nonNegativeInteger">1</owl:maxCardinality>
            </owl:Restriction>
        </rdfs:subClassOf>
        <rdfs:subClassOf>
            <owl:Restriction>
                <owl:onProperty rdf:resource="http://cybox.mitre.org/cybox_core#negate"/>
                <owl:cardinality rdf:datatype="http://www.w3.org/2001/XMLSchema#nonNegativeInteger">1</owl:cardinality>
            </owl:Restriction>
        </rdfs:subClassOf>
        <rdfs:subClassOf>
            <owl:Restriction>
                <owl:onProperty rdf:resource="http://cybox.mitre.org/cybox_core#description"/>
                <owl:maxCardinality rdf:datatype="http://www.w3.org/2001/XMLSchema#nonNegativeInteger">1</owl:maxCardinality>
            </owl:Restriction>
        </rdfs:subClassOf>
        <rdfs:subClassOf>
            <owl:Restriction>
                <owl:onProperty rdf:resource="http://cybox.mitre.org/cybox_core#patternFidelity.easeOfEvasion"/>
                <owl:maxCardinality rdf:datatype="http://www.w3.org/2001/XMLSchema#nonNegativeInteger">1</owl:maxCardinality>
            </owl:Restriction>
        </rdfs:subClassOf>
        <rdfs:subClassOf>
            <owl:Restriction>
                <owl:onProperty rdf:resource="http://cybox.mitre.org/cybox_core#patternFidelity.noisiness"/>
                <owl:maxCardinality rdf:datatype="http://www.w3.org/2001/XMLSchema#nonNegativeInteger">1</owl:maxCardinality>
            </owl:Restriction>
        </rdfs:subClassOf>
        <rdfs:subClassOf>
            <owl:Restriction>
                <owl:onProperty rdf:resource="http://cybox.mitre.org/cybox_core#sightingCount"/>
                <owl:maxCardinality rdf:datatype="http://www.w3.org/2001/XMLSchema#nonNegativeInteger">1</owl:maxCardinality>
            </owl:Restriction>
        </rdfs:subClassOf>
        <rdfs:subClassOf>
            <owl:Restriction>
                <owl:onProperty rdf:resource="http://cybox.mitre.org/cybox_core#title"/>
                <owl:maxCardinality rdf:datatype="http://www.w3.org/2001/XMLSchema#nonNegativeInteger">1</owl:maxCardinality>
            </owl:Restriction>
        </rdfs:subClassOf>
        <rdfs:comment>Characterizes a description of a single cyber observable.</rdfs:comment>
        <rdfs:isDefinedBy rdf:resource="http://cybox.mitre.org/cybox_core"/>
        <rdfs:label>Observable</rdfs:label>
    </owl:Class>
    


    <!-- http://cybox.mitre.org/cybox_core#ObservableComposition -->

    <owl:Class rdf:about="http://cybox.mitre.org/cybox_core#ObservableComposition">
        <rdfs:subClassOf>
            <owl:Restriction>
                <owl:onProperty rdf:resource="http://cybox.mitre.org/cybox_core#observable"/>
                <owl:minCardinality rdf:datatype="http://www.w3.org/2001/XMLSchema#nonNegativeInteger">1</owl:minCardinality>
            </owl:Restriction>
        </rdfs:subClassOf>
        <rdfs:subClassOf>
            <owl:Restriction>
                <owl:onProperty rdf:resource="http://cybox.mitre.org/cybox_core#operator"/>
                <owl:cardinality rdf:datatype="http://www.w3.org/2001/XMLSchema#nonNegativeInteger">1</owl:cardinality>
            </owl:Restriction>
        </rdfs:subClassOf>
        <rdfs:comment>Characterizes a higher-order composite observables composed of logical combinations of other observables.</rdfs:comment>
        <rdfs:isDefinedBy rdf:resource="http://cybox.mitre.org/cybox_core"/>
        <rdfs:label>Observable Composition</rdfs:label>
    </owl:Class>
    


    <!-- http://cybox.mitre.org/cybox_core#Observables -->

    <owl:Class rdf:about="http://cybox.mitre.org/cybox_core#Observables">
        <rdfs:subClassOf>
            <owl:Restriction>
                <owl:onProperty rdf:resource="http://cybox.mitre.org/cybox_core#observable"/>
                <owl:minCardinality rdf:datatype="http://www.w3.org/2001/XMLSchema#nonNegativeInteger">1</owl:minCardinality>
            </owl:Restriction>
        </rdfs:subClassOf>
        <rdfs:subClassOf>
            <owl:Restriction>
                <owl:onProperty rdf:resource="http://cybox.mitre.org/cybox_core#observablePackageSource"/>
                <owl:maxCardinality rdf:datatype="http://www.w3.org/2001/XMLSchema#nonNegativeInteger">1</owl:maxCardinality>
            </owl:Restriction>
        </rdfs:subClassOf>
        <rdfs:comment>Characterizes a collection of cyber observables.</rdfs:comment>
        <rdfs:isDefinedBy rdf:resource="http://cybox.mitre.org/cybox_core"/>
        <rdfs:label>Observables</rdfs:label>
    </owl:Class>
    


    <!-- http://cybox.mitre.org/cybox_core#PropertiesEnumeratedEffect -->

    <owl:Class rdf:about="http://cybox.mitre.org/cybox_core#PropertiesEnumeratedEffect">
        <rdfs:subClassOf rdf:resource="http://cybox.mitre.org/cybox_core#DefinedEffect"/>
        <rdfs:comment>Characterize the effects of actions upon objects where some properties of the object are enumerated, such as the startup parameters for a process.</rdfs:comment>
        <rdfs:isDefinedBy rdf:resource="http://cybox.mitre.org/cybox_core"/>
        <rdfs:label>Properties Enumerated Effect</rdfs:label>
    </owl:Class>
    


    <!-- http://cybox.mitre.org/cybox_core#PropertyReadEffect -->

    <owl:Class rdf:about="http://cybox.mitre.org/cybox_core#PropertyReadEffect">
        <rdfs:subClassOf rdf:resource="http://cybox.mitre.org/cybox_core#DefinedEffect"/>
        <rdfs:comment>Characterizes the effects of actions upon objects where some specific property is read from an object, such as the current running state of a process.</rdfs:comment>
        <rdfs:isDefinedBy rdf:resource="http://cybox.mitre.org/cybox_core"/>
        <rdfs:label>Property Read Effect</rdfs:label>
    </owl:Class>
    


    <!-- http://cybox.mitre.org/cybox_core#SendControlCodeEffect -->

    <owl:Class rdf:about="http://cybox.mitre.org/cybox_core#SendControlCodeEffect">
        <rdfs:subClassOf rdf:resource="http://cybox.mitre.org/cybox_core#DefinedEffect"/>
        <rdfs:subClassOf>
            <owl:Restriction>
                <owl:onProperty rdf:resource="http://cybox.mitre.org/cybox_core#controlCode"/>
                <owl:cardinality rdf:datatype="http://www.w3.org/2001/XMLSchema#nonNegativeInteger">1</owl:cardinality>
            </owl:Restriction>
        </rdfs:subClassOf>
        <rdfs:comment>Characterize the effects of actions upon objects where some control code, or other control-oriented communication signal, is sent to the object. For example, an action may send a control code to change the running state of a process.</rdfs:comment>
        <rdfs:isDefinedBy rdf:resource="http://cybox.mitre.org/cybox_core"/>
        <rdfs:label>Send Control Code Effect</rdfs:label>
    </owl:Class>
    


    <!-- http://cybox.mitre.org/cybox_core#StateChangeEffect -->

    <owl:Class rdf:about="http://cybox.mitre.org/cybox_core#StateChangeEffect">
        <rdfs:subClassOf rdf:resource="http://cybox.mitre.org/cybox_core#DefinedEffect"/>
        <rdfs:subClassOf>
            <owl:Restriction>
                <owl:onProperty rdf:resource="http://cybox.mitre.org/cybox_core#newObject"/>
                <owl:cardinality rdf:datatype="http://www.w3.org/2001/XMLSchema#nonNegativeInteger">1</owl:cardinality>
            </owl:Restriction>
        </rdfs:subClassOf>
        <rdfs:subClassOf>
            <owl:Restriction>
                <owl:onProperty rdf:resource="http://cybox.mitre.org/cybox_core#oldObject"/>
                <owl:maxCardinality rdf:datatype="http://www.w3.org/2001/XMLSchema#nonNegativeInteger">1</owl:maxCardinality>
            </owl:Restriction>
        </rdfs:subClassOf>
        <rdfs:comment>Characterizing the effects of actions upon objects where the some state of the object is changed.</rdfs:comment>
        <rdfs:isDefinedBy rdf:resource="http://cybox.mitre.org/cybox_core"/>
        <rdfs:label>State Change Effect</rdfs:label>
    </owl:Class>
    


    <!-- http://cybox.mitre.org/cybox_core#ValuesEnumeratedEffect -->

    <owl:Class rdf:about="http://cybox.mitre.org/cybox_core#ValuesEnumeratedEffect">
        <rdfs:subClassOf rdf:resource="http://cybox.mitre.org/cybox_core#DefinedEffect"/>
        <rdfs:comment>Characterize the effects of actions upon objects where some values of the object are enumerated, such as the values of a registry key.</rdfs:comment>
        <rdfs:isDefinedBy rdf:resource="http://cybox.mitre.org/cybox_core"/>
        <rdfs:label>Values enumerated effect</rdfs:label>
    </owl:Class>
    


    <!-- http://www.w3.org/1999/02/22-rdf-syntax-ns#Statement -->

    <owl:Class rdf:about="http://www.w3.org/1999/02/22-rdf-syntax-ns#Statement"/>
    <rdf:Description>
        <owl:maxCardinality rdf:datatype="http://www.w3.org/2001/XMLSchema#nonNegativeInteger">1</owl:maxCardinality>
    </rdf:Description>
    <rdf:Description>
        <owl:maxCardinality rdf:datatype="http://www.w3.org/2001/XMLSchema#nonNegativeInteger">1</owl:maxCardinality>
    </rdf:Description>
    <rdf:Description>
        <owl:maxCardinality rdf:datatype="http://www.w3.org/2001/XMLSchema#nonNegativeInteger">1</owl:maxCardinality>
    </rdf:Description>
    <rdf:Description>
        <owl:maxCardinality rdf:datatype="http://www.w3.org/2001/XMLSchema#nonNegativeInteger">1</owl:maxCardinality>
    </rdf:Description>
    <rdf:Description>
        <owl:maxCardinality rdf:datatype="http://www.w3.org/2001/XMLSchema#nonNegativeInteger">1</owl:maxCardinality>
    </rdf:Description>
    <rdf:Description>
        <owl:cardinality rdf:datatype="http://www.w3.org/2001/XMLSchema#nonNegativeInteger">1</owl:cardinality>
    </rdf:Description>
    <rdf:Description>
        <owl:cardinality rdf:datatype="http://www.w3.org/2001/XMLSchema#nonNegativeInteger">1</owl:cardinality>
    </rdf:Description>
    <rdf:Description>
        <owl:maxCardinality rdf:datatype="http://www.w3.org/2001/XMLSchema#nonNegativeInteger">1</owl:maxCardinality>
    </rdf:Description>
    <rdf:Description>
        <owl:maxCardinality rdf:datatype="http://www.w3.org/2001/XMLSchema#nonNegativeInteger">1</owl:maxCardinality>
    </rdf:Description>
    <rdf:Description>
        <owl:cardinality rdf:datatype="http://www.w3.org/2001/XMLSchema#nonNegativeInteger">1</owl:cardinality>
    </rdf:Description>
    <rdf:Description>
        <owl:maxCardinality rdf:datatype="http://www.w3.org/2001/XMLSchema#nonNegativeInteger">1</owl:maxCardinality>
    </rdf:Description>
    <rdf:Description>
        <owl:cardinality rdf:datatype="http://www.w3.org/2001/XMLSchema#nonNegativeInteger">1</owl:cardinality>
    </rdf:Description>
    <rdf:Description>
        <owl:cardinality rdf:datatype="http://www.w3.org/2001/XMLSchema#nonNegativeInteger">1</owl:cardinality>
    </rdf:Description>
    <rdf:Description>
        <owl:maxCardinality rdf:datatype="http://www.w3.org/2001/XMLSchema#nonNegativeInteger">1</owl:maxCardinality>
    </rdf:Description>
    <rdf:Description>
        <owl:cardinality rdf:datatype="http://www.w3.org/2001/XMLSchema#nonNegativeInteger">1</owl:cardinality>
    </rdf:Description>
    <rdf:Description>
        <owl:maxCardinality rdf:datatype="http://www.w3.org/2001/XMLSchema#nonNegativeInteger">1</owl:maxCardinality>
    </rdf:Description>
    <rdf:Description>
        <owl:maxCardinality rdf:datatype="http://www.w3.org/2001/XMLSchema#nonNegativeInteger">1</owl:maxCardinality>
    </rdf:Description>
    <rdf:Description>
        <owl:maxCardinality rdf:datatype="http://www.w3.org/2001/XMLSchema#nonNegativeInteger">1</owl:maxCardinality>
    </rdf:Description>
    <rdf:Description>
        <owl:maxCardinality rdf:datatype="http://www.w3.org/2001/XMLSchema#nonNegativeInteger">1</owl:maxCardinality>
    </rdf:Description>
    <rdf:Description>
        <owl:maxCardinality rdf:datatype="http://www.w3.org/2001/XMLSchema#nonNegativeInteger">1</owl:maxCardinality>
    </rdf:Description>
    <rdf:Description>
        <owl:maxCardinality rdf:datatype="http://www.w3.org/2001/XMLSchema#nonNegativeInteger">1</owl:maxCardinality>
    </rdf:Description>
    <rdf:Description>
        <owl:maxCardinality rdf:datatype="http://www.w3.org/2001/XMLSchema#nonNegativeInteger">1</owl:maxCardinality>
    </rdf:Description>
    <rdf:Description>
        <owl:cardinality rdf:datatype="http://www.w3.org/2001/XMLSchema#nonNegativeInteger">1</owl:cardinality>
    </rdf:Description>
    <rdf:Description>
        <owl:maxCardinality rdf:datatype="http://www.w3.org/2001/XMLSchema#nonNegativeInteger">1</owl:maxCardinality>
    </rdf:Description>
    <rdf:Description>
        <owl:maxCardinality rdf:datatype="http://www.w3.org/2001/XMLSchema#nonNegativeInteger">1</owl:maxCardinality>
    </rdf:Description>
    <rdf:Description>
        <owl:maxCardinality rdf:datatype="http://www.w3.org/2001/XMLSchema#nonNegativeInteger">1</owl:maxCardinality>
    </rdf:Description>
    <rdf:Description>
        <owl:maxCardinality rdf:datatype="http://www.w3.org/2001/XMLSchema#nonNegativeInteger">1</owl:maxCardinality>
    </rdf:Description>
    <rdf:Description>
        <owl:maxCardinality rdf:datatype="http://www.w3.org/2001/XMLSchema#nonNegativeInteger">1</owl:maxCardinality>
    </rdf:Description>
    <rdf:Description>
        <owl:maxCardinality rdf:datatype="http://www.w3.org/2001/XMLSchema#nonNegativeInteger">1</owl:maxCardinality>
    </rdf:Description>
    <rdf:Description>
        <owl:maxCardinality rdf:datatype="http://www.w3.org/2001/XMLSchema#nonNegativeInteger">1</owl:maxCardinality>
    </rdf:Description>
    <rdf:Description>
        <owl:cardinality rdf:datatype="http://www.w3.org/2001/XMLSchema#nonNegativeInteger">1</owl:cardinality>
    </rdf:Description>
    <rdf:Description>
        <owl:maxCardinality rdf:datatype="http://www.w3.org/2001/XMLSchema#nonNegativeInteger">1</owl:maxCardinality>
    </rdf:Description>
    <rdf:Description>
        <owl:maxCardinality rdf:datatype="http://www.w3.org/2001/XMLSchema#nonNegativeInteger">1</owl:maxCardinality>
    </rdf:Description>
    <rdf:Description>
        <owl:cardinality rdf:datatype="http://www.w3.org/2001/XMLSchema#nonNegativeInteger">1</owl:cardinality>
    </rdf:Description>
    <rdf:Description>
        <owl:maxCardinality rdf:datatype="http://www.w3.org/2001/XMLSchema#nonNegativeInteger">1</owl:maxCardinality>
    </rdf:Description>
    <rdf:Description>
        <owl:maxCardinality rdf:datatype="http://www.w3.org/2001/XMLSchema#nonNegativeInteger">1</owl:maxCardinality>
    </rdf:Description>
    <rdf:Description>
        <owl:maxCardinality rdf:datatype="http://www.w3.org/2001/XMLSchema#nonNegativeInteger">1</owl:maxCardinality>
    </rdf:Description>
    <rdf:Description>
        <owl:maxCardinality rdf:datatype="http://www.w3.org/2001/XMLSchema#nonNegativeInteger">1</owl:maxCardinality>
    </rdf:Description>
    <rdf:Description>
        <owl:maxCardinality rdf:datatype="http://www.w3.org/2001/XMLSchema#nonNegativeInteger">1</owl:maxCardinality>
    </rdf:Description>
    <rdf:Description>
        <owl:maxCardinality rdf:datatype="http://www.w3.org/2001/XMLSchema#nonNegativeInteger">1</owl:maxCardinality>
    </rdf:Description>
    <rdf:Description>
        <owl:cardinality rdf:datatype="http://www.w3.org/2001/XMLSchema#nonNegativeInteger">1</owl:cardinality>
    </rdf:Description>
    <rdf:Description>
        <owl:maxCardinality rdf:datatype="http://www.w3.org/2001/XMLSchema#nonNegativeInteger">1</owl:maxCardinality>
    </rdf:Description>
    <rdf:Description>
        <owl:maxCardinality rdf:datatype="http://www.w3.org/2001/XMLSchema#nonNegativeInteger">1</owl:maxCardinality>
    </rdf:Description>
</rdf:RDF>



<!-- Generated by the OWL API (version 4.2.6.20160910-2108) https://github.com/owlcs/owlapi -->

