<?xml version="1.0"?>
<rdf:RDF xmlns="http://cybox.mitre.org/cyboxCommon#"
     xml:base="http://cybox.mitre.org/cyboxCommon"
     xmlns:rdf="http://www.w3.org/1999/02/22-rdf-syntax-ns#"
     xmlns:owl="http://www.w3.org/2002/07/owl#"
     xmlns:xml="http://www.w3.org/XML/1998/namespace"
     xmlns:xsd="http://www.w3.org/2001/XMLSchema#"
     xmlns:ciq_xnl="http://www.oasis-open.org/ciq_xnl#"
     xmlns:wgs84_pos="http://www.w3.org/2003/01/geo/wgs84_pos#"
     xmlns:rdfs="http://www.w3.org/2000/01/rdf-schema#"
     xmlns:cyboxCommon="http://cybox.mitre.org/cyboxCommon#"
     xmlns:foaf="http://xmlns.com/foaf/0.1/"
     xmlns:dc="http://purl.org/dc/elements/1.1/">
    <owl:Ontology rdf:about="http://cybox.mitre.org/cyboxCommon">
        <owl:imports rdf:resource="http://cpe.mitre.org/cpe"/>
        <owl:imports rdf:resource="http://www.oasis-open.org/ciq_xal"/>
        <owl:imports rdf:resource="http://cybox.mitre.org/objects/Process"/>
        <owl:imports rdf:resource="http://www.oasis-open.org/ciq_xpil"/>
        <rdfs:label>Cyber Observable eXpression (CybOX) Common Types Ontology</rdfs:label>
        <rdfs:comment>This ontology provides a vocabulary and representation for the  Cyber Observable eXpression (CybOX) core types.  

CybOX provides a common mechansim (structure and content) for addressing cyber observables across and among this full range of use cases improving consistency, efficiency, interoperability,and overall situational awareness.

Copyright (c) 2014, DaedaFusion, LLC.  All rights reserved.</rdfs:comment>
        <owl:versionInfo rdf:datatype="http://www.w3.org/2001/XMLSchema#string">1.0.0-000</owl:versionInfo>
    </owl:Ontology>
    


    <!-- 
    ///////////////////////////////////////////////////////////////////////////////////////
    //
    // Datatypes
    //
    ///////////////////////////////////////////////////////////////////////////////////////
     -->

    


    <!-- http://www.w3.org/2001/XMLSchema#anySimpleType -->

    <rdfs:Datatype rdf:about="http://www.w3.org/2001/XMLSchema#anySimpleType"/>
    


    <!-- http://www.w3.org/2001/XMLSchema#date -->

    <rdfs:Datatype rdf:about="http://www.w3.org/2001/XMLSchema#date"/>
    


    <!-- 
    ///////////////////////////////////////////////////////////////////////////////////////
    //
    // Object Properties
    //
    ///////////////////////////////////////////////////////////////////////////////////////
     -->

    


    <!-- http://cybox.mitre.org/cyboxCommon#blockHash.segments -->

    <owl:ObjectProperty rdf:about="http://cybox.mitre.org/cyboxCommon#blockHash.segments">
        <rdfs:range rdf:resource="http://cybox.mitre.org/cyboxCommon#HashSegment"/>
        <rdfs:comment>Specifies a single segment identified and utilized within this fuzzy hash calculation.</rdfs:comment>
        <rdfs:isDefinedBy rdf:resource="http://cybox.mitre.org/cyboxCommon"/>
        <rdfs:label>Segments</rdfs:label>
    </owl:ObjectProperty>
    


    <!-- http://cybox.mitre.org/cyboxCommon#buildInfo.buildUtilityPlatformSpecification -->

    <owl:ObjectProperty rdf:about="http://cybox.mitre.org/cyboxCommon#buildInfo.buildUtilityPlatformSpecification">
        <rdfs:range>
            <owl:Class>
                <owl:unionOf rdf:parseType="Collection">
                    <rdf:Description rdf:about="http://cpe.mitre.org/cpe#Platform"/>
                    <rdf:Description rdf:about="http://cybox.mitre.org/cyboxCommon#PlatformSpecification"/>
                </owl:unionOf>
            </owl:Class>
        </rdfs:range>
        <rdfs:comment>Specifies the build utility used to build this application.</rdfs:comment>
        <rdfs:isDefinedBy rdf:resource="http://cybox.mitre.org/cyboxCommon"/>
        <rdfs:label>Build Utility Platform Specification</rdfs:label>
    </owl:ObjectProperty>
    


    <!-- http://cybox.mitre.org/cyboxCommon#buildInfo.compilers -->

    <owl:ObjectProperty rdf:about="http://cybox.mitre.org/cyboxCommon#buildInfo.compilers">
        <rdfs:range rdf:resource="http://cybox.mitre.org/cyboxCommon#Compiler"/>
        <rdfs:comment>Specifies the compilers utilized during this build of this application.</rdfs:comment>
        <rdfs:isDefinedBy rdf:resource="http://cybox.mitre.org/cyboxCommon"/>
        <rdfs:label>Build Compilers</rdfs:label>
    </owl:ObjectProperty>
    


    <!-- http://cybox.mitre.org/cyboxCommon#buildInfo.configurationSettings -->

    <owl:ObjectProperty rdf:about="http://cybox.mitre.org/cyboxCommon#buildInfo.configurationSettings">
        <rdfs:range rdf:resource="http://cybox.mitre.org/cyboxCommon#ConfigurationSetting"/>
        <rdfs:comment>Specifies the configuration settings for this build of this application instance.</rdfs:comment>
        <rdfs:isDefinedBy rdf:resource="http://cybox.mitre.org/cyboxCommon"/>
        <rdfs:label>Build Configuration Settings</rdfs:label>
    </owl:ObjectProperty>
    


    <!-- http://cybox.mitre.org/cyboxCommon#buildInfo.libraries -->

    <owl:ObjectProperty rdf:about="http://cybox.mitre.org/cyboxCommon#buildInfo.libraries">
        <rdfs:range rdf:resource="http://cybox.mitre.org/cyboxCommon#Library"/>
        <rdfs:comment>Specifies the libraries incorporated into the build of the tool.</rdfs:comment>
        <rdfs:isDefinedBy rdf:resource="http://cybox.mitre.org/cyboxCommon"/>
        <rdfs:label>Build Libraries</rdfs:label>
    </owl:ObjectProperty>
    


    <!-- http://cybox.mitre.org/cyboxCommon#byteRuns -->

    <owl:ObjectProperty rdf:about="http://cybox.mitre.org/cyboxCommon#byteRuns">
        <rdfs:range rdf:resource="http://cybox.mitre.org/cyboxCommon#ByteRun"/>
        <rdfs:comment>Specifies a list of byte runs from the raw file or its storage medium.</rdfs:comment>
        <rdfs:isDefinedBy rdf:resource="http://cybox.mitre.org/cyboxCommon"/>
        <rdfs:label>byte runs</rdfs:label>
    </owl:ObjectProperty>
    


    <!-- http://cybox.mitre.org/cyboxCommon#compiler.platformSpecification -->

    <owl:ObjectProperty rdf:about="http://cybox.mitre.org/cyboxCommon#compiler.platformSpecification">
        <rdfs:range>
            <owl:Class>
                <owl:unionOf rdf:parseType="Collection">
                    <rdf:Description rdf:about="http://cpe.mitre.org/cpe#Platform"/>
                    <rdf:Description rdf:about="http://cybox.mitre.org/cyboxCommon#PlatformSpecification"/>
                </owl:unionOf>
            </owl:Class>
        </rdfs:range>
        <rdfs:comment>Specifies this compiler instance.</rdfs:comment>
        <rdfs:isDefinedBy rdf:resource="http://cybox.mitre.org/cyboxCommon"/>
        <rdfs:label>Platform Specification</rdfs:label>
    </owl:ObjectProperty>
    


    <!-- http://cybox.mitre.org/cyboxCommon#configurationSettings -->

    <owl:ObjectProperty rdf:about="http://cybox.mitre.org/cyboxCommon#configurationSettings">
        <rdfs:range rdf:resource="http://cybox.mitre.org/cyboxCommon#ConfigurationSetting"/>
        <rdfs:comment>Specifies the configuration settings of this tool instance.</rdfs:comment>
        <rdfs:isDefinedBy rdf:resource="http://cybox.mitre.org/cyboxCommon"/>
        <rdfs:label>Configuration Settings</rdfs:label>
    </owl:ObjectProperty>
    


    <!-- http://cybox.mitre.org/cyboxCommon#contributors -->

    <owl:ObjectProperty rdf:about="http://cybox.mitre.org/cyboxCommon#contributors">
        <rdfs:range rdf:resource="http://cybox.mitre.org/cyboxCommon#Contributor"/>
        <rdfs:comment>Specifies a description of the individual contributors involved in this cyber observation source.</rdfs:comment>
        <rdfs:isDefinedBy rdf:resource="http://cybox.mitre.org/cyboxCommon"/>
        <rdfs:label>Contributors</rdfs:label>
    </owl:ObjectProperty>
    


    <!-- http://cybox.mitre.org/cyboxCommon#dependencies -->

    <owl:ObjectProperty rdf:about="http://cybox.mitre.org/cyboxCommon#dependencies">
        <rdfs:range rdf:resource="http://cybox.mitre.org/cyboxCommon#Dependency"/>
        <rdfs:comment>Specifies information describing the relevant dependencies for this tool.</rdfs:comment>
        <rdfs:isDefinedBy rdf:resource="http://cybox.mitre.org/cyboxCommon"/>
        <rdfs:label>Dependencies</rdfs:label>
    </owl:ObjectProperty>
    


    <!-- http://cybox.mitre.org/cyboxCommon#digitalSignatures -->

    <owl:ObjectProperty rdf:about="http://cybox.mitre.org/cyboxCommon#digitalSignatures">
        <rdfs:range rdf:resource="http://cybox.mitre.org/cyboxCommon#DigitalSignature"/>
        <rdfs:comment>Specifies one or more digital signatures for the associated entity</rdfs:comment>
        <rdfs:isDefinedBy rdf:resource="http://cybox.mitre.org/cyboxCommon"/>
        <rdfs:label>Digital Signatures</rdfs:label>
    </owl:ObjectProperty>
    


    <!-- http://cybox.mitre.org/cyboxCommon#environmentVariables -->

    <owl:ObjectProperty rdf:about="http://cybox.mitre.org/cyboxCommon#environmentVariables">
        <rdfs:range rdf:resource="http://cybox.mitre.org/cyboxCommon#EnvironmentVariable"/>
        <rdfs:comment>Specifies any environment variables associated with the process</rdfs:comment>
        <rdfs:isDefinedBy rdf:resource="http://cybox.mitre.org/cyboxCommon"/>
        <rdfs:label>Environment Variables</rdfs:label>
    </owl:ObjectProperty>
    


    <!-- http://cybox.mitre.org/cyboxCommon#errors -->

    <owl:ObjectProperty rdf:about="http://cybox.mitre.org/cyboxCommon#errors">
        <rdfs:range rdf:resource="http://cybox.mitre.org/cyboxCommon#Error"/>
        <rdfs:comment>Specifies any errors generated during the run of the tool.</rdfs:comment>
        <rdfs:isDefinedBy rdf:resource="http://cybox.mitre.org/cyboxCommon"/>
        <rdfs:label>Errors</rdfs:label>
    </owl:ObjectProperty>
    


    <!-- http://cybox.mitre.org/cyboxCommon#executionEnvironment -->

    <owl:ObjectProperty rdf:about="http://cybox.mitre.org/cyboxCommon#executionEnvironment">
        <rdfs:range rdf:resource="http://cybox.mitre.org/cyboxCommon#ExecutionEnvironment"/>
        <rdfs:comment>Specifies information describing the execution environment of the tool.</rdfs:comment>
        <rdfs:isDefinedBy rdf:resource="http://cybox.mitre.org/cyboxCommon"/>
        <rdfs:label>Execution Environment</rdfs:label>
    </owl:ObjectProperty>
    


    <!-- http://cybox.mitre.org/cyboxCommon#extractedFeature.codeSnippets -->

    <owl:ObjectProperty rdf:about="http://cybox.mitre.org/cyboxCommon#extractedFeature.codeSnippets">
        <rdfs:comment>Specifies a set of code snippets extracted from a raw cyber object. 

Instances should be of type codeObj:Code</rdfs:comment>
        <rdfs:isDefinedBy rdf:resource="http://cybox.mitre.org/cyboxCommon"/>
        <rdfs:label>Code Snippets</rdfs:label>
    </owl:ObjectProperty>
    


    <!-- http://cybox.mitre.org/cyboxCommon#extractedFeature.strings -->

    <owl:ObjectProperty rdf:about="http://cybox.mitre.org/cyboxCommon#extractedFeature.strings">
        <rdfs:range rdf:resource="http://cybox.mitre.org/cyboxCommon#ExtractedString"/>
        <rdfs:comment>Specifies a set of static strings extracted from a raw cyber object.</rdfs:comment>
        <rdfs:isDefinedBy rdf:resource="http://cybox.mitre.org/cyboxCommon"/>
        <rdfs:label>Extracted Feature Strings</rdfs:label>
    </owl:ObjectProperty>
    


    <!-- http://cybox.mitre.org/cyboxCommon#fuzzyHashStructure -->

    <owl:ObjectProperty rdf:about="http://cybox.mitre.org/cyboxCommon#fuzzyHashStructure">
        <rdfs:range rdf:resource="http://cybox.mitre.org/cyboxCommon#FuzzyHashStructure"/>
        <rdfs:comment>Specifies the key internal components of a fuzzy hash calculation with a given block size.</rdfs:comment>
        <rdfs:isDefinedBy rdf:resource="http://cybox.mitre.org/cyboxCommon"/>
        <rdfs:label>Suzzy Hash Structure</rdfs:label>
    </owl:ObjectProperty>
    


    <!-- http://cybox.mitre.org/cyboxCommon#hash.details -->

    <owl:ObjectProperty rdf:about="http://cybox.mitre.org/cyboxCommon#hash.details">
        <rdfs:range rdf:resource="http://cybox.mitre.org/cyboxCommon#Hash"/>
        <rdfs:comment>Specifies details about any computed hash values for this the data.</rdfs:comment>
        <rdfs:isDefinedBy rdf:resource="http://cybox.mitre.org/cyboxCommon"/>
        <rdfs:label>Hashes</rdfs:label>
    </owl:ObjectProperty>
    


    <!-- http://cybox.mitre.org/cyboxCommon#identifier -->

    <owl:ObjectProperty rdf:about="http://cybox.mitre.org/cyboxCommon#identifier">
        <rdfs:range rdf:resource="http://cybox.mitre.org/cyboxCommon#PlatformIdentifier"/>
        <rdfs:comment>Specifies a pre-defined name for the given platform using some naming scheme. For example, one could provide a CPE (Common Platform Enumeration) name using the CPE naming format.</rdfs:comment>
        <rdfs:isDefinedBy rdf:resource="http://cybox.mitre.org/cyboxCommon"/>
        <rdfs:label>Identifier</rdfs:label>
    </owl:ObjectProperty>
    


    <!-- http://cybox.mitre.org/cyboxCommon#individualDetails -->

    <owl:ObjectProperty rdf:about="http://cybox.mitre.org/cyboxCommon#individualDetails">
        <rdfs:range rdf:resource="http://www.oasis-open.org/ciq_xpil#Person"/>
        <rdfs:comment>Specifies details about the individual contributor.</rdfs:comment>
        <rdfs:isDefinedBy rdf:resource="http://cybox.mitre.org/cyboxCommon"/>
        <rdfs:label>Individual Details</rdfs:label>
    </owl:ObjectProperty>
    


    <!-- http://cybox.mitre.org/cyboxCommon#internationalizationSettings -->

    <owl:ObjectProperty rdf:about="http://cybox.mitre.org/cyboxCommon#internationalizationSettings">
        <rdfs:range rdf:resource="http://cybox.mitre.org/cyboxCommon#InternalString"/>
        <rdfs:comment>Specifies information describing relevant internationalization setting for this tool.</rdfs:comment>
        <rdfs:isDefinedBy rdf:resource="http://cybox.mitre.org/cyboxCommon"/>
        <rdfs:label>International Settings</rdfs:label>
    </owl:ObjectProperty>
    


    <!-- http://cybox.mitre.org/cyboxCommon#locationAddress -->

    <owl:ObjectProperty rdf:about="http://cybox.mitre.org/cyboxCommon#locationAddress">
        <rdfs:range rdf:resource="http://www.oasis-open.org/ciq_xal#Address"/>
        <rdfs:comment></rdfs:comment>
        <rdfs:isDefinedBy rdf:resource="http://cybox.mitre.org/cyboxCommon"/>
        <rdfs:label>Location Address</rdfs:label>
    </owl:ObjectProperty>
    


    <!-- http://cybox.mitre.org/cyboxCommon#locationDetails -->

    <owl:ObjectProperty rdf:about="http://cybox.mitre.org/cyboxCommon#locationDetails">
        <rdfs:range rdf:resource="http://www.oasis-open.org/ciq_xal#Address"/>
        <rdfs:comment>Specifies detailed information describing the location at which the contributory activity occured.</rdfs:comment>
        <rdfs:isDefinedBy rdf:resource="http://cybox.mitre.org/cyboxCommon"/>
        <rdfs:label>Location Details</rdfs:label>
    </owl:ObjectProperty>
    


    <!-- http://cybox.mitre.org/cyboxCommon#metadata -->

    <owl:ObjectProperty rdf:about="http://cybox.mitre.org/cyboxCommon#metadata">
        <rdfs:range rdf:resource="http://cybox.mitre.org/cyboxCommon#Metadata"/>
        <rdfs:comment>Specifies other relevant metadata including tool-specific fields.</rdfs:comment>
        <rdfs:isDefinedBy rdf:resource="http://cybox.mitre.org/cyboxCommon"/>
        <rdfs:label>Metadata</rdfs:label>
    </owl:ObjectProperty>
    


    <!-- http://cybox.mitre.org/cyboxCommon#metadataSubdatum -->

    <owl:ObjectProperty rdf:about="http://cybox.mitre.org/cyboxCommon#metadataSubdatum">
        <rdfs:range rdf:resource="http://cybox.mitre.org/cyboxCommon#Metadata"/>
        <rdfs:comment>Specifies subdatum structures for this metadata field.</rdfs:comment>
        <rdfs:isDefinedBy rdf:resource="http://cybox.mitre.org/cyboxCommon"/>
        <rdfs:label>SubDatum</rdfs:label>
    </owl:ObjectProperty>
    


    <!-- http://cybox.mitre.org/cyboxCommon#observableLocation -->

    <owl:ObjectProperty rdf:about="http://cybox.mitre.org/cyboxCommon#observableLocation">
        <rdfs:range rdf:resource="http://www.oasis-open.org/ciq_xal#Address"/>
        <rdfs:comment>Specifies a relevant physical location for the associated Observable.</rdfs:comment>
        <rdfs:isDefinedBy rdf:resource="http://cybox.mitre.org/cyboxCommon"/>
        <rdfs:label>Observable Location</rdfs:label>
    </owl:ObjectProperty>
    


    <!-- http://cybox.mitre.org/cyboxCommon#observationLocation -->

    <owl:ObjectProperty rdf:about="http://cybox.mitre.org/cyboxCommon#observationLocation">
        <rdfs:range rdf:resource="http://www.oasis-open.org/ciq_xal#Address"/>
        <rdfs:comment>Specifies a relevant physical location for the observation measurement of the associated Observable.</rdfs:comment>
        <rdfs:isDefinedBy rdf:resource="http://cybox.mitre.org/cyboxCommon"/>
        <rdfs:label>Observation Location</rdfs:label>
    </owl:ObjectProperty>
    


    <!-- http://cybox.mitre.org/cyboxCommon#organizationDetails -->

    <owl:ObjectProperty rdf:about="http://cybox.mitre.org/cyboxCommon#organizationDetails">
        <rdfs:range rdf:resource="http://www.oasis-open.org/ciq_xpil#Organization"/>
        <rdfs:comment>Specifies details about the contributor&apos;s organization.</rdfs:comment>
        <rdfs:isDefinedBy rdf:resource="http://cybox.mitre.org/cyboxCommon"/>
        <rdfs:label>Organization Details</rdfs:label>
    </owl:ObjectProperty>
    


    <!-- http://cybox.mitre.org/cyboxCommon#platform -->

    <owl:ObjectProperty rdf:about="http://cybox.mitre.org/cyboxCommon#platform">
        <rdfs:range>
            <owl:Class>
                <owl:unionOf rdf:parseType="Collection">
                    <rdf:Description rdf:about="http://cpe.mitre.org/cpe#Platform"/>
                    <rdf:Description rdf:about="http://cybox.mitre.org/cyboxCommon#PlatformSpecification"/>
                </owl:unionOf>
            </owl:Class>
        </rdfs:range>
        <rdfs:comment>Specifies a formal, standardized specification of the platform for this cyber observation source.</rdfs:comment>
        <rdfs:isDefinedBy rdf:resource="http://cybox.mitre.org/cyboxCommon"/>
        <rdfs:label>Platform</rdfs:label>
    </owl:ObjectProperty>
    


    <!-- http://cybox.mitre.org/cyboxCommon#processInstance -->

    <owl:ObjectProperty rdf:about="http://cybox.mitre.org/cyboxCommon#processInstance">
        <rdfs:range rdf:resource="http://cybox.mitre.org/objects/Process#Process"/>
        <rdfs:comment>Specifies the process instance in which the mechanism of cyber observation executed. 

Instance should be of type ProcessObj:ProcessObjectType.</rdfs:comment>
        <rdfs:isDefinedBy rdf:resource="http://cybox.mitre.org/cyboxCommon"/>
        <rdfs:label>Process Instance</rdfs:label>
    </owl:ObjectProperty>
    


    <!-- http://cybox.mitre.org/cyboxCommon#processInstance.customProperties -->

    <owl:ObjectProperty rdf:about="http://cybox.mitre.org/cyboxCommon#processInstance.customProperties">
        <rdfs:range rdf:resource="http://cybox.mitre.org/cyboxCommon#Property"/>
        <rdfs:comment>Specifies a set of custom Object Properties that may not be defined in existing Properties schemas.</rdfs:comment>
        <rdfs:isDefinedBy rdf:resource="http://cybox.mitre.org/cyboxCommon"/>
        <rdfs:label>Process Instance Custom Properties</rdfs:label>
    </owl:ObjectProperty>
    


    <!-- http://cybox.mitre.org/cyboxCommon#system -->

    <owl:ObjectProperty rdf:about="http://cybox.mitre.org/cyboxCommon#system">
        <rdfs:range rdf:resource="http://cybox.mitre.org/objects/System#System"/>
        <rdfs:comment>Specifies information describing the system on which the tool was executed.</rdfs:comment>
        <rdfs:isDefinedBy rdf:resource="http://cybox.mitre.org/cyboxCommon"/>
        <rdfs:label>System</rdfs:label>
    </owl:ObjectProperty>
    


    <!-- http://cybox.mitre.org/cyboxCommon#toolConfiguration -->

    <owl:ObjectProperty rdf:about="http://cybox.mitre.org/cyboxCommon#toolConfiguration">
        <rdfs:range rdf:resource="http://cybox.mitre.org/cyboxCommon#ToolConfiguration"/>
        <rdfs:comment>Specifies information describing the configuration and usage of the tool.</rdfs:comment>
        <rdfs:isDefinedBy rdf:resource="http://cybox.mitre.org/cyboxCommon"/>
        <rdfs:label>Configuration</rdfs:label>
    </owl:ObjectProperty>
    


    <!-- http://cybox.mitre.org/cyboxCommon#toolHash.details -->

    <owl:ObjectProperty rdf:about="http://cybox.mitre.org/cyboxCommon#toolHash.details">
        <rdfs:range rdf:resource="http://cybox.mitre.org/cyboxCommon#Hash"/>
        <rdfs:comment>Specifies details about hash values computed on the tool file content in order to verify its integrity.</rdfs:comment>
        <rdfs:isDefinedBy rdf:resource="http://cybox.mitre.org/cyboxCommon"/>
        <rdfs:label>Tool Hash Details</rdfs:label>
    </owl:ObjectProperty>
    


    <!-- http://cybox.mitre.org/cyboxCommon#toolReferences -->

    <owl:ObjectProperty rdf:about="http://cybox.mitre.org/cyboxCommon#toolReferences">
        <rdfs:range rdf:resource="http://cybox.mitre.org/cyboxCommon#ToolReference"/>
        <rdfs:comment>Specifies references to instances or additional information for this tool.</rdfs:comment>
        <rdfs:isDefinedBy rdf:resource="http://cybox.mitre.org/cyboxCommon"/>
        <rdfs:label>Tool References</rdfs:label>
    </owl:ObjectProperty>
    


    <!-- http://cybox.mitre.org/cyboxCommon#toolSpecificData -->

    <owl:ObjectProperty rdf:about="http://cybox.mitre.org/cyboxCommon#toolSpecificData"/>
    


    <!-- http://cybox.mitre.org/cyboxCommon#tools -->

    <owl:ObjectProperty rdf:about="http://cybox.mitre.org/cyboxCommon#tools">
        <rdfs:range rdf:resource="http://cybox.mitre.org/cyboxCommon#ToolInformation"/>
        <rdfs:comment>Specifies a description of a set of automated tools.</rdfs:comment>
        <rdfs:isDefinedBy rdf:resource="http://cybox.mitre.org/cyboxCommon"/>
        <rdfs:label>Tools</rdfs:label>
    </owl:ObjectProperty>
    


    <!-- http://cybox.mitre.org/cyboxCommon#userAccount -->

    <owl:ObjectProperty rdf:about="http://cybox.mitre.org/cyboxCommon#userAccount">
        <rdfs:range rdf:resource="http://cybox.mitre.org/objects/Account#UserAccount"/>
        <rdfs:comment>Specifies the user account that executed the tool. 

userAccount should be an instance of type UserAccountObj:UserAccountObjectType.</rdfs:comment>
        <rdfs:isDefinedBy rdf:resource="http://cybox.mitre.org/cyboxCommon"/>
        <rdfs:label>User Account</rdfs:label>
    </owl:ObjectProperty>
    


    <!-- http://cybox.mitre.org/cyboxCommon#vendor -->

    <owl:ObjectProperty rdf:about="http://cybox.mitre.org/cyboxCommon#vendor">
        <rdfs:range rdf:resource="http://www.oasis-open.org/ciq_xpil#Organization"/>
        <rdfs:comment>Specifies information identifying the vendor organization for this tool.</rdfs:comment>
        <rdfs:isDefinedBy rdf:resource="http://cybox.mitre.org/cyboxCommon"/>
        <rdfs:label>Vendor</rdfs:label>
    </owl:ObjectProperty>
    


    <!-- 
    ///////////////////////////////////////////////////////////////////////////////////////
    //
    // Data properties
    //
    ///////////////////////////////////////////////////////////////////////////////////////
     -->

    


    <!-- http://cybox.mitre.org/cyboxCommon#blockHash.fuzzyHashValue -->

    <owl:DatatypeProperty rdf:about="http://cybox.mitre.org/cyboxCommon#blockHash.fuzzyHashValue">
        <rdfs:range rdf:resource="http://www.w3.org/2001/XMLSchema#string"/>
        <rdfs:comment>Specifies a fuzzy hash calculation result value for this Block specified a single result value of a cryptograhic fuzzy hash function outputting a single complex string based hash value. (e.g. SSDEEP&apos;s Block1hash:Block2hash format).</rdfs:comment>
        <rdfs:isDefinedBy rdf:resource="http://cybox.mitre.org/cyboxCommon"/>
        <rdfs:label>Block Hash Value Fuzzy Hash Value</rdfs:label>
    </owl:DatatypeProperty>
    


    <!-- http://cybox.mitre.org/cyboxCommon#blockHash.segmentCount -->

    <owl:DatatypeProperty rdf:about="http://cybox.mitre.org/cyboxCommon#blockHash.segmentCount">
        <rdfs:range rdf:resource="http://www.w3.org/2001/XMLSchema#integer"/>
        <rdfs:comment>Specifies the number of segments identified and utilized within this fuzzy hash calculation.</rdfs:comment>
        <rdfs:isDefinedBy rdf:resource="http://cybox.mitre.org/cyboxCommon"/>
        <rdfs:label>block hash.segment count</rdfs:label>
    </owl:DatatypeProperty>
    


    <!-- http://cybox.mitre.org/cyboxCommon#blockHash.simpleHashValue -->

    <owl:DatatypeProperty rdf:about="http://cybox.mitre.org/cyboxCommon#blockHash.simpleHashValue">
        <rdfs:range rdf:resource="http://www.w3.org/2001/XMLSchema#string"/>
        <rdfs:comment>Specifies a fuzzy hash calculation result value for this Block. Specifies a single result value of a basic cryptograhic hash function outputting a single hexbinary hash value.</rdfs:comment>
        <rdfs:isDefinedBy rdf:resource="http://cybox.mitre.org/cyboxCommon"/>
        <rdfs:label>Block Hash Value</rdfs:label>
    </owl:DatatypeProperty>
    


    <!-- http://cybox.mitre.org/cyboxCommon#blockSize -->

    <owl:DatatypeProperty rdf:about="http://cybox.mitre.org/cyboxCommon#blockSize">
        <rdfs:range rdf:resource="http://www.w3.org/2001/XMLSchema#integer"/>
        <rdfs:comment>Specifies the calculated block size for this fuzzy hash calculation.</rdfs:comment>
        <rdfs:isDefinedBy rdf:resource="http://cybox.mitre.org/cyboxCommon"/>
        <rdfs:label>Block Size</rdfs:label>
    </owl:DatatypeProperty>
    


    <!-- http://cybox.mitre.org/cyboxCommon#buildInfo.buildScript -->

    <owl:DatatypeProperty rdf:about="http://cybox.mitre.org/cyboxCommon#buildInfo.buildScript">
        <rdfs:range rdf:resource="http://www.w3.org/2001/XMLSchema#string"/>
        <rdfs:comment>Specifies the actual build script for this build of this application instance.</rdfs:comment>
        <rdfs:isDefinedBy rdf:resource="http://cybox.mitre.org/cyboxCommon"/>
        <rdfs:label>Build Script</rdfs:label>
    </owl:DatatypeProperty>
    


    <!-- http://cybox.mitre.org/cyboxCommon#buildInfo.buildUtilityName -->

    <owl:DatatypeProperty rdf:about="http://cybox.mitre.org/cyboxCommon#buildInfo.buildUtilityName">
        <rdfs:range rdf:resource="http://www.w3.org/2001/XMLSchema#string"/>
        <rdfs:comment>Specifies the informally defined name of the utility used to build this application instance.</rdfs:comment>
        <rdfs:isDefinedBy rdf:resource="http://cybox.mitre.org/cyboxCommon"/>
        <rdfs:label>Build Utility Name</rdfs:label>
    </owl:DatatypeProperty>
    


    <!-- http://cybox.mitre.org/cyboxCommon#buildInfo.compilationDate -->

    <owl:DatatypeProperty rdf:about="http://cybox.mitre.org/cyboxCommon#buildInfo.compilationDate">
        <rdfs:range rdf:resource="http://www.w3.org/2001/XMLSchema#dateTime"/>
        <rdfs:comment>Specifies the compilation date for the build of the tool. 

In order to avoid ambiguity, it is strongly suggest that all timestamps in this field include a specification of the timezone if it is known.</rdfs:comment>
        <rdfs:isDefinedBy rdf:resource="http://cybox.mitre.org/cyboxCommon"/>
        <rdfs:label>Build Compilation Date</rdfs:label>
    </owl:DatatypeProperty>
    


    <!-- http://cybox.mitre.org/cyboxCommon#buildInfo.configurationSettingDescription -->

    <owl:DatatypeProperty rdf:about="http://cybox.mitre.org/cyboxCommon#buildInfo.configurationSettingDescription">
        <rdfs:range rdf:resource="http://www.w3.org/2001/XMLSchema#string"/>
        <rdfs:comment>Specifies a description of the configuration settings for this build of this application instance.</rdfs:comment>
        <rdfs:isDefinedBy rdf:resource="http://cybox.mitre.org/cyboxCommon"/>
        <rdfs:label>Build Configuration Description</rdfs:label>
    </owl:DatatypeProperty>
    


    <!-- http://cybox.mitre.org/cyboxCommon#buildInfo.id -->

    <owl:DatatypeProperty rdf:about="http://cybox.mitre.org/cyboxCommon#buildInfo.id">
        <rdfs:range rdf:resource="http://www.w3.org/2001/XMLSchema#string"/>
        <rdfs:comment>Specifies an externally defined unique identifier of this build of this application instance.</rdfs:comment>
        <rdfs:isDefinedBy rdf:resource="http://cybox.mitre.org/cyboxCommon"/>
        <rdfs:label>Build Identifier</rdfs:label>
    </owl:DatatypeProperty>
    


    <!-- http://cybox.mitre.org/cyboxCommon#buildInfo.label -->

    <owl:DatatypeProperty rdf:about="http://cybox.mitre.org/cyboxCommon#buildInfo.label">
        <rdfs:range rdf:resource="http://www.w3.org/2001/XMLSchema#string"/>
        <rdfs:comment>Specifies any relevant label for this build of this application instance.</rdfs:comment>
        <rdfs:isDefinedBy rdf:resource="http://cybox.mitre.org/cyboxCommon"/>
        <rdfs:label>Build Label</rdfs:label>
    </owl:DatatypeProperty>
    


    <!-- http://cybox.mitre.org/cyboxCommon#buildInfo.outputLog -->

    <owl:DatatypeProperty rdf:about="http://cybox.mitre.org/cyboxCommon#buildInfo.outputLog">
        <rdfs:range rdf:resource="http://www.w3.org/2001/XMLSchema#string"/>
        <rdfs:comment>Specifies a capture of the output log of the build process.</rdfs:comment>
        <rdfs:isDefinedBy rdf:resource="http://cybox.mitre.org/cyboxCommon"/>
        <rdfs:label>Build Output Log</rdfs:label>
    </owl:DatatypeProperty>
    


    <!-- http://cybox.mitre.org/cyboxCommon#buildInfo.project -->

    <owl:DatatypeProperty rdf:about="http://cybox.mitre.org/cyboxCommon#buildInfo.project">
        <rdfs:range rdf:resource="http://www.w3.org/2001/XMLSchema#string"/>
        <rdfs:comment>Specifies the project name of this build of this application instance.</rdfs:comment>
        <rdfs:isDefinedBy rdf:resource="http://cybox.mitre.org/cyboxCommon"/>
        <rdfs:label>Build Project Name</rdfs:label>
    </owl:DatatypeProperty>
    


    <!-- http://cybox.mitre.org/cyboxCommon#buildInfo.version -->

    <owl:DatatypeProperty rdf:about="http://cybox.mitre.org/cyboxCommon#buildInfo.version">
        <rdfs:range rdf:resource="http://www.w3.org/2001/XMLSchema#string"/>
        <rdfs:comment>Specifies the build utility used to build this application.</rdfs:comment>
        <rdfs:isDefinedBy rdf:resource="http://cybox.mitre.org/cyboxCommon"/>
        <rdfs:label>build Version</rdfs:label>
    </owl:DatatypeProperty>
    


    <!-- http://cybox.mitre.org/cyboxCommon#byteOrder -->

    <owl:DatatypeProperty rdf:about="http://cybox.mitre.org/cyboxCommon#byteOrder">
        <rdfs:range rdf:resource="http://www.w3.org/2001/XMLSchema#string"/>
        <rdfs:comment>Specifies the endianness of the unpacked (e.g., decoded, unencrypted, etc.) data stored within the DataSegment.</rdfs:comment>
        <rdfs:isDefinedBy rdf:resource="http://cybox.mitre.org/cyboxCommon"/>
        <rdfs:label>Byte Order</rdfs:label>
    </owl:DatatypeProperty>
    


    <!-- http://cybox.mitre.org/cyboxCommon#byteRunData -->

    <owl:DatatypeProperty rdf:about="http://cybox.mitre.org/cyboxCommon#byteRunData">
        <rdfs:range rdf:resource="http://www.w3.org/2001/XMLSchema#anySimpleType"/>
        <rdfs:comment>Specifies a raw dump of the byte run data, typically enclosed within an XML CDATA section.</rdfs:comment>
        <rdfs:isDefinedBy rdf:resource="http://cybox.mitre.org/cyboxCommon"/>
        <rdfs:label>Byterun Data</rdfs:label>
    </owl:DatatypeProperty>
    


    <!-- http://cybox.mitre.org/cyboxCommon#byteRunLength -->

    <owl:DatatypeProperty rdf:about="http://cybox.mitre.org/cyboxCommon#byteRunLength">
        <rdfs:range rdf:resource="http://www.w3.org/2001/XMLSchema#integer"/>
        <rdfs:comment>Specifies the lenght of the byte run</rdfs:comment>
        <rdfs:isDefinedBy rdf:resource="http://cybox.mitre.org/cyboxCommon"/>
        <rdfs:label>Byterun Length</rdfs:label>
    </owl:DatatypeProperty>
    


    <!-- http://cybox.mitre.org/cyboxCommon#byteStringValue -->

    <owl:DatatypeProperty rdf:about="http://cybox.mitre.org/cyboxCommon#byteStringValue">
        <rdfs:range rdf:resource="http://www.w3.org/2001/XMLSchema#hexBinary"/>
        <rdfs:comment>Specifies the raw, byte-string representation of the string extracted from the CybOX object, in hexadecimal format.</rdfs:comment>
        <rdfs:isDefinedBy rdf:resource="http://cybox.mitre.org/cyboxCommon"/>
        <rdfs:label>Byte String Value</rdfs:label>
    </owl:DatatypeProperty>
    


    <!-- http://cybox.mitre.org/cyboxCommon#certificateIssuer -->

    <owl:DatatypeProperty rdf:about="http://cybox.mitre.org/cyboxCommon#certificateIssuer">
        <rdfs:range rdf:resource="http://www.w3.org/2001/XMLSchema#string"/>
        <rdfs:comment>Specifies the certificate issuer of the digital signature.</rdfs:comment>
        <rdfs:isDefinedBy rdf:resource="http://cybox.mitre.org/cyboxCommon"/>
        <rdfs:label>Certificate Issuer</rdfs:label>
    </owl:DatatypeProperty>
    


    <!-- http://cybox.mitre.org/cyboxCommon#certificateSubject -->

    <owl:DatatypeProperty rdf:about="http://cybox.mitre.org/cyboxCommon#certificateSubject">
        <rdfs:range rdf:resource="http://www.w3.org/2001/XMLSchema#string"/>
        <rdfs:comment>Specifies the certificate subject of the digital signature.</rdfs:comment>
        <rdfs:isDefinedBy rdf:resource="http://cybox.mitre.org/cyboxCommon"/>
        <rdfs:label>Certificate Subject</rdfs:label>
    </owl:DatatypeProperty>
    


    <!-- http://cybox.mitre.org/cyboxCommon#commandLine -->

    <owl:DatatypeProperty rdf:about="http://cybox.mitre.org/cyboxCommon#commandLine">
        <rdfs:range rdf:resource="http://www.w3.org/2001/XMLSchema#string"/>
        <rdfs:comment>Specifies the command line string used to run the tool.</rdfs:comment>
        <rdfs:isDefinedBy rdf:resource="http://cybox.mitre.org/cyboxCommon"/>
        <rdfs:label>Command Line</rdfs:label>
    </owl:DatatypeProperty>
    


    <!-- http://cybox.mitre.org/cyboxCommon#compensationModel -->

    <owl:DatatypeProperty rdf:about="http://cybox.mitre.org/cyboxCommon#compensationModel">
        <rdfs:range>
            <rdfs:Datatype>
                <owl:oneOf>
                    <rdf:Description>
                        <rdf:type rdf:resource="http://www.w3.org/1999/02/22-rdf-syntax-ns#List"/>
                        <rdf:first rdf:datatype="http://www.w3.org/2001/XMLSchema#string">Adware</rdf:first>
                        <rdf:rest>
                            <rdf:Description>
                                <rdf:type rdf:resource="http://www.w3.org/1999/02/22-rdf-syntax-ns#List"/>
                                <rdf:first rdf:datatype="http://www.w3.org/2001/XMLSchema#string">Commercial</rdf:first>
                                <rdf:rest>
                                    <rdf:Description>
                                        <rdf:type rdf:resource="http://www.w3.org/1999/02/22-rdf-syntax-ns#List"/>
                                        <rdf:first rdf:datatype="http://www.w3.org/2001/XMLSchema#string">Freeware</rdf:first>
                                        <rdf:rest>
                                            <rdf:Description>
                                                <rdf:type rdf:resource="http://www.w3.org/1999/02/22-rdf-syntax-ns#List"/>
                                                <rdf:first rdf:datatype="http://www.w3.org/2001/XMLSchema#string">Shareware</rdf:first>
                                                <rdf:rest rdf:resource="http://www.w3.org/1999/02/22-rdf-syntax-ns#nil"/>
                                            </rdf:Description>
                                        </rdf:rest>
                                    </rdf:Description>
                                </rdf:rest>
                            </rdf:Description>
                        </rdf:rest>
                    </rdf:Description>
                </owl:oneOf>
            </rdfs:Datatype>
        </rdfs:range>
        <rdfs:comment>Specifies the name of the compensation model used for the tool.</rdfs:comment>
        <rdfs:isDefinedBy rdf:resource="http://cybox.mitre.org/cyboxCommon"/>
        <rdfs:label>Compensation Model</rdfs:label>
    </owl:DatatypeProperty>
    


    <!-- http://cybox.mitre.org/cyboxCommon#compilerName -->

    <owl:DatatypeProperty rdf:about="http://cybox.mitre.org/cyboxCommon#compilerName">
        <rdfs:range rdf:resource="http://www.w3.org/2001/XMLSchema#string"/>
        <rdfs:comment>Specifies the name of the compiler.</rdfs:comment>
        <rdfs:isDefinedBy rdf:resource="http://cybox.mitre.org/cyboxCommon"/>
        <rdfs:label>Name</rdfs:label>
    </owl:DatatypeProperty>
    


    <!-- http://cybox.mitre.org/cyboxCommon#compilerVersion -->

    <owl:DatatypeProperty rdf:about="http://cybox.mitre.org/cyboxCommon#compilerVersion">
        <rdfs:range rdf:resource="http://www.w3.org/2001/XMLSchema#string"/>
        <rdfs:comment>Specifies the version of the compiler.</rdfs:comment>
        <rdfs:isDefinedBy rdf:resource="http://cybox.mitre.org/cyboxCommon"/>
        <rdfs:label>Version</rdfs:label>
    </owl:DatatypeProperty>
    


    <!-- http://cybox.mitre.org/cyboxCommon#content -->

    <owl:DatatypeProperty rdf:about="http://cybox.mitre.org/cyboxCommon#content">
        <rdfs:range rdf:resource="http://www.w3.org/2001/XMLSchema#string"/>
        <rdfs:comment>Specifies the actual content of this internal string instance.</rdfs:comment>
        <rdfs:isDefinedBy rdf:resource="http://cybox.mitre.org/cyboxCommon"/>
        <rdfs:label>Content</rdfs:label>
    </owl:DatatypeProperty>
    


    <!-- http://cybox.mitre.org/cyboxCommon#contributionEndDate -->

    <owl:DatatypeProperty rdf:about="http://cybox.mitre.org/cyboxCommon#contributionEndDate">
        <rdfs:range rdf:resource="http://www.w3.org/2001/XMLSchema#date"/>
        <rdfs:comment>Specifies the end date for this contributor&apos;s involvement.</rdfs:comment>
        <rdfs:isDefinedBy rdf:resource="http://cybox.mitre.org/cyboxCommon"/>
        <rdfs:label>Contribution End Date</rdfs:label>
    </owl:DatatypeProperty>
    


    <!-- http://cybox.mitre.org/cyboxCommon#contributionLocation -->

    <owl:DatatypeProperty rdf:about="http://cybox.mitre.org/cyboxCommon#contributionLocation">
        <rdfs:range rdf:resource="http://www.w3.org/2001/XMLSchema#string"/>
        <rdfs:comment>Specifies information describing the location at which the contributory activity occured.</rdfs:comment>
        <rdfs:isDefinedBy rdf:resource="http://cybox.mitre.org/cyboxCommon"/>
        <rdfs:label>Location</rdfs:label>
    </owl:DatatypeProperty>
    


    <!-- http://cybox.mitre.org/cyboxCommon#contributionStartDate -->

    <owl:DatatypeProperty rdf:about="http://cybox.mitre.org/cyboxCommon#contributionStartDate">
        <rdfs:range rdf:resource="http://www.w3.org/2001/XMLSchema#date"/>
        <rdfs:comment>Specifies the start date for this contributor&apos;s involvement.</rdfs:comment>
        <rdfs:isDefinedBy rdf:resource="http://cybox.mitre.org/cyboxCommon"/>
        <rdfs:label>Contribution Start Date</rdfs:label>
    </owl:DatatypeProperty>
    


    <!-- http://cybox.mitre.org/cyboxCommon#contributorEmail -->

    <owl:DatatypeProperty rdf:about="http://cybox.mitre.org/cyboxCommon#contributorEmail">
        <rdfs:range rdf:resource="http://www.w3.org/2001/XMLSchema#string"/>
        <rdfs:comment>Specifies the email of this contributor.</rdfs:comment>
        <rdfs:isDefinedBy rdf:resource="http://cybox.mitre.org/cyboxCommon"/>
        <rdfs:label>Email</rdfs:label>
    </owl:DatatypeProperty>
    


    <!-- http://cybox.mitre.org/cyboxCommon#contributorName -->

    <owl:DatatypeProperty rdf:about="http://cybox.mitre.org/cyboxCommon#contributorName">
        <rdfs:range rdf:resource="http://www.w3.org/2001/XMLSchema#string"/>
        <rdfs:comment>Specifies the name of this contributor.</rdfs:comment>
        <rdfs:isDefinedBy rdf:resource="http://cybox.mitre.org/cyboxCommon"/>
        <rdfs:label>Name</rdfs:label>
    </owl:DatatypeProperty>
    


    <!-- http://cybox.mitre.org/cyboxCommon#contributorOrganization -->

    <owl:DatatypeProperty rdf:about="http://cybox.mitre.org/cyboxCommon#contributorOrganization">
        <rdfs:range rdf:resource="http://www.w3.org/2001/XMLSchema#string"/>
        <rdfs:comment>Specifies the organization name of this contributor.</rdfs:comment>
        <rdfs:isDefinedBy rdf:resource="http://cybox.mitre.org/cyboxCommon"/>
        <rdfs:label>Organization Name</rdfs:label>
    </owl:DatatypeProperty>
    


    <!-- http://cybox.mitre.org/cyboxCommon#contributorPhone -->

    <owl:DatatypeProperty rdf:about="http://cybox.mitre.org/cyboxCommon#contributorPhone">
        <rdfs:range rdf:resource="http://www.w3.org/2001/XMLSchema#string"/>
        <rdfs:comment>Specifies  a telephone number of this contributor.</rdfs:comment>
        <rdfs:isDefinedBy rdf:resource="http://cybox.mitre.org/cyboxCommon"/>
        <rdfs:label>Phone Number</rdfs:label>
    </owl:DatatypeProperty>
    


    <!-- http://cybox.mitre.org/cyboxCommon#contributorRole -->

    <owl:DatatypeProperty rdf:about="http://cybox.mitre.org/cyboxCommon#contributorRole">
        <rdfs:range rdf:resource="http://www.w3.org/2001/XMLSchema#string"/>
        <rdfs:comment>Specifies the role played by this contributor.</rdfs:comment>
        <rdfs:label>Role</rdfs:label>
    </owl:DatatypeProperty>
    


    <!-- http://cybox.mitre.org/cyboxCommon#creationDateTime -->

    <owl:DatatypeProperty rdf:about="http://cybox.mitre.org/cyboxCommon#creationDateTime">
        <rdfs:range rdf:resource="http://www.w3.org/2001/XMLSchema#dateTime"/>
        <rdfs:comment>Specifies the date/time at which the entity was created.</rdfs:comment>
        <rdfs:isDefinedBy rdf:resource="http://cybox.mitre.org/cyboxCommon"/>
        <rdfs:label>Creation Time</rdfs:label>
    </owl:DatatypeProperty>
    


    <!-- http://cybox.mitre.org/cyboxCommon#dataFormat -->

    <owl:DatatypeProperty rdf:about="http://cybox.mitre.org/cyboxCommon#dataFormat">
        <rdfs:range>
            <rdfs:Datatype>
                <owl:oneOf>
                    <rdf:Description>
                        <rdf:type rdf:resource="http://www.w3.org/1999/02/22-rdf-syntax-ns#List"/>
                        <rdf:first rdf:datatype="http://www.w3.org/2001/XMLSchema#string">Binary</rdf:first>
                        <rdf:rest>
                            <rdf:Description>
                                <rdf:type rdf:resource="http://www.w3.org/1999/02/22-rdf-syntax-ns#List"/>
                                <rdf:first rdf:datatype="http://www.w3.org/2001/XMLSchema#string">Hexidecimal</rdf:first>
                                <rdf:rest>
                                    <rdf:Description>
                                        <rdf:type rdf:resource="http://www.w3.org/1999/02/22-rdf-syntax-ns#List"/>
                                        <rdf:first rdf:datatype="http://www.w3.org/2001/XMLSchema#string">Other</rdf:first>
                                        <rdf:rest>
                                            <rdf:Description>
                                                <rdf:type rdf:resource="http://www.w3.org/1999/02/22-rdf-syntax-ns#List"/>
                                                <rdf:first rdf:datatype="http://www.w3.org/2001/XMLSchema#string">Text</rdf:first>
                                                <rdf:rest rdf:resource="http://www.w3.org/1999/02/22-rdf-syntax-ns#nil"/>
                                            </rdf:Description>
                                        </rdf:rest>
                                    </rdf:Description>
                                </rdf:rest>
                            </rdf:Description>
                        </rdf:rest>
                    </rdf:Description>
                </owl:oneOf>
            </rdfs:Datatype>
        </rdfs:range>
        <rdfs:comment>Specifies the type of data contained in the Data_Segment element.</rdfs:comment>
        <rdfs:isDefinedBy rdf:resource="http://cybox.mitre.org/cyboxCommon"/>
        <rdfs:label>Data Format</rdfs:label>
    </owl:DatatypeProperty>
    


    <!-- http://cybox.mitre.org/cyboxCommon#dataSegment -->

    <owl:DatatypeProperty rdf:about="http://cybox.mitre.org/cyboxCommon#dataSegment">
        <rdfs:range rdf:resource="http://www.w3.org/2001/XMLSchema#string"/>
        <rdfs:comment>Specifies the actual segment of data being characterized.</rdfs:comment>
        <rdfs:isDefinedBy rdf:resource="http://cybox.mitre.org/cyboxCommon"/>
        <rdfs:label>Data Segment</rdfs:label>
    </owl:DatatypeProperty>
    


    <!-- http://cybox.mitre.org/cyboxCommon#dataSize -->

    <owl:DatatypeProperty rdf:about="http://cybox.mitre.org/cyboxCommon#dataSize">
        <rdfs:range rdf:resource="http://www.w3.org/2001/XMLSchema#integer"/>
        <rdfs:comment>Specifies the size of the data segment.</rdfs:comment>
        <rdfs:isDefinedBy rdf:resource="http://cybox.mitre.org/cyboxCommon"/>
        <rdfs:label>Data Size</rdfs:label>
    </owl:DatatypeProperty>
    


    <!-- http://cybox.mitre.org/cyboxCommon#dataSizeUnits -->

    <owl:DatatypeProperty rdf:about="http://cybox.mitre.org/cyboxCommon#dataSizeUnits">
        <rdfs:range>
            <rdfs:Datatype>
                <owl:oneOf>
                    <rdf:Description>
                        <rdf:type rdf:resource="http://www.w3.org/1999/02/22-rdf-syntax-ns#List"/>
                        <rdf:first rdf:datatype="http://www.w3.org/2001/XMLSchema#string">Bytes</rdf:first>
                        <rdf:rest>
                            <rdf:Description>
                                <rdf:type rdf:resource="http://www.w3.org/1999/02/22-rdf-syntax-ns#List"/>
                                <rdf:first rdf:datatype="http://www.w3.org/2001/XMLSchema#string">Kilobytes</rdf:first>
                                <rdf:rest>
                                    <rdf:Description>
                                        <rdf:type rdf:resource="http://www.w3.org/1999/02/22-rdf-syntax-ns#List"/>
                                        <rdf:first rdf:datatype="http://www.w3.org/2001/XMLSchema#string">Megabytes</rdf:first>
                                        <rdf:rest rdf:resource="http://www.w3.org/1999/02/22-rdf-syntax-ns#nil"/>
                                    </rdf:Description>
                                </rdf:rest>
                            </rdf:Description>
                        </rdf:rest>
                    </rdf:Description>
                </owl:oneOf>
            </rdfs:Datatype>
        </rdfs:range>
        <rdfs:comment>Specifies data size units associated with the dataSize property.</rdfs:comment>
        <rdfs:isDefinedBy rdf:resource="http://cybox.mitre.org/cyboxCommon"/>
        <rdfs:label>Data Size Units</rdfs:label>
    </owl:DatatypeProperty>
    


    <!-- http://cybox.mitre.org/cyboxCommon#dependencyDescription -->

    <owl:DatatypeProperty rdf:about="http://cybox.mitre.org/cyboxCommon#dependencyDescription">
        <rdfs:range rdf:resource="http://www.w3.org/2001/XMLSchema#string"/>
        <rdfs:comment>Specifies a description of this dependency instance.</rdfs:comment>
        <rdfs:isDefinedBy rdf:resource="http://cybox.mitre.org/cyboxCommon"/>
        <rdfs:label>Description</rdfs:label>
    </owl:DatatypeProperty>
    


    <!-- http://cybox.mitre.org/cyboxCommon#dependencyType -->

    <owl:DatatypeProperty rdf:about="http://cybox.mitre.org/cyboxCommon#dependencyType">
        <rdfs:range rdf:resource="http://www.w3.org/2001/XMLSchema#string"/>
        <rdfs:comment>Specifies the type of this dependency instance.</rdfs:comment>
        <rdfs:isDefinedBy rdf:resource="http://cybox.mitre.org/cyboxCommon"/>
        <rdfs:label>Type</rdfs:label>
    </owl:DatatypeProperty>
    


    <!-- http://cybox.mitre.org/cyboxCommon#encoding -->

    <owl:DatatypeProperty rdf:about="http://cybox.mitre.org/cyboxCommon#encoding">
        <rdfs:range rdf:resource="http://www.w3.org/2001/XMLSchema#string"/>
        <rdfs:comment>Specifies the encoding method used for the string extracted from the CybOX object, via a standardized controlled vocabulary.</rdfs:comment>
        <rdfs:isDefinedBy rdf:resource="http://cybox.mitre.org/cyboxCommon"/>
        <rdfs:label>Encoding</rdfs:label>
    </owl:DatatypeProperty>
    


    <!-- http://cybox.mitre.org/cyboxCommon#englishTranslation -->

    <owl:DatatypeProperty rdf:about="http://cybox.mitre.org/cyboxCommon#englishTranslation">
        <rdfs:range rdf:resource="http://www.w3.org/2001/XMLSchema#string"/>
        <rdfs:comment>Specifies the English translation of the string, if it is not written in English.</rdfs:comment>
        <rdfs:isDefinedBy rdf:resource="http://cybox.mitre.org/cyboxCommon"/>
        <rdfs:label>English Translation</rdfs:label>
    </owl:DatatypeProperty>
    


    <!-- http://cybox.mitre.org/cyboxCommon#envVarName -->

    <owl:DatatypeProperty rdf:about="http://cybox.mitre.org/cyboxCommon#envVarName">
        <rdfs:range rdf:resource="http://www.w3.org/2001/XMLSchema#string"/>
        <rdfs:comment>Specifies the name of the environment variable.</rdfs:comment>
        <rdfs:isDefinedBy rdf:resource="http://cybox.mitre.org/cyboxCommon"/>
        <rdfs:label>Name</rdfs:label>
    </owl:DatatypeProperty>
    


    <!-- http://cybox.mitre.org/cyboxCommon#envVarValue -->

    <owl:DatatypeProperty rdf:about="http://cybox.mitre.org/cyboxCommon#envVarValue">
        <rdfs:range rdf:resource="http://www.w3.org/2001/XMLSchema#string"/>
        <rdfs:comment>Specifies the value of the environment variable</rdfs:comment>
        <rdfs:isDefinedBy rdf:resource="http://cybox.mitre.org/cyboxCommon"/>
        <rdfs:label>Value</rdfs:label>
    </owl:DatatypeProperty>
    


    <!-- http://cybox.mitre.org/cyboxCommon#errorCount -->

    <owl:DatatypeProperty rdf:about="http://cybox.mitre.org/cyboxCommon#errorCount">
        <rdfs:range rdf:resource="http://www.w3.org/2001/XMLSchema#integer"/>
        <rdfs:comment>Specifies the count of instances for this error in the tool run.</rdfs:comment>
        <rdfs:isDefinedBy rdf:resource="http://cybox.mitre.org/cyboxCommon"/>
        <rdfs:label>Error Count</rdfs:label>
    </owl:DatatypeProperty>
    


    <!-- http://cybox.mitre.org/cyboxCommon#errorInstances -->

    <owl:DatatypeProperty rdf:about="http://cybox.mitre.org/cyboxCommon#errorInstances">
        <rdfs:range rdf:resource="http://www.w3.org/2001/XMLSchema#string"/>
        <rdfs:comment>Specifies the actual error output for each instance of this type of error.</rdfs:comment>
        <rdfs:isDefinedBy rdf:resource="http://cybox.mitre.org/cyboxCommon"/>
        <rdfs:label>Error Instances</rdfs:label>
    </owl:DatatypeProperty>
    


    <!-- http://cybox.mitre.org/cyboxCommon#errorType -->

    <owl:DatatypeProperty rdf:about="http://cybox.mitre.org/cyboxCommon#errorType">
        <rdfs:range rdf:resource="http://www.w3.org/2001/XMLSchema#string"/>
        <rdfs:comment>Specifies the type for this tool run error.</rdfs:comment>
        <rdfs:isDefinedBy rdf:resource="http://cybox.mitre.org/cyboxCommon"/>
        <rdfs:label>Error Type</rdfs:label>
    </owl:DatatypeProperty>
    


    <!-- http://cybox.mitre.org/cyboxCommon#externalReference -->

    <owl:DatatypeProperty rdf:about="http://cybox.mitre.org/cyboxCommon#externalReference">
        <rdfs:range rdf:resource="http://www.w3.org/2001/XMLSchema#anyURI"/>
        <rdfs:comment>Specifies the hyperlink to the reference</rdfs:comment>
        <rdfs:isDefinedBy rdf:resource="http://cybox.mitre.org/cyboxCommon"/>
        <rdfs:label>External Reference</rdfs:label>
    </owl:DatatypeProperty>
    


    <!-- http://cybox.mitre.org/cyboxCommon#extractedFeature.functions -->

    <owl:DatatypeProperty rdf:about="http://cybox.mitre.org/cyboxCommon#extractedFeature.functions">
        <rdfs:range rdf:resource="http://www.w3.org/2001/XMLSchema#string"/>
        <rdfs:comment>Specifies a set of references to functions called by a raw cyber object.</rdfs:comment>
        <rdfs:isDefinedBy rdf:resource="http://cybox.mitre.org/cyboxCommon"/>
        <rdfs:label>Extracted Feature Functions</rdfs:label>
    </owl:DatatypeProperty>
    


    <!-- http://cybox.mitre.org/cyboxCommon#extractedFeature.imports -->

    <owl:DatatypeProperty rdf:about="http://cybox.mitre.org/cyboxCommon#extractedFeature.imports">
        <rdfs:range rdf:resource="http://www.w3.org/2001/XMLSchema#string"/>
        <rdfs:comment>Specifies  a set of references to external resources imported by a raw cyber object.</rdfs:comment>
        <rdfs:isDefinedBy rdf:resource="http://cybox.mitre.org/cyboxCommon"/>
        <rdfs:label>extracted feature.imports</rdfs:label>
    </owl:DatatypeProperty>
    


    <!-- http://cybox.mitre.org/cyboxCommon#fileSystemOffset -->

    <owl:DatatypeProperty rdf:about="http://cybox.mitre.org/cyboxCommon#fileSystemOffset">
        <rdfs:range rdf:resource="http://www.w3.org/2001/XMLSchema#integer"/>
        <rdfs:comment>Specifies the offset of the beginning of the byte run as measured from the beginning of the relevant file system.

This field is relevant only for byte runs of tiles in forensic analysis.</rdfs:comment>
        <rdfs:isDefinedBy rdf:resource="http://cybox.mitre.org/cyboxCommon"/>
        <rdfs:label>File System Offset</rdfs:label>
    </owl:DatatypeProperty>
    


    <!-- http://cybox.mitre.org/cyboxCommon#hash.value -->

    <owl:DatatypeProperty rdf:about="http://cybox.mitre.org/cyboxCommon#hash.value">
        <rdfs:range rdf:resource="http://www.w3.org/2001/XMLSchema#string"/>
        <rdfs:comment>Specifies the value and type of a hash in the format hash-type:hash-value</rdfs:comment>
        <rdfs:isDefinedBy rdf:resource="http://cybox.mitre.org/cyboxCommon"/>
        <rdfs:label>Hash Value</rdfs:label>
    </owl:DatatypeProperty>
    


    <!-- http://cybox.mitre.org/cyboxCommon#hashType -->

    <owl:DatatypeProperty rdf:about="http://cybox.mitre.org/cyboxCommon#hashType">
        <rdfs:range rdf:resource="http://www.w3.org/2001/XMLSchema#string"/>
        <rdfs:comment>Specifies the type of hash used in the Simple_Hash_Value or Fuzzy_Hash_Value elements, using a standardized controlled vocabulary.</rdfs:comment>
        <rdfs:isDefinedBy rdf:resource="http://cybox.mitre.org/cyboxCommon"/>
        <rdfs:label>Hash Type</rdfs:label>
    </owl:DatatypeProperty>
    


    <!-- http://cybox.mitre.org/cyboxCommon#hashValue -->

    <owl:DatatypeProperty rdf:about="http://cybox.mitre.org/cyboxCommon#hashValue"/>
    


    <!-- http://cybox.mitre.org/cyboxCommon#id -->

    <owl:DatatypeProperty rdf:about="http://cybox.mitre.org/cyboxCommon#id">
        <rdfs:range rdf:resource="http://www.w3.org/2001/XMLSchema#string"/>
        <rdfs:comment>Specifies the unique identifier associated with this entity instance.

An identifier MUST take the format [ns-prefix]:[construct-type]-[UUID], where [ns-prefix] should be the namespace prefix owned/controlled by the producer of the content

The format of the Id must be in the format of [ns-prefix]:construct-type-[UUID], there the [ns-prefix] SHOULD be a namespace prefix bound to a namespace owned/controlled by the producer of the content, and [UUID] SHOULD correspond to a globally unique identifier.</rdfs:comment>
        <rdfs:isDefinedBy rdf:resource="http://cybox.mitre.org/cyboxCommon"/>
        <rdfs:label>Id</rdfs:label>
    </owl:DatatypeProperty>
    


    <!-- http://cybox.mitre.org/cyboxCommon#imageOffset -->

    <owl:DatatypeProperty rdf:about="http://cybox.mitre.org/cyboxCommon#imageOffset">
        <rdfs:range rdf:resource="http://www.w3.org/2001/XMLSchema#integer"/>
        <rdfs:comment>Specifies the offset of the beginning of the byte run as measured form the beginning of the relevant forensic image.

This field is provided for forensic analysis purposes.</rdfs:comment>
        <rdfs:isDefinedBy rdf:resource="http://cybox.mitre.org/cyboxCommon"/>
        <rdfs:label>Image Offset</rdfs:label>
    </owl:DatatypeProperty>
    


    <!-- http://cybox.mitre.org/cyboxCommon#informationSourceType -->

    <owl:DatatypeProperty rdf:about="http://cybox.mitre.org/cyboxCommon#informationSourceType">
        <rdfs:range rdf:resource="http://www.w3.org/2001/XMLSchema#string"/>
        <rdfs:comment>Specifies the type of information source leveraged for this cyber observation source,  through a standardized controlled vocabulary.</rdfs:comment>
        <rdfs:isDefinedBy rdf:resource="http://cybox.mitre.org/cyboxCommon"/>
        <rdfs:label>Information Source Type</rdfs:label>
    </owl:DatatypeProperty>
    


    <!-- http://cybox.mitre.org/cyboxCommon#key -->

    <owl:DatatypeProperty rdf:about="http://cybox.mitre.org/cyboxCommon#key">
        <rdfs:range rdf:resource="http://www.w3.org/2001/XMLSchema#string"/>
        <rdfs:comment>Specifies the actual key of this internal string instance.</rdfs:comment>
        <rdfs:isDefinedBy rdf:resource="http://cybox.mitre.org/cyboxCommon"/>
        <rdfs:label>Key</rdfs:label>
    </owl:DatatypeProperty>
    


    <!-- http://cybox.mitre.org/cyboxCommon#libraryName -->

    <owl:DatatypeProperty rdf:about="http://cybox.mitre.org/cyboxCommon#libraryName">
        <rdfs:range rdf:resource="http://www.w3.org/2001/XMLSchema#string"/>
        <rdfs:comment>Specifies the name of the library</rdfs:comment>
        <rdfs:isDefinedBy rdf:resource="http://cybox.mitre.org/cyboxCommon"/>
        <rdfs:label>Name</rdfs:label>
    </owl:DatatypeProperty>
    


    <!-- http://cybox.mitre.org/cyboxCommon#libraryVersion -->

    <owl:DatatypeProperty rdf:about="http://cybox.mitre.org/cyboxCommon#libraryVersion">
        <rdfs:range rdf:resource="http://www.w3.org/2001/XMLSchema#string"/>
        <rdfs:comment>Specifies the version of the library.</rdfs:comment>
        <rdfs:isDefinedBy rdf:resource="http://cybox.mitre.org/cyboxCommon"/>
        <rdfs:label>Version</rdfs:label>
    </owl:DatatypeProperty>
    


    <!-- http://cybox.mitre.org/cyboxCommon#locationName -->

    <owl:DatatypeProperty rdf:about="http://cybox.mitre.org/cyboxCommon#locationName">
        <rdfs:range rdf:resource="http://www.w3.org/2001/XMLSchema#string"/>
        <rdfs:comment>Specifies a location through a simple name.</rdfs:comment>
        <rdfs:isDefinedBy rdf:resource="http://cybox.mitre.org/cyboxCommon"/>
        <rdfs:label>Location Name</rdfs:label>
    </owl:DatatypeProperty>
    


    <!-- http://cybox.mitre.org/cyboxCommon#metadataType -->

    <owl:DatatypeProperty rdf:about="http://cybox.mitre.org/cyboxCommon#metadataType">
        <rdfs:range rdf:resource="http://www.w3.org/2001/XMLSchema#string"/>
        <rdfs:comment>Specifies the type of name of a single metadata field.</rdfs:comment>
        <rdfs:isDefinedBy rdf:resource="http://cybox.mitre.org/cyboxCommon"/>
        <rdfs:label>Type</rdfs:label>
    </owl:DatatypeProperty>
    


    <!-- http://cybox.mitre.org/cyboxCommon#metadataValue -->

    <owl:DatatypeProperty rdf:about="http://cybox.mitre.org/cyboxCommon#metadataValue">
        <rdfs:range rdf:resource="http://www.w3.org/2001/XMLSchema#string"/>
        <rdfs:comment>Specifies the value of name of a single metadata field.</rdfs:comment>
        <rdfs:isDefinedBy rdf:resource="http://cybox.mitre.org/cyboxCommon"/>
        <rdfs:label>Value</rdfs:label>
    </owl:DatatypeProperty>
    


    <!-- http://cybox.mitre.org/cyboxCommon#namingSystem -->

    <owl:DatatypeProperty rdf:about="http://cybox.mitre.org/cyboxCommon#namingSystem">
        <rdfs:range rdf:resource="http://www.w3.org/2001/XMLSchema#string"/>
        <rdfs:comment>Specifies the naming system from which the indicated name was drawn.</rdfs:comment>
        <rdfs:isDefinedBy rdf:resource="http://cybox.mitre.org/cyboxCommon"/>
        <rdfs:label>Platform Identifier Naming System</rdfs:label>
    </owl:DatatypeProperty>
    


    <!-- http://cybox.mitre.org/cyboxCommon#offset -->

    <owl:DatatypeProperty rdf:about="http://cybox.mitre.org/cyboxCommon#offset">
        <rdfs:range rdf:resource="http://www.w3.org/2001/XMLSchema#integer"/>
        <rdfs:comment>Specifies where to start searching for the specified data segment in an object, in bytes.</rdfs:comment>
        <rdfs:isDefinedBy rdf:resource="http://cybox.mitre.org/cyboxCommon"/>
        <rdfs:label>Offset</rdfs:label>
    </owl:DatatypeProperty>
    


    <!-- http://cybox.mitre.org/cyboxCommon#offsetAddress -->

    <owl:DatatypeProperty rdf:about="http://cybox.mitre.org/cyboxCommon#offsetAddress">
        <rdfs:range rdf:resource="http://www.w3.org/2001/XMLSchema#hexBinary"/>
        <rdfs:comment>Specifies the location or offset of the specified string in the CybOX objects.</rdfs:comment>
        <rdfs:isDefinedBy rdf:resource="http://cybox.mitre.org/cyboxCommon"/>
        <rdfs:label>Offset Address</rdfs:label>
    </owl:DatatypeProperty>
    


    <!-- http://cybox.mitre.org/cyboxCommon#ordinalPosition -->

    <owl:DatatypeProperty rdf:about="http://cybox.mitre.org/cyboxCommon#ordinalPosition">
        <rdfs:range rdf:resource="http://www.w3.org/2001/XMLSchema#positiveInteger"/>
        <rdfs:comment>Specifies the ordinal position of the parameter with respect to the function where it is used.</rdfs:comment>
        <rdfs:isDefinedBy rdf:resource="http://cybox.mitre.org/cyboxCommon"/>
        <rdfs:label>Ordinal Position</rdfs:label>
    </owl:DatatypeProperty>
    


    <!-- http://cybox.mitre.org/cyboxCommon#parameterName -->

    <owl:DatatypeProperty rdf:about="http://cybox.mitre.org/cyboxCommon#parameterName">
        <rdfs:range rdf:resource="http://www.w3.org/2001/XMLSchema#string"/>
        <rdfs:comment>Specifies the name of the parameter.</rdfs:comment>
        <rdfs:isDefinedBy rdf:resource="http://cybox.mitre.org/cyboxCommon"/>
        <rdfs:label>Name</rdfs:label>
    </owl:DatatypeProperty>
    


    <!-- http://cybox.mitre.org/cyboxCommon#parameterValue -->

    <owl:DatatypeProperty rdf:about="http://cybox.mitre.org/cyboxCommon#parameterValue">
        <rdfs:range rdf:resource="http://www.w3.org/2001/XMLSchema#string"/>
        <rdfs:comment>Specifies the actual value of the parameter.</rdfs:comment>
        <rdfs:isDefinedBy rdf:resource="http://cybox.mitre.org/cyboxCommon"/>
        <rdfs:label>Value</rdfs:label>
    </owl:DatatypeProperty>
    


    <!-- http://cybox.mitre.org/cyboxCommon#parentId -->

    <owl:DatatypeProperty rdf:about="http://cybox.mitre.org/cyboxCommon#parentId">
        <rdfs:range rdf:resource="http://www.w3.org/2001/XMLSchema#string"/>
        <rdfs:comment>Specifies the identifier for the parent object</rdfs:comment>
        <rdfs:isDefinedBy rdf:resource="http://cybox.mitre.org/cybox_core"/>
        <rdfs:label>Parent ID</rdfs:label>
    </owl:DatatypeProperty>
    


    <!-- http://cybox.mitre.org/cyboxCommon#platformDescription -->

    <owl:DatatypeProperty rdf:about="http://cybox.mitre.org/cyboxCommon#platformDescription">
        <rdfs:range rdf:resource="http://www.w3.org/2001/XMLSchema#string"/>
        <rdfs:comment>Specifies description of the indicated platform.</rdfs:comment>
        <rdfs:isDefinedBy rdf:resource="http://cybox.mitre.org/cyboxCommon"/>
        <rdfs:label>Description</rdfs:label>
    </owl:DatatypeProperty>
    


    <!-- http://cybox.mitre.org/cyboxCommon#platformIdentifier -->

    <owl:DatatypeProperty rdf:about="http://cybox.mitre.org/cyboxCommon#platformIdentifier">
        <rdfs:range rdf:resource="http://www.w3.org/2001/XMLSchema#string"/>
        <rdfs:comment>Specifies a pre-defined name for the given platform using some naming scheme.  For example, one coupld provide a CPE (Common Platform Enumeration) name using the CPE naming format.</rdfs:comment>
        <rdfs:isDefinedBy rdf:resource="http://cybox.mitre.org/cyboxCommon"/>
        <rdfs:label>platform identifier</rdfs:label>
    </owl:DatatypeProperty>
    


    <!-- http://cybox.mitre.org/cyboxCommon#propertyDescription -->

    <owl:DatatypeProperty rdf:about="http://cybox.mitre.org/cyboxCommon#propertyDescription">
        <rdfs:range rdf:resource="http://www.w3.org/2001/XMLSchema#string"/>
        <rdfs:comment>Specifies a description of what this property represents.</rdfs:comment>
        <rdfs:isDefinedBy rdf:resource="http://cybox.mitre.org/cyboxCommon"/>
        <rdfs:label>Property Description</rdfs:label>
    </owl:DatatypeProperty>
    


    <!-- http://cybox.mitre.org/cyboxCommon#propertyName -->

    <owl:DatatypeProperty rdf:about="http://cybox.mitre.org/cyboxCommon#propertyName">
        <rdfs:range rdf:resource="http://www.w3.org/2001/XMLSchema#string"/>
        <rdfs:comment>Specifies a name for this property.</rdfs:comment>
        <rdfs:isDefinedBy rdf:resource="http://cybox.mitre.org/cyboxCommon"/>
        <rdfs:label>Property Name</rdfs:label>
    </owl:DatatypeProperty>
    


    <!-- http://cybox.mitre.org/cyboxCommon#propertyValue -->

    <owl:DatatypeProperty rdf:about="http://cybox.mitre.org/cyboxCommon#propertyValue">
        <rdfs:range rdf:resource="http://www.w3.org/2001/XMLSchema#string"/>
        <rdfs:comment>Specifies the value of the property</rdfs:comment>
        <rdfs:isDefinedBy rdf:resource="http://cybox.mitre.org/cyboxCommon"/>
        <rdfs:label>Property Value</rdfs:label>
    </owl:DatatypeProperty>
    


    <!-- http://cybox.mitre.org/cyboxCommon#rawSegmentContent -->

    <owl:DatatypeProperty rdf:about="http://cybox.mitre.org/cyboxCommon#rawSegmentContent">
        <rdfs:range rdf:resource="http://www.w3.org/2001/XMLSchema#anySimpleType"/>
        <rdfs:comment>Specifies the raw content of this segment of the hashed object.</rdfs:comment>
        <rdfs:isDefinedBy rdf:resource="http://cybox.mitre.org/cyboxCommon"/>
        <rdfs:label>Raw Segment Content</rdfs:label>
    </owl:DatatypeProperty>
    


    <!-- http://cybox.mitre.org/cyboxCommon#referenceType -->

    <owl:DatatypeProperty rdf:about="http://cybox.mitre.org/cyboxCommon#referenceType">
        <rdfs:range>
            <rdfs:Datatype>
                <owl:oneOf>
                    <rdf:Description>
                        <rdf:type rdf:resource="http://www.w3.org/1999/02/22-rdf-syntax-ns#List"/>
                        <rdf:first rdf:datatype="http://www.w3.org/2001/XMLSchema#string">Documentation</rdf:first>
                        <rdf:rest>
                            <rdf:Description>
                                <rdf:type rdf:resource="http://www.w3.org/1999/02/22-rdf-syntax-ns#List"/>
                                <rdf:first rdf:datatype="http://www.w3.org/2001/XMLSchema#string">Download</rdf:first>
                                <rdf:rest>
                                    <rdf:Description>
                                        <rdf:type rdf:resource="http://www.w3.org/1999/02/22-rdf-syntax-ns#List"/>
                                        <rdf:first rdf:datatype="http://www.w3.org/2001/XMLSchema#string">Execute</rdf:first>
                                        <rdf:rest>
                                            <rdf:Description>
                                                <rdf:type rdf:resource="http://www.w3.org/1999/02/22-rdf-syntax-ns#List"/>
                                                <rdf:first rdf:datatype="http://www.w3.org/2001/XMLSchema#string">Other</rdf:first>
                                                <rdf:rest>
                                                    <rdf:Description>
                                                        <rdf:type rdf:resource="http://www.w3.org/1999/02/22-rdf-syntax-ns#List"/>
                                                        <rdf:first rdf:datatype="http://www.w3.org/2001/XMLSchema#string">Source</rdf:first>
                                                        <rdf:rest rdf:resource="http://www.w3.org/1999/02/22-rdf-syntax-ns#nil"/>
                                                    </rdf:Description>
                                                </rdf:rest>
                                            </rdf:Description>
                                        </rdf:rest>
                                    </rdf:Description>
                                </rdf:rest>
                            </rdf:Description>
                        </rdf:rest>
                    </rdf:Description>
                </owl:oneOf>
            </rdfs:Datatype>
        </rdfs:range>
        <rdfs:comment>Specifies the nature of the referenced material (documentation, source, executable, etc.).</rdfs:comment>
        <rdfs:isDefinedBy rdf:resource="http://cybox.mitre.org/cyboxCommon"/>
        <rdfs:label>Reference Type</rdfs:label>
    </owl:DatatypeProperty>
    


    <!-- http://cybox.mitre.org/cyboxCommon#regionalInternetRegistry -->

    <owl:DatatypeProperty rdf:about="http://cybox.mitre.org/cyboxCommon#regionalInternetRegistry">
        <rdfs:range rdf:resource="http://www.w3.org/2001/XMLSchema#string"/>
        <rdfs:comment>Specifies the name of the Regional Internet Registry (RIR).</rdfs:comment>
        <rdfs:isDefinedBy rdf:resource="http://cybox.mitre.org/cyboxCommon"/>
        <rdfs:label>Regional Internet Registry (RIR)</rdfs:label>
    </owl:DatatypeProperty>
    


    <!-- http://cybox.mitre.org/cyboxCommon#searchDistance -->

    <owl:DatatypeProperty rdf:about="http://cybox.mitre.org/cyboxCommon#searchDistance">
        <rdfs:range rdf:resource="http://www.w3.org/2001/XMLSchema#integer"/>
        <rdfs:comment>Specifies how far into an object should be ignored, in bytes, before starting to search for the specified data segment relative to the end of the previous data segment.</rdfs:comment>
        <rdfs:isDefinedBy rdf:resource="http://cybox.mitre.org/cyboxCommon"/>
        <rdfs:label>Search Distance</rdfs:label>
    </owl:DatatypeProperty>
    


    <!-- http://cybox.mitre.org/cyboxCommon#searchWithin -->

    <owl:DatatypeProperty rdf:about="http://cybox.mitre.org/cyboxCommon#searchWithin">
        <rdfs:range rdf:resource="http://www.w3.org/2001/XMLSchema#integer"/>
        <rdfs:comment>Specifies that at most N bytes are between data segments in related objects.</rdfs:comment>
        <rdfs:isDefinedBy rdf:resource="http://cybox.mitre.org/cyboxCommon"/>
        <rdfs:label>Search Within</rdfs:label>
    </owl:DatatypeProperty>
    


    <!-- http://cybox.mitre.org/cyboxCommon#securityID -->

    <owl:DatatypeProperty rdf:about="http://cybox.mitre.org/cyboxCommon#securityID">
        <rdfs:range rdf:resource="http://www.w3.org/2001/XMLSchema#string"/>
        <rdfs:comment>Specifies the Security ID (SID) value assigned to the file</rdfs:comment>
        <rdfs:isDefinedBy rdf:resource="http://cybox.mitre.org/cyboxCommon"/>
        <rdfs:label>Security ID (SID)</rdfs:label>
    </owl:DatatypeProperty>
    


    <!-- http://cybox.mitre.org/cyboxCommon#securityIDType -->

    <owl:DatatypeProperty rdf:about="http://cybox.mitre.org/cyboxCommon#securityIDType">
        <rdfs:range rdf:resource="http://www.w3.org/2001/XMLSchema#string"/>
        <rdfs:comment>Specifies the type of Security ID (SID) assigned to the file</rdfs:comment>
        <rdfs:isDefinedBy rdf:resource="http://cybox.mitre.org/cyboxCommon"/>
        <rdfs:label>Security Id (SID) Type</rdfs:label>
    </owl:DatatypeProperty>
    


    <!-- http://cybox.mitre.org/cyboxCommon#segmentHash.fuzzyHashValue -->

    <owl:DatatypeProperty rdf:about="http://cybox.mitre.org/cyboxCommon#segmentHash.fuzzyHashValue">
        <rdfs:range rdf:resource="http://www.w3.org/2001/XMLSchema#string"/>
        <rdfs:comment>Specifies a single result value of a cryptograhic fuzzy hash function outputting a single complex string based hash value. (e.g. SSDEEP&apos;s Block1hash:Block2hash format).</rdfs:comment>
        <rdfs:isDefinedBy rdf:resource="http://cybox.mitre.org/cyboxCommon"/>
        <rdfs:label>Segment Fuzzy Hash Value</rdfs:label>
    </owl:DatatypeProperty>
    


    <!-- http://cybox.mitre.org/cyboxCommon#segmentHash.simpleHashValue -->

    <owl:DatatypeProperty rdf:about="http://cybox.mitre.org/cyboxCommon#segmentHash.simpleHashValue">
        <rdfs:range rdf:resource="http://www.w3.org/2001/XMLSchema#string"/>
        <rdfs:comment>Specifies a calculated hash value for this segment.</rdfs:comment>
        <rdfs:isDefinedBy rdf:resource="http://cybox.mitre.org/cyboxCommon"/>
        <rdfs:label>Segment Hash</rdfs:label>
    </owl:DatatypeProperty>
    


    <!-- http://cybox.mitre.org/cyboxCommon#settingDescription -->

    <owl:DatatypeProperty rdf:about="http://cybox.mitre.org/cyboxCommon#settingDescription">
        <rdfs:range rdf:resource="http://www.w3.org/2001/XMLSchema#string"/>
        <rdfs:comment>Specifies a description of the configuration item referenced in this configuration setting instance.</rdfs:comment>
        <rdfs:isDefinedBy rdf:resource="http://cybox.mitre.org/cyboxCommon"/>
        <rdfs:label>Description</rdfs:label>
    </owl:DatatypeProperty>
    


    <!-- http://cybox.mitre.org/cyboxCommon#settingName -->

    <owl:DatatypeProperty rdf:about="http://cybox.mitre.org/cyboxCommon#settingName">
        <rdfs:range rdf:resource="http://www.w3.org/2001/XMLSchema#string"/>
        <rdfs:comment>Specifies the name of the configuration item referenced by this configuration setting instance.</rdfs:comment>
        <rdfs:isDefinedBy rdf:resource="http://cybox.mitre.org/cyboxCommon"/>
        <rdfs:label>Setting Name</rdfs:label>
    </owl:DatatypeProperty>
    


    <!-- http://cybox.mitre.org/cyboxCommon#settingType -->

    <owl:DatatypeProperty rdf:about="http://cybox.mitre.org/cyboxCommon#settingType">
        <rdfs:range rdf:resource="http://www.w3.org/2001/XMLSchema#string"/>
        <rdfs:comment>Specifies the type of the configuration item referenced in this configuration setting instance.</rdfs:comment>
        <rdfs:isDefinedBy rdf:resource="http://cybox.mitre.org/cyboxCommon"/>
        <rdfs:label>Type</rdfs:label>
    </owl:DatatypeProperty>
    


    <!-- http://cybox.mitre.org/cyboxCommon#settingValue -->

    <owl:DatatypeProperty rdf:about="http://cybox.mitre.org/cyboxCommon#settingValue">
        <rdfs:range rdf:resource="http://www.w3.org/2001/XMLSchema#string"/>
        <rdfs:comment>Specifies he value of this configuration setting instance.</rdfs:comment>
        <rdfs:isDefinedBy rdf:resource="http://cybox.mitre.org/cyboxCommon"/>
        <rdfs:label>Value</rdfs:label>
    </owl:DatatypeProperty>
    


    <!-- http://cybox.mitre.org/cyboxCommon#sightingCount -->

    <owl:DatatypeProperty rdf:about="http://cybox.mitre.org/cyboxCommon#sightingCount">
        <rdfs:range rdf:resource="http://www.w3.org/2001/XMLSchema#positiveInteger"/>
        <rdfs:comment>Specifies how many different identical instances of a given Observable may have been seen/sighted by the observation source.</rdfs:comment>
        <rdfs:isDefinedBy rdf:resource="http://cybox.mitre.org/cyboxCommon"/>
        <rdfs:label>Sighting Count</rdfs:label>
    </owl:DatatypeProperty>
    


    <!-- http://cybox.mitre.org/cyboxCommon#signatureDescription -->

    <owl:DatatypeProperty rdf:about="http://cybox.mitre.org/cyboxCommon#signatureDescription">
        <rdfs:range rdf:resource="http://www.w3.org/2001/XMLSchema#string"/>
        <rdfs:comment>Specifies a description of the digitial signature</rdfs:comment>
        <rdfs:isDefinedBy rdf:resource="http://cybox.mitre.org/cyboxCommon"/>
        <rdfs:label>Signature Description</rdfs:label>
    </owl:DatatypeProperty>
    


    <!-- http://cybox.mitre.org/cyboxCommon#signatureExists -->

    <owl:DatatypeProperty rdf:about="http://cybox.mitre.org/cyboxCommon#signatureExists">
        <rdfs:range rdf:resource="http://www.w3.org/2001/XMLSchema#boolean"/>
        <rdfs:comment>Specifies whether the digital signature exists.</rdfs:comment>
        <rdfs:isDefinedBy rdf:resource="http://cybox.mitre.org/cyboxCommon"/>
        <rdfs:label>Signature Exists</rdfs:label>
    </owl:DatatypeProperty>
    


    <!-- http://cybox.mitre.org/cyboxCommon#signatureVerified -->

    <owl:DatatypeProperty rdf:about="http://cybox.mitre.org/cyboxCommon#signatureVerified">
        <rdfs:range rdf:resource="http://www.w3.org/2001/XMLSchema#boolean"/>
        <rdfs:comment>Specifies if the digital signature is verified.</rdfs:comment>
        <rdfs:isDefinedBy rdf:resource="http://cybox.mitre.org/cyboxCommon"/>
        <rdfs:label>Signature Verified</rdfs:label>
    </owl:DatatypeProperty>
    


    <!-- http://cybox.mitre.org/cyboxCommon#sourceClass -->

    <owl:DatatypeProperty rdf:about="http://cybox.mitre.org/cyboxCommon#sourceClass">
        <rdfs:range>
            <rdfs:Datatype>
                <owl:oneOf>
                    <rdf:Description>
                        <rdf:type rdf:resource="http://www.w3.org/1999/02/22-rdf-syntax-ns#List"/>
                        <rdf:first rdf:datatype="http://www.w3.org/2001/XMLSchema#string">Network</rdf:first>
                        <rdf:rest>
                            <rdf:Description>
                                <rdf:type rdf:resource="http://www.w3.org/1999/02/22-rdf-syntax-ns#List"/>
                                <rdf:first rdf:datatype="http://www.w3.org/2001/XMLSchema#string">Software</rdf:first>
                                <rdf:rest>
                                    <rdf:Description>
                                        <rdf:type rdf:resource="http://www.w3.org/1999/02/22-rdf-syntax-ns#List"/>
                                        <rdf:first rdf:datatype="http://www.w3.org/2001/XMLSchema#string">System</rdf:first>
                                        <rdf:rest rdf:resource="http://www.w3.org/1999/02/22-rdf-syntax-ns#nil"/>
                                    </rdf:Description>
                                </rdf:rest>
                            </rdf:Description>
                        </rdf:rest>
                    </rdf:Description>
                </owl:oneOf>
            </rdfs:Datatype>
        </rdfs:range>
        <rdfs:comment>Specifies the high-level class of this cyber observation source.</rdfs:comment>
        <rdfs:isDefinedBy rdf:resource="http://cybox.mitre.org/cyboxCommon"/>
        <rdfs:label>Source Class</rdfs:label>
    </owl:DatatypeProperty>
    


    <!-- http://cybox.mitre.org/cyboxCommon#sourceDescription -->

    <owl:DatatypeProperty rdf:about="http://cybox.mitre.org/cyboxCommon#sourceDescription">
        <rdfs:range rdf:resource="http://www.w3.org/2001/XMLSchema#string"/>
        <rdfs:comment>Specifies a generalized but structured description of this cyber observation source.</rdfs:comment>
        <rdfs:isDefinedBy rdf:resource="http://cybox.mitre.org/cyboxCommon"/>
        <rdfs:label>Source Description</rdfs:label>
    </owl:DatatypeProperty>
    


    <!-- http://cybox.mitre.org/cyboxCommon#sourceName -->

    <owl:DatatypeProperty rdf:about="http://cybox.mitre.org/cyboxCommon#sourceName">
        <rdfs:range rdf:resource="http://www.w3.org/2001/XMLSchema#string"/>
        <rdfs:comment>Specifies a relevant name to this Discovery Method.</rdfs:comment>
        <rdfs:isDefinedBy rdf:resource="http://cybox.mitre.org/cyboxCommon"/>
        <rdfs:label>Source Name</rdfs:label>
    </owl:DatatypeProperty>
    


    <!-- http://cybox.mitre.org/cyboxCommon#sourceType -->

    <owl:DatatypeProperty rdf:about="http://cybox.mitre.org/cyboxCommon#sourceType">
        <rdfs:range>
            <rdfs:Datatype>
                <owl:oneOf>
                    <rdf:Description>
                        <rdf:type rdf:resource="http://www.w3.org/1999/02/22-rdf-syntax-ns#List"/>
                        <rdf:first rdf:datatype="http://www.w3.org/2001/XMLSchema#string">Analysis</rdf:first>
                        <rdf:rest>
                            <rdf:Description>
                                <rdf:type rdf:resource="http://www.w3.org/1999/02/22-rdf-syntax-ns#List"/>
                                <rdf:first rdf:datatype="http://www.w3.org/2001/XMLSchema#string">Information Source</rdf:first>
                                <rdf:rest>
                                    <rdf:Description>
                                        <rdf:type rdf:resource="http://www.w3.org/1999/02/22-rdf-syntax-ns#List"/>
                                        <rdf:first rdf:datatype="http://www.w3.org/2001/XMLSchema#string">Tool</rdf:first>
                                        <rdf:rest rdf:resource="http://www.w3.org/1999/02/22-rdf-syntax-ns#nil"/>
                                    </rdf:Description>
                                </rdf:rest>
                            </rdf:Description>
                        </rdf:rest>
                    </rdf:Description>
                </owl:oneOf>
            </rdfs:Datatype>
        </rdfs:range>
        <rdfs:comment>Specifies the broad type of this cyber observation source.</rdfs:comment>
        <rdfs:isDefinedBy rdf:resource="http://cybox.mitre.org/cyboxCommon"/>
        <rdfs:label>Source Type</rdfs:label>
    </owl:DatatypeProperty>
    


    <!-- http://cybox.mitre.org/cyboxCommon#stringLanguage -->

    <owl:DatatypeProperty rdf:about="http://cybox.mitre.org/cyboxCommon#stringLanguage">
        <rdfs:range rdf:resource="http://www.w3.org/2001/XMLSchema#string"/>
        <rdfs:comment>Specifies the language the string is written in, e.g. English.

For consistency, we strongly recommend using the ISO 639-2 language code, if available. Please see http://www.loc.gov/standards/iso639-2/php/code_list.php for a list of ISO 639-2 codes.</rdfs:comment>
        <rdfs:isDefinedBy rdf:resource="http://cybox.mitre.org/cyboxCommon"/>
        <rdfs:label>Language</rdfs:label>
    </owl:DatatypeProperty>
    


    <!-- http://cybox.mitre.org/cyboxCommon#stringLength -->

    <owl:DatatypeProperty rdf:about="http://cybox.mitre.org/cyboxCommon#stringLength">
        <rdfs:range rdf:resource="http://www.w3.org/2001/XMLSchema#positiveInteger"/>
        <rdfs:comment>Specifies the length, in characters, of the string extracted from the CybOX object.</rdfs:comment>
        <rdfs:isDefinedBy rdf:resource="http://cybox.mitre.org/cyboxCommon"/>
        <rdfs:label>length</rdfs:label>
    </owl:DatatypeProperty>
    


    <!-- http://cybox.mitre.org/cyboxCommon#stringValue -->

    <owl:DatatypeProperty rdf:about="http://cybox.mitre.org/cyboxCommon#stringValue">
        <rdfs:range rdf:resource="http://www.w3.org/2001/XMLSchema#string"/>
        <rdfs:comment>Specifies the actual value of the string extracted from the CybOX object, if it is capable of being represented in the encoding scheme used in the document (most commonly UTF-8).</rdfs:comment>
        <rdfs:isDefinedBy rdf:resource="http://cybox.mitre.org/cyboxCommon"/>
        <rdfs:label>String Value</rdfs:label>
    </owl:DatatypeProperty>
    


    <!-- http://cybox.mitre.org/cyboxCommon#time.endDateTime -->

    <owl:DatatypeProperty rdf:about="http://cybox.mitre.org/cyboxCommon#time.endDateTime">
        <rdfs:range rdf:resource="http://www.w3.org/2001/XMLSchema#dateTime"/>
        <rdfs:comment>Specifies the ending time for this construct. 

In order to avoid ambiguity, it is strongly suggest that all timestamps in this field include a specification of the timezone if it is known.</rdfs:comment>
        <rdfs:isDefinedBy rdf:resource="http://cybox.mitre.org/cyboxCommon"/>
        <rdfs:label>End Time</rdfs:label>
    </owl:DatatypeProperty>
    


    <!-- http://cybox.mitre.org/cyboxCommon#time.producedDateTime -->

    <owl:DatatypeProperty rdf:about="http://cybox.mitre.org/cyboxCommon#time.producedDateTime">
        <rdfs:range rdf:resource="http://www.w3.org/2001/XMLSchema#dateTime"/>
        <rdfs:comment>Specifies the time that this construct was produced. 

In order to avoid ambiguity, it is strongly suggest that all timestamps in this field include a specification of the timezone if it is known.</rdfs:comment>
        <rdfs:isDefinedBy rdf:resource="http://cybox.mitre.org/cyboxCommon"/>
        <rdfs:label>Produced Time</rdfs:label>
    </owl:DatatypeProperty>
    


    <!-- http://cybox.mitre.org/cyboxCommon#time.receivedDateTime -->

    <owl:DatatypeProperty rdf:about="http://cybox.mitre.org/cyboxCommon#time.receivedDateTime">
        <rdfs:range rdf:resource="http://www.w3.org/2001/XMLSchema#dateTime"/>
        <rdfs:comment>Specifies the time that this construct was received. 

In order to avoid ambiguity, it is strongly suggest that all timestamps in this field include a specification of the timezone if it is known.</rdfs:comment>
        <rdfs:isDefinedBy rdf:resource="http://cybox.mitre.org/cyboxCommon"/>
        <rdfs:label>Received Time</rdfs:label>
    </owl:DatatypeProperty>
    


    <!-- http://cybox.mitre.org/cyboxCommon#time.startDateTime -->

    <owl:DatatypeProperty rdf:about="http://cybox.mitre.org/cyboxCommon#time.startDateTime">
        <rdfs:range rdf:resource="http://www.w3.org/2001/XMLSchema#dateTime"/>
        <rdfs:comment>Specifies the starting time for this construct. 

In order to avoid ambiguity, it is strongly suggest that all timestamps in this field include a specification of the timezone if it is known.</rdfs:comment>
        <rdfs:isDefinedBy rdf:resource="http://cybox.mitre.org/cyboxCommon"/>
        <rdfs:label>Start Time</rdfs:label>
    </owl:DatatypeProperty>
    


    <!-- http://cybox.mitre.org/cyboxCommon#toolDescription -->

    <owl:DatatypeProperty rdf:about="http://cybox.mitre.org/cyboxCommon#toolDescription">
        <rdfs:range rdf:resource="http://www.w3.org/2001/XMLSchema#string"/>
        <rdfs:comment>Specifies a generalized but structured descriptive information for this tool.</rdfs:comment>
        <rdfs:isDefinedBy rdf:resource="http://cybox.mitre.org/cyboxCommon"/>
        <rdfs:label>Tool Description</rdfs:label>
    </owl:DatatypeProperty>
    


    <!-- http://cybox.mitre.org/cyboxCommon#toolHash.value -->

    <owl:DatatypeProperty rdf:about="http://cybox.mitre.org/cyboxCommon#toolHash.value">
        <rdfs:range rdf:resource="http://www.w3.org/2001/XMLSchema#string"/>
        <rdfs:comment>Specifies the values, in the format of &apos;hash-type:hash-value&apos;, for any hash computed on the tool file content in order to verify its integrity</rdfs:comment>
        <rdfs:isDefinedBy rdf:resource="http://cybox.mitre.org/cyboxCommon"/>
        <rdfs:label>Tool Hash Value</rdfs:label>
    </owl:DatatypeProperty>
    


    <!-- http://cybox.mitre.org/cyboxCommon#toolName -->

    <owl:DatatypeProperty rdf:about="http://cybox.mitre.org/cyboxCommon#toolName">
        <rdfs:range rdf:resource="http://www.w3.org/2001/XMLSchema#string"/>
        <rdfs:comment>Specifies the name of the tool.</rdfs:comment>
        <rdfs:isDefinedBy rdf:resource="http://cybox.mitre.org/cyboxCommon"/>
        <rdfs:label>Name</rdfs:label>
    </owl:DatatypeProperty>
    


    <!-- http://cybox.mitre.org/cyboxCommon#toolServicePack -->

    <owl:DatatypeProperty rdf:about="http://cybox.mitre.org/cyboxCommon#toolServicePack">
        <rdfs:range rdf:resource="http://www.w3.org/2001/XMLSchema#string"/>
        <rdfs:comment>Specifies an appropriate service pack descriptor for this tool.</rdfs:comment>
        <rdfs:isDefinedBy rdf:resource="http://cybox.mitre.org/cyboxCommon"/>
        <rdfs:label>Service Pack</rdfs:label>
    </owl:DatatypeProperty>
    


    <!-- http://cybox.mitre.org/cyboxCommon#toolSpecificData -->

    <owl:DatatypeProperty rdf:about="http://cybox.mitre.org/cyboxCommon#toolSpecificData">
        <rdfs:range rdf:resource="http://www.w3.org/2001/XMLSchema#anyURI"/>
    </owl:DatatypeProperty>
    


    <!-- http://cybox.mitre.org/cyboxCommon#toolType -->

    <owl:DatatypeProperty rdf:about="http://cybox.mitre.org/cyboxCommon#toolType">
        <rdfs:range rdf:resource="http://www.w3.org/2001/XMLSchema#string"/>
        <rdfs:comment>Specifies the type of information source leveraged for this cyber observation source.</rdfs:comment>
        <rdfs:isDefinedBy rdf:resource="http://cybox.mitre.org/cyboxCommon"/>
        <rdfs:label>Tool Type</rdfs:label>
    </owl:DatatypeProperty>
    


    <!-- http://cybox.mitre.org/cyboxCommon#toolVersion -->

    <owl:DatatypeProperty rdf:about="http://cybox.mitre.org/cyboxCommon#toolVersion">
        <rdfs:range rdf:resource="http://www.w3.org/2001/XMLSchema#string"/>
        <rdfs:comment>Specifies an appropriate version descriptor of this tool.</rdfs:comment>
        <rdfs:isDefinedBy rdf:resource="http://cybox.mitre.org/cyboxCommon"/>
        <rdfs:label>Version</rdfs:label>
    </owl:DatatypeProperty>
    


    <!-- http://cybox.mitre.org/cyboxCommon#triggerPoint -->

    <owl:DatatypeProperty rdf:about="http://cybox.mitre.org/cyboxCommon#triggerPoint">
        <rdfs:range rdf:resource="http://www.w3.org/2001/XMLSchema#hexBinary"/>
        <rdfs:comment>Specifies the offset within the hashed object of the trigger point for this segment.</rdfs:comment>
        <rdfs:isDefinedBy rdf:resource="http://cybox.mitre.org/cyboxCommon"/>
        <rdfs:label>Trigger Point</rdfs:label>
    </owl:DatatypeProperty>
    


    <!-- http://cybox.mitre.org/cyboxCommon#usageContextAssumptions -->

    <owl:DatatypeProperty rdf:about="http://cybox.mitre.org/cyboxCommon#usageContextAssumptions">
        <rdfs:range rdf:resource="http://www.w3.org/2001/XMLSchema#string"/>
        <rdfs:comment>Specifies descriptions of the various relevant usage context assumptions for this tool.</rdfs:comment>
        <rdfs:isDefinedBy rdf:resource="http://cybox.mitre.org/cyboxCommon"/>
        <rdfs:label>Usage Context Assumptions</rdfs:label>
    </owl:DatatypeProperty>
    


    <!-- http://cybox.mitre.org/cyboxCommon#vendorName -->

    <owl:DatatypeProperty rdf:about="http://cybox.mitre.org/cyboxCommon#vendorName">
        <rdfs:range rdf:resource="http://www.w3.org/2001/XMLSchema#string"/>
        <rdfs:comment>Specifies the name of the vendor that created the tool</rdfs:comment>
        <rdfs:isDefinedBy rdf:resource="http://cybox.mitre.org/cyboxCommon"/>
        <rdfs:label>Vendor Name</rdfs:label>
    </owl:DatatypeProperty>
    


    <!-- 
    ///////////////////////////////////////////////////////////////////////////////////////
    //
    // Classes
    //
    ///////////////////////////////////////////////////////////////////////////////////////
     -->

    


    <!-- http://cpe.mitre.org/cpe#Platform -->

    <owl:Class rdf:about="http://cpe.mitre.org/cpe#Platform"/>
    


    <!-- http://cybox.mitre.org/cyboxCommon#ByteRun -->

    <owl:Class rdf:about="http://cybox.mitre.org/cyboxCommon#ByteRun">
        <rdfs:subClassOf>
            <owl:Restriction>
                <owl:onProperty rdf:resource="http://cybox.mitre.org/cyboxCommon#byteRunData"/>
                <owl:someValuesFrom rdf:resource="http://www.w3.org/2000/01/rdf-schema#Literal"/>
            </owl:Restriction>
        </rdfs:subClassOf>
        <rdfs:subClassOf>
            <owl:Restriction>
                <owl:onProperty rdf:resource="http://cybox.mitre.org/cyboxCommon#byteRunLength"/>
                <owl:someValuesFrom rdf:resource="http://www.w3.org/2000/01/rdf-schema#Literal"/>
            </owl:Restriction>
        </rdfs:subClassOf>
        <rdfs:subClassOf>
            <owl:Restriction>
                <owl:onProperty rdf:resource="http://cybox.mitre.org/cyboxCommon#fileSystemOffset"/>
                <owl:someValuesFrom rdf:resource="http://www.w3.org/2000/01/rdf-schema#Literal"/>
            </owl:Restriction>
        </rdfs:subClassOf>
        <rdfs:subClassOf>
            <owl:Restriction>
                <owl:onProperty rdf:resource="http://cybox.mitre.org/cyboxCommon#id"/>
                <owl:someValuesFrom rdf:resource="http://www.w3.org/2000/01/rdf-schema#Literal"/>
            </owl:Restriction>
        </rdfs:subClassOf>
        <rdfs:subClassOf>
            <owl:Restriction>
                <owl:onProperty rdf:resource="http://cybox.mitre.org/cyboxCommon#imageOffset"/>
                <owl:someValuesFrom rdf:resource="http://www.w3.org/2000/01/rdf-schema#Literal"/>
            </owl:Restriction>
        </rdfs:subClassOf>
        <rdfs:subClassOf>
            <owl:Restriction>
                <owl:onProperty rdf:resource="http://cybox.mitre.org/cyboxCommon#offset"/>
                <owl:someValuesFrom rdf:resource="http://www.w3.org/2000/01/rdf-schema#Literal"/>
            </owl:Restriction>
        </rdfs:subClassOf>
        <rdfs:comment>Characterize a list of byte runs from within a raw object.</rdfs:comment>
        <rdfs:isDefinedBy rdf:resource="http://cybox.mitre.org/cyboxCommon"/>
        <rdfs:label>Byte Run</rdfs:label>
    </owl:Class>
    


    <!-- http://cybox.mitre.org/cyboxCommon#Compiler -->

    <owl:Class rdf:about="http://cybox.mitre.org/cyboxCommon#Compiler">
        <rdfs:subClassOf>
            <owl:Restriction>
                <owl:onProperty rdf:resource="http://cybox.mitre.org/cyboxCommon#compiler.platformSpecification"/>
                <owl:someValuesFrom rdf:resource="http://www.w3.org/2002/07/owl#Thing"/>
            </owl:Restriction>
        </rdfs:subClassOf>
        <rdfs:subClassOf>
            <owl:Restriction>
                <owl:onProperty rdf:resource="http://cybox.mitre.org/cyboxCommon#compilerName"/>
                <owl:someValuesFrom rdf:resource="http://www.w3.org/2000/01/rdf-schema#Literal"/>
            </owl:Restriction>
        </rdfs:subClassOf>
        <rdfs:subClassOf>
            <owl:Restriction>
                <owl:onProperty rdf:resource="http://cybox.mitre.org/cyboxCommon#compilerVersion"/>
                <owl:someValuesFrom rdf:resource="http://www.w3.org/2000/01/rdf-schema#Literal"/>
            </owl:Restriction>
        </rdfs:subClassOf>
        <rdfs:comment>Characterizes a single compiler utilized during this build of this application.</rdfs:comment>
        <rdfs:isDefinedBy rdf:resource="http://cybox.mitre.org/cyboxCommon"/>
        <rdfs:label>Compiler</rdfs:label>
    </owl:Class>
    


    <!-- http://cybox.mitre.org/cyboxCommon#ConfigurationSetting -->

    <owl:Class rdf:about="http://cybox.mitre.org/cyboxCommon#ConfigurationSetting">
        <rdfs:subClassOf>
            <owl:Restriction>
                <owl:onProperty rdf:resource="http://cybox.mitre.org/cyboxCommon#settingDescription"/>
                <owl:someValuesFrom rdf:resource="http://www.w3.org/2000/01/rdf-schema#Literal"/>
            </owl:Restriction>
        </rdfs:subClassOf>
        <rdfs:subClassOf>
            <owl:Restriction>
                <owl:onProperty rdf:resource="http://cybox.mitre.org/cyboxCommon#settingName"/>
                <owl:someValuesFrom rdf:resource="http://www.w3.org/2000/01/rdf-schema#Literal"/>
            </owl:Restriction>
        </rdfs:subClassOf>
        <rdfs:subClassOf>
            <owl:Restriction>
                <owl:onProperty rdf:resource="http://cybox.mitre.org/cyboxCommon#settingType"/>
                <owl:someValuesFrom rdf:resource="http://www.w3.org/2000/01/rdf-schema#Literal"/>
            </owl:Restriction>
        </rdfs:subClassOf>
        <rdfs:subClassOf>
            <owl:Restriction>
                <owl:onProperty rdf:resource="http://cybox.mitre.org/cyboxCommon#settingValue"/>
                <owl:someValuesFrom rdf:resource="http://www.w3.org/2000/01/rdf-schema#Literal"/>
            </owl:Restriction>
        </rdfs:subClassOf>
        <rdfs:comment>Characterizes a particular configuration setting for a tool, application or other cyber object.</rdfs:comment>
        <rdfs:isDefinedBy rdf:resource="http://cybox.mitre.org/cyboxCommon"/>
        <rdfs:label>Configuration Setting</rdfs:label>
    </owl:Class>
    


    <!-- http://cybox.mitre.org/cyboxCommon#Contributor -->

    <owl:Class rdf:about="http://cybox.mitre.org/cyboxCommon#Contributor">
        <rdfs:subClassOf>
            <owl:Restriction>
                <owl:onProperty rdf:resource="http://cybox.mitre.org/cyboxCommon#individualDetails"/>
                <owl:someValuesFrom rdf:resource="http://www.w3.org/2002/07/owl#Thing"/>
            </owl:Restriction>
        </rdfs:subClassOf>
        <rdfs:subClassOf>
            <owl:Restriction>
                <owl:onProperty rdf:resource="http://cybox.mitre.org/cyboxCommon#locationDetails"/>
                <owl:someValuesFrom rdf:resource="http://www.w3.org/2002/07/owl#Thing"/>
            </owl:Restriction>
        </rdfs:subClassOf>
        <rdfs:subClassOf>
            <owl:Restriction>
                <owl:onProperty rdf:resource="http://cybox.mitre.org/cyboxCommon#organizationDetails"/>
                <owl:someValuesFrom rdf:resource="http://www.w3.org/2002/07/owl#Thing"/>
            </owl:Restriction>
        </rdfs:subClassOf>
        <rdfs:subClassOf>
            <owl:Restriction>
                <owl:onProperty rdf:resource="http://cybox.mitre.org/cyboxCommon#contributionEndDate"/>
                <owl:someValuesFrom rdf:resource="http://www.w3.org/2000/01/rdf-schema#Literal"/>
            </owl:Restriction>
        </rdfs:subClassOf>
        <rdfs:subClassOf>
            <owl:Restriction>
                <owl:onProperty rdf:resource="http://cybox.mitre.org/cyboxCommon#contributionLocation"/>
                <owl:someValuesFrom rdf:resource="http://www.w3.org/2000/01/rdf-schema#Literal"/>
            </owl:Restriction>
        </rdfs:subClassOf>
        <rdfs:subClassOf>
            <owl:Restriction>
                <owl:onProperty rdf:resource="http://cybox.mitre.org/cyboxCommon#contributionStartDate"/>
                <owl:someValuesFrom rdf:resource="http://www.w3.org/2000/01/rdf-schema#Literal"/>
            </owl:Restriction>
        </rdfs:subClassOf>
        <rdfs:subClassOf>
            <owl:Restriction>
                <owl:onProperty rdf:resource="http://cybox.mitre.org/cyboxCommon#contributorEmail"/>
                <owl:someValuesFrom rdf:resource="http://www.w3.org/2000/01/rdf-schema#Literal"/>
            </owl:Restriction>
        </rdfs:subClassOf>
        <rdfs:subClassOf>
            <owl:Restriction>
                <owl:onProperty rdf:resource="http://cybox.mitre.org/cyboxCommon#contributorName"/>
                <owl:someValuesFrom rdf:resource="http://www.w3.org/2000/01/rdf-schema#Literal"/>
            </owl:Restriction>
        </rdfs:subClassOf>
        <rdfs:subClassOf>
            <owl:Restriction>
                <owl:onProperty rdf:resource="http://cybox.mitre.org/cyboxCommon#contributorOrganization"/>
                <owl:someValuesFrom rdf:resource="http://www.w3.org/2000/01/rdf-schema#Literal"/>
            </owl:Restriction>
        </rdfs:subClassOf>
        <rdfs:subClassOf>
            <owl:Restriction>
                <owl:onProperty rdf:resource="http://cybox.mitre.org/cyboxCommon#contributorRole"/>
                <owl:someValuesFrom rdf:resource="http://www.w3.org/2000/01/rdf-schema#Literal"/>
            </owl:Restriction>
        </rdfs:subClassOf>
        <rdfs:comment>Characterizes a description of an individual who contributed as a source of cyber observation data.</rdfs:comment>
        <rdfs:isDefinedBy rdf:resource="http://cybox.mitre.org/cyboxCommon"/>
        <rdfs:label>Contributor</rdfs:label>
    </owl:Class>
    


    <!-- http://cybox.mitre.org/cyboxCommon#DataSegment -->

    <owl:Class rdf:about="http://cybox.mitre.org/cyboxCommon#DataSegment">
        <rdfs:subClassOf>
            <owl:Restriction>
                <owl:onProperty rdf:resource="http://cybox.mitre.org/cyboxCommon#byteOrder"/>
                <owl:someValuesFrom rdf:resource="http://www.w3.org/2000/01/rdf-schema#Literal"/>
            </owl:Restriction>
        </rdfs:subClassOf>
        <rdfs:subClassOf>
            <owl:Restriction>
                <owl:onProperty rdf:resource="http://cybox.mitre.org/cyboxCommon#dataFormat"/>
                <owl:someValuesFrom rdf:resource="http://www.w3.org/2000/01/rdf-schema#Literal"/>
            </owl:Restriction>
        </rdfs:subClassOf>
        <rdfs:subClassOf>
            <owl:Restriction>
                <owl:onProperty rdf:resource="http://cybox.mitre.org/cyboxCommon#dataSegment"/>
                <owl:someValuesFrom rdf:resource="http://www.w3.org/2000/01/rdf-schema#Literal"/>
            </owl:Restriction>
        </rdfs:subClassOf>
        <rdfs:subClassOf>
            <owl:Restriction>
                <owl:onProperty rdf:resource="http://cybox.mitre.org/cyboxCommon#dataSize"/>
                <owl:someValuesFrom rdf:resource="http://www.w3.org/2000/01/rdf-schema#Literal"/>
            </owl:Restriction>
        </rdfs:subClassOf>
        <rdfs:subClassOf>
            <owl:Restriction>
                <owl:onProperty rdf:resource="http://cybox.mitre.org/cyboxCommon#dataSizeUnits"/>
                <owl:someValuesFrom rdf:resource="http://www.w3.org/2000/01/rdf-schema#Literal"/>
            </owl:Restriction>
        </rdfs:subClassOf>
        <rdfs:subClassOf>
            <owl:Restriction>
                <owl:onProperty rdf:resource="http://cybox.mitre.org/cyboxCommon#id"/>
                <owl:someValuesFrom rdf:resource="http://www.w3.org/2000/01/rdf-schema#Literal"/>
            </owl:Restriction>
        </rdfs:subClassOf>
        <rdfs:subClassOf>
            <owl:Restriction>
                <owl:onProperty rdf:resource="http://cybox.mitre.org/cyboxCommon#offset"/>
                <owl:someValuesFrom rdf:resource="http://www.w3.org/2000/01/rdf-schema#Literal"/>
            </owl:Restriction>
        </rdfs:subClassOf>
        <rdfs:subClassOf>
            <owl:Restriction>
                <owl:onProperty rdf:resource="http://cybox.mitre.org/cyboxCommon#searchDistance"/>
                <owl:someValuesFrom rdf:resource="http://www.w3.org/2000/01/rdf-schema#Literal"/>
            </owl:Restriction>
        </rdfs:subClassOf>
        <rdfs:subClassOf>
            <owl:Restriction>
                <owl:onProperty rdf:resource="http://cybox.mitre.org/cyboxCommon#searchWithin"/>
                <owl:someValuesFrom rdf:resource="http://www.w3.org/2000/01/rdf-schema#Literal"/>
            </owl:Restriction>
        </rdfs:subClassOf>
        <rdfs:comment>Characterizes data segments that may be written/read/transmitted or otherwise utilized in actions or behaviors.</rdfs:comment>
        <rdfs:isDefinedBy rdf:resource="http://cybox.mitre.org/cyboxCommon"/>
        <rdfs:label>Data segment</rdfs:label>
    </owl:Class>
    


    <!-- http://cybox.mitre.org/cyboxCommon#Dependency -->

    <owl:Class rdf:about="http://cybox.mitre.org/cyboxCommon#Dependency">
        <rdfs:subClassOf>
            <owl:Restriction>
                <owl:onProperty rdf:resource="http://cybox.mitre.org/cyboxCommon#dependencyDescription"/>
                <owl:someValuesFrom rdf:resource="http://www.w3.org/2000/01/rdf-schema#Literal"/>
            </owl:Restriction>
        </rdfs:subClassOf>
        <rdfs:subClassOf>
            <owl:Restriction>
                <owl:onProperty rdf:resource="http://cybox.mitre.org/cyboxCommon#dependencyType"/>
                <owl:someValuesFrom rdf:resource="http://www.w3.org/2000/01/rdf-schema#Literal"/>
            </owl:Restriction>
        </rdfs:subClassOf>
        <rdfs:comment>Characterizes a single dependency for a tool.</rdfs:comment>
        <rdfs:isDefinedBy rdf:resource="http://cybox.mitre.org/cyboxCommon"/>
        <rdfs:label>Dependency</rdfs:label>
    </owl:Class>
    


    <!-- http://cybox.mitre.org/cyboxCommon#DigitalSignature -->

    <owl:Class rdf:about="http://cybox.mitre.org/cyboxCommon#DigitalSignature">
        <rdfs:subClassOf>
            <owl:Restriction>
                <owl:onProperty rdf:resource="http://cybox.mitre.org/cyboxCommon#certificateIssuer"/>
                <owl:someValuesFrom rdf:resource="http://www.w3.org/2000/01/rdf-schema#Literal"/>
            </owl:Restriction>
        </rdfs:subClassOf>
        <rdfs:subClassOf>
            <owl:Restriction>
                <owl:onProperty rdf:resource="http://cybox.mitre.org/cyboxCommon#certificateSubject"/>
                <owl:someValuesFrom rdf:resource="http://www.w3.org/2000/01/rdf-schema#Literal"/>
            </owl:Restriction>
        </rdfs:subClassOf>
        <rdfs:subClassOf>
            <owl:Restriction>
                <owl:onProperty rdf:resource="http://cybox.mitre.org/cyboxCommon#id"/>
                <owl:someValuesFrom rdf:resource="http://www.w3.org/2000/01/rdf-schema#Literal"/>
            </owl:Restriction>
        </rdfs:subClassOf>
        <rdfs:subClassOf>
            <owl:Restriction>
                <owl:onProperty rdf:resource="http://cybox.mitre.org/cyboxCommon#signatureDescription"/>
                <owl:someValuesFrom rdf:resource="http://www.w3.org/2000/01/rdf-schema#Literal"/>
            </owl:Restriction>
        </rdfs:subClassOf>
        <rdfs:subClassOf>
            <owl:Restriction>
                <owl:onProperty rdf:resource="http://cybox.mitre.org/cyboxCommon#signatureExists"/>
                <owl:someValuesFrom rdf:resource="http://www.w3.org/2000/01/rdf-schema#Literal"/>
            </owl:Restriction>
        </rdfs:subClassOf>
        <rdfs:subClassOf>
            <owl:Restriction>
                <owl:onProperty rdf:resource="http://cybox.mitre.org/cyboxCommon#signatureVerified"/>
                <owl:someValuesFrom rdf:resource="http://www.w3.org/2000/01/rdf-schema#Literal"/>
            </owl:Restriction>
        </rdfs:subClassOf>
        <rdfs:comment>Characterizes some of the basic information about a digital signature.</rdfs:comment>
        <rdfs:isDefinedBy rdf:resource="http://cybox.mitre.org/cyboxCommon"/>
        <rdfs:label>Digital signature</rdfs:label>
    </owl:Class>
    


    <!-- http://cybox.mitre.org/cyboxCommon#EnvironmentVariable -->

    <owl:Class rdf:about="http://cybox.mitre.org/cyboxCommon#EnvironmentVariable">
        <rdfs:subClassOf>
            <owl:Restriction>
                <owl:onProperty rdf:resource="http://cybox.mitre.org/cyboxCommon#envVarName"/>
                <owl:someValuesFrom rdf:resource="http://www.w3.org/2000/01/rdf-schema#Literal"/>
            </owl:Restriction>
        </rdfs:subClassOf>
        <rdfs:subClassOf>
            <owl:Restriction>
                <owl:onProperty rdf:resource="http://cybox.mitre.org/cyboxCommon#envVarValue"/>
                <owl:someValuesFrom rdf:resource="http://www.w3.org/2000/01/rdf-schema#Literal"/>
            </owl:Restriction>
        </rdfs:subClassOf>
        <rdfs:subClassOf>
            <owl:Restriction>
                <owl:onProperty rdf:resource="http://cybox.mitre.org/cyboxCommon#id"/>
                <owl:someValuesFrom rdf:resource="http://www.w3.org/2000/01/rdf-schema#Literal"/>
            </owl:Restriction>
        </rdfs:subClassOf>
        <rdfs:comment>Characterizes an environment variable using a name/value pair.</rdfs:comment>
        <rdfs:isDefinedBy rdf:resource="http://cybox.mitre.org/cyboxCommon"/>
        <rdfs:label>Environment Variable</rdfs:label>
    </owl:Class>
    


    <!-- http://cybox.mitre.org/cyboxCommon#Error -->

    <owl:Class rdf:about="http://cybox.mitre.org/cyboxCommon#Error">
        <rdfs:subClassOf>
            <owl:Restriction>
                <owl:onProperty rdf:resource="http://cybox.mitre.org/cyboxCommon#errorType"/>
                <owl:someValuesFrom rdf:resource="http://www.w3.org/2000/01/rdf-schema#Literal"/>
            </owl:Restriction>
        </rdfs:subClassOf>
        <rdfs:comment>Characterizes a single error generated during the run of the tool.</rdfs:comment>
        <rdfs:isDefinedBy rdf:resource="http://cybox.mitre.org/cyboxCommon"/>
        <rdfs:label>Error</rdfs:label>
    </owl:Class>
    


    <!-- http://cybox.mitre.org/cyboxCommon#ExecutionEnvironment -->

    <owl:Class rdf:about="http://cybox.mitre.org/cyboxCommon#ExecutionEnvironment">
        <rdfs:subClassOf>
            <owl:Restriction>
                <owl:onProperty rdf:resource="http://cybox.mitre.org/cyboxCommon#system"/>
                <owl:someValuesFrom rdf:resource="http://www.w3.org/2002/07/owl#Thing"/>
            </owl:Restriction>
        </rdfs:subClassOf>
        <rdfs:subClassOf>
            <owl:Restriction>
                <owl:onProperty rdf:resource="http://cybox.mitre.org/cyboxCommon#userAccount"/>
                <owl:someValuesFrom rdf:resource="http://www.w3.org/2002/07/owl#Thing"/>
            </owl:Restriction>
        </rdfs:subClassOf>
        <rdfs:subClassOf>
            <owl:Restriction>
                <owl:onProperty rdf:resource="http://cybox.mitre.org/cyboxCommon#commandLine"/>
                <owl:someValuesFrom rdf:resource="http://www.w3.org/2000/01/rdf-schema#Literal"/>
            </owl:Restriction>
        </rdfs:subClassOf>
        <rdfs:subClassOf>
            <owl:Restriction>
                <owl:onProperty rdf:resource="http://cybox.mitre.org/cyboxCommon#time.endDateTime"/>
                <owl:someValuesFrom rdf:resource="http://www.w3.org/2000/01/rdf-schema#Literal"/>
            </owl:Restriction>
        </rdfs:subClassOf>
        <rdfs:subClassOf>
            <owl:Restriction>
                <owl:onProperty rdf:resource="http://cybox.mitre.org/cyboxCommon#time.startDateTime"/>
                <owl:someValuesFrom rdf:resource="http://www.w3.org/2000/01/rdf-schema#Literal"/>
            </owl:Restriction>
        </rdfs:subClassOf>
        <rdfs:comment>Characterizes the execution environment.</rdfs:comment>
        <rdfs:isDefinedBy rdf:resource="http://cybox.mitre.org/cyboxCommon"/>
        <rdfs:label>Execution Environment</rdfs:label>
    </owl:Class>
    


    <!-- http://cybox.mitre.org/cyboxCommon#ExtractedString -->

    <owl:Class rdf:about="http://cybox.mitre.org/cyboxCommon#ExtractedString">
        <rdfs:subClassOf>
            <owl:Restriction>
                <owl:onProperty rdf:resource="http://cybox.mitre.org/cyboxCommon#byteStringValue"/>
                <owl:someValuesFrom rdf:resource="http://www.w3.org/2000/01/rdf-schema#Literal"/>
            </owl:Restriction>
        </rdfs:subClassOf>
        <rdfs:subClassOf>
            <owl:Restriction>
                <owl:onProperty rdf:resource="http://cybox.mitre.org/cyboxCommon#encoding"/>
                <owl:someValuesFrom rdf:resource="http://www.w3.org/2000/01/rdf-schema#Literal"/>
            </owl:Restriction>
        </rdfs:subClassOf>
        <rdfs:subClassOf>
            <owl:Restriction>
                <owl:onProperty rdf:resource="http://cybox.mitre.org/cyboxCommon#englishTranslation"/>
                <owl:someValuesFrom rdf:resource="http://www.w3.org/2000/01/rdf-schema#Literal"/>
            </owl:Restriction>
        </rdfs:subClassOf>
        <rdfs:subClassOf>
            <owl:Restriction>
                <owl:onProperty rdf:resource="http://cybox.mitre.org/cyboxCommon#offsetAddress"/>
                <owl:someValuesFrom rdf:resource="http://www.w3.org/2000/01/rdf-schema#Literal"/>
            </owl:Restriction>
        </rdfs:subClassOf>
        <rdfs:subClassOf>
            <owl:Restriction>
                <owl:onProperty rdf:resource="http://cybox.mitre.org/cyboxCommon#stringLanguage"/>
                <owl:someValuesFrom rdf:resource="http://www.w3.org/2000/01/rdf-schema#Literal"/>
            </owl:Restriction>
        </rdfs:subClassOf>
        <rdfs:subClassOf>
            <owl:Restriction>
                <owl:onProperty rdf:resource="http://cybox.mitre.org/cyboxCommon#stringLength"/>
                <owl:someValuesFrom rdf:resource="http://www.w3.org/2000/01/rdf-schema#Literal"/>
            </owl:Restriction>
        </rdfs:subClassOf>
        <rdfs:subClassOf>
            <owl:Restriction>
                <owl:onProperty rdf:resource="http://cybox.mitre.org/cyboxCommon#stringValue"/>
                <owl:someValuesFrom rdf:resource="http://www.w3.org/2000/01/rdf-schema#Literal"/>
            </owl:Restriction>
        </rdfs:subClassOf>
        <rdfs:comment>Characterizes a single string extracted from a CybOX object.</rdfs:comment>
        <rdfs:isDefinedBy rdf:resource="http://cybox.mitre.org/cyboxCommon"/>
        <rdfs:label>Extracted String</rdfs:label>
    </owl:Class>
    


    <!-- http://cybox.mitre.org/cyboxCommon#FuzzyHashStructure -->

    <owl:Class rdf:about="http://cybox.mitre.org/cyboxCommon#FuzzyHashStructure">
        <rdfs:subClassOf>
            <owl:Restriction>
                <owl:onProperty rdf:resource="http://cybox.mitre.org/cyboxCommon#blockHash.segments"/>
                <owl:someValuesFrom rdf:resource="http://www.w3.org/2002/07/owl#Thing"/>
            </owl:Restriction>
        </rdfs:subClassOf>
        <rdfs:subClassOf>
            <owl:Restriction>
                <owl:onProperty rdf:resource="http://cybox.mitre.org/cyboxCommon#blockHash.fuzzyHashValue"/>
                <owl:someValuesFrom rdf:resource="http://www.w3.org/2000/01/rdf-schema#Literal"/>
            </owl:Restriction>
        </rdfs:subClassOf>
        <rdfs:subClassOf>
            <owl:Restriction>
                <owl:onProperty rdf:resource="http://cybox.mitre.org/cyboxCommon#blockHash.segmentCount"/>
                <owl:someValuesFrom rdf:resource="http://www.w3.org/2000/01/rdf-schema#Literal"/>
            </owl:Restriction>
        </rdfs:subClassOf>
        <rdfs:subClassOf>
            <owl:Restriction>
                <owl:onProperty rdf:resource="http://cybox.mitre.org/cyboxCommon#blockHash.simpleHashValue"/>
                <owl:someValuesFrom rdf:resource="http://www.w3.org/2000/01/rdf-schema#Literal"/>
            </owl:Restriction>
        </rdfs:subClassOf>
        <rdfs:subClassOf>
            <owl:Restriction>
                <owl:onProperty rdf:resource="http://cybox.mitre.org/cyboxCommon#blockSize"/>
                <owl:someValuesFrom rdf:resource="http://www.w3.org/2000/01/rdf-schema#Literal"/>
            </owl:Restriction>
        </rdfs:subClassOf>
        <rdfs:subClassOf>
            <owl:Restriction>
                <owl:onProperty rdf:resource="http://cybox.mitre.org/cyboxCommon#id"/>
                <owl:someValuesFrom rdf:resource="http://www.w3.org/2000/01/rdf-schema#Literal"/>
            </owl:Restriction>
        </rdfs:subClassOf>
        <rdfs:comment>Characterizes the internal components of a cryptograhic fuzzy hash algorithmic calculation.</rdfs:comment>
        <rdfs:isDefinedBy rdf:resource="http://cybox.mitre.org/cyboxCommon"/>
        <rdfs:label>Fuzzy hash structure</rdfs:label>
    </owl:Class>
    


    <!-- http://cybox.mitre.org/cyboxCommon#Hash -->

    <owl:Class rdf:about="http://cybox.mitre.org/cyboxCommon#Hash">
        <rdfs:subClassOf>
            <owl:Restriction>
                <owl:onProperty rdf:resource="http://cybox.mitre.org/cyboxCommon#hashType"/>
                <owl:someValuesFrom rdf:resource="http://www.w3.org/2000/01/rdf-schema#Literal"/>
            </owl:Restriction>
        </rdfs:subClassOf>
        <rdfs:subClassOf>
            <owl:Restriction>
                <owl:onProperty rdf:resource="http://cybox.mitre.org/cyboxCommon#id"/>
                <owl:someValuesFrom rdf:resource="http://www.w3.org/2000/01/rdf-schema#Literal"/>
            </owl:Restriction>
        </rdfs:subClassOf>
        <rdfs:comment>Characterize a single hash value.</rdfs:comment>
        <rdfs:isDefinedBy rdf:resource="http://cybox.mitre.org/cyboxCommon"/>
        <rdfs:label>Hash</rdfs:label>
    </owl:Class>
    


    <!-- http://cybox.mitre.org/cyboxCommon#HashSegment -->

    <owl:Class rdf:about="http://cybox.mitre.org/cyboxCommon#HashSegment">
        <rdfs:subClassOf>
            <owl:Restriction>
                <owl:onProperty rdf:resource="http://cybox.mitre.org/cyboxCommon#id"/>
                <owl:someValuesFrom rdf:resource="http://www.w3.org/2000/01/rdf-schema#Literal"/>
            </owl:Restriction>
        </rdfs:subClassOf>
        <rdfs:subClassOf>
            <owl:Restriction>
                <owl:onProperty rdf:resource="http://cybox.mitre.org/cyboxCommon#rawSegmentContent"/>
                <owl:someValuesFrom rdf:resource="http://www.w3.org/2000/01/rdf-schema#Literal"/>
            </owl:Restriction>
        </rdfs:subClassOf>
        <rdfs:subClassOf>
            <owl:Restriction>
                <owl:onProperty rdf:resource="http://cybox.mitre.org/cyboxCommon#segmentHash.fuzzyHashValue"/>
                <owl:someValuesFrom rdf:resource="http://www.w3.org/2000/01/rdf-schema#Literal"/>
            </owl:Restriction>
        </rdfs:subClassOf>
        <rdfs:subClassOf>
            <owl:Restriction>
                <owl:onProperty rdf:resource="http://cybox.mitre.org/cyboxCommon#segmentHash.simpleHashValue"/>
                <owl:someValuesFrom rdf:resource="http://www.w3.org/2000/01/rdf-schema#Literal"/>
            </owl:Restriction>
        </rdfs:subClassOf>
        <rdfs:subClassOf>
            <owl:Restriction>
                <owl:onProperty rdf:resource="http://cybox.mitre.org/cyboxCommon#triggerPoint"/>
                <owl:someValuesFrom rdf:resource="http://www.w3.org/2000/01/rdf-schema#Literal"/>
            </owl:Restriction>
        </rdfs:subClassOf>
        <rdfs:comment>Characterizes the internal components of a single trigger point-delimited segment in a cryptograhic fuzzy hash algorithmic calculation.</rdfs:comment>
        <rdfs:isDefinedBy rdf:resource="http://cybox.mitre.org/cyboxCommon"/>
        <rdfs:label>Hash Segment</rdfs:label>
    </owl:Class>
    


    <!-- http://cybox.mitre.org/cyboxCommon#InternalString -->

    <owl:Class rdf:about="http://cybox.mitre.org/cyboxCommon#InternalString">
        <rdfs:subClassOf>
            <owl:Restriction>
                <owl:onProperty rdf:resource="http://cybox.mitre.org/cyboxCommon#content"/>
                <owl:someValuesFrom rdf:resource="http://www.w3.org/2000/01/rdf-schema#Literal"/>
            </owl:Restriction>
        </rdfs:subClassOf>
        <rdfs:subClassOf>
            <owl:Restriction>
                <owl:onProperty rdf:resource="http://cybox.mitre.org/cyboxCommon#key"/>
                <owl:someValuesFrom rdf:resource="http://www.w3.org/2000/01/rdf-schema#Literal"/>
            </owl:Restriction>
        </rdfs:subClassOf>
        <rdfs:comment>Characterizes a single internal string instance for this internationalization setting instance.</rdfs:comment>
        <rdfs:isDefinedBy rdf:resource="http://cybox.mitre.org/cyboxCommon"/>
        <rdfs:label>Internal Settings</rdfs:label>
    </owl:Class>
    


    <!-- http://cybox.mitre.org/cyboxCommon#Library -->

    <owl:Class rdf:about="http://cybox.mitre.org/cyboxCommon#Library">
        <rdfs:subClassOf>
            <owl:Restriction>
                <owl:onProperty rdf:resource="http://cybox.mitre.org/cyboxCommon#libraryName"/>
                <owl:someValuesFrom rdf:resource="http://www.w3.org/2000/01/rdf-schema#Literal"/>
            </owl:Restriction>
        </rdfs:subClassOf>
        <rdfs:subClassOf>
            <owl:Restriction>
                <owl:onProperty rdf:resource="http://cybox.mitre.org/cyboxCommon#libraryVersion"/>
                <owl:someValuesFrom rdf:resource="http://www.w3.org/2000/01/rdf-schema#Literal"/>
            </owl:Restriction>
        </rdfs:subClassOf>
        <rdfs:comment>Characterizes a single library incorporated into the build of the tool.</rdfs:comment>
        <rdfs:isDefinedBy rdf:resource="http://cybox.mitre.org/cyboxCommon"/>
        <rdfs:label>Library</rdfs:label>
    </owl:Class>
    


    <!-- http://cybox.mitre.org/cyboxCommon#Location -->

    <owl:Class rdf:about="http://cybox.mitre.org/cyboxCommon#Location">
        <rdfs:subClassOf>
            <owl:Restriction>
                <owl:onProperty rdf:resource="http://cybox.mitre.org/cyboxCommon#locationAddress"/>
                <owl:someValuesFrom rdf:resource="http://www.w3.org/2002/07/owl#Thing"/>
            </owl:Restriction>
        </rdfs:subClassOf>
        <rdfs:subClassOf>
            <owl:Restriction>
                <owl:onProperty rdf:resource="http://cybox.mitre.org/cyboxCommon#id"/>
                <owl:someValuesFrom rdf:resource="http://www.w3.org/2000/01/rdf-schema#Literal"/>
            </owl:Restriction>
        </rdfs:subClassOf>
        <rdfs:subClassOf>
            <owl:Restriction>
                <owl:onProperty rdf:resource="http://cybox.mitre.org/cyboxCommon#locationName"/>
                <owl:someValuesFrom rdf:resource="http://www.w3.org/2000/01/rdf-schema#Literal"/>
            </owl:Restriction>
        </rdfs:subClassOf>
        <rdfs:comment>Characterizes geographic location information.</rdfs:comment>
        <rdfs:isDefinedBy rdf:resource="http://cybox.mitre.org/cyboxCommon"/>
        <rdfs:label>Location</rdfs:label>
    </owl:Class>
    


    <!-- http://cybox.mitre.org/cyboxCommon#MeasureSource -->

    <owl:Class rdf:about="http://cybox.mitre.org/cyboxCommon#MeasureSource">
        <rdfs:subClassOf>
            <owl:Restriction>
                <owl:onProperty rdf:resource="http://cybox.mitre.org/cyboxCommon#observableLocation"/>
                <owl:someValuesFrom rdf:resource="http://www.w3.org/2002/07/owl#Thing"/>
            </owl:Restriction>
        </rdfs:subClassOf>
        <rdfs:subClassOf>
            <owl:Restriction>
                <owl:onProperty rdf:resource="http://cybox.mitre.org/cyboxCommon#observationLocation"/>
                <owl:someValuesFrom rdf:resource="http://www.w3.org/2002/07/owl#Thing"/>
            </owl:Restriction>
        </rdfs:subClassOf>
        <rdfs:subClassOf>
            <owl:Restriction>
                <owl:onProperty rdf:resource="http://cybox.mitre.org/cyboxCommon#platform"/>
                <owl:someValuesFrom rdf:resource="http://www.w3.org/2002/07/owl#Thing"/>
            </owl:Restriction>
        </rdfs:subClassOf>
        <rdfs:subClassOf>
            <owl:Restriction>
                <owl:onProperty rdf:resource="http://cybox.mitre.org/cyboxCommon#processInstance"/>
                <owl:someValuesFrom rdf:resource="http://www.w3.org/2002/07/owl#Thing"/>
            </owl:Restriction>
        </rdfs:subClassOf>
        <rdfs:subClassOf>
            <owl:Restriction>
                <owl:onProperty rdf:resource="http://cybox.mitre.org/cyboxCommon#system"/>
                <owl:someValuesFrom rdf:resource="http://www.w3.org/2002/07/owl#Thing"/>
            </owl:Restriction>
        </rdfs:subClassOf>
        <rdfs:subClassOf>
            <owl:Restriction>
                <owl:onProperty rdf:resource="http://cybox.mitre.org/cyboxCommon#informationSourceType"/>
                <owl:someValuesFrom rdf:resource="http://www.w3.org/2000/01/rdf-schema#Literal"/>
            </owl:Restriction>
        </rdfs:subClassOf>
        <rdfs:subClassOf>
            <owl:Restriction>
                <owl:onProperty rdf:resource="http://cybox.mitre.org/cyboxCommon#sightingCount"/>
                <owl:someValuesFrom rdf:resource="http://www.w3.org/2000/01/rdf-schema#Literal"/>
            </owl:Restriction>
        </rdfs:subClassOf>
        <rdfs:subClassOf>
            <owl:Restriction>
                <owl:onProperty rdf:resource="http://cybox.mitre.org/cyboxCommon#sourceClass"/>
                <owl:someValuesFrom rdf:resource="http://www.w3.org/2000/01/rdf-schema#Literal"/>
            </owl:Restriction>
        </rdfs:subClassOf>
        <rdfs:subClassOf>
            <owl:Restriction>
                <owl:onProperty rdf:resource="http://cybox.mitre.org/cyboxCommon#sourceDescription"/>
                <owl:someValuesFrom rdf:resource="http://www.w3.org/2000/01/rdf-schema#Literal"/>
            </owl:Restriction>
        </rdfs:subClassOf>
        <rdfs:subClassOf>
            <owl:Restriction>
                <owl:onProperty rdf:resource="http://cybox.mitre.org/cyboxCommon#sourceName"/>
                <owl:someValuesFrom rdf:resource="http://www.w3.org/2000/01/rdf-schema#Literal"/>
            </owl:Restriction>
        </rdfs:subClassOf>
        <rdfs:subClassOf>
            <owl:Restriction>
                <owl:onProperty rdf:resource="http://cybox.mitre.org/cyboxCommon#sourceType"/>
                <owl:someValuesFrom rdf:resource="http://www.w3.org/2000/01/rdf-schema#Literal"/>
            </owl:Restriction>
        </rdfs:subClassOf>
        <rdfs:subClassOf>
            <owl:Restriction>
                <owl:onProperty rdf:resource="http://cybox.mitre.org/cyboxCommon#time.endDateTime"/>
                <owl:someValuesFrom rdf:resource="http://www.w3.org/2000/01/rdf-schema#Literal"/>
            </owl:Restriction>
        </rdfs:subClassOf>
        <rdfs:subClassOf>
            <owl:Restriction>
                <owl:onProperty rdf:resource="http://cybox.mitre.org/cyboxCommon#time.producedDateTime"/>
                <owl:someValuesFrom rdf:resource="http://www.w3.org/2000/01/rdf-schema#Literal"/>
            </owl:Restriction>
        </rdfs:subClassOf>
        <rdfs:subClassOf>
            <owl:Restriction>
                <owl:onProperty rdf:resource="http://cybox.mitre.org/cyboxCommon#time.receivedDateTime"/>
                <owl:someValuesFrom rdf:resource="http://www.w3.org/2000/01/rdf-schema#Literal"/>
            </owl:Restriction>
        </rdfs:subClassOf>
        <rdfs:subClassOf>
            <owl:Restriction>
                <owl:onProperty rdf:resource="http://cybox.mitre.org/cyboxCommon#time.startDateTime"/>
                <owl:someValuesFrom rdf:resource="http://www.w3.org/2000/01/rdf-schema#Literal"/>
            </owl:Restriction>
        </rdfs:subClassOf>
        <rdfs:subClassOf>
            <owl:Restriction>
                <owl:onProperty rdf:resource="http://cybox.mitre.org/cyboxCommon#toolType"/>
                <owl:someValuesFrom rdf:resource="http://www.w3.org/2000/01/rdf-schema#Literal"/>
            </owl:Restriction>
        </rdfs:subClassOf>
        <rdfs:comment>Characterizes a description of a single cyber observation source.</rdfs:comment>
        <rdfs:isDefinedBy rdf:resource="http://cybox.mitre.org/cyboxCommon"/>
        <rdfs:label>Measure Source</rdfs:label>
    </owl:Class>
    


    <!-- http://cybox.mitre.org/cyboxCommon#Metadata -->

    <owl:Class rdf:about="http://cybox.mitre.org/cyboxCommon#Metadata">
        <rdfs:subClassOf>
            <owl:Restriction>
                <owl:onProperty rdf:resource="http://cybox.mitre.org/cyboxCommon#metadataType"/>
                <owl:someValuesFrom rdf:resource="http://www.w3.org/2000/01/rdf-schema#Literal"/>
            </owl:Restriction>
        </rdfs:subClassOf>
        <rdfs:subClassOf>
            <owl:Restriction>
                <owl:onProperty rdf:resource="http://cybox.mitre.org/cyboxCommon#metadataValue"/>
                <owl:someValuesFrom rdf:resource="http://www.w3.org/2000/01/rdf-schema#Literal"/>
            </owl:Restriction>
        </rdfs:subClassOf>
        <rdfs:comment>Characterizes any non-context-specific metadata.</rdfs:comment>
        <rdfs:isDefinedBy rdf:resource="http://cybox.mitre.org/cyboxCommon"/>
        <rdfs:label>Metadata</rdfs:label>
    </owl:Class>
    


    <!-- http://cybox.mitre.org/cyboxCommon#Parameter -->

    <owl:Class rdf:about="http://cybox.mitre.org/cyboxCommon#Parameter">
        <rdfs:subClassOf>
            <owl:Restriction>
                <owl:onProperty rdf:resource="http://cybox.mitre.org/cyboxCommon#ordinalPosition"/>
                <owl:someValuesFrom rdf:resource="http://www.w3.org/2000/01/rdf-schema#Literal"/>
            </owl:Restriction>
        </rdfs:subClassOf>
        <rdfs:subClassOf>
            <owl:Restriction>
                <owl:onProperty rdf:resource="http://cybox.mitre.org/cyboxCommon#parameterName"/>
                <owl:someValuesFrom rdf:resource="http://www.w3.org/2000/01/rdf-schema#Literal"/>
            </owl:Restriction>
        </rdfs:subClassOf>
        <rdfs:subClassOf>
            <owl:Restriction>
                <owl:onProperty rdf:resource="http://cybox.mitre.org/cyboxCommon#parameterValue"/>
                <owl:someValuesFrom rdf:resource="http://www.w3.org/2000/01/rdf-schema#Literal"/>
            </owl:Restriction>
        </rdfs:subClassOf>
        <rdfs:comment>Characterizes a function or argument parameter.</rdfs:comment>
        <rdfs:isDefinedBy rdf:resource="http://cybox.mitre.org/cyboxCommon"/>
        <rdfs:label>Parameter</rdfs:label>
    </owl:Class>
    


    <!-- http://cybox.mitre.org/cyboxCommon#PlatformIdentifier -->

    <owl:Class rdf:about="http://cybox.mitre.org/cyboxCommon#PlatformIdentifier">
        <rdfs:subClassOf>
            <owl:Restriction>
                <owl:onProperty rdf:resource="http://cybox.mitre.org/cyboxCommon#externalReference"/>
                <owl:someValuesFrom rdf:resource="http://www.w3.org/2000/01/rdf-schema#Literal"/>
            </owl:Restriction>
        </rdfs:subClassOf>
        <rdfs:subClassOf>
            <owl:Restriction>
                <owl:onProperty rdf:resource="http://cybox.mitre.org/cyboxCommon#id"/>
                <owl:someValuesFrom rdf:resource="http://www.w3.org/2000/01/rdf-schema#Literal"/>
            </owl:Restriction>
        </rdfs:subClassOf>
        <rdfs:subClassOf>
            <owl:Restriction>
                <owl:onProperty rdf:resource="http://cybox.mitre.org/cyboxCommon#namingSystem"/>
                <owl:someValuesFrom rdf:resource="http://www.w3.org/2000/01/rdf-schema#Literal"/>
            </owl:Restriction>
        </rdfs:subClassOf>
        <rdfs:subClassOf>
            <owl:Restriction>
                <owl:onProperty rdf:resource="http://cybox.mitre.org/cyboxCommon#platformIdentifier"/>
                <owl:someValuesFrom rdf:resource="http://www.w3.org/2000/01/rdf-schema#Literal"/>
            </owl:Restriction>
        </rdfs:subClassOf>
        <rdfs:comment>Characterizes a name for a platform using a particular naming system and also allowing a reference pointing to more information about that naming scheme. For example, one could provide a CPE (Common Platform Enumeration) name using the CPE naming format.   In this case, the system value could be &quot;CPE&quot; while the system_ref value could be &quot;http://scap.nist.gov/specifications/cpe/&quot;.</rdfs:comment>
        <rdfs:isDefinedBy rdf:resource="http://cybox.mitre.org/cyboxCommon"/>
        <rdfs:label>Platform Identifier</rdfs:label>
    </owl:Class>
    


    <!-- http://cybox.mitre.org/cyboxCommon#PlatformSpecification -->

    <owl:Class rdf:about="http://cybox.mitre.org/cyboxCommon#PlatformSpecification">
        <rdfs:subClassOf>
            <owl:Restriction>
                <owl:onProperty rdf:resource="http://cybox.mitre.org/cyboxCommon#id"/>
                <owl:someValuesFrom rdf:resource="http://www.w3.org/2000/01/rdf-schema#Literal"/>
            </owl:Restriction>
        </rdfs:subClassOf>
        <rdfs:subClassOf>
            <owl:Restriction>
                <owl:onProperty rdf:resource="http://cybox.mitre.org/cyboxCommon#namingSystem"/>
                <owl:someValuesFrom rdf:resource="http://www.w3.org/2000/01/rdf-schema#Literal"/>
            </owl:Restriction>
        </rdfs:subClassOf>
        <rdfs:subClassOf>
            <owl:Restriction>
                <owl:onProperty rdf:resource="http://cybox.mitre.org/cyboxCommon#platformDescription"/>
                <owl:someValuesFrom rdf:resource="http://www.w3.org/2000/01/rdf-schema#Literal"/>
            </owl:Restriction>
        </rdfs:subClassOf>
        <rdfs:subClassOf>
            <owl:Restriction>
                <owl:onProperty rdf:resource="http://cybox.mitre.org/cyboxCommon#platformIdentifier"/>
                <owl:someValuesFrom rdf:resource="http://www.w3.org/2000/01/rdf-schema#Literal"/>
            </owl:Restriction>
        </rdfs:subClassOf>
        <rdfs:comment>Characterizes a consistent approach to uniquely specifying a simple identity of a specific platform.</rdfs:comment>
        <rdfs:isDefinedBy rdf:resource="http://cybox.mitre.org/cyboxCommon"/>
        <rdfs:label>Platform Specification</rdfs:label>
    </owl:Class>
    


    <!-- http://cybox.mitre.org/cyboxCommon#Property -->

    <owl:Class rdf:about="http://cybox.mitre.org/cyboxCommon#Property">
        <rdfs:subClassOf>
            <owl:Restriction>
                <owl:onProperty rdf:resource="http://cybox.mitre.org/cyboxCommon#propertyDescription"/>
                <owl:someValuesFrom rdf:resource="http://www.w3.org/2000/01/rdf-schema#Literal"/>
            </owl:Restriction>
        </rdfs:subClassOf>
        <rdfs:subClassOf>
            <owl:Restriction>
                <owl:onProperty rdf:resource="http://cybox.mitre.org/cyboxCommon#propertyName"/>
                <owl:someValuesFrom rdf:resource="http://www.w3.org/2000/01/rdf-schema#Literal"/>
            </owl:Restriction>
        </rdfs:subClassOf>
        <rdfs:subClassOf>
            <owl:Restriction>
                <owl:onProperty rdf:resource="http://cybox.mitre.org/cyboxCommon#propertyValue"/>
                <owl:someValuesFrom rdf:resource="http://www.w3.org/2000/01/rdf-schema#Literal"/>
            </owl:Restriction>
        </rdfs:subClassOf>
        <rdfs:comment>Characterizes the specification of a single Object Property.</rdfs:comment>
        <rdfs:isDefinedBy rdf:resource="http://cybox.mitre.org/cyboxCommon"/>
        <rdfs:label>Property</rdfs:label>
    </owl:Class>
    


    <!-- http://cybox.mitre.org/cyboxCommon#ToolConfiguration -->

    <owl:Class rdf:about="http://cybox.mitre.org/cyboxCommon#ToolConfiguration">
        <rdfs:subClassOf>
            <owl:Restriction>
                <owl:onProperty rdf:resource="http://cybox.mitre.org/cyboxCommon#buildInfo.buildUtilityPlatformSpecification"/>
                <owl:someValuesFrom rdf:resource="http://www.w3.org/2002/07/owl#Thing"/>
            </owl:Restriction>
        </rdfs:subClassOf>
        <rdfs:subClassOf>
            <owl:Restriction>
                <owl:onProperty rdf:resource="http://cybox.mitre.org/cyboxCommon#buildInfo.buildScript"/>
                <owl:someValuesFrom rdf:resource="http://www.w3.org/2000/01/rdf-schema#Literal"/>
            </owl:Restriction>
        </rdfs:subClassOf>
        <rdfs:subClassOf>
            <owl:Restriction>
                <owl:onProperty rdf:resource="http://cybox.mitre.org/cyboxCommon#buildInfo.buildUtilityName"/>
                <owl:someValuesFrom rdf:resource="http://www.w3.org/2000/01/rdf-schema#Literal"/>
            </owl:Restriction>
        </rdfs:subClassOf>
        <rdfs:subClassOf>
            <owl:Restriction>
                <owl:onProperty rdf:resource="http://cybox.mitre.org/cyboxCommon#buildInfo.compilationDate"/>
                <owl:someValuesFrom rdf:resource="http://www.w3.org/2000/01/rdf-schema#Literal"/>
            </owl:Restriction>
        </rdfs:subClassOf>
        <rdfs:subClassOf>
            <owl:Restriction>
                <owl:onProperty rdf:resource="http://cybox.mitre.org/cyboxCommon#buildInfo.configurationSettingDescription"/>
                <owl:someValuesFrom rdf:resource="http://www.w3.org/2000/01/rdf-schema#Literal"/>
            </owl:Restriction>
        </rdfs:subClassOf>
        <rdfs:subClassOf>
            <owl:Restriction>
                <owl:onProperty rdf:resource="http://cybox.mitre.org/cyboxCommon#buildInfo.id"/>
                <owl:someValuesFrom rdf:resource="http://www.w3.org/2000/01/rdf-schema#Literal"/>
            </owl:Restriction>
        </rdfs:subClassOf>
        <rdfs:subClassOf>
            <owl:Restriction>
                <owl:onProperty rdf:resource="http://cybox.mitre.org/cyboxCommon#buildInfo.label"/>
                <owl:someValuesFrom rdf:resource="http://www.w3.org/2000/01/rdf-schema#Literal"/>
            </owl:Restriction>
        </rdfs:subClassOf>
        <rdfs:subClassOf>
            <owl:Restriction>
                <owl:onProperty rdf:resource="http://cybox.mitre.org/cyboxCommon#buildInfo.outputLog"/>
                <owl:someValuesFrom rdf:resource="http://www.w3.org/2000/01/rdf-schema#Literal"/>
            </owl:Restriction>
        </rdfs:subClassOf>
        <rdfs:subClassOf>
            <owl:Restriction>
                <owl:onProperty rdf:resource="http://cybox.mitre.org/cyboxCommon#buildInfo.project"/>
                <owl:someValuesFrom rdf:resource="http://www.w3.org/2000/01/rdf-schema#Literal"/>
            </owl:Restriction>
        </rdfs:subClassOf>
        <rdfs:subClassOf>
            <owl:Restriction>
                <owl:onProperty rdf:resource="http://cybox.mitre.org/cyboxCommon#buildInfo.version"/>
                <owl:someValuesFrom rdf:resource="http://www.w3.org/2000/01/rdf-schema#Literal"/>
            </owl:Restriction>
        </rdfs:subClassOf>
        <rdfs:subClassOf>
            <owl:Restriction>
                <owl:onProperty rdf:resource="http://cybox.mitre.org/cyboxCommon#id"/>
                <owl:someValuesFrom rdf:resource="http://www.w3.org/2000/01/rdf-schema#Literal"/>
            </owl:Restriction>
        </rdfs:subClassOf>
        <rdfs:comment>Characterizes the configuration for a tool used as a cyber observation source.</rdfs:comment>
        <rdfs:isDefinedBy rdf:resource="http://cybox.mitre.org/cyboxCommon"/>
        <rdfs:label>Tool Configuration</rdfs:label>
    </owl:Class>
    


    <!-- http://cybox.mitre.org/cyboxCommon#ToolInformation -->

    <owl:Class rdf:about="http://cybox.mitre.org/cyboxCommon#ToolInformation">
        <rdfs:subClassOf>
            <owl:Restriction>
                <owl:onProperty rdf:resource="http://cybox.mitre.org/cyboxCommon#executionEnvironment"/>
                <owl:someValuesFrom rdf:resource="http://www.w3.org/2002/07/owl#Thing"/>
            </owl:Restriction>
        </rdfs:subClassOf>
        <rdfs:subClassOf>
            <owl:Restriction>
                <owl:onProperty rdf:resource="http://cybox.mitre.org/cyboxCommon#toolConfiguration"/>
                <owl:someValuesFrom rdf:resource="http://www.w3.org/2002/07/owl#Thing"/>
            </owl:Restriction>
        </rdfs:subClassOf>
        <rdfs:subClassOf>
            <owl:Restriction>
                <owl:onProperty rdf:resource="http://cybox.mitre.org/cyboxCommon#vendor"/>
                <owl:someValuesFrom rdf:resource="http://www.w3.org/2002/07/owl#Thing"/>
            </owl:Restriction>
        </rdfs:subClassOf>
        <rdfs:subClassOf>
            <owl:Restriction>
                <owl:onProperty rdf:resource="http://cybox.mitre.org/cyboxCommon#compensationModel"/>
                <owl:someValuesFrom rdf:resource="http://www.w3.org/2000/01/rdf-schema#Literal"/>
            </owl:Restriction>
        </rdfs:subClassOf>
        <rdfs:subClassOf>
            <owl:Restriction>
                <owl:onProperty rdf:resource="http://cybox.mitre.org/cyboxCommon#id"/>
                <owl:someValuesFrom rdf:resource="http://www.w3.org/2000/01/rdf-schema#Literal"/>
            </owl:Restriction>
        </rdfs:subClassOf>
        <rdfs:subClassOf>
            <owl:Restriction>
                <owl:onProperty rdf:resource="http://cybox.mitre.org/cyboxCommon#toolDescription"/>
                <owl:someValuesFrom rdf:resource="http://www.w3.org/2000/01/rdf-schema#Literal"/>
            </owl:Restriction>
        </rdfs:subClassOf>
        <rdfs:subClassOf>
            <owl:Restriction>
                <owl:onProperty rdf:resource="http://cybox.mitre.org/cyboxCommon#toolName"/>
                <owl:someValuesFrom rdf:resource="http://www.w3.org/2000/01/rdf-schema#Literal"/>
            </owl:Restriction>
        </rdfs:subClassOf>
        <rdfs:subClassOf>
            <owl:Restriction>
                <owl:onProperty rdf:resource="http://cybox.mitre.org/cyboxCommon#toolServicePack"/>
                <owl:someValuesFrom rdf:resource="http://www.w3.org/2000/01/rdf-schema#Literal"/>
            </owl:Restriction>
        </rdfs:subClassOf>
        <rdfs:subClassOf>
            <owl:Restriction>
                <owl:onProperty rdf:resource="http://cybox.mitre.org/cyboxCommon#toolType"/>
                <owl:someValuesFrom rdf:resource="http://www.w3.org/2000/01/rdf-schema#Literal"/>
            </owl:Restriction>
        </rdfs:subClassOf>
        <rdfs:subClassOf>
            <owl:Restriction>
                <owl:onProperty rdf:resource="http://cybox.mitre.org/cyboxCommon#toolVersion"/>
                <owl:someValuesFrom rdf:resource="http://www.w3.org/2000/01/rdf-schema#Literal"/>
            </owl:Restriction>
        </rdfs:subClassOf>
        <rdfs:subClassOf>
            <owl:Restriction>
                <owl:onProperty rdf:resource="http://cybox.mitre.org/cyboxCommon#vendorName"/>
                <owl:someValuesFrom rdf:resource="http://www.w3.org/2000/01/rdf-schema#Literal"/>
            </owl:Restriction>
        </rdfs:subClassOf>
        <rdfs:comment>Characterizes the properties of a hardware or software tool, including those related to instances of its use.</rdfs:comment>
        <rdfs:isDefinedBy rdf:resource="http://cybox.mitre.org/cyboxCommon"/>
        <rdfs:label>Tool</rdfs:label>
    </owl:Class>
    


    <!-- http://cybox.mitre.org/cyboxCommon#ToolReference -->

    <owl:Class rdf:about="http://cybox.mitre.org/cyboxCommon#ToolReference">
        <rdfs:subClassOf>
            <owl:Restriction>
                <owl:onProperty rdf:resource="http://cybox.mitre.org/cyboxCommon#externalReference"/>
                <owl:someValuesFrom rdf:resource="http://www.w3.org/2000/01/rdf-schema#Literal"/>
            </owl:Restriction>
        </rdfs:subClassOf>
        <rdfs:subClassOf>
            <owl:Restriction>
                <owl:onProperty rdf:resource="http://cybox.mitre.org/cyboxCommon#referenceType"/>
                <owl:someValuesFrom rdf:resource="http://www.w3.org/2000/01/rdf-schema#Literal"/>
            </owl:Restriction>
        </rdfs:subClassOf>
        <rdfs:comment>Characterizes reference to information or instances of a given tool.</rdfs:comment>
        <rdfs:isDefinedBy rdf:resource="http://cybox.mitre.org/cyboxCommon"/>
        <rdfs:label>Tool reference</rdfs:label>
    </owl:Class>
    


    <!-- http://cybox.mitre.org/objects/Account#UserAccount -->

    <owl:Class rdf:about="http://cybox.mitre.org/objects/Account#UserAccount"/>
    


    <!-- http://cybox.mitre.org/objects/Process#Process -->

    <owl:Class rdf:about="http://cybox.mitre.org/objects/Process#Process"/>
    


    <!-- http://cybox.mitre.org/objects/System#System -->

    <owl:Class rdf:about="http://cybox.mitre.org/objects/System#System"/>
    


    <!-- http://www.oasis-open.org/ciq_xal#Address -->

    <owl:Class rdf:about="http://www.oasis-open.org/ciq_xal#Address"/>
    


    <!-- http://www.oasis-open.org/ciq_xpil#Organization -->

    <owl:Class rdf:about="http://www.oasis-open.org/ciq_xpil#Organization"/>
    


    <!-- http://www.oasis-open.org/ciq_xpil#Person -->

    <owl:Class rdf:about="http://www.oasis-open.org/ciq_xpil#Person"/>
    


    <!-- 
    ///////////////////////////////////////////////////////////////////////////////////////
    //
    // Annotations
    //
    ///////////////////////////////////////////////////////////////////////////////////////
     -->

    <rdf:Description rdf:about="http://cybox.mitre.org/cyboxCommon#toolSpecificData">
        <rdfs:comment>Specifies a flexible mechanism for enabling tool-specific data to be included.</rdfs:comment>
        <rdfs:isDefinedBy rdf:resource="http://cybox.mitre.org/cyboxCommon"/>
        <rdfs:label>Tool Specific Data</rdfs:label>
    </rdf:Description>
</rdf:RDF>



<!-- Generated by the OWL API (version 4.2.6.20160910-2108) https://github.com/owlcs/owlapi -->

