<?xml version="1.0"?>
<rdf:RDF xmlns="http://cybox.mitre.org/objects/EmailMessage#"
     xml:base="http://cybox.mitre.org/objects/EmailMessage"
     xmlns:emailMsgObj="http://cybox.mitre.org/objects/EmailMessage#"
     xmlns:rdf="http://www.w3.org/1999/02/22-rdf-syntax-ns#"
     xmlns:owl="http://www.w3.org/2002/07/owl#"
     xmlns:xml="http://www.w3.org/XML/1998/namespace"
     xmlns:xsd="http://www.w3.org/2001/XMLSchema#"
     xmlns:rdfs="http://www.w3.org/2000/01/rdf-schema#">
    <owl:Ontology rdf:about="http://cybox.mitre.org/objects/EmailMessage">
        <owl:imports rdf:resource="http://cybox.mitre.org/objects/URI"/>
        <owl:imports rdf:resource="http://cybox.mitre.org/cybox_core"/>
        <owl:imports rdf:resource="http://cybox.mitre.org/objects/File"/>
        <rdfs:label>Cyber Observable eXpression (CybOX) Email Message Ontology</rdfs:label>
        <owl:versionInfo rdf:datatype="http://www.w3.org/2001/XMLSchema#string">Created with TopBraid Composer</owl:versionInfo>
        <rdfs:comment>This ontology provides a vocabulary and representation of an Email Message for the  Cyber Observable eXpression (CybOX).  

CybOX  provides a common mechansim (structure and content) to convey the full range of potential cyber observable information and strives to be fully expressive, flexible, extensible, automatable, and as human-readable as possible.

The ontology is based on the Cybox Email Message object schema maintained by The MITRE Corporation copyright 2012-2014.  The version number of the ontology is kept in sync with the schema in order to more easily relate between the ontology and the corresponding schema version.

Copyright (c) 2014, DaedaFusion, LLC.  All rights reserved.</rdfs:comment>
    </owl:Ontology>
    


    <!-- 
    ///////////////////////////////////////////////////////////////////////////////////////
    //
    // Annotation properties
    //
    ///////////////////////////////////////////////////////////////////////////////////////
     -->

    


    <!-- http://www.w3.org/2002/07/owl#cardinality -->

    <owl:AnnotationProperty rdf:about="http://www.w3.org/2002/07/owl#cardinality"/>
    


    <!-- 
    ///////////////////////////////////////////////////////////////////////////////////////
    //
    // Object Properties
    //
    ///////////////////////////////////////////////////////////////////////////////////////
     -->

    


    <!-- http://cybox.mitre.org/objects/EmailMessage#attachments -->

    <owl:ObjectProperty rdf:about="http://cybox.mitre.org/objects/EmailMessage#attachments">
        <rdfs:range rdf:resource="http://cybox.mitre.org/objects/File#File"/>
        <rdfs:comment>Specifies any files that were attached to the email message.</rdfs:comment>
        <rdfs:isDefinedBy rdf:resource="http://cybox.mitre.org/objects/EmailMessage"/>
        <rdfs:label>Attachments</rdfs:label>
    </owl:ObjectProperty>
    


    <!-- http://cybox.mitre.org/objects/EmailMessage#header.bcc -->

    <owl:ObjectProperty rdf:about="http://cybox.mitre.org/objects/EmailMessage#header.bcc">
        <rdfs:range rdf:resource="http://cybox.mitre.org/objects/Address#EmailAddress"/>
        <rdfs:comment>Specifies the email addresses of any recipients that were included in the blind carbon copy header of the email message.</rdfs:comment>
        <rdfs:isDefinedBy rdf:resource="http://cybox.mitre.org/objects/EmailMessage"/>
        <rdfs:label>Blind Carbon Copied (bcc)</rdfs:label>
    </owl:ObjectProperty>
    


    <!-- http://cybox.mitre.org/objects/EmailMessage#header.cc -->

    <owl:ObjectProperty rdf:about="http://cybox.mitre.org/objects/EmailMessage#header.cc">
        <rdfs:range rdf:resource="http://cybox.mitre.org/objects/Address#EmailAddress"/>
        <rdfs:comment>Specifies the email addresses of any recipients that were included in the carbon copy header of the email message.</rdfs:comment>
        <rdfs:isDefinedBy rdf:resource="http://cybox.mitre.org/objects/EmailMessage"/>
        <rdfs:label>Carbon Copied (cc)</rdfs:label>
    </owl:ObjectProperty>
    


    <!-- http://cybox.mitre.org/objects/EmailMessage#header.from -->

    <owl:ObjectProperty rdf:about="http://cybox.mitre.org/objects/EmailMessage#header.from">
        <rdfs:range rdf:resource="http://cybox.mitre.org/objects/Address#EmailAddress"/>
        <rdfs:comment>Specifies the email address of the sender of the email message.</rdfs:comment>
        <rdfs:isDefinedBy rdf:resource="http://cybox.mitre.org/objects/EmailMessage"/>
        <rdfs:label>Header From</rdfs:label>
    </owl:ObjectProperty>
    


    <!-- http://cybox.mitre.org/objects/EmailMessage#header.receivedLines -->

    <owl:ObjectProperty rdf:about="http://cybox.mitre.org/objects/EmailMessage#header.receivedLines">
        <rdfs:range rdf:resource="http://cybox.mitre.org/objects/EmailMessage#EmailReceivedLine"/>
        <rdfs:comment>Specifies one or more &apos;Received&apos; lines that may be included in the email header.</rdfs:comment>
        <rdfs:isDefinedBy rdf:resource="http://cybox.mitre.org/objects/EmailMessage"/>
        <rdfs:label>Received Lines</rdfs:label>
    </owl:ObjectProperty>
    


    <!-- http://cybox.mitre.org/objects/EmailMessage#header.replyTo -->

    <owl:ObjectProperty rdf:about="http://cybox.mitre.org/objects/EmailMessage#header.replyTo">
        <rdfs:range rdf:resource="http://cybox.mitre.org/objects/Address#EmailAddress"/>
        <rdfs:comment>Specifies the email address that should be used when replying to the email message.</rdfs:comment>
        <rdfs:isDefinedBy rdf:resource="http://cybox.mitre.org/objects/EmailMessage"/>
        <rdfs:label>Reply To</rdfs:label>
    </owl:ObjectProperty>
    


    <!-- http://cybox.mitre.org/objects/EmailMessage#header.sender -->

    <owl:ObjectProperty rdf:about="http://cybox.mitre.org/objects/EmailMessage#header.sender">
        <rdfs:range rdf:resource="http://cybox.mitre.org/objects/Address#EmailAddress"/>
        <rdfs:comment>Specifies the email address of the sender who is acting on behalf of the author listed in the From: field.</rdfs:comment>
        <rdfs:isDefinedBy rdf:resource="http://cybox.mitre.org/objects/EmailMessage"/>
        <rdfs:label>Sender</rdfs:label>
    </owl:ObjectProperty>
    


    <!-- http://cybox.mitre.org/objects/EmailMessage#header.to -->

    <owl:ObjectProperty rdf:about="http://cybox.mitre.org/objects/EmailMessage#header.to">
        <rdfs:range rdf:resource="http://cybox.mitre.org/objects/Address#EmailAddress"/>
        <rdfs:comment>Specifies the email addresses of the recipients of the email message.</rdfs:comment>
        <rdfs:isDefinedBy rdf:resource="http://cybox.mitre.org/objects/EmailMessage"/>
        <rdfs:label>To</rdfs:label>
    </owl:ObjectProperty>
    


    <!-- http://cybox.mitre.org/objects/EmailMessage#header.xOriginatingIP -->

    <owl:ObjectProperty rdf:about="http://cybox.mitre.org/objects/EmailMessage#header.xOriginatingIP">
        <rdfs:range>
            <owl:Class>
                <owl:unionOf rdf:parseType="Collection">
                    <rdf:Description rdf:about="http://cybox.mitre.org/objects/Address#IPv4Address"/>
                    <rdf:Description rdf:about="http://cybox.mitre.org/objects/Address#IPv6Address"/>
                </owl:unionOf>
            </owl:Class>
        </rdfs:range>
        <rdfs:comment>Specifies the originating IP Address of the email sender, in terms of their connection to the mail server used to send the email message.

This field is non-standard.</rdfs:comment>
        <rdfs:isDefinedBy rdf:resource="http://cybox.mitre.org/objects/EmailMessage"/>
        <rdfs:label>X-Originating-IP</rdfs:label>
    </owl:ObjectProperty>
    


    <!-- http://cybox.mitre.org/objects/EmailMessage#links -->

    <owl:ObjectProperty rdf:about="http://cybox.mitre.org/objects/EmailMessage#links">
        <rdfs:range rdf:resource="http://cybox.mitre.org/objects/URI#Link"/>
        <rdfs:comment>Specifies any URL links contained within the email message.</rdfs:comment>
        <rdfs:isDefinedBy rdf:resource="http://cybox.mitre.org/objects/EmailMessage"/>
        <rdfs:label>Links</rdfs:label>
    </owl:ObjectProperty>
    


    <!-- 
    ///////////////////////////////////////////////////////////////////////////////////////
    //
    // Data properties
    //
    ///////////////////////////////////////////////////////////////////////////////////////
     -->

    


    <!-- http://cybox.mitre.org/objects/EmailMessage#ID -->

    <owl:DatatypeProperty rdf:about="http://cybox.mitre.org/objects/EmailMessage#ID">
        <rdfs:range rdf:resource="http://www.w3.org/2001/XMLSchema#string"/>
        <rdfs:comment>Specifies the &apos;id&apos; portion of the Received line, if applicable.</rdfs:comment>
        <rdfs:isDefinedBy rdf:resource="http://cybox.mitre.org/objects/EmailMessage"/>
        <rdfs:label>ID</rdfs:label>
    </owl:DatatypeProperty>
    


    <!-- http://cybox.mitre.org/objects/EmailMessage#by -->

    <owl:DatatypeProperty rdf:about="http://cybox.mitre.org/objects/EmailMessage#by">
        <rdfs:range rdf:resource="http://www.w3.org/2001/XMLSchema#string"/>
        <rdfs:comment>Specifies  the &apos;by&apos; portion of the Received line, if applicable.</rdfs:comment>
        <rdfs:isDefinedBy rdf:resource="http://cybox.mitre.org/objects/EmailMessage"/>
        <rdfs:label>By</rdfs:label>
    </owl:DatatypeProperty>
    


    <!-- http://cybox.mitre.org/objects/EmailMessage#emailServer -->

    <owl:DatatypeProperty rdf:about="http://cybox.mitre.org/objects/EmailMessage#emailServer">
        <rdfs:range rdf:resource="http://www.w3.org/2001/XMLSchema#string"/>
        <rdfs:comment>Specifies the relevant email server.</rdfs:comment>
        <rdfs:isDefinedBy rdf:resource="http://cybox.mitre.org/objects/EmailMessage"/>
        <rdfs:label>Email Server</rdfs:label>
    </owl:DatatypeProperty>
    


    <!-- http://cybox.mitre.org/objects/EmailMessage#for -->

    <owl:DatatypeProperty rdf:about="http://cybox.mitre.org/objects/EmailMessage#for">
        <rdfs:range rdf:resource="http://www.w3.org/2001/XMLSchema#string"/>
        <rdfs:comment>Specifies the &apos;for&apos; portion of the Received line, if applicable.</rdfs:comment>
        <rdfs:isDefinedBy rdf:resource="http://cybox.mitre.org/objects/EmailMessage"/>
        <rdfs:label>For</rdfs:label>
    </owl:DatatypeProperty>
    


    <!-- http://cybox.mitre.org/objects/EmailMessage#from -->

    <owl:DatatypeProperty rdf:about="http://cybox.mitre.org/objects/EmailMessage#from">
        <rdfs:range rdf:resource="http://www.w3.org/2001/XMLSchema#string"/>
        <rdfs:comment>Specifies the &apos;from&apos; portion of the Received line, if applicable.</rdfs:comment>
        <rdfs:isDefinedBy rdf:resource="http://cybox.mitre.org/objects/EmailMessage"/>
        <rdfs:label>From</rdfs:label>
    </owl:DatatypeProperty>
    


    <!-- http://cybox.mitre.org/objects/EmailMessage#header.boundary -->

    <owl:DatatypeProperty rdf:about="http://cybox.mitre.org/objects/EmailMessage#header.boundary">
        <rdfs:range rdf:resource="http://www.w3.org/2001/XMLSchema#string"/>
        <rdfs:comment>Specifies a boundary tag that may be included in a MIME multipart message. This boundary tag is used to indicate the parts of a multipart message.</rdfs:comment>
        <rdfs:isDefinedBy rdf:resource="http://cybox.mitre.org/objects/EmailMessage"/>
        <rdfs:label>Boundary</rdfs:label>
    </owl:DatatypeProperty>
    


    <!-- http://cybox.mitre.org/objects/EmailMessage#header.contentType -->

    <owl:DatatypeProperty rdf:about="http://cybox.mitre.org/objects/EmailMessage#header.contentType">
        <rdfs:range rdf:resource="http://www.w3.org/2001/XMLSchema#string"/>
        <rdfs:comment>Specifies the internet media, or MIME, type of the email message content.</rdfs:comment>
        <rdfs:isDefinedBy rdf:resource="http://cybox.mitre.org/objects/EmailMessage"/>
        <rdfs:label>Content Type</rdfs:label>
    </owl:DatatypeProperty>
    


    <!-- http://cybox.mitre.org/objects/EmailMessage#header.dateSentDateTime -->

    <owl:DatatypeProperty rdf:about="http://cybox.mitre.org/objects/EmailMessage#header.dateSentDateTime">
        <rdfs:range rdf:resource="http://www.w3.org/2001/XMLSchema#dateTime"/>
        <rdfs:comment>Specifies the date/time that the email message was sent.</rdfs:comment>
        <rdfs:isDefinedBy rdf:resource="http://cybox.mitre.org/objects/EmailMessage"/>
        <rdfs:label>Date Sent</rdfs:label>
    </owl:DatatypeProperty>
    


    <!-- http://cybox.mitre.org/objects/EmailMessage#header.errorsTo -->

    <owl:DatatypeProperty rdf:about="http://cybox.mitre.org/objects/EmailMessage#header.errorsTo">
        <rdfs:range rdf:resource="http://www.w3.org/2001/XMLSchema#string"/>
        <rdfs:comment>Specifies the entry in the (deprecated) errors_to header of the email message.</rdfs:comment>
        <rdfs:isDefinedBy rdf:resource="http://cybox.mitre.org/objects/EmailMessage"/>
        <rdfs:label>Errors To</rdfs:label>
    </owl:DatatypeProperty>
    


    <!-- http://cybox.mitre.org/objects/EmailMessage#header.inReplyTo -->

    <owl:DatatypeProperty rdf:about="http://cybox.mitre.org/objects/EmailMessage#header.inReplyTo">
        <rdfs:range rdf:resource="http://www.w3.org/2001/XMLSchema#string"/>
        <rdfs:comment>Specifies the message ID of the message that this email is a reply to.</rdfs:comment>
        <rdfs:isDefinedBy rdf:resource="http://cybox.mitre.org/objects/EmailMessage"/>
        <rdfs:label>In Reply To</rdfs:label>
    </owl:DatatypeProperty>
    


    <!-- http://cybox.mitre.org/objects/EmailMessage#header.messageID -->

    <owl:DatatypeProperty rdf:about="http://cybox.mitre.org/objects/EmailMessage#header.messageID">
        <rdfs:range rdf:resource="http://www.w3.org/2001/XMLSchema#string"/>
        <rdfs:comment>Specifies the automatically generated ID of the email message.</rdfs:comment>
        <rdfs:isDefinedBy rdf:resource="http://cybox.mitre.org/objects/EmailMessage"/>
        <rdfs:label>Message ID</rdfs:label>
    </owl:DatatypeProperty>
    


    <!-- http://cybox.mitre.org/objects/EmailMessage#header.mimeVersion -->

    <owl:DatatypeProperty rdf:about="http://cybox.mitre.org/objects/EmailMessage#header.mimeVersion">
        <rdfs:range rdf:resource="http://www.w3.org/2001/XMLSchema#string"/>
        <rdfs:comment>Specifies the version of the MIME formatting used in the email message.</rdfs:comment>
        <rdfs:isDefinedBy rdf:resource="http://cybox.mitre.org/objects/EmailMessage"/>
        <rdfs:label>MIME Version</rdfs:label>
    </owl:DatatypeProperty>
    


    <!-- http://cybox.mitre.org/objects/EmailMessage#header.precedence -->

    <owl:DatatypeProperty rdf:about="http://cybox.mitre.org/objects/EmailMessage#header.precedence">
        <rdfs:range rdf:resource="http://www.w3.org/2001/XMLSchema#string"/>
        <rdfs:comment>Specifies the (non-standard) priority value of the message, which can influence transmission speed and delivery.

Use of this field is typically discouraged, as per IETF RFC2076 (http://www.faqs.org/rfcs/rfc2076.html).</rdfs:comment>
        <rdfs:isDefinedBy rdf:resource="http://cybox.mitre.org/objects/EmailMessage"/>
        <rdfs:label>Precedence</rdfs:label>
    </owl:DatatypeProperty>
    


    <!-- http://cybox.mitre.org/objects/EmailMessage#header.subject -->

    <owl:DatatypeProperty rdf:about="http://cybox.mitre.org/objects/EmailMessage#header.subject">
        <rdfs:range rdf:resource="http://www.w3.org/2001/XMLSchema#string"/>
        <rdfs:comment>Specifies the subject (a brief summary of the message topic) of the email message.</rdfs:comment>
        <rdfs:isDefinedBy rdf:resource="http://cybox.mitre.org/objects/EmailMessage"/>
        <rdfs:label>Subject</rdfs:label>
    </owl:DatatypeProperty>
    


    <!-- http://cybox.mitre.org/objects/EmailMessage#header.userAgent -->

    <owl:DatatypeProperty rdf:about="http://cybox.mitre.org/objects/EmailMessage#header.userAgent">
        <rdfs:range rdf:resource="http://www.w3.org/2001/XMLSchema#string"/>
        <rdfs:comment>Specifies the identity of the email user agent software that may have been used to send the email message.</rdfs:comment>
        <rdfs:isDefinedBy rdf:resource="http://cybox.mitre.org/objects/EmailMessage"/>
        <rdfs:label>User Agent</rdfs:label>
    </owl:DatatypeProperty>
    


    <!-- http://cybox.mitre.org/objects/EmailMessage#header.xMailer -->

    <owl:DatatypeProperty rdf:about="http://cybox.mitre.org/objects/EmailMessage#header.xMailer">
        <rdfs:range rdf:resource="http://www.w3.org/2001/XMLSchema#string"/>
        <rdfs:comment>Specifies the software used to send the email message. This field is non-standard.</rdfs:comment>
        <rdfs:isDefinedBy rdf:resource="http://cybox.mitre.org/objects/EmailMessage"/>
        <rdfs:label>X-Mailer</rdfs:label>
    </owl:DatatypeProperty>
    


    <!-- http://cybox.mitre.org/objects/EmailMessage#header.xPriority -->

    <owl:DatatypeProperty rdf:about="http://cybox.mitre.org/objects/EmailMessage#header.xPriority">
        <rdfs:range rdf:resource="http://www.w3.org/2001/XMLSchema#positiveInteger"/>
        <rdfs:comment>Specifies the numerical priority of the email message. 

This is a non-standard field, but typically a value of &apos;1&apos; is considered the highest priority, &apos;3&apos; is normal, and &apos;5&apos; is the lowest priority.</rdfs:comment>
        <rdfs:isDefinedBy rdf:resource="http://cybox.mitre.org/objects/EmailMessage"/>
        <rdfs:label>X-Priority</rdfs:label>
    </owl:DatatypeProperty>
    


    <!-- http://cybox.mitre.org/objects/EmailMessage#rawBody -->

    <owl:DatatypeProperty rdf:about="http://cybox.mitre.org/objects/EmailMessage#rawBody">
        <rdfs:range rdf:resource="http://www.w3.org/2001/XMLSchema#string"/>
        <rdfs:comment>Specifies the complete (raw) body of the email message.</rdfs:comment>
        <rdfs:isDefinedBy rdf:resource="http://cybox.mitre.org/objects/EmailMessage"/>
        <rdfs:label>Raw Body</rdfs:label>
    </owl:DatatypeProperty>
    


    <!-- http://cybox.mitre.org/objects/EmailMessage#rawHeader -->

    <owl:DatatypeProperty rdf:about="http://cybox.mitre.org/objects/EmailMessage#rawHeader">
        <rdfs:range rdf:resource="http://www.w3.org/2001/XMLSchema#string"/>
        <rdfs:comment>Specifies the complete (raw) headers of the email message.</rdfs:comment>
        <rdfs:isDefinedBy rdf:resource="http://cybox.mitre.org/objects/EmailMessage"/>
        <rdfs:label>Raw Header</rdfs:label>
    </owl:DatatypeProperty>
    


    <!-- http://cybox.mitre.org/objects/EmailMessage#timestamp -->

    <owl:DatatypeProperty rdf:about="http://cybox.mitre.org/objects/EmailMessage#timestamp">
        <rdfs:range rdf:resource="http://www.w3.org/2001/XMLSchema#dateTime"/>
        <rdfs:comment>Specifies the timestamp portion of the Received line, if applicable.</rdfs:comment>
        <rdfs:isDefinedBy rdf:resource="http://cybox.mitre.org/objects/EmailMessage"/>
        <rdfs:label>Timestamp</rdfs:label>
    </owl:DatatypeProperty>
    


    <!-- http://cybox.mitre.org/objects/EmailMessage#via -->

    <owl:DatatypeProperty rdf:about="http://cybox.mitre.org/objects/EmailMessage#via">
        <rdfs:range rdf:resource="http://www.w3.org/2001/XMLSchema#string"/>
        <rdfs:comment>Specifies  the &apos;via&apos; portion of the Received line, if applicable.</rdfs:comment>
        <rdfs:isDefinedBy rdf:resource="http://cybox.mitre.org/objects/EmailMessage"/>
        <rdfs:label>Via</rdfs:label>
    </owl:DatatypeProperty>
    


    <!-- http://cybox.mitre.org/objects/EmailMessage#with -->

    <owl:DatatypeProperty rdf:about="http://cybox.mitre.org/objects/EmailMessage#with">
        <rdfs:range rdf:resource="http://www.w3.org/2001/XMLSchema#string"/>
        <rdfs:comment>Specifies the &apos;with&apos; portion of the Received line, if applicable.</rdfs:comment>
        <rdfs:isDefinedBy rdf:resource="http://cybox.mitre.org/objects/EmailMessage"/>
        <rdfs:label>With</rdfs:label>
    </owl:DatatypeProperty>
    


    <!-- 
    ///////////////////////////////////////////////////////////////////////////////////////
    //
    // Classes
    //
    ///////////////////////////////////////////////////////////////////////////////////////
     -->

    




    <!-- http://cybox.mitre.org/objects/EmailMessage#EmailMessage -->

    <owl:Class rdf:about="http://cybox.mitre.org/objects/EmailMessage#EmailMessage">
        <rdfs:subClassOf rdf:resource="http://cybox.mitre.org/cybox_core#Object"/>
        <rdfs:subClassOf>
            <owl:Restriction>
                <owl:onProperty rdf:resource="http://cybox.mitre.org/objects/EmailMessage#header.from"/>
                <owl:someValuesFrom rdf:resource="http://www.w3.org/2002/07/owl#Thing"/>
            </owl:Restriction>
        </rdfs:subClassOf>
        <rdfs:subClassOf>
            <owl:Restriction>
                <owl:onProperty rdf:resource="http://cybox.mitre.org/objects/EmailMessage#header.replyTo"/>
                <owl:someValuesFrom rdf:resource="http://www.w3.org/2002/07/owl#Thing"/>
            </owl:Restriction>
        </rdfs:subClassOf>
        <rdfs:subClassOf>
            <owl:Restriction>
                <owl:onProperty rdf:resource="http://cybox.mitre.org/objects/EmailMessage#header.xOriginatingIP"/>
                <owl:someValuesFrom rdf:resource="http://www.w3.org/2002/07/owl#Thing"/>
            </owl:Restriction>
        </rdfs:subClassOf>
        <rdfs:subClassOf>
            <owl:Restriction>
                <owl:onProperty rdf:resource="http://cybox.mitre.org/objects/EmailMessage#emailServer"/>
                <owl:someValuesFrom rdf:resource="http://www.w3.org/2000/01/rdf-schema#Literal"/>
            </owl:Restriction>
        </rdfs:subClassOf>
        <rdfs:subClassOf>
            <owl:Restriction>
                <owl:onProperty rdf:resource="http://cybox.mitre.org/objects/EmailMessage#header.boundary"/>
                <owl:someValuesFrom rdf:resource="http://www.w3.org/2000/01/rdf-schema#Literal"/>
            </owl:Restriction>
        </rdfs:subClassOf>
        <rdfs:subClassOf>
            <owl:Restriction>
                <owl:onProperty rdf:resource="http://cybox.mitre.org/objects/EmailMessage#header.contentType"/>
                <owl:someValuesFrom rdf:resource="http://www.w3.org/2000/01/rdf-schema#Literal"/>
            </owl:Restriction>
        </rdfs:subClassOf>
        <rdfs:subClassOf>
            <owl:Restriction>
                <owl:onProperty rdf:resource="http://cybox.mitre.org/objects/EmailMessage#header.errorsTo"/>
                <owl:someValuesFrom rdf:resource="http://www.w3.org/2000/01/rdf-schema#Literal"/>
            </owl:Restriction>
        </rdfs:subClassOf>
        <rdfs:subClassOf>
            <owl:Restriction>
                <owl:onProperty rdf:resource="http://cybox.mitre.org/objects/EmailMessage#header.inReplyTo"/>
                <owl:someValuesFrom rdf:resource="http://www.w3.org/2000/01/rdf-schema#Literal"/>
            </owl:Restriction>
        </rdfs:subClassOf>
        <rdfs:subClassOf>
            <owl:Restriction>
                <owl:onProperty rdf:resource="http://cybox.mitre.org/objects/EmailMessage#header.messageID"/>
                <owl:someValuesFrom rdf:resource="http://www.w3.org/2000/01/rdf-schema#Literal"/>
            </owl:Restriction>
        </rdfs:subClassOf>
        <rdfs:subClassOf>
            <owl:Restriction>
                <owl:onProperty rdf:resource="http://cybox.mitre.org/objects/EmailMessage#header.precedence"/>
                <owl:someValuesFrom rdf:resource="http://www.w3.org/2000/01/rdf-schema#Literal"/>
            </owl:Restriction>
        </rdfs:subClassOf>
        <rdfs:subClassOf>
            <owl:Restriction>
                <owl:onProperty rdf:resource="http://cybox.mitre.org/objects/EmailMessage#header.subject"/>
                <owl:someValuesFrom rdf:resource="http://www.w3.org/2000/01/rdf-schema#Literal"/>
            </owl:Restriction>
        </rdfs:subClassOf>
        <rdfs:subClassOf>
            <owl:Restriction>
                <owl:onProperty rdf:resource="http://cybox.mitre.org/objects/EmailMessage#header.userAgent"/>
                <owl:someValuesFrom rdf:resource="http://www.w3.org/2000/01/rdf-schema#Literal"/>
            </owl:Restriction>
        </rdfs:subClassOf>
        <rdfs:subClassOf>
            <owl:Restriction>
                <owl:onProperty rdf:resource="http://cybox.mitre.org/objects/EmailMessage#header.xMailer"/>
                <owl:someValuesFrom rdf:resource="http://www.w3.org/2000/01/rdf-schema#Literal"/>
            </owl:Restriction>
        </rdfs:subClassOf>
        <rdfs:subClassOf>
            <owl:Restriction>
                <owl:onProperty rdf:resource="http://cybox.mitre.org/objects/EmailMessage#header.xPriority"/>
                <owl:someValuesFrom rdf:resource="http://www.w3.org/2000/01/rdf-schema#Literal"/>
            </owl:Restriction>
        </rdfs:subClassOf>
        <rdfs:subClassOf>
            <owl:Restriction>
                <owl:onProperty rdf:resource="http://cybox.mitre.org/objects/EmailMessage#rawBody"/>
                <owl:someValuesFrom rdf:resource="http://www.w3.org/2000/01/rdf-schema#Literal"/>
            </owl:Restriction>
        </rdfs:subClassOf>
        <rdfs:comment>Characterize an individual email message.</rdfs:comment>
        <rdfs:isDefinedBy rdf:resource="http://cybox.mitre.org/objects/EmailMessage"/>
        <rdfs:label>Email Message</rdfs:label>
    </owl:Class>
    


    <!-- http://cybox.mitre.org/objects/EmailMessage#EmailReceivedLine -->

    <owl:Class rdf:about="http://cybox.mitre.org/objects/EmailMessage#EmailReceivedLine">
        <rdfs:subClassOf>
            <owl:Restriction>
                <owl:onProperty rdf:resource="http://cybox.mitre.org/objects/EmailMessage#ID"/>
                <owl:someValuesFrom rdf:resource="http://www.w3.org/2000/01/rdf-schema#Literal"/>
            </owl:Restriction>
        </rdfs:subClassOf>
        <rdfs:subClassOf>
            <owl:Restriction>
                <owl:onProperty rdf:resource="http://cybox.mitre.org/objects/EmailMessage#by"/>
                <owl:someValuesFrom rdf:resource="http://www.w3.org/2000/01/rdf-schema#Literal"/>
            </owl:Restriction>
        </rdfs:subClassOf>
        <rdfs:subClassOf>
            <owl:Restriction>
                <owl:onProperty rdf:resource="http://cybox.mitre.org/objects/EmailMessage#for"/>
                <owl:someValuesFrom rdf:resource="http://www.w3.org/2000/01/rdf-schema#Literal"/>
            </owl:Restriction>
        </rdfs:subClassOf>
        <rdfs:subClassOf>
            <owl:Restriction>
                <owl:onProperty rdf:resource="http://cybox.mitre.org/objects/EmailMessage#from"/>
                <owl:someValuesFrom rdf:resource="http://www.w3.org/2000/01/rdf-schema#Literal"/>
            </owl:Restriction>
        </rdfs:subClassOf>
        <rdfs:subClassOf>
            <owl:Restriction>
                <owl:onProperty rdf:resource="http://cybox.mitre.org/objects/EmailMessage#timestamp"/>
                <owl:someValuesFrom rdf:resource="http://www.w3.org/2000/01/rdf-schema#Literal"/>
            </owl:Restriction>
        </rdfs:subClassOf>
        <rdfs:subClassOf>
            <owl:Restriction>
                <owl:onProperty rdf:resource="http://cybox.mitre.org/objects/EmailMessage#via"/>
                <owl:someValuesFrom rdf:resource="http://www.w3.org/2000/01/rdf-schema#Literal"/>
            </owl:Restriction>
        </rdfs:subClassOf>
        <rdfs:subClassOf>
            <owl:Restriction>
                <owl:onProperty rdf:resource="http://cybox.mitre.org/objects/EmailMessage#with"/>
                <owl:someValuesFrom rdf:resource="http://www.w3.org/2000/01/rdf-schema#Literal"/>
            </owl:Restriction>
        </rdfs:subClassOf>
        <rdfs:comment>Characterizes  a single &apos;Received&apos; line in an email message header.</rdfs:comment>
        <rdfs:isDefinedBy rdf:resource="http://cybox.mitre.org/objects/EmailMessage"/>
        <rdfs:label>Email Received Line</rdfs:label>
    </owl:Class>
    


</rdf:RDF>



<!-- Generated by the OWL API (version 4.2.6.20160910-2108) https://github.com/owlcs/owlapi -->

