<?xml version="1.0"?>
<rdf:RDF xmlns="http://cybox.mitre.org/objects/EventLog#"
     xml:base="http://cybox.mitre.org/objects/EventLog"
     xmlns:rdf="http://www.w3.org/1999/02/22-rdf-syntax-ns#"
     xmlns:owl="http://www.w3.org/2002/07/owl#"
     xmlns:xml="http://www.w3.org/XML/1998/namespace"
     xmlns:eventLogObj="http://cybox.mitre.org/objects/EventLog#"
     xmlns:xsd="http://www.w3.org/2001/XMLSchema#"
     xmlns:rdfs="http://www.w3.org/2000/01/rdf-schema#">
    <owl:Ontology rdf:about="http://cybox.mitre.org/objects/EventLog">
        <owl:imports rdf:resource="http://cybox.mitre.org/cybox_core"/>
        <rdfs:label>Cyber Observable eXpression (CybOX) Event Log Ontology</rdfs:label>
        <owl:versionInfo rdf:datatype="http://www.w3.org/2001/XMLSchema#string">2.1.0-000</owl:versionInfo>
        <rdfs:comment>This ontology provides a vocabulary and representation of an  EventLog for the  Cyber Observable eXpression (CybOX).  

CybOX  provides a common mechansim (structure and content) to convey the full range of potential cyber observable information and strives to be fully expressive, flexible, extensible, automatable, and as human-readable as possible.

The ontology is based on the CybOX Windows Event Log object schema maintained by The MITRE Corporation copyright 2012-2014.  The version number of the ontology is kept in sync with the schema in order to more easily relate between the ontology and the corresponding schema version.

Copyright (c) 2014, DaedaFusion, LLC.  All rights reserved.</rdfs:comment>
    </owl:Ontology>
    


    <!-- 
    ///////////////////////////////////////////////////////////////////////////////////////
    //
    // Data properties
    //
    ///////////////////////////////////////////////////////////////////////////////////////
     -->

    


    <!-- http://cybox.mitre.org/objects/EventLog#blob -->

    <owl:DatatypeProperty rdf:about="http://cybox.mitre.org/objects/EventLog#blob">
        <rdfs:range rdf:resource="http://www.w3.org/2001/XMLSchema#base64Binary"/>
        <rdfs:comment>Specifies the event data as a binary blob.</rdfs:comment>
        <rdfs:isDefinedBy rdf:resource="http://cybox.mitre.org/objects/EventLog"/>
        <rdfs:label>Blob</rdfs:label>
    </owl:DatatypeProperty>
    


    <!-- http://cybox.mitre.org/objects/EventLog#category -->

    <owl:DatatypeProperty rdf:about="http://cybox.mitre.org/objects/EventLog#category">
        <rdfs:range rdf:resource="http://www.w3.org/2001/XMLSchema#string"/>
        <rdfs:comment>Specifies the text associated with Category Number</rdfs:comment>
        <rdfs:isDefinedBy rdf:resource="http://cybox.mitre.org/objects/EventLog"/>
        <rdfs:label>Category</rdfs:label>
    </owl:DatatypeProperty>
    


    <!-- http://cybox.mitre.org/objects/EventLog#categoryNum -->

    <owl:DatatypeProperty rdf:about="http://cybox.mitre.org/objects/EventLog#categoryNum">
        <rdfs:range rdf:resource="http://www.w3.org/2001/XMLSchema#long"/>
        <rdfs:comment>Specifies the event entry&apos;s category number, as defined by the source.</rdfs:comment>
        <rdfs:isDefinedBy rdf:resource="http://cybox.mitre.org/objects/EventLog"/>
        <rdfs:label>Category Number</rdfs:label>
    </owl:DatatypeProperty>
    


    <!-- http://cybox.mitre.org/objects/EventLog#correlationActivityID -->

    <owl:DatatypeProperty rdf:about="http://cybox.mitre.org/objects/EventLog#correlationActivityID">
        <rdfs:range rdf:resource="http://www.w3.org/2001/XMLSchema#string"/>
        <rdfs:comment>Specifies a globally unique identifier that identifies the current activity.</rdfs:comment>
        <rdfs:isDefinedBy rdf:resource="http://cybox.mitre.org/objects/EventLog"/>
        <rdfs:label>Correlation Activity ID</rdfs:label>
    </owl:DatatypeProperty>
    


    <!-- http://cybox.mitre.org/objects/EventLog#correlationRelatedActivityID -->

    <owl:DatatypeProperty rdf:about="http://cybox.mitre.org/objects/EventLog#correlationRelatedActivityID">
        <rdfs:range rdf:resource="http://www.w3.org/2001/XMLSchema#string"/>
        <rdfs:comment>Specifies a globally unique identifier that identifies the activity to which control was transferred to.</rdfs:comment>
        <rdfs:isDefinedBy rdf:resource="http://cybox.mitre.org/objects/EventLog"/>
        <rdfs:label>Correlation Related Activity ID</rdfs:label>
    </owl:DatatypeProperty>
    


    <!-- http://cybox.mitre.org/objects/EventLog#eventID -->

    <owl:DatatypeProperty rdf:about="http://cybox.mitre.org/objects/EventLog#eventID">
        <rdfs:range rdf:resource="http://www.w3.org/2001/XMLSchema#long"/>
        <rdfs:comment>Specifies the ID of the event for which the event log entry was created.</rdfs:comment>
        <rdfs:isDefinedBy rdf:resource="http://cybox.mitre.org/objects/EventLog"/>
        <rdfs:label>Event ID</rdfs:label>
    </owl:DatatypeProperty>
    


    <!-- http://cybox.mitre.org/objects/EventLog#eventType -->

    <owl:DatatypeProperty rdf:about="http://cybox.mitre.org/objects/EventLog#eventType">
        <rdfs:range rdf:resource="http://www.w3.org/2001/XMLSchema#string"/>
        <rdfs:comment>Specifies the event type associated with the entry in the event log, e.g., warning, information, error.</rdfs:comment>
        <rdfs:isDefinedBy rdf:resource="http://cybox.mitre.org/objects/EventLog"/>
        <rdfs:label>Event Type</rdfs:label>
    </owl:DatatypeProperty>
    


    <!-- http://cybox.mitre.org/objects/EventLog#executionProcessID -->

    <owl:DatatypeProperty rdf:about="http://cybox.mitre.org/objects/EventLog#executionProcessID">
        <rdfs:range rdf:resource="http://www.w3.org/2001/XMLSchema#string"/>
        <rdfs:comment>Specifies the Process ID (PID) of the process which created the event.</rdfs:comment>
        <rdfs:isDefinedBy rdf:resource="http://cybox.mitre.org/objects/EventLog"/>
        <rdfs:label>Execution Process ID</rdfs:label>
    </owl:DatatypeProperty>
    


    <!-- http://cybox.mitre.org/objects/EventLog#executionThreadID -->

    <owl:DatatypeProperty rdf:about="http://cybox.mitre.org/objects/EventLog#executionThreadID">
        <rdfs:range rdf:resource="http://www.w3.org/2001/XMLSchema#string"/>
        <rdfs:comment>Specifies the Thread ID (TID) of the thread which created the event.</rdfs:comment>
        <rdfs:isDefinedBy rdf:resource="http://cybox.mitre.org/objects/EventLog"/>
        <rdfs:label>Execution Thread ID</rdfs:label>
    </owl:DatatypeProperty>
    


    <!-- http://cybox.mitre.org/objects/EventLog#generationDateTime -->

    <owl:DatatypeProperty rdf:about="http://cybox.mitre.org/objects/EventLog#generationDateTime">
        <rdfs:range rdf:resource="http://www.w3.org/2001/XMLSchema#dateTime"/>
        <rdfs:comment>Specifies the date/time the event was generated.</rdfs:comment>
        <rdfs:isDefinedBy rdf:resource="http://cybox.mitre.org/objects/EventLog"/>
        <rdfs:label>Generation Time</rdfs:label>
    </owl:DatatypeProperty>
    


    <!-- http://cybox.mitre.org/objects/EventLog#index -->

    <owl:DatatypeProperty rdf:about="http://cybox.mitre.org/objects/EventLog#index">
        <rdfs:range rdf:resource="http://www.w3.org/2001/XMLSchema#long"/>
        <rdfs:comment>Specifies the index of the event entry in the log.</rdfs:comment>
        <rdfs:isDefinedBy rdf:resource="http://cybox.mitre.org/objects/EventLog"/>
        <rdfs:label>Index</rdfs:label>
    </owl:DatatypeProperty>
    


    <!-- http://cybox.mitre.org/objects/EventLog#logName -->

    <owl:DatatypeProperty rdf:about="http://cybox.mitre.org/objects/EventLog#logName">
        <rdfs:range rdf:resource="http://www.w3.org/2001/XMLSchema#string"/>
        <rdfs:comment>Specifies the name of the log</rdfs:comment>
        <rdfs:isDefinedBy rdf:resource="http://cybox.mitre.org/objects/EventLog"/>
        <rdfs:label>Log Name</rdfs:label>
    </owl:DatatypeProperty>
    


    <!-- http://cybox.mitre.org/objects/EventLog#machine -->

    <owl:DatatypeProperty rdf:about="http://cybox.mitre.org/objects/EventLog#machine">
        <rdfs:range rdf:resource="http://www.w3.org/2001/XMLSchema#string"/>
        <rdfs:comment>Specifies the name of the computer on which the event log entry was generated.</rdfs:comment>
        <rdfs:isDefinedBy rdf:resource="http://cybox.mitre.org/objects/EventLog"/>
        <rdfs:label>Machine</rdfs:label>
    </owl:DatatypeProperty>
    


    <!-- http://cybox.mitre.org/objects/EventLog#message -->

    <owl:DatatypeProperty rdf:about="http://cybox.mitre.org/objects/EventLog#message">
        <rdfs:range rdf:resource="http://www.w3.org/2001/XMLSchema#string"/>
        <rdfs:comment>Specifies the rendered message string for the event.</rdfs:comment>
        <rdfs:isDefinedBy rdf:resource="http://cybox.mitre.org/objects/EventLog"/>
        <rdfs:label>Message</rdfs:label>
    </owl:DatatypeProperty>
    


    <!-- http://cybox.mitre.org/objects/EventLog#reserved -->

    <owl:DatatypeProperty rdf:about="http://cybox.mitre.org/objects/EventLog#reserved">
        <rdfs:range rdf:resource="http://www.w3.org/2001/XMLSchema#long"/>
        <rdfs:comment>Specifies a DWORD value that is always set to ELF_LOG_SIGNATURE (the value 0x654c664c), which is ASCII for eLfL.</rdfs:comment>
        <rdfs:isDefinedBy rdf:resource="http://cybox.mitre.org/objects/EventLog"/>
        <rdfs:label>Reserved</rdfs:label>
    </owl:DatatypeProperty>
    


    <!-- http://cybox.mitre.org/objects/EventLog#source -->

    <owl:DatatypeProperty rdf:about="http://cybox.mitre.org/objects/EventLog#source">
        <rdfs:range rdf:resource="http://www.w3.org/2001/XMLSchema#string"/>
        <rdfs:comment>Specifies the source that logged the event, typically the name of an application or sub-component.</rdfs:comment>
        <rdfs:isDefinedBy rdf:resource="http://cybox.mitre.org/objects/EventLog"/>
        <rdfs:label>Source</rdfs:label>
    </owl:DatatypeProperty>
    


    <!-- http://cybox.mitre.org/objects/EventLog#unformattedMessages -->

    <owl:DatatypeProperty rdf:about="http://cybox.mitre.org/objects/EventLog#unformattedMessages">
        <rdfs:range rdf:resource="http://www.w3.org/2001/XMLSchema#string"/>
        <rdfs:comment>Specifies one or more unformatted messages in the event log entry.</rdfs:comment>
        <rdfs:isDefinedBy rdf:resource="http://cybox.mitre.org/objects/EventLog"/>
        <rdfs:label>Unformatted Messages</rdfs:label>
    </owl:DatatypeProperty>
    


    <!-- http://cybox.mitre.org/objects/EventLog#user -->

    <owl:DatatypeProperty rdf:about="http://cybox.mitre.org/objects/EventLog#user">
        <rdfs:range rdf:resource="http://www.w3.org/2001/XMLSchema#string"/>
        <rdfs:comment>Specifies the name of the user (the security ID) responsible for the event.</rdfs:comment>
        <rdfs:isDefinedBy rdf:resource="http://cybox.mitre.org/objects/EventLog"/>
        <rdfs:label>User</rdfs:label>
    </owl:DatatypeProperty>
    


    <!-- http://cybox.mitre.org/objects/EventLog#writeDateTime -->

    <owl:DatatypeProperty rdf:about="http://cybox.mitre.org/objects/EventLog#writeDateTime">
        <rdfs:range rdf:resource="http://www.w3.org/2001/XMLSchema#dateTime"/>
        <rdfs:comment>Specifies the date/time that the entry was written into the event log.</rdfs:comment>
        <rdfs:isDefinedBy rdf:resource="http://cybox.mitre.org/objects/EventLog"/>
        <rdfs:label>Write Time</rdfs:label>
    </owl:DatatypeProperty>
    


    <!-- 
    ///////////////////////////////////////////////////////////////////////////////////////
    //
    // Classes
    //
    ///////////////////////////////////////////////////////////////////////////////////////
     -->

    

    <!-- http://cybox.mitre.org/objects/EventLog#WindowsEventLog -->

    <owl:Class rdf:about="http://cybox.mitre.org/objects/EventLog#WindowsEventLog">
        <rdfs:subClassOf rdf:resource="http://cybox.mitre.org/cybox_core#Object"/>
        <rdfs:subClassOf>
            <owl:Restriction>
                <owl:onProperty rdf:resource="http://cybox.mitre.org/objects/EventLog#eventID"/>
                <owl:cardinality rdf:datatype="http://www.w3.org/2001/XMLSchema#nonNegativeInteger">1</owl:cardinality>
            </owl:Restriction>
        </rdfs:subClassOf>
        <rdfs:subClassOf>
            <owl:Restriction>
                <owl:onProperty rdf:resource="http://cybox.mitre.org/objects/EventLog#eventType"/>
                <owl:cardinality rdf:datatype="http://www.w3.org/2001/XMLSchema#nonNegativeInteger">1</owl:cardinality>
            </owl:Restriction>
        </rdfs:subClassOf>
        <rdfs:subClassOf>
            <owl:Restriction>
                <owl:onProperty rdf:resource="http://cybox.mitre.org/objects/EventLog#generationDateTime"/>
                <owl:cardinality rdf:datatype="http://www.w3.org/2001/XMLSchema#nonNegativeInteger">1</owl:cardinality>
            </owl:Restriction>
        </rdfs:subClassOf>
        <rdfs:subClassOf>
            <owl:Restriction>
                <owl:onProperty rdf:resource="http://cybox.mitre.org/objects/EventLog#logName"/>
                <owl:cardinality rdf:datatype="http://www.w3.org/2001/XMLSchema#nonNegativeInteger">1</owl:cardinality>
            </owl:Restriction>
        </rdfs:subClassOf>
        <rdfs:subClassOf>
            <owl:Restriction>
                <owl:onProperty rdf:resource="http://cybox.mitre.org/objects/EventLog#source"/>
                <owl:cardinality rdf:datatype="http://www.w3.org/2001/XMLSchema#nonNegativeInteger">1</owl:cardinality>
            </owl:Restriction>
        </rdfs:subClassOf>
        <rdfs:subClassOf>
            <owl:Restriction>
                <owl:onProperty rdf:resource="http://cybox.mitre.org/objects/EventLog#blob"/>
                <owl:maxCardinality rdf:datatype="http://www.w3.org/2001/XMLSchema#nonNegativeInteger">1</owl:maxCardinality>
            </owl:Restriction>
        </rdfs:subClassOf>
        <rdfs:subClassOf>
            <owl:Restriction>
                <owl:onProperty rdf:resource="http://cybox.mitre.org/objects/EventLog#category"/>
                <owl:maxCardinality rdf:datatype="http://www.w3.org/2001/XMLSchema#nonNegativeInteger">1</owl:maxCardinality>
            </owl:Restriction>
        </rdfs:subClassOf>
        <rdfs:subClassOf>
            <owl:Restriction>
                <owl:onProperty rdf:resource="http://cybox.mitre.org/objects/EventLog#categoryNum"/>
                <owl:maxCardinality rdf:datatype="http://www.w3.org/2001/XMLSchema#nonNegativeInteger">1</owl:maxCardinality>
            </owl:Restriction>
        </rdfs:subClassOf>
        <rdfs:subClassOf>
            <owl:Restriction>
                <owl:onProperty rdf:resource="http://cybox.mitre.org/objects/EventLog#correlationActivityID"/>
                <owl:maxCardinality rdf:datatype="http://www.w3.org/2001/XMLSchema#nonNegativeInteger">1</owl:maxCardinality>
            </owl:Restriction>
        </rdfs:subClassOf>
        <rdfs:subClassOf>
            <owl:Restriction>
                <owl:onProperty rdf:resource="http://cybox.mitre.org/objects/EventLog#correlationRelatedActivityID"/>
                <owl:maxCardinality rdf:datatype="http://www.w3.org/2001/XMLSchema#nonNegativeInteger">1</owl:maxCardinality>
            </owl:Restriction>
        </rdfs:subClassOf>
        <rdfs:subClassOf>
            <owl:Restriction>
                <owl:onProperty rdf:resource="http://cybox.mitre.org/objects/EventLog#executionProcessID"/>
                <owl:maxCardinality rdf:datatype="http://www.w3.org/2001/XMLSchema#nonNegativeInteger">1</owl:maxCardinality>
            </owl:Restriction>
        </rdfs:subClassOf>
        <rdfs:subClassOf>
            <owl:Restriction>
                <owl:onProperty rdf:resource="http://cybox.mitre.org/objects/EventLog#executionThreadID"/>
                <owl:maxCardinality rdf:datatype="http://www.w3.org/2001/XMLSchema#nonNegativeInteger">1</owl:maxCardinality>
            </owl:Restriction>
        </rdfs:subClassOf>
        <rdfs:subClassOf>
            <owl:Restriction>
                <owl:onProperty rdf:resource="http://cybox.mitre.org/objects/EventLog#index"/>
                <owl:maxCardinality rdf:datatype="http://www.w3.org/2001/XMLSchema#nonNegativeInteger">1</owl:maxCardinality>
            </owl:Restriction>
        </rdfs:subClassOf>
        <rdfs:subClassOf>
            <owl:Restriction>
                <owl:onProperty rdf:resource="http://cybox.mitre.org/objects/EventLog#machine"/>
                <owl:maxCardinality rdf:datatype="http://www.w3.org/2001/XMLSchema#nonNegativeInteger">1</owl:maxCardinality>
            </owl:Restriction>
        </rdfs:subClassOf>
        <rdfs:subClassOf>
            <owl:Restriction>
                <owl:onProperty rdf:resource="http://cybox.mitre.org/objects/EventLog#message"/>
                <owl:maxCardinality rdf:datatype="http://www.w3.org/2001/XMLSchema#nonNegativeInteger">1</owl:maxCardinality>
            </owl:Restriction>
        </rdfs:subClassOf>
        <rdfs:subClassOf>
            <owl:Restriction>
                <owl:onProperty rdf:resource="http://cybox.mitre.org/objects/EventLog#reserved"/>
                <owl:maxCardinality rdf:datatype="http://www.w3.org/2001/XMLSchema#nonNegativeInteger">1</owl:maxCardinality>
            </owl:Restriction>
        </rdfs:subClassOf>
        <rdfs:subClassOf>
            <owl:Restriction>
                <owl:onProperty rdf:resource="http://cybox.mitre.org/objects/EventLog#user"/>
                <owl:maxCardinality rdf:datatype="http://www.w3.org/2001/XMLSchema#nonNegativeInteger">1</owl:maxCardinality>
            </owl:Restriction>
        </rdfs:subClassOf>
        <rdfs:subClassOf>
            <owl:Restriction>
                <owl:onProperty rdf:resource="http://cybox.mitre.org/objects/EventLog#writeDateTime"/>
                <owl:maxCardinality rdf:datatype="http://www.w3.org/2001/XMLSchema#nonNegativeInteger">1</owl:maxCardinality>
            </owl:Restriction>
        </rdfs:subClassOf>
        <rdfs:comment>Characterize entries in the Windows event log.</rdfs:comment>
        <rdfs:isDefinedBy rdf:resource="http://cybox.mitre.org/objects/EventLog"/>
        <rdfs:label>Windows Event Log</rdfs:label>
    </owl:Class>
</rdf:RDF>



<!-- Generated by the OWL API (version 4.2.6.20160910-2108) https://github.com/owlcs/owlapi -->

