<?xml version="1.0"?>
<rdf:RDF xmlns="http://cybox.mitre.org/objects/NetworkConnection#"
     xml:base="http://cybox.mitre.org/objects/NetworkConnection"
     xmlns:netConnectObj="http://cybox.mitre.org/objects/NetworkConnection#"
     xmlns:rdf="http://www.w3.org/1999/02/22-rdf-syntax-ns#"
     xmlns:owl="http://www.w3.org/2002/07/owl#"
     xmlns:xml="http://www.w3.org/XML/1998/namespace"
     xmlns:xsd="http://www.w3.org/2001/XMLSchema#"
     xmlns:rdfs="http://www.w3.org/2000/01/rdf-schema#">
    <owl:Ontology rdf:about="http://cybox.mitre.org/objects/NetworkConnection">
        <owl:imports rdf:resource="http://cybox.mitre.org/objects/HTTP_Session"/>
        <owl:imports rdf:resource="http://cybox.mitre.org/cybox_core"/>
        <owl:imports rdf:resource="http://cybox.mitre.org/objects/NetworkProtocol"/>
        <owl:imports rdf:resource="http://cybox.mitre.org/objects/DNS"/>
        <owl:imports rdf:resource="http://cybox.mitre.org/objects/Socket_Address"/>
        <owl:versionInfo rdf:datatype="http://www.w3.org/2001/XMLSchema#string">2.1.0-000</owl:versionInfo>
        <rdfs:label>Cyber Observable eXpression (CybOX) Network Connection Ontology</rdfs:label>
        <rdfs:comment>This ontology provides a vocabulary and representation of a Network Connection for the  Cyber Observable eXpression (CybOX).  

CybOX  provides a common mechansim (structure and content) to convey the full range of potential cyber observable information and strives to be fully expressive, flexible, extensible, automatable, and as human-readable as possible.

The ontology is based on the Cybox Network Connection object schema maintained by The MITRE Corporation copyright 2012-2014.  The version number of the ontology is kept in sync with the schema in order to more easily relate between the ontology and the corresponding schema version.

Copyright (c) 2014, DaedaFusion, LLC.  All rights reserved.</rdfs:comment>
    </owl:Ontology>
    


    <!-- 
    ///////////////////////////////////////////////////////////////////////////////////////
    //
    // Object Properties
    //
    ///////////////////////////////////////////////////////////////////////////////////////
     -->

    


    <!-- http://cybox.mitre.org/objects/NetworkConnection#destinationSocketAddress -->

    <owl:ObjectProperty rdf:about="http://cybox.mitre.org/objects/NetworkConnection#destinationSocketAddress">
        <rdfs:range rdf:resource="http://cybox.mitre.org/objects/Socket_Address#SocketAddress"/>
        <rdfs:comment>Specifies the destination socket address, consisting of an IP Address and port number, used in the connection.</rdfs:comment>
        <rdfs:isDefinedBy rdf:resource="http://cybox.mitre.org/objects/NetworkConnection"/>
        <rdfs:label>Destination Socket Address</rdfs:label>
    </owl:ObjectProperty>
    


    <!-- http://cybox.mitre.org/objects/NetworkConnection#layer3Protocol -->

    <owl:ObjectProperty rdf:about="http://cybox.mitre.org/objects/NetworkConnection#layer3Protocol">
        <rdfs:range rdf:resource="http://cybox.mitre.org/objects/NetworkProtocol#NetworkProtocol"/>
        <rdfs:comment>Specifies the particular network (layer 3 in the OSI model) layer protocol used in the connection.</rdfs:comment>
        <rdfs:isDefinedBy rdf:resource="http://cybox.mitre.org/objects/NetworkConnection"/>
        <rdfs:label>Layer 3 Protocols</rdfs:label>
    </owl:ObjectProperty>
    


    <!-- http://cybox.mitre.org/objects/NetworkConnection#layer4Protocol -->

    <owl:ObjectProperty rdf:about="http://cybox.mitre.org/objects/NetworkConnection#layer4Protocol">
        <rdfs:range rdf:resource="http://cybox.mitre.org/objects/NetworkProtocol#NetworkProtocol"/>
        <rdfs:comment>Specifies the particular transport (layer 4 in the OSI model) layer protocol used in the connection.</rdfs:comment>
        <rdfs:isDefinedBy rdf:resource="http://cybox.mitre.org/objects/NetworkConnection"/>
        <rdfs:label>Layer 4 Protocol</rdfs:label>
    </owl:ObjectProperty>
    


    <!-- http://cybox.mitre.org/objects/NetworkConnection#layer7Connection.dnsQuery -->

    <owl:ObjectProperty rdf:about="http://cybox.mitre.org/objects/NetworkConnection#layer7Connection.dnsQuery">
        <rdfs:range rdf:resource="http://cybox.mitre.org/objects/DNS#DNSQuery"/>
        <rdfs:comment>Specifies a single DNS query/answer pair initiated between source and destination IP addresses/ports.</rdfs:comment>
        <rdfs:isDefinedBy rdf:resource="http://cybox.mitre.org/objects/NetworkConnection"/>
        <rdfs:label>Layer 7 Connection DNS Query</rdfs:label>
    </owl:ObjectProperty>
    


    <!-- http://cybox.mitre.org/objects/NetworkConnection#layer7Connection.httpSession -->

    <owl:ObjectProperty rdf:about="http://cybox.mitre.org/objects/NetworkConnection#layer7Connection.httpSession">
        <rdfs:range rdf:resource="http://cybox.mitre.org/objects/HTTP_Session#HTTPSession"/>
        <rdfs:comment>Specifies a single HTTP session initiated between source and destination IP addresses/ports, and includes 1-n HTTP Request/Response pairs.</rdfs:comment>
        <rdfs:isDefinedBy rdf:resource="http://cybox.mitre.org/objects/NetworkConnection"/>
        <rdfs:label>Layer 7 Connection HTTP Session</rdfs:label>
    </owl:ObjectProperty>
    


    <!-- http://cybox.mitre.org/objects/NetworkConnection#layer7Protocol -->

    <owl:ObjectProperty rdf:about="http://cybox.mitre.org/objects/NetworkConnection#layer7Protocol">
        <rdfs:range rdf:resource="http://cybox.mitre.org/objects/NetworkProtocol#NetworkProtocol"/>
        <rdfs:comment>Specifies the particular application (layer 7 in the OSI model) layer protocol used in the connection.</rdfs:comment>
        <rdfs:isDefinedBy rdf:resource="http://cybox.mitre.org/objects/NetworkConnection"/>
        <rdfs:label>Layer7 Protocol</rdfs:label>
    </owl:ObjectProperty>
    


    <!-- http://cybox.mitre.org/objects/NetworkConnection#sourceSocketAddress -->

    <owl:ObjectProperty rdf:about="http://cybox.mitre.org/objects/NetworkConnection#sourceSocketAddress">
        <rdfs:range rdf:resource="http://cybox.mitre.org/objects/Socket_Address#SocketAddress"/>
        <rdfs:comment>Specifies the source socket address, consisting of an IP Address and port number, used in the connection.</rdfs:comment>
        <rdfs:isDefinedBy rdf:resource="http://cybox.mitre.org/objects/NetworkConnection"/>
        <rdfs:label>Source Socket Address</rdfs:label>
    </owl:ObjectProperty>
    


    <!-- 
    ///////////////////////////////////////////////////////////////////////////////////////
    //
    // Data properties
    //
    ///////////////////////////////////////////////////////////////////////////////////////
     -->

    


    <!-- http://cybox.mitre.org/objects/NetworkConnection#destinationTCPState -->

    <owl:DatatypeProperty rdf:about="http://cybox.mitre.org/objects/NetworkConnection#destinationTCPState">
        <rdfs:range rdf:resource="http://www.w3.org/2001/XMLSchema#string"/>
        <rdfs:comment>Specifies the current state of the TCP network connection at the destination, if applicable.</rdfs:comment>
        <rdfs:isDefinedBy rdf:resource="http://cybox.mitre.org/objects/NetworkConnection"/>
        <rdfs:label>Destination TCP State</rdfs:label>
    </owl:DatatypeProperty>
    


    <!-- http://cybox.mitre.org/objects/NetworkConnection#sourceTCPState -->

    <owl:DatatypeProperty rdf:about="http://cybox.mitre.org/objects/NetworkConnection#sourceTCPState">
        <rdfs:range rdf:resource="http://www.w3.org/2001/XMLSchema#string"/>
        <rdfs:comment>Specifies the current state of the TCP network connection at the source, if applicable.</rdfs:comment>
        <rdfs:isDefinedBy rdf:resource="http://cybox.mitre.org/objects/NetworkConnection"/>
        <rdfs:label>Source TCP State</rdfs:label>
    </owl:DatatypeProperty>
    


    <!-- http://cybox.mitre.org/objects/NetworkConnection#tlsUsed -->

    <owl:DatatypeProperty rdf:about="http://cybox.mitre.org/objects/NetworkConnection#tlsUsed">
        <rdfs:range rdf:resource="http://www.w3.org/2001/XMLSchema#boolean"/>
        <rdfs:comment>Specifies whether or not Transport Layer Security (TLS) is used in the network connection.</rdfs:comment>
        <rdfs:isDefinedBy rdf:resource="http://cybox.mitre.org/objects/NetworkConnection"/>
        <rdfs:label>TLS Used</rdfs:label>
    </owl:DatatypeProperty>
    


    <!-- 
    ///////////////////////////////////////////////////////////////////////////////////////
    //
    // Classes
    //
    ///////////////////////////////////////////////////////////////////////////////////////
     -->

    


    <!-- http://cybox.mitre.org/objects/DNS#DNSQuery -->

    <owl:Class rdf:about="http://cybox.mitre.org/objects/DNS#DNSQuery"/>
    


    <!-- http://cybox.mitre.org/objects/HTTP_Session#HTTPSession -->

    <owl:Class rdf:about="http://cybox.mitre.org/objects/HTTP_Session#HTTPSession"/>
    


    <!-- http://cybox.mitre.org/objects/NetworkConnection#NetworkConnection -->

    <owl:Class rdf:about="http://cybox.mitre.org/objects/NetworkConnection#NetworkConnection">
        <rdfs:subClassOf rdf:resource="http://cybox.mitre.org/objects/Socket_Address#SocketAddress"/>
        <rdfs:subClassOf>
            <owl:Restriction>
                <owl:onProperty rdf:resource="http://cybox.mitre.org/objects/NetworkConnection#destinationSocketAddress"/>
                <owl:maxCardinality rdf:datatype="http://www.w3.org/2001/XMLSchema#nonNegativeInteger">1</owl:maxCardinality>
            </owl:Restriction>
        </rdfs:subClassOf>
        <rdfs:subClassOf>
            <owl:Restriction>
                <owl:onProperty rdf:resource="http://cybox.mitre.org/objects/NetworkConnection#layer3Protocol"/>
                <owl:maxCardinality rdf:datatype="http://www.w3.org/2001/XMLSchema#nonNegativeInteger">1</owl:maxCardinality>
            </owl:Restriction>
        </rdfs:subClassOf>
        <rdfs:subClassOf>
            <owl:Restriction>
                <owl:onProperty rdf:resource="http://cybox.mitre.org/objects/NetworkConnection#layer4Protocol"/>
                <owl:maxCardinality rdf:datatype="http://www.w3.org/2001/XMLSchema#nonNegativeInteger">1</owl:maxCardinality>
            </owl:Restriction>
        </rdfs:subClassOf>
        <rdfs:subClassOf>
            <owl:Restriction>
                <owl:onProperty rdf:resource="http://cybox.mitre.org/objects/NetworkConnection#layer7Connection.httpSession"/>
                <owl:maxCardinality rdf:datatype="http://www.w3.org/2001/XMLSchema#nonNegativeInteger">1</owl:maxCardinality>
            </owl:Restriction>
        </rdfs:subClassOf>
        <rdfs:subClassOf>
            <owl:Restriction>
                <owl:onProperty rdf:resource="http://cybox.mitre.org/objects/NetworkConnection#layer7Protocol"/>
                <owl:maxCardinality rdf:datatype="http://www.w3.org/2001/XMLSchema#nonNegativeInteger">1</owl:maxCardinality>
            </owl:Restriction>
        </rdfs:subClassOf>
        <rdfs:subClassOf>
            <owl:Restriction>
                <owl:onProperty rdf:resource="http://cybox.mitre.org/objects/NetworkConnection#sourceSocketAddress"/>
                <owl:maxCardinality rdf:datatype="http://www.w3.org/2001/XMLSchema#nonNegativeInteger">1</owl:maxCardinality>
            </owl:Restriction>
        </rdfs:subClassOf>
        <rdfs:subClassOf>
            <owl:Restriction>
                <owl:onProperty rdf:resource="http://cybox.mitre.org/objects/NetworkConnection#destinationTCPState"/>
                <owl:maxCardinality rdf:datatype="http://www.w3.org/2001/XMLSchema#nonNegativeInteger">1</owl:maxCardinality>
            </owl:Restriction>
        </rdfs:subClassOf>
        <rdfs:subClassOf>
            <owl:Restriction>
                <owl:onProperty rdf:resource="http://cybox.mitre.org/objects/NetworkConnection#sourceTCPState"/>
                <owl:maxCardinality rdf:datatype="http://www.w3.org/2001/XMLSchema#nonNegativeInteger">1</owl:maxCardinality>
            </owl:Restriction>
        </rdfs:subClassOf>
        <rdfs:subClassOf>
            <owl:Restriction>
                <owl:onProperty rdf:resource="http://cybox.mitre.org/objects/NetworkConnection#tlsUsed"/>
                <owl:maxCardinality rdf:datatype="http://www.w3.org/2001/XMLSchema#nonNegativeInteger">1</owl:maxCardinality>
            </owl:Restriction>
        </rdfs:subClassOf>
        <rdfs:comment>Characterizes local or remote (i.e. Internet) network connections.</rdfs:comment>
        <rdfs:isDefinedBy rdf:resource="http://cybox.mitre.org/objects/NetworkConnection"/>
        <rdfs:label>Network Connection</rdfs:label>
    </owl:Class>
    


    <!-- http://cybox.mitre.org/objects/NetworkProtocol#NetworkProtocol -->

    <owl:Class rdf:about="http://cybox.mitre.org/objects/NetworkProtocol#NetworkProtocol"/>
    


    <!-- http://cybox.mitre.org/objects/Socket_Address#SocketAddress -->

    <owl:Class rdf:about="http://cybox.mitre.org/objects/Socket_Address#SocketAddress"/>
</rdf:RDF>



<!-- Generated by the OWL API (version 4.2.6.20160910-2108) https://github.com/owlcs/owlapi -->

