<?xml version="1.0"?>
<rdf:RDF
    xmlns:rdf="http://www.w3.org/1999/02/22-rdf-syntax-ns#"
    xmlns:owl="http://www.w3.org/2002/07/owl#"
    xmlns:netConnectObj="http://cybox.mitre.org/objects/NetworkConnection#"
    xmlns:xsd="http://www.w3.org/2001/XMLSchema#"
    
    xmlns:rdfs="http://www.w3.org/2000/01/rdf-schema#"
  xml:base="http://cybox.mitre.org/objects/NetworkConnection">
  <owl:Ontology rdf:about="http://cybox.mitre.org/objects/NetworkConnection">
    <owl:imports rdf:resource="http://cybox.mitre.org/objects/Socket_Address"/>
    <owl:imports rdf:resource="http://cybox.mitre.org/cybox_core"/>
    <rdfs:label >Cyber Observable eXpression (CybOX) Network Connection Ontology</rdfs:label>
    
    <owl:imports rdf:resource="http://cybox.mitre.org/objects/NetworkProtocol"/>
    <owl:imports rdf:resource="http://cybox.mitre.org/objects/DNS"/>
    <owl:versionInfo rdf:datatype="http://www.w3.org/2001/XMLSchema#string"
    >2.1.0-000</owl:versionInfo>
    <owl:imports rdf:resource="http://cybox.mitre.org/objects/HTTP_Session"/>
    <rdfs:comment >This ontology provides a vocabulary and representation of a Network Connection for the  Cyber Observable eXpression (CybOX).  

CybOX  provides a common mechansim (structure and content) to convey the full range of potential cyber observable information and strives to be fully expressive, flexible, extensible, automatable, and as human-readable as possible.

The ontology is based on the Cybox Network Connection object schema maintained by The MITRE Corporation copyright 2012-2014.  The version number of the ontology is kept in sync with the schema in order to more easily relate between the ontology and the corresponding schema version.

Copyright (c) 2014, DaedaFusion, LLC.  All rights reserved.</rdfs:comment>
  </owl:Ontology>
  <owl:Class rdf:ID="NetworkConnection">
    
<!--     <rdfs:subClassOf>
      <owl:Restriction>
        <owl:onProperty rdf:resource="http://cybox.mitre.org/cybox_core#physicalLocation"/>
        <owl:maxCardinality rdf:datatype="http://www.w3.org/2001/XMLSchema#nonNegativeInteger"
        >1</owl:maxCardinality>
      </owl:Restriction>
    </rdfs:subClassOf> -->
    <rdfs:subClassOf>
      <owl:Restriction>
        <owl:onProperty>
          <owl:DatatypeProperty rdf:ID="sourceTCPState"/>
        </owl:onProperty>
        <owl:maxCardinality rdf:datatype="http://www.w3.org/2001/XMLSchema#nonNegativeInteger"
        >1</owl:maxCardinality>
      </owl:Restriction>
    </rdfs:subClassOf>
<!--     <rdfs:subClassOf>
      <owl:Restriction>
        <owl:onProperty>
          <rdf:Description rdf:about="http://cybox.mitre.org/cyboxCommon#creationDateTime">
            <rdfs:domain rdf:resource="#NetworkConnection"/>
          </rdf:Description>
        </owl:onProperty>
        <owl:cardinality rdf:datatype="http://www.w3.org/2001/XMLSchema#nonNegativeInteger"
        >1</owl:cardinality>
      </owl:Restriction>
    </rdfs:subClassOf> -->
    <rdfs:isDefinedBy rdf:resource=""/>
    <rdfs:subClassOf>
      <owl:Restriction>
        <owl:onProperty>
          <owl:ObjectProperty rdf:ID="sourceSocketAddress"/>
        </owl:onProperty>
        <owl:maxCardinality rdf:datatype="http://www.w3.org/2001/XMLSchema#nonNegativeInteger"
        >1</owl:maxCardinality>
      </owl:Restriction>
    </rdfs:subClassOf>
<!--     <rdfs:subClassOf>
      <owl:Restriction>
        <owl:onProperty rdf:resource="http://cybox.mitre.org/cybox_core#discoveryMethod"/>
        <owl:maxCardinality rdf:datatype="http://www.w3.org/2001/XMLSchema#nonNegativeInteger"
        >1</owl:maxCardinality>
      </owl:Restriction>
    </rdfs:subClassOf> -->
    <rdfs:subClassOf>
      <owl:Restriction>
        <owl:onProperty>
          <owl:DatatypeProperty rdf:ID="tlsUsed"/>
        </owl:onProperty>
        <owl:maxCardinality rdf:datatype="http://www.w3.org/2001/XMLSchema#nonNegativeInteger"
        >1</owl:maxCardinality>
      </owl:Restriction>
    </rdfs:subClassOf>
    
<!--     <rdfs:subClassOf>
      <owl:Restriction>
        <owl:onProperty rdf:resource="http://cybox.mitre.org/cybox_core#definedEffect"/>
        <owl:maxCardinality rdf:datatype="http://www.w3.org/2001/XMLSchema#nonNegativeInteger"
        >1</owl:maxCardinality>
      </owl:Restriction>
    </rdfs:subClassOf> -->
    <rdfs:subClassOf>
      <owl:Restriction>
        <owl:onProperty>
          <owl:ObjectProperty rdf:ID="layer4Protocol"/>
        </owl:onProperty>
        <owl:maxCardinality rdf:datatype="http://www.w3.org/2001/XMLSchema#nonNegativeInteger"
        >1</owl:maxCardinality>
      </owl:Restriction>
    </rdfs:subClassOf>
<!--     <rdfs:subClassOf>
      <owl:Restriction>
        <owl:onProperty rdf:resource="http://cybox.mitre.org/cybox_core#hasChanged"/>
        <owl:maxCardinality rdf:datatype="http://www.w3.org/2001/XMLSchema#nonNegativeInteger"
        >1</owl:maxCardinality>
      </owl:Restriction>
    </rdfs:subClassOf> -->
    <rdfs:subClassOf>
      <owl:Restriction>
        <owl:onProperty>
          <owl:DatatypeProperty rdf:ID="destinationTCPState"/>
        </owl:onProperty>
        <owl:maxCardinality rdf:datatype="http://www.w3.org/2001/XMLSchema#nonNegativeInteger"
        >1</owl:maxCardinality>
      </owl:Restriction>
    </rdfs:subClassOf>
    <rdfs:subClassOf>
      <owl:Restriction>
        <owl:maxCardinality rdf:datatype="http://www.w3.org/2001/XMLSchema#nonNegativeInteger"
        >1</owl:maxCardinality>
        <owl:onProperty>
          <owl:ObjectProperty rdf:ID="layer3Protocol"/>
        </owl:onProperty>
      </owl:Restriction>
    </rdfs:subClassOf>
    <rdfs:comment >Characterizes local or remote (i.e. Internet) network connections.</rdfs:comment>
    
    <rdfs:subClassOf>
      <owl:Restriction>
        <owl:onProperty>
          <owl:ObjectProperty rdf:ID="destinationSocketAddress"/>
        </owl:onProperty>
        <owl:maxCardinality rdf:datatype="http://www.w3.org/2001/XMLSchema#nonNegativeInteger"
        >1</owl:maxCardinality>
      </owl:Restriction>
    </rdfs:subClassOf>
    <rdfs:subClassOf>
      <owl:Restriction>
        <owl:onProperty>
          <owl:ObjectProperty rdf:ID="layer7Connection.httpSession"/>
        </owl:onProperty>
        <owl:maxCardinality rdf:datatype="http://www.w3.org/2001/XMLSchema#nonNegativeInteger"
        >1</owl:maxCardinality>
      </owl:Restriction>
    </rdfs:subClassOf>
    <rdfs:subClassOf rdf:resource="http://cybox.mitre.org/cybox_core#Object"/>
<!--     <rdfs:subClassOf>
      <owl:Restriction>
        <owl:onProperty rdf:resource="http://cybox.mitre.org/cybox_core#state"/>
        <owl:maxCardinality rdf:datatype="http://www.w3.org/2001/XMLSchema#nonNegativeInteger"
        >1</owl:maxCardinality>
      </owl:Restriction>
    </rdfs:subClassOf> -->
<!--     <rdfs:subClassOf>
      <owl:Restriction>
        <owl:onProperty rdf:resource="http://cybox.mitre.org/cyboxCommon#id"/>
        <owl:cardinality rdf:datatype="http://www.w3.org/2001/XMLSchema#nonNegativeInteger"
        >1</owl:cardinality>
      </owl:Restriction>
    </rdfs:subClassOf> -->
<!--     <rdfs:subClassOf>
      <owl:Restriction>
        <owl:onProperty rdf:resource="http://cybox.mitre.org/cybox_core#description"/>
        <owl:maxCardinality rdf:datatype="http://www.w3.org/2001/XMLSchema#nonNegativeInteger"
        >1</owl:maxCardinality>
      </owl:Restriction>
    </rdfs:subClassOf> -->
    <rdfs:label >Network Connection</rdfs:label>
    <rdfs:subClassOf>
      <owl:Restriction>
        <owl:onProperty>
          <owl:ObjectProperty rdf:ID="layer7Protocol"/>
        </owl:onProperty>
        <owl:maxCardinality rdf:datatype="http://www.w3.org/2001/XMLSchema#nonNegativeInteger"
        >1</owl:maxCardinality>
      </owl:Restriction>
    </rdfs:subClassOf>
  </owl:Class>
  <owl:ObjectProperty rdf:about="#destinationSocketAddress">
    <rdfs:isDefinedBy rdf:resource=""/>
    
    <rdfs:label >Destination Socket Address</rdfs:label>
    <rdfs:comment >Specifies the destination socket address, consisting of an IP Address and port number, used in the connection.</rdfs:comment>
    <!-- <rdfs:domain rdf:resource="#NetworkConnection"/> -->
    <rdfs:range rdf:resource="http://cybox.mitre.org/objects/Socket_Address#SocketAddress"/>
  </owl:ObjectProperty>
  <owl:ObjectProperty rdf:ID="layer7Connection.dnsQuery">
    <rdfs:range rdf:resource="http://cybox.mitre.org/objects/DNS#DNSQuery"/>
    <!-- <rdfs:domain rdf:resource="#NetworkConnection"/> -->
    <rdfs:comment >Specifies a single DNS query/answer pair initiated between source and destination IP addresses/ports.</rdfs:comment>
    <rdfs:label >Layer 7 Connection DNS Query</rdfs:label>
    
    <rdfs:isDefinedBy rdf:resource=""/>
  </owl:ObjectProperty>
  <owl:ObjectProperty rdf:about="#layer7Connection.httpSession">
    <rdfs:isDefinedBy rdf:resource=""/>
    
    <!-- <rdfs:domain rdf:resource="#NetworkConnection"/> -->
    <rdfs:comment >Specifies a single HTTP session initiated between source and destination IP addresses/ports, and includes 1-n HTTP Request/Response pairs.</rdfs:comment>
    <rdfs:label >Layer 7 Connection HTTP Session</rdfs:label>
    <rdfs:range rdf:resource="http://cybox.mitre.org/objects/HTTP_Session#HTTPSession"/>
  </owl:ObjectProperty>
  <owl:ObjectProperty rdf:about="#sourceSocketAddress">
    <rdfs:isDefinedBy rdf:resource=""/>
    
    <rdfs:label >Source Socket Address</rdfs:label>
    <!-- <rdfs:domain rdf:resource="#NetworkConnection"/> -->
    <rdfs:comment >Specifies the source socket address, consisting of an IP Address and port number, used in the connection.</rdfs:comment>
    <rdfs:range rdf:resource="http://cybox.mitre.org/objects/Socket_Address#SocketAddress"/>
  </owl:ObjectProperty>
  <owl:ObjectProperty rdf:about="#layer7Protocol">
    <rdfs:isDefinedBy rdf:resource=""/>
    
    <rdfs:label >Layer7 Protocol</rdfs:label>
    <rdfs:comment >Specifies the particular application (layer 7 in the OSI model) layer protocol used in the connection.</rdfs:comment>
    <!-- <rdfs:domain rdf:resource="#NetworkConnection"/> -->
    <rdfs:range rdf:resource="http://cybox.mitre.org/objects/NetworkProtocol#NetworkProtocol"/>
  </owl:ObjectProperty>
  <owl:ObjectProperty rdf:about="#layer4Protocol">
    <rdfs:isDefinedBy rdf:resource=""/>
    
    <rdfs:label >Layer 4 Protocol</rdfs:label>
    <rdfs:comment >Specifies the particular transport (layer 4 in the OSI model) layer protocol used in the connection.</rdfs:comment>
    <!-- <rdfs:domain rdf:resource="#NetworkConnection"/> -->
    <rdfs:range rdf:resource="http://cybox.mitre.org/objects/NetworkProtocol#NetworkProtocol"/>
  </owl:ObjectProperty>
  <owl:ObjectProperty rdf:about="#layer3Protocol">
    <rdfs:isDefinedBy rdf:resource=""/>
    <rdfs:comment >Specifies the particular network (layer 3 in the OSI model) layer protocol used in the connection.</rdfs:comment>
    <rdfs:label >Layer 3 Protocols</rdfs:label>
    <!-- <rdfs:domain rdf:resource="#NetworkConnection"/> -->
    
    <rdfs:range rdf:resource="http://cybox.mitre.org/objects/NetworkProtocol#NetworkProtocol"/>
  </owl:ObjectProperty>
  <owl:DatatypeProperty rdf:about="#tlsUsed">
    <!-- <rdfs:domain rdf:resource="#NetworkConnection"/> -->
    
    <rdfs:label >TLS Used</rdfs:label>
    <rdfs:isDefinedBy rdf:resource=""/>
    <rdfs:range rdf:resource="http://www.w3.org/2001/XMLSchema#boolean"/>
    <rdfs:comment >Specifies whether or not Transport Layer Security (TLS) is used in the network connection.</rdfs:comment>
  </owl:DatatypeProperty>
  <owl:DatatypeProperty rdf:about="#sourceTCPState">
    
    <rdfs:isDefinedBy rdf:resource=""/>
    
    <!-- <rdfs:domain rdf:resource="#NetworkConnection"/> -->
    <rdfs:comment >Specifies the current state of the TCP network connection at the source, if applicable.</rdfs:comment>
    <rdfs:label >Source TCP State</rdfs:label>
    <rdfs:range rdf:resource="http://www.w3.org/2001/XMLSchema#string"/>
    
  </owl:DatatypeProperty>
  <owl:DatatypeProperty rdf:about="#destinationTCPState">
    
    <rdfs:isDefinedBy rdf:resource=""/>
    
    <rdfs:label >Destination TCP State</rdfs:label>
    
    <!-- <rdfs:domain rdf:resource="#NetworkConnection"/> -->
    <rdfs:range rdf:resource="http://www.w3.org/2001/XMLSchema#string"/>
    <rdfs:comment >Specifies the current state of the TCP network connection at the destination, if applicable.</rdfs:comment>
  </owl:DatatypeProperty>
</rdf:RDF>

<!-- Created with TopBraid -->
