<?xml version="1.0"?>
<rdf:RDF xmlns="http://cybox.mitre.org/objects/System#"
     xml:base="http://cybox.mitre.org/objects/System"
     xmlns:systemObj="http://cybox.mitre.org/objects/System#"
     xmlns:rdf="http://www.w3.org/1999/02/22-rdf-syntax-ns#"
     xmlns:owl="http://www.w3.org/2002/07/owl#"
     xmlns:xml="http://www.w3.org/XML/1998/namespace"
     xmlns:xsd="http://www.w3.org/2001/XMLSchema#"
     xmlns:rdfs="http://www.w3.org/2000/01/rdf-schema#">
    <owl:Ontology rdf:about="http://cybox.mitre.org/objects/System">
        <owl:imports rdf:resource="http://cybox.mitre.org/objects/Hostname"/>
        <owl:imports rdf:resource="http://cybox.mitre.org/cyboxCommon"/>
        <owl:imports rdf:resource="http://cybox.mitre.org/objects/Account"/>
        <owl:imports rdf:resource="http://cybox.mitre.org/cybox_core"/>
        <owl:imports rdf:resource="http://cybox.mitre.org/objects/WindowsHandle"/>
        <owl:imports rdf:resource="http://cybox.mitre.org/objects/Address"/>
        <rdfs:label>Cyber Observable eXpression (CybOX) System Ontology</rdfs:label>
        <rdfs:comment>This ontology provides a vocabulary and representation of a System for the  Cyber Observable eXpression (CybOX).  

CybOX  provides a common mechansim (structure and content) to convey the full range of potential cyber observable information and strives to be fully expressive, flexible, extensible, automatable, and as human-readable as possible.

Copyright (c) 2014, DaedaFusion, LLC.  All rights reserved.</rdfs:comment>
        <owl:versionInfo rdf:datatype="http://www.w3.org/2001/XMLSchema#string">1.0.0-000</owl:versionInfo>
    </owl:Ontology>
    


    <!-- 
    ///////////////////////////////////////////////////////////////////////////////////////
    //
    // Datatypes
    //
    ///////////////////////////////////////////////////////////////////////////////////////
     -->

    


    <!-- http://www.w3.org/2001/XMLSchema#date -->

    <rdfs:Datatype rdf:about="http://www.w3.org/2001/XMLSchema#date"/>
    


    <!-- http://www.w3.org/2001/XMLSchema#duration -->

    <rdfs:Datatype rdf:about="http://www.w3.org/2001/XMLSchema#duration"/>
    


    <!-- http://www.w3.org/2001/XMLSchema#time -->

    <rdfs:Datatype rdf:about="http://www.w3.org/2001/XMLSchema#time"/>
    


    <!-- 
    ///////////////////////////////////////////////////////////////////////////////////////
    //
    // Object Properties
    //
    ///////////////////////////////////////////////////////////////////////////////////////
     -->

    


    <!-- http://cybox.mitre.org/objects/System#BIOS.manufacturerDetails -->

    <owl:ObjectProperty rdf:about="http://cybox.mitre.org/objects/System#BIOS.manufacturerDetails">
        <rdfs:range rdf:resource="http://www.oasis-open.org/ciq_xpil#Organization"/>
        <rdfs:comment>Specifies the manufacturer of the BIOS.</rdfs:comment>
        <rdfs:isDefinedBy rdf:resource="http://cybox.mitre.org/objects/System"/>
        <rdfs:label>BIOS Manufacturer</rdfs:label>
    </owl:ObjectProperty>
    


    <!-- http://cybox.mitre.org/objects/System#dhcpServers -->

    <owl:ObjectProperty rdf:about="http://cybox.mitre.org/objects/System#dhcpServers">
        <rdfs:range>
            <owl:Class>
                <owl:unionOf rdf:parseType="Collection">
                    <rdf:Description rdf:about="http://cybox.mitre.org/objects/Address#IPv4Address"/>
                    <rdf:Description rdf:about="http://cybox.mitre.org/objects/Address#IPv6Address"/>
                </owl:unionOf>
            </owl:Class>
        </rdfs:range>
        <rdfs:comment>Specifies the list of DHCP servers used by the network interface.</rdfs:comment>
        <rdfs:isDefinedBy rdf:resource="http://cybox.mitre.org/objects/System"/>
        <rdfs:label>DHCP Servers</rdfs:label>
    </owl:ObjectProperty>
    


    <!-- http://cybox.mitre.org/objects/System#environmentVariableList -->

    <owl:ObjectProperty rdf:about="http://cybox.mitre.org/objects/System#environmentVariableList">
        <rdfs:range rdf:resource="http://cybox.mitre.org/cyboxCommon#EnvironmentVariable"/>
        <rdfs:comment>Specifies a list of environment variables present on the operating system.</rdfs:comment>
        <rdfs:isDefinedBy rdf:resource="http://cybox.mitre.org/objects/System"/>
        <rdfs:label>Environment Variable list</rdfs:label>
    </owl:ObjectProperty>
    


    <!-- http://cybox.mitre.org/objects/System#globalFlags -->

    <owl:ObjectProperty rdf:about="http://cybox.mitre.org/objects/System#globalFlags">
        <rdfs:range rdf:resource="http://cybox.mitre.org/objects/System#GlobalFlag"/>
        <rdfs:comment>Specifies a list of global flags. 

See also: http://msdn.microsoft.com/en-us/library/windows/hardware/ff549557(v=vs.85).aspx.</rdfs:comment>
        <rdfs:isDefinedBy rdf:resource="http://cybox.mitre.org/objects/System"/>
        <rdfs:label>Global Flags</rdfs:label>
    </owl:ObjectProperty>
    


    <!-- http://cybox.mitre.org/objects/System#handles -->

    <owl:ObjectProperty rdf:about="http://cybox.mitre.org/objects/System#handles">
        <rdfs:range rdf:resource="http://cybox.mitre.org/objects/WindowsHandle#WindowsHandle"/>
        <rdfs:comment>Specifies the list of open handles for the Windows system.</rdfs:comment>
        <rdfs:isDefinedBy rdf:resource="http://cybox.mitre.org/objects/System"/>
        <rdfs:label>Handles</rdfs:label>
    </owl:ObjectProperty>
    


    <!-- http://cybox.mitre.org/objects/System#hostname.details -->

    <owl:ObjectProperty rdf:about="http://cybox.mitre.org/objects/System#hostname.details">
        <rdfs:range rdf:resource="http://cybox.mitre.org/objects/Hostname#Hostname"/>
        <rdfs:comment>Specifies detailed information about  the hostname of the system.</rdfs:comment>
        <rdfs:isDefinedBy rdf:resource="http://cybox.mitre.org/objects/System"/>
        <rdfs:label>Hostname Details</rdfs:label>
    </owl:ObjectProperty>
    


    <!-- http://cybox.mitre.org/objects/System#ipAddress -->

    <owl:ObjectProperty rdf:about="http://cybox.mitre.org/objects/System#ipAddress">
        <rdfs:range>
            <owl:Class>
                <owl:unionOf rdf:parseType="Collection">
                    <rdf:Description rdf:about="http://cybox.mitre.org/objects/Address#IPv4Address"/>
                    <rdf:Description rdf:about="http://cybox.mitre.org/objects/Address#IPv6Address"/>
                </owl:unionOf>
            </owl:Class>
        </rdfs:range>
        <rdfs:comment>Specifies an IP address.</rdfs:comment>
        <rdfs:isDefinedBy rdf:resource="http://cybox.mitre.org/objects/System"/>
        <rdfs:label>IP Address</rdfs:label>
    </owl:ObjectProperty>
    


    <!-- http://cybox.mitre.org/objects/System#ipAddresses -->

    <owl:ObjectProperty rdf:about="http://cybox.mitre.org/objects/System#ipAddresses">
        <rdfs:range rdf:resource="http://cybox.mitre.org/objects/System#IPInfo"/>
        <rdfs:comment>Specifies the list of IP addresses used by the network interface.</rdfs:comment>
        <rdfs:isDefinedBy rdf:resource="http://cybox.mitre.org/objects/System"/>
        <rdfs:label>IP Addresses</rdfs:label>
    </owl:ObjectProperty>
    


    <!-- http://cybox.mitre.org/objects/System#ipGateways -->

    <owl:ObjectProperty rdf:about="http://cybox.mitre.org/objects/System#ipGateways">
        <rdfs:range>
            <owl:Class>
                <owl:unionOf rdf:parseType="Collection">
                    <rdf:Description rdf:about="http://cybox.mitre.org/objects/Address#IPv4Address"/>
                    <rdf:Description rdf:about="http://cybox.mitre.org/objects/Address#IPv6Address"/>
                </owl:unionOf>
            </owl:Class>
        </rdfs:range>
        <rdfs:comment>Specifies the list of IP Gateways used by the network interface.</rdfs:comment>
        <rdfs:isDefinedBy rdf:resource="http://cybox.mitre.org/objects/System"/>
        <rdfs:label>IP Gateways</rdfs:label>
    </owl:ObjectProperty>
    


    <!-- http://cybox.mitre.org/objects/System#macAddress -->

    <owl:ObjectProperty rdf:about="http://cybox.mitre.org/objects/System#macAddress">
        <rdfs:range rdf:resource="http://cybox.mitre.org/objects/Address#MACAddress"/>
        <rdfs:comment>Specifies the MAC or hardware address of the physical network card.</rdfs:comment>
        <rdfs:isDefinedBy rdf:resource="http://cybox.mitre.org/objects/System"/>
        <rdfs:label>MAC Address</rdfs:label>
    </owl:ObjectProperty>
    


    <!-- http://cybox.mitre.org/objects/System#networkInterfaces -->

    <owl:ObjectProperty rdf:about="http://cybox.mitre.org/objects/System#networkInterfaces">
        <rdfs:range rdf:resource="http://cybox.mitre.org/objects/System#NetworkInterface"/>
        <rdfs:comment>Specifies the list of network interfaces present on the system.</rdfs:comment>
        <rdfs:isDefinedBy rdf:resource="http://cybox.mitre.org/objects/System"/>
        <rdfs:label>Network Interfaces</rdfs:label>
    </owl:ObjectProperty>
    


    <!-- http://cybox.mitre.org/objects/System#operatingSystem -->

    <owl:ObjectProperty rdf:about="http://cybox.mitre.org/objects/System#operatingSystem">
        <rdfs:range rdf:resource="http://cybox.mitre.org/objects/System#OperatingSystemInfo"/>
        <rdfs:comment>Specifies information about the operating system installed on the system.</rdfs:comment>
        <rdfs:isDefinedBy rdf:resource="http://cybox.mitre.org/objects/System"/>
        <rdfs:label>Operating System</rdfs:label>
    </owl:ObjectProperty>
    


    <!-- http://cybox.mitre.org/objects/System#platform -->

    <owl:ObjectProperty rdf:about="http://cybox.mitre.org/objects/System#platform">
        <rdfs:range rdf:resource="http://cybox.mitre.org/cyboxCommon#PlatformSpecification"/>
        <rdfs:comment>Specifies a general identifier for the Operation System</rdfs:comment>
        <rdfs:isDefinedBy rdf:resource="http://cybox.mitre.org/objects/System"/>
        <rdfs:label>Platform</rdfs:label>
    </owl:ObjectProperty>
    


    <!-- http://cybox.mitre.org/objects/System#subnetMask -->

    <owl:ObjectProperty rdf:about="http://cybox.mitre.org/objects/System#subnetMask">
        <rdfs:range>
            <owl:Class>
                <owl:unionOf rdf:parseType="Collection">
                    <rdf:Description rdf:about="http://cybox.mitre.org/objects/Address#IPv4Netmask"/>
                    <rdf:Description rdf:about="http://cybox.mitre.org/objects/Address#IPv6Netmask"/>
                </owl:unionOf>
            </owl:Class>
        </rdfs:range>
        <rdfs:comment>Specifies a subnet mask.</rdfs:comment>
        <rdfs:isDefinedBy rdf:resource="http://cybox.mitre.org/objects/System"/>
        <rdfs:label>Subnet Mask</rdfs:label>
    </owl:ObjectProperty>
    


    <!-- http://cybox.mitre.org/objects/System#username.details -->

    <owl:ObjectProperty rdf:about="http://cybox.mitre.org/objects/System#username.details">
        <rdfs:range rdf:resource="http://cybox.mitre.org/objects/Account#UserAccount"/>
        <rdfs:comment>Specifies detailed information about  the username.</rdfs:comment>
        <rdfs:isDefinedBy rdf:resource="http://cybox.mitre.org/cyboxCommon"/>
        <rdfs:label>Username Details</rdfs:label>
    </owl:ObjectProperty>
    


    <!-- 
    ///////////////////////////////////////////////////////////////////////////////////////
    //
    // Data properties
    //
    ///////////////////////////////////////////////////////////////////////////////////////
     -->

    


    <!-- http://cybox.mitre.org/objects/System#BIOS.date -->

    <owl:DatatypeProperty rdf:about="http://cybox.mitre.org/objects/System#BIOS.date">
        <rdfs:range rdf:resource="http://www.w3.org/2001/XMLSchema#date"/>
        <rdfs:comment>Specifies the date of the bios (e.g. the datestamp of the BIOS revision).</rdfs:comment>
        <rdfs:isDefinedBy rdf:resource="http://cybox.mitre.org/objects/System"/>
        <rdfs:label>BIOS Date</rdfs:label>
    </owl:DatatypeProperty>
    


    <!-- http://cybox.mitre.org/objects/System#BIOS.manufactureName -->

    <owl:DatatypeProperty rdf:about="http://cybox.mitre.org/objects/System#BIOS.manufactureName">
        <rdfs:range rdf:resource="http://www.w3.org/2001/XMLSchema#string"/>
        <rdfs:comment>Specifies the name of the manufacturer of the BIOS.</rdfs:comment>
        <rdfs:isDefinedBy rdf:resource="http://cybox.mitre.org/objects/System"/>
        <rdfs:label>BIOS Manufacture Name</rdfs:label>
    </owl:DatatypeProperty>
    


    <!-- http://cybox.mitre.org/objects/System#BIOS.releaseDate -->

    <owl:DatatypeProperty rdf:about="http://cybox.mitre.org/objects/System#BIOS.releaseDate">
        <rdfs:range rdf:resource="http://www.w3.org/2001/XMLSchema#date"/>
        <rdfs:comment>Specifies the date the BIOS was released.</rdfs:comment>
        <rdfs:isDefinedBy rdf:resource="http://cybox.mitre.org/objects/System"/>
        <rdfs:label>BIOS Release Date</rdfs:label>
    </owl:DatatypeProperty>
    


    <!-- http://cybox.mitre.org/objects/System#BIOS.serialNumber -->

    <owl:DatatypeProperty rdf:about="http://cybox.mitre.org/objects/System#BIOS.serialNumber">
        <rdfs:range rdf:resource="http://www.w3.org/2001/XMLSchema#string"/>
        <rdfs:comment>Specifies the serial number of the BIOS.</rdfs:comment>
        <rdfs:isDefinedBy rdf:resource="http://cybox.mitre.org/objects/System"/>
        <rdfs:label>BIOS Serial Number</rdfs:label>
    </owl:DatatypeProperty>
    


    <!-- http://cybox.mitre.org/objects/System#BIOS.version -->

    <owl:DatatypeProperty rdf:about="http://cybox.mitre.org/objects/System#BIOS.version">
        <rdfs:range rdf:resource="http://www.w3.org/2001/XMLSchema#string"/>
        <rdfs:comment>Specifies the version of the BIOS.</rdfs:comment>
        <rdfs:isDefinedBy rdf:resource="http://cybox.mitre.org/objects/System"/>
        <rdfs:label>BIOS Version</rdfs:label>
    </owl:DatatypeProperty>
    


    <!-- http://cybox.mitre.org/objects/System#abbreviation -->

    <owl:DatatypeProperty rdf:about="http://cybox.mitre.org/objects/System#abbreviation">
        <rdfs:range rdf:resource="http://www.w3.org/2001/XMLSchema#string"/>
        <rdfs:comment>Specifies the abbreviation of a global flag. 

See also: http://msdn.microsoft.com/en-us/library/windows/hardware/ff549646(v=vs.85).aspx.</rdfs:comment>
        <rdfs:isDefinedBy rdf:resource="http://cybox.mitre.org/objects/System"/>
        <rdfs:label>Abbreviation</rdfs:label>
    </owl:DatatypeProperty>
    


    <!-- http://cybox.mitre.org/objects/System#adapter -->

    <owl:DatatypeProperty rdf:about="http://cybox.mitre.org/objects/System#adapter">
        <rdfs:range rdf:resource="http://www.w3.org/2001/XMLSchema#string"/>
        <rdfs:comment>Specifies the name of the network adapter used by the network interface.</rdfs:comment>
        <rdfs:isDefinedBy rdf:resource="http://cybox.mitre.org/objects/System"/>
        <rdfs:label>Adapter</rdfs:label>
    </owl:DatatypeProperty>
    


    <!-- http://cybox.mitre.org/objects/System#availPhysicalMemory -->

    <owl:DatatypeProperty rdf:about="http://cybox.mitre.org/objects/System#availPhysicalMemory">
        <rdfs:range rdf:resource="http://www.w3.org/2001/XMLSchema#unsignedLong"/>
        <rdfs:comment>Specifies the amount of physical memory available on the system, in bytes.</rdfs:comment>
        <rdfs:isDefinedBy rdf:resource="http://cybox.mitre.org/objects/System"/>
        <rdfs:label>Available Physical Memory</rdfs:label>
    </owl:DatatypeProperty>
    


    <!-- http://cybox.mitre.org/objects/System#bitness -->

    <owl:DatatypeProperty rdf:about="http://cybox.mitre.org/objects/System#bitness">
        <rdfs:range>
            <rdfs:Datatype>
                <owl:oneOf>
                    <rdf:Description>
                        <rdf:type rdf:resource="http://www.w3.org/1999/02/22-rdf-syntax-ns#List"/>
                        <rdf:first rdf:datatype="http://www.w3.org/2001/XMLSchema#string">32</rdf:first>
                        <rdf:rest>
                            <rdf:Description>
                                <rdf:type rdf:resource="http://www.w3.org/1999/02/22-rdf-syntax-ns#List"/>
                                <rdf:first rdf:datatype="http://www.w3.org/2001/XMLSchema#string">64</rdf:first>
                                <rdf:rest rdf:resource="http://www.w3.org/1999/02/22-rdf-syntax-ns#nil"/>
                            </rdf:Description>
                        </rdf:rest>
                    </rdf:Description>
                </owl:oneOf>
            </rdfs:Datatype>
        </rdfs:range>
        <rdfs:comment>Specifies the bitness of the operating system (i.e. 32 or 64). 

Note that this is potentially different from the word size of the underlying hardware or CPU. A 32-bit operating system can be installed on a machine running a 64-bit processor.</rdfs:comment>
        <rdfs:isDefinedBy rdf:resource="http://cybox.mitre.org/objects/System"/>
        <rdfs:label>Bitness</rdfs:label>
    </owl:DatatypeProperty>
    


    <!-- http://cybox.mitre.org/objects/System#buildNumber -->

    <owl:DatatypeProperty rdf:about="http://cybox.mitre.org/objects/System#buildNumber">
        <rdfs:range rdf:resource="http://www.w3.org/2001/XMLSchema#string"/>
        <rdfs:comment>Specifies the build number of the operating system.</rdfs:comment>
        <rdfs:isDefinedBy rdf:resource="http://cybox.mitre.org/objects/System"/>
        <rdfs:label>Build Number</rdfs:label>
    </owl:DatatypeProperty>
    


    <!-- http://cybox.mitre.org/objects/System#currentDate -->

    <owl:DatatypeProperty rdf:about="http://cybox.mitre.org/objects/System#currentDate">
        <rdfs:range rdf:resource="http://www.w3.org/2001/XMLSchema#date"/>
        <rdfs:comment>Specifies the current date on the system.</rdfs:comment>
        <rdfs:isDefinedBy rdf:resource="http://cybox.mitre.org/objects/System"/>
        <rdfs:label>Current Date</rdfs:label>
    </owl:DatatypeProperty>
    


    <!-- http://cybox.mitre.org/objects/System#description -->

    <owl:DatatypeProperty rdf:about="http://cybox.mitre.org/objects/System#description">
        <rdfs:range rdf:resource="http://www.w3.org/2001/XMLSchema#string"/>
        <rdfs:comment>Specifies the description of the network interface.</rdfs:comment>
        <rdfs:isDefinedBy rdf:resource="http://cybox.mitre.org/objects/System"/>
        <rdfs:label>Description</rdfs:label>
    </owl:DatatypeProperty>
    


    <!-- http://cybox.mitre.org/objects/System#destination -->

    <owl:DatatypeProperty rdf:about="http://cybox.mitre.org/objects/System#destination">
        <rdfs:range rdf:resource="http://www.w3.org/2001/XMLSchema#string"/>
        <rdfs:comment>Specifies the destination of a global flag. See also: http://msdn.microsoft.com/en-us/library/windows/hardware/ff549646(v=vs.85).aspx.</rdfs:comment>
        <rdfs:isDefinedBy rdf:resource="http://cybox.mitre.org/objects/System"/>
        <rdfs:label>Destination</rdfs:label>
    </owl:DatatypeProperty>
    


    <!-- http://cybox.mitre.org/objects/System#dhcpLeaseExpiresDateTime -->

    <owl:DatatypeProperty rdf:about="http://cybox.mitre.org/objects/System#dhcpLeaseExpiresDateTime">
        <rdfs:range rdf:resource="http://www.w3.org/2001/XMLSchema#dateTime"/>
        <rdfs:comment>Specifies the date/time that the DHCP lease obtained on the network interface expires.</rdfs:comment>
        <rdfs:isDefinedBy rdf:resource="http://cybox.mitre.org/objects/System"/>
        <rdfs:label>DHCP Lease Expires</rdfs:label>
    </owl:DatatypeProperty>
    


    <!-- http://cybox.mitre.org/objects/System#dhcpLeaseObtainedDateTime -->

    <owl:DatatypeProperty rdf:about="http://cybox.mitre.org/objects/System#dhcpLeaseObtainedDateTime">
        <rdfs:range rdf:resource="http://www.w3.org/2001/XMLSchema#dateTime"/>
        <rdfs:comment>Specifies the date/time that the DHCP lease was obtained on the network interface.</rdfs:comment>
        <rdfs:isDefinedBy rdf:resource="http://cybox.mitre.org/objects/System"/>
        <rdfs:label>DHCP Lease Obtained</rdfs:label>
    </owl:DatatypeProperty>
    


    <!-- http://cybox.mitre.org/objects/System#domain -->

    <owl:DatatypeProperty rdf:about="http://cybox.mitre.org/objects/System#domain">
        <rdfs:range rdf:resource="http://www.w3.org/2001/XMLSchema#string"/>
        <rdfs:comment>Specifies the domain that the system belongs to.</rdfs:comment>
        <rdfs:isDefinedBy rdf:resource="http://cybox.mitre.org/objects/System"/>
        <rdfs:label>Domain</rdfs:label>
    </owl:DatatypeProperty>
    


    <!-- http://cybox.mitre.org/objects/System#hexadecimalValue -->

    <owl:DatatypeProperty rdf:about="http://cybox.mitre.org/objects/System#hexadecimalValue">
        <rdfs:range rdf:resource="http://www.w3.org/2001/XMLSchema#hexBinary"/>
        <rdfs:comment>Specifies the hexadecimal value of a global flag. See also: http://msdn.microsoft.com/en-us/library/windows/hardware/ff549646(v=vs.85).aspx.</rdfs:comment>
        <rdfs:isDefinedBy rdf:resource="http://cybox.mitre.org/objects/System"/>
        <rdfs:label>Hexadecimal Value</rdfs:label>
    </owl:DatatypeProperty>
    


    <!-- http://cybox.mitre.org/objects/System#hostname -->

    <owl:DatatypeProperty rdf:about="http://cybox.mitre.org/objects/System#hostname">
        <rdfs:range rdf:resource="http://www.w3.org/2001/XMLSchema#string"/>
        <rdfs:comment>Specifies the hostname of the system.</rdfs:comment>
        <rdfs:isDefinedBy rdf:resource="http://cybox.mitre.org/objects/System"/>
        <rdfs:label>Hostname</rdfs:label>
    </owl:DatatypeProperty>
    


    <!-- http://cybox.mitre.org/objects/System#installDate -->

    <owl:DatatypeProperty rdf:about="http://cybox.mitre.org/objects/System#installDate">
        <rdfs:range rdf:resource="http://www.w3.org/2001/XMLSchema#date"/>
        <rdfs:comment>Specifies the date the operating system was installed.</rdfs:comment>
        <rdfs:isDefinedBy rdf:resource="http://cybox.mitre.org/objects/System"/>
        <rdfs:label>Install Date</rdfs:label>
    </owl:DatatypeProperty>
    


    <!-- http://cybox.mitre.org/objects/System#localTime -->

    <owl:DatatypeProperty rdf:about="http://cybox.mitre.org/objects/System#localTime">
        <rdfs:range rdf:resource="http://www.w3.org/2001/XMLSchema#time"/>
        <rdfs:comment>Specifies the local time on the system.</rdfs:comment>
        <rdfs:isDefinedBy rdf:resource="http://cybox.mitre.org/objects/System"/>
        <rdfs:label>System Local Time</rdfs:label>
    </owl:DatatypeProperty>
    


    <!-- http://cybox.mitre.org/objects/System#microsoftProductID -->

    <owl:DatatypeProperty rdf:about="http://cybox.mitre.org/objects/System#microsoftProductID">
        <rdfs:range rdf:resource="http://www.w3.org/2001/XMLSchema#string"/>
        <rdfs:comment>Specifies the Product ID. 

See also: http://support.microsoft.com/gp/pidwin.</rdfs:comment>
        <rdfs:isDefinedBy rdf:resource="http://cybox.mitre.org/objects/System"/>
        <rdfs:label>Microsoft Product ID</rdfs:label>
    </owl:DatatypeProperty>
    


    <!-- http://cybox.mitre.org/objects/System#netBIOSName -->

    <owl:DatatypeProperty rdf:about="http://cybox.mitre.org/objects/System#netBIOSName">
        <rdfs:range rdf:resource="http://www.w3.org/2001/XMLSchema#string"/>
        <rdfs:comment>Specifies the NetBIOS (Network Basic Input/Output System) name of the Windows system. This is not the same as the host name.</rdfs:comment>
        <rdfs:isDefinedBy rdf:resource="http://cybox.mitre.org/objects/System"/>
        <rdfs:label>NetBIOS Name</rdfs:label>
    </owl:DatatypeProperty>
    


    <!-- http://cybox.mitre.org/objects/System#patchLevel -->

    <owl:DatatypeProperty rdf:about="http://cybox.mitre.org/objects/System#patchLevel">
        <rdfs:range rdf:resource="http://www.w3.org/2001/XMLSchema#string"/>
        <rdfs:comment>Specifies the patch level of the operating system.</rdfs:comment>
        <rdfs:isDefinedBy rdf:resource="http://cybox.mitre.org/objects/System"/>
        <rdfs:label>Patch Level</rdfs:label>
    </owl:DatatypeProperty>
    


    <!-- http://cybox.mitre.org/objects/System#processor -->

    <owl:DatatypeProperty rdf:about="http://cybox.mitre.org/objects/System#processor">
        <rdfs:range rdf:resource="http://www.w3.org/2001/XMLSchema#string"/>
        <rdfs:comment>Specifies the name of the CPU used by the system.</rdfs:comment>
        <rdfs:isDefinedBy rdf:resource="http://cybox.mitre.org/objects/System"/>
        <rdfs:label>Processor</rdfs:label>
    </owl:DatatypeProperty>
    


    <!-- http://cybox.mitre.org/objects/System#processorArchitecture -->

    <owl:DatatypeProperty rdf:about="http://cybox.mitre.org/objects/System#processorArchitecture">
        <rdfs:range rdf:resource="http://www.w3.org/2001/XMLSchema#string"/>
        <rdfs:comment>Specifies the specific architecture (e.g. x86) used by the CPU of the system.</rdfs:comment>
        <rdfs:isDefinedBy rdf:resource="http://cybox.mitre.org/objects/System"/>
        <rdfs:label>Processor Architecture</rdfs:label>
    </owl:DatatypeProperty>
    


    <!-- http://cybox.mitre.org/objects/System#productName -->

    <owl:DatatypeProperty rdf:about="http://cybox.mitre.org/objects/System#productName">
        <rdfs:range rdf:resource="http://www.w3.org/2001/XMLSchema#string"/>
        <rdfs:comment>Specifies the ProductName of the current installation of Windows. 

This is typically found in HKEY_LOCAL_MACHINE\Software\Microsoft\Windows\CurrentVersion!ProductName.</rdfs:comment>
        <rdfs:isDefinedBy rdf:resource="http://cybox.mitre.org/objects/System"/>
        <rdfs:label>Product Name</rdfs:label>
    </owl:DatatypeProperty>
    


    <!-- http://cybox.mitre.org/objects/System#registerdOwner -->

    <owl:DatatypeProperty rdf:about="http://cybox.mitre.org/objects/System#registerdOwner">
        <rdfs:range rdf:resource="http://www.w3.org/2001/XMLSchema#string"/>
        <rdfs:comment>Specifies the person or organization that is the registered owner of this copy of Windows.</rdfs:comment>
        <rdfs:isDefinedBy rdf:resource="http://cybox.mitre.org/objects/System"/>
        <rdfs:label>Registerd Owner</rdfs:label>
    </owl:DatatypeProperty>
    


    <!-- http://cybox.mitre.org/objects/System#registeredOrganization -->

    <owl:DatatypeProperty rdf:about="http://cybox.mitre.org/objects/System#registeredOrganization">
        <rdfs:range rdf:resource="http://www.w3.org/2001/XMLSchema#string"/>
        <rdfs:comment>Specifies the organization that this copy of Windows is registered to.</rdfs:comment>
        <rdfs:isDefinedBy rdf:resource="http://cybox.mitre.org/objects/System"/>
        <rdfs:label>Registered Organization</rdfs:label>
    </owl:DatatypeProperty>
    


    <!-- http://cybox.mitre.org/objects/System#symbolicName -->

    <owl:DatatypeProperty rdf:about="http://cybox.mitre.org/objects/System#symbolicName">
        <rdfs:range rdf:resource="http://www.w3.org/2001/XMLSchema#string"/>
        <rdfs:comment>Specifies the symbolic name of a global flag. 

See also: http://msdn.microsoft.com/en-us/library/windows/hardware/ff549646(v=vs.85).aspx.</rdfs:comment>
        <rdfs:isDefinedBy rdf:resource="http://cybox.mitre.org/objects/System"/>
        <rdfs:label>Symbolic Name</rdfs:label>
    </owl:DatatypeProperty>
    


    <!-- http://cybox.mitre.org/objects/System#systemTime -->

    <owl:DatatypeProperty rdf:about="http://cybox.mitre.org/objects/System#systemTime">
        <rdfs:range rdf:resource="http://www.w3.org/2001/XMLSchema#time"/>
        <rdfs:comment>Specifies the system or hardware, time on the system.</rdfs:comment>
        <rdfs:isDefinedBy rdf:resource="http://cybox.mitre.org/objects/System"/>
        <rdfs:label>System Time</rdfs:label>
    </owl:DatatypeProperty>
    


    <!-- http://cybox.mitre.org/objects/System#timezoneDST -->

    <owl:DatatypeProperty rdf:about="http://cybox.mitre.org/objects/System#timezoneDST">
        <rdfs:range rdf:resource="http://www.w3.org/2001/XMLSchema#string"/>
        <rdfs:comment>Specifies the time zone used by the system, taking daylight savings time (DST) into account.</rdfs:comment>
        <rdfs:isDefinedBy rdf:resource="http://cybox.mitre.org/objects/System"/>
        <rdfs:label>Timezone (with DST)</rdfs:label>
    </owl:DatatypeProperty>
    


    <!-- http://cybox.mitre.org/objects/System#timezoneStandard -->

    <owl:DatatypeProperty rdf:about="http://cybox.mitre.org/objects/System#timezoneStandard">
        <rdfs:range rdf:resource="http://www.w3.org/2001/XMLSchema#string"/>
        <rdfs:comment>Specifies the time zone used by the system, without taking daylight savings time (DST) into account.</rdfs:comment>
        <rdfs:isDefinedBy rdf:resource="http://cybox.mitre.org/objects/System"/>
        <rdfs:label>Timezone (No DST)</rdfs:label>
    </owl:DatatypeProperty>
    


    <!-- http://cybox.mitre.org/objects/System#totalPhysicalMemory -->

    <owl:DatatypeProperty rdf:about="http://cybox.mitre.org/objects/System#totalPhysicalMemory">
        <rdfs:range rdf:resource="http://www.w3.org/2001/XMLSchema#unsignedLong"/>
        <rdfs:comment>Specifies the total amount of physical memory present on the system, in bytes.</rdfs:comment>
        <rdfs:isDefinedBy rdf:resource="http://cybox.mitre.org/objects/System"/>
        <rdfs:label>Total Physical Memory</rdfs:label>
    </owl:DatatypeProperty>
    


    <!-- http://cybox.mitre.org/objects/System#uptime -->

    <owl:DatatypeProperty rdf:about="http://cybox.mitre.org/objects/System#uptime">
        <rdfs:range rdf:resource="http://www.w3.org/2001/XMLSchema#duration"/>
        <rdfs:comment>Specifies the duration that represents the current amount of time that the system has been up. 

The format for specifying Uptime is &apos;P&apos; + &lt;# of years&gt; + &apos;Y&apos; + &lt;# of months&gt; + &apos;M&apos; + &lt;# of days&gt; + &apos;DT&apos; + &lt;# of hours&gt; + &apos;H&apos; + &lt;# of minutes&gt; + &apos;M&apos; + &lt;# of seconds&gt; +&apos;S&apos;.</rdfs:comment>
        <rdfs:isDefinedBy rdf:resource="http://cybox.mitre.org/objects/System"/>
        <rdfs:label>Uptime</rdfs:label>
    </owl:DatatypeProperty>
    


    <!-- http://cybox.mitre.org/objects/System#username -->

    <owl:DatatypeProperty rdf:about="http://cybox.mitre.org/objects/System#username">
        <rdfs:range rdf:resource="http://www.w3.org/2001/XMLSchema#string"/>
        <rdfs:comment>Specifies the name of the user currently logged into the system.</rdfs:comment>
        <rdfs:isDefinedBy rdf:resource="http://cybox.mitre.org/objects/System"/>
        <rdfs:label>Username of Current User</rdfs:label>
    </owl:DatatypeProperty>
    


    <!-- http://cybox.mitre.org/objects/System#windowsDirectory -->

    <owl:DatatypeProperty rdf:about="http://cybox.mitre.org/objects/System#windowsDirectory">
        <rdfs:range rdf:resource="http://www.w3.org/2001/XMLSchema#string"/>
        <rdfs:comment>Specifies the fully-qualified path to the Windows install directory.</rdfs:comment>
        <rdfs:isDefinedBy rdf:resource="http://cybox.mitre.org/objects/System"/>
        <rdfs:label>Windows Directory</rdfs:label>
    </owl:DatatypeProperty>
    


    <!-- http://cybox.mitre.org/objects/System#windowsSystemDirectory -->

    <owl:DatatypeProperty rdf:about="http://cybox.mitre.org/objects/System#windowsSystemDirectory">
        <rdfs:range rdf:resource="http://www.w3.org/2001/XMLSchema#string"/>
        <rdfs:comment>Specifies the fully-qualified path to the Windows system directory.</rdfs:comment>
        <rdfs:isDefinedBy rdf:resource="http://cybox.mitre.org/objects/System"/>
        <rdfs:label>Windows System Directory</rdfs:label>
    </owl:DatatypeProperty>
    


    <!-- http://cybox.mitre.org/objects/System#windowsTempDirectory -->

    <owl:DatatypeProperty rdf:about="http://cybox.mitre.org/objects/System#windowsTempDirectory">
        <rdfs:range rdf:resource="http://www.w3.org/2001/XMLSchema#string"/>
        <rdfs:comment>Specifies the fully-qualified path to the Windows temporary files directory.</rdfs:comment>
        <rdfs:isDefinedBy rdf:resource="http://cybox.mitre.org/objects/System"/>
        <rdfs:label>Windows Temp Directory</rdfs:label>
    </owl:DatatypeProperty>
    


    <!-- 
    ///////////////////////////////////////////////////////////////////////////////////////
    //
    // Classes
    //
    ///////////////////////////////////////////////////////////////////////////////////////
     -->

    




    <!-- http://cybox.mitre.org/objects/System#GlobalFlag -->

    <owl:Class rdf:about="http://cybox.mitre.org/objects/System#GlobalFlag">
        <rdfs:subClassOf>
            <owl:Restriction>
                <owl:onProperty rdf:resource="http://cybox.mitre.org/objects/System#hexadecimalValue"/>
                <owl:cardinality rdf:datatype="http://www.w3.org/2001/XMLSchema#nonNegativeInteger">1</owl:cardinality>
            </owl:Restriction>
        </rdfs:subClassOf>
        <rdfs:subClassOf>
            <owl:Restriction>
                <owl:onProperty rdf:resource="http://cybox.mitre.org/objects/System#symbolicName"/>
                <owl:cardinality rdf:datatype="http://www.w3.org/2001/XMLSchema#nonNegativeInteger">1</owl:cardinality>
            </owl:Restriction>
        </rdfs:subClassOf>
        <rdfs:subClassOf>
            <owl:Restriction>
                <owl:onProperty rdf:resource="http://cybox.mitre.org/objects/System#abbreviation"/>
                <owl:maxCardinality rdf:datatype="http://www.w3.org/2001/XMLSchema#nonNegativeInteger">1</owl:maxCardinality>
            </owl:Restriction>
        </rdfs:subClassOf>
        <rdfs:subClassOf>
            <owl:Restriction>
                <owl:onProperty rdf:resource="http://cybox.mitre.org/objects/System#destination"/>
                <owl:maxCardinality rdf:datatype="http://www.w3.org/2001/XMLSchema#nonNegativeInteger">1</owl:maxCardinality>
            </owl:Restriction>
        </rdfs:subClassOf>
        <rdfs:comment>Characterize Windows global flags.</rdfs:comment>
        <rdfs:isDefinedBy rdf:resource="http://cybox.mitre.org/objects/System"/>
        <rdfs:label>Global flag</rdfs:label>
    </owl:Class>
    


    <!-- http://cybox.mitre.org/objects/System#IPInfo -->

    <owl:Class rdf:about="http://cybox.mitre.org/objects/System#IPInfo">
        <rdfs:subClassOf>
            <owl:Restriction>
                <owl:onProperty rdf:resource="http://cybox.mitre.org/objects/System#ipAddress"/>
                <owl:cardinality rdf:datatype="http://www.w3.org/2001/XMLSchema#nonNegativeInteger">1</owl:cardinality>
            </owl:Restriction>
        </rdfs:subClassOf>
        <rdfs:subClassOf>
            <owl:Restriction>
                <owl:onProperty rdf:resource="http://cybox.mitre.org/objects/System#subnetMask"/>
                <owl:maxCardinality rdf:datatype="http://www.w3.org/2001/XMLSchema#nonNegativeInteger">1</owl:maxCardinality>
            </owl:Restriction>
        </rdfs:subClassOf>
        <rdfs:comment>Characterizes  information about the IP address and its associated subnet mask used by a network interface.</rdfs:comment>
        <rdfs:isDefinedBy rdf:resource="http://cybox.mitre.org/objects/System"/>
        <rdfs:label>IPInfo</rdfs:label>
    </owl:Class>
    


    <!-- http://cybox.mitre.org/objects/System#NetworkInterface -->

    <owl:Class rdf:about="http://cybox.mitre.org/objects/System#NetworkInterface">
        <rdfs:subClassOf>
            <owl:Restriction>
                <owl:onProperty rdf:resource="http://cybox.mitre.org/objects/System#macAddress"/>
                <owl:maxCardinality rdf:datatype="http://www.w3.org/2001/XMLSchema#nonNegativeInteger">1</owl:maxCardinality>
            </owl:Restriction>
        </rdfs:subClassOf>
        <rdfs:subClassOf>
            <owl:Restriction>
                <owl:onProperty rdf:resource="http://cybox.mitre.org/objects/System#adapter"/>
                <owl:cardinality rdf:datatype="http://www.w3.org/2001/XMLSchema#nonNegativeInteger">1</owl:cardinality>
            </owl:Restriction>
        </rdfs:subClassOf>
        <rdfs:subClassOf>
            <owl:Restriction>
                <owl:onProperty rdf:resource="http://cybox.mitre.org/objects/System#description"/>
                <owl:maxCardinality rdf:datatype="http://www.w3.org/2001/XMLSchema#nonNegativeInteger">1</owl:maxCardinality>
            </owl:Restriction>
        </rdfs:subClassOf>
        <rdfs:subClassOf>
            <owl:Restriction>
                <owl:onProperty rdf:resource="http://cybox.mitre.org/objects/System#dhcpLeaseExpiresDateTime"/>
                <owl:maxCardinality rdf:datatype="http://www.w3.org/2001/XMLSchema#nonNegativeInteger">1</owl:maxCardinality>
            </owl:Restriction>
        </rdfs:subClassOf>
        <rdfs:subClassOf>
            <owl:Restriction>
                <owl:onProperty rdf:resource="http://cybox.mitre.org/objects/System#dhcpLeaseObtainedDateTime"/>
                <owl:maxCardinality rdf:datatype="http://www.w3.org/2001/XMLSchema#nonNegativeInteger">1</owl:maxCardinality>
            </owl:Restriction>
        </rdfs:subClassOf>
        <rdfs:comment>Characterizes information about a network interface, such as its MAC address.</rdfs:comment>
        <rdfs:isDefinedBy rdf:resource="http://cybox.mitre.org/objects/System"/>
        <rdfs:label>Network Interface</rdfs:label>
    </owl:Class>
    


    <!-- http://cybox.mitre.org/objects/System#OperatingSystemInfo -->

    <owl:Class rdf:about="http://cybox.mitre.org/objects/System#OperatingSystemInfo">
        <rdfs:subClassOf rdf:resource="http://cybox.mitre.org/cyboxCommon#PlatformSpecification"/>
        <rdfs:subClassOf>
            <owl:Restriction>
                <owl:onProperty rdf:resource="http://cybox.mitre.org/objects/System#platform"/>
                <owl:maxCardinality rdf:datatype="http://www.w3.org/2001/XMLSchema#nonNegativeInteger">1</owl:maxCardinality>
            </owl:Restriction>
        </rdfs:subClassOf>
        <rdfs:subClassOf>
            <owl:Restriction>
                <owl:onProperty rdf:resource="http://cybox.mitre.org/objects/System#bitness"/>
                <owl:maxCardinality rdf:datatype="http://www.w3.org/2001/XMLSchema#nonNegativeInteger">1</owl:maxCardinality>
            </owl:Restriction>
        </rdfs:subClassOf>
        <rdfs:subClassOf>
            <owl:Restriction>
                <owl:onProperty rdf:resource="http://cybox.mitre.org/objects/System#buildNumber"/>
                <owl:maxCardinality rdf:datatype="http://www.w3.org/2001/XMLSchema#nonNegativeInteger">1</owl:maxCardinality>
            </owl:Restriction>
        </rdfs:subClassOf>
        <rdfs:subClassOf>
            <owl:Restriction>
                <owl:onProperty rdf:resource="http://cybox.mitre.org/objects/System#installDate"/>
                <owl:maxCardinality rdf:datatype="http://www.w3.org/2001/XMLSchema#nonNegativeInteger">1</owl:maxCardinality>
            </owl:Restriction>
        </rdfs:subClassOf>
        <rdfs:subClassOf>
            <owl:Restriction>
                <owl:onProperty rdf:resource="http://cybox.mitre.org/objects/System#patchLevel"/>
                <owl:maxCardinality rdf:datatype="http://www.w3.org/2001/XMLSchema#nonNegativeInteger">1</owl:maxCardinality>
            </owl:Restriction>
        </rdfs:subClassOf>
        <rdfs:comment>Characterizes informatinon about an installation of an operating system.</rdfs:comment>
        <rdfs:isDefinedBy rdf:resource="http://cybox.mitre.org/objects/System"/>
        <rdfs:label>Operating System Information</rdfs:label>
    </owl:Class>
    


    <!-- http://cybox.mitre.org/objects/System#System -->

    <owl:Class rdf:about="http://cybox.mitre.org/objects/System#System">
        <rdfs:subClassOf rdf:resource="http://cybox.mitre.org/cybox_core#Object"/>
        <rdfs:subClassOf>
            <owl:Restriction>
                <owl:onProperty rdf:resource="http://cybox.mitre.org/objects/System#BIOS.manufacturerDetails"/>
                <owl:maxCardinality rdf:datatype="http://www.w3.org/2001/XMLSchema#nonNegativeInteger">1</owl:maxCardinality>
            </owl:Restriction>
        </rdfs:subClassOf>
        <rdfs:subClassOf>
            <owl:Restriction>
                <owl:onProperty rdf:resource="http://cybox.mitre.org/objects/System#hostname.details"/>
                <owl:maxCardinality rdf:datatype="http://www.w3.org/2001/XMLSchema#nonNegativeInteger">1</owl:maxCardinality>
            </owl:Restriction>
        </rdfs:subClassOf>
        <rdfs:subClassOf>
            <owl:Restriction>
                <owl:onProperty rdf:resource="http://cybox.mitre.org/objects/System#operatingSystem"/>
                <owl:maxCardinality rdf:datatype="http://www.w3.org/2001/XMLSchema#nonNegativeInteger">1</owl:maxCardinality>
            </owl:Restriction>
        </rdfs:subClassOf>
        <rdfs:subClassOf>
            <owl:Restriction>
                <owl:onProperty rdf:resource="http://cybox.mitre.org/objects/System#username.details"/>
                <owl:maxCardinality rdf:datatype="http://www.w3.org/2001/XMLSchema#nonNegativeInteger">1</owl:maxCardinality>
            </owl:Restriction>
        </rdfs:subClassOf>
        <rdfs:subClassOf>
            <owl:Restriction>
                <owl:onProperty rdf:resource="http://cybox.mitre.org/objects/System#hostname"/>
                <owl:cardinality rdf:datatype="http://www.w3.org/2001/XMLSchema#nonNegativeInteger">1</owl:cardinality>
            </owl:Restriction>
        </rdfs:subClassOf>
        <rdfs:subClassOf>
            <owl:Restriction>
                <owl:onProperty rdf:resource="http://cybox.mitre.org/objects/System#processorArchitecture"/>
                <owl:cardinality rdf:datatype="http://www.w3.org/2001/XMLSchema#nonNegativeInteger">1</owl:cardinality>
            </owl:Restriction>
        </rdfs:subClassOf>
        <rdfs:subClassOf>
            <owl:Restriction>
                <owl:onProperty rdf:resource="http://cybox.mitre.org/objects/System#BIOS.date"/>
                <owl:maxCardinality rdf:datatype="http://www.w3.org/2001/XMLSchema#nonNegativeInteger">1</owl:maxCardinality>
            </owl:Restriction>
        </rdfs:subClassOf>
        <rdfs:subClassOf>
            <owl:Restriction>
                <owl:onProperty rdf:resource="http://cybox.mitre.org/objects/System#BIOS.manufactureName"/>
                <owl:maxCardinality rdf:datatype="http://www.w3.org/2001/XMLSchema#nonNegativeInteger">1</owl:maxCardinality>
            </owl:Restriction>
        </rdfs:subClassOf>
        <rdfs:subClassOf>
            <owl:Restriction>
                <owl:onProperty rdf:resource="http://cybox.mitre.org/objects/System#BIOS.releaseDate"/>
                <owl:maxCardinality rdf:datatype="http://www.w3.org/2001/XMLSchema#nonNegativeInteger">1</owl:maxCardinality>
            </owl:Restriction>
        </rdfs:subClassOf>
        <rdfs:subClassOf>
            <owl:Restriction>
                <owl:onProperty rdf:resource="http://cybox.mitre.org/objects/System#BIOS.serialNumber"/>
                <owl:maxCardinality rdf:datatype="http://www.w3.org/2001/XMLSchema#nonNegativeInteger">1</owl:maxCardinality>
            </owl:Restriction>
        </rdfs:subClassOf>
        <rdfs:subClassOf>
            <owl:Restriction>
                <owl:onProperty rdf:resource="http://cybox.mitre.org/objects/System#BIOS.version"/>
                <owl:maxCardinality rdf:datatype="http://www.w3.org/2001/XMLSchema#nonNegativeInteger">1</owl:maxCardinality>
            </owl:Restriction>
        </rdfs:subClassOf>
        <rdfs:subClassOf>
            <owl:Restriction>
                <owl:onProperty rdf:resource="http://cybox.mitre.org/objects/System#availPhysicalMemory"/>
                <owl:maxCardinality rdf:datatype="http://www.w3.org/2001/XMLSchema#nonNegativeInteger">1</owl:maxCardinality>
            </owl:Restriction>
        </rdfs:subClassOf>
        <rdfs:subClassOf>
            <owl:Restriction>
                <owl:onProperty rdf:resource="http://cybox.mitre.org/objects/System#currentDate"/>
                <owl:maxCardinality rdf:datatype="http://www.w3.org/2001/XMLSchema#nonNegativeInteger">1</owl:maxCardinality>
            </owl:Restriction>
        </rdfs:subClassOf>
        <rdfs:subClassOf>
            <owl:Restriction>
                <owl:onProperty rdf:resource="http://cybox.mitre.org/objects/System#localTime"/>
                <owl:maxCardinality rdf:datatype="http://www.w3.org/2001/XMLSchema#nonNegativeInteger">1</owl:maxCardinality>
            </owl:Restriction>
        </rdfs:subClassOf>
        <rdfs:subClassOf>
            <owl:Restriction>
                <owl:onProperty rdf:resource="http://cybox.mitre.org/objects/System#processor"/>
                <owl:maxCardinality rdf:datatype="http://www.w3.org/2001/XMLSchema#nonNegativeInteger">1</owl:maxCardinality>
            </owl:Restriction>
        </rdfs:subClassOf>
        <rdfs:subClassOf>
            <owl:Restriction>
                <owl:onProperty rdf:resource="http://cybox.mitre.org/objects/System#systemTime"/>
                <owl:maxCardinality rdf:datatype="http://www.w3.org/2001/XMLSchema#nonNegativeInteger">1</owl:maxCardinality>
            </owl:Restriction>
        </rdfs:subClassOf>
        <rdfs:subClassOf>
            <owl:Restriction>
                <owl:onProperty rdf:resource="http://cybox.mitre.org/objects/System#timezoneDST"/>
                <owl:maxCardinality rdf:datatype="http://www.w3.org/2001/XMLSchema#nonNegativeInteger">1</owl:maxCardinality>
            </owl:Restriction>
        </rdfs:subClassOf>
        <rdfs:subClassOf>
            <owl:Restriction>
                <owl:onProperty rdf:resource="http://cybox.mitre.org/objects/System#timezoneStandard"/>
                <owl:maxCardinality rdf:datatype="http://www.w3.org/2001/XMLSchema#nonNegativeInteger">1</owl:maxCardinality>
            </owl:Restriction>
        </rdfs:subClassOf>
        <rdfs:subClassOf>
            <owl:Restriction>
                <owl:onProperty rdf:resource="http://cybox.mitre.org/objects/System#totalPhysicalMemory"/>
                <owl:maxCardinality rdf:datatype="http://www.w3.org/2001/XMLSchema#nonNegativeInteger">1</owl:maxCardinality>
            </owl:Restriction>
        </rdfs:subClassOf>
        <rdfs:subClassOf>
            <owl:Restriction>
                <owl:onProperty rdf:resource="http://cybox.mitre.org/objects/System#uptime"/>
                <owl:maxCardinality rdf:datatype="http://www.w3.org/2001/XMLSchema#nonNegativeInteger">1</owl:maxCardinality>
            </owl:Restriction>
        </rdfs:subClassOf>
        <rdfs:subClassOf>
            <owl:Restriction>
                <owl:onProperty rdf:resource="http://cybox.mitre.org/objects/System#username"/>
                <owl:maxCardinality rdf:datatype="http://www.w3.org/2001/XMLSchema#nonNegativeInteger">1</owl:maxCardinality>
            </owl:Restriction>
        </rdfs:subClassOf>
        <rdfs:comment>Characterize computer systems (as a combination of both software and hardware).</rdfs:comment>
        <rdfs:isDefinedBy rdf:resource="http://cybox.mitre.org/objects/System"/>
        <rdfs:label>System</rdfs:label>
    </owl:Class>
    


    <!-- http://cybox.mitre.org/objects/System#WindowsSystem -->

    <owl:Class rdf:about="http://cybox.mitre.org/objects/System#WindowsSystem">
        <rdfs:subClassOf rdf:resource="http://cybox.mitre.org/objects/System#System"/>
        <rdfs:subClassOf>
            <owl:Restriction>
                <owl:onProperty rdf:resource="http://cybox.mitre.org/objects/System#netBIOSName"/>
                <owl:cardinality rdf:datatype="http://www.w3.org/2001/XMLSchema#nonNegativeInteger">1</owl:cardinality>
            </owl:Restriction>
        </rdfs:subClassOf>
        <rdfs:subClassOf>
            <owl:Restriction>
                <owl:onProperty rdf:resource="http://cybox.mitre.org/objects/System#microsoftProductID"/>
                <owl:maxCardinality rdf:datatype="http://www.w3.org/2001/XMLSchema#nonNegativeInteger">1</owl:maxCardinality>
            </owl:Restriction>
        </rdfs:subClassOf>
        <rdfs:subClassOf>
            <owl:Restriction>
                <owl:onProperty rdf:resource="http://cybox.mitre.org/objects/System#productName"/>
                <owl:maxCardinality rdf:datatype="http://www.w3.org/2001/XMLSchema#nonNegativeInteger">1</owl:maxCardinality>
            </owl:Restriction>
        </rdfs:subClassOf>
        <rdfs:subClassOf>
            <owl:Restriction>
                <owl:onProperty rdf:resource="http://cybox.mitre.org/objects/System#registerdOwner"/>
                <owl:maxCardinality rdf:datatype="http://www.w3.org/2001/XMLSchema#nonNegativeInteger">1</owl:maxCardinality>
            </owl:Restriction>
        </rdfs:subClassOf>
        <rdfs:subClassOf>
            <owl:Restriction>
                <owl:onProperty rdf:resource="http://cybox.mitre.org/objects/System#registeredOrganization"/>
                <owl:maxCardinality rdf:datatype="http://www.w3.org/2001/XMLSchema#nonNegativeInteger">1</owl:maxCardinality>
            </owl:Restriction>
        </rdfs:subClassOf>
        <rdfs:subClassOf>
            <owl:Restriction>
                <owl:onProperty rdf:resource="http://cybox.mitre.org/objects/System#windowsDirectory"/>
                <owl:maxCardinality rdf:datatype="http://www.w3.org/2001/XMLSchema#nonNegativeInteger">1</owl:maxCardinality>
            </owl:Restriction>
        </rdfs:subClassOf>
        <rdfs:subClassOf>
            <owl:Restriction>
                <owl:onProperty rdf:resource="http://cybox.mitre.org/objects/System#windowsSystemDirectory"/>
                <owl:maxCardinality rdf:datatype="http://www.w3.org/2001/XMLSchema#nonNegativeInteger">1</owl:maxCardinality>
            </owl:Restriction>
        </rdfs:subClassOf>
        <rdfs:subClassOf>
            <owl:Restriction>
                <owl:onProperty rdf:resource="http://cybox.mitre.org/objects/System#windowsTempDirectory"/>
                <owl:maxCardinality rdf:datatype="http://www.w3.org/2001/XMLSchema#nonNegativeInteger">1</owl:maxCardinality>
            </owl:Restriction>
        </rdfs:subClassOf>
        <rdfs:comment>Characterize Windows systems.</rdfs:comment>
        <rdfs:isDefinedBy rdf:resource="http://cybox.mitre.org/objects/System"/>
        <rdfs:label>Windows system</rdfs:label>
    </owl:Class>
    


</rdf:RDF>



<!-- Generated by the OWL API (version 4.2.6.20160910-2108) https://github.com/owlcs/owlapi -->

