<?xml version="1.0"?>
<rdf:RDF xmlns="http://cybox.mitre.org/objects/URLHistory#"
     xml:base="http://cybox.mitre.org/objects/URLHistory"
     xmlns:rdf="http://www.w3.org/1999/02/22-rdf-syntax-ns#"
     xmlns:owl="http://www.w3.org/2002/07/owl#"
     xmlns:xml="http://www.w3.org/XML/1998/namespace"
     xmlns:urlHistoryObj="http://cybox.mitre.org/objects/URLHistory#"
     xmlns:xsd="http://www.w3.org/2001/XMLSchema#"
     xmlns:rdfs="http://www.w3.org/2000/01/rdf-schema#">
    <owl:Ontology rdf:about="http://cybox.mitre.org/objects/URLHistory">
        <owl:imports rdf:resource="http://cybox.mitre.org/objects/URI"/>
        <owl:imports rdf:resource="http://cybox.mitre.org/objects/Hostname"/>
        <owl:imports rdf:resource="http://cybox.mitre.org/cybox_core"/>
        <rdfs:label>Cyber Observable eXpression (CybOX) URL History Ontology</rdfs:label>
        <owl:versionInfo rdf:datatype="http://www.w3.org/2001/XMLSchema#string">2.1.0-000</owl:versionInfo>
        <rdfs:comment>This ontology provides a vocabulary and representation of a URL History for the  Cyber Observable eXpression (CybOX).  

CybOX  provides a common mechansim (structure and content) to convey the full range of potential cyber observable information and strives to be fully expressive, flexible, extensible, automatable, and as human-readable as possible.

The ontology is based on the CybOX URL History object schema maintained by The MITRE Corporation copyright 2012-2014.  The version number of the ontology is kept in sync with the schema in order to more easily relate between the ontology and the corresponding schema version.

Copyright (c) 2014, DaedaFusion, LLC.  All rights reserved.</rdfs:comment>
    </owl:Ontology>
    


    <!-- 
    ///////////////////////////////////////////////////////////////////////////////////////
    //
    // Object Properties
    //
    ///////////////////////////////////////////////////////////////////////////////////////
     -->

    


    <!-- http://cybox.mitre.org/objects/URLHistory#browerInformation -->

    <owl:ObjectProperty rdf:about="http://cybox.mitre.org/objects/URLHistory#browerInformation">
        <rdfs:domain rdf:resource="http://cybox.mitre.org/objects/URLHistory#URLHistory"/>
        <rdfs:range rdf:resource="http://cybox.mitre.org/cyboxCommon#ToolInformation"/>
        <rdfs:comment>Specifies information about the particular Web Browser whose URL history is being captured.</rdfs:comment>
        <rdfs:isDefinedBy rdf:resource="http://cybox.mitre.org/objects/URLHistory"/>
        <rdfs:label>Brower Information</rdfs:label>
    </owl:ObjectProperty>
    


    <!-- http://cybox.mitre.org/objects/URLHistory#hostname -->

    <owl:ObjectProperty rdf:about="http://cybox.mitre.org/objects/URLHistory#hostname">
        <rdfs:domain rdf:resource="http://cybox.mitre.org/objects/URLHistory#URLHistoryEntry"/>
        <rdfs:range rdf:resource="http://cybox.mitre.org/objects/Hostname#Hostname"/>
        <rdfs:comment>Specifies the hostname portion of the URL that the URL history entry points to (captured in the URL field).</rdfs:comment>
        <rdfs:isDefinedBy rdf:resource="http://cybox.mitre.org/objects/URLHistory"/>
        <rdfs:label>Hostname</rdfs:label>
    </owl:ObjectProperty>
    


    <!-- http://cybox.mitre.org/objects/URLHistory#referrerURL -->

    <owl:ObjectProperty rdf:about="http://cybox.mitre.org/objects/URLHistory#referrerURL">
        <rdfs:domain rdf:resource="http://cybox.mitre.org/objects/URLHistory#URLHistoryEntry"/>
        <rdfs:range rdf:resource="http://cybox.mitre.org/objects/URI#URL"/>
        <rdfs:comment>Specifies the origination point (i.e., URL) of the URL captured in the URL history entry, if applicable.</rdfs:comment>
        <rdfs:isDefinedBy rdf:resource="http://cybox.mitre.org/objects/URLHistory"/>
        <rdfs:label>Referrer URL</rdfs:label>
    </owl:ObjectProperty>
    


    <!-- http://cybox.mitre.org/objects/URLHistory#url -->

    <owl:ObjectProperty rdf:about="http://cybox.mitre.org/objects/URLHistory#url">
        <rdfs:domain rdf:resource="http://cybox.mitre.org/objects/URLHistory#URLHistoryEntry"/>
        <rdfs:range rdf:resource="http://cybox.mitre.org/objects/URI#URL"/>
        <rdfs:comment>Specifies the URL that the URL history entry points to.</rdfs:comment>
        <rdfs:isDefinedBy rdf:resource="http://cybox.mitre.org/objects/URLHistory"/>
        <rdfs:label>URL</rdfs:label>
    </owl:ObjectProperty>
    


    <!-- http://cybox.mitre.org/objects/URLHistory#urlHistoryEntries -->

    <owl:ObjectProperty rdf:about="http://cybox.mitre.org/objects/URLHistory#urlHistoryEntries">
        <rdfs:domain rdf:resource="http://cybox.mitre.org/objects/URLHistory#URLHistory"/>
        <rdfs:range rdf:resource="http://cybox.mitre.org/objects/URLHistory#URLHistoryEntry"/>
        <rdfs:comment>Specifies one or more URL history records stored in the browser&apos;s history.</rdfs:comment>
        <rdfs:isDefinedBy rdf:resource="http://cybox.mitre.org/objects/URLHistory"/>
        <rdfs:label>URL History Entries</rdfs:label>
    </owl:ObjectProperty>
    


    <!-- 
    ///////////////////////////////////////////////////////////////////////////////////////
    //
    // Data properties
    //
    ///////////////////////////////////////////////////////////////////////////////////////
     -->

    


    <!-- http://cybox.mitre.org/objects/URLHistory#expirationDateTime -->

    <owl:DatatypeProperty rdf:about="http://cybox.mitre.org/objects/URLHistory#expirationDateTime">
        <rdfs:domain rdf:resource="http://cybox.mitre.org/objects/URLHistory#URLHistoryEntry"/>
        <rdfs:range rdf:resource="http://www.w3.org/2001/XMLSchema#dateTime"/>
        <rdfs:comment>Specifies the date/time that the URL history entry expires.</rdfs:comment>
        <rdfs:isDefinedBy rdf:resource="http://cybox.mitre.org/objects/URLHistory"/>
        <rdfs:label>Expiration Date</rdfs:label>
    </owl:DatatypeProperty>
    


    <!-- http://cybox.mitre.org/objects/URLHistory#firstVisitDateTime -->

    <owl:DatatypeProperty rdf:about="http://cybox.mitre.org/objects/URLHistory#firstVisitDateTime">
        <rdfs:domain rdf:resource="http://cybox.mitre.org/objects/URLHistory#URLHistoryEntry"/>
        <rdfs:range rdf:resource="http://www.w3.org/2001/XMLSchema#dateTime"/>
        <rdfs:comment>Specifies the date/time that the URL referred to by the URL field was first visited.</rdfs:comment>
        <rdfs:isDefinedBy rdf:resource="http://cybox.mitre.org/objects/URLHistory"/>
        <rdfs:label>First Visit Date</rdfs:label>
    </owl:DatatypeProperty>
    


    <!-- http://cybox.mitre.org/objects/URLHistory#lastModifiedDateTime -->

    <owl:DatatypeProperty rdf:about="http://cybox.mitre.org/objects/URLHistory#lastModifiedDateTime">
        <rdfs:domain rdf:resource="http://cybox.mitre.org/objects/URLHistory#URLHistoryEntry"/>
        <rdfs:range rdf:resource="http://www.w3.org/2001/XMLSchema#dateTime"/>
        <rdfs:comment>Specifies the date/time that the URL history entry was last modified.</rdfs:comment>
        <rdfs:isDefinedBy rdf:resource="http://cybox.mitre.org/objects/URLHistory"/>
        <rdfs:label>Last Modified</rdfs:label>
    </owl:DatatypeProperty>
    


    <!-- http://cybox.mitre.org/objects/URLHistory#lastVisitDateTime -->

    <owl:DatatypeProperty rdf:about="http://cybox.mitre.org/objects/URLHistory#lastVisitDateTime">
        <rdfs:domain rdf:resource="http://cybox.mitre.org/objects/URLHistory#URLHistoryEntry"/>
        <rdfs:range rdf:resource="http://www.w3.org/2001/XMLSchema#dateTime"/>
        <rdfs:comment>Specifies the date/time that the URL referred to by the URL field was last visited.</rdfs:comment>
        <rdfs:isDefinedBy rdf:resource="http://cybox.mitre.org/objects/URLHistory"/>
        <rdfs:label>Last Visit Date</rdfs:label>
    </owl:DatatypeProperty>
    


    <!-- http://cybox.mitre.org/objects/URLHistory#manuallyEnteredCount -->

    <owl:DatatypeProperty rdf:about="http://cybox.mitre.org/objects/URLHistory#manuallyEnteredCount">
        <rdfs:domain rdf:resource="http://cybox.mitre.org/objects/URLHistory#URLHistoryEntry"/>
        <rdfs:range rdf:resource="http://www.w3.org/2001/XMLSchema#nonNegativeInteger"/>
        <rdfs:comment>Specifies the number of times the URL referred to by the URL field was manually entered into the browser&apos;s address field by the user. 

This field is only applicable for URL history entries generated by Google&apos;s Chrome browser.</rdfs:comment>
        <rdfs:isDefinedBy rdf:resource="http://cybox.mitre.org/objects/URLHistory"/>
        <rdfs:label>Manually-Entered Count</rdfs:label>
    </owl:DatatypeProperty>
    


    <!-- http://cybox.mitre.org/objects/URLHistory#pageTitle -->

    <owl:DatatypeProperty rdf:about="http://cybox.mitre.org/objects/URLHistory#pageTitle">
        <rdfs:domain rdf:resource="http://cybox.mitre.org/objects/URLHistory#URLHistoryEntry"/>
        <rdfs:range rdf:resource="http://www.w3.org/2001/XMLSchema#string"/>
        <rdfs:comment>Specifies the title of the web page referred to by the URL captured in the URL field.</rdfs:comment>
        <rdfs:isDefinedBy rdf:resource="http://cybox.mitre.org/objects/URLHistory"/>
        <rdfs:label>Page Title</rdfs:label>
    </owl:DatatypeProperty>
    


    <!-- http://cybox.mitre.org/objects/URLHistory#userProfileName -->

    <owl:DatatypeProperty rdf:about="http://cybox.mitre.org/objects/URLHistory#userProfileName">
        <rdfs:domain rdf:resource="http://cybox.mitre.org/objects/URLHistory#URLHistoryEntry"/>
        <rdfs:range rdf:resource="http://www.w3.org/2001/XMLSchema#string"/>
        <rdfs:comment>Specifies the name of the web browser user profile for which the URL history entry was created.</rdfs:comment>
        <rdfs:isDefinedBy rdf:resource="http://cybox.mitre.org/objects/URLHistory"/>
        <rdfs:label>User Profile Name</rdfs:label>
    </owl:DatatypeProperty>
    


    <!-- http://cybox.mitre.org/objects/URLHistory#visitCount -->

    <owl:DatatypeProperty rdf:about="http://cybox.mitre.org/objects/URLHistory#visitCount">
        <rdfs:domain rdf:resource="http://cybox.mitre.org/objects/URLHistory#URLHistoryEntry"/>
        <rdfs:range rdf:resource="http://www.w3.org/2001/XMLSchema#nonNegativeInteger"/>
        <rdfs:comment>Specifies the number of times the URL referred to by the URL field has been visited.</rdfs:comment>
        <rdfs:isDefinedBy rdf:resource="http://cybox.mitre.org/objects/URLHistory"/>
        <rdfs:label>Visit Count</rdfs:label>
    </owl:DatatypeProperty>
    


    <!-- 
    ///////////////////////////////////////////////////////////////////////////////////////
    //
    // Classes
    //
    ///////////////////////////////////////////////////////////////////////////////////////
     -->

   

    <!-- http://cybox.mitre.org/objects/URLHistory#URLHistory -->

    <owl:Class rdf:about="http://cybox.mitre.org/objects/URLHistory#URLHistory">
        <rdfs:subClassOf rdf:resource="http://cybox.mitre.org/cybox_core#Object"/>
        <rdfs:subClassOf>
            <owl:Restriction>
                <owl:onProperty rdf:resource="http://cybox.mitre.org/objects/URLHistory#browerInformation"/>
                <owl:maxCardinality rdf:datatype="http://www.w3.org/2001/XMLSchema#nonNegativeInteger">1</owl:maxCardinality>
            </owl:Restriction>
        </rdfs:subClassOf>
        <rdfs:comment>Characterizes the stored URL history for a particular web browser</rdfs:comment>
        <rdfs:isDefinedBy rdf:resource="http://cybox.mitre.org/objects/URLHistory"/>
    </owl:Class>
    


    <!-- http://cybox.mitre.org/objects/URLHistory#URLHistoryEntry -->

    <owl:Class rdf:about="http://cybox.mitre.org/objects/URLHistory#URLHistoryEntry">
        <rdfs:subClassOf>
            <owl:Restriction>
                <owl:onProperty rdf:resource="http://cybox.mitre.org/objects/URLHistory#hostname"/>
                <owl:maxCardinality rdf:datatype="http://www.w3.org/2001/XMLSchema#nonNegativeInteger">1</owl:maxCardinality>
            </owl:Restriction>
        </rdfs:subClassOf>
        <rdfs:subClassOf>
            <owl:Restriction>
                <owl:onProperty rdf:resource="http://cybox.mitre.org/objects/URLHistory#referrerURL"/>
                <owl:maxCardinality rdf:datatype="http://www.w3.org/2001/XMLSchema#nonNegativeInteger">1</owl:maxCardinality>
            </owl:Restriction>
        </rdfs:subClassOf>
        <rdfs:subClassOf>
            <owl:Restriction>
                <owl:onProperty rdf:resource="http://cybox.mitre.org/objects/URLHistory#url"/>
                <owl:maxCardinality rdf:datatype="http://www.w3.org/2001/XMLSchema#nonNegativeInteger">1</owl:maxCardinality>
            </owl:Restriction>
        </rdfs:subClassOf>
        <rdfs:subClassOf>
            <owl:Restriction>
                <owl:onProperty rdf:resource="http://cybox.mitre.org/objects/URLHistory#expirationDateTime"/>
                <owl:maxCardinality rdf:datatype="http://www.w3.org/2001/XMLSchema#nonNegativeInteger">1</owl:maxCardinality>
            </owl:Restriction>
        </rdfs:subClassOf>
        <rdfs:subClassOf>
            <owl:Restriction>
                <owl:onProperty rdf:resource="http://cybox.mitre.org/objects/URLHistory#firstVisitDateTime"/>
                <owl:maxCardinality rdf:datatype="http://www.w3.org/2001/XMLSchema#nonNegativeInteger">1</owl:maxCardinality>
            </owl:Restriction>
        </rdfs:subClassOf>
        <rdfs:subClassOf>
            <owl:Restriction>
                <owl:onProperty rdf:resource="http://cybox.mitre.org/objects/URLHistory#lastModifiedDateTime"/>
                <owl:maxCardinality rdf:datatype="http://www.w3.org/2001/XMLSchema#nonNegativeInteger">1</owl:maxCardinality>
            </owl:Restriction>
        </rdfs:subClassOf>
        <rdfs:subClassOf>
            <owl:Restriction>
                <owl:onProperty rdf:resource="http://cybox.mitre.org/objects/URLHistory#lastVisitDateTime"/>
                <owl:maxCardinality rdf:datatype="http://www.w3.org/2001/XMLSchema#nonNegativeInteger">1</owl:maxCardinality>
            </owl:Restriction>
        </rdfs:subClassOf>
        <rdfs:subClassOf>
            <owl:Restriction>
                <owl:onProperty rdf:resource="http://cybox.mitre.org/objects/URLHistory#manuallyEnteredCount"/>
                <owl:maxCardinality rdf:datatype="http://www.w3.org/2001/XMLSchema#nonNegativeInteger">1</owl:maxCardinality>
            </owl:Restriction>
        </rdfs:subClassOf>
        <rdfs:subClassOf>
            <owl:Restriction>
                <owl:onProperty rdf:resource="http://cybox.mitre.org/objects/URLHistory#pageTitle"/>
                <owl:maxCardinality rdf:datatype="http://www.w3.org/2001/XMLSchema#nonNegativeInteger">1</owl:maxCardinality>
            </owl:Restriction>
        </rdfs:subClassOf>
        <rdfs:subClassOf>
            <owl:Restriction>
                <owl:onProperty rdf:resource="http://cybox.mitre.org/objects/URLHistory#userProfileName"/>
                <owl:maxCardinality rdf:datatype="http://www.w3.org/2001/XMLSchema#nonNegativeInteger">1</owl:maxCardinality>
            </owl:Restriction>
        </rdfs:subClassOf>
        <rdfs:subClassOf>
            <owl:Restriction>
                <owl:onProperty rdf:resource="http://cybox.mitre.org/objects/URLHistory#visitCount"/>
                <owl:maxCardinality rdf:datatype="http://www.w3.org/2001/XMLSchema#nonNegativeInteger">1</owl:maxCardinality>
            </owl:Restriction>
        </rdfs:subClassOf>
        <rdfs:comment>Characterizes the properties of a URL history entry for a particular browser.</rdfs:comment>
        <rdfs:isDefinedBy rdf:resource="http://cybox.mitre.org/objects/URLHistory"/>
        <rdfs:label>URL History Entry</rdfs:label>
    </owl:Class>
</rdf:RDF>



<!-- Generated by the OWL API (version 4.2.6.20160910-2108) https://github.com/owlcs/owlapi -->

