<?xml version="1.0"?>
<rdf:RDF xmlns="http://cybox.mitre.org/objects/WindowsKernel#"
     xml:base="http://cybox.mitre.org/objects/WindowsKernel"
     xmlns:rdf="http://www.w3.org/1999/02/22-rdf-syntax-ns#"
     xmlns:owl="http://www.w3.org/2002/07/owl#"
     xmlns:xml="http://www.w3.org/XML/1998/namespace"
     xmlns:xsd="http://www.w3.org/2001/XMLSchema#"
     xmlns:rdfs="http://www.w3.org/2000/01/rdf-schema#"
     xmlns:winKernelObj="http://cybox.mitre.org/objects/WindowsKernel#">
    <owl:Ontology rdf:about="http://cybox.mitre.org/objects/WindowsKernel">
        <owl:imports rdf:resource="http://cybox.mitre.org/cybox_core"/>
        <rdfs:label>Cyber Observable eXpression (CybOX) Windows Kernel Ontology</rdfs:label>
        <owl:versionInfo rdf:datatype="http://www.w3.org/2001/XMLSchema#string">2.1.0-000</owl:versionInfo>
        <rdfs:comment>This ontology provides a vocabulary and representation of a Windows Kernel for the  Cyber Observable eXpression (CybOX).  

CybOX provides a common mechansim (structure and content) to convey the full range of potential cyber observable information and strives to be fully expressive, flexible, extensible, automatable, and as human-readable as possible.

The ontology is based on the CybOX Windows Kernel object schema maintained by The MITRE Corporation copyright 2012-2014.  The version number of the ontology is kept in sync with the schema in order to more easily relate between the ontology and the corresponding schema version.

Copyright (c) 2014, DaedaFusion, LLC.  All rights reserved.</rdfs:comment>
    </owl:Ontology>
    


    <!-- 
    ///////////////////////////////////////////////////////////////////////////////////////
    //
    // Object Properties
    //
    ///////////////////////////////////////////////////////////////////////////////////////
     -->

    


    <!-- http://cybox.mitre.org/objects/WindowsKernel#idtEntries -->

    <owl:ObjectProperty rdf:about="http://cybox.mitre.org/objects/WindowsKernel#idtEntries">
        <rdfs:domain rdf:resource="http://cybox.mitre.org/objects/WindowsKernel#WindowsKernel"/>
        <rdfs:range rdf:resource="http://cybox.mitre.org/objects/WindowsKernel#IDTEntry"/>
        <rdfs:comment>Specifies an entry in the he Windows Interrupt Descriptor Table (IDT).</rdfs:comment>
        <rdfs:isDefinedBy rdf:resource="http://cybox.mitre.org/objects/WindowsKernel"/>
        <rdfs:label>IDT Entries</rdfs:label>
    </owl:ObjectProperty>
    


    <!-- http://cybox.mitre.org/objects/WindowsKernel#ssdtEntries -->

    <owl:ObjectProperty rdf:about="http://cybox.mitre.org/objects/WindowsKernel#ssdtEntries">
        <rdfs:domain rdf:resource="http://cybox.mitre.org/objects/WindowsKernel#WindowsKernel"/>
        <rdfs:range rdf:resource="http://cybox.mitre.org/objects/WindowsKernel#SSDTEntry"/>
        <rdfs:comment>Specifies an entry in the Windows System Service Descriptor Table (SSDT). 

The SSDT is a structure that kernel uses to dispatch functions. KeServiceDescriptorTable is a table exported by the kernel that contains pointers to four SSDTs, one for the native API, one for user/GDI support, one of</rdfs:comment>
        <rdfs:isDefinedBy rdf:resource="http://cybox.mitre.org/objects/WindowsKernel"/>
        <rdfs:label>SSDT Entries</rdfs:label>
    </owl:ObjectProperty>
    


    <!-- 
    ///////////////////////////////////////////////////////////////////////////////////////
    //
    // Data properties
    //
    ///////////////////////////////////////////////////////////////////////////////////////
     -->

    


    <!-- http://cybox.mitre.org/objects/WindowsKernel#argumentTableBase -->

    <owl:DatatypeProperty rdf:about="http://cybox.mitre.org/objects/WindowsKernel#argumentTableBase">
        <rdfs:domain rdf:resource="http://cybox.mitre.org/objects/WindowsKernel#SSDTEntry"/>
        <rdfs:range rdf:resource="http://www.w3.org/2001/XMLSchema#hexBinary"/>
        <rdfs:comment>Specifies a pointer to an array of bytes, which indicate the number of bytes used by the function&apos;s arguments.</rdfs:comment>
        <rdfs:isDefinedBy rdf:resource="http://cybox.mitre.org/objects/WindowsKernel"/>
        <rdfs:label>Argument Table Base</rdfs:label>
    </owl:DatatypeProperty>
    


    <!-- http://cybox.mitre.org/objects/WindowsKernel#hooked -->

    <owl:DatatypeProperty rdf:about="http://cybox.mitre.org/objects/WindowsKernel#hooked">
        <rdfs:domain rdf:resource="http://cybox.mitre.org/objects/WindowsKernel#SSDTEntry"/>
        <rdfs:range rdf:resource="http://www.w3.org/2001/XMLSchema#boolean"/>
        <rdfs:comment>Specifies whether the SSDT entry is hooked.</rdfs:comment>
        <rdfs:isDefinedBy rdf:resource="http://cybox.mitre.org/objects/WindowsKernel"/>
        <rdfs:label>Hooked</rdfs:label>
    </owl:DatatypeProperty>
    


    <!-- http://cybox.mitre.org/objects/WindowsKernel#numberOfServices -->

    <owl:DatatypeProperty rdf:about="http://cybox.mitre.org/objects/WindowsKernel#numberOfServices">
        <rdfs:domain rdf:resource="http://cybox.mitre.org/objects/WindowsKernel#SSDTEntry"/>
        <rdfs:range rdf:resource="http://www.w3.org/2001/XMLSchema#nonNegativeInteger"/>
        <rdfs:comment>Specifies the number of entries in the System Service Dispatch Table</rdfs:comment>
        <rdfs:isDefinedBy rdf:resource="http://cybox.mitre.org/objects/WindowsKernel"/>
        <rdfs:label>Number of Services</rdfs:label>
    </owl:DatatypeProperty>
    


    <!-- http://cybox.mitre.org/objects/WindowsKernel#offsetHigh -->

    <owl:DatatypeProperty rdf:about="http://cybox.mitre.org/objects/WindowsKernel#offsetHigh">
        <rdfs:domain rdf:resource="http://cybox.mitre.org/objects/WindowsKernel#IDTEntry"/>
        <rdfs:range rdf:resource="http://www.w3.org/2001/XMLSchema#hexBinary"/>
        <rdfs:comment>Specifies the higher part of the interrupt function&apos;s offset address bits 16-31 in 32-bit, bits 32-63 in 64-bit).</rdfs:comment>
        <rdfs:isDefinedBy rdf:resource="http://cybox.mitre.org/objects/WindowsKernel"/>
        <rdfs:label>Offset High</rdfs:label>
    </owl:DatatypeProperty>
    


    <!-- http://cybox.mitre.org/objects/WindowsKernel#offsetLow -->

    <owl:DatatypeProperty rdf:about="http://cybox.mitre.org/objects/WindowsKernel#offsetLow">
        <rdfs:domain rdf:resource="http://cybox.mitre.org/objects/WindowsKernel#IDTEntry"/>
        <rdfs:range rdf:resource="http://www.w3.org/2001/XMLSchema#hexBinary"/>
        <rdfs:comment>Specifies the lower part of the interrupt function&apos;s offset address (bits 0-15).</rdfs:comment>
        <rdfs:isDefinedBy rdf:resource="http://cybox.mitre.org/objects/WindowsKernel"/>
        <rdfs:label>Offset Low</rdfs:label>
    </owl:DatatypeProperty>
    


    <!-- http://cybox.mitre.org/objects/WindowsKernel#offsetMiddle -->

    <owl:DatatypeProperty rdf:about="http://cybox.mitre.org/objects/WindowsKernel#offsetMiddle">
        <rdfs:domain rdf:resource="http://cybox.mitre.org/objects/WindowsKernel#IDTEntry"/>
        <rdfs:range rdf:resource="http://www.w3.org/2001/XMLSchema#hexBinary"/>
        <rdfs:comment>Specifies in 64-bit architectures, middle part of the interrupt function&apos;s offset address (bits 16-31).</rdfs:comment>
        <rdfs:isDefinedBy rdf:resource="http://cybox.mitre.org/objects/WindowsKernel"/>
        <rdfs:label>Offset Middle (64-bit Only)</rdfs:label>
    </owl:DatatypeProperty>
    


    <!-- http://cybox.mitre.org/objects/WindowsKernel#selector -->

    <owl:DatatypeProperty rdf:about="http://cybox.mitre.org/objects/WindowsKernel#selector">
        <rdfs:domain rdf:resource="http://cybox.mitre.org/objects/WindowsKernel#IDTEntry"/>
        <rdfs:range rdf:resource="http://www.w3.org/2001/XMLSchema#hexBinary"/>
        <rdfs:comment>Specifes a 16-bit value that points to a code segment selector in the Global Descriptot Table.</rdfs:comment>
        <rdfs:isDefinedBy rdf:resource="http://cybox.mitre.org/objects/WindowsKernel"/>
        <rdfs:label>Selector</rdfs:label>
    </owl:DatatypeProperty>
    


    <!-- http://cybox.mitre.org/objects/WindowsKernel#serviceCounterTableBase -->

    <owl:DatatypeProperty rdf:about="http://cybox.mitre.org/objects/WindowsKernel#serviceCounterTableBase">
        <rdfs:domain rdf:resource="http://cybox.mitre.org/objects/WindowsKernel#SSDTEntry"/>
        <rdfs:range rdf:resource="http://www.w3.org/2001/XMLSchema#hexBinary"/>
        <rdfs:comment>Specifies a pointer to an array of usage counters.</rdfs:comment>
        <rdfs:isDefinedBy rdf:resource="http://cybox.mitre.org/objects/WindowsKernel"/>
        <rdfs:label>Service Counter Table Base</rdfs:label>
    </owl:DatatypeProperty>
    


    <!-- http://cybox.mitre.org/objects/WindowsKernel#serviceTableBase -->

    <owl:DatatypeProperty rdf:about="http://cybox.mitre.org/objects/WindowsKernel#serviceTableBase">
        <rdfs:domain rdf:resource="http://cybox.mitre.org/objects/WindowsKernel#SSDTEntry"/>
        <rdfs:range rdf:resource="http://www.w3.org/2001/XMLSchema#hexBinary"/>
        <rdfs:comment>Specifies a pointer to the system service dispatch table, an array of function addresses which is indexed by the system call number.</rdfs:comment>
        <rdfs:isDefinedBy rdf:resource="http://cybox.mitre.org/objects/WindowsKernel"/>
        <rdfs:label>Service Table Base</rdfs:label>
    </owl:DatatypeProperty>
    


    <!-- http://cybox.mitre.org/objects/WindowsKernel#typeAttr -->

    <owl:DatatypeProperty rdf:about="http://cybox.mitre.org/objects/WindowsKernel#typeAttr">
        <rdfs:domain rdf:resource="http://cybox.mitre.org/objects/WindowsKernel#IDTEntry"/>
        <rdfs:range rdf:resource="http://www.w3.org/2001/XMLSchema#hexBinary"/>
        <rdfs:comment>Specifies A byte that encodes the gate type and interrupt attributes (e.g., the Descriptor Privilege Level) of the Interrupt Descriptor Table.</rdfs:comment>
        <rdfs:isDefinedBy rdf:resource="http://cybox.mitre.org/objects/WindowsKernel"/>
        <rdfs:label>Type Attributes</rdfs:label>
    </owl:DatatypeProperty>
    


    <!-- 
    ///////////////////////////////////////////////////////////////////////////////////////
    //
    // Classes
    //
    ///////////////////////////////////////////////////////////////////////////////////////
     -->

    


    <!-- http://cybox.mitre.org/cybox_core#Object -->

    <owl:Class rdf:about="http://cybox.mitre.org/cybox_core#Object"/>
    


    <!-- http://cybox.mitre.org/objects/WindowsKernel#IDTEntry -->

    <owl:Class rdf:about="http://cybox.mitre.org/objects/WindowsKernel#IDTEntry">
        <rdfs:subClassOf>
            <owl:Restriction>
                <owl:onProperty rdf:resource="http://cybox.mitre.org/objects/WindowsKernel#offsetHigh"/>
                <owl:cardinality rdf:datatype="http://www.w3.org/2001/XMLSchema#nonNegativeInteger">1</owl:cardinality>
            </owl:Restriction>
        </rdfs:subClassOf>
        <rdfs:subClassOf>
            <owl:Restriction>
                <owl:onProperty rdf:resource="http://cybox.mitre.org/objects/WindowsKernel#offsetLow"/>
                <owl:cardinality rdf:datatype="http://www.w3.org/2001/XMLSchema#nonNegativeInteger">1</owl:cardinality>
            </owl:Restriction>
        </rdfs:subClassOf>
        <rdfs:subClassOf>
            <owl:Restriction>
                <owl:onProperty rdf:resource="http://cybox.mitre.org/objects/WindowsKernel#selector"/>
                <owl:cardinality rdf:datatype="http://www.w3.org/2001/XMLSchema#nonNegativeInteger">1</owl:cardinality>
            </owl:Restriction>
        </rdfs:subClassOf>
        <rdfs:subClassOf>
            <owl:Restriction>
                <owl:onProperty rdf:resource="http://cybox.mitre.org/objects/WindowsKernel#typeAttr"/>
                <owl:cardinality rdf:datatype="http://www.w3.org/2001/XMLSchema#nonNegativeInteger">1</owl:cardinality>
            </owl:Restriction>
        </rdfs:subClassOf>
        <rdfs:subClassOf>
            <owl:Restriction>
                <owl:onProperty rdf:resource="http://cybox.mitre.org/objects/WindowsKernel#offsetMiddle"/>
                <owl:maxCardinality rdf:datatype="http://www.w3.org/2001/XMLSchema#nonNegativeInteger">1</owl:maxCardinality>
            </owl:Restriction>
        </rdfs:subClassOf>
        <rdfs:comment>Characterizes a single entry in the Interrupt Descriptor Table (IDT). Entries can be interrupt gates, task gates, and trap gates.</rdfs:comment>
        <rdfs:isDefinedBy rdf:resource="http://cybox.mitre.org/objects/WindowsKernel"/>
        <rdfs:label>Interrupt Descriptor Table (IDT) Entry</rdfs:label>
    </owl:Class>
    


    <!-- http://cybox.mitre.org/objects/WindowsKernel#SSDTEntry -->

    <owl:Class rdf:about="http://cybox.mitre.org/objects/WindowsKernel#SSDTEntry">
        <rdfs:subClassOf>
            <owl:Restriction>
                <owl:onProperty rdf:resource="http://cybox.mitre.org/objects/WindowsKernel#argumentTableBase"/>
                <owl:cardinality rdf:datatype="http://www.w3.org/2001/XMLSchema#nonNegativeInteger">1</owl:cardinality>
            </owl:Restriction>
        </rdfs:subClassOf>
        <rdfs:subClassOf>
            <owl:Restriction>
                <owl:onProperty rdf:resource="http://cybox.mitre.org/objects/WindowsKernel#serviceCounterTableBase"/>
                <owl:cardinality rdf:datatype="http://www.w3.org/2001/XMLSchema#nonNegativeInteger">1</owl:cardinality>
            </owl:Restriction>
        </rdfs:subClassOf>
        <rdfs:subClassOf>
            <owl:Restriction>
                <owl:onProperty rdf:resource="http://cybox.mitre.org/objects/WindowsKernel#serviceTableBase"/>
                <owl:cardinality rdf:datatype="http://www.w3.org/2001/XMLSchema#nonNegativeInteger">1</owl:cardinality>
            </owl:Restriction>
        </rdfs:subClassOf>
        <rdfs:subClassOf>
            <owl:Restriction>
                <owl:onProperty rdf:resource="http://cybox.mitre.org/objects/WindowsKernel#hooked"/>
                <owl:maxCardinality rdf:datatype="http://www.w3.org/2001/XMLSchema#nonNegativeInteger">1</owl:maxCardinality>
            </owl:Restriction>
        </rdfs:subClassOf>
        <rdfs:subClassOf>
            <owl:Restriction>
                <owl:onProperty rdf:resource="http://cybox.mitre.org/objects/WindowsKernel#numberOfServices"/>
                <owl:maxCardinality rdf:datatype="http://www.w3.org/2001/XMLSchema#nonNegativeInteger">1</owl:maxCardinality>
            </owl:Restriction>
        </rdfs:subClassOf>
        <rdfs:comment>Characterizes a single entry in the System Service Descriptor Table (SSDT).</rdfs:comment>
        <rdfs:isDefinedBy rdf:resource="http://cybox.mitre.org/objects/WindowsKernel"/>
        <rdfs:label>System Service Ddescriptor Table (SSDT) Entry</rdfs:label>
    </owl:Class>
    


    <!-- http://cybox.mitre.org/objects/WindowsKernel#WindowsKernel -->

    <owl:Class rdf:about="http://cybox.mitre.org/objects/WindowsKernel#WindowsKernel">
        <rdfs:subClassOf rdf:resource="http://cybox.mitre.org/cybox_core#Object"/>
        <rdfs:comment>Characterize Windows Kernel structures.</rdfs:comment>
        <rdfs:label>Windows Kernel</rdfs:label>
    </owl:Class>
</rdf:RDF>



<!-- Generated by the OWL API (version 4.2.6.20160910-2108) https://github.com/owlcs/owlapi -->

