<?xml version="1.0"?>
<rdf:RDF xmlns="http://cybox.mitre.org/objects/WindowsRegistry#"
     xml:base="http://cybox.mitre.org/objects/WindowsRegistry"
     xmlns:rdf="http://www.w3.org/1999/02/22-rdf-syntax-ns#"
     xmlns:owl="http://www.w3.org/2002/07/owl#"
     xmlns:xml="http://www.w3.org/XML/1998/namespace"
     xmlns:xsd="http://www.w3.org/2001/XMLSchema#"
     xmlns:winRegistryObj="http://cybox.mitre.org/objects/WindowsRegistry#"
     xmlns:rdfs="http://www.w3.org/2000/01/rdf-schema#"
     xmlns:cyboxCommon="http://cybox.mitre.org/cyboxCommon#">
    <owl:Ontology rdf:about="http://cybox.mitre.org/objects/WindowsRegistry">
        <owl:imports rdf:resource="http://cybox.mitre.org/objects/Account"/>
        <owl:imports rdf:resource="http://cybox.mitre.org/cybox_core"/>
        <owl:imports rdf:resource="http://cybox.mitre.org/objects/WindowsHandle"/>
        <rdfs:label>Cyber Observable eXpression (CybOX) Windows Registry Ontology</rdfs:label>
        <owl:versionInfo rdf:datatype="http://www.w3.org/2001/XMLSchema#string">2.1.0-000</owl:versionInfo>
        <rdfs:comment>This ontology provides a vocabulary and representation of the Windows Registry Keys and Values for the  Cyber Observable eXpression (CybOX).  

CybOX  provides a common mechansim (structure and content) to convey the full range of potential cyber observable information and strives to be fully expressive, flexible, extensible, automatable, and as human-readable as possible.

The ontology is based on the CybOX Windows Registry Key object schema maintained by The MITRE Corporation copyright 2012-2014.  The version number of the ontology is kept in sync with the schema in order to more easily relate between the ontology and the corresponding schema version.

Copyright (c) 2014, DaedaFusion, LLC.  All rights reserved.</rdfs:comment>
    </owl:Ontology>
    


    <!-- 
    ///////////////////////////////////////////////////////////////////////////////////////
    //
    // Object Properties
    //
    ///////////////////////////////////////////////////////////////////////////////////////
     -->

    


    <!-- http://cybox.mitre.org/objects/WindowsRegistry#byteRuns -->

    <owl:ObjectProperty rdf:about="http://cybox.mitre.org/objects/WindowsRegistry#byteRuns">
        <rdfs:range rdf:resource="http://cybox.mitre.org/cyboxCommon#ByteRun"/>
        <rdfs:comment>Specifies a list of byte runs from the raw registry key entry.</rdfs:comment>
        <rdfs:isDefinedBy rdf:resource="http://cybox.mitre.org/objects/WindowsRegistry"/>
        <rdfs:label>Byte Runs</rdfs:label>
    </owl:ObjectProperty>
    


    <!-- http://cybox.mitre.org/objects/WindowsRegistry#creator -->

    <owl:ObjectProperty rdf:about="http://cybox.mitre.org/objects/WindowsRegistry#creator">
        <rdfs:range rdf:resource="http://cybox.mitre.org/objects/Account#WindowsUserAccount"/>
        <rdfs:comment>Specifies the user who created the registry object.</rdfs:comment>
        <rdfs:isDefinedBy rdf:resource="http://cybox.mitre.org/objects/WindowsRegistry"/>
        <rdfs:label>Creator</rdfs:label>
    </owl:ObjectProperty>
    


    <!-- http://cybox.mitre.org/objects/WindowsRegistry#handles -->

    <owl:ObjectProperty rdf:about="http://cybox.mitre.org/objects/WindowsRegistry#handles">
        <rdfs:range rdf:resource="http://cybox.mitre.org/objects/WindowsHandle#WindowsHandle"/>
        <rdfs:comment>Specifies a list of open Handles for this registry object.</rdfs:comment>
        <rdfs:isDefinedBy rdf:resource="http://cybox.mitre.org/objects/WindowsRegistry"/>
        <rdfs:label>Handles</rdfs:label>
    </owl:ObjectProperty>
    


    <!-- http://cybox.mitre.org/objects/WindowsRegistry#keys -->

    <owl:ObjectProperty rdf:about="http://cybox.mitre.org/objects/WindowsRegistry#keys">
        <rdfs:range rdf:resource="http://cybox.mitre.org/objects/WindowsRegistry#WindowsRegistryKey"/>
        <rdfs:comment>Specifies the keys contained under the registry hive</rdfs:comment>
        <rdfs:isDefinedBy rdf:resource="http://cybox.mitre.org/objects/WindowsRegistry"/>
        <rdfs:label>Keys</rdfs:label>
    </owl:ObjectProperty>
    


    <!-- http://cybox.mitre.org/objects/WindowsRegistry#subkeys -->

    <owl:ObjectProperty rdf:about="http://cybox.mitre.org/objects/WindowsRegistry#subkeys">
        <rdfs:range rdf:resource="http://cybox.mitre.org/objects/WindowsRegistry#WindowsRegistryKey"/>
        <rdfs:comment>Specifies the set of subkeys contained under the registry key.</rdfs:comment>
        <rdfs:isDefinedBy rdf:resource="http://cybox.mitre.org/objects/WindowsRegistry"/>
        <rdfs:label>Subkeys</rdfs:label>
    </owl:ObjectProperty>
    


    <!-- http://cybox.mitre.org/objects/WindowsRegistry#values -->

    <owl:ObjectProperty rdf:about="http://cybox.mitre.org/objects/WindowsRegistry#values">
        <rdfs:range rdf:resource="http://cybox.mitre.org/objects/WindowsRegistry#RegistryValue"/>
        <rdfs:comment>Specifies the values (with their name/data pairs) held within the registry key.</rdfs:comment>
        <rdfs:isDefinedBy rdf:resource="http://cybox.mitre.org/objects/WindowsRegistry"/>
        <rdfs:label>Values</rdfs:label>
    </owl:ObjectProperty>
    


    <!-- 
    ///////////////////////////////////////////////////////////////////////////////////////
    //
    // Data properties
    //
    ///////////////////////////////////////////////////////////////////////////////////////
     -->

    


    <!-- http://cybox.mitre.org/objects/WindowsRegistry#creatorUsername -->

    <owl:DatatypeProperty rdf:about="http://cybox.mitre.org/objects/WindowsRegistry#creatorUsername">
        <rdfs:range rdf:resource="http://www.w3.org/2001/XMLSchema#string"/>
        <rdfs:comment>Specifies the name of the user who created the registry object.</rdfs:comment>
        <rdfs:isDefinedBy rdf:resource="http://cybox.mitre.org/objects/WindowsRegistry"/>
        <rdfs:label>Creator Username</rdfs:label>
    </owl:DatatypeProperty>
    


    <!-- http://cybox.mitre.org/objects/WindowsRegistry#hiveName -->

    <owl:DatatypeProperty rdf:about="http://cybox.mitre.org/objects/WindowsRegistry#hiveName">
        <rdfs:range rdf:resource="http://www.w3.org/2001/XMLSchema#string"/>
        <rdfs:comment>Specifies the Windows registry hive to which the registry object belongs to.</rdfs:comment>
        <rdfs:isDefinedBy rdf:resource="http://cybox.mitre.org/objects/WindowsRegistry"/>
        <rdfs:label>Hive</rdfs:label>
    </owl:DatatypeProperty>
    


    <!-- http://cybox.mitre.org/objects/WindowsRegistry#key -->

    <owl:DatatypeProperty rdf:about="http://cybox.mitre.org/objects/WindowsRegistry#key">
        <rdfs:range rdf:resource="http://www.w3.org/2001/XMLSchema#string"/>
        <rdfs:comment>Specifies the full key to the Windows registry object, not including the hive.</rdfs:comment>
        <rdfs:isDefinedBy rdf:resource="http://cybox.mitre.org/objects/WindowsRegistry"/>
        <rdfs:label>Key</rdfs:label>
    </owl:DatatypeProperty>
    


    <!-- http://cybox.mitre.org/objects/WindowsRegistry#modifiedDateTime -->

    <owl:DatatypeProperty rdf:about="http://cybox.mitre.org/objects/WindowsRegistry#modifiedDateTime">
        <rdfs:range rdf:resource="http://www.w3.org/2001/XMLSchema#dateTime"/>
        <rdfs:comment>Specifies the last date/time that the registry object was modified.</rdfs:comment>
        <rdfs:isDefinedBy rdf:resource="http://cybox.mitre.org/objects/WindowsRegistry"/>
        <rdfs:label>Modified Time</rdfs:label>
    </owl:DatatypeProperty>
    


    <!-- http://cybox.mitre.org/objects/WindowsRegistry#numberOfSubkeys -->

    <owl:DatatypeProperty rdf:about="http://cybox.mitre.org/objects/WindowsRegistry#numberOfSubkeys">
        <rdfs:range rdf:resource="http://www.w3.org/2001/XMLSchema#unsignedInt"/>
        <rdfs:comment>Specifies the number of subkeys contained under the registry key.</rdfs:comment>
        <rdfs:isDefinedBy rdf:resource="http://cybox.mitre.org/objects/WindowsRegistry"/>
        <rdfs:label>Number of Subkeys</rdfs:label>
    </owl:DatatypeProperty>
    


    <!-- http://cybox.mitre.org/objects/WindowsRegistry#numberOfValues -->

    <owl:DatatypeProperty rdf:about="http://cybox.mitre.org/objects/WindowsRegistry#numberOfValues">
        <rdfs:range rdf:resource="http://www.w3.org/2001/XMLSchema#unsignedInt"/>
        <rdfs:comment>Specifies the number of values found in the registry key.</rdfs:comment>
        <rdfs:isDefinedBy rdf:resource="http://cybox.mitre.org/objects/WindowsRegistry"/>
        <rdfs:label>Number of Values</rdfs:label>
    </owl:DatatypeProperty>
    


    <!-- http://cybox.mitre.org/objects/WindowsRegistry#valueData -->

    <owl:DatatypeProperty rdf:about="http://cybox.mitre.org/objects/WindowsRegistry#valueData">
        <rdfs:range rdf:resource="http://www.w3.org/2001/XMLSchema#string"/>
        <rdfs:comment>Specifies the data contained in the registry value.</rdfs:comment>
        <rdfs:isDefinedBy rdf:resource="http://cybox.mitre.org/objects/WindowsRegistry"/>
        <rdfs:label>Value Data</rdfs:label>
    </owl:DatatypeProperty>
    


    <!-- http://cybox.mitre.org/objects/WindowsRegistry#valueDatatype -->

    <owl:DatatypeProperty rdf:about="http://cybox.mitre.org/objects/WindowsRegistry#valueDatatype">
        <rdfs:range rdf:resource="http://www.w3.org/2001/XMLSchema#string"/>
        <rdfs:comment>Specifies the registry (REG_*) datatype used in the registry value.</rdfs:comment>
        <rdfs:isDefinedBy rdf:resource="http://cybox.mitre.org/objects/WindowsRegistry"/>
        <rdfs:label>Value Datatype</rdfs:label>
    </owl:DatatypeProperty>
    


    <!-- http://cybox.mitre.org/objects/WindowsRegistry#valueName -->

    <owl:DatatypeProperty rdf:about="http://cybox.mitre.org/objects/WindowsRegistry#valueName">
        <rdfs:range rdf:resource="http://www.w3.org/2001/XMLSchema#string"/>
        <rdfs:comment>Specifies the name of the registry value.

For specifying the default value in a registry key, an empty string should be used.</rdfs:comment>
        <rdfs:isDefinedBy rdf:resource="http://cybox.mitre.org/objects/WindowsRegistry"/>
        <rdfs:label>Value Name</rdfs:label>
    </owl:DatatypeProperty>
    


    <!-- 
    ///////////////////////////////////////////////////////////////////////////////////////
    //
    // Classes
    //
    ///////////////////////////////////////////////////////////////////////////////////////
     -->

    


    <!-- http://cybox.mitre.org/cyboxCommon#ByteRun -->

    <owl:Class rdf:about="http://cybox.mitre.org/cyboxCommon#ByteRun"/>
    


    <!-- http://cybox.mitre.org/cybox_core#Object -->

    <owl:Class rdf:about="http://cybox.mitre.org/cybox_core#Object"/>
    


    <!-- http://cybox.mitre.org/objects/Account#WindowsUserAccount -->

    <owl:Class rdf:about="http://cybox.mitre.org/objects/Account#WindowsUserAccount"/>
    


    <!-- http://cybox.mitre.org/objects/WindowsHandle#WindowsHandle -->

    <owl:Class rdf:about="http://cybox.mitre.org/objects/WindowsHandle#WindowsHandle"/>
    


    <!-- http://cybox.mitre.org/objects/WindowsRegistry#RegistryHive -->

    <owl:Class rdf:about="http://cybox.mitre.org/objects/WindowsRegistry#RegistryHive">
        <rdfs:subClassOf>
            <owl:Restriction>
                <owl:onProperty rdf:resource="http://cybox.mitre.org/objects/WindowsRegistry#hiveName"/>
                <owl:cardinality rdf:datatype="http://www.w3.org/2001/XMLSchema#nonNegativeInteger">1</owl:cardinality>
            </owl:Restriction>
        </rdfs:subClassOf>
        <rdfs:comment>Characterizes a Windows registry hive.</rdfs:comment>
        <rdfs:isDefinedBy rdf:resource="http://cybox.mitre.org/objects/WindowsRegistry"/>
        <rdfs:label>Registry Hive</rdfs:label>
    </owl:Class>
    


    <!-- http://cybox.mitre.org/objects/WindowsRegistry#RegistryValue -->

    <owl:Class rdf:about="http://cybox.mitre.org/objects/WindowsRegistry#RegistryValue">
        <rdfs:subClassOf>
            <owl:Restriction>
                <owl:onProperty rdf:resource="http://cybox.mitre.org/objects/WindowsRegistry#valueData"/>
                <owl:cardinality rdf:datatype="http://www.w3.org/2001/XMLSchema#nonNegativeInteger">1</owl:cardinality>
            </owl:Restriction>
        </rdfs:subClassOf>
        <rdfs:subClassOf>
            <owl:Restriction>
                <owl:onProperty rdf:resource="http://cybox.mitre.org/objects/WindowsRegistry#valueName"/>
                <owl:cardinality rdf:datatype="http://www.w3.org/2001/XMLSchema#nonNegativeInteger">1</owl:cardinality>
            </owl:Restriction>
        </rdfs:subClassOf>
        <rdfs:subClassOf>
            <owl:Restriction>
                <owl:onProperty rdf:resource="http://cybox.mitre.org/objects/WindowsRegistry#valueDatatype"/>
                <owl:maxCardinality rdf:datatype="http://www.w3.org/2001/XMLSchema#nonNegativeInteger">1</owl:maxCardinality>
            </owl:Restriction>
        </rdfs:subClassOf>
        <rdfs:comment>Characterizes  the values (with their name/data pairs) held within a registry key.</rdfs:comment>
        <rdfs:isDefinedBy rdf:resource="http://cybox.mitre.org/objects/WindowsRegistry"/>
        <rdfs:label>Registry Value</rdfs:label>
    </owl:Class>
    


    <!-- http://cybox.mitre.org/objects/WindowsRegistry#WindowsRegistryKey -->

    <owl:Class rdf:about="http://cybox.mitre.org/objects/WindowsRegistry#WindowsRegistryKey">
        <rdfs:subClassOf rdf:resource="http://cybox.mitre.org/cybox_core#Object"/>
        <rdfs:subClassOf>
            <owl:Restriction>
                <owl:onProperty rdf:resource="http://cybox.mitre.org/objects/WindowsRegistry#creator"/>
                <owl:maxCardinality rdf:datatype="http://www.w3.org/2001/XMLSchema#nonNegativeInteger">1</owl:maxCardinality>
            </owl:Restriction>
        </rdfs:subClassOf>
        <rdfs:subClassOf>
            <owl:Restriction>
                <owl:onProperty rdf:resource="http://cybox.mitre.org/objects/WindowsRegistry#hiveName"/>
                <owl:cardinality rdf:datatype="http://www.w3.org/2001/XMLSchema#nonNegativeInteger">1</owl:cardinality>
            </owl:Restriction>
        </rdfs:subClassOf>
        <rdfs:subClassOf>
            <owl:Restriction>
                <owl:onProperty rdf:resource="http://cybox.mitre.org/objects/WindowsRegistry#key"/>
                <owl:cardinality rdf:datatype="http://www.w3.org/2001/XMLSchema#nonNegativeInteger">1</owl:cardinality>
            </owl:Restriction>
        </rdfs:subClassOf>
        <rdfs:subClassOf>
            <owl:Restriction>
                <owl:onProperty rdf:resource="http://cybox.mitre.org/objects/WindowsRegistry#creatorUsername"/>
                <owl:maxCardinality rdf:datatype="http://www.w3.org/2001/XMLSchema#nonNegativeInteger">1</owl:maxCardinality>
            </owl:Restriction>
        </rdfs:subClassOf>
        <rdfs:subClassOf>
            <owl:Restriction>
                <owl:onProperty rdf:resource="http://cybox.mitre.org/objects/WindowsRegistry#modifiedDateTime"/>
                <owl:maxCardinality rdf:datatype="http://www.w3.org/2001/XMLSchema#nonNegativeInteger">1</owl:maxCardinality>
            </owl:Restriction>
        </rdfs:subClassOf>
        <rdfs:subClassOf>
            <owl:Restriction>
                <owl:onProperty rdf:resource="http://cybox.mitre.org/objects/WindowsRegistry#numberOfSubkeys"/>
                <owl:maxCardinality rdf:datatype="http://www.w3.org/2001/XMLSchema#nonNegativeInteger">1</owl:maxCardinality>
            </owl:Restriction>
        </rdfs:subClassOf>
        <rdfs:subClassOf>
            <owl:Restriction>
                <owl:onProperty rdf:resource="http://cybox.mitre.org/objects/WindowsRegistry#numberOfValues"/>
                <owl:maxCardinality rdf:datatype="http://www.w3.org/2001/XMLSchema#nonNegativeInteger">1</owl:maxCardinality>
            </owl:Restriction>
        </rdfs:subClassOf>
        <rdfs:comment>Characterize Windows Registry Keys.</rdfs:comment>
        <rdfs:label>Windows Registry Key</rdfs:label>
    </owl:Class>
</rdf:RDF>



<!-- Generated by the OWL API (version 4.2.6.20160910-2108) https://github.com/owlcs/owlapi -->

