<?xml version="1.0"?>
<rdf:RDF xmlns="http://cybox.mitre.org/objects/X509Certificate#"
     xml:base="http://cybox.mitre.org/objects/X509Certificate"
     xmlns:rdf="http://www.w3.org/1999/02/22-rdf-syntax-ns#"
     xmlns:owl="http://www.w3.org/2002/07/owl#"
     xmlns:xml="http://www.w3.org/XML/1998/namespace"
     xmlns:xsd="http://www.w3.org/2001/XMLSchema#"
     xmlns:x509CertObj="http://cybox.mitre.org/objects/X509Certificate#"
     xmlns:rdfs="http://www.w3.org/2000/01/rdf-schema#">
    <owl:Ontology rdf:about="http://cybox.mitre.org/objects/X509Certificate">
        <owl:imports rdf:resource="http://cybox.mitre.org/cybox_core"/>
        <owl:versionInfo rdf:datatype="http://www.w3.org/2001/XMLSchema#string">2.1.0-000</owl:versionInfo>
        <rdfs:comment>This ontology provides a vocabulary and representation of an X509 Certificate for the  Cyber Observable eXpression (CybOX).  

CybOX  provides a common mechansim (structure and content) to convey the full range of potential cyber observable information and strives to be fully expressive, flexible, extensible, automatable, and as human-readable as possible.

The ontology is based on the CybOX X509 Certificate object schema maintained by The MITRE Corporation copyright 2012-2014.  The version number of the ontology is kept in sync with the schema in order to more easily relate between the ontology and the corresponding schema version.

Copyright (c) 2014, DaedaFusion, LLC.  All rights reserved.</rdfs:comment>
        <rdfs:label>Cyber Observable eXpression (CybOX) X509 Certificate Ontology</rdfs:label>
    </owl:Ontology>
    


    <!-- 
    ///////////////////////////////////////////////////////////////////////////////////////
    //
    // Object Properties
    //
    ///////////////////////////////////////////////////////////////////////////////////////
     -->

    


    <!-- http://cybox.mitre.org/objects/X509Certificate#nonStandardExtensions -->

    <owl:ObjectProperty rdf:about="http://cybox.mitre.org/objects/X509Certificate#nonStandardExtensions">
        <rdfs:range rdf:resource="http://cybox.mitre.org/objects/X509Certificate#X509Extension"/>
        <rdfs:comment>Specifies the non-standard X509 extensions that may be specified in the certificate.</rdfs:comment>
        <rdfs:isDefinedBy rdf:resource="http://cybox.mitre.org/objects/X509Certificate"/>
        <rdfs:label>Non-standard Extensions</rdfs:label>
    </owl:ObjectProperty>
    


    <!-- http://cybox.mitre.org/objects/X509Certificate#standardExtensions -->

    <owl:ObjectProperty rdf:about="http://cybox.mitre.org/objects/X509Certificate#standardExtensions">
        <rdfs:range rdf:resource="http://cybox.mitre.org/objects/X509Certificate#X509Extension"/>
        <rdfs:comment>Specifies the  standard X509 V3 extensions that may be specified in the certificate.</rdfs:comment>
        <rdfs:isDefinedBy rdf:resource="http://cybox.mitre.org/objects/X509Certificate"/>
        <rdfs:label>Standard Extensions</rdfs:label>
    </owl:ObjectProperty>
    


    <!-- 
    ///////////////////////////////////////////////////////////////////////////////////////
    //
    // Data properties
    //
    ///////////////////////////////////////////////////////////////////////////////////////
     -->

    


    <!-- http://cybox.mitre.org/objects/X509Certificate#certificateSignature.algorithm -->

    <owl:DatatypeProperty rdf:about="http://cybox.mitre.org/objects/X509Certificate#certificateSignature.algorithm">
        <rdfs:range rdf:resource="http://www.w3.org/2001/XMLSchema#string"/>
        <rdfs:comment>Specifies the algorithm identifier for the algorithm used by the Certificate Authority to compute the signature.</rdfs:comment>
        <rdfs:isDefinedBy rdf:resource="http://cybox.mitre.org/objects/X509Certificate"/>
        <rdfs:label>Certificate Signature Algorithm</rdfs:label>
    </owl:DatatypeProperty>
    


    <!-- http://cybox.mitre.org/objects/X509Certificate#certificateSignature.value -->

    <owl:DatatypeProperty rdf:about="http://cybox.mitre.org/objects/X509Certificate#certificateSignature.value">
        <rdfs:range rdf:resource="http://www.w3.org/2001/XMLSchema#string"/>
        <rdfs:comment>Specifies a digital signature computed upon this X.509 certificate using the specified certificate signature algorithm.</rdfs:comment>
        <rdfs:isDefinedBy rdf:resource="http://cybox.mitre.org/objects/X509Certificate"/>
        <rdfs:label>Certificate Signature Value</rdfs:label>
    </owl:DatatypeProperty>
    


    <!-- http://cybox.mitre.org/objects/X509Certificate#extensionName -->

    <owl:DatatypeProperty rdf:about="http://cybox.mitre.org/objects/X509Certificate#extensionName">
        <rdfs:range rdf:resource="http://www.w3.org/2001/XMLSchema#string"/>
        <rdfs:comment>Specifies the human-friendly name of the X509 Extension</rdfs:comment>
        <rdfs:isDefinedBy rdf:resource="http://cybox.mitre.org/objects/X509Certificate"/>
        <rdfs:label>Extension Name</rdfs:label>
    </owl:DatatypeProperty>
    


    <!-- http://cybox.mitre.org/objects/X509Certificate#identifier -->

    <owl:DatatypeProperty rdf:about="http://cybox.mitre.org/objects/X509Certificate#identifier">
        <rdfs:range rdf:resource="http://www.w3.org/2001/XMLSchema#string"/>
        <rdfs:comment>Specifies the IANA Object Identifier for the extension</rdfs:comment>
        <rdfs:isDefinedBy rdf:resource="http://cybox.mitre.org/objects/X509Certificate"/>
        <rdfs:label>Identifier</rdfs:label>
    </owl:DatatypeProperty>
    


    <!-- http://cybox.mitre.org/objects/X509Certificate#isCritical -->

    <owl:DatatypeProperty rdf:about="http://cybox.mitre.org/objects/X509Certificate#isCritical">
        <rdfs:range rdf:resource="http://www.w3.org/2001/XMLSchema#boolean"/>
        <rdfs:comment>Specifies whether the extension is considered critical</rdfs:comment>
        <rdfs:isDefinedBy rdf:resource="http://cybox.mitre.org/objects/X509Certificate"/>
        <rdfs:label>is critical</rdfs:label>
    </owl:DatatypeProperty>
    


    <!-- http://cybox.mitre.org/objects/X509Certificate#isDeprecated -->

    <owl:DatatypeProperty rdf:about="http://cybox.mitre.org/objects/X509Certificate#isDeprecated">
        <rdfs:range rdf:resource="http://www.w3.org/2001/XMLSchema#boolean"/>
        <rdfs:comment>Specifies that use of the extension has been deprecated.</rdfs:comment>
        <rdfs:isDefinedBy rdf:resource="http://cybox.mitre.org/objects/X509Certificate"/>
        <rdfs:label>is deprecated</rdfs:label>
    </owl:DatatypeProperty>
    


    <!-- http://cybox.mitre.org/objects/X509Certificate#issuer -->

    <owl:DatatypeProperty rdf:about="http://cybox.mitre.org/objects/X509Certificate#issuer">
        <rdfs:range rdf:resource="http://www.w3.org/2001/XMLSchema#string"/>
        <rdfs:comment>Specifies the  issuer is the Certificate Authority who issued the X.509 certificate.</rdfs:comment>
        <rdfs:isDefinedBy rdf:resource="http://cybox.mitre.org/objects/X509Certificate"/>
        <rdfs:label>Issuer</rdfs:label>
    </owl:DatatypeProperty>
    


    <!-- http://cybox.mitre.org/objects/X509Certificate#notAfterDateTime -->

    <owl:DatatypeProperty rdf:about="http://cybox.mitre.org/objects/X509Certificate#notAfterDateTime">
        <rdfs:range rdf:resource="http://www.w3.org/2001/XMLSchema#dateTime"/>
        <rdfs:comment>Specifies the date and time after which the extension should  not be honored when specifying a period of validity.</rdfs:comment>
        <rdfs:isDefinedBy rdf:resource="http://cybox.mitre.org/objects/X509Certificate"/>
        <rdfs:label>Not After</rdfs:label>
    </owl:DatatypeProperty>
    


    <!-- http://cybox.mitre.org/objects/X509Certificate#notBeforeDateTime -->

    <owl:DatatypeProperty rdf:about="http://cybox.mitre.org/objects/X509Certificate#notBeforeDateTime">
        <rdfs:range rdf:resource="http://www.w3.org/2001/XMLSchema#dateTime"/>
        <rdfs:comment>Specifies the date and time as which the extension should be honored when specifying a period of validity.</rdfs:comment>
        <rdfs:isDefinedBy rdf:resource="http://cybox.mitre.org/objects/X509Certificate"/>
        <rdfs:label>Not Before</rdfs:label>
    </owl:DatatypeProperty>
    


    <!-- http://cybox.mitre.org/objects/X509Certificate#rawCertificate -->

    <owl:DatatypeProperty rdf:about="http://cybox.mitre.org/objects/X509Certificate#rawCertificate">
        <rdfs:range rdf:resource="http://www.w3.org/2001/XMLSchema#string"/>
        <rdfs:comment>Specifies the raw content of an X.509 certificate as Based64 encoded DER certificate including the -----BEGIN CERTIFICATE----- and -----END CERTIFICATE----- lines.</rdfs:comment>
        <rdfs:isDefinedBy rdf:resource="http://cybox.mitre.org/objects/X509Certificate"/>
        <rdfs:label>Raw Certificate</rdfs:label>
    </owl:DatatypeProperty>
    


    <!-- http://cybox.mitre.org/objects/X509Certificate#serialNumber -->

    <owl:DatatypeProperty rdf:about="http://cybox.mitre.org/objects/X509Certificate#serialNumber">
        <rdfs:range rdf:resource="http://www.w3.org/2001/XMLSchema#string"/>
        <rdfs:comment>Specifies a unique identifier for each X.509 certificate issued by a specific Certificate Authority.</rdfs:comment>
        <rdfs:isDefinedBy rdf:resource="http://cybox.mitre.org/objects/X509Certificate"/>
        <rdfs:label>Serial Number</rdfs:label>
    </owl:DatatypeProperty>
    


    <!-- http://cybox.mitre.org/objects/X509Certificate#signatureAlgorithm -->

    <owl:DatatypeProperty rdf:about="http://cybox.mitre.org/objects/X509Certificate#signatureAlgorithm">
        <rdfs:range rdf:resource="http://www.w3.org/2001/XMLSchema#string"/>
        <rdfs:comment>Specifies the algorithm used to sign the X.509 certificate.</rdfs:comment>
        <rdfs:isDefinedBy rdf:resource="http://cybox.mitre.org/objects/X509Certificate"/>
        <rdfs:label>Signature Algorithm</rdfs:label>
    </owl:DatatypeProperty>
    


    <!-- http://cybox.mitre.org/objects/X509Certificate#subject -->

    <owl:DatatypeProperty rdf:about="http://cybox.mitre.org/objects/X509Certificate#subject">
        <rdfs:range rdf:resource="http://www.w3.org/2001/XMLSchema#string"/>
        <rdfs:comment>Specifies the entity associated with the public key stored in the subject public key field of the X.509 certificate.</rdfs:comment>
        <rdfs:isDefinedBy rdf:resource="http://cybox.mitre.org/objects/X509Certificate"/>
        <rdfs:label>Subject</rdfs:label>
    </owl:DatatypeProperty>
    


    <!-- http://cybox.mitre.org/objects/X509Certificate#subjectPublicKey.algorithm -->

    <owl:DatatypeProperty rdf:about="http://cybox.mitre.org/objects/X509Certificate#subjectPublicKey.algorithm">
        <rdfs:range rdf:resource="http://www.w3.org/2001/XMLSchema#string"/>
        <rdfs:comment>Specifies the algorithm with which to encrypt data being sent to the subject.</rdfs:comment>
        <rdfs:isDefinedBy rdf:resource="http://cybox.mitre.org/objects/X509Certificate"/>
        <rdfs:label>Subject Public Key Algorithm</rdfs:label>
    </owl:DatatypeProperty>
    


    <!-- http://cybox.mitre.org/objects/X509Certificate#subjectPublicKey.rsaPublicKeyExponent -->

    <owl:DatatypeProperty rdf:about="http://cybox.mitre.org/objects/X509Certificate#subjectPublicKey.rsaPublicKeyExponent">
        <rdfs:range rdf:resource="http://www.w3.org/2001/XMLSchema#string"/>
        <rdfs:comment>Specifies the exponent portion of a public key.</rdfs:comment>
        <rdfs:isDefinedBy rdf:resource="http://cybox.mitre.org/objects/X509Certificate"/>
        <rdfs:label>Subject Public Key RSA Key Exponent</rdfs:label>
    </owl:DatatypeProperty>
    


    <!-- http://cybox.mitre.org/objects/X509Certificate#subjectPublicKey.rsaPublicKeyModulus -->

    <owl:DatatypeProperty rdf:about="http://cybox.mitre.org/objects/X509Certificate#subjectPublicKey.rsaPublicKeyModulus">
        <rdfs:range rdf:resource="http://www.w3.org/2001/XMLSchema#string"/>
        <rdfs:comment>Specifies the modulus portion of a public key.</rdfs:comment>
        <rdfs:isDefinedBy rdf:resource="http://cybox.mitre.org/objects/X509Certificate"/>
        <rdfs:label>Subject Public Key RSA Key Modulus</rdfs:label>
    </owl:DatatypeProperty>
    


    <!-- http://cybox.mitre.org/objects/X509Certificate#validity.notAfterDateTime -->

    <owl:DatatypeProperty rdf:about="http://cybox.mitre.org/objects/X509Certificate#validity.notAfterDateTime">
        <rdfs:range rdf:resource="http://www.w3.org/2001/XMLSchema#dateTime"/>
        <rdfs:comment>Specifies  the date on which the certificate validity period ends.</rdfs:comment>
        <rdfs:isDefinedBy rdf:resource="http://cybox.mitre.org/objects/X509Certificate"/>
        <rdfs:label>Not Valid After</rdfs:label>
    </owl:DatatypeProperty>
    


    <!-- http://cybox.mitre.org/objects/X509Certificate#validity.notBeforeDateTime -->

    <owl:DatatypeProperty rdf:about="http://cybox.mitre.org/objects/X509Certificate#validity.notBeforeDateTime">
        <rdfs:range rdf:resource="http://www.w3.org/2001/XMLSchema#dateTime"/>
        <rdfs:comment>Specifies the date on which the certificate validity period begins.</rdfs:comment>
        <rdfs:isDefinedBy rdf:resource="http://cybox.mitre.org/objects/X509Certificate"/>
        <rdfs:label>Not Valid Before</rdfs:label>
    </owl:DatatypeProperty>
    


    <!-- http://cybox.mitre.org/objects/X509Certificate#value -->

    <owl:DatatypeProperty rdf:about="http://cybox.mitre.org/objects/X509Certificate#value">
        <rdfs:range rdf:resource="http://www.w3.org/2001/XMLSchema#string"/>
        <rdfs:comment>Specifies the raw value of the extension</rdfs:comment>
        <rdfs:isDefinedBy rdf:resource="http://cybox.mitre.org/objects/X509Certificate"/>
        <rdfs:label>Raw Value</rdfs:label>
    </owl:DatatypeProperty>
    


    <!-- http://cybox.mitre.org/objects/X509Certificate#version -->

    <owl:DatatypeProperty rdf:about="http://cybox.mitre.org/objects/X509Certificate#version">
        <rdfs:range rdf:resource="http://www.w3.org/2001/XMLSchema#integer"/>
        <rdfs:comment>Specifies the version of the encoded certificate.</rdfs:comment>
        <rdfs:isDefinedBy rdf:resource="http://cybox.mitre.org/objects/X509Certificate"/>
        <rdfs:label>Version</rdfs:label>
    </owl:DatatypeProperty>
    


    <!-- 
    ///////////////////////////////////////////////////////////////////////////////////////
    //
    // Classes
    //
    ///////////////////////////////////////////////////////////////////////////////////////
     -->

    


    <!-- http://cybox.mitre.org/objects/X509Certificate#X509Certificate -->

    <owl:Class rdf:about="http://cybox.mitre.org/objects/X509Certificate#X509Certificate">
        <rdfs:subClassOf rdf:resource="http://cybox.mitre.org/cybox_core#Object"/>
        <rdfs:subClassOf>
            <owl:Restriction>
                <owl:onProperty rdf:resource="http://cybox.mitre.org/objects/X509Certificate#nonStandardExtensions"/>
                <owl:someValuesFrom rdf:resource="http://www.w3.org/2002/07/owl#Thing"/>
            </owl:Restriction>
        </rdfs:subClassOf>
        <rdfs:subClassOf>
            <owl:Restriction>
                <owl:onProperty rdf:resource="http://cybox.mitre.org/objects/X509Certificate#standardExtensions"/>
                <owl:someValuesFrom rdf:resource="http://www.w3.org/2002/07/owl#Thing"/>
            </owl:Restriction>
        </rdfs:subClassOf>
        <rdfs:subClassOf>
            <owl:Restriction>
                <owl:onProperty rdf:resource="http://cybox.mitre.org/objects/X509Certificate#certificateSignature.algorithm"/>
                <owl:someValuesFrom rdf:resource="http://www.w3.org/2000/01/rdf-schema#Literal"/>
            </owl:Restriction>
        </rdfs:subClassOf>
        <rdfs:subClassOf>
            <owl:Restriction>
                <owl:onProperty rdf:resource="http://cybox.mitre.org/objects/X509Certificate#certificateSignature.value"/>
                <owl:someValuesFrom rdf:resource="http://www.w3.org/2000/01/rdf-schema#Literal"/>
            </owl:Restriction>
        </rdfs:subClassOf>
        <rdfs:subClassOf>
            <owl:Restriction>
                <owl:onProperty rdf:resource="http://cybox.mitre.org/objects/X509Certificate#issuer"/>
                <owl:someValuesFrom rdf:resource="http://www.w3.org/2000/01/rdf-schema#Literal"/>
            </owl:Restriction>
        </rdfs:subClassOf>
        <rdfs:subClassOf>
            <owl:Restriction>
                <owl:onProperty rdf:resource="http://cybox.mitre.org/objects/X509Certificate#rawCertificate"/>
                <owl:someValuesFrom rdf:resource="http://www.w3.org/2000/01/rdf-schema#Literal"/>
            </owl:Restriction>
        </rdfs:subClassOf>
        <rdfs:subClassOf>
            <owl:Restriction>
                <owl:onProperty rdf:resource="http://cybox.mitre.org/objects/X509Certificate#serialNumber"/>
                <owl:someValuesFrom rdf:resource="http://www.w3.org/2000/01/rdf-schema#Literal"/>
            </owl:Restriction>
        </rdfs:subClassOf>
        <rdfs:subClassOf>
            <owl:Restriction>
                <owl:onProperty rdf:resource="http://cybox.mitre.org/objects/X509Certificate#subject"/>
                <owl:someValuesFrom rdf:resource="http://www.w3.org/2000/01/rdf-schema#Literal"/>
            </owl:Restriction>
        </rdfs:subClassOf>
        <rdfs:subClassOf>
            <owl:Restriction>
                <owl:onProperty rdf:resource="http://cybox.mitre.org/objects/X509Certificate#subjectPublicKey.algorithm"/>
                <owl:someValuesFrom rdf:resource="http://www.w3.org/2000/01/rdf-schema#Literal"/>
            </owl:Restriction>
        </rdfs:subClassOf>
        <rdfs:subClassOf>
            <owl:Restriction>
                <owl:onProperty rdf:resource="http://cybox.mitre.org/objects/X509Certificate#subjectPublicKey.rsaPublicKeyExponent"/>
                <owl:someValuesFrom rdf:resource="http://www.w3.org/2000/01/rdf-schema#Literal"/>
            </owl:Restriction>
        </rdfs:subClassOf>
        <rdfs:subClassOf>
            <owl:Restriction>
                <owl:onProperty rdf:resource="http://cybox.mitre.org/objects/X509Certificate#subjectPublicKey.rsaPublicKeyModulus"/>
                <owl:someValuesFrom rdf:resource="http://www.w3.org/2000/01/rdf-schema#Literal"/>
            </owl:Restriction>
        </rdfs:subClassOf>
        <rdfs:subClassOf>
            <owl:Restriction>
                <owl:onProperty rdf:resource="http://cybox.mitre.org/objects/X509Certificate#validity.notAfterDateTime"/>
                <owl:someValuesFrom rdf:resource="http://www.w3.org/2000/01/rdf-schema#Literal"/>
            </owl:Restriction>
        </rdfs:subClassOf>
        <rdfs:subClassOf>
            <owl:Restriction>
                <owl:onProperty rdf:resource="http://cybox.mitre.org/objects/X509Certificate#validity.notBeforeDateTime"/>
                <owl:someValuesFrom rdf:resource="http://www.w3.org/2000/01/rdf-schema#Literal"/>
            </owl:Restriction>
        </rdfs:subClassOf>
        <rdfs:subClassOf>
            <owl:Restriction>
                <owl:onProperty rdf:resource="http://cybox.mitre.org/objects/X509Certificate#version"/>
                <owl:someValuesFrom rdf:resource="http://www.w3.org/2000/01/rdf-schema#Literal"/>
            </owl:Restriction>
        </rdfs:subClassOf>
        <rdfs:comment>Characterize X.509 certificates.</rdfs:comment>
        <rdfs:isDefinedBy rdf:resource="http://cybox.mitre.org/objects/X509Certificate"/>
    </owl:Class>
    


    <!-- http://cybox.mitre.org/objects/X509Certificate#X509Extension -->

    <owl:Class rdf:about="http://cybox.mitre.org/objects/X509Certificate#X509Extension">
        <rdfs:subClassOf>
            <owl:Restriction>
                <owl:onProperty rdf:resource="http://cybox.mitre.org/objects/X509Certificate#extensionName"/>
                <owl:someValuesFrom rdf:resource="http://www.w3.org/2000/01/rdf-schema#Literal"/>
            </owl:Restriction>
        </rdfs:subClassOf>
        <rdfs:subClassOf>
            <owl:Restriction>
                <owl:onProperty rdf:resource="http://cybox.mitre.org/objects/X509Certificate#identifier"/>
                <owl:someValuesFrom rdf:resource="http://www.w3.org/2000/01/rdf-schema#Literal"/>
            </owl:Restriction>
        </rdfs:subClassOf>
        <rdfs:subClassOf>
            <owl:Restriction>
                <owl:onProperty rdf:resource="http://cybox.mitre.org/objects/X509Certificate#isCritical"/>
                <owl:someValuesFrom rdf:resource="http://www.w3.org/2000/01/rdf-schema#Literal"/>
            </owl:Restriction>
        </rdfs:subClassOf>
        <rdfs:subClassOf>
            <owl:Restriction>
                <owl:onProperty rdf:resource="http://cybox.mitre.org/objects/X509Certificate#isDeprecated"/>
                <owl:someValuesFrom rdf:resource="http://www.w3.org/2000/01/rdf-schema#Literal"/>
            </owl:Restriction>
        </rdfs:subClassOf>
        <rdfs:subClassOf>
            <owl:Restriction>
                <owl:onProperty rdf:resource="http://cybox.mitre.org/objects/X509Certificate#notAfterDateTime"/>
                <owl:someValuesFrom rdf:resource="http://www.w3.org/2000/01/rdf-schema#Literal"/>
            </owl:Restriction>
        </rdfs:subClassOf>
        <rdfs:subClassOf>
            <owl:Restriction>
                <owl:onProperty rdf:resource="http://cybox.mitre.org/objects/X509Certificate#notBeforeDateTime"/>
                <owl:someValuesFrom rdf:resource="http://www.w3.org/2000/01/rdf-schema#Literal"/>
            </owl:Restriction>
        </rdfs:subClassOf>
        <rdfs:subClassOf>
            <owl:Restriction>
                <owl:onProperty rdf:resource="http://cybox.mitre.org/objects/X509Certificate#value"/>
                <owl:someValuesFrom rdf:resource="http://www.w3.org/2000/01/rdf-schema#Literal"/>
            </owl:Restriction>
        </rdfs:subClassOf>
        <rdfs:comment>Characterizes a extension to an X509 Certificate</rdfs:comment>
    </owl:Class>
</rdf:RDF>



<!-- Generated by the OWL API (version 4.2.6.20160910-2108) https://github.com/owlcs/owlapi -->

