<?xml version="1.0"?>
<rdf:RDF xmlns="http://scap.nist.gov/patch#"
     xml:base="http://scap.nist.gov/patch"
	 xmlns:patch="http://scap.nist.gov/patch#"
     xmlns:rdf="http://www.w3.org/1999/02/22-rdf-syntax-ns#"
     xmlns:owl="http://www.w3.org/2002/07/owl#"
     xmlns:xml="http://www.w3.org/XML/1998/namespace"
     xmlns:xsd="http://www.w3.org/2001/XMLSchema#"
     xmlns:rdfs="http://www.w3.org/2000/01/rdf-schema#">
    <owl:Ontology rdf:about="http://scap.nist.gov/patch">
        <owl:imports rdf:resource="http://scap.nist.gov/scap_core"/>
        <rdfs:comment>This ontology provides a vocabulary and representation for the Security Content Automation Protocol (SCAP) Patch data type which provides a standardized method of describing and identifying patches to address vulnerabilities.  The SCAP is a method for using specific standards to enable automatedmpliance evaluation, vulnerability management, measurement, and policy compliance evaluation. 

Copyright (c) 2014, DaedaFusion, LLC.  All rights reserved.</rdfs:comment>
        <rdfs:label>Security Content Automation Protocol (SCAP) Patch Ontology</rdfs:label>
        <owl:versionInfo rdf:datatype="http://www.w3.org/2001/XMLSchema#string">1.0.0-001</owl:versionInfo>
    </owl:Ontology>
    


    <!-- 
    ///////////////////////////////////////////////////////////////////////////////////////
    //
    // Object Properties
    //
    ///////////////////////////////////////////////////////////////////////////////////////
     -->

    


    <!-- http://scap.nist.gov/patch#check -->

    <owl:ObjectProperty rdf:about="http://scap.nist.gov/patch#check">
        <rdfs:range rdf:resource="http://scap.nist.gov/scap_core#CheckReference"/>
        <rdfs:comment>Specifies zero or more references to check systems associated with this patch.</rdfs:comment>
        <rdfs:isDefinedBy rdf:resource="http://scap.nist.gov/patch"/>
        <rdfs:label>Checks</rdfs:label>
    </owl:ObjectProperty>
    


    <!-- http://scap.nist.gov/patch#references -->

    <owl:ObjectProperty rdf:about="http://scap.nist.gov/patch#references">
        <rdfs:range rdf:resource="http://scap.nist.gov/scap_core#Reference"/>
        <rdfs:comment>Specifies zero or more references associated with the patch.</rdfs:comment>
        <rdfs:isDefinedBy rdf:resource="http://scap.nist.gov/patch"/>
        <rdfs:label>References</rdfs:label>
    </owl:ObjectProperty>
    


    <!-- http://scap.nist.gov/patch#supersededBy -->

    <owl:ObjectProperty rdf:about="http://scap.nist.gov/patch#supersededBy">
        <rdfs:range rdf:resource="http://scap.nist.gov/patch#Patch"/>
        <rdfs:comment>Specifies zero or more patches that supersede this patch.</rdfs:comment>
        <rdfs:isDefinedBy rdf:resource="http://scap.nist.gov/patch"/>
        <rdfs:label>Superseded By</rdfs:label>
    </owl:ObjectProperty>
    


    <!-- http://scap.nist.gov/patch#supersedes -->

    <owl:ObjectProperty rdf:about="http://scap.nist.gov/patch#supersedes">
        <rdfs:range rdf:resource="http://scap.nist.gov/patch#Patch"/>
        <rdfs:comment>Specifies zero or more patches that are superceded by the referenced patch.</rdfs:comment>
        <rdfs:isDefinedBy rdf:resource="http://scap.nist.gov/patch"/>
        <rdfs:label>Supersedes Patches</rdfs:label>
    </owl:ObjectProperty>
    


    <!-- 
    ///////////////////////////////////////////////////////////////////////////////////////
    //
    // Data properties
    //
    ///////////////////////////////////////////////////////////////////////////////////////
     -->

    


    <!-- http://scap.nist.gov/patch#deprecated -->

    <owl:DatatypeProperty rdf:about="http://scap.nist.gov/patch#deprecated">
        <rdfs:range rdf:resource="http://www.w3.org/2001/XMLSchema#boolean"/>
        <rdfs:comment>Specifies that the patch has been depreciated and thus should not be used.</rdfs:comment>
        <rdfs:isDefinedBy rdf:resource="http://scap.nist.gov/patch"/>
        <rdfs:label>Deprecated</rdfs:label>
    </owl:DatatypeProperty>
    


    <!-- http://scap.nist.gov/patch#notes -->

    <owl:DatatypeProperty rdf:about="http://scap.nist.gov/patch#notes">
        <rdfs:range rdf:resource="http://www.w3.org/2001/XMLSchema#string"/>
        <rdfs:comment>Specifies zero or more notes associated with the patch.</rdfs:comment>
        <rdfs:isDefinedBy rdf:resource="http://scap.nist.gov/patch"/>
        <rdfs:label>Notes</rdfs:label>
    </owl:DatatypeProperty>
    


    <!-- http://scap.nist.gov/patch#patchIdentifier -->

    <owl:DatatypeProperty rdf:about="http://scap.nist.gov/patch#patchIdentifier">
        <rdfs:range rdf:resource="http://www.w3.org/2001/XMLSchema#double"/>
        <rdfs:comment>Specifies a unique identifier for the patch</rdfs:comment>
        <rdfs:isDefinedBy rdf:resource="http://scap.nist.gov/patch"/>
        <rdfs:label>Patch Identifier</rdfs:label>
    </owl:DatatypeProperty>
    


    <!-- http://scap.nist.gov/patch#patchName -->

    <owl:DatatypeProperty rdf:about="http://scap.nist.gov/patch#patchName">
        <rdfs:range rdf:resource="http://www.w3.org/2001/XMLSchema#string"/>
        <rdfs:comment>Specifies the vendor-supplied for the patch.  The patch name should be in all lower-case and use underscores for spaces.</rdfs:comment>
        <rdfs:isDefinedBy rdf:resource="http://scap.nist.gov/patch"/>
        <rdfs:label>Patch Name</rdfs:label>
    </owl:DatatypeProperty>
    


    <!-- http://scap.nist.gov/patch#superseded -->

    <owl:DatatypeProperty rdf:about="http://scap.nist.gov/patch#superseded">
        <rdfs:range rdf:resource="http://www.w3.org/2001/XMLSchema#boolean"/>
        <rdfs:comment>Specifies that the patch has been superseded if true.</rdfs:comment>
        <rdfs:isDefinedBy rdf:resource="http://scap.nist.gov/patch"/>
        <rdfs:label>Superseded</rdfs:label>
    </owl:DatatypeProperty>
    


    <!-- http://scap.nist.gov/patch#title -->

    <owl:DatatypeProperty rdf:about="http://scap.nist.gov/patch#title">
        <rdfs:range rdf:resource="http://www.w3.org/2001/XMLSchema#string"/>
        <rdfs:comment>Specifies a human-formatted title for the patch</rdfs:comment>
        <rdfs:isDefinedBy rdf:resource="http://scap.nist.gov/patch"/>
        <rdfs:label>Title</rdfs:label>
    </owl:DatatypeProperty>
    


    <!-- 
    ///////////////////////////////////////////////////////////////////////////////////////
    //
    // Classes
    //
    ///////////////////////////////////////////////////////////////////////////////////////
     -->

    


    <!-- http://scap.nist.gov/patch#Patch -->

    <owl:Class rdf:about="http://scap.nist.gov/patch#Patch">
        <rdfs:subClassOf>
            <owl:Restriction>
                <owl:onProperty rdf:resource="http://scap.nist.gov/patch#deprecated"/>
                <owl:someValuesFrom rdf:resource="http://www.w3.org/2000/01/rdf-schema#Literal"/>
            </owl:Restriction>
        </rdfs:subClassOf>
        <rdfs:subClassOf>
            <owl:Restriction>
                <owl:onProperty rdf:resource="http://scap.nist.gov/patch#patchIdentifier"/>
                <owl:someValuesFrom rdf:resource="http://www.w3.org/2000/01/rdf-schema#Literal"/>
            </owl:Restriction>
        </rdfs:subClassOf>
        <rdfs:subClassOf>
            <owl:Restriction>
                <owl:onProperty rdf:resource="http://scap.nist.gov/patch#patchName"/>
                <owl:someValuesFrom rdf:resource="http://www.w3.org/2000/01/rdf-schema#Literal"/>
            </owl:Restriction>
        </rdfs:subClassOf>
        <rdfs:subClassOf>
            <owl:Restriction>
                <owl:onProperty rdf:resource="http://scap.nist.gov/patch#superseded"/>
                <owl:someValuesFrom rdf:resource="http://www.w3.org/2000/01/rdf-schema#Literal"/>
            </owl:Restriction>
        </rdfs:subClassOf>
        <rdfs:subClassOf>
            <owl:Restriction>
                <owl:onProperty rdf:resource="http://scap.nist.gov/patch#title"/>
                <owl:someValuesFrom rdf:resource="http://www.w3.org/2000/01/rdf-schema#Literal"/>
            </owl:Restriction>
        </rdfs:subClassOf>
        <rdfs:comment>Defines a patch</rdfs:comment>
        <rdfs:isDefinedBy rdf:resource="http://scap.nist.gov/patch"/>
        <rdfs:label>Patch</rdfs:label>
    </owl:Class>
    

</rdf:RDF>



<!-- Generated by the OWL API (version 4.2.6.20160910-2108) https://github.com/owlcs/owlapi -->

