<?xml version="1.0"?>
<rdf:RDF xmlns="http://scap.nist.gov/scap_core#"
     xml:base="http://scap.nist.gov/scap_core"
     xmlns:rdf="http://www.w3.org/1999/02/22-rdf-syntax-ns#"
     xmlns:owl="http://www.w3.org/2002/07/owl#"
     xmlns:xml="http://www.w3.org/XML/1998/namespace"
     xmlns:xsd="http://www.w3.org/2001/XMLSchema#"
     xmlns:cpe="http://cpe.mitre.org/cpe#"
     xmlns:scap_core="http://scap.nist.gov/scap_core#"
     xmlns:rdfs="http://www.w3.org/2000/01/rdf-schema#">
    <owl:Ontology rdf:about="http://scap.nist.gov/scap_core">
        <rdfs:label>Security Content Automation Protocol (SCAP) Core  Ontology</rdfs:label>
        <rdfs:comment>This ontology provides a vocabulary and representation for the Security Content Automation Protocol (SCAP) core data types.  The SCAP is a method for using specific standards to enable automated compliance evaluation, vulnerability management, measurement, and policy compliance evaluation.

Copyright (c) 2014, DaedaFusion, LLC.  All rights reserved.</rdfs:comment>
        <owl:versionInfo rdf:datatype="http://www.w3.org/2001/XMLSchema#string">1.0.0-001</owl:versionInfo>
    </owl:Ontology>
    


    <!-- 
    ///////////////////////////////////////////////////////////////////////////////////////
    //
    // Datatypes
    //
    ///////////////////////////////////////////////////////////////////////////////////////
     -->

    


    <!-- http://www.w3.org/2001/XMLSchema#date -->

    <rdfs:Datatype rdf:about="http://www.w3.org/2001/XMLSchema#date"/>
    


    <!-- 
    ///////////////////////////////////////////////////////////////////////////////////////
    //
    // Object Properties
    //
    ///////////////////////////////////////////////////////////////////////////////////////
     -->

    


    <!-- http://scap.nist.gov/scap_core#generator -->

    <owl:ObjectProperty rdf:about="http://scap.nist.gov/scap_core#generator">
        <rdfs:comment>Specifies information about the tool used to generate the catalog</rdfs:comment>
        <rdfs:isDefinedBy rdf:resource="http://scap.nist.gov/scap_core"/>
        <rdfs:label>Generator</rdfs:label>
    </owl:ObjectProperty>
    


    <!-- 
    ///////////////////////////////////////////////////////////////////////////////////////
    //
    // Data properties
    //
    ///////////////////////////////////////////////////////////////////////////////////////
     -->

    


    <!-- http://scap.nist.gov/scap_core#catalogDate -->

    <owl:DatatypeProperty rdf:about="http://scap.nist.gov/scap_core#catalogDate">
        <rdfs:range rdf:resource="http://www.w3.org/2001/XMLSchema#date"/>
        <rdfs:comment>Specifies the date the catalog was created or last updated.</rdfs:comment>
        <rdfs:isDefinedBy rdf:resource="http://scap.nist.gov/scap_core"/>
        <rdfs:label>Date</rdfs:label>
    </owl:DatatypeProperty>
    


    <!-- http://scap.nist.gov/scap_core#catalogName -->

    <owl:DatatypeProperty rdf:about="http://scap.nist.gov/scap_core#catalogName">
        <rdfs:range rdf:resource="http://www.w3.org/2001/XMLSchema#string"/>
        <rdfs:comment>Specifies the name of the catalog</rdfs:comment>
        <rdfs:isDefinedBy rdf:resource="http://scap.nist.gov/scap_core"/>
        <rdfs:label>Name</rdfs:label>
    </owl:DatatypeProperty>
    


    <!-- http://scap.nist.gov/scap_core#catalogVersion -->

    <owl:DatatypeProperty rdf:about="http://scap.nist.gov/scap_core#catalogVersion">
        <rdfs:range rdf:resource="http://www.w3.org/2001/XMLSchema#string"/>
        <rdfs:comment>Specifies the version of the catalog</rdfs:comment>
        <rdfs:isDefinedBy rdf:resource="http://scap.nist.gov/scap_core"/>
        <rdfs:label>Version</rdfs:label>
    </owl:DatatypeProperty>
    


    <!-- http://scap.nist.gov/scap_core#checkIdentifier -->

    <owl:DatatypeProperty rdf:about="http://scap.nist.gov/scap_core#checkIdentifier">
        <rdfs:range rdf:resource="http://www.w3.org/2001/XMLSchema#string"/>
        <rdfs:comment>Specifies an identifier of a test written in the check system language.</rdfs:comment>
        <rdfs:isDefinedBy rdf:resource="http://scap.nist.gov/scap_core"/>
        <rdfs:label>Check Identifier</rdfs:label>
    </owl:DatatypeProperty>
    


    <!-- http://scap.nist.gov/scap_core#checkSystem -->

    <owl:DatatypeProperty rdf:about="http://scap.nist.gov/scap_core#checkSystem">
        <rdfs:range rdf:resource="http://www.w3.org/2001/XMLSchema#anyURI"/>
        <rdfs:comment></rdfs:comment>
        <rdfs:isDefinedBy rdf:resource="http://scap.nist.gov/scap_core"/>
        <rdfs:label>Check System URI</rdfs:label>
    </owl:DatatypeProperty>
    


    <!-- http://scap.nist.gov/scap_core#description -->

    <owl:DatatypeProperty rdf:about="http://scap.nist.gov/scap_core#description">
        <rdfs:range rdf:resource="http://www.w3.org/2001/XMLSchema#string"/>
        <rdfs:comment>Specifies a brief description of the catalog contents</rdfs:comment>
        <rdfs:isDefinedBy rdf:resource="http://scap.nist.gov/scap_core"/>
        <rdfs:label>Description</rdfs:label>
    </owl:DatatypeProperty>
    


    <!-- http://scap.nist.gov/scap_core#externalLink -->

    <owl:DatatypeProperty rdf:about="http://scap.nist.gov/scap_core#externalLink">
        <rdfs:range rdf:resource="http://www.w3.org/2001/XMLSchema#anyURI"/>
        <rdfs:comment>Specifies a URI to an external file or resource.</rdfs:comment>
        <rdfs:isDefinedBy rdf:resource="http://scap.nist.gov/scap_core"/>
        <rdfs:label>External Link</rdfs:label>
    </owl:DatatypeProperty>
    


    <!-- http://scap.nist.gov/scap_core#id -->

    <owl:DatatypeProperty rdf:about="http://scap.nist.gov/scap_core#id">
        <rdfs:range rdf:resource="http://www.w3.org/2001/XMLSchema#string"/>
        <rdfs:comment>Specifies the unique identifier associated with this entity instance.

An identifier MUST take the format [ns-prefix]:[construct-type]-[identifier], where [ns-prefix] should be the namespace prefix owned/controlled by the producer of the content

The format of the Id must be in the format of [ns-prefix]:construct-type-[identifier], there the [ns-prefix] SHOULD be a namespace prefix bound to a namespace owned/controlled by the producer of the content, and [identifier] SHOULD correspond to a globally unique identifier or information that uniquely identifies the entity.</rdfs:comment>
        <rdfs:isDefinedBy rdf:resource="http://scap.nist.gov/scap_core"/>
        <rdfs:label>Id</rdfs:label>
    </owl:DatatypeProperty>
    


    <!-- http://scap.nist.gov/scap_core#name -->

    <owl:DatatypeProperty rdf:about="http://scap.nist.gov/scap_core#name">
        <rdfs:range rdf:resource="http://www.w3.org/2001/XMLSchema#string"/>
        <rdfs:comment>Specifies a piece of human-readable text that provides a meaningful name.</rdfs:comment>
        <rdfs:isDefinedBy rdf:resource="http://scap.nist.gov/scap_core"/>
        <rdfs:label>Name</rdfs:label>
    </owl:DatatypeProperty>
    


    <!-- http://scap.nist.gov/scap_core#notes -->

    <owl:DatatypeProperty rdf:about="http://scap.nist.gov/scap_core#notes">
        <rdfs:range rdf:resource="http://www.w3.org/2001/XMLSchema#string"/>
        <rdfs:comment>Specifies one or more notes about an entity</rdfs:comment>
        <rdfs:isDefinedBy rdf:resource="http://scap.nist.gov/scap_core"/>
        <rdfs:label>Notes</rdfs:label>
    </owl:DatatypeProperty>
    


    <!-- 
    ///////////////////////////////////////////////////////////////////////////////////////
    //
    // Classes
    //
    ///////////////////////////////////////////////////////////////////////////////////////
     -->

    


    <!-- http://scap.nist.gov/scap_core#Catalog -->

    <owl:Class rdf:about="http://scap.nist.gov/scap_core#Catalog">
        <rdfs:subClassOf>
            <owl:Restriction>
                <owl:onProperty rdf:resource="http://scap.nist.gov/scap_core#catalogDate"/>
                <owl:someValuesFrom rdf:resource="http://www.w3.org/2000/01/rdf-schema#Literal"/>
            </owl:Restriction>
        </rdfs:subClassOf>
        <rdfs:subClassOf>
            <owl:Restriction>
                <owl:onProperty rdf:resource="http://scap.nist.gov/scap_core#catalogName"/>
                <owl:someValuesFrom rdf:resource="http://www.w3.org/2000/01/rdf-schema#Literal"/>
            </owl:Restriction>
        </rdfs:subClassOf>
        <rdfs:subClassOf>
            <owl:Restriction>
                <owl:onProperty rdf:resource="http://scap.nist.gov/scap_core#catalogVersion"/>
                <owl:someValuesFrom rdf:resource="http://www.w3.org/2000/01/rdf-schema#Literal"/>
            </owl:Restriction>
        </rdfs:subClassOf>
        <rdfs:subClassOf>
            <owl:Restriction>
                <owl:onProperty rdf:resource="http://scap.nist.gov/scap_core#description"/>
                <owl:someValuesFrom rdf:resource="http://www.w3.org/2000/01/rdf-schema#Literal"/>
            </owl:Restriction>
        </rdfs:subClassOf>
        <rdfs:subClassOf>
            <owl:Restriction>
                <owl:onProperty rdf:resource="http://scap.nist.gov/scap_core#id"/>
                <owl:someValuesFrom rdf:resource="http://www.w3.org/2000/01/rdf-schema#Literal"/>
            </owl:Restriction>
        </rdfs:subClassOf>
        <rdfs:comment>Characterizes a Catalog of information</rdfs:comment>
        <rdfs:isDefinedBy rdf:resource="http://scap.nist.gov/scap_core"/>
        <rdfs:label>Catalog</rdfs:label>
    </owl:Class>
    


    <!-- http://scap.nist.gov/scap_core#CheckReference -->

    <owl:Class rdf:about="http://scap.nist.gov/scap_core#CheckReference">
        <rdfs:subClassOf>
            <owl:Restriction>
                <owl:onProperty rdf:resource="http://scap.nist.gov/scap_core#checkIdentifier"/>
                <owl:someValuesFrom rdf:resource="http://www.w3.org/2000/01/rdf-schema#Literal"/>
            </owl:Restriction>
        </rdfs:subClassOf>
        <rdfs:subClassOf>
            <owl:Restriction>
                <owl:onProperty rdf:resource="http://scap.nist.gov/scap_core#checkSystem"/>
                <owl:someValuesFrom rdf:resource="http://www.w3.org/2000/01/rdf-schema#Literal"/>
            </owl:Restriction>
        </rdfs:subClassOf>
        <rdfs:subClassOf>
            <owl:Restriction>
                <owl:onProperty rdf:resource="http://scap.nist.gov/scap_core#externalLink"/>
                <owl:someValuesFrom rdf:resource="http://www.w3.org/2000/01/rdf-schema#Literal"/>
            </owl:Restriction>
        </rdfs:subClassOf>
        <rdfs:comment>Defines a checking system specification URI, string content, and optional external file reference.  The checking system specification should be the URI for a particular version of OVAL or a related system testing language, and the content will should be an identifier of a test written in that language.  The external file reference could be used to point to the file in whcih the content test identifier is defined.</rdfs:comment>
        <rdfs:isDefinedBy rdf:resource="http://scap.nist.gov/scap_core"/>
        <rdfs:label>Check Reference</rdfs:label>
    </owl:Class>
    


    <!-- http://scap.nist.gov/scap_core#Reference -->

    <owl:Class rdf:about="http://scap.nist.gov/scap_core#Reference">
        <rdfs:subClassOf>
            <owl:Restriction>
                <owl:onProperty rdf:resource="http://scap.nist.gov/scap_core#externalLink"/>
                <owl:someValuesFrom rdf:resource="http://www.w3.org/2000/01/rdf-schema#Literal"/>
            </owl:Restriction>
        </rdfs:subClassOf>
        <rdfs:subClassOf>
            <owl:Restriction>
                <owl:onProperty rdf:resource="http://scap.nist.gov/scap_core#name"/>
                <owl:someValuesFrom rdf:resource="http://www.w3.org/2000/01/rdf-schema#Literal"/>
            </owl:Restriction>
        </rdfs:subClassOf>
        <rdfs:comment>Defines a general reference that is normally used to point to extra descriptive material, or a supplier&apos;s web site, or platform documentation.</rdfs:comment>
        <rdfs:isDefinedBy rdf:resource="http://scap.nist.gov/scap_core"/>
        <rdfs:label>Reference</rdfs:label>
    </owl:Class>
</rdf:RDF>



<!-- Generated by the OWL API (version 4.2.6.20160910-2108) https://github.com/owlcs/owlapi -->

