<?xml version="1.0"?>
<rdf:RDF
    xmlns:rdf="http://www.w3.org/1999/02/22-rdf-syntax-ns#"
    xmlns:et="http://stix.mitre.org/ExploitTarget#"
    xmlns:owl="http://www.w3.org/2002/07/owl#"
    xmlns:xsd="http://www.w3.org/2001/XMLSchema#"
    
    xmlns:rdfs="http://www.w3.org/2000/01/rdf-schema#"
  xml:base="http://stix.mitre.org/ExploitTarget">
  <owl:Ontology rdf:about="http://stix.mitre.org/ExploitTarget">
    <owl:imports rdf:resource="http://data-marking.mitre.org/Data_Marking"/>
    <owl:versionIRI rdf:resource="http://stix.mitre.org/ExploitTarget/1.2"/>
    <owl:imports rdf:resource="http://cce.mitre.org/cce"/>
    <owl:imports rdf:resource="http://stix.mitre.org/stixCommon"/>
	<owl:imports rdf:resource="http://www.oasis-open.org/ciq_common"/> <!-- Ryan added 11/28/2016 -->
    <owl:versionInfo rdf:datatype="http://www.w3.org/2001/XMLSchema#string"
    >1.2.0-000</owl:versionInfo>
    <rdfs:label >STIX Exploit Target Ontology</rdfs:label>
    <owl:imports rdf:resource="http://nvd.nist.gov/cve"/>
    <owl:imports rdf:resource="http://cpe.mitre.org/cpe"/>
    <owl:imports rdf:resource="http://nvd.nist.gov/cvss"/>
    <rdfs:comment >This ontology provides a vocabulary and representation for the Structured Threat Information eXpression (STIX) Exploit Target.  The Exploit Target ontology provides a characterization of potential targets for exploit and provides insight about targeted victims that may make them vulnerable to attack.

A STIX Exploit Target conveys information about a technical vulnerability, weakness, or misconfiguration in software, systems, or networks that may be targeted for exploitation by an adversary. The Exploit Target component leverages current standard approaches in identifying and describing vulnerabilities through the suggested option of using CVE and/or OSVDB IDs to identify named vulnerabilities, CVRF to describe 0-day or other unnamed vulnerabilities, and CVSS to score vulnerabilities. Additionally, CCE is used as the suggested method to identify configuration items and CWE as a mechanism for representing software weaknesses.

In the STIX relationship model, exploit targets are used to identify possible targets of a TTP and can reference courses of action as potential mechanisms to remediate the exploit target.</rdfs:comment>
    
    <owl:imports rdf:resource="http://cybox.mitre.org/objects/NetworkProtocol"/>
  </owl:Ontology>
  <owl:Class rdf:ID="Weakness">
    <rdfs:subClassOf>
      <owl:Restriction>
        <owl:onProperty>
          <rdf:Description rdf:about="http://stix.mitre.org/stixCommon#shortDescription">
            <rdfs:domain>
              <owl:Class rdf:ID="ConfigurationIssue"/>
            </rdfs:domain>
            <rdfs:domain rdf:resource="#Weakness"/>
            <rdfs:domain>
              <owl:Class rdf:ID="Vulnerability"/>
            </rdfs:domain>
            <rdfs:domain>
              <owl:Class rdf:ID="ExploitTarget"/>
            </rdfs:domain>
          </rdf:Description>
        </owl:onProperty>
        <owl:minCardinality rdf:datatype="http://www.w3.org/2001/XMLSchema#nonNegativeInteger"
        >1</owl:minCardinality>
      </owl:Restriction>
    </rdfs:subClassOf>
    
    <rdfs:comment >Characterizes a weakeness as a potential Exploit Target.</rdfs:comment>
    
    <rdfs:isDefinedBy rdf:resource=""/>
    
    
    <rdfs:subClassOf>
      <owl:Restriction>
        <owl:maxCardinality rdf:datatype="http://www.w3.org/2001/XMLSchema#nonNegativeInteger"
        >1</owl:maxCardinality>
        <owl:onProperty>
          <owl:ObjectProperty rdf:ID="cweDetails"/>
        </owl:onProperty>
      </owl:Restriction>
    </rdfs:subClassOf>
    <rdfs:subClassOf>
      <owl:Restriction>
        <owl:cardinality rdf:datatype="http://www.w3.org/2001/XMLSchema#nonNegativeInteger"
        >1</owl:cardinality>
        <owl:onProperty>
          <rdf:Description rdf:about="http://stix.mitre.org/stixCommon#id">
            <rdfs:domain>
              <owl:Class rdf:about="#ConfigurationIssue"/>
            </rdfs:domain>
            <rdfs:domain>
              <owl:Class rdf:about="#Vulnerability"/>
            </rdfs:domain>
            <rdfs:domain rdf:resource="#Weakness"/>
          </rdf:Description>
        </owl:onProperty>
      </owl:Restriction>
    </rdfs:subClassOf>
    <rdfs:label >Weakness</rdfs:label>
    <rdfs:subClassOf>
      <owl:Restriction>
        <owl:cardinality rdf:datatype="http://www.w3.org/2001/XMLSchema#nonNegativeInteger"
        >1</owl:cardinality>
        <owl:onProperty>
          <owl:DatatypeProperty rdf:ID="cweId"/>
        </owl:onProperty>
      </owl:Restriction>
    </rdfs:subClassOf>
  </owl:Class>
  <owl:Class rdf:about="#Vulnerability">
    
    <rdfs:subClassOf>
      <owl:Restriction>
        <owl:onProperty>
          <owl:DatatypeProperty rdf:ID="isPubliclyAcknowledge"/>
        </owl:onProperty>
        <owl:cardinality rdf:datatype="http://www.w3.org/2001/XMLSchema#nonNegativeInteger"
        >1</owl:cardinality>
      </owl:Restriction>
    </rdfs:subClassOf>
    
    <rdfs:subClassOf>
      <owl:Restriction>
        <owl:cardinality rdf:datatype="http://www.w3.org/2001/XMLSchema#nonNegativeInteger"
        >1</owl:cardinality>
        <owl:onProperty rdf:resource="http://stix.mitre.org/stixCommon#id"/>
      </owl:Restriction>
    </rdfs:subClassOf>
    <rdfs:subClassOf>
      <owl:Restriction>
        <owl:maxCardinality rdf:datatype="http://www.w3.org/2001/XMLSchema#nonNegativeInteger"
        >1</owl:maxCardinality>
        <owl:onProperty>
          <rdf:Description rdf:about="http://stix.mitre.org/stixCommon#title">
            <rdfs:domain rdf:resource="#Vulnerability"/>
            <rdfs:domain>
              <owl:Class rdf:about="#ExploitTarget"/>
            </rdfs:domain>
          </rdf:Description>
        </owl:onProperty>
      </owl:Restriction>
    </rdfs:subClassOf>
    <rdfs:isDefinedBy rdf:resource=""/>
    <rdfs:label >Vulnerability</rdfs:label>
    <rdfs:subClassOf>
      <owl:Restriction>
        <owl:onProperty>
          <owl:DatatypeProperty rdf:ID="isKnown"/>
        </owl:onProperty>
        <owl:cardinality rdf:datatype="http://www.w3.org/2001/XMLSchema#nonNegativeInteger"
        >1</owl:cardinality>
      </owl:Restriction>
    </rdfs:subClassOf>
    <rdfs:subClassOf>
      <owl:Restriction>
        <owl:onProperty rdf:resource="http://stix.mitre.org/stixCommon#shortDescription"/>
        <owl:minCardinality rdf:datatype="http://www.w3.org/2001/XMLSchema#nonNegativeInteger"
        >1</owl:minCardinality>
      </owl:Restriction>
    </rdfs:subClassOf>
    <rdfs:comment >Characterizes an individual vulnerability.

The Vulnerability class captures basic information and references to vulnerability registries.  In addition, it can be used as the base class by which to extend to enable the structured description of a vulnerability.</rdfs:comment>
    
  </owl:Class>
  <owl:Class rdf:about="#ExploitTarget">
    <rdfs:subClassOf>
      <owl:Restriction>
        <owl:maxCardinality rdf:datatype="http://www.w3.org/2001/XMLSchema#nonNegativeInteger"
        >1</owl:maxCardinality>
        <owl:onProperty>
          <rdf:Description rdf:about="http://www.oasis-open.org/ciq_common#validFromDateTime">
            <rdfs:domain rdf:resource="http://stix.mitre.org/stixCommon#ExploitTargetBase"/>
          </rdf:Description>
        </owl:onProperty>
      </owl:Restriction>
    </rdfs:subClassOf>
    <rdfs:subClassOf>
      <owl:Restriction>
        <owl:onProperty rdf:resource="http://stix.mitre.org/stixCommon#title"/>
        <owl:cardinality rdf:datatype="http://www.w3.org/2001/XMLSchema#nonNegativeInteger"
        >1</owl:cardinality>
      </owl:Restriction>
    </rdfs:subClassOf>
    <rdfs:subClassOf rdf:resource="http://stix.mitre.org/stixCommon#ExploitTargetBase"/>
    <rdfs:subClassOf>
      <owl:Restriction>
        <owl:maxCardinality rdf:datatype="http://www.w3.org/2001/XMLSchema#nonNegativeInteger"
        >1</owl:maxCardinality>
        <owl:onProperty>
          <rdf:Description rdf:about="http://www.oasis-open.org/ciq_common#validToDateTime">
            <rdfs:domain rdf:resource="http://stix.mitre.org/stixCommon#ExploitTargetBase"/>
          </rdf:Description>
        </owl:onProperty>
      </owl:Restriction>
    </rdfs:subClassOf>
    
    <rdfs:label >Exploit Target</rdfs:label>
    
    <rdfs:isDefinedBy rdf:resource=""/>
    <rdfs:subClassOf>
      <owl:Restriction>
        <owl:onProperty>
          <rdf:Description rdf:about="http://stix.mitre.org/stixCommon#informationSource">
            <rdfs:domain rdf:resource="#ExploitTarget"/>
          </rdf:Description>
        </owl:onProperty>
        <owl:maxCardinality rdf:datatype="http://www.w3.org/2001/XMLSchema#nonNegativeInteger"
        >1</owl:maxCardinality>
      </owl:Restriction>
    </rdfs:subClassOf>
    <rdfs:subClassOf>
      <owl:Restriction>
        <owl:onProperty>
          <rdf:Description rdf:about="http://www.oasis-open.org/ciq_common#status">
            <rdfs:domain rdf:resource="http://stix.mitre.org/stixCommon#ExploitTargetBase"/>
          </rdf:Description>
        </owl:onProperty>
        <owl:maxCardinality rdf:datatype="http://www.w3.org/2001/XMLSchema#nonNegativeInteger"
        >1</owl:maxCardinality>
      </owl:Restriction>
    </rdfs:subClassOf>
    <rdfs:comment >Characterizes potential targets for exploitation by capturing characteristics of targeted victims they may make them vulnerable to attack.

ExploitTargets are vulnerabilities or weaknesses in software, systems, networks or configurations that are targeted for exploitation by the TTP of a ThreatActor. In a structured sense, ExploitTargets consist of vulnerability identifications or characterizations, weakness identifications or characterizations, configuration identifications or characterizations, potential Courses of Action, source of the ExploitTarget information, handling guidance, etc.</rdfs:comment>
    <rdfs:subClassOf>
      <owl:Restriction>
        <owl:onProperty rdf:resource="http://stix.mitre.org/stixCommon#id"/>
        <owl:cardinality rdf:datatype="http://www.w3.org/2001/XMLSchema#nonNegativeInteger"
        >1</owl:cardinality>
      </owl:Restriction>
    </rdfs:subClassOf>
    <rdfs:subClassOf>
      <owl:Restriction>
        <owl:onProperty rdf:resource="http://data-marking.mitre.org/Data_Marking#informationSource"/>
        <owl:maxCardinality rdf:datatype="http://www.w3.org/2001/XMLSchema#nonNegativeInteger"
        >1</owl:maxCardinality>
      </owl:Restriction>
    </rdfs:subClassOf>
    <rdfs:subClassOf>
      <owl:Restriction>
        <owl:onProperty rdf:resource="http://stix.mitre.org/stixCommon#shortDescription"/>
        <owl:minCardinality rdf:datatype="http://www.w3.org/2001/XMLSchema#nonNegativeInteger"
        >1</owl:minCardinality>
      </owl:Restriction>
    </rdfs:subClassOf>
    <rdfs:subClassOf>
      <owl:Restriction>
        <owl:onProperty rdf:resource="http://stix.mitre.org/stixCommon#timestamp"/>
        <owl:cardinality rdf:datatype="http://www.w3.org/2001/XMLSchema#nonNegativeInteger"
        >1</owl:cardinality>
      </owl:Restriction>
    </rdfs:subClassOf>
    
  </owl:Class>
  <owl:Class rdf:about="#ConfigurationIssue">
    <rdfs:label >Configuration Issue</rdfs:label>
    <rdfs:subClassOf>
      <owl:Restriction>
        <owl:maxCardinality rdf:datatype="http://www.w3.org/2001/XMLSchema#nonNegativeInteger"
        >1</owl:maxCardinality>
        <owl:onProperty>
          <owl:ObjectProperty rdf:ID="cceDetails"/>
        </owl:onProperty>
      </owl:Restriction>
    </rdfs:subClassOf>
    <rdfs:subClassOf>
      <owl:Restriction>
        <owl:onProperty rdf:resource="http://stix.mitre.org/stixCommon#shortDescription"/>
        <owl:minCardinality rdf:datatype="http://www.w3.org/2001/XMLSchema#nonNegativeInteger"
        >1</owl:minCardinality>
      </owl:Restriction>
    </rdfs:subClassOf>
    
    <rdfs:subClassOf>
      <owl:Restriction>
        <owl:cardinality rdf:datatype="http://www.w3.org/2001/XMLSchema#nonNegativeInteger"
        >1</owl:cardinality>
        <owl:onProperty>
          <owl:DatatypeProperty rdf:ID="cceId"/>
        </owl:onProperty>
      </owl:Restriction>
    </rdfs:subClassOf>
    
    
    <rdfs:comment >Characterizes a software or hardware configuratioin as a potential Exploit Target.</rdfs:comment>
    <rdfs:isDefinedBy rdf:resource=""/>
    
    <rdfs:subClassOf>
      <owl:Restriction>
        <owl:cardinality rdf:datatype="http://www.w3.org/2001/XMLSchema#nonNegativeInteger"
        >1</owl:cardinality>
        <owl:onProperty rdf:resource="http://stix.mitre.org/stixCommon#id"/>
      </owl:Restriction>
    </rdfs:subClassOf>
  </owl:Class>
  <owl:ObjectProperty rdf:ID="cvrfdoc">
    <rdfs:comment >Specifies references to the related structured characterization of Vulnerabilities utilizing the Common Vulnerability Reporting Framework (CVRF).  

The use of the Common Vulnerability Reporting Framework (CVRF) allows characterization of 0-day or other vulnerabilities that have not been assigned a CVE or OSVDB Identifier.</rdfs:comment>
    <rdfs:domain rdf:resource="#Vulnerability"/>
    <rdfs:label >Related CVRF document</rdfs:label>
  </owl:ObjectProperty>
  <owl:ObjectProperty rdf:ID="configurationIssues">
    <rdfs:comment >Specifies references to a characterization of a configuration issue</rdfs:comment>
    <rdfs:domain rdf:resource="#ExploitTarget"/>
    <rdfs:label >Related Configurations</rdfs:label>
    <rdfs:range rdf:resource="http://cce.mitre.org/cce#CCE"/>
  </owl:ObjectProperty>
  <owl:ObjectProperty rdf:ID="cveDetails">
    <rdfs:comment >Specifies a reference to the related Common Vulnerability Enumeration (CVE) entity</rdfs:comment>
    <rdfs:domain rdf:resource="#Vulnerability"/>
    <rdfs:range rdf:resource="http://nvd.nist.gov/cve#Vulnerability"/>
    <rdfs:label >CVE Reference</rdfs:label>
  </owl:ObjectProperty>
  <owl:ObjectProperty rdf:ID="vulnerabilities">
    <rdfs:comment >Specifies a reference to a characterization of a vulnerability as a potential exploit target</rdfs:comment>
    <rdfs:label >Related Vulnerabilities</rdfs:label>
    <rdfs:domain rdf:resource="#ExploitTarget"/>
    <rdfs:range rdf:resource="#Vulnerability"/>
  </owl:ObjectProperty>
  <owl:ObjectProperty rdf:ID="osvdbDetails">
    <rdfs:comment >Specifies a reference to the the related Open Source Vulnerabilty DataBase (OSVDB) entity</rdfs:comment>
    <rdfs:domain rdf:resource="#Vulnerability"/>
    <rdfs:label >OSVDB Reference</rdfs:label>
  </owl:ObjectProperty>
  <owl:ObjectProperty rdf:ID="affectedSoftware">
    <rdfs:comment >Specifies references to the list of platforms and software that are affected by this vulnerability.</rdfs:comment>
    <rdfs:label >Affected Software</rdfs:label>
    <rdfs:domain rdf:resource="#Vulnerability"/>
    <rdfs:range rdf:resource="http://stix.mitre.org/stixCommon#ObservableRelationship"/>
  </owl:ObjectProperty>
  <owl:ObjectProperty rdf:ID="potentialCOAs">
    <rdfs:label >Potential COAs</rdfs:label>
    <rdfs:comment >Specifies a reference to a potential Course of Action for this exploit target</rdfs:comment>
    <rdfs:domain rdf:resource="#ExploitTarget"/>
    <rdfs:range rdf:resource="http://stix.mitre.org/stixCommon#CourseOfActionBase"/>
  </owl:ObjectProperty>
  <owl:ObjectProperty rdf:ID="weaknesses">
    <rdfs:comment >Specifies a reference to a characterization of a weakness as a potential exploit target</rdfs:comment>
    <rdfs:domain rdf:resource="#ExploitTarget"/>
    <rdfs:label >Related Weakness</rdfs:label>
    <rdfs:range rdf:resource="#Weakness"/>
  </owl:ObjectProperty>
  <owl:ObjectProperty rdf:ID="cvssScore">
    <rdfs:comment >Specifies a reference to the full CVSS 2.0 base, termporal, and environmental vectors</rdfs:comment>
    <rdfs:label >CVSS Score</rdfs:label>
    <rdfs:domain rdf:resource="#Vulnerability"/>
    <rdfs:range rdf:resource="http://nvd.nist.gov/cvss#CVSSImpact"/>
  </owl:ObjectProperty>
  <owl:ObjectProperty rdf:about="#cceDetails">
    <rdfs:domain rdf:resource="#ConfigurationIssue"/>
    <rdfs:comment >Specifies a reference to details for the CCE ID</rdfs:comment>
    <rdfs:isDefinedBy rdf:resource=""/>
    <rdfs:label >CCE Details</rdfs:label>
    
    <rdfs:range rdf:resource="http://cce.mitre.org/cce#CCE"/>
  </owl:ObjectProperty>
  <owl:ObjectProperty rdf:about="#cweDetails">
    <rdfs:comment >Specifies a reference to the related Common Weakness Enumeration (CWE) entity.</rdfs:comment>
    <rdfs:label >CWE Details</rdfs:label>
    <rdfs:isDefinedBy rdf:resource=""/>
    <rdfs:domain rdf:resource="#Weakness"/>
    
    <rdfs:range rdf:resource="http://cwe.mitre.org/cwe#Weakness"/>
  </owl:ObjectProperty>
  <owl:DatatypeProperty rdf:ID="publishedTimestamp">
    <rdfs:range rdf:resource="http://www.w3.org/2001/XMLSchema#dateTime"/>
    <rdfs:comment >Specifies the date and time the vulnerability was first published.</rdfs:comment>
    <rdfs:domain rdf:resource="#Vulnerability"/>
    <rdfs:label >Published Timestamp</rdfs:label>
  </owl:DatatypeProperty>
  <owl:DatatypeProperty rdf:ID="cveId">
    <rdfs:domain rdf:resource="#Vulnerability"/>
    <rdfs:range rdf:resource="http://www.w3.org/2001/XMLSchema#string"/>
    <rdfs:comment >Specifies the Common Vulnerability Enumeration (CVE) Identifier for a particular vulnerability</rdfs:comment>
    <rdfs:label >CVE Identifier</rdfs:label>
  </owl:DatatypeProperty>
  <owl:DatatypeProperty rdf:ID="timestamp">
    <rdfs:comment >Specifies a timestamp for the defintion of of a specific version of an Exploit Target.  

When used in conjunction with the id, this field is specifying the definition time for the specific version of the Exploit Target.</rdfs:comment>
    <rdfs:label >timestamp</rdfs:label>
    <rdfs:range rdf:resource="http://www.w3.org/2001/XMLSchema#dateTime"/>
  </owl:DatatypeProperty>
  <owl:DatatypeProperty rdf:ID="discoveryTimestamp">
    <rdfs:domain rdf:resource="#Vulnerability"/>
    <rdfs:comment >Specifies the date and time that the vulnerability was first discovered</rdfs:comment>
    <rdfs:range rdf:resource="http://www.w3.org/2001/XMLSchema#dateTime"/>
    <rdfs:label >Discovery Timestamp</rdfs:label>
  </owl:DatatypeProperty>
  <owl:DatatypeProperty rdf:about="#cweId">
    <rdfs:range rdf:resource="http://www.w3.org/2001/XMLSchema#string"/>
    <rdfs:isDefinedBy rdf:resource=""/>
    <rdfs:comment >Sspecifies a CWE identifier for a particular weakness.</rdfs:comment>
    <rdfs:domain rdf:resource="#Weakness"/>
    
    <rdfs:label >CWE ID</rdfs:label>
  </owl:DatatypeProperty>
  <owl:DatatypeProperty rdf:about="#isKnown">
    <rdfs:domain rdf:resource="#Vulnerability"/>
    <rdfs:comment >Specifies whether or not the vulnerability is known (i.e. not a 0-day) at the time of characterization.</rdfs:comment>
    <rdfs:range rdf:resource="http://www.w3.org/2001/XMLSchema#boolean"/>
    <rdfs:label >Known</rdfs:label>
  </owl:DatatypeProperty>
  <owl:DatatypeProperty rdf:about="#cceId">
    <rdfs:domain rdf:resource="#ConfigurationIssue"/>
    <rdfs:range rdf:resource="http://www.w3.org/2001/XMLSchema#string"/>
    <rdfs:isDefinedBy rdf:resource=""/>
    <rdfs:label >CCE ID</rdfs:label>
    
    <rdfs:comment >Specifies a CCE identifier for a particular configuration item.</rdfs:comment>
  </owl:DatatypeProperty>
  <owl:DatatypeProperty rdf:about="#isPubliclyAcknowledge">
    <rdfs:domain rdf:resource="#Vulnerability"/>
    <rdfs:comment >Specifies whether or not the vulnerability is publicly acknowledged by the vendor.</rdfs:comment>
    <rdfs:label >Publicly Acknowledge</rdfs:label>
    <rdfs:range rdf:resource="http://www.w3.org/2001/XMLSchema#boolean"/>
  </owl:DatatypeProperty>
  <owl:DatatypeProperty rdf:ID="references">
    <rdfs:range rdf:resource="http://www.w3.org/2001/XMLSchema#anyURI"/>
    <rdfs:domain rdf:resource="#Vulnerability"/>
    <rdfs:comment >Specifies a list of external references describing the vulnerability</rdfs:comment>
    <rdfs:label >References</rdfs:label>
  </owl:DatatypeProperty>
  <owl:DatatypeProperty rdf:ID="osvdbID">
    <rdfs:domain rdf:resource="#Vulnerability"/>
    <rdfs:comment >Specifies the OSVDB Identifier for a particular vulnerability</rdfs:comment>
    <rdfs:range rdf:resource="http://www.w3.org/2001/XMLSchema#string"/>
    <rdfs:label >OSVDB Identifier</rdfs:label>
  </owl:DatatypeProperty>
  <owl:DatatypeProperty rdf:ID="source">
    <rdfs:domain rdf:resource="#Vulnerability"/>
    <rdfs:comment >Specifies the source of the CVE or OSVDB as a textual description or URL</rdfs:comment>
    <rdfs:range rdf:resource="http://www.w3.org/2001/XMLSchema#string"/>
    <rdfs:label >Source</rdfs:label>
  </owl:DatatypeProperty>
  <rdf:Description rdf:about="http://stix.mitre.org/stixCommon#relatedExploitTarget">
    <rdfs:domain rdf:resource="#ExploitTarget"/>
  </rdf:Description>
  <rdf:Description rdf:about="http://stix.mitre.org/stixCommon#description">
    <rdfs:domain rdf:resource="#ConfigurationIssue"/>
    <rdfs:domain rdf:resource="#Weakness"/>
    <rdfs:domain rdf:resource="#Vulnerability"/>
    <rdfs:domain rdf:resource="#ExploitTarget"/>
  </rdf:Description>
  <rdf:Description rdf:about="http://stix.mitre.org/stixCommon#relatedPackages">
    <rdfs:domain rdf:resource="#ExploitTarget"/>
  </rdf:Description>
  <rdf:Description rdf:about="http://data-marking.mitre.org/Data_Marking#handling">
    <rdfs:domain rdf:resource="#ExploitTarget"/>
  </rdf:Description>
</rdf:RDF>

<!-- Created with TopBraid -->
