<?xml version="1.0"?>
<rdf:RDF xmlns="http://stix.mitre.org/Indicator#"
     xml:base="http://stix.mitre.org/Indicator"
     xmlns:indicator="http://stix.mitre.org/Indicator#"
     xmlns:stixCommon="http://stix.mitre.org/stixCommon#"
     xmlns:ciq_common="http://www.oasis-open.org/ciq_common#"
     xmlns:rdf="http://www.w3.org/1999/02/22-rdf-syntax-ns#"
     xmlns:owl="http://www.w3.org/2002/07/owl#"
     xmlns:xml="http://www.w3.org/XML/1998/namespace"
     xmlns:xsd="http://www.w3.org/2001/XMLSchema#"
     xmlns:rdfs="http://www.w3.org/2000/01/rdf-schema#"
     xmlns:data_marking="http://data-marking.mitre.org/Data_Marking#">
    <owl:Ontology rdf:about="http://stix.mitre.org/Indicator">
        <owl:versionIRI rdf:resource="http://stix.mitre.org/Indicator/1.2"/>
        <owl:imports rdf:resource="http://data-marking.mitre.org/Data_Marking"/>
        <owl:imports rdf:resource="http://www.oasis-open.org/ciq_common"/>
        <owl:imports rdf:resource="http://stix.mitre.org/stixCommon"/>
        <owl:imports rdf:resource="http://ioc.mandiant.com/IoC"/>
        <owl:versionInfo rdf:datatype="http://www.w3.org/2001/XMLSchema#string">1.2.0-000</owl:versionInfo>
        <rdfs:label>STIX Indicator Ontology</rdfs:label>
        <rdfs:comment>This ontology provides a vocabulary and representation for the Structured Threat Information eXpression (STIX) Indicator.  The STIX Indicator ontology provides a characterization of a single STIX Indicator.

A STIX Indicator conveys specific Observable patterns combined with contextual information intended to represent artifacts and/or behaviors of interest within a cyber security context. They consist of one or more Observable patterns potentially mapped to a related TTP context and adorned with other relevant metadata on things like confidence in the indicator’s assertion, handling restrictions, valid time windows, likely impact, sightings of the indicator, structured test mechanisms for detection, related campaigns, suggested courses of action, related indicators, the source of the Indicator, etc. Recognizing limitations in current standardized approaches of representation, STIX leverages community knowledge and best practices to define a new Indicator structure for representing Indicator information.</rdfs:comment>
    </owl:Ontology>
    


    <!-- 
    ///////////////////////////////////////////////////////////////////////////////////////
    //
    // Annotation properties
    //
    ///////////////////////////////////////////////////////////////////////////////////////
     -->

    


    <!-- http://data-marking.mitre.org/Data_Marking#handling -->

    <owl:AnnotationProperty rdf:about="http://data-marking.mitre.org/Data_Marking#handling">
        <rdfs:domain rdf:resource="http://stix.mitre.org/Indicator#Indicator"/>
    </owl:AnnotationProperty>
    


    <!-- http://stix.mitre.org/stixCommon#confidence -->

    <owl:AnnotationProperty rdf:about="http://stix.mitre.org/stixCommon#confidence">
        <rdfs:domain rdf:resource="http://stix.mitre.org/Indicator#Indicator"/>
    </owl:AnnotationProperty>
    


    <!-- http://stix.mitre.org/stixCommon#lastModifiedDateTime -->

    <owl:AnnotationProperty rdf:about="http://stix.mitre.org/stixCommon#lastModifiedDateTime">
        <rdfs:domain rdf:resource="http://stix.mitre.org/Indicator#OpenIOCTestMechanism"/>
    </owl:AnnotationProperty>
    


    <!-- http://stix.mitre.org/stixCommon#parentId -->

    <owl:AnnotationProperty rdf:about="http://stix.mitre.org/stixCommon#parentId">
        <rdfs:domain rdf:resource="http://stix.mitre.org/Indicator#ValidTime"/>
    </owl:AnnotationProperty>
    


    <!-- http://stix.mitre.org/stixCommon#relatedCampaign -->

    <owl:AnnotationProperty rdf:about="http://stix.mitre.org/stixCommon#relatedCampaign">
        <rdfs:domain rdf:resource="http://stix.mitre.org/Indicator#Indicator"/>
    </owl:AnnotationProperty>
    


    <!-- http://stix.mitre.org/stixCommon#relatedIndicator -->

    <owl:AnnotationProperty rdf:about="http://stix.mitre.org/stixCommon#relatedIndicator">
        <rdfs:domain rdf:resource="http://stix.mitre.org/Indicator#Indicator"/>
    </owl:AnnotationProperty>
    


    <!-- http://stix.mitre.org/stixCommon#relatedObservable -->

    <owl:AnnotationProperty rdf:about="http://stix.mitre.org/stixCommon#relatedObservable">
        <rdfs:domain rdf:resource="http://stix.mitre.org/Indicator#Sighting"/>
    </owl:AnnotationProperty>
    


    <!-- http://stix.mitre.org/stixCommon#relatedPackages -->

    <owl:AnnotationProperty rdf:about="http://stix.mitre.org/stixCommon#relatedPackages">
        <rdfs:domain rdf:resource="http://stix.mitre.org/Indicator#Indicator"/>
    </owl:AnnotationProperty>
    


    <!-- http://stix.mitre.org/stixCommon#shortDescription -->

    <owl:AnnotationProperty rdf:about="http://stix.mitre.org/stixCommon#shortDescription">
        <rdfs:domain rdf:resource="http://stix.mitre.org/Indicator#Indicator"/>
    </owl:AnnotationProperty>
    


    <!-- http://stix.mitre.org/stixCommon#timestamp -->

    <owl:AnnotationProperty rdf:about="http://stix.mitre.org/stixCommon#timestamp">
        <rdfs:domain rdf:resource="http://stix.mitre.org/Indicator#Sighting"/>
    </owl:AnnotationProperty>
    


    <!-- http://stix.mitre.org/stixCommon#timestampPrecision -->

    <owl:AnnotationProperty rdf:about="http://stix.mitre.org/stixCommon#timestampPrecision">
        <rdfs:domain rdf:resource="http://stix.mitre.org/Indicator#Sighting"/>
    </owl:AnnotationProperty>
    


    <!-- http://stix.mitre.org/stixCommon#title -->

    <owl:AnnotationProperty rdf:about="http://stix.mitre.org/stixCommon#title">
        <rdfs:domain rdf:resource="http://stix.mitre.org/Indicator#Indicator"/>
    </owl:AnnotationProperty>
    


    <!-- http://www.oasis-open.org/ciq_common#status -->

    <owl:AnnotationProperty rdf:about="http://www.oasis-open.org/ciq_common#status">
        <rdfs:domain rdf:resource="http://stix.mitre.org/stixCommon#IndicatorBase"/>
    </owl:AnnotationProperty>
    


    <!-- http://www.oasis-open.org/ciq_common#validFromDateTime -->

    <owl:AnnotationProperty rdf:about="http://www.oasis-open.org/ciq_common#validFromDateTime">
        <rdfs:domain rdf:resource="http://stix.mitre.org/stixCommon#IndicatorBase"/>
    </owl:AnnotationProperty>
    


    <!-- http://www.oasis-open.org/ciq_common#validToDateTime -->

    <owl:AnnotationProperty rdf:about="http://www.oasis-open.org/ciq_common#validToDateTime">
        <rdfs:domain rdf:resource="http://stix.mitre.org/stixCommon#IndicatorBase"/>
    </owl:AnnotationProperty>
    


    <!-- http://www.w3.org/2002/07/owl#cardinality -->

    <owl:AnnotationProperty rdf:about="http://www.w3.org/2002/07/owl#cardinality"/>
    


    <!-- http://www.w3.org/2002/07/owl#maxCardinality -->

    <owl:AnnotationProperty rdf:about="http://www.w3.org/2002/07/owl#maxCardinality"/>
    


    <!-- http://www.w3.org/2002/07/owl#minCardinality -->

    <owl:AnnotationProperty rdf:about="http://www.w3.org/2002/07/owl#minCardinality"/>
    


    <!-- 
    ///////////////////////////////////////////////////////////////////////////////////////
    //
    // Object Properties
    //
    ///////////////////////////////////////////////////////////////////////////////////////
     -->

    


    <!-- http://stix.mitre.org/Indicator#efficacy -->

    <owl:ObjectProperty rdf:about="http://stix.mitre.org/Indicator#efficacy">
        <rdfs:domain rdf:resource="http://stix.mitre.org/Indicator#TestMechanism"/>
        <rdfs:range rdf:resource="http://stix.mitre.org/stixCommon#EfficacyStatement"/>
        <rdfs:comment>Specifies an assertion of likely effectiveness of this TestMechanism to detect the targeted cyber Observables. 

The field includes a description of the asserted efficacy of this TestMechanism and a confidence held in the asserted efficacy of this TestMechanism to detect the targeted cyber Observables.</rdfs:comment>
        <rdfs:isDefinedBy rdf:resource="http://stix.mitre.org/Indicator"/>
        <rdfs:label>Efficacy</rdfs:label>
    </owl:ObjectProperty>
    


    <!-- http://stix.mitre.org/Indicator#eventFilter -->

    <owl:ObjectProperty rdf:about="http://stix.mitre.org/Indicator#eventFilter">
        <rdfs:domain rdf:resource="http://stix.mitre.org/Indicator#SnortTestMechanism"/>
        <rdfs:range rdf:resource="http://stix.mitre.org/stixCommon#EncodedCDATA"/>
        <rdfs:comment>Specifies a reference to a Snort event filter line in its native format.

The specification should be within a CDATA construct.</rdfs:comment>
        <rdfs:isDefinedBy rdf:resource="http://stix.mitre.org/Indicator"/>
        <rdfs:label>Event Filter</rdfs:label>
    </owl:ObjectProperty>
    


    <!-- http://stix.mitre.org/Indicator#eventSuppression -->

    <owl:ObjectProperty rdf:about="http://stix.mitre.org/Indicator#eventSuppression">
        <rdfs:domain rdf:resource="http://stix.mitre.org/Indicator#SnortTestMechanism"/>
        <rdfs:range rdf:resource="http://stix.mitre.org/stixCommon#EncodedCDATA"/>
        <rdfs:comment>Specifies a reference to a Snort event suppression line in its native format. 

The specification should be within a CDATA construct.</rdfs:comment>
        <rdfs:isDefinedBy rdf:resource="http://stix.mitre.org/Indicator"/>
        <rdfs:label>Event Suppression</rdfs:label>
    </owl:ObjectProperty>
    


    <!-- http://stix.mitre.org/Indicator#indicatedTTP -->

    <owl:ObjectProperty rdf:about="http://stix.mitre.org/Indicator#indicatedTTP">
        <rdfs:domain rdf:resource="http://stix.mitre.org/Indicator#Indicator"/>
        <rdfs:range rdf:resource="http://stix.mitre.org/stixCommon#TTPBase"/>
        <rdfs:comment>Specifies a reference to the relevant TTP indicated by this Indicator.</rdfs:comment>
        <rdfs:isDefinedBy rdf:resource="http://stix.mitre.org/Indicator"/>
        <rdfs:label>Indicated TTP</rdfs:label>
    </owl:ObjectProperty>
    


    <!-- http://stix.mitre.org/Indicator#indicator -->

    <owl:ObjectProperty rdf:about="http://stix.mitre.org/Indicator#indicator">
        <rdfs:domain rdf:resource="http://stix.mitre.org/Indicator#CompositeIndicator"/>
        <rdfs:range rdf:resource="http://stix.mitre.org/Indicator#Indicator"/>
        <rdfs:comment>Specifies a reference to one cyber threat indicator made up of a pattern identifying certain observable conditions as well as contextual information about the patterns meaning, how and when it should be acted on, etc.</rdfs:comment>
        <rdfs:isDefinedBy rdf:resource="http://stix.mitre.org/Indicator"/>
        <rdfs:label>Indicator</rdfs:label>
    </owl:ObjectProperty>
    


    <!-- http://stix.mitre.org/Indicator#iocIndicator -->

    <owl:ObjectProperty rdf:about="http://stix.mitre.org/Indicator#iocIndicator">
        <rdfs:domain rdf:resource="http://stix.mitre.org/Indicator#OpenIOCTestMechanism"/>
        <rdfs:range rdf:resource="http://ioc.mandiant.com/IoC#IndicatorOfCompromise"/>
        <rdfs:comment>Specifies a reference to the OpenIOC Indicator of Compromise</rdfs:comment>
        <rdfs:isDefinedBy rdf:resource="http://stix.mitre.org/Indicator"/>
        <rdfs:label>OpenIOC Indicator</rdfs:label>
    </owl:ObjectProperty>
    


    <!-- http://stix.mitre.org/Indicator#killchainPhases -->

    <owl:ObjectProperty rdf:about="http://stix.mitre.org/Indicator#killchainPhases">
        <rdfs:domain rdf:resource="http://stix.mitre.org/Indicator#Indicator"/>
        <rdfs:range rdf:resource="http://stix.mitre.org/stixCommon#KillChainPhase"/>
        <rdfs:comment>Specifies a reference to a relevant kill chain phases relevant to the Indicator.</rdfs:comment>
        <rdfs:isDefinedBy rdf:resource="http://stix.mitre.org/Indicator"/>
        <rdfs:label>Kill Chain Phases</rdfs:label>
    </owl:ObjectProperty>
    


    <!-- http://stix.mitre.org/Indicator#likelyImpact -->

    <owl:ObjectProperty rdf:about="http://stix.mitre.org/Indicator#likelyImpact">
        <rdfs:domain rdf:resource="http://stix.mitre.org/Indicator#Indicator"/>
        <rdfs:range rdf:resource="http://stix.mitre.org/stixCommon#LikelyImpactStatement"/>
        <rdfs:comment>Specifies a reference to a characterization of the likely potential impact within the relevant context if this Indicator were to occur.</rdfs:comment>
        <rdfs:isDefinedBy rdf:resource="http://stix.mitre.org/Indicator"/>
        <rdfs:label>Likely Impact</rdfs:label>
    </owl:ObjectProperty>
    


    <!-- http://stix.mitre.org/Indicator#observation -->

    <owl:ObjectProperty rdf:about="http://stix.mitre.org/Indicator#observation">
        <rdfs:domain rdf:resource="http://stix.mitre.org/Indicator#Indicator"/>
        <rdfs:range>
            <owl:Class>
                <owl:unionOf rdf:parseType="Collection">
                    <rdf:Description rdf:about="http://cybox.mitre.org/cybox_core#Observable"/>
                    <rdf:Description rdf:about="http://stix.mitre.org/Indicator#CompositeIndicator"/>
                </owl:unionOf>
            </owl:Class>
        </rdfs:range>
        <rdfs:comment>Specifies a relevant cyber observable or a multi-part composite Indicator for this Indicator.</rdfs:comment>
        <rdfs:isDefinedBy rdf:resource="http://stix.mitre.org/Indicator"/>
        <rdfs:label>Observation</rdfs:label>
    </owl:ObjectProperty>
    


    <!-- http://stix.mitre.org/Indicator#ovalDefinitions -->

    <owl:ObjectProperty rdf:about="http://stix.mitre.org/Indicator#ovalDefinitions">
        <rdfs:domain rdf:resource="http://stix.mitre.org/Indicator#OVALTestMechanism"/>
        <rdfs:comment>Specifies a reference to one or more OVAL Definitions.</rdfs:comment>
        <rdfs:isDefinedBy rdf:resource="http://stix.mitre.org/Indicator"/>
        <rdfs:label>OVAL Definitions</rdfs:label>
    </owl:ObjectProperty>
    


    <!-- http://stix.mitre.org/Indicator#ovalDefinitionsGenerator -->

    <owl:ObjectProperty rdf:about="http://stix.mitre.org/Indicator#ovalDefinitionsGenerator">
        <rdfs:domain rdf:resource="http://stix.mitre.org/Indicator#OVALTestMechanism"/>
        <rdfs:range rdf:resource="http://stix.mitre.org/stixCommon#ToolInformation"/>
        <rdfs:comment>Specifies a reference to information about when the OVAL Definition file was compiled and under what version.</rdfs:comment>
        <rdfs:isDefinedBy rdf:resource="http://stix.mitre.org/Indicator"/>
        <rdfs:label>OVAL Definitions Generator</rdfs:label>
    </owl:ObjectProperty>
    


    <!-- http://stix.mitre.org/Indicator#ovalDefinitionsObjects -->

    <owl:ObjectProperty rdf:about="http://stix.mitre.org/Indicator#ovalDefinitionsObjects">
        <rdfs:domain rdf:resource="http://stix.mitre.org/Indicator#OVALTestMechanism"/>
        <rdfs:comment>Specifies a reference to one or more OVAL Definition objects.</rdfs:comment>
        <rdfs:isDefinedBy rdf:resource="http://stix.mitre.org/Indicator"/>
        <rdfs:label>OVAL Definitions Objects</rdfs:label>
    </owl:ObjectProperty>
    


    <!-- http://stix.mitre.org/Indicator#ovalDefinitionsStates -->

    <owl:ObjectProperty rdf:about="http://stix.mitre.org/Indicator#ovalDefinitionsStates">
        <rdfs:domain rdf:resource="http://stix.mitre.org/Indicator#OVALTestMechanism"/>
        <rdfs:comment>Specifies a reference to one or more OVAL Definition States</rdfs:comment>
        <rdfs:isDefinedBy rdf:resource="http://stix.mitre.org/Indicator"/>
        <rdfs:label>OVAL Definitions States</rdfs:label>
    </owl:ObjectProperty>
    


    <!-- http://stix.mitre.org/Indicator#ovalDefinitionsTests -->

    <owl:ObjectProperty rdf:about="http://stix.mitre.org/Indicator#ovalDefinitionsTests">
        <rdfs:domain rdf:resource="http://stix.mitre.org/Indicator#OVALTestMechanism"/>
        <rdfs:comment>Specifies a reference to one or more OVAL Definition Tests</rdfs:comment>
        <rdfs:isDefinedBy rdf:resource="http://stix.mitre.org/Indicator"/>
        <rdfs:label>OVAL Definitions Test</rdfs:label>
    </owl:ObjectProperty>
    


    <!-- http://stix.mitre.org/Indicator#ovalDefinitionsVariables -->

    <owl:ObjectProperty rdf:about="http://stix.mitre.org/Indicator#ovalDefinitionsVariables">
        <rdfs:domain rdf:resource="http://stix.mitre.org/Indicator#OVALTestMechanism"/>
        <rdfs:comment>Specifies a reference to one or more OVAL Definition Varaibles</rdfs:comment>
        <rdfs:isDefinedBy rdf:resource="http://stix.mitre.org/Indicator"/>
        <rdfs:label>OVAL Definitions Variables</rdfs:label>
    </owl:ObjectProperty>
    


    <!-- http://stix.mitre.org/Indicator#ovalVariables -->

    <owl:ObjectProperty rdf:about="http://stix.mitre.org/Indicator#ovalVariables">
        <rdfs:domain rdf:resource="http://stix.mitre.org/Indicator#OVALTestMechanism"/>
        <rdfs:comment>Specifies a reference to a valid OVAL Variables document.

This SHOULD only be used to supply external variable values needed by this OVAL Test Mechanism&apos;s OVAL Definitions.</rdfs:comment>
        <rdfs:isDefinedBy rdf:resource="http://stix.mitre.org/Indicator"/>
        <rdfs:label>OVAL Variables</rdfs:label>
    </owl:ObjectProperty>
    


    <!-- http://stix.mitre.org/Indicator#ovalVariablesGenerator -->

    <owl:ObjectProperty rdf:about="http://stix.mitre.org/Indicator#ovalVariablesGenerator">
        <rdfs:domain rdf:resource="http://stix.mitre.org/Indicator#OVALTestMechanism"/>
        <rdfs:range rdf:resource="http://stix.mitre.org/stixCommon#ToolInformation"/>
        <rdfs:comment>Specifies a reference to information about when the variables file was compiled and under what version.</rdfs:comment>
        <rdfs:isDefinedBy rdf:resource="http://stix.mitre.org/Indicator"/>
        <rdfs:label>OVAL Variables Generator</rdfs:label>
    </owl:ObjectProperty>
    


    <!-- http://stix.mitre.org/Indicator#producer -->

    <owl:ObjectProperty rdf:about="http://stix.mitre.org/Indicator#producer">
        <rdfs:domain rdf:resource="http://stix.mitre.org/Indicator#Indicator"/>
        <rdfs:domain rdf:resource="http://stix.mitre.org/Indicator#TestMechanism"/>
        <rdfs:range rdf:resource="http://stix.mitre.org/stixCommon#InformationSource"/>
        <rdfs:comment>Specifies a reference to the source of this entry.</rdfs:comment>
        <rdfs:isDefinedBy rdf:resource="http://stix.mitre.org/Indicator"/>
        <rdfs:label>Producer</rdfs:label>
    </owl:ObjectProperty>
    


    <!-- http://stix.mitre.org/Indicator#rateFilter -->

    <owl:ObjectProperty rdf:about="http://stix.mitre.org/Indicator#rateFilter">
        <rdfs:domain rdf:resource="http://stix.mitre.org/Indicator#SnortTestMechanism"/>
        <rdfs:range>
            <owl:Class>
                <owl:unionOf rdf:parseType="Collection">
                    <rdf:Description rdf:about="http://www.w3.org/2001/XMLSchema#base64Binary"/>
                    <rdf:Description rdf:about="http://www.w3.org/2001/XMLSchema#string"/>
                </owl:unionOf>
            </owl:Class>
        </rdfs:range>
    </owl:ObjectProperty>
    


    <!-- http://stix.mitre.org/Indicator#sightingConfidence -->

    <owl:ObjectProperty rdf:about="http://stix.mitre.org/Indicator#sightingConfidence">
        <rdfs:domain rdf:resource="http://stix.mitre.org/Indicator#Sighting"/>
        <rdfs:range rdf:resource="http://stix.mitre.org/stixCommon#Confidence"/>
        <rdfs:comment>Specifies a reference to a confidence assertion in the accuracy of this sighting.</rdfs:comment>
        <rdfs:isDefinedBy rdf:resource="http://stix.mitre.org/Indicator"/>
        <rdfs:label>Sighting Confidence</rdfs:label>
    </owl:ObjectProperty>
    


    <!-- http://stix.mitre.org/Indicator#sightingSource -->

    <owl:ObjectProperty rdf:about="http://stix.mitre.org/Indicator#sightingSource">
        <rdfs:domain rdf:resource="http://stix.mitre.org/Indicator#Sighting"/>
        <rdfs:range rdf:resource="http://stix.mitre.org/stixCommon#InformationSource"/>
        <rdfs:comment>Specifies a reference to the source of the sighting</rdfs:comment>
        <rdfs:isDefinedBy rdf:resource="http://stix.mitre.org/Indicator"/>
        <rdfs:label>Sighting Source</rdfs:label>
    </owl:ObjectProperty>
    


    <!-- http://stix.mitre.org/Indicator#sightings -->

    <owl:ObjectProperty rdf:about="http://stix.mitre.org/Indicator#sightings">
        <rdfs:domain rdf:resource="http://stix.mitre.org/Indicator#Indicator"/>
        <rdfs:range rdf:resource="http://stix.mitre.org/Indicator#Sighting"/>
        <rdfs:comment>Specifies a reference to one or more sighting reports for this Indicator.</rdfs:comment>
        <rdfs:isDefinedBy rdf:resource="http://stix.mitre.org/Indicator"/>
        <rdfs:label>Sightings</rdfs:label>
    </owl:ObjectProperty>
    


    <!-- http://stix.mitre.org/Indicator#snortRule -->

    <owl:ObjectProperty rdf:about="http://stix.mitre.org/Indicator#snortRule">
        <rdfs:domain rdf:resource="http://stix.mitre.org/Indicator#SnortTestMechanism"/>
        <rdfs:range>
            <owl:Class>
                <owl:unionOf rdf:parseType="Collection">
                    <rdf:Description rdf:about="http://www.w3.org/2001/XMLSchema#base64Binary"/>
                    <rdf:Description rdf:about="http://www.w3.org/2001/XMLSchema#string"/>
                </owl:unionOf>
            </owl:Class>
        </rdfs:range>
    </owl:ObjectProperty>
    


    <!-- http://stix.mitre.org/Indicator#specification -->

    <owl:ObjectProperty rdf:about="http://stix.mitre.org/Indicator#specification">
        <rdfs:domain rdf:resource="http://stix.mitre.org/Indicator#GenericTestMechanism"/>
        <rdfs:range>
            <owl:Class>
                <owl:unionOf rdf:parseType="Collection">
                    <rdf:Description rdf:about="http://www.w3.org/2001/XMLSchema#base64Binary"/>
                    <rdf:Description rdf:about="http://www.w3.org/2001/XMLSchema#string"/>
                </owl:unionOf>
            </owl:Class>
        </rdfs:range>
    </owl:ObjectProperty>
    


    <!-- http://stix.mitre.org/Indicator#suggestedCOAs -->

    <owl:ObjectProperty rdf:about="http://stix.mitre.org/Indicator#suggestedCOAs">
        <rdfs:domain rdf:resource="http://stix.mitre.org/Indicator#Indicator"/>
        <rdfs:range rdf:resource="http://stix.mitre.org/stixCommon#CourseOfActionBase"/>
        <rdfs:comment>Specifies a reference to suggested Courses of Action relevant for this cyber threat Indicator.</rdfs:comment>
        <rdfs:isDefinedBy rdf:resource="http://stix.mitre.org/Indicator"/>
        <rdfs:label>Suggested COAs</rdfs:label>
    </owl:ObjectProperty>
    


    <!-- http://stix.mitre.org/Indicator#testMechanisms -->

    <owl:ObjectProperty rdf:about="http://stix.mitre.org/Indicator#testMechanisms">
        <rdfs:domain rdf:resource="http://stix.mitre.org/Indicator#Indicator"/>
        <rdfs:range rdf:resource="http://stix.mitre.org/Indicator#TestMechanism"/>
        <rdfs:comment>Specifies a reference to one or more Test Mechanisms effective at identifying the cyber Observables specified in this cyber threat Indicator.</rdfs:comment>
        <rdfs:isDefinedBy rdf:resource="http://stix.mitre.org/Indicator"/>
        <rdfs:label>Test Mechanisms</rdfs:label>
    </owl:ObjectProperty>
    


    <!-- http://stix.mitre.org/Indicator#tool -->

    <owl:ObjectProperty rdf:about="http://stix.mitre.org/Indicator#tool">
        <rdfs:domain rdf:resource="http://stix.mitre.org/Indicator#SnortTestMechanism"/>
        <rdfs:range rdf:resource="http://stix.mitre.org/stixCommon#ToolInformation"/>
        <rdfs:comment>Specifies a reference to the Common Platform Enumeration (CPE) Name for the product</rdfs:comment>
        <rdfs:isDefinedBy rdf:resource="http://stix.mitre.org/Indicator"/>
        <rdfs:label>Snort Tool</rdfs:label>
    </owl:ObjectProperty>
    


    <!-- http://stix.mitre.org/Indicator#validTimePosition -->

    <owl:ObjectProperty rdf:about="http://stix.mitre.org/Indicator#validTimePosition">
        <rdfs:domain rdf:resource="http://stix.mitre.org/Indicator#Indicator"/>
        <rdfs:range rdf:resource="http://stix.mitre.org/Indicator#ValidTime"/>
        <rdfs:comment>Specifies a reference to the time window for which this indicator is valid.</rdfs:comment>
        <rdfs:isDefinedBy rdf:resource="http://stix.mitre.org/Indicator"/>
        <rdfs:label>valid time position</rdfs:label>
    </owl:ObjectProperty>
    


    <!-- http://stix.mitre.org/Indicator#yaraRule -->

    <owl:ObjectProperty rdf:about="http://stix.mitre.org/Indicator#yaraRule">
        <rdfs:domain rdf:resource="http://stix.mitre.org/Indicator#YaraTestMechanism"/>
        <rdfs:range>
            <owl:Class>
                <owl:unionOf rdf:parseType="Collection">
                    <rdf:Description rdf:about="http://www.w3.org/2001/XMLSchema#base64Binary"/>
                    <rdf:Description rdf:about="http://www.w3.org/2001/XMLSchema#string"/>
                </owl:unionOf>
            </owl:Class>
        </rdfs:range>
    </owl:ObjectProperty>
    


    <!-- 
    ///////////////////////////////////////////////////////////////////////////////////////
    //
    // Data properties
    //
    ///////////////////////////////////////////////////////////////////////////////////////
     -->

    


    <!-- http://stix.mitre.org/Indicator#alternativeIdentifiers -->

    <owl:DatatypeProperty rdf:about="http://stix.mitre.org/Indicator#alternativeIdentifiers">
        <rdfs:domain rdf:resource="http://stix.mitre.org/Indicator#Indicator"/>
        <rdfs:range rdf:resource="http://www.w3.org/2001/XMLSchema#string"/>
        <rdfs:comment>Specifies an alternative identifier (or alias) for the cyber threat Indicator.</rdfs:comment>
        <rdfs:isDefinedBy rdf:resource="http://stix.mitre.org/Indicator"/>
        <rdfs:label>Alternative Identifiers</rdfs:label>
    </owl:DatatypeProperty>
    


    <!-- http://stix.mitre.org/Indicator#indicatorID -->

    <owl:DatatypeProperty rdf:about="http://stix.mitre.org/Indicator#indicatorID">
        <rdfs:domain rdf:resource="http://stix.mitre.org/Indicator#OpenIOCTestMechanism"/>
        <rdfs:range rdf:resource="http://www.w3.org/2001/XMLSchema#string"/>
        <rdfs:comment>Specifies the identifier for the OpenIOC Indicator of Compromise</rdfs:comment>
        <rdfs:isDefinedBy rdf:resource="http://stix.mitre.org/Indicator"/>
        <rdfs:label>OpenIOC Indicator ID</rdfs:label>
    </owl:DatatypeProperty>
    


    <!-- http://stix.mitre.org/Indicator#indicatorPattern -->

    <owl:DatatypeProperty rdf:about="http://stix.mitre.org/Indicator#indicatorPattern">
        <rdfs:domain rdf:resource="http://stix.mitre.org/Indicator#Indicator"/>
        <rdfs:range rdf:resource="http://www.w3.org/2001/XMLSchema#boolean"/>
        <rdfs:comment>Specifies whether the indicator&apos;s observables are for an observable instance or an observable pattern.</rdfs:comment>
        <rdfs:isDefinedBy rdf:resource="http://stix.mitre.org/Indicator"/>
        <rdfs:label>Indicator Pattern</rdfs:label>
    </owl:DatatypeProperty>
    


    <!-- http://stix.mitre.org/Indicator#indicatorType -->

    <owl:DatatypeProperty rdf:about="http://stix.mitre.org/Indicator#indicatorType">
        <rdfs:domain rdf:resource="http://stix.mitre.org/Indicator#Indicator"/>
        <rdfs:range rdf:resource="http://www.w3.org/2001/XMLSchema#string"/>
        <rdfs:comment>Specifies the type or types for this Indicator. 

Examples of types of indicators include malicious e-mail, URL watchlist, and malware artifacts (these specific values are only provided to help explainthe property: they are neither recommended values nor necessarily part of any existing vocabulary).  The content creator may choose any arbitrary value or may constrain the set of possible values by referencing an externally-defined vocabulary or leveraging a formally defined vocabulary.

By default, the Indicator Type Vocabulary is used to defined a restricted set of values.</rdfs:comment>
        <rdfs:isDefinedBy rdf:resource="http://stix.mitre.org/Indicator"/>
        <rdfs:label>Indicator Type</rdfs:label>
    </owl:DatatypeProperty>
    


    <!-- http://stix.mitre.org/Indicator#operator -->

    <owl:DatatypeProperty rdf:about="http://stix.mitre.org/Indicator#operator">
        <rdfs:domain rdf:resource="http://stix.mitre.org/Indicator#CompositeIndicator"/>
        <rdfs:range>
            <rdfs:Datatype>
                <owl:oneOf>
                    <rdf:Description>
                        <rdf:type rdf:resource="http://www.w3.org/1999/02/22-rdf-syntax-ns#List"/>
                        <rdf:first rdf:datatype="http://www.w3.org/2001/XMLSchema#string">AND</rdf:first>
                        <rdf:rest>
                            <rdf:Description>
                                <rdf:type rdf:resource="http://www.w3.org/1999/02/22-rdf-syntax-ns#List"/>
                                <rdf:first rdf:datatype="http://www.w3.org/2001/XMLSchema#string">OR</rdf:first>
                                <rdf:rest rdf:resource="http://www.w3.org/1999/02/22-rdf-syntax-ns#nil"/>
                            </rdf:Description>
                        </rdf:rest>
                    </rdf:Description>
                </owl:oneOf>
            </rdfs:Datatype>
        </rdfs:range>
        <rdfs:comment>Specifies the logical composition operator for this composite cyber threat Indicator.</rdfs:comment>
        <rdfs:isDefinedBy rdf:resource="http://stix.mitre.org/Indicator"/>
        <rdfs:label>Operator</rdfs:label>
    </owl:DatatypeProperty>
    


    <!-- http://stix.mitre.org/Indicator#ovalDefinitionsTimestamp -->

    <owl:DatatypeProperty rdf:about="http://stix.mitre.org/Indicator#ovalDefinitionsTimestamp">
        <rdfs:domain rdf:resource="http://stix.mitre.org/Indicator#OVALTestMechanism"/>
        <rdfs:range rdf:resource="http://www.w3.org/2001/XMLSchema#dateTime"/>
        <rdfs:comment>Specifies when the particular OVAL document was compiled.

Note that the timestamp element does not specify when a definition (or set of definitions) was created or modified but rather when the actual document that contains the definition was created. For example, the document might have pulled a bunch of existing OVAL Definitions together, each of the definitions having been created at some point in the past. The timestamp in this case would be when the combined document was created</rdfs:comment>
        <rdfs:isDefinedBy rdf:resource="http://stix.mitre.org/Indicator"/>
        <rdfs:label>OVAL Definitions Timestamp</rdfs:label>
    </owl:DatatypeProperty>
    


    <!-- http://stix.mitre.org/Indicator#ovalVariablesTimestamp -->

    <owl:DatatypeProperty rdf:about="http://stix.mitre.org/Indicator#ovalVariablesTimestamp">
        <rdfs:domain rdf:resource="http://stix.mitre.org/Indicator#OVALTestMechanism"/>
        <rdfs:range rdf:resource="http://www.w3.org/2001/XMLSchema#dateTime"/>
        <rdfs:comment>Specifies when the particular OVAL document was compiled.

Note that the timestamp element does not specify when a varaible (or set of variables) was created or modified but rather when the actual document that contains the definition was created. For example, the document might have pulled a bunch of existing OVAL Variables together, each of the variables having been created at some point in the past. The timestamp in this case would be when the combined document was created</rdfs:comment>
        <rdfs:isDefinedBy rdf:resource="http://stix.mitre.org/Indicator"/>
        <rdfs:label>OVAL Variables Timestamp</rdfs:label>
    </owl:DatatypeProperty>
    


    <!-- http://stix.mitre.org/Indicator#productName -->

    <owl:DatatypeProperty rdf:about="http://stix.mitre.org/Indicator#productName">
        <rdfs:domain rdf:resource="http://stix.mitre.org/Indicator#SnortTestMechanism"/>
        <rdfs:range rdf:resource="http://www.w3.org/2001/XMLSchema#string"/>
        <rdfs:comment>Specifies the name of the Snort-compatible tool that the rules were written against.

If the tool has a CPE name, use of that name is suggested, otherwise a simple name like &quot;Snort&quot;, &quot;Suricata&quot;, or &quot;Sourcefire&quot; could be used.</rdfs:comment>
        <rdfs:isDefinedBy rdf:resource="http://stix.mitre.org/Indicator"/>
        <rdfs:label>Product Name</rdfs:label>
    </owl:DatatypeProperty>
    


    <!-- http://stix.mitre.org/Indicator#rateFilter -->

    <owl:DatatypeProperty rdf:about="http://stix.mitre.org/Indicator#rateFilter"/>
    


    <!-- http://stix.mitre.org/Indicator#reference -->

    <owl:DatatypeProperty rdf:about="http://stix.mitre.org/Indicator#reference">
        <rdfs:domain rdf:resource="http://stix.mitre.org/Indicator#Sighting"/>
        <rdfs:range rdf:resource="http://www.w3.org/2001/XMLSchema#anyURI"/>
        <rdfs:comment>Specifies a formal reference to the sighting source.</rdfs:comment>
        <rdfs:isDefinedBy rdf:resource="http://stix.mitre.org/Indicator"/>
        <rdfs:label>Source Reference</rdfs:label>
    </owl:DatatypeProperty>
    


    <!-- http://stix.mitre.org/Indicator#referenceLocation -->

    <owl:DatatypeProperty rdf:about="http://stix.mitre.org/Indicator#referenceLocation">
        <rdfs:domain rdf:resource="http://stix.mitre.org/Indicator#GenericTestMechanism"/>
        <rdfs:range rdf:resource="http://www.w3.org/2001/XMLSchema#anyURI"/>
        <rdfs:comment>Specifies a reference URL for the location of the Generic Test Mechanism.</rdfs:comment>
        <rdfs:isDefinedBy rdf:resource="http://stix.mitre.org/Indicator"/>
        <rdfs:label>Reference Location</rdfs:label>
    </owl:DatatypeProperty>
    


    <!-- http://stix.mitre.org/Indicator#sightingsCount -->

    <owl:DatatypeProperty rdf:about="http://stix.mitre.org/Indicator#sightingsCount">
        <rdfs:domain rdf:resource="http://stix.mitre.org/Indicator#Indicator"/>
        <rdfs:range rdf:resource="http://www.w3.org/2001/XMLSchema#integer"/>
        <rdfs:comment>Specifies the total number of times this Indicator was reported as sighted.</rdfs:comment>
        <rdfs:isDefinedBy rdf:resource="http://stix.mitre.org/Indicator"/>
        <rdfs:label>Sightings Count</rdfs:label>
    </owl:DatatypeProperty>
    


    <!-- http://stix.mitre.org/Indicator#snortRule -->

    <owl:DatatypeProperty rdf:about="http://stix.mitre.org/Indicator#snortRule"/>
    


    <!-- http://stix.mitre.org/Indicator#specification -->

    <owl:DatatypeProperty rdf:about="http://stix.mitre.org/Indicator#specification"/>
    


    <!-- http://stix.mitre.org/Indicator#testMechanismType -->

    <owl:DatatypeProperty rdf:about="http://stix.mitre.org/Indicator#testMechanismType">
        <rdfs:domain rdf:resource="http://stix.mitre.org/Indicator#GenericTestMechanism"/>
        <rdfs:range rdf:resource="http://www.w3.org/2001/XMLSchema#string"/>
        <rdfs:comment>Specifies the type of Generic Test Mechanism.</rdfs:comment>
        <rdfs:isDefinedBy rdf:resource="http://stix.mitre.org/Indicator"/>
        <rdfs:label>Type</rdfs:label>
    </owl:DatatypeProperty>
    


    <!-- http://stix.mitre.org/Indicator#validTime.endDateTime -->

    <owl:DatatypeProperty rdf:about="http://stix.mitre.org/Indicator#validTime.endDateTime">
        <rdfs:domain rdf:resource="http://stix.mitre.org/Indicator#ValidTime"/>
        <rdfs:range rdf:resource="http://www.w3.org/2001/XMLSchema#dateTime"/>
        <rdfs:comment>Specifies the ending of the time window for which this Indicator is valid. If not present, the valid time position of the indicator does not have an upper bound (i.e., temporal window is only bounded by the start-time).</rdfs:comment>
        <rdfs:isDefinedBy rdf:resource="http://stix.mitre.org/Indicator"/>
        <rdfs:label>Indicator Validity End</rdfs:label>
    </owl:DatatypeProperty>
    


    <!-- http://stix.mitre.org/Indicator#validTime.startDateTime -->

    <owl:DatatypeProperty rdf:about="http://stix.mitre.org/Indicator#validTime.startDateTime">
        <rdfs:domain rdf:resource="http://stix.mitre.org/Indicator#ValidTime"/>
        <rdfs:range rdf:resource="http://www.w3.org/2001/XMLSchema#dateTime"/>
        <rdfs:comment>Specifies the beginning of the time window for which this Indicator is valid.  If not present, the valid time position of the indicator does not have a lower bound (i.e., temporal window is only bounded by the end-time).</rdfs:comment>
        <rdfs:isDefinedBy rdf:resource="http://stix.mitre.org/Indicator"/>
        <rdfs:label>Indicator Validity Start</rdfs:label>
    </owl:DatatypeProperty>
    


    <!-- http://stix.mitre.org/Indicator#version -->

    <owl:DatatypeProperty rdf:about="http://stix.mitre.org/Indicator#version">
        <rdfs:domain rdf:resource="http://stix.mitre.org/Indicator#SnortTestMechanism"/>
        <rdfs:domain rdf:resource="http://stix.mitre.org/Indicator#YaraTestMechanism"/>
        <rdfs:range rdf:resource="http://www.w3.org/2001/XMLSchema#string"/>
        <rdfs:comment>Specifies the version of format or format-compatible tool that the rules were written against.</rdfs:comment>
        <rdfs:isDefinedBy rdf:resource="http://stix.mitre.org/Indicator"/>
        <rdfs:label>Version</rdfs:label>
    </owl:DatatypeProperty>
    


    <!-- http://stix.mitre.org/Indicator#yaraRule -->

    <owl:DatatypeProperty rdf:about="http://stix.mitre.org/Indicator#yaraRule"/>
    


    <!-- 
    ///////////////////////////////////////////////////////////////////////////////////////
    //
    // Classes
    //
    ///////////////////////////////////////////////////////////////////////////////////////
     -->

    

    <!-- http://stix.mitre.org/Indicator#CompositeIndicator -->

    <owl:Class rdf:about="http://stix.mitre.org/Indicator#CompositeIndicator">
        <rdfs:subClassOf>
            <owl:Restriction>
                <owl:onProperty rdf:resource="http://stix.mitre.org/Indicator#operator"/>
                <owl:cardinality rdf:datatype="http://www.w3.org/2001/XMLSchema#nonNegativeInteger">1</owl:cardinality>
            </owl:Restriction>
        </rdfs:subClassOf>
        <rdfs:comment>Characterizes a composite Indicator expression through the specification of a single operator (the operator of the expression) and zero or more Indicators (the operands of the expression).</rdfs:comment>
        <rdfs:isDefinedBy rdf:resource="http://stix.mitre.org/Indicator"/>
        <rdfs:label>Composite Indicator</rdfs:label>
    </owl:Class>
    


    <!-- http://stix.mitre.org/Indicator#GenericTestMechanism -->

    <owl:Class rdf:about="http://stix.mitre.org/Indicator#GenericTestMechanism">
        <rdfs:subClassOf rdf:resource="http://stix.mitre.org/Indicator#TestMechanism"/>
        <rdfs:subClassOf>
            <owl:Restriction>
                <owl:onProperty rdf:resource="http://stix.mitre.org/Indicator#specification"/>
                <owl:cardinality rdf:datatype="http://www.w3.org/2001/XMLSchema#nonNegativeInteger">1</owl:cardinality>
            </owl:Restriction>
        </rdfs:subClassOf>
        <rdfs:subClassOf>
            <owl:Restriction>
                <owl:onProperty rdf:resource="http://stix.mitre.org/Indicator#testMechanismType"/>
                <owl:cardinality rdf:datatype="http://www.w3.org/2001/XMLSchema#nonNegativeInteger">1</owl:cardinality>
            </owl:Restriction>
        </rdfs:subClassOf>
        <rdfs:subClassOf>
            <owl:Restriction>
                <owl:onProperty rdf:resource="http://stix.mitre.org/Indicator#referenceLocation"/>
                <owl:maxCardinality rdf:datatype="http://www.w3.org/2001/XMLSchema#nonNegativeInteger">1</owl:maxCardinality>
            </owl:Restriction>
        </rdfs:subClassOf>
        <rdfs:comment>Characterizes an instantial extension test mechanism to support a generic test mechanism through the use of a raw data section.</rdfs:comment>
        <rdfs:isDefinedBy rdf:resource="http://stix.mitre.org/Indicator"/>
        <rdfs:label>Generic Test Mechanism</rdfs:label>
    </owl:Class>
    


    <!-- http://stix.mitre.org/Indicator#Indicator -->

    <owl:Class rdf:about="http://stix.mitre.org/Indicator#Indicator">
        <rdfs:subClassOf rdf:resource="http://stix.mitre.org/stixCommon#IndicatorBase"/>
        <rdfs:subClassOf>
            <owl:Restriction>
                <owl:onProperty rdf:resource="http://stix.mitre.org/Indicator#observation"/>
                <owl:maxCardinality rdf:datatype="http://www.w3.org/2001/XMLSchema#nonNegativeInteger">1</owl:maxCardinality>
            </owl:Restriction>
        </rdfs:subClassOf>
        <rdfs:subClassOf>
            <owl:Restriction>
                <owl:onProperty rdf:resource="http://stix.mitre.org/Indicator#producer"/>
                <owl:maxCardinality rdf:datatype="http://www.w3.org/2001/XMLSchema#nonNegativeInteger">1</owl:maxCardinality>
            </owl:Restriction>
        </rdfs:subClassOf>
        <rdfs:subClassOf>
            <owl:Restriction>
                <owl:onProperty rdf:resource="http://stix.mitre.org/Indicator#indicatorType"/>
                <owl:cardinality rdf:datatype="http://www.w3.org/2001/XMLSchema#nonNegativeInteger">1</owl:cardinality>
            </owl:Restriction>
        </rdfs:subClassOf>
        <rdfs:subClassOf>
            <owl:Restriction>
                <owl:onProperty rdf:resource="http://stix.mitre.org/Indicator#indicatorPattern"/>
                <owl:maxCardinality rdf:datatype="http://www.w3.org/2001/XMLSchema#nonNegativeInteger">1</owl:maxCardinality>
            </owl:Restriction>
        </rdfs:subClassOf>
        <rdfs:subClassOf>
            <owl:Restriction>
                <owl:onProperty rdf:resource="http://stix.mitre.org/Indicator#validTime.endDateTime"/>
                <owl:maxCardinality rdf:datatype="http://www.w3.org/2001/XMLSchema#nonNegativeInteger">1</owl:maxCardinality>
            </owl:Restriction>
        </rdfs:subClassOf>
        <rdfs:subClassOf>
            <owl:Restriction>
                <owl:onProperty rdf:resource="http://stix.mitre.org/Indicator#validTime.startDateTime"/>
                <owl:maxCardinality rdf:datatype="http://www.w3.org/2001/XMLSchema#nonNegativeInteger">1</owl:maxCardinality>
            </owl:Restriction>
        </rdfs:subClassOf>
        <rdfs:comment>Characterizes a single STIX Indicator.

A STIX Indicator characterizes a cyber threat indicator by capturing an asserted relationship between a pattern identifying certain observable conditions and a particular TTP likely in play if those observable conditions are seen, as well as contextual information about how and when it should be acted on and how it relates to other Indicators, Campaigns, and TTPs.

Indicators convey specific Observable patterns combined with contextual information intended to represent artifacts and/or behaviors of interest within a cyber security context. They consist of one or more Observable patterns potentially mapped to a related TTP context and adorned with other relevant metadata on things like confidence in the indicator’s assertion, handling restrictions, valid time windows, likely impact, sightings of the indicator, structured test mechanisms for detection, related campaigns, suggested courses of action, related indicators, the source of the Indicator, etc.</rdfs:comment>
        <rdfs:isDefinedBy rdf:resource="http://stix.mitre.org/Indicator"/>
        <rdfs:label>Indicator</rdfs:label>
    </owl:Class>
    


    <!-- http://stix.mitre.org/Indicator#OVALTestMechanism -->

    <owl:Class rdf:about="http://stix.mitre.org/Indicator#OVALTestMechanism">
        <rdfs:subClassOf rdf:resource="http://stix.mitre.org/Indicator#TestMechanism"/>
        <rdfs:subClassOf>
            <owl:Restriction>
                <owl:onProperty rdf:resource="http://stix.mitre.org/Indicator#ovalDefinitions"/>
                <owl:minCardinality rdf:datatype="http://www.w3.org/2001/XMLSchema#nonNegativeInteger">1</owl:minCardinality>
            </owl:Restriction>
        </rdfs:subClassOf>
        <rdfs:subClassOf>
            <owl:Restriction>
                <owl:onProperty rdf:resource="http://stix.mitre.org/Indicator#ovalDefinitionsGenerator"/>
                <owl:cardinality rdf:datatype="http://www.w3.org/2001/XMLSchema#nonNegativeInteger">1</owl:cardinality>
            </owl:Restriction>
        </rdfs:subClassOf>
        <rdfs:subClassOf>
            <owl:Restriction>
                <owl:onProperty rdf:resource="http://stix.mitre.org/Indicator#ovalVariables"/>
                <owl:maxCardinality rdf:datatype="http://www.w3.org/2001/XMLSchema#nonNegativeInteger">1</owl:maxCardinality>
            </owl:Restriction>
        </rdfs:subClassOf>
        <rdfs:subClassOf>
            <owl:Restriction>
                <owl:onProperty rdf:resource="http://stix.mitre.org/Indicator#ovalVariablesGenerator"/>
                <owl:maxCardinality rdf:datatype="http://www.w3.org/2001/XMLSchema#nonNegativeInteger">1</owl:maxCardinality>
            </owl:Restriction>
        </rdfs:subClassOf>
        <rdfs:subClassOf>
            <owl:Restriction>
                <owl:onProperty rdf:resource="http://stix.mitre.org/Indicator#ovalDefinitionsTimestamp"/>
                <owl:maxCardinality rdf:datatype="http://www.w3.org/2001/XMLSchema#nonNegativeInteger">1</owl:maxCardinality>
            </owl:Restriction>
        </rdfs:subClassOf>
        <rdfs:subClassOf>
            <owl:Restriction>
                <owl:onProperty rdf:resource="http://stix.mitre.org/Indicator#ovalVariablesTimestamp"/>
                <owl:maxCardinality rdf:datatype="http://www.w3.org/2001/XMLSchema#nonNegativeInteger">1</owl:maxCardinality>
            </owl:Restriction>
        </rdfs:subClassOf>
        <rdfs:comment>Characterizes an instantial extension test mechanism to provide support for the specification using OVAL Definitions.</rdfs:comment>
        <rdfs:isDefinedBy rdf:resource="http://stix.mitre.org/Indicator"/>
        <rdfs:label>OVAL Test Mechanism</rdfs:label>
    </owl:Class>
    


    <!-- http://stix.mitre.org/Indicator#OpenIOCTestMechanism -->

    <owl:Class rdf:about="http://stix.mitre.org/Indicator#OpenIOCTestMechanism">
        <rdfs:subClassOf rdf:resource="http://stix.mitre.org/Indicator#TestMechanism"/>
        <rdfs:subClassOf>
            <owl:Restriction>
                <owl:onProperty rdf:resource="http://stix.mitre.org/Indicator#iocIndicator"/>
                <owl:cardinality rdf:datatype="http://www.w3.org/2001/XMLSchema#nonNegativeInteger">1</owl:cardinality>
            </owl:Restriction>
        </rdfs:subClassOf>
        <rdfs:subClassOf>
            <owl:Restriction>
                <owl:onProperty rdf:resource="http://stix.mitre.org/Indicator#indicatorID"/>
                <owl:cardinality rdf:datatype="http://www.w3.org/2001/XMLSchema#nonNegativeInteger">1</owl:cardinality>
            </owl:Restriction>
        </rdfs:subClassOf>
        <rdfs:comment>Characterizes an instantial extension test mechanism to provide support for the specification using an OpenIOC test.</rdfs:comment>
        <rdfs:isDefinedBy rdf:resource="http://stix.mitre.org/Indicator"/>
        <rdfs:label>OpenIOC Test Mechanism</rdfs:label>
    </owl:Class>
    


    <!-- http://stix.mitre.org/Indicator#Sighting -->

    <owl:Class rdf:about="http://stix.mitre.org/Indicator#Sighting">
        <rdfs:subClassOf>
            <owl:Restriction>
                <owl:onProperty rdf:resource="http://stix.mitre.org/Indicator#sightingConfidence"/>
                <owl:maxCardinality rdf:datatype="http://www.w3.org/2001/XMLSchema#nonNegativeInteger">1</owl:maxCardinality>
            </owl:Restriction>
        </rdfs:subClassOf>
        <rdfs:subClassOf>
            <owl:Restriction>
                <owl:onProperty rdf:resource="http://stix.mitre.org/Indicator#sightingSource"/>
                <owl:maxCardinality rdf:datatype="http://www.w3.org/2001/XMLSchema#nonNegativeInteger">1</owl:maxCardinality>
            </owl:Restriction>
        </rdfs:subClassOf>
        <rdfs:comment>Characterizes a single sighting report of an indicator. 

An Indicator sighting report may capture a variety of information associated with an observable instance that matches the Indicator’s observable pattern including the time the sighting occurred, a textual description of the sighting, the set of Observables (instances) related to the sighting, the source of the sighting information (e.g., tool or an analyst name), and the level of confidence that the sighting information actually represents a sighting of that particular Indicator.</rdfs:comment>
        <rdfs:isDefinedBy rdf:resource="http://stix.mitre.org/Indicator"/>
        <rdfs:label>Sighting</rdfs:label>
    </owl:Class>
    


    <!-- http://stix.mitre.org/Indicator#SnortTestMechanism -->

    <owl:Class rdf:about="http://stix.mitre.org/Indicator#SnortTestMechanism">
        <rdfs:subClassOf rdf:resource="http://stix.mitre.org/Indicator#TestMechanism"/>
        <rdfs:subClassOf>
            <owl:Restriction>
                <owl:onProperty rdf:resource="http://stix.mitre.org/Indicator#tool"/>
                <owl:maxCardinality rdf:datatype="http://www.w3.org/2001/XMLSchema#nonNegativeInteger">1</owl:maxCardinality>
            </owl:Restriction>
        </rdfs:subClassOf>
        <rdfs:subClassOf>
            <owl:Restriction>
                <owl:onProperty rdf:resource="http://stix.mitre.org/Indicator#productName"/>
                <owl:maxCardinality rdf:datatype="http://www.w3.org/2001/XMLSchema#nonNegativeInteger">1</owl:maxCardinality>
            </owl:Restriction>
        </rdfs:subClassOf>
        <rdfs:subClassOf>
            <owl:Restriction>
                <owl:onProperty rdf:resource="http://stix.mitre.org/Indicator#version"/>
                <owl:maxCardinality rdf:datatype="http://www.w3.org/2001/XMLSchema#nonNegativeInteger">1</owl:maxCardinality>
            </owl:Restriction>
        </rdfs:subClassOf>
        <rdfs:comment>Characterizes an instantial extension test mechanism to provide support for the specification using Snort rules.</rdfs:comment>
        <rdfs:isDefinedBy rdf:resource="http://stix.mitre.org/Indicator"/>
        <rdfs:label>Snort Test Mechanism</rdfs:label>
    </owl:Class>
    


    <!-- http://stix.mitre.org/Indicator#TestMechanism -->

    <owl:Class rdf:about="http://stix.mitre.org/Indicator#TestMechanism">
        <rdfs:subClassOf>
            <owl:Restriction>
                <owl:onProperty rdf:resource="http://stix.mitre.org/Indicator#efficacy"/>
                <owl:maxCardinality rdf:datatype="http://www.w3.org/2001/XMLSchema#nonNegativeInteger">1</owl:maxCardinality>
            </owl:Restriction>
        </rdfs:subClassOf>
        <rdfs:subClassOf>
            <owl:Restriction>
                <owl:onProperty rdf:resource="http://stix.mitre.org/Indicator#producer"/>
                <owl:maxCardinality rdf:datatype="http://www.w3.org/2001/XMLSchema#nonNegativeInteger">1</owl:maxCardinality>
            </owl:Restriction>
        </rdfs:subClassOf>
        <rdfs:comment>Characterizes an alternative (non-CybOX) test mechanism effective at identifying the cyber Observables specified in this cyber threat Indicator. 

The TestMechanism class is an abstract class, so it MUST be extended via a subclass to enable the expression of any structured or unstructured test mechanism.

Test mechanisms may be different for different use cases. For example, one consumer may routinely rely on Snort signatures while another uses Yara rules and OVAL definitions. Individual test mechanisms are intended to test for the same conditions as the Observable (CybOX) patterns; however, STIX does not enforce equivalency.</rdfs:comment>
        <rdfs:isDefinedBy rdf:resource="http://stix.mitre.org/Indicator"/>
        <rdfs:label>Test Mechanism</rdfs:label>
    </owl:Class>
    


    <!-- http://stix.mitre.org/Indicator#ValidTime -->

    <owl:Class rdf:about="http://stix.mitre.org/Indicator#ValidTime">
        <rdfs:subClassOf>
            <owl:Restriction>
                <owl:onProperty rdf:resource="http://stix.mitre.org/Indicator#validTime.startDateTime"/>
                <owl:cardinality rdf:datatype="http://www.w3.org/2001/XMLSchema#nonNegativeInteger">1</owl:cardinality>
            </owl:Restriction>
        </rdfs:subClassOf>
        <rdfs:subClassOf>
            <owl:Restriction>
                <owl:onProperty rdf:resource="http://stix.mitre.org/Indicator#validTime.endDateTime"/>
                <owl:maxCardinality rdf:datatype="http://www.w3.org/2001/XMLSchema#nonNegativeInteger">1</owl:maxCardinality>
            </owl:Restriction>
        </rdfs:subClassOf>
        <rdfs:comment>Characterizes a temporal window during which the Indicator is able to accurately detect the TTP.</rdfs:comment>
        <rdfs:isDefinedBy rdf:resource="http://stix.mitre.org/Indicator"/>
        <rdfs:label>Valid Time Position</rdfs:label>
    </owl:Class>
    


    <!-- http://stix.mitre.org/Indicator#YaraTestMechanism -->

    <owl:Class rdf:about="http://stix.mitre.org/Indicator#YaraTestMechanism">
        <rdfs:subClassOf rdf:resource="http://stix.mitre.org/Indicator#TestMechanism"/>
        <rdfs:subClassOf>
            <owl:Restriction>
                <owl:onProperty rdf:resource="http://stix.mitre.org/Indicator#yaraRule"/>
                <owl:cardinality rdf:datatype="http://www.w3.org/2001/XMLSchema#nonNegativeInteger">1</owl:cardinality>
            </owl:Restriction>
        </rdfs:subClassOf>
        <rdfs:subClassOf>
            <owl:Restriction>
                <owl:onProperty rdf:resource="http://stix.mitre.org/Indicator#version"/>
                <owl:maxCardinality rdf:datatype="http://www.w3.org/2001/XMLSchema#nonNegativeInteger">1</owl:maxCardinality>
            </owl:Restriction>
        </rdfs:subClassOf>
        <rdfs:comment>Characterizes an instantial extension test mechanism to provide support for the specification using YARA rules.</rdfs:comment>
        <rdfs:isDefinedBy rdf:resource="http://stix.mitre.org/Indicator"/>
        <rdfs:label>YARA Test Mechanism</rdfs:label>
    </owl:Class>
    


    


    <!-- 
    ///////////////////////////////////////////////////////////////////////////////////////
    //
    // Annotations
    //
    ///////////////////////////////////////////////////////////////////////////////////////
     -->

    <rdf:Description rdf:about="http://stix.mitre.org/Indicator#rateFilter">
        <rdfs:isDefinedBy rdf:resource="http://stix.mitre.org/Indicator"/>
        <rdfs:label>Rate Filter</rdfs:label>
        <rdfs:comment>Specifies a Snort rate filter line in its native format. 

The specification should be within a CDATA construct.</rdfs:comment>
    </rdf:Description>
    <rdf:Description rdf:about="http://stix.mitre.org/Indicator#snortRule">
        <rdfs:comment>Specifies a Snort rule in its native format. 

The specification should be within a CDATA construct.</rdfs:comment>
        <rdfs:isDefinedBy rdf:resource="http://stix.mitre.org/Indicator"/>
        <rdfs:label>Snort Rule</rdfs:label>
    </rdf:Description>
    <rdf:Description rdf:about="http://stix.mitre.org/Indicator#specification">
        <rdfs:comment>Specifies any test mechnism specification in its native format. 

The specification should be within a CDATA construct.</rdfs:comment>
        <rdfs:isDefinedBy rdf:resource="http://stix.mitre.org/Indicator"/>
        <rdfs:label>specification</rdfs:label>
    </rdf:Description>
    <rdf:Description rdf:about="http://stix.mitre.org/Indicator#yaraRule">
        <rdfs:label>YARA Rule</rdfs:label>
        <rdfs:comment>Specifies a YARA rule in its native format. 

The specification should be within a CDATA construct.</rdfs:comment>
        <rdfs:isDefinedBy rdf:resource="http://stix.mitre.org/Indicator"/>
    </rdf:Description>
</rdf:RDF>



<!-- Generated by the OWL API (version 4.2.6.20160910-2108) https://github.com/owlcs/owlapi -->

