<?xml version="1.0"?>
<rdf:RDF xmlns="http://data-marking.mitre.org/Data_Marking#"
     xml:base="http://data-marking.mitre.org/Data_Marking"
     xmlns:marking="http://data-marking.mitre.org/Data_Marking#"
     xmlns:rdf="http://www.w3.org/1999/02/22-rdf-syntax-ns#"
     xmlns:owl="http://www.w3.org/2002/07/owl#"
     xmlns:xml="http://www.w3.org/XML/1998/namespace"
     xmlns:xsd="http://www.w3.org/2001/XMLSchema#"
     xmlns:ciq_xnl="http://www.oasis-open.org/ciq_xnl#"
     xmlns:wgs84_pos="http://www.w3.org/2003/01/geo/wgs84_pos#"
     xmlns:rdfs="http://www.w3.org/2000/01/rdf-schema#"
     xmlns:foaf="http://xmlns.com/foaf/0.1/"
     xmlns:dc="http://purl.org/dc/elements/1.1/">
    <owl:Ontology rdf:about="http://data-marking.mitre.org/Data_Marking">
        <owl:versionIRI rdf:resource="http://data-marking.mitre.org/Data_Marking/1.2"/>
        <owl:imports rdf:resource="http://stix.mitre.org/stixCommon"/>
        <rdfs:comment>This ontology provides a vocabulary and representation which provides a standardized method of describing data markings used to convey sensativity and the ability to share.</rdfs:comment>
        <owl:versionInfo rdf:datatype="http://www.w3.org/2001/XMLSchema#string">1.2.0-000</owl:versionInfo>
        <rdfs:label>Data Markings Ontology</rdfs:label>
    </owl:Ontology>
    


    <!-- 
    ///////////////////////////////////////////////////////////////////////////////////////
    //
    // Object Properties
    //
    ///////////////////////////////////////////////////////////////////////////////////////
     -->

    


    <!-- http://data-marking.mitre.org/Data_Marking#handling -->

    <owl:ObjectProperty rdf:about="http://data-marking.mitre.org/Data_Marking#handling">
        <rdfs:range>
            <owl:Class>
                <owl:unionOf rdf:parseType="Collection">
                    <rdf:Description rdf:about="http://data-marking.mitre.org/Data_Marking#SimpleMarking"/>
                    <rdf:Description rdf:about="http://data-marking.mitre.org/Data_Marking#TLPMarking"/>
                    <rdf:Description rdf:about="http://data-marking.mitre.org/Data_Marking#TermsOfUseMarking"/>
                </owl:unionOf>
            </owl:Class>
        </rdfs:range>
        <rdfs:comment>Specifies the appropriate data handling markings for the elements of this entity&apos;s characterization.</rdfs:comment>
        <rdfs:isDefinedBy rdf:resource="http://data-marking.mitre.org/Data_Marking"/>
        <rdfs:label>Handling Instructions</rdfs:label>
    </owl:ObjectProperty>
    


    <!-- http://data-marking.mitre.org/Data_Marking#informationSource -->

    <owl:ObjectProperty rdf:about="http://data-marking.mitre.org/Data_Marking#informationSource">
        <rdfs:domain rdf:resource="http://data-marking.mitre.org/Data_Marking#Marking"/>
        <rdfs:range rdf:resource="http://stix.mitre.org/stixCommon#InformationSource"/>
        <rdfs:comment>Specifies the source of this information</rdfs:comment>
        <rdfs:isDefinedBy rdf:resource="http://data-marking.mitre.org/Data_Marking"/>
        <rdfs:label>Information Source for markings</rdfs:label>
    </owl:ObjectProperty>
    


    <!-- http://data-marking.mitre.org/Data_Marking#markingData -->

    <owl:ObjectProperty rdf:about="http://data-marking.mitre.org/Data_Marking#markingData">
        <rdfs:domain rdf:resource="http://data-marking.mitre.org/Data_Marking#Marking"/>
        <rdfs:range rdf:resource="http://data-marking.mitre.org/Data_Marking#MarkingStructure"/>
        <rdfs:comment>Specifies the marking information to be applied</rdfs:comment>
        <rdfs:isDefinedBy rdf:resource="http://data-marking.mitre.org/Data_Marking"/>
        <rdfs:label>Marking Data</rdfs:label>
    </owl:ObjectProperty>
    


    <!-- 
    ///////////////////////////////////////////////////////////////////////////////////////
    //
    // Data properties
    //
    ///////////////////////////////////////////////////////////////////////////////////////
     -->

    


    <!-- http://data-marking.mitre.org/Data_Marking#color -->

    <owl:DatatypeProperty rdf:about="http://data-marking.mitre.org/Data_Marking#color">
        <rdfs:domain rdf:resource="http://data-marking.mitre.org/Data_Marking#TLPMarking"/>
        <rdfs:range>
            <rdfs:Datatype>
                <owl:oneOf>
                    <rdf:Description>
                        <rdf:type rdf:resource="http://www.w3.org/1999/02/22-rdf-syntax-ns#List"/>
                        <rdf:first rdf:datatype="http://www.w3.org/2001/XMLSchema#string">AMBER</rdf:first>
                        <rdf:rest>
                            <rdf:Description>
                                <rdf:type rdf:resource="http://www.w3.org/1999/02/22-rdf-syntax-ns#List"/>
                                <rdf:first rdf:datatype="http://www.w3.org/2001/XMLSchema#string">GREEN</rdf:first>
                                <rdf:rest>
                                    <rdf:Description>
                                        <rdf:type rdf:resource="http://www.w3.org/1999/02/22-rdf-syntax-ns#List"/>
                                        <rdf:first rdf:datatype="http://www.w3.org/2001/XMLSchema#string">RED</rdf:first>
                                        <rdf:rest>
                                            <rdf:Description>
                                                <rdf:type rdf:resource="http://www.w3.org/1999/02/22-rdf-syntax-ns#List"/>
                                                <rdf:first rdf:datatype="http://www.w3.org/2001/XMLSchema#string">WHITE</rdf:first>
                                                <rdf:rest rdf:resource="http://www.w3.org/1999/02/22-rdf-syntax-ns#nil"/>
                                            </rdf:Description>
                                        </rdf:rest>
                                    </rdf:Description>
                                </rdf:rest>
                            </rdf:Description>
                        </rdf:rest>
                    </rdf:Description>
                </owl:oneOf>
            </rdfs:Datatype>
        </rdfs:range>
        <rdfs:comment>Specifies the TLP color designation of the marked structure</rdfs:comment>
        <rdfs:label>Color</rdfs:label>
    </owl:DatatypeProperty>
    


    <!-- http://data-marking.mitre.org/Data_Marking#controlledStructure -->

    <owl:DatatypeProperty rdf:about="http://data-marking.mitre.org/Data_Marking#controlledStructure">
        <rdfs:domain rdf:resource="http://data-marking.mitre.org/Data_Marking#Marking"/>
        <rdfs:range rdf:resource="http://www.w3.org/2001/XMLSchema#string"/>
        <rdfs:comment>Specify the structures for which the Marking is to be applied.</rdfs:comment>
        <rdfs:isDefinedBy rdf:resource="http://data-marking.mitre.org/Data_Marking"/>
        <rdfs:label>Controlled Structure</rdfs:label>
    </owl:DatatypeProperty>
    


    <!-- http://data-marking.mitre.org/Data_Marking#markingId -->

    <owl:DatatypeProperty rdf:about="http://data-marking.mitre.org/Data_Marking#markingId">
        <rdfs:domain rdf:resource="http://data-marking.mitre.org/Data_Marking#Marking"/>
        <rdfs:range rdf:resource="http://www.w3.org/2001/XMLSchema#string"/>
        <rdfs:comment>Specifies the unique identifier associated with this Marking instance.

The format of the identifier MUST be in the format of &quot;marking-[UUID]&quot;, where [UUID] SHOULD correspond to a universally unique identifier.</rdfs:comment>
        <rdfs:isDefinedBy rdf:resource="http://data-marking.mitre.org/Data_Marking"/>
        <rdfs:label>Identifier</rdfs:label>
    </owl:DatatypeProperty>
    


    <!-- http://data-marking.mitre.org/Data_Marking#markingStructureId -->

    <owl:DatatypeProperty rdf:about="http://data-marking.mitre.org/Data_Marking#markingStructureId">
        <rdfs:domain rdf:resource="http://data-marking.mitre.org/Data_Marking#MarkingStructure"/>
        <rdfs:range rdf:resource="http://www.w3.org/2001/XMLSchema#string"/>
        <rdfs:comment>Specifies the unique identifier associated with this MarkingSpec instance.

The format of the identifier MUST be in the format of &quot;marking_spec-[UUID]&quot;, where [UUID] SHOULD correspond to a universally unique identifier. {@en-US}</rdfs:comment>
        <rdfs:isDefinedBy rdf:resource="http://data-marking.mitre.org/Data_Marking"/>
        <rdfs:label>Marking Structure ID</rdfs:label>
    </owl:DatatypeProperty>
    


    <!-- http://data-marking.mitre.org/Data_Marking#modelName -->

    <owl:DatatypeProperty rdf:about="http://data-marking.mitre.org/Data_Marking#modelName">
        <rdfs:domain rdf:resource="http://data-marking.mitre.org/Data_Marking#MarkingStructure"/>
        <rdfs:range rdf:resource="http://www.w3.org/2001/XMLSchema#string"/>
        <rdfs:comment>Specifies the name of the marking model to be applied within this Marking</rdfs:comment>
        <rdfs:isDefinedBy rdf:resource="http://data-marking.mitre.org/Data_Marking"/>
        <rdfs:label>Marking Model Name</rdfs:label>
    </owl:DatatypeProperty>
    


    <!-- http://data-marking.mitre.org/Data_Marking#modelRef -->

    <owl:DatatypeProperty rdf:about="http://data-marking.mitre.org/Data_Marking#modelRef">
        <rdfs:domain rdf:resource="http://data-marking.mitre.org/Data_Marking#MarkingStructure"/>
        <rdfs:range rdf:resource="http://www.w3.org/2001/XMLSchema#anyURI"/>
        <rdfs:comment>Specifies an external reference to an authoritative source on the marking model to be applied within this Marking Structure</rdfs:comment>
        <rdfs:isDefinedBy rdf:resource="http://data-marking.mitre.org/Data_Marking"/>
        <rdfs:label>Marking Model Reference</rdfs:label>
    </owl:DatatypeProperty>
    


    <!-- http://data-marking.mitre.org/Data_Marking#statement -->

    <owl:DatatypeProperty rdf:about="http://data-marking.mitre.org/Data_Marking#statement">
        <rdfs:domain rdf:resource="http://data-marking.mitre.org/Data_Marking#SimpleMarking"/>
        <rdfs:range rdf:resource="http://www.w3.org/2001/XMLSchema#string"/>
        <rdfs:comment>Specifies the statement to apply to the structure for which the Marking is to be applied.</rdfs:comment>
        <rdfs:isDefinedBy rdf:resource="http://data-marking.mitre.org/Data_Marking"/>
        <rdfs:label>Statement</rdfs:label>
    </owl:DatatypeProperty>
    


    <!-- http://data-marking.mitre.org/Data_Marking#termsOfUse -->

    <owl:DatatypeProperty rdf:about="http://data-marking.mitre.org/Data_Marking#termsOfUse">
        <rdfs:domain rdf:resource="http://data-marking.mitre.org/Data_Marking#TermsOfUseMarking"/>
        <rdfs:range rdf:resource="http://www.w3.org/2001/XMLSchema#string"/>
        <rdfs:comment>Specifies the terms of use that apply to the structure for hwich the Marking is to be applied.</rdfs:comment>
        <rdfs:isDefinedBy rdf:resource="http://data-marking.mitre.org/Data_Marking"/>
        <rdfs:label>terms of use</rdfs:label>
    </owl:DatatypeProperty>
    


    <!-- 
    ///////////////////////////////////////////////////////////////////////////////////////
    //
    // Classes
    //
    ///////////////////////////////////////////////////////////////////////////////////////
     -->

    


    <!-- http://data-marking.mitre.org/Data_Marking#Marking -->

    <owl:Class rdf:about="http://data-marking.mitre.org/Data_Marking#Marking">
        <rdfs:subClassOf>
            <owl:Restriction>
                <owl:onProperty rdf:resource="http://data-marking.mitre.org/Data_Marking#markingData"/>
                <owl:minCardinality rdf:datatype="http://www.w3.org/2001/XMLSchema#nonNegativeInteger">1</owl:minCardinality>
            </owl:Restriction>
        </rdfs:subClassOf>
        <rdfs:subClassOf>
            <owl:Restriction>
                <owl:onProperty rdf:resource="http://data-marking.mitre.org/Data_Marking#informationSource"/>
                <owl:maxCardinality rdf:datatype="http://www.w3.org/2001/XMLSchema#nonNegativeInteger">1</owl:maxCardinality>
            </owl:Restriction>
        </rdfs:subClassOf>
        <rdfs:subClassOf>
            <owl:Restriction>
                <owl:onProperty rdf:resource="http://data-marking.mitre.org/Data_Marking#controlledStructure"/>
                <owl:maxCardinality rdf:datatype="http://www.w3.org/2001/XMLSchema#nonNegativeInteger">1</owl:maxCardinality>
            </owl:Restriction>
        </rdfs:subClassOf>
        <rdfs:subClassOf>
            <owl:Restriction>
                <owl:onProperty rdf:resource="http://data-marking.mitre.org/Data_Marking#markingId"/>
                <owl:maxCardinality rdf:datatype="http://www.w3.org/2001/XMLSchema#nonNegativeInteger">1</owl:maxCardinality>
            </owl:Restriction>
        </rdfs:subClassOf>
        <rdfs:comment>Characterizes a structure for marking information to be applied to portions of STIX content</rdfs:comment>
        <rdfs:isDefinedBy rdf:resource="http://data-marking.mitre.org/Data_Marking"/>
        <rdfs:label>Marking</rdfs:label>
    </owl:Class>
    


    <!-- http://data-marking.mitre.org/Data_Marking#MarkingStructure -->

    <owl:Class rdf:about="http://data-marking.mitre.org/Data_Marking#MarkingStructure">
        <rdfs:subClassOf>
            <owl:Restriction>
                <owl:onProperty rdf:resource="http://data-marking.mitre.org/Data_Marking#markingStructureId"/>
                <owl:cardinality rdf:datatype="http://www.w3.org/2001/XMLSchema#nonNegativeInteger">1</owl:cardinality>
            </owl:Restriction>
        </rdfs:subClassOf>
        <rdfs:subClassOf>
            <owl:Restriction>
                <owl:onProperty rdf:resource="http://data-marking.mitre.org/Data_Marking#modelName"/>
                <owl:cardinality rdf:datatype="http://www.w3.org/2001/XMLSchema#nonNegativeInteger">1</owl:cardinality>
            </owl:Restriction>
        </rdfs:subClassOf>
        <rdfs:subClassOf>
            <owl:Restriction>
                <owl:onProperty rdf:resource="http://data-marking.mitre.org/Data_Marking#modelRef"/>
                <owl:maxCardinality rdf:datatype="http://www.w3.org/2001/XMLSchema#nonNegativeInteger">1</owl:maxCardinality>
            </owl:Restriction>
        </rdfs:subClassOf>
        <rdfs:comment>Characterizes the marking information to be applied to STIX content.

The MarkingStructure class provides a simple mechanism for leveraging externally defined marking systems, and it is intended to be extended to enable the expresssion of any structured or unstructured data marking mechanism.

The MarkingStructure class is an abstract class, so it MUST be extended via a subclass to express additional activity information. The definition of this base class in the minimizes the inter-dependencies between ontologies.</rdfs:comment>
        <rdfs:isDefinedBy rdf:resource="http://data-marking.mitre.org/Data_Marking"/>
        <rdfs:label>Marking Structure</rdfs:label>
    </owl:Class>
    


    <!-- http://data-marking.mitre.org/Data_Marking#SimpleMarking -->

    <owl:Class rdf:about="http://data-marking.mitre.org/Data_Marking#SimpleMarking">
        <rdfs:subClassOf rdf:resource="http://data-marking.mitre.org/Data_Marking#MarkingStructure"/>
        <rdfs:subClassOf>
            <owl:Restriction>
                <owl:onProperty rdf:resource="http://data-marking.mitre.org/Data_Marking#statement"/>
                <owl:cardinality rdf:datatype="http://www.w3.org/2001/XMLSchema#nonNegativeInteger">1</owl:cardinality>
            </owl:Restriction>
        </rdfs:subClassOf>
        <rdfs:comment>Characterizes a simple marking used to allow users to make a text statement to mark the content.

An example of a simple marking is to apply simple copyright information, for example &quot;Copyright 2014 Acme Inc.&quot;</rdfs:comment>
        <rdfs:isDefinedBy rdf:resource="http://data-marking.mitre.org/Data_Marking"/>
        <rdfs:label>Simple Marking</rdfs:label>
    </owl:Class>
    


    <!-- http://data-marking.mitre.org/Data_Marking#TLPMarking -->

    <owl:Class rdf:about="http://data-marking.mitre.org/Data_Marking#TLPMarking">
        <rdfs:subClassOf rdf:resource="http://data-marking.mitre.org/Data_Marking#MarkingStructure"/>
        <rdfs:subClassOf>
            <owl:Restriction>
                <owl:onProperty rdf:resource="http://data-marking.mitre.org/Data_Marking#color"/>
                <owl:cardinality rdf:datatype="http://www.w3.org/2001/XMLSchema#nonNegativeInteger">1</owl:cardinality>
            </owl:Restriction>
        </rdfs:subClassOf>
        <rdfs:comment>Characterizes a data marking scheme that follows the Traffic Light Protocol (TLP) designation.

The Traffic Light Protocol marking was created by US-CERT and used throughout the cyber threat sharing industry to indicate how marked content may be shared via a color (RED, AMBER, GREEN, WHITE) ala &quot;traffic light&quot; scheme.   Each color provides an indication as to how the marked content should be treated with regards to sharing and with whom sharing is permitted.

RED:  Sources use when information cannot be effectively acted upon by additional parties and could lead to impacts on a party&apos;s privacy, reputation, or opertions if misused.  Recepients may not share information with any prarties outside of the specific exchange, meeting, or conversation in which it was originally disclosed.

AMBER: Sources use when information requires support to be effectively acted upon, but carries risk to privacy, reputation, or operations if shared outside of the organizations involved.  Recepients may only share information with members of their own organization who need to know, and only as widely as necessary to act on that information. 

GREEN: Sources use when information is useful for teh awareness of all participating organizations as well as with peers within the broader community or sector.  Recepients may share information with peers and partner organizations within their sector or community, but not via publicly accessible channels.

WHITE: Sources use when information carries minimal or no foreseeable risk of misuse, in accordance with applicable rules and procedures for public release.  Recepients may share information without restriction, subject to copyright controls.</rdfs:comment>
        <rdfs:isDefinedBy rdf:resource="http://data-marking.mitre.org/Data_Marking"/>
        <rdfs:label>Traffic Light Protocol (TLP) Marking</rdfs:label>
    </owl:Class>
    


    <!-- http://data-marking.mitre.org/Data_Marking#TermsOfUseMarking -->

    <owl:Class rdf:about="http://data-marking.mitre.org/Data_Marking#TermsOfUseMarking">
        <rdfs:subClassOf rdf:resource="http://data-marking.mitre.org/Data_Marking#MarkingStructure"/>
        <rdfs:subClassOf>
            <owl:Restriction>
                <owl:onProperty rdf:resource="http://data-marking.mitre.org/Data_Marking#termsOfUse"/>
                <owl:cardinality rdf:datatype="http://www.w3.org/2001/XMLSchema#nonNegativeInteger">1</owl:cardinality>
            </owl:Restriction>
        </rdfs:subClassOf>
        <rdfs:comment>Characterizes a marking used to make a text statement to specify the Terms of Use of the marked content.

For example, the Terms of Use marking can be used to communicate a simple statement, such as &quot;Acme Inc. is not responsible for the content of this file&quot;.  The Terms of Use marking is similar to the Simple Marking but has stronger semantic meaning.</rdfs:comment>
        <rdfs:isDefinedBy rdf:resource="http://data-marking.mitre.org/Data_Marking"/>
        <rdfs:label>Terms of Use Marking</rdfs:label>
    </owl:Class>
</rdf:RDF>



<!-- Generated by the OWL API (version 4.2.6.20160910-2108) https://github.com/owlcs/owlapi -->

