<?xml version="1.0"?>
<rdf:RDF xmlns="http://stix.mitre.org/stixCommon#"
     xml:base="http://stix.mitre.org/stixCommon"
     xmlns:stixCommon="http://stix.mitre.org/stixCommon#"
     xmlns:ciq_xal="http://www.oasis-open.org/ciq_xal#"
     xmlns:rdf="http://www.w3.org/1999/02/22-rdf-syntax-ns#"
     xmlns:owl="http://www.w3.org/2002/07/owl#"
     xmlns:ciq_xpil="http://www.oasis-open.org/ciq_xpil#"
     xmlns:xml="http://www.w3.org/XML/1998/namespace"
     xmlns:xsd="http://www.w3.org/2001/XMLSchema#"
     xmlns:ciq_xnl="http://www.oasis-open.org/ciq_xnl#"
     xmlns:wgs84_pos="http://www.w3.org/2003/01/geo/wgs84_pos#"
     xmlns:rdfs="http://www.w3.org/2000/01/rdf-schema#"
     xmlns:foaf="http://xmlns.com/foaf/0.1/"
     xmlns:dc="http://purl.org/dc/elements/1.1/">
    <owl:Ontology rdf:about="http://stix.mitre.org/stixCommon">
        <owl:versionIRI rdf:resource="http://stix.mitre.org/stixCommon/1.2"/>
        <owl:imports rdf:resource="http://www.oasis-open.org/ciq_common"/>
        <owl:imports rdf:resource="http://cybox.mitre.org/cyboxCommon"/>
        <owl:versionInfo rdf:datatype="http://www.w3.org/2001/XMLSchema#string">1.2.0-000</owl:versionInfo>
        <rdfs:label>STIX Common Ontology</rdfs:label>
        <rdfs:comment>This ontology defines classes and properties that are shared across the various Structured Threat Information eXpression (STIX) ontologies.  At a high-level, the STIX Common ontology provides base classes, relationship-oriented classes, content-aggregation classes, and shared classes.</rdfs:comment>
    </owl:Ontology>
    



    <!-- 
    ///////////////////////////////////////////////////////////////////////////////////////
    //
    // Object Properties
    //
    ///////////////////////////////////////////////////////////////////////////////////////
     -->

    


    <!-- http://stix.mitre.org/stixCommon#TTPs -->

    <owl:ObjectProperty rdf:about="http://stix.mitre.org/stixCommon#TTPs">
        <rdfs:range rdf:resource="http://stix.mitre.org/stixCommon#TTPBase"/>
        <rdfs:comment>Specifies a reference to one or more cyber threat TTPs</rdfs:comment>
        <rdfs:isDefinedBy rdf:resource="http://stix.mitre.org/stixCommon"/>
        <rdfs:label>TTPs</rdfs:label>
    </owl:ObjectProperty>
    


    <!-- http://stix.mitre.org/stixCommon#author.Details -->

    <owl:ObjectProperty rdf:about="http://stix.mitre.org/stixCommon#author.Details">
        <rdfs:range>
            <owl:Class>
                <owl:unionOf rdf:parseType="Collection">
                    <rdf:Description rdf:about="http://www.oasis-open.org/ciq_xpil#Organization"/>
                    <rdf:Description rdf:about="http://www.oasis-open.org/ciq_xpil#Party"/>
                    <rdf:Description rdf:about="http://www.oasis-open.org/ciq_xpil#Person"/>
                </owl:unionOf>
            </owl:Class>
        </rdfs:range>
        <rdfs:comment>Specifies a reference to details about the author</rdfs:comment>
        <rdfs:isDefinedBy rdf:resource="http://stix.mitre.org/stixCommon"/>
        <rdfs:label>Author Details</rdfs:label>
    </owl:ObjectProperty>
    


    <!-- http://stix.mitre.org/stixCommon#campaigns -->

    <owl:ObjectProperty rdf:about="http://stix.mitre.org/stixCommon#campaigns">
        <rdfs:range rdf:resource="http://stix.mitre.org/stixCommon#CampaignBase"/>
        <rdfs:comment>Specifies a reference to one more cyber threat Campaigns</rdfs:comment>
        <rdfs:isDefinedBy rdf:resource="http://stix.mitre.org/stixCommon"/>
        <rdfs:label>Campaigns</rdfs:label>
    </owl:ObjectProperty>
    


    <!-- http://stix.mitre.org/stixCommon#confidence -->

    <owl:ObjectProperty rdf:about="http://stix.mitre.org/stixCommon#confidence">
        <rdfs:range rdf:resource="http://stix.mitre.org/stixCommon#Confidence"/>
        <rdfs:comment>Specifies a reference to the level of confidence held in the characterization of this entity.</rdfs:comment>
        <rdfs:isDefinedBy rdf:resource="http://stix.mitre.org/stixCommon"/>
        <rdfs:label>Confidence</rdfs:label>
    </owl:ObjectProperty>
    


    <!-- http://stix.mitre.org/stixCommon#confidence.assertionChain -->

    <owl:ObjectProperty rdf:about="http://stix.mitre.org/stixCommon#confidence.assertionChain">
        <rdfs:range rdf:resource="http://stix.mitre.org/stixCommon#Confidence"/>
        <rdfs:comment>Specifies a reference to a set of related confidence levels in this assertion along with who made them, when they were made and how they were made.</rdfs:comment>
        <rdfs:isDefinedBy rdf:resource="http://stix.mitre.org/stixCommon"/>
        <rdfs:label>Confidence Assertion Chain</rdfs:label>
    </owl:ObjectProperty>
    


    <!-- http://stix.mitre.org/stixCommon#confidence.source -->

    <owl:ObjectProperty rdf:about="http://stix.mitre.org/stixCommon#confidence.source">
        <rdfs:range rdf:resource="http://stix.mitre.org/stixCommon#InformationSource"/>
        <rdfs:comment>Specifies a reference to the source of this confidence assertion.</rdfs:comment>
        <rdfs:isDefinedBy rdf:resource="http://stix.mitre.org/stixCommon"/>
        <rdfs:label>Confidence Source</rdfs:label>
    </owl:ObjectProperty>
    


    <!-- http://stix.mitre.org/stixCommon#contributors -->

    <owl:ObjectProperty rdf:about="http://stix.mitre.org/stixCommon#contributors">
        <rdfs:range rdf:resource="http://cybox.mitre.org/cyboxCommon#Contributor"/>
        <rdfs:comment>Specifies a reference to contributing actors to an activity</rdfs:comment>
        <rdfs:isDefinedBy rdf:resource="http://stix.mitre.org/stixCommon"/>
        <rdfs:label>Contributors</rdfs:label>
    </owl:ObjectProperty>
    


    <!-- http://stix.mitre.org/stixCommon#courseOfAction -->

    <owl:ObjectProperty rdf:about="http://stix.mitre.org/stixCommon#courseOfAction">
        <rdfs:range rdf:resource="http://stix.mitre.org/stixCommon#CourseOfActionBase"/>
        <rdfs:comment>Specifies a reference to the Course of Action taken.</rdfs:comment>
        <rdfs:isDefinedBy rdf:resource="http://stix.mitre.org/stixCommon"/>
        <rdfs:label>Course of Action</rdfs:label>
    </owl:ObjectProperty>
    


    <!-- http://stix.mitre.org/stixCommon#coursesOfAction -->

    <owl:ObjectProperty rdf:about="http://stix.mitre.org/stixCommon#coursesOfAction">
        <rdfs:range rdf:resource="http://stix.mitre.org/stixCommon#CourseOfActionBase"/>
        <rdfs:comment>Specifies a reference to one or more cyber threat Courses of Action.</rdfs:comment>
        <rdfs:isDefinedBy rdf:resource="http://stix.mitre.org/stixCommon"/>
        <rdfs:label>Courses of Action</rdfs:label>
    </owl:ObjectProperty>
    


    <!-- http://stix.mitre.org/stixCommon#exploitTargets -->

    <owl:ObjectProperty rdf:about="http://stix.mitre.org/stixCommon#exploitTargets">
        <rdfs:range rdf:resource="http://stix.mitre.org/stixCommon#ExploitTargetBase"/>
        <rdfs:comment>Specifies a reference to one or more cyber threat exploit targets</rdfs:comment>
        <rdfs:isDefinedBy rdf:resource="http://stix.mitre.org/stixCommon"/>
        <rdfs:label>Exploit Targets</rdfs:label>
    </owl:ObjectProperty>
    


    <!-- http://stix.mitre.org/stixCommon#identity -->

    <owl:ObjectProperty rdf:about="http://stix.mitre.org/stixCommon#identity">
        <rdfs:range>
            <owl:Class>
                <owl:unionOf rdf:parseType="Collection">
                    <rdf:Description rdf:about="http://stix.mitre.org/stixCommon#CIQIdentity"/>
                    <rdf:Description rdf:about="http://www.oasis-open.org/ciq_xpil#Organization"/>
                    <rdf:Description rdf:about="http://www.oasis-open.org/ciq_xpil#Person"/>
                </owl:unionOf>
            </owl:Class>
        </rdfs:range>
        <rdfs:comment>Specifies a reference to the identity of the entity.</rdfs:comment>
        <rdfs:isDefinedBy rdf:resource="http://stix.mitre.org/stixCommon"/>
        <rdfs:label>Identity</rdfs:label>
    </owl:ObjectProperty>
    


    <!-- http://stix.mitre.org/stixCommon#incidents -->

    <owl:ObjectProperty rdf:about="http://stix.mitre.org/stixCommon#incidents">
        <rdfs:range rdf:resource="http://stix.mitre.org/stixCommon#IncidentBase"/>
        <rdfs:comment>Specifies a reference to one or more cyber threat incidents</rdfs:comment>
        <rdfs:isDefinedBy rdf:resource="http://stix.mitre.org/stixCommon"/>
        <rdfs:label>Incidents</rdfs:label>
    </owl:ObjectProperty>
    


    <!-- http://stix.mitre.org/stixCommon#indicators -->

    <owl:ObjectProperty rdf:about="http://stix.mitre.org/stixCommon#indicators">
        <rdfs:range rdf:resource="http://stix.mitre.org/stixCommon#IndicatorBase"/>
        <rdfs:comment>Specifies a reference to one or more cyber threat indicators</rdfs:comment>
        <rdfs:isDefinedBy rdf:resource="http://stix.mitre.org/stixCommon"/>
        <rdfs:label>Indicators</rdfs:label>
    </owl:ObjectProperty>
    


    <!-- http://stix.mitre.org/stixCommon#infoSource.contributingSources -->

    <owl:ObjectProperty rdf:about="http://stix.mitre.org/stixCommon#infoSource.contributingSources">
        <rdfs:range rdf:resource="http://stix.mitre.org/stixCommon#InformationSource"/>
        <rdfs:comment>Specifies a reference to a description of the individual contributing sources involved in this instance.</rdfs:comment>
        <rdfs:isDefinedBy rdf:resource="http://stix.mitre.org/stixCommon"/>
        <rdfs:label>Contributing Sources</rdfs:label>
    </owl:ObjectProperty>
    


    <!-- http://stix.mitre.org/stixCommon#infoSource.identity -->

    <owl:ObjectProperty rdf:about="http://stix.mitre.org/stixCommon#infoSource.identity">
        <rdfs:range>
            <owl:Class>
                <owl:unionOf rdf:parseType="Collection">
                    <rdf:Description rdf:about="http://www.oasis-open.org/ciq_xpil#Organization"/>
                    <rdf:Description rdf:about="http://www.oasis-open.org/ciq_xpil#Party"/>
                    <rdf:Description rdf:about="http://www.oasis-open.org/ciq_xpil#Person"/>
                </owl:unionOf>
            </owl:Class>
        </rdfs:range>
        <rdfs:comment>Specifies a reference to the identity of the source of the information</rdfs:comment>
        <rdfs:isDefinedBy rdf:resource="http://stix.mitre.org/stixCommon"/>
        <rdfs:label>Information Source Identity</rdfs:label>
    </owl:ObjectProperty>
    


    <!-- http://stix.mitre.org/stixCommon#informationSource -->

    <owl:ObjectProperty rdf:about="http://stix.mitre.org/stixCommon#informationSource">
        <rdfs:range rdf:resource="http://stix.mitre.org/stixCommon#InformationSource"/>
        <rdfs:comment>Specifies a reference to the source of the information for this entity.</rdfs:comment>
        <rdfs:isDefinedBy rdf:resource="http://stix.mitre.org/stixCommon"/>
        <rdfs:label>Information Source</rdfs:label>
    </owl:ObjectProperty>
    


    <!-- http://stix.mitre.org/stixCommon#killChainPhases -->

    <owl:ObjectProperty rdf:about="http://stix.mitre.org/stixCommon#killChainPhases">
        <rdfs:range rdf:resource="http://stix.mitre.org/stixCommon#KillChainPhase"/>
        <rdfs:comment>Specifies references to each of the phases of the kill chain.</rdfs:comment>
        <rdfs:isDefinedBy rdf:resource="http://stix.mitre.org/stixCommon"/>
        <rdfs:label>Kill Chain Phases</rdfs:label>
    </owl:ObjectProperty>
    


    <!-- http://stix.mitre.org/stixCommon#location -->

    <owl:ObjectProperty rdf:about="http://stix.mitre.org/stixCommon#location">
        <rdfs:range rdf:resource="http://www.oasis-open.org/ciq_xal#Address"/>
        <rdfs:comment>Specifies a reference to the physical location of the affected asset.</rdfs:comment>
        <rdfs:isDefinedBy rdf:resource="http://stix.mitre.org/stixCommon"/>
        <rdfs:label>Location</rdfs:label>
    </owl:ObjectProperty>
    


    <!-- http://stix.mitre.org/stixCommon#observables -->

    <owl:ObjectProperty rdf:about="http://stix.mitre.org/stixCommon#observables">
        <rdfs:range rdf:resource="http://cybox.mitre.org/cybox_core#Observables"/>
        <rdfs:comment>Specifies a reference to one or more cyber observables</rdfs:comment>
        <rdfs:isDefinedBy rdf:resource="http://stix.mitre.org/stixCommon"/>
        <rdfs:label>Observables</rdfs:label>
    </owl:ObjectProperty>
    


    <!-- http://stix.mitre.org/stixCommon#relatedCampaign -->

    <owl:ObjectProperty rdf:about="http://stix.mitre.org/stixCommon#relatedCampaign">
        <rdfs:range rdf:resource="http://stix.mitre.org/stixCommon#CampaignBase"/>
        <rdfs:comment>Specifies a reference to one or more related campaigns.</rdfs:comment>
        <rdfs:isDefinedBy rdf:resource="http://stix.mitre.org/stixCommon"/>
        <rdfs:label>Related Campaign</rdfs:label>
    </owl:ObjectProperty>
    


    <!-- http://stix.mitre.org/stixCommon#relatedCourseOfAction -->

    <owl:ObjectProperty rdf:about="http://stix.mitre.org/stixCommon#relatedCourseOfAction">
        <rdfs:range rdf:resource="http://stix.mitre.org/stixCommon#CourseOfActionBase"/>
        <rdfs:comment>Specifies a reference to one or more related Courses of Action.</rdfs:comment>
        <rdfs:isDefinedBy rdf:resource="http://stix.mitre.org/stixCommon"/>
        <rdfs:label>Related Course of Action</rdfs:label>
    </owl:ObjectProperty>
    


    <!-- http://stix.mitre.org/stixCommon#relatedExploitTarget -->

    <owl:ObjectProperty rdf:about="http://stix.mitre.org/stixCommon#relatedExploitTarget">
        <rdfs:range rdf:resource="http://stix.mitre.org/stixCommon#ExploitTargetBase"/>
        <rdfs:comment>Specifies a reference to one or more related exploit targets.</rdfs:comment>
        <rdfs:isDefinedBy rdf:resource="http://stix.mitre.org/stixCommon"/>
        <rdfs:label>Exploit Target</rdfs:label>
    </owl:ObjectProperty>
    


    <!-- http://stix.mitre.org/stixCommon#relatedIdentity -->

    <owl:ObjectProperty rdf:about="http://stix.mitre.org/stixCommon#relatedIdentity">
        <rdfs:range>
            <owl:Class>
                <owl:unionOf rdf:parseType="Collection">
                    <rdf:Description rdf:about="http://stix.mitre.org/stixCommon#CIQIdentity"/>
                    <rdf:Description rdf:about="http://www.oasis-open.org/ciq_xpil#Organization"/>
                    <rdf:Description rdf:about="http://www.oasis-open.org/ciq_xpil#Party"/>
                    <rdf:Description rdf:about="http://www.oasis-open.org/ciq_xpil#Person"/>
                </owl:unionOf>
            </owl:Class>
        </rdfs:range>
        <rdfs:comment>Specifies a reference to one or more related identities.</rdfs:comment>
        <rdfs:isDefinedBy rdf:resource="http://stix.mitre.org/stixCommon"/>
        <rdfs:label>Related Identity</rdfs:label>
    </owl:ObjectProperty>
    


    <!-- http://stix.mitre.org/stixCommon#relatedIncident -->

    <owl:ObjectProperty rdf:about="http://stix.mitre.org/stixCommon#relatedIncident">
        <rdfs:range rdf:resource="http://stix.mitre.org/stixCommon#IncidentBase"/>
        <rdfs:comment>Specifies a reference to one or more related incidents.</rdfs:comment>
        <rdfs:isDefinedBy rdf:resource="http://stix.mitre.org/stixCommon"/>
        <rdfs:label>Related Incident</rdfs:label>
    </owl:ObjectProperty>
    


    <!-- http://stix.mitre.org/stixCommon#relatedIndicator -->

    <owl:ObjectProperty rdf:about="http://stix.mitre.org/stixCommon#relatedIndicator">
        <rdfs:range rdf:resource="http://stix.mitre.org/stixCommon#IndicatorBase"/>
        <rdfs:comment>Specifies a reference to one or more related indicators.</rdfs:comment>
        <rdfs:isDefinedBy rdf:resource="http://stix.mitre.org/stixCommon"/>
        <rdfs:label>Related Indicator</rdfs:label>
    </owl:ObjectProperty>
    


    <!-- http://stix.mitre.org/stixCommon#relatedObservable -->

    <owl:ObjectProperty rdf:about="http://stix.mitre.org/stixCommon#relatedObservable">
        <rdfs:range rdf:resource="http://cybox.mitre.org/cybox_core#Observable"/>
        <rdfs:comment>Specifies a reference to the related observable.</rdfs:comment>
        <rdfs:isDefinedBy rdf:resource="http://stix.mitre.org/stixCommon"/>
        <rdfs:label>Related Observable</rdfs:label>
    </owl:ObjectProperty>
    


    <!-- http://stix.mitre.org/stixCommon#relatedObservables -->

    <owl:ObjectProperty rdf:about="http://stix.mitre.org/stixCommon#relatedObservables">
        <rdfs:range rdf:resource="http://cybox.mitre.org/cybox_core#Observables"/>
        <rdfs:comment>Specifies a reference to the related observables.</rdfs:comment>
        <rdfs:isDefinedBy rdf:resource="http://stix.mitre.org/stixCommon"/>
        <rdfs:label>Related Sbservables</rdfs:label>
    </owl:ObjectProperty>
    


    <!-- http://stix.mitre.org/stixCommon#relatedPackage -->

    <owl:ObjectProperty rdf:about="http://stix.mitre.org/stixCommon#relatedPackage">
        <rdfs:range rdf:resource="http://stix.mitre.org/stixCommon#PackageBase"/>
        <rdfs:comment>Specifies a reference to one or more related package.</rdfs:comment>
        <rdfs:isDefinedBy rdf:resource="http://stix.mitre.org/stixCommon"/>
        <rdfs:label>Related Package</rdfs:label>
    </owl:ObjectProperty>
    


    <!-- http://stix.mitre.org/stixCommon#relatedPackages -->

    <owl:ObjectProperty rdf:about="http://stix.mitre.org/stixCommon#relatedPackages">
        <rdfs:range rdf:resource="http://stix.mitre.org/stixCommon#PackageBase"/>
        <rdfs:comment>Specifies a reference to one or more related Packages.</rdfs:comment>
        <rdfs:isDefinedBy rdf:resource="http://stix.mitre.org/stixCommon"/>
        <rdfs:label>Related Packages</rdfs:label>
    </owl:ObjectProperty>
    


    <!-- http://stix.mitre.org/stixCommon#relatedTTP -->

    <owl:ObjectProperty rdf:about="http://stix.mitre.org/stixCommon#relatedTTP">
        <rdfs:range rdf:resource="http://stix.mitre.org/stixCommon#TTPBase"/>
        <rdfs:comment>Specifies a reference to one or more related TTPs.</rdfs:comment>
        <rdfs:isDefinedBy rdf:resource="http://stix.mitre.org/stixCommon"/>
        <rdfs:label>Related TTP</rdfs:label>
    </owl:ObjectProperty>
    


    <!-- http://stix.mitre.org/stixCommon#relatedThreatActor -->

    <owl:ObjectProperty rdf:about="http://stix.mitre.org/stixCommon#relatedThreatActor">
        <rdfs:range rdf:resource="http://stix.mitre.org/stixCommon#ThreatActorBase"/>
        <rdfs:comment>Specifies a reference to one or more related threat actors.</rdfs:comment>
        <rdfs:isDefinedBy rdf:resource="http://stix.mitre.org/stixCommon"/>
        <rdfs:label>Related Threat Actor</rdfs:label>
    </owl:ObjectProperty>
    


    <!-- http://stix.mitre.org/stixCommon#structuredDescription -->

    <owl:ObjectProperty rdf:about="http://stix.mitre.org/stixCommon#structuredDescription">
        <rdfs:range rdf:resource="http://cybox.mitre.org/cybox_core#Observables"/>
        <rdfs:comment>Specifies a reference to a structured description.</rdfs:comment>
        <rdfs:isDefinedBy rdf:resource="http://stix.mitre.org/stixCommon"/>
        <rdfs:label>Structured Description</rdfs:label>
    </owl:ObjectProperty>
    


    <!-- http://stix.mitre.org/stixCommon#threatActors -->

    <owl:ObjectProperty rdf:about="http://stix.mitre.org/stixCommon#threatActors">
        <rdfs:range rdf:resource="http://stix.mitre.org/stixCommon#ThreatActorBase"/>
        <rdfs:comment>Specifies a reference to one or more cyber Threat Actors</rdfs:comment>
        <rdfs:isDefinedBy rdf:resource="http://stix.mitre.org/stixCommon"/>
        <rdfs:label>Threat Actors</rdfs:label>
    </owl:ObjectProperty>
    


    <!-- http://stix.mitre.org/stixCommon#tools -->

    <owl:ObjectProperty rdf:about="http://stix.mitre.org/stixCommon#tools">
        <rdfs:range rdf:resource="http://cybox.mitre.org/cyboxCommon#ToolInformation"/>
        <rdfs:comment>Specifies a reference to a description of the tools utilized for this instance.</rdfs:comment>
        <rdfs:isDefinedBy rdf:resource="http://stix.mitre.org/stixCommon"/>
        <rdfs:label>Tools</rdfs:label>
    </owl:ObjectProperty>
    


    <!-- 
    ///////////////////////////////////////////////////////////////////////////////////////
    //
    // Data properties
    //
    ///////////////////////////////////////////////////////////////////////////////////////
     -->

    


    <!-- http://stix.mitre.org/stixCommon#assetDescription -->

    <owl:DatatypeProperty rdf:about="http://stix.mitre.org/stixCommon#assetDescription">
        <rdfs:range rdf:resource="http://www.w3.org/2001/XMLSchema#string"/>
        <rdfs:comment>Specifies an unstructured, text description of the asset.</rdfs:comment>
        <rdfs:isDefinedBy rdf:resource="http://stix.mitre.org/stixCommon"/>
        <rdfs:label>Description</rdfs:label>
    </owl:DatatypeProperty>
    


    <!-- http://stix.mitre.org/stixCommon#assetType -->

    <owl:DatatypeProperty rdf:about="http://stix.mitre.org/stixCommon#assetType">
        <rdfs:range rdf:resource="http://www.w3.org/2001/XMLSchema#string"/>
        <rdfs:comment>Specifies the type of the asset.

Examples of types of assets include directory, firewall, PBX, and cashier (these specific values are only provided to help explainthe property: they are neither recommended values nor necessarily part of any existing vocabulary).  The content creator may choose any arbitrary value or may constrain the set of possible values by referencing an externally-defined vocabulary or leveraging a formally defined vocabulary.

By default, the Asset Type Vocabulary is used to defined a restricted set of values.</rdfs:comment>
        <rdfs:isDefinedBy rdf:resource="http://stix.mitre.org/stixCommon"/>
        <rdfs:label>Type</rdfs:label>
    </owl:DatatypeProperty>
    


    <!-- http://stix.mitre.org/stixCommon#author -->

    <owl:DatatypeProperty rdf:about="http://stix.mitre.org/stixCommon#author">
        <rdfs:range rdf:resource="http://www.w3.org/2001/XMLSchema#string"/>
        <rdfs:comment>Specifies the name of the author</rdfs:comment>
        <rdfs:isDefinedBy rdf:resource="http://stix.mitre.org/stixCommon"/>
        <rdfs:label>Author</rdfs:label>
    </owl:DatatypeProperty>
    


    <!-- http://stix.mitre.org/stixCommon#businessFunction -->

    <owl:DatatypeProperty rdf:about="http://stix.mitre.org/stixCommon#businessFunction">
        <rdfs:range rdf:resource="http://www.w3.org/2001/XMLSchema#string"/>
        <rdfs:comment>Specifies a brief description of the asset&apos;s role, mission, and importance within the organization.</rdfs:comment>
        <rdfs:isDefinedBy rdf:resource="http://stix.mitre.org/stixCommon"/>
        <rdfs:label>Business Function</rdfs:label>
    </owl:DatatypeProperty>
    


    <!-- http://stix.mitre.org/stixCommon#confidence.description -->

    <owl:DatatypeProperty rdf:about="http://stix.mitre.org/stixCommon#confidence.description">
        <rdfs:range rdf:resource="http://www.w3.org/2001/XMLSchema#string"/>
        <rdfs:comment>Specifies a description of the confidence value and how it was derived.</rdfs:comment>
        <rdfs:isDefinedBy rdf:resource="http://stix.mitre.org/stixCommon"/>
        <rdfs:label>Confidence Description</rdfs:label>
    </owl:DatatypeProperty>
    


    <!-- http://stix.mitre.org/stixCommon#confidence.timestamp -->

    <owl:DatatypeProperty rdf:about="http://stix.mitre.org/stixCommon#confidence.timestamp">
        <rdfs:range rdf:resource="http://www.w3.org/2001/XMLSchema#dateTime"/>
        <rdfs:comment>Specifies the time of this Confidence assertion.</rdfs:comment>
        <rdfs:isDefinedBy rdf:resource="http://stix.mitre.org/stixCommon"/>
        <rdfs:label>Confidence Timestamp</rdfs:label>
    </owl:DatatypeProperty>
    


    <!-- http://stix.mitre.org/stixCommon#confidence.timestampPrecision -->

    <owl:DatatypeProperty rdf:about="http://stix.mitre.org/stixCommon#confidence.timestampPrecision">
       <rdfs:range rdf:resource="http://www.w3.org/2001/XMLSchema#string"/>
        <rdfs:comment>Specifies the precision of the associated timestamp value. If omitted, the default is &quot;second&quot;, meaning the timestamp is precise to the full field value.</rdfs:comment>
        <rdfs:isDefinedBy rdf:resource="http://stix.mitre.org/stixCommon"/>
        <rdfs:label>Confidence Timestamp Precision</rdfs:label>
    </owl:DatatypeProperty>
    


    <!-- http://stix.mitre.org/stixCommon#confidence.value -->

    <owl:DatatypeProperty rdf:about="http://stix.mitre.org/stixCommon#confidence.value">
        <rdfs:range rdf:resource="http://www.w3.org/2001/XMLSchema#string"/>
        <rdfs:comment>Specifies the level of confidence held in this direct assertion. 

Examples of confidence levels include High, Medium, and Low (these specific values are only provided to help explainthe property: they are neither recommended values nor necessarily part of any existing vocabulary).  The content creator may choose any arbitrary value or may constrain the set of possible values by referencing an externally-defined vocabulary or leveraging a formally defined vocabulary.

By default, the High Medium Low Vocabulary is used to defined a restricted set of values.</rdfs:comment>
        <rdfs:isDefinedBy rdf:resource="http://stix.mitre.org/stixCommon"/>
        <rdfs:label>Confidence Level</rdfs:label>
    </owl:DatatypeProperty>
    


    <!-- http://stix.mitre.org/stixCommon#costValue -->

    <owl:DatatypeProperty rdf:about="http://stix.mitre.org/stixCommon#costValue">
        <rdfs:range rdf:resource="http://www.w3.org/2001/XMLSchema#string"/>
        <rdfs:comment>Specifies a value characterizing the estimated cost for applying this Course of Action. 

Examples of cost levels include High, Medium, and Low (these specific values are only provided to help explainthe property: they are neither recommended values nor necessarily part of any existing vocabulary).  The content creator may choose any arbitrary value or may constrain the set of possible values by referencing an externally-defined vocabulary or leveraging a formally defined vocabulary.

By default, the High Medium Low Vocabulary is used to defined a restricted set of values.</rdfs:comment>
        <rdfs:isDefinedBy rdf:resource="http://stix.mitre.org/stixCommon"/>
        <rdfs:label>Value</rdfs:label>
    </owl:DatatypeProperty>
    


    <!-- http://stix.mitre.org/stixCommon#description -->

    <owl:DatatypeProperty rdf:about="http://stix.mitre.org/stixCommon#description">
        <rdfs:range rdf:resource="http://www.w3.org/2001/XMLSchema#string"/>
        <rdfs:comment>Specifies an unstructured text description</rdfs:comment>
        <rdfs:isDefinedBy rdf:resource="http://stix.mitre.org/stixCommon"/>
        <rdfs:label>Description</rdfs:label>
    </owl:DatatypeProperty>
    


    <!-- http://stix.mitre.org/stixCommon#efficacyValue -->

    <owl:DatatypeProperty rdf:about="http://stix.mitre.org/stixCommon#efficacyValue">
        <rdfs:range rdf:resource="http://www.w3.org/2001/XMLSchema#string"/>
        <rdfs:comment>Specifies a value characterizing the effectiveness.

Examples of effectiveness levels include High, Medium, and Low (these specific values are only provided to help explainthe property: they are neither recommended values nor necessarily part of any existing vocabulary).  The content creator may choose any arbitrary value or may constrain the set of possible values by referencing an externally-defined vocabulary or leveraging a formally defined vocabulary.

By default, the High Medium Low Vocabulary is used to defined a restricted set of values.</rdfs:comment>
        <rdfs:isDefinedBy rdf:resource="http://stix.mitre.org/stixCommon"/>
        <rdfs:label>Value</rdfs:label>
    </owl:DatatypeProperty>
    


    <!-- http://stix.mitre.org/stixCommon#encoded -->

    <owl:DatatypeProperty rdf:about="http://stix.mitre.org/stixCommon#encoded">
        <rdfs:range rdf:resource="http://www.w3.org/2001/XMLSchema#boolean"/>
        <rdfs:comment>Specifies whether the content encoded in the element is encoded using Base64 per RFC4648.  

If true, the data is encoded, else the data is not encoded.</rdfs:comment>
        <rdfs:isDefinedBy rdf:resource="http://stix.mitre.org/stixCommon"/>
        <rdfs:label>Encoded</rdfs:label>
    </owl:DatatypeProperty>
    


    <!-- http://stix.mitre.org/stixCommon#encodedValue -->

    <owl:DatatypeProperty rdf:about="http://stix.mitre.org/stixCommon#encodedValue">
        <rdfs:range rdf:resource="http://www.w3.org/1999/02/22-rdf-syntax-ns#XMLLiteral"/>
        <rdfs:comment>Specifies the data enoded as CDATA</rdfs:comment>
        <rdfs:isDefinedBy rdf:resource="http://stix.mitre.org/stixCommon"/>
        <rdfs:label>Encoded Value</rdfs:label>
    </owl:DatatypeProperty>
    


    <!-- http://stix.mitre.org/stixCommon#externalReference -->

    <owl:DatatypeProperty rdf:about="http://stix.mitre.org/stixCommon#externalReference">
        <rdfs:range rdf:resource="http://www.w3.org/2001/XMLSchema#anyURI"/>
        <rdfs:comment>Specifies a resource reference for this kill chain definition.</rdfs:comment>
        <rdfs:isDefinedBy rdf:resource="http://stix.mitre.org/stixCommon"/>
        <rdfs:label>External Reference</rdfs:label>
    </owl:DatatypeProperty>
    


    <!-- http://stix.mitre.org/stixCommon#id -->

    <owl:DatatypeProperty rdf:about="http://stix.mitre.org/stixCommon#id">
        <rdfs:range rdf:resource="http://www.w3.org/2001/XMLSchema#string"/>
        <rdfs:comment>Specifies the unique identifier associated with this entity instance.

The format of the identifier MUST be in the format of [construct-type]-[UUID], where [construct-type] should be associated with the entity&apos;s construct and [UUID] SHOULD correspond to a universally unique identifier.</rdfs:comment>
        <rdfs:isDefinedBy rdf:resource="http://stix.mitre.org/stixCommon"/>
        <rdfs:label>Identifier</rdfs:label>
    </owl:DatatypeProperty>
    


    <!-- http://stix.mitre.org/stixCommon#identityRole -->

    <owl:DatatypeProperty rdf:about="http://stix.mitre.org/stixCommon#identityRole">
        <rdfs:range rdf:resource="http://www.w3.org/2001/XMLSchema#string"/>
        <rdfs:comment>Specifies a relevant role played by this entity.</rdfs:comment>
        <rdfs:isDefinedBy rdf:resource="http://stix.mitre.org/stixCommon"/>
        <rdfs:label>Role</rdfs:label>
    </owl:DatatypeProperty>
    


    <!-- http://stix.mitre.org/stixCommon#impactValue -->

    <owl:DatatypeProperty rdf:about="http://stix.mitre.org/stixCommon#impactValue">
        <rdfs:range rdf:resource="http://www.w3.org/2001/XMLSchema#string"/>
        <rdfs:comment>Specifies a value characterizing the estimated impact. 

Examples of impact levels include High, Medium, and Low (these specific values are only provided to help explainthe property: they are neither recommended values nor necessarily part of any existing vocabulary).  The content creator may choose any arbitrary value or may constrain the set of possible values by referencing an externally-defined vocabulary or leveraging a formally defined vocabulary.

By default, the High Medium Low Vocabulary is used to defined a restricted set of values.</rdfs:comment>
        <rdfs:isDefinedBy rdf:resource="http://stix.mitre.org/stixCommon"/>
        <rdfs:label>Value</rdfs:label>
    </owl:DatatypeProperty>
    


    <!-- http://stix.mitre.org/stixCommon#infoSource.description -->

    <owl:DatatypeProperty rdf:about="http://stix.mitre.org/stixCommon#infoSource.description">
        <rdfs:range rdf:resource="http://www.w3.org/2001/XMLSchema#string"/>
        <rdfs:comment>Specifies a description of the information source.</rdfs:comment>
        <rdfs:isDefinedBy rdf:resource="http://stix.mitre.org/stixCommon"/>
        <rdfs:label>Description</rdfs:label>
    </owl:DatatypeProperty>
    


    <!-- http://stix.mitre.org/stixCommon#infoSource.role -->

    <owl:DatatypeProperty rdf:about="http://stix.mitre.org/stixCommon#infoSource.role">
        <rdfs:range rdf:resource="http://www.w3.org/2001/XMLSchema#string"/>
        <rdfs:comment>Specifies a characterization of the sourcing Role played by this Information Source. 

Examples of sourcing role include Initial Author, Aggregator, and Transformer/Translator (these specific values are only provided to help explainthe property: they are neither recommended values nor necessarily part of any existing vocabulary).  The content creator may choose any arbitrary value or may constrain the set of possible values by referencing an externally-defined vocabulary or leveraging a formally defined vocabulary.

By default, the Information Source Role Vocabulary is used to defined a restricted set of values.</rdfs:comment>
        <rdfs:isDefinedBy rdf:resource="http://stix.mitre.org/stixCommon"/>
        <rdfs:label>Role</rdfs:label>
    </owl:DatatypeProperty>
    


    <!-- http://stix.mitre.org/stixCommon#intendedEffectVaue -->

    <owl:DatatypeProperty rdf:about="http://stix.mitre.org/stixCommon#intendedEffectVaue">
        <rdfs:range rdf:resource="http://www.w3.org/2001/XMLSchema#string"/>
        <rdfs:comment>Specifies a value characterizing the intended effect.

Examples of intended effect levels include Destruction, Financial Loss, and Unintended Access (these specific values are only provided to help explainthe property: they are neither recommended values nor necessarily part of any existing vocabulary).  The content creator may choose any arbitrary value or may constrain the set of possible values by referencing an externally-defined vocabulary or leveraging a formally defined vocabulary.

By default, the Intended Effect Vocabulary is used to defined a restricted set of values.</rdfs:comment>
        <rdfs:isDefinedBy rdf:resource="http://stix.mitre.org/stixCommon"/>
        <rdfs:label>Value</rdfs:label>
    </owl:DatatypeProperty>
    


    <!-- http://stix.mitre.org/stixCommon#killChainDefiner -->

    <owl:DatatypeProperty rdf:about="http://stix.mitre.org/stixCommon#killChainDefiner">
        <rdfs:range rdf:resource="http://www.w3.org/2001/XMLSchema#string"/>
        <rdfs:comment>Specifies the organization or individual responsible for this kill chain definition.</rdfs:comment>
        <rdfs:isDefinedBy rdf:resource="http://stix.mitre.org/stixCommon"/>
        <rdfs:label>Killchain Definer</rdfs:label>
    </owl:DatatypeProperty>
    


    <!-- http://stix.mitre.org/stixCommon#killChainName -->

    <owl:DatatypeProperty rdf:about="http://stix.mitre.org/stixCommon#killChainName">
        <rdfs:range rdf:resource="http://www.w3.org/2001/XMLSchema#string"/>
        <rdfs:comment>Specifies a descriptive name for this kill chain definition.</rdfs:comment>
        <rdfs:isDefinedBy rdf:resource="http://stix.mitre.org/stixCommon"/>
        <rdfs:label>Kill Chain Name</rdfs:label>
    </owl:DatatypeProperty>
    


    <!-- http://stix.mitre.org/stixCommon#lastModifiedDateTime -->

    <owl:DatatypeProperty rdf:about="http://stix.mitre.org/stixCommon#lastModifiedDateTime">
        <rdfs:range rdf:resource="http://www.w3.org/2001/XMLSchema#dateTime"/>
        <rdfs:comment>Specifies the date and time the entity was last modified.</rdfs:comment>
        <rdfs:isDefinedBy rdf:resource="http://stix.mitre.org/stixCommon"/>
        <rdfs:label>Last Modified</rdfs:label>
    </owl:DatatypeProperty>
    


    <!-- http://stix.mitre.org/stixCommon#likelyImpactValue -->

    <owl:DatatypeProperty rdf:about="http://stix.mitre.org/stixCommon#likelyImpactValue">
        <rdfs:range rdf:resource="http://www.w3.org/2001/XMLSchema#string"/>
        <rdfs:comment>Specifies a value characterizing the likely potential impact within the relevant context if this Indicator were to occur. 

Examples of likely potential impact levels include High, Medium, and Low (these specific values are only provided to help explainthe property: they are neither recommended values nor necessarily part of any existing vocabulary).  The content creator may choose any arbitrary value or may constrain the set of possible values by referencing an externally-defined vocabulary or leveraging a formally defined vocabulary.

By default, the High Medium Low Vocabulary is used to defined a restricted set of values.</rdfs:comment>
        <rdfs:isDefinedBy rdf:resource="http://stix.mitre.org/stixCommon"/>
        <rdfs:label>Likely Impact</rdfs:label>
    </owl:DatatypeProperty>
    


    <!-- http://stix.mitre.org/stixCommon#locationClass -->

    <owl:DatatypeProperty rdf:about="http://stix.mitre.org/stixCommon#locationClass">
        <rdfs:range rdf:resource="http://www.w3.org/2001/XMLSchema#string"/>
        <rdfs:comment>Specifies a high-level characterization of where this asset is physically located (e.g. Internal location, External location, Co-located, Mobile). 

Examples of location class include Internally-Located, Co-Located, and Mobile (these specific values are only provided to help explainthe property: they are neither recommended values nor necessarily part of any existing vocabulary).  The content creator may choose any arbitrary value or may constrain the set of possible values by referencing an externally-defined vocabulary or leveraging a formally defined vocabulary.

By default, the Location Class Vocabulary is used to defined a restricted set of values.</rdfs:comment>
        <rdfs:isDefinedBy rdf:resource="http://stix.mitre.org/stixCommon"/>
        <rdfs:label>Location Class</rdfs:label>
    </owl:DatatypeProperty>
    


    <!-- http://stix.mitre.org/stixCommon#managementClass -->

    <owl:DatatypeProperty rdf:about="http://stix.mitre.org/stixCommon#managementClass">
        <rdfs:range rdf:resource="http://www.w3.org/2001/XMLSchema#string"/>
        <rdfs:comment>Specifies a high-level characterization of who is responsible for the day-to-day management and administration of this asset (e.g. Managed Internally, Managed by External Party, Co-managed). 

Examples of management class include Internally-Managed, Co-Managed, and Unknown (these specific values are only provided to help explainthe property: they are neither recommended values nor necessarily part of any existing vocabulary).  The content creator may choose any arbitrary value or may constrain the set of possible values by referencing an externally-defined vocabulary or leveraging a formally defined vocabulary.

By default, the Management Class Vocabulary is used to defined a restricted set of values.</rdfs:comment>
        <rdfs:isDefinedBy rdf:resource="http://stix.mitre.org/stixCommon"/>
        <rdfs:label>Management Class</rdfs:label>
    </owl:DatatypeProperty>
    


    <!-- http://stix.mitre.org/stixCommon#motivationValue -->

    <owl:DatatypeProperty rdf:about="http://stix.mitre.org/stixCommon#motivationValue">
        <rdfs:range rdf:resource="http://www.w3.org/2001/XMLSchema#string"/>
        <rdfs:comment>Specifies a value characterizing the statement within some vocabulary.

Examples of motivation include Ideological, Ego, Military, and Political (these specific values are only provided to help explainthe property: they are neither recommended values nor necessarily part of any existing vocabulary).  The content creator may choose any arbitrary value or may constrain the set of possible values by referencing an externally-defined vocabulary or leveraging a formally defined vocabulary.

By default, the Motivation Vocabulary is used to defined a restricted set of values.</rdfs:comment>
        <rdfs:isDefinedBy rdf:resource="http://stix.mitre.org/stixCommon"/>
        <rdfs:label>Value</rdfs:label>
    </owl:DatatypeProperty>
    


    <!-- http://stix.mitre.org/stixCommon#numberOfPhases -->

    <owl:DatatypeProperty rdf:about="http://stix.mitre.org/stixCommon#numberOfPhases">
        <rdfs:range rdf:resource="http://www.w3.org/2001/XMLSchema#integer"/>
        <rdfs:comment>Specifies the number of phases in the kill chain.</rdfs:comment>
        <rdfs:isDefinedBy rdf:resource="http://stix.mitre.org/stixCommon"/>
        <rdfs:label>Number of Phases</rdfs:label>
    </owl:DatatypeProperty>
    


    <!-- http://stix.mitre.org/stixCommon#ordinalValue -->

    <owl:DatatypeProperty rdf:about="http://stix.mitre.org/stixCommon#ordinalValue">
        <rdfs:range rdf:resource="http://www.w3.org/2001/XMLSchema#int"/>
        <rdfs:comment>Specifies the ordinality (e.g. 1, 2 or 3) of this entity.</rdfs:comment>
        <rdfs:isDefinedBy rdf:resource="http://stix.mitre.org/stixCommon"/>
        <rdfs:label>Ordinal Value</rdfs:label>
    </owl:DatatypeProperty>
    


    <!-- http://stix.mitre.org/stixCommon#ownershipClass -->

    <owl:DatatypeProperty rdf:about="http://stix.mitre.org/stixCommon#ownershipClass">
        <rdfs:range rdf:resource="http://www.w3.org/2001/XMLSchema#string"/>
        <rdfs:comment>Specifies a high-level characterization of who owns (or controls) this asset (e.g. Internally-owned, Employee-owned, Partner-owned, Customer-owned).

Examples of ownership class include Internally-Owned, Partner-Owned, and Customer-Owned (these specific values are only provided to help explainthe property: they are neither recommended values nor necessarily part of any existing vocabulary).  The content creator may choose any arbitrary value or may constrain the set of possible values by referencing an externally-defined vocabulary or leveraging a formally defined vocabulary.

By default, the Ownership Class Vocabulary is used to defined a restricted set of values.</rdfs:comment>
        <rdfs:isDefinedBy rdf:resource="http://stix.mitre.org/stixCommon"/>
        <rdfs:label>Ownership Class</rdfs:label>
    </owl:DatatypeProperty>
    


    <!-- http://stix.mitre.org/stixCommon#parentId -->

    <owl:DatatypeProperty rdf:about="http://stix.mitre.org/stixCommon#parentId">
        <rdfs:range rdf:resource="http://www.w3.org/2001/XMLSchema#string"/>
        <rdfs:comment>Specifies the identifier for the parent object</rdfs:comment>
        <rdfs:isDefinedBy rdf:resource="http://stix.mitre.org/stixCommon"/>
        <rdfs:label>Parent ID</rdfs:label>
    </owl:DatatypeProperty>
    


    <!-- http://stix.mitre.org/stixCommon#phaseDescription -->

    <owl:DatatypeProperty rdf:about="http://stix.mitre.org/stixCommon#phaseDescription">
        <rdfs:range rdf:resource="http://www.w3.org/2001/XMLSchema#string"/>
        <rdfs:comment>Specifies a brief description of the kill chain phase.</rdfs:comment>
        <rdfs:isDefinedBy rdf:resource="http://stix.mitre.org/stixCommon"/>
        <rdfs:label>Phase Description</rdfs:label>
    </owl:DatatypeProperty>
    


    <!-- http://stix.mitre.org/stixCommon#phaseId -->

    <owl:DatatypeProperty rdf:about="http://stix.mitre.org/stixCommon#phaseId">
        <rdfs:range rdf:resource="http://www.w3.org/2001/XMLSchema#string"/>
        <rdfs:comment>Specifies a globally unique identifier for this kill chain phase.</rdfs:comment>
        <rdfs:isDefinedBy rdf:resource="http://stix.mitre.org/stixCommon"/>
        <rdfs:label>Phase Id</rdfs:label>
    </owl:DatatypeProperty>
    


    <!-- http://stix.mitre.org/stixCommon#phaseName -->

    <owl:DatatypeProperty rdf:about="http://stix.mitre.org/stixCommon#phaseName">
        <rdfs:range rdf:resource="http://www.w3.org/2001/XMLSchema#string"/>
        <rdfs:comment>Specifies the descriptive name of the relevant kill chain phase.</rdfs:comment>
        <rdfs:isDefinedBy rdf:resource="http://stix.mitre.org/stixCommon"/>
        <rdfs:label>Phase Name</rdfs:label>
    </owl:DatatypeProperty>
    


    <!-- http://stix.mitre.org/stixCommon#planningAndOpSupportValue -->

    <owl:DatatypeProperty rdf:about="http://stix.mitre.org/stixCommon#planningAndOpSupportValue">
        <rdfs:range rdf:resource="http://www.w3.org/2001/XMLSchema#string"/>
        <rdfs:comment>Specifies a value characterizing the suspected planning and operational support performed by this threat actor. 

Examples of planning and operational support include Data Exploitation, Planning, and Skill Development / Recuritment (these specific values are only provided to help explainthe property: they are neither recommended values nor necessarily part of any existing vocabulary).  The content creator may choose any arbitrary value or may constrain the set of possible values by referencing an externally-defined vocabulary or leveraging a formally defined vocabulary.

By default, the Planning and Operational Support Vocabulary is used to defined a restricted set of values.</rdfs:comment>
        <rdfs:isDefinedBy rdf:resource="http://stix.mitre.org/stixCommon"/>
        <rdfs:label>Value</rdfs:label>
    </owl:DatatypeProperty>
    


    <!-- http://stix.mitre.org/stixCommon#references -->

    <owl:DatatypeProperty rdf:about="http://stix.mitre.org/stixCommon#references">
        <rdfs:range rdf:resource="http://www.w3.org/2001/XMLSchema#anyURI"/>
        <rdfs:comment>Specifies references to information source material for this instance.</rdfs:comment>
        <rdfs:isDefinedBy rdf:resource="http://stix.mitre.org/stixCommon"/>
        <rdfs:label>References</rdfs:label>
    </owl:DatatypeProperty>
    


    <!-- http://stix.mitre.org/stixCommon#relationshipScope -->

    <owl:DatatypeProperty rdf:about="http://stix.mitre.org/stixCommon#relationshipScope">
       <rdfs:range rdf:resource="http://www.w3.org/2001/XMLSchema#string"/>
        <rdfs:comment>Specifies how multiple related items should be interpreted in this relationship. 

If &quot;inclusive&quot; is specified, then a single conceptual relationship is being defined between the subject and the collection of objects indicated by the related items (i.e. the relationship is not necessarily relevant for any one particular object being referenced, but for the aggregated collection of objects referenced). In this situation, the number of related objects should be at least one or more.

If &quot;exclusive&quot; is specified, then multiple relationships are being defined between the specific subject and each object individually.  In this situation, the number of related objects must be limited to one.</rdfs:comment>
        <rdfs:isDefinedBy rdf:resource="http://stix.mitre.org/stixCommon"/>
        <rdfs:label>Relationship Scope</rdfs:label>
    </owl:DatatypeProperty>
    


    <!-- http://stix.mitre.org/stixCommon#relationshipType -->

    <owl:DatatypeProperty rdf:about="http://stix.mitre.org/stixCommon#relationshipType">
        <rdfs:range rdf:resource="http://www.w3.org/2001/XMLSchema#string"/>
        <rdfs:comment>Specifies the type of the relationship between the two components.</rdfs:comment>
        <rdfs:isDefinedBy rdf:resource="http://stix.mitre.org/stixCommon"/>
        <rdfs:label>Relationship Type</rdfs:label>
    </owl:DatatypeProperty>
    


    <!-- http://stix.mitre.org/stixCommon#shortDescription -->

    <owl:DatatypeProperty rdf:about="http://stix.mitre.org/stixCommon#shortDescription">
        <rdfs:range rdf:resource="http://www.w3.org/2001/XMLSchema#string"/>
        <rdfs:comment>Specifies a short, unstructured, text description</rdfs:comment>
        <rdfs:isDefinedBy rdf:resource="http://stix.mitre.org/stixCommon"/>
        <rdfs:label>Short Description</rdfs:label>
    </owl:DatatypeProperty>
    


    <!-- http://stix.mitre.org/stixCommon#sophisticationValue -->

    <owl:DatatypeProperty rdf:about="http://stix.mitre.org/stixCommon#sophisticationValue">
        <rdfs:range rdf:resource="http://www.w3.org/2001/XMLSchema#string"/>
        <rdfs:comment rdf:datatype="http://www.w3.org/2001/XMLSchema#string">Specifies a value characterizing the sophistication of a Threat Actor .

Examples of theat actor sophistication include Expert, Practitioner, and Novice (these specific values are only provided to help explainthe property: they are neither recommended values nor necessarily part of any existing vocabulary).  The content creator may choose any arbitrary value or may constrain the set of possible values by referencing an externally-defined vocabulary or leveraging a formally defined vocabulary.

By default, the Threat Actor Sophistication Vocabulary is used to defined a restricted set of values.@en-US}</rdfs:comment>
        <rdfs:isDefinedBy rdf:resource="http://stix.mitre.org/stixCommon"/>
        <rdfs:label>Value</rdfs:label>
    </owl:DatatypeProperty>
    


    <!-- http://stix.mitre.org/stixCommon#statementValue -->

    <owl:DatatypeProperty rdf:about="http://stix.mitre.org/stixCommon#statementValue">
        <rdfs:range rdf:resource="http://www.w3.org/2001/XMLSchema#string"/>
        <rdfs:comment>Specifies a value characterizing the statement within some vocabulary.

Examples of statement levels include High, Medium, and Low (these specific values are only provided to help explainthe property: they are neither recommended values nor necessarily part of any existing vocabulary).  The content creator may choose any arbitrary value or may constrain the set of possible values by referencing an externally-defined vocabulary or leveraging a formally defined vocabulary.

By default, the High Medium Low Vocabulary is used to defined a restricted set of values.</rdfs:comment>
        <rdfs:isDefinedBy rdf:resource="http://stix.mitre.org/stixCommon"/>
        <rdfs:label>Value</rdfs:label>
    </owl:DatatypeProperty>
    


    <!-- http://stix.mitre.org/stixCommon#threatActorTypeValue -->

    <owl:DatatypeProperty rdf:about="http://stix.mitre.org/stixCommon#threatActorTypeValue">
        <rdfs:range rdf:resource="http://www.w3.org/2001/XMLSchema#string"/>
        <rdfs:comment>Specifies a value characterizing the type(s) of a threat actor. 

Examples of threat actor type include Hacker, Hacktivist, and State Actor/Agency (these specific values are only provided to help explainthe property: they are neither recommended values nor necessarily part of any existing vocabulary).  The content creator may choose any arbitrary value or may constrain the set of possible values by referencing an externally-defined vocabulary or leveraging a formally defined vocabulary.

By default, the Threat Actor Type Vocabulary is used to defined a restricted set of values.</rdfs:comment>
        <rdfs:isDefinedBy rdf:resource="http://stix.mitre.org/stixCommon"/>
        <rdfs:label>Value</rdfs:label>
    </owl:DatatypeProperty>
    


    <!-- http://stix.mitre.org/stixCommon#time.endTimestamp -->

    <owl:DatatypeProperty rdf:about="http://stix.mitre.org/stixCommon#time.endTimestamp">
        <rdfs:range rdf:resource="http://www.w3.org/2001/XMLSchema#dateTime"/>
        <rdfs:comment>Specifies the time at which the activity was completed.</rdfs:comment>
        <rdfs:isDefinedBy rdf:resource="http://stix.mitre.org/stixCommon"/>
        <rdfs:label>End Time</rdfs:label>
    </owl:DatatypeProperty>
    


    <!-- http://stix.mitre.org/stixCommon#time.startTimestamp -->

    <owl:DatatypeProperty rdf:about="http://stix.mitre.org/stixCommon#time.startTimestamp">
        <rdfs:range rdf:resource="http://www.w3.org/2001/XMLSchema#dateTime"/>
        <rdfs:comment>Specifies the time at which the activity was begun.</rdfs:comment>
        <rdfs:isDefinedBy rdf:resource="http://stix.mitre.org/stixCommon"/>
        <rdfs:label>Start Time</rdfs:label>
    </owl:DatatypeProperty>
    


    <!-- http://stix.mitre.org/stixCommon#timestamp -->

    <owl:DatatypeProperty rdf:about="http://stix.mitre.org/stixCommon#timestamp">
        <rdfs:range rdf:resource="http://www.w3.org/2001/XMLSchema#dateTime"/>
        <rdfs:comment>Specifies a timestamp for the definition of a specific version of an entity.</rdfs:comment>
        <rdfs:isDefinedBy rdf:resource="http://stix.mitre.org/stixCommon"/>
        <rdfs:label>Timestamp</rdfs:label>
    </owl:DatatypeProperty>
    


    <!-- http://stix.mitre.org/stixCommon#timestampPrecision -->

    <owl:DatatypeProperty rdf:about="http://stix.mitre.org/stixCommon#timestampPrecision">
       <rdfs:range rdf:resource="http://www.w3.org/2001/XMLSchema#string"/>
        <rdfs:comment>Specifies the precision of the associated timestamp value.

If omitted, the default is &quot;seconds&quot;, meaning the timestamp is precise to the full field value.</rdfs:comment>
        <rdfs:isDefinedBy rdf:resource="http://stix.mitre.org/stixCommon"/>
        <rdfs:label>Timestamp Precision</rdfs:label>
    </owl:DatatypeProperty>
    


    <!-- http://stix.mitre.org/stixCommon#title -->

    <owl:DatatypeProperty rdf:about="http://stix.mitre.org/stixCommon#title">
        <rdfs:range rdf:resource="http://www.w3.org/2001/XMLSchema#string"/>
        <rdfs:comment>Specifies a simple title for the entity</rdfs:comment>
        <rdfs:isDefinedBy rdf:resource="http://stix.mitre.org/stixCommon"/>
        <rdfs:label>Title</rdfs:label>
    </owl:DatatypeProperty>
    


    <!-- 
    ///////////////////////////////////////////////////////////////////////////////////////
    //
    // Classes
    //
    ///////////////////////////////////////////////////////////////////////////////////////
     -->


    


    <!-- http://stix.mitre.org/stixCommon#ActionEntry -->

    <owl:Class rdf:about="http://stix.mitre.org/stixCommon#ActionEntry">
        <rdfs:subClassOf>
            <owl:Restriction>
                <owl:onProperty rdf:resource="http://stix.mitre.org/stixCommon#id"/>
                <owl:someValuesFrom rdf:resource="http://www.w3.org/2000/01/rdf-schema#Literal"/>
            </owl:Restriction>
        </rdfs:subClassOf>
        <rdfs:subClassOf>
            <owl:Restriction>
                <owl:onProperty rdf:resource="http://stix.mitre.org/stixCommon#time.endTimestamp"/>
                <owl:someValuesFrom rdf:resource="http://www.w3.org/2000/01/rdf-schema#Literal"/>
            </owl:Restriction>
        </rdfs:subClassOf>
        <rdfs:subClassOf>
            <owl:Restriction>
                <owl:onProperty rdf:resource="http://stix.mitre.org/stixCommon#time.startTimestamp"/>
                <owl:someValuesFrom rdf:resource="http://www.w3.org/2000/01/rdf-schema#Literal"/>
            </owl:Restriction>
        </rdfs:subClassOf>
        <rdfs:comment>Characterizes a based definition for an action entry used to record actions taken.</rdfs:comment>
        <rdfs:isDefinedBy rdf:resource="http://stix.mitre.org/stixCommon"/>
        <rdfs:label>Action Entry</rdfs:label>
    </owl:Class>
    


    <!-- http://stix.mitre.org/stixCommon#Activity -->

    <owl:Class rdf:about="http://stix.mitre.org/stixCommon#Activity">
        <rdfs:subClassOf>
            <owl:Restriction>
                <owl:onProperty rdf:resource="http://stix.mitre.org/stixCommon#description"/>
                <owl:someValuesFrom rdf:resource="http://www.w3.org/2000/01/rdf-schema#Literal"/>
            </owl:Restriction>
        </rdfs:subClassOf>
        <rdfs:subClassOf>
            <owl:Restriction>
                <owl:onProperty rdf:resource="http://stix.mitre.org/stixCommon#id"/>
                <owl:someValuesFrom rdf:resource="http://www.w3.org/2000/01/rdf-schema#Literal"/>
            </owl:Restriction>
        </rdfs:subClassOf>
        <rdfs:subClassOf>
            <owl:Restriction>
                <owl:onProperty rdf:resource="http://stix.mitre.org/stixCommon#timestamp"/>
                <owl:someValuesFrom rdf:resource="http://www.w3.org/2000/01/rdf-schema#Literal"/>
            </owl:Restriction>
        </rdfs:subClassOf>
        <rdfs:subClassOf>
            <owl:Restriction>
                <owl:onProperty rdf:resource="http://stix.mitre.org/stixCommon#timestampPrecision"/>
                <owl:someValuesFrom rdf:resource="http://www.w3.org/2000/01/rdf-schema#Literal"/>
            </owl:Restriction>
        </rdfs:subClassOf>
        <rdfs:comment>Characterizes basic information about an activity a defender might use.

The Activity class is an abstract class, so it MUST be extended via a subclass to express additional activity information.  STIX does not currently define a defaul subclass.  Note that an activity defined by the Activity class is fairly simple and includes only date/time information and a description.  By contrast, a Course of Action construct contains detailed information such as the stage in the cyber threat management lifecycle to which the course of action is relevant, the impact and cost of applying the course of action, and the efficacy of the course of action.</rdfs:comment>
        <rdfs:isDefinedBy rdf:resource="http://stix.mitre.org/stixCommon"/>
        <rdfs:label>Activity</rdfs:label>
    </owl:Class>
    


    <!-- http://stix.mitre.org/stixCommon#Asset -->

    <owl:Class rdf:about="http://stix.mitre.org/stixCommon#Asset">
        <rdfs:subClassOf>
            <owl:Restriction>
                <owl:onProperty rdf:resource="http://stix.mitre.org/stixCommon#location"/>
                <owl:someValuesFrom rdf:resource="http://www.w3.org/2002/07/owl#Thing"/>
            </owl:Restriction>
        </rdfs:subClassOf>
        <rdfs:subClassOf>
            <owl:Restriction>
                <owl:onProperty rdf:resource="http://stix.mitre.org/stixCommon#structuredDescription"/>
                <owl:someValuesFrom rdf:resource="http://www.w3.org/2002/07/owl#Thing"/>
            </owl:Restriction>
        </rdfs:subClassOf>
        <rdfs:subClassOf>
            <owl:Restriction>
                <owl:onProperty rdf:resource="http://stix.mitre.org/stixCommon#assetDescription"/>
                <owl:someValuesFrom rdf:resource="http://www.w3.org/2000/01/rdf-schema#Literal"/>
            </owl:Restriction>
        </rdfs:subClassOf>
        <rdfs:subClassOf>
            <owl:Restriction>
                <owl:onProperty rdf:resource="http://stix.mitre.org/stixCommon#assetType"/>
                <owl:someValuesFrom rdf:resource="http://www.w3.org/2000/01/rdf-schema#Literal"/>
            </owl:Restriction>
        </rdfs:subClassOf>
        <rdfs:subClassOf>
            <owl:Restriction>
                <owl:onProperty rdf:resource="http://stix.mitre.org/stixCommon#businessFunction"/>
                <owl:someValuesFrom rdf:resource="http://www.w3.org/2000/01/rdf-schema#Literal"/>
            </owl:Restriction>
        </rdfs:subClassOf>
        <rdfs:subClassOf>
            <owl:Restriction>
                <owl:onProperty rdf:resource="http://stix.mitre.org/stixCommon#id"/>
                <owl:someValuesFrom rdf:resource="http://www.w3.org/2000/01/rdf-schema#Literal"/>
            </owl:Restriction>
        </rdfs:subClassOf>
        <rdfs:subClassOf>
            <owl:Restriction>
                <owl:onProperty rdf:resource="http://stix.mitre.org/stixCommon#locationClass"/>
                <owl:someValuesFrom rdf:resource="http://www.w3.org/2000/01/rdf-schema#Literal"/>
            </owl:Restriction>
        </rdfs:subClassOf>
        <rdfs:subClassOf>
            <owl:Restriction>
                <owl:onProperty rdf:resource="http://stix.mitre.org/stixCommon#managementClass"/>
                <owl:someValuesFrom rdf:resource="http://www.w3.org/2000/01/rdf-schema#Literal"/>
            </owl:Restriction>
        </rdfs:subClassOf>
        <rdfs:subClassOf>
            <owl:Restriction>
                <owl:onProperty rdf:resource="http://stix.mitre.org/stixCommon#ownershipClass"/>
                <owl:someValuesFrom rdf:resource="http://www.w3.org/2000/01/rdf-schema#Literal"/>
            </owl:Restriction>
        </rdfs:subClassOf>
        <rdfs:subClassOf>
            <owl:Restriction>
                <owl:onProperty rdf:resource="http://stix.mitre.org/stixCommon#parentId"/>
                <owl:someValuesFrom rdf:resource="http://www.w3.org/2000/01/rdf-schema#Literal"/>
            </owl:Restriction>
        </rdfs:subClassOf>
        <rdfs:comment>Characterizes information about an asset.</rdfs:comment>
        <rdfs:isDefinedBy rdf:resource="http://stix.mitre.org/stixCommon"/>
        <rdfs:label>Asset</rdfs:label>
    </owl:Class>
    


    <!-- http://stix.mitre.org/stixCommon#CIQIdentity -->

    <owl:Class rdf:about="http://stix.mitre.org/stixCommon#CIQIdentity">
        <rdfs:comment>Characterizes identity information for both individuals and organizations.

The CIQIdentity class is an extension of the concept of STIX Identity found in the STIX Common XLM schema and is based on the OASIS Customer Information Quality (CIQ) data model.  To avoid overlapping properties, the concept of STIX Identity is not model in the STIX Common ontology and the CIQIdentity class is used in its place.</rdfs:comment>
        <rdfs:isDefinedBy rdf:resource="http://stix.mitre.org/stixCommon"/>
        <rdfs:label>STIXCIQIdentity</rdfs:label>
    </owl:Class>
    


    <!-- http://stix.mitre.org/stixCommon#CampaignBase -->

    <owl:Class rdf:about="http://stix.mitre.org/stixCommon#CampaignBase">
        <rdfs:subClassOf>
            <owl:Restriction>
                <owl:onProperty rdf:resource="http://stix.mitre.org/stixCommon#id"/>
                <owl:someValuesFrom rdf:resource="http://www.w3.org/2000/01/rdf-schema#Literal"/>
            </owl:Restriction>
        </rdfs:subClassOf>
        <rdfs:subClassOf>
            <owl:Restriction>
                <owl:onProperty rdf:resource="http://stix.mitre.org/stixCommon#timestamp"/>
                <owl:someValuesFrom rdf:resource="http://www.w3.org/2000/01/rdf-schema#Literal"/>
            </owl:Restriction>
        </rdfs:subClassOf>
        <rdfs:comment>Characterizes a based definition of information for a Campaign. 

The CampaignBase class is an abstract class, so it MUST be extended via a subclass to express additional activity information. The definition of the base class in the STIX Common ontology minimizes the inter-dependencies between STIX components.  The default and strongly RECOMMENDED subclass to extend the CampaignBase class is defined in the STIX Campaign ontology.</rdfs:comment>
        <rdfs:isDefinedBy rdf:resource="http://stix.mitre.org/stixCommon"/>
        <rdfs:label>Campaign base</rdfs:label>
    </owl:Class>
    


    <!-- http://stix.mitre.org/stixCommon#CampaignRelationship -->

    <owl:Class rdf:about="http://stix.mitre.org/stixCommon#CampaignRelationship">
        <rdfs:subClassOf rdf:resource="http://stix.mitre.org/stixCommon#RelationshipStatement"/>
        <rdfs:subClassOf>
            <owl:Restriction>
                <owl:onProperty rdf:resource="http://stix.mitre.org/stixCommon#confidence.assertionChain"/>
                <owl:someValuesFrom rdf:resource="http://www.w3.org/2002/07/owl#Thing"/>
            </owl:Restriction>
        </rdfs:subClassOf>
        <rdfs:subClassOf>
            <owl:Restriction>
                <owl:onProperty rdf:resource="http://stix.mitre.org/stixCommon#confidence.source"/>
                <owl:someValuesFrom rdf:resource="http://www.w3.org/2002/07/owl#Thing"/>
            </owl:Restriction>
        </rdfs:subClassOf>
        <rdfs:subClassOf>
            <owl:Restriction>
                <owl:onProperty rdf:resource="http://stix.mitre.org/stixCommon#relatedCampaign"/>
                <owl:someValuesFrom rdf:resource="http://www.w3.org/2002/07/owl#Thing"/>
            </owl:Restriction>
        </rdfs:subClassOf>
        <rdfs:subClassOf>
            <owl:Restriction>
                <owl:onProperty rdf:resource="http://stix.mitre.org/stixCommon#confidence.description"/>
                <owl:someValuesFrom rdf:resource="http://www.w3.org/2000/01/rdf-schema#Literal"/>
            </owl:Restriction>
        </rdfs:subClassOf>
        <rdfs:subClassOf>
            <owl:Restriction>
                <owl:onProperty rdf:resource="http://stix.mitre.org/stixCommon#confidence.timestamp"/>
                <owl:someValuesFrom rdf:resource="http://www.w3.org/2000/01/rdf-schema#Literal"/>
            </owl:Restriction>
        </rdfs:subClassOf>
        <rdfs:subClassOf>
            <owl:Restriction>
                <owl:onProperty rdf:resource="http://stix.mitre.org/stixCommon#confidence.timestampPrecision"/>
                <owl:someValuesFrom rdf:resource="http://www.w3.org/2000/01/rdf-schema#Literal"/>
            </owl:Restriction>
        </rdfs:subClassOf>
        <rdfs:subClassOf>
            <owl:Restriction>
                <owl:onProperty rdf:resource="http://stix.mitre.org/stixCommon#confidence.value"/>
                <owl:someValuesFrom rdf:resource="http://www.w3.org/2000/01/rdf-schema#Literal"/>
            </owl:Restriction>
        </rdfs:subClassOf>
        <rdfs:subClassOf>
            <owl:Restriction>
                <owl:onProperty rdf:resource="http://stix.mitre.org/stixCommon#relationshipScope"/>
                <owl:someValuesFrom rdf:resource="http://www.w3.org/2000/01/rdf-schema#Literal"/>
            </owl:Restriction>
        </rdfs:subClassOf>
        <rdfs:subClassOf>
            <owl:Restriction>
                <owl:onProperty rdf:resource="http://stix.mitre.org/stixCommon#relationshipType"/>
                <owl:someValuesFrom rdf:resource="http://www.w3.org/2000/01/rdf-schema#Literal"/>
            </owl:Restriction>
        </rdfs:subClassOf>
        <rdfs:comment>Characterizes a relationship to a Campaign.

The CampaignRelationship class is designed to support its use in representing the relationship attributes as an nary-relationship that can be associated with relationship between a subject STIX construct and a STIX Campaign through the use of the rdf:subject, rdf:predicate, and rdf:object properties.  The CampaignRelationship class inherits from the RelationshipStatement class but is extended with the relatedCampaign property that references an instance of the CampaignBase class or one of its subclasses.

The CampaignRelationship class MUST only be used to represent the relationship&apos;s attributes as an nary-relationship.</rdfs:comment>
        <rdfs:isDefinedBy rdf:resource="http://stix.mitre.org/stixCommon"/>
        <rdfs:label>Campaign Relationship</rdfs:label>
    </owl:Class>
    


    <!-- http://stix.mitre.org/stixCommon#Confidence -->

    <owl:Class rdf:about="http://stix.mitre.org/stixCommon#Confidence">
        <rdfs:subClassOf>
            <owl:Restriction>
                <owl:onProperty rdf:resource="http://stix.mitre.org/stixCommon#confidence.assertionChain"/>
                <owl:someValuesFrom rdf:resource="http://www.w3.org/2002/07/owl#Thing"/>
            </owl:Restriction>
        </rdfs:subClassOf>
        <rdfs:subClassOf>
            <owl:Restriction>
                <owl:onProperty rdf:resource="http://stix.mitre.org/stixCommon#confidence.source"/>
                <owl:someValuesFrom rdf:resource="http://www.w3.org/2002/07/owl#Thing"/>
            </owl:Restriction>
        </rdfs:subClassOf>
        <rdfs:subClassOf>
            <owl:Restriction>
                <owl:onProperty rdf:resource="http://stix.mitre.org/stixCommon#confidence.description"/>
                <owl:someValuesFrom rdf:resource="http://www.w3.org/2000/01/rdf-schema#Literal"/>
            </owl:Restriction>
        </rdfs:subClassOf>
        <rdfs:subClassOf>
            <owl:Restriction>
                <owl:onProperty rdf:resource="http://stix.mitre.org/stixCommon#confidence.timestamp"/>
                <owl:someValuesFrom rdf:resource="http://www.w3.org/2000/01/rdf-schema#Literal"/>
            </owl:Restriction>
        </rdfs:subClassOf>
        <rdfs:subClassOf>
            <owl:Restriction>
                <owl:onProperty rdf:resource="http://stix.mitre.org/stixCommon#confidence.timestampPrecision"/>
                <owl:someValuesFrom rdf:resource="http://www.w3.org/2000/01/rdf-schema#Literal"/>
            </owl:Restriction>
        </rdfs:subClassOf>
        <rdfs:subClassOf>
            <owl:Restriction>
                <owl:onProperty rdf:resource="http://stix.mitre.org/stixCommon#confidence.value"/>
                <owl:someValuesFrom rdf:resource="http://www.w3.org/2000/01/rdf-schema#Literal"/>
            </owl:Restriction>
        </rdfs:subClassOf>
        <rdfs:subClassOf>
            <owl:Restriction>
                <owl:onProperty rdf:resource="http://stix.mitre.org/stixCommon#id"/>
                <owl:someValuesFrom rdf:resource="http://www.w3.org/2000/01/rdf-schema#Literal"/>
            </owl:Restriction>
        </rdfs:subClassOf>
        <rdfs:comment>Characterizes a level of confidence held in some assertion.</rdfs:comment>
        <rdfs:isDefinedBy rdf:resource="http://stix.mitre.org/stixCommon"/>
        <rdfs:label>Confidence</rdfs:label>
    </owl:Class>
    


    <!-- http://stix.mitre.org/stixCommon#CostStatement -->

    <owl:Class rdf:about="http://stix.mitre.org/stixCommon#CostStatement">
        <rdfs:subClassOf rdf:resource="http://stix.mitre.org/stixCommon#Statement"/>
        <rdfs:subClassOf>
            <owl:Restriction>
                <owl:onProperty rdf:resource="http://stix.mitre.org/stixCommon#confidence.assertionChain"/>
                <owl:someValuesFrom rdf:resource="http://www.w3.org/2002/07/owl#Thing"/>
            </owl:Restriction>
        </rdfs:subClassOf>
        <rdfs:subClassOf>
            <owl:Restriction>
                <owl:onProperty rdf:resource="http://stix.mitre.org/stixCommon#confidence.source"/>
                <owl:someValuesFrom rdf:resource="http://www.w3.org/2002/07/owl#Thing"/>
            </owl:Restriction>
        </rdfs:subClassOf>
        <rdfs:subClassOf>
            <owl:Restriction>
                <owl:onProperty rdf:resource="http://stix.mitre.org/stixCommon#informationSource"/>
                <owl:someValuesFrom rdf:resource="http://www.w3.org/2002/07/owl#Thing"/>
            </owl:Restriction>
        </rdfs:subClassOf>
        <rdfs:subClassOf>
            <owl:Restriction>
                <owl:onProperty rdf:resource="http://stix.mitre.org/stixCommon#confidence.description"/>
                <owl:someValuesFrom rdf:resource="http://www.w3.org/2000/01/rdf-schema#Literal"/>
            </owl:Restriction>
        </rdfs:subClassOf>
        <rdfs:subClassOf>
            <owl:Restriction>
                <owl:onProperty rdf:resource="http://stix.mitre.org/stixCommon#confidence.timestamp"/>
                <owl:someValuesFrom rdf:resource="http://www.w3.org/2000/01/rdf-schema#Literal"/>
            </owl:Restriction>
        </rdfs:subClassOf>
        <rdfs:subClassOf>
            <owl:Restriction>
                <owl:onProperty rdf:resource="http://stix.mitre.org/stixCommon#confidence.timestampPrecision"/>
                <owl:someValuesFrom rdf:resource="http://www.w3.org/2000/01/rdf-schema#Literal"/>
            </owl:Restriction>
        </rdfs:subClassOf>
        <rdfs:subClassOf>
            <owl:Restriction>
                <owl:onProperty rdf:resource="http://stix.mitre.org/stixCommon#confidence.value"/>
                <owl:someValuesFrom rdf:resource="http://www.w3.org/2000/01/rdf-schema#Literal"/>
            </owl:Restriction>
        </rdfs:subClassOf>
        <rdfs:subClassOf>
            <owl:Restriction>
                <owl:onProperty rdf:resource="http://stix.mitre.org/stixCommon#costValue"/>
                <owl:someValuesFrom rdf:resource="http://www.w3.org/2000/01/rdf-schema#Literal"/>
            </owl:Restriction>
        </rdfs:subClassOf>
        <rdfs:subClassOf>
            <owl:Restriction>
                <owl:onProperty rdf:resource="http://stix.mitre.org/stixCommon#description"/>
                <owl:someValuesFrom rdf:resource="http://www.w3.org/2000/01/rdf-schema#Literal"/>
            </owl:Restriction>
        </rdfs:subClassOf>
        <rdfs:subClassOf>
            <owl:Restriction>
                <owl:onProperty rdf:resource="http://stix.mitre.org/stixCommon#id"/>
                <owl:someValuesFrom rdf:resource="http://www.w3.org/2000/01/rdf-schema#Literal"/>
            </owl:Restriction>
        </rdfs:subClassOf>
        <rdfs:subClassOf>
            <owl:Restriction>
                <owl:onProperty rdf:resource="http://stix.mitre.org/stixCommon#timestamp"/>
                <owl:someValuesFrom rdf:resource="http://www.w3.org/2000/01/rdf-schema#Literal"/>
            </owl:Restriction>
        </rdfs:subClassOf>
        <rdfs:subClassOf>
            <owl:Restriction>
                <owl:onProperty rdf:resource="http://stix.mitre.org/stixCommon#timestampPrecision"/>
                <owl:someValuesFrom rdf:resource="http://www.w3.org/2000/01/rdf-schema#Literal"/>
            </owl:Restriction>
        </rdfs:subClassOf>
        <rdfs:comment>Characterizes a statement about the estimated cost for applying the action. 

The CostStatement class allows for the expression of a statement, a description of the statement, a confidence in the statement, and the source of the statement.</rdfs:comment>
        <rdfs:isDefinedBy rdf:resource="http://stix.mitre.org/stixCommon"/>
        <rdfs:label>Cost Statement</rdfs:label>
    </owl:Class>
    


    <!-- http://stix.mitre.org/stixCommon#CourseOfActionBase -->

    <owl:Class rdf:about="http://stix.mitre.org/stixCommon#CourseOfActionBase">
        <rdfs:subClassOf>
            <owl:Restriction>
                <owl:onProperty rdf:resource="http://stix.mitre.org/stixCommon#id"/>
                <owl:someValuesFrom rdf:resource="http://www.w3.org/2000/01/rdf-schema#Literal"/>
            </owl:Restriction>
        </rdfs:subClassOf>
        <rdfs:subClassOf>
            <owl:Restriction>
                <owl:onProperty rdf:resource="http://stix.mitre.org/stixCommon#timestamp"/>
                <owl:someValuesFrom rdf:resource="http://www.w3.org/2000/01/rdf-schema#Literal"/>
            </owl:Restriction>
        </rdfs:subClassOf>
        <rdfs:comment>haracterizes a based definition of information for a Course of Action. 

The CourseOfActionBase class is an abstract class, so it MUST be extended via a subclass to express additional activity information. The definition of the base class in the STIX Common ontology minimizes the inter-dependencies between STIX components.  The default and strongly RECOMMENDED subclass to extend the CourseOfActionBase class is defined in the STIX Course of Action ontology</rdfs:comment>
        <rdfs:isDefinedBy rdf:resource="http://stix.mitre.org/stixCommon"/>
        <rdfs:label>Course of action base</rdfs:label>
    </owl:Class>
    


    <!-- http://stix.mitre.org/stixCommon#CourseOfActionRelationship -->

    <owl:Class rdf:about="http://stix.mitre.org/stixCommon#CourseOfActionRelationship">
        <rdfs:subClassOf rdf:resource="http://stix.mitre.org/stixCommon#RelationshipStatement"/>
        <rdfs:subClassOf>
            <owl:Restriction>
                <owl:onProperty rdf:resource="http://stix.mitre.org/stixCommon#confidence.assertionChain"/>
                <owl:someValuesFrom rdf:resource="http://www.w3.org/2002/07/owl#Thing"/>
            </owl:Restriction>
        </rdfs:subClassOf>
        <rdfs:subClassOf>
            <owl:Restriction>
                <owl:onProperty rdf:resource="http://stix.mitre.org/stixCommon#confidence.source"/>
                <owl:someValuesFrom rdf:resource="http://www.w3.org/2002/07/owl#Thing"/>
            </owl:Restriction>
        </rdfs:subClassOf>
        <rdfs:subClassOf>
            <owl:Restriction>
                <owl:onProperty rdf:resource="http://stix.mitre.org/stixCommon#relatedCourseOfAction"/>
                <owl:someValuesFrom rdf:resource="http://www.w3.org/2002/07/owl#Thing"/>
            </owl:Restriction>
        </rdfs:subClassOf>
        <rdfs:subClassOf>
            <owl:Restriction>
                <owl:onProperty rdf:resource="http://stix.mitre.org/stixCommon#confidence.description"/>
                <owl:someValuesFrom rdf:resource="http://www.w3.org/2000/01/rdf-schema#Literal"/>
            </owl:Restriction>
        </rdfs:subClassOf>
        <rdfs:subClassOf>
            <owl:Restriction>
                <owl:onProperty rdf:resource="http://stix.mitre.org/stixCommon#confidence.timestamp"/>
                <owl:someValuesFrom rdf:resource="http://www.w3.org/2000/01/rdf-schema#Literal"/>
            </owl:Restriction>
        </rdfs:subClassOf>
        <rdfs:subClassOf>
            <owl:Restriction>
                <owl:onProperty rdf:resource="http://stix.mitre.org/stixCommon#confidence.timestampPrecision"/>
                <owl:someValuesFrom rdf:resource="http://www.w3.org/2000/01/rdf-schema#Literal"/>
            </owl:Restriction>
        </rdfs:subClassOf>
        <rdfs:subClassOf>
            <owl:Restriction>
                <owl:onProperty rdf:resource="http://stix.mitre.org/stixCommon#confidence.value"/>
                <owl:someValuesFrom rdf:resource="http://www.w3.org/2000/01/rdf-schema#Literal"/>
            </owl:Restriction>
        </rdfs:subClassOf>
        <rdfs:subClassOf>
            <owl:Restriction>
                <owl:onProperty rdf:resource="http://stix.mitre.org/stixCommon#relationshipScope"/>
                <owl:someValuesFrom rdf:resource="http://www.w3.org/2000/01/rdf-schema#Literal"/>
            </owl:Restriction>
        </rdfs:subClassOf>
        <rdfs:subClassOf>
            <owl:Restriction>
                <owl:onProperty rdf:resource="http://stix.mitre.org/stixCommon#relationshipType"/>
                <owl:someValuesFrom rdf:resource="http://www.w3.org/2000/01/rdf-schema#Literal"/>
            </owl:Restriction>
        </rdfs:subClassOf>
        <rdfs:comment>Characterizes a relationship to a Course of Action. 

The CourseOfActionRelationship class is designed to support its use in representing the relationship attributes as an nary-relationship that can be associated with relationship between a subject STIX construct and a STIX Course of Action through the use of the rdf:subject, rdf:predicate, and rdf:object properties.  The CourseOfActionRelationship class inherits from the RelationshipStatement class but is extended with the relatedCourseOfAction property that references an instance of the CourseOfActionBase class or one of its subclasses.

The CourseOfActionRelationship class MUST only be used to represent the relationship&apos;s attributes as an nary-relationship.</rdfs:comment>
        <rdfs:isDefinedBy rdf:resource="http://stix.mitre.org/stixCommon"/>
        <rdfs:label>Course of Action Relationship</rdfs:label>
    </owl:Class>
    


    <!-- http://stix.mitre.org/stixCommon#EfficacyStatement -->

    <owl:Class rdf:about="http://stix.mitre.org/stixCommon#EfficacyStatement">
        <rdfs:subClassOf rdf:resource="http://stix.mitre.org/stixCommon#Statement"/>
        <rdfs:subClassOf>
            <owl:Restriction>
                <owl:onProperty rdf:resource="http://stix.mitre.org/stixCommon#confidence.assertionChain"/>
                <owl:someValuesFrom rdf:resource="http://www.w3.org/2002/07/owl#Thing"/>
            </owl:Restriction>
        </rdfs:subClassOf>
        <rdfs:subClassOf>
            <owl:Restriction>
                <owl:onProperty rdf:resource="http://stix.mitre.org/stixCommon#confidence.source"/>
                <owl:someValuesFrom rdf:resource="http://www.w3.org/2002/07/owl#Thing"/>
            </owl:Restriction>
        </rdfs:subClassOf>
        <rdfs:subClassOf>
            <owl:Restriction>
                <owl:onProperty rdf:resource="http://stix.mitre.org/stixCommon#informationSource"/>
                <owl:someValuesFrom rdf:resource="http://www.w3.org/2002/07/owl#Thing"/>
            </owl:Restriction>
        </rdfs:subClassOf>
        <rdfs:subClassOf>
            <owl:Restriction>
                <owl:onProperty rdf:resource="http://stix.mitre.org/stixCommon#confidence.description"/>
                <owl:someValuesFrom rdf:resource="http://www.w3.org/2000/01/rdf-schema#Literal"/>
            </owl:Restriction>
        </rdfs:subClassOf>
        <rdfs:subClassOf>
            <owl:Restriction>
                <owl:onProperty rdf:resource="http://stix.mitre.org/stixCommon#confidence.timestamp"/>
                <owl:someValuesFrom rdf:resource="http://www.w3.org/2000/01/rdf-schema#Literal"/>
            </owl:Restriction>
        </rdfs:subClassOf>
        <rdfs:subClassOf>
            <owl:Restriction>
                <owl:onProperty rdf:resource="http://stix.mitre.org/stixCommon#confidence.timestampPrecision"/>
                <owl:someValuesFrom rdf:resource="http://www.w3.org/2000/01/rdf-schema#Literal"/>
            </owl:Restriction>
        </rdfs:subClassOf>
        <rdfs:subClassOf>
            <owl:Restriction>
                <owl:onProperty rdf:resource="http://stix.mitre.org/stixCommon#confidence.value"/>
                <owl:someValuesFrom rdf:resource="http://www.w3.org/2000/01/rdf-schema#Literal"/>
            </owl:Restriction>
        </rdfs:subClassOf>
        <rdfs:subClassOf>
            <owl:Restriction>
                <owl:onProperty rdf:resource="http://stix.mitre.org/stixCommon#description"/>
                <owl:someValuesFrom rdf:resource="http://www.w3.org/2000/01/rdf-schema#Literal"/>
            </owl:Restriction>
        </rdfs:subClassOf>
        <rdfs:subClassOf>
            <owl:Restriction>
                <owl:onProperty rdf:resource="http://stix.mitre.org/stixCommon#efficacyValue"/>
                <owl:someValuesFrom rdf:resource="http://www.w3.org/2000/01/rdf-schema#Literal"/>
            </owl:Restriction>
        </rdfs:subClassOf>
        <rdfs:subClassOf>
            <owl:Restriction>
                <owl:onProperty rdf:resource="http://stix.mitre.org/stixCommon#id"/>
                <owl:someValuesFrom rdf:resource="http://www.w3.org/2000/01/rdf-schema#Literal"/>
            </owl:Restriction>
        </rdfs:subClassOf>
        <rdfs:subClassOf>
            <owl:Restriction>
                <owl:onProperty rdf:resource="http://stix.mitre.org/stixCommon#timestamp"/>
                <owl:someValuesFrom rdf:resource="http://www.w3.org/2000/01/rdf-schema#Literal"/>
            </owl:Restriction>
        </rdfs:subClassOf>
        <rdfs:subClassOf>
            <owl:Restriction>
                <owl:onProperty rdf:resource="http://stix.mitre.org/stixCommon#timestampPrecision"/>
                <owl:someValuesFrom rdf:resource="http://www.w3.org/2000/01/rdf-schema#Literal"/>
            </owl:Restriction>
        </rdfs:subClassOf>
        <rdfs:comment>Characterizes a statement about the effectiveness of applying an action. 

The EfficacyStatement class allows for the expression of a statement, a description of the statement, a confidence in the statement, and the source of the statement.</rdfs:comment>
        <rdfs:isDefinedBy rdf:resource="http://stix.mitre.org/stixCommon"/>
        <rdfs:label>Efficacy Statement</rdfs:label>
    </owl:Class>
    


    <!-- http://stix.mitre.org/stixCommon#EncodedCDATA -->

    <owl:Class rdf:about="http://stix.mitre.org/stixCommon#EncodedCDATA">
        <rdfs:subClassOf>
            <owl:Restriction>
                <owl:onProperty rdf:resource="http://stix.mitre.org/stixCommon#encoded"/>
                <owl:someValuesFrom rdf:resource="http://www.w3.org/2000/01/rdf-schema#Literal"/>
            </owl:Restriction>
        </rdfs:subClassOf>
        <rdfs:subClassOf>
            <owl:Restriction>
                <owl:onProperty rdf:resource="http://stix.mitre.org/stixCommon#encodedValue"/>
                <owl:someValuesFrom rdf:resource="http://www.w3.org/2000/01/rdf-schema#Literal"/>
            </owl:Restriction>
        </rdfs:subClassOf>
        <rdfs:subClassOf>
            <owl:Restriction>
                <owl:onProperty rdf:resource="http://stix.mitre.org/stixCommon#id"/>
                <owl:someValuesFrom rdf:resource="http://www.w3.org/2000/01/rdf-schema#Literal"/>
            </owl:Restriction>
        </rdfs:subClassOf>
        <rdfs:comment>Characterizes data represented in an XML CDATA block. 

Data in a CDATA block may either be represented as-is or, in cases where it may contain characters that are not valid in CDATA, it may be encoded in Base64 per RFC4648. Data encoded in Base64 must be denoted as such using the encoded attribute.</rdfs:comment>
        <rdfs:isDefinedBy rdf:resource="http://stix.mitre.org/stixCommon"/>
        <rdfs:label>Encoded CDATA</rdfs:label>
    </owl:Class>
    


    <!-- http://stix.mitre.org/stixCommon#ExploitTargetBase -->

    <owl:Class rdf:about="http://stix.mitre.org/stixCommon#ExploitTargetBase">
        <rdfs:subClassOf>
            <owl:Restriction>
                <owl:onProperty rdf:resource="http://stix.mitre.org/stixCommon#id"/>
                <owl:someValuesFrom rdf:resource="http://www.w3.org/2000/01/rdf-schema#Literal"/>
            </owl:Restriction>
        </rdfs:subClassOf>
        <rdfs:subClassOf>
            <owl:Restriction>
                <owl:onProperty rdf:resource="http://stix.mitre.org/stixCommon#timestamp"/>
                <owl:someValuesFrom rdf:resource="http://www.w3.org/2000/01/rdf-schema#Literal"/>
            </owl:Restriction>
        </rdfs:subClassOf>
        <rdfs:comment>Characterizes a based definition of information for an Exploit Target. 

The ExploitTargetBase class is an abstract class, so it MUST be extended via a subclass to express additional activity information. The definition of the base class in the STIX Common ontology minimizes the inter-dependencies between STIX components.  The default and strongly RECOMMENDED subclass to extend the ExploitTargetBase class is defined in the STIX Exploit Target ontology.</rdfs:comment>
        <rdfs:isDefinedBy rdf:resource="http://stix.mitre.org/stixCommon"/>
        <rdfs:label>Exploit Target Base</rdfs:label>
    </owl:Class>
    


    <!-- http://stix.mitre.org/stixCommon#ExploitTargetRelationship -->

    <owl:Class rdf:about="http://stix.mitre.org/stixCommon#ExploitTargetRelationship">
        <rdfs:subClassOf rdf:resource="http://stix.mitre.org/stixCommon#IdentityRelationship"/>
        <rdfs:subClassOf>
            <owl:Restriction>
                <owl:onProperty rdf:resource="http://stix.mitre.org/stixCommon#confidence.assertionChain"/>
                <owl:someValuesFrom rdf:resource="http://www.w3.org/2002/07/owl#Thing"/>
            </owl:Restriction>
        </rdfs:subClassOf>
        <rdfs:subClassOf>
            <owl:Restriction>
                <owl:onProperty rdf:resource="http://stix.mitre.org/stixCommon#confidence.source"/>
                <owl:someValuesFrom rdf:resource="http://www.w3.org/2002/07/owl#Thing"/>
            </owl:Restriction>
        </rdfs:subClassOf>
        <rdfs:subClassOf>
            <owl:Restriction>
                <owl:onProperty rdf:resource="http://stix.mitre.org/stixCommon#infoSource.identity"/>
                <owl:someValuesFrom rdf:resource="http://www.w3.org/2002/07/owl#Thing"/>
            </owl:Restriction>
        </rdfs:subClassOf>
        <rdfs:subClassOf>
            <owl:Restriction>
                <owl:onProperty rdf:resource="http://stix.mitre.org/stixCommon#relatedExploitTarget"/>
                <owl:someValuesFrom rdf:resource="http://www.w3.org/2002/07/owl#Thing"/>
            </owl:Restriction>
        </rdfs:subClassOf>
        <rdfs:subClassOf>
            <owl:Restriction>
                <owl:onProperty rdf:resource="http://stix.mitre.org/stixCommon#confidence.description"/>
                <owl:someValuesFrom rdf:resource="http://www.w3.org/2000/01/rdf-schema#Literal"/>
            </owl:Restriction>
        </rdfs:subClassOf>
        <rdfs:subClassOf>
            <owl:Restriction>
                <owl:onProperty rdf:resource="http://stix.mitre.org/stixCommon#confidence.timestamp"/>
                <owl:someValuesFrom rdf:resource="http://www.w3.org/2000/01/rdf-schema#Literal"/>
            </owl:Restriction>
        </rdfs:subClassOf>
        <rdfs:subClassOf>
            <owl:Restriction>
                <owl:onProperty rdf:resource="http://stix.mitre.org/stixCommon#confidence.timestampPrecision"/>
                <owl:someValuesFrom rdf:resource="http://www.w3.org/2000/01/rdf-schema#Literal"/>
            </owl:Restriction>
        </rdfs:subClassOf>
        <rdfs:subClassOf>
            <owl:Restriction>
                <owl:onProperty rdf:resource="http://stix.mitre.org/stixCommon#confidence.value"/>
                <owl:someValuesFrom rdf:resource="http://www.w3.org/2000/01/rdf-schema#Literal"/>
            </owl:Restriction>
        </rdfs:subClassOf>
        <rdfs:subClassOf>
            <owl:Restriction>
                <owl:onProperty rdf:resource="http://stix.mitre.org/stixCommon#infoSource.description"/>
                <owl:someValuesFrom rdf:resource="http://www.w3.org/2000/01/rdf-schema#Literal"/>
            </owl:Restriction>
        </rdfs:subClassOf>
        <rdfs:subClassOf>
            <owl:Restriction>
                <owl:onProperty rdf:resource="http://stix.mitre.org/stixCommon#relationshipScope"/>
                <owl:someValuesFrom rdf:resource="http://www.w3.org/2000/01/rdf-schema#Literal"/>
            </owl:Restriction>
        </rdfs:subClassOf>
        <rdfs:subClassOf>
            <owl:Restriction>
                <owl:onProperty rdf:resource="http://stix.mitre.org/stixCommon#relationshipType"/>
                <owl:someValuesFrom rdf:resource="http://www.w3.org/2000/01/rdf-schema#Literal"/>
            </owl:Restriction>
        </rdfs:subClassOf>
        <rdfs:comment>Characterizes a relationship to an Exploit Target. 

The ExploitTargetRelationship class is designed to support its use in representing the relationship attributes as an nary-relationship that can be associated with relationship between a subject STIX construct and a STIX Exploit Target through the use of the rdf:subject, rdf:predicate, and rdf:object properties.  The ExploitTargetRelationship class inherits from the RelationshipStatement class but is extended with the relatedExpoloitTarget property that references an instance of the ExploitTargetBase class or one of its subclasses.

The ExploitTargetRelationship class MUST only be used to represent the relationship&apos;s attributes as an nary-relationship.</rdfs:comment>
        <rdfs:isDefinedBy rdf:resource="http://stix.mitre.org/stixCommon"/>
        <rdfs:label>Exploit Target Relationship</rdfs:label>
    </owl:Class>
    


    <!-- http://stix.mitre.org/stixCommon#IdentityRelationship -->

    <owl:Class rdf:about="http://stix.mitre.org/stixCommon#IdentityRelationship">
        <rdfs:subClassOf rdf:resource="http://stix.mitre.org/stixCommon#RelationshipStatement"/>
        <rdfs:subClassOf>
            <owl:Restriction>
                <owl:onProperty rdf:resource="http://stix.mitre.org/stixCommon#confidence.assertionChain"/>
                <owl:someValuesFrom rdf:resource="http://www.w3.org/2002/07/owl#Thing"/>
            </owl:Restriction>
        </rdfs:subClassOf>
        <rdfs:subClassOf>
            <owl:Restriction>
                <owl:onProperty rdf:resource="http://stix.mitre.org/stixCommon#confidence.source"/>
                <owl:someValuesFrom rdf:resource="http://www.w3.org/2002/07/owl#Thing"/>
            </owl:Restriction>
        </rdfs:subClassOf>
        <rdfs:subClassOf>
            <owl:Restriction>
                <owl:onProperty rdf:resource="http://stix.mitre.org/stixCommon#relatedIdentity"/>
                <owl:someValuesFrom rdf:resource="http://www.w3.org/2002/07/owl#Thing"/>
            </owl:Restriction>
        </rdfs:subClassOf>
        <rdfs:subClassOf>
            <owl:Restriction>
                <owl:onProperty rdf:resource="http://stix.mitre.org/stixCommon#confidence.description"/>
                <owl:someValuesFrom rdf:resource="http://www.w3.org/2000/01/rdf-schema#Literal"/>
            </owl:Restriction>
        </rdfs:subClassOf>
        <rdfs:subClassOf>
            <owl:Restriction>
                <owl:onProperty rdf:resource="http://stix.mitre.org/stixCommon#confidence.timestamp"/>
                <owl:someValuesFrom rdf:resource="http://www.w3.org/2000/01/rdf-schema#Literal"/>
            </owl:Restriction>
        </rdfs:subClassOf>
        <rdfs:subClassOf>
            <owl:Restriction>
                <owl:onProperty rdf:resource="http://stix.mitre.org/stixCommon#confidence.timestampPrecision"/>
                <owl:someValuesFrom rdf:resource="http://www.w3.org/2000/01/rdf-schema#Literal"/>
            </owl:Restriction>
        </rdfs:subClassOf>
        <rdfs:subClassOf>
            <owl:Restriction>
                <owl:onProperty rdf:resource="http://stix.mitre.org/stixCommon#confidence.value"/>
                <owl:someValuesFrom rdf:resource="http://www.w3.org/2000/01/rdf-schema#Literal"/>
            </owl:Restriction>
        </rdfs:subClassOf>
        <rdfs:subClassOf>
            <owl:Restriction>
                <owl:onProperty rdf:resource="http://stix.mitre.org/stixCommon#relationshipScope"/>
                <owl:someValuesFrom rdf:resource="http://www.w3.org/2000/01/rdf-schema#Literal"/>
            </owl:Restriction>
        </rdfs:subClassOf>
        <rdfs:subClassOf>
            <owl:Restriction>
                <owl:onProperty rdf:resource="http://stix.mitre.org/stixCommon#relationshipType"/>
                <owl:someValuesFrom rdf:resource="http://www.w3.org/2000/01/rdf-schema#Literal"/>
            </owl:Restriction>
        </rdfs:subClassOf>
        <rdfs:comment>Characterizes a relationship to an Identity. 

The IdentityRelationship class is designed to support its use in representing the relationship attributes as an nary-relationship that can be associated with relationship between a subject STIX construct and a STIX Identity through the use of the rdf:subject, rdf:predicate, and rdf:object properties.  The IdentityRelationship class inherits from the RelationshipStatement class but is extended with the relatedIdentity property that references an instance of CIQIdentity, xpil:Organization, or xpil:Person.

The IdentityRelationship class MUST only be used to represent the relationship&apos;s attributes as an nary-relationship.</rdfs:comment>
        <rdfs:isDefinedBy rdf:resource="http://stix.mitre.org/stixCommon"/>
        <rdfs:label>Identity Relationship</rdfs:label>
    </owl:Class>
    


    <!-- http://stix.mitre.org/stixCommon#ImpactStatement -->

    <owl:Class rdf:about="http://stix.mitre.org/stixCommon#ImpactStatement">
        <rdfs:subClassOf rdf:resource="http://stix.mitre.org/stixCommon#Statement"/>
        <rdfs:subClassOf>
            <owl:Restriction>
                <owl:onProperty rdf:resource="http://stix.mitre.org/stixCommon#confidence.assertionChain"/>
                <owl:someValuesFrom rdf:resource="http://www.w3.org/2002/07/owl#Thing"/>
            </owl:Restriction>
        </rdfs:subClassOf>
        <rdfs:subClassOf>
            <owl:Restriction>
                <owl:onProperty rdf:resource="http://stix.mitre.org/stixCommon#confidence.source"/>
                <owl:someValuesFrom rdf:resource="http://www.w3.org/2002/07/owl#Thing"/>
            </owl:Restriction>
        </rdfs:subClassOf>
        <rdfs:subClassOf>
            <owl:Restriction>
                <owl:onProperty rdf:resource="http://stix.mitre.org/stixCommon#informationSource"/>
                <owl:someValuesFrom rdf:resource="http://www.w3.org/2002/07/owl#Thing"/>
            </owl:Restriction>
        </rdfs:subClassOf>
        <rdfs:subClassOf>
            <owl:Restriction>
                <owl:onProperty rdf:resource="http://stix.mitre.org/stixCommon#confidence.description"/>
                <owl:someValuesFrom rdf:resource="http://www.w3.org/2000/01/rdf-schema#Literal"/>
            </owl:Restriction>
        </rdfs:subClassOf>
        <rdfs:subClassOf>
            <owl:Restriction>
                <owl:onProperty rdf:resource="http://stix.mitre.org/stixCommon#confidence.timestamp"/>
                <owl:someValuesFrom rdf:resource="http://www.w3.org/2000/01/rdf-schema#Literal"/>
            </owl:Restriction>
        </rdfs:subClassOf>
        <rdfs:subClassOf>
            <owl:Restriction>
                <owl:onProperty rdf:resource="http://stix.mitre.org/stixCommon#confidence.timestampPrecision"/>
                <owl:someValuesFrom rdf:resource="http://www.w3.org/2000/01/rdf-schema#Literal"/>
            </owl:Restriction>
        </rdfs:subClassOf>
        <rdfs:subClassOf>
            <owl:Restriction>
                <owl:onProperty rdf:resource="http://stix.mitre.org/stixCommon#confidence.value"/>
                <owl:someValuesFrom rdf:resource="http://www.w3.org/2000/01/rdf-schema#Literal"/>
            </owl:Restriction>
        </rdfs:subClassOf>
        <rdfs:subClassOf>
            <owl:Restriction>
                <owl:onProperty rdf:resource="http://stix.mitre.org/stixCommon#description"/>
                <owl:someValuesFrom rdf:resource="http://www.w3.org/2000/01/rdf-schema#Literal"/>
            </owl:Restriction>
        </rdfs:subClassOf>
        <rdfs:subClassOf>
            <owl:Restriction>
                <owl:onProperty rdf:resource="http://stix.mitre.org/stixCommon#id"/>
                <owl:someValuesFrom rdf:resource="http://www.w3.org/2000/01/rdf-schema#Literal"/>
            </owl:Restriction>
        </rdfs:subClassOf>
        <rdfs:subClassOf>
            <owl:Restriction>
                <owl:onProperty rdf:resource="http://stix.mitre.org/stixCommon#impactValue"/>
                <owl:someValuesFrom rdf:resource="http://www.w3.org/2000/01/rdf-schema#Literal"/>
            </owl:Restriction>
        </rdfs:subClassOf>
        <rdfs:subClassOf>
            <owl:Restriction>
                <owl:onProperty rdf:resource="http://stix.mitre.org/stixCommon#timestamp"/>
                <owl:someValuesFrom rdf:resource="http://www.w3.org/2000/01/rdf-schema#Literal"/>
            </owl:Restriction>
        </rdfs:subClassOf>
        <rdfs:subClassOf>
            <owl:Restriction>
                <owl:onProperty rdf:resource="http://stix.mitre.org/stixCommon#timestampPrecision"/>
                <owl:someValuesFrom rdf:resource="http://www.w3.org/2000/01/rdf-schema#Literal"/>
            </owl:Restriction>
        </rdfs:subClassOf>
        <rdfs:comment>Characterizes a statement about the estimated impact. 

The ImpactStatement class allows for the expression of a statement, a description of the statement, a confidence in the statement, and the source of the statement.</rdfs:comment>
        <rdfs:isDefinedBy rdf:resource="http://stix.mitre.org/stixCommon"/>
        <rdfs:label>Impact Statement</rdfs:label>
    </owl:Class>
    


    <!-- http://stix.mitre.org/stixCommon#IncidentBase -->

    <owl:Class rdf:about="http://stix.mitre.org/stixCommon#IncidentBase">
        <rdfs:subClassOf rdf:resource="http://stix.mitre.org/stixCommon#ExploitTargetBase"/>
        <rdfs:subClassOf>
            <owl:Restriction>
                <owl:onProperty rdf:resource="http://stix.mitre.org/stixCommon#id"/>
                <owl:someValuesFrom rdf:resource="http://www.w3.org/2000/01/rdf-schema#Literal"/>
            </owl:Restriction>
        </rdfs:subClassOf>
        <rdfs:subClassOf>
            <owl:Restriction>
                <owl:onProperty rdf:resource="http://stix.mitre.org/stixCommon#timestamp"/>
                <owl:someValuesFrom rdf:resource="http://www.w3.org/2000/01/rdf-schema#Literal"/>
            </owl:Restriction>
        </rdfs:subClassOf>
        <rdfs:comment>Characterizes a based definition of information for an Incident. 

The IncidentBase class is an abstract class, so it MUST be extended via a subclass to express additional activity information. The definition of the base class in the STIX Common ontology minimizes the inter-dependencies between STIX components.  The default and strongly RECOMMENDED subclass to extend the IncidentBase class is defined in the STIX Incident ontology</rdfs:comment>
        <rdfs:isDefinedBy rdf:resource="http://stix.mitre.org/stixCommon"/>
        <rdfs:label>Incident Base</rdfs:label>
    </owl:Class>
    


    <!-- http://stix.mitre.org/stixCommon#IncidentRelationship -->

    <owl:Class rdf:about="http://stix.mitre.org/stixCommon#IncidentRelationship">
        <rdfs:subClassOf rdf:resource="http://stix.mitre.org/stixCommon#RelationshipStatement"/>
        <rdfs:subClassOf>
            <owl:Restriction>
                <owl:onProperty rdf:resource="http://stix.mitre.org/stixCommon#confidence.assertionChain"/>
                <owl:someValuesFrom rdf:resource="http://www.w3.org/2002/07/owl#Thing"/>
            </owl:Restriction>
        </rdfs:subClassOf>
        <rdfs:subClassOf>
            <owl:Restriction>
                <owl:onProperty rdf:resource="http://stix.mitre.org/stixCommon#confidence.source"/>
                <owl:someValuesFrom rdf:resource="http://www.w3.org/2002/07/owl#Thing"/>
            </owl:Restriction>
        </rdfs:subClassOf>
        <rdfs:subClassOf>
            <owl:Restriction>
                <owl:onProperty rdf:resource="http://stix.mitre.org/stixCommon#relatedIncident"/>
                <owl:someValuesFrom rdf:resource="http://www.w3.org/2002/07/owl#Thing"/>
            </owl:Restriction>
        </rdfs:subClassOf>
        <rdfs:subClassOf>
            <owl:Restriction>
                <owl:onProperty rdf:resource="http://stix.mitre.org/stixCommon#confidence.description"/>
                <owl:someValuesFrom rdf:resource="http://www.w3.org/2000/01/rdf-schema#Literal"/>
            </owl:Restriction>
        </rdfs:subClassOf>
        <rdfs:subClassOf>
            <owl:Restriction>
                <owl:onProperty rdf:resource="http://stix.mitre.org/stixCommon#confidence.timestamp"/>
                <owl:someValuesFrom rdf:resource="http://www.w3.org/2000/01/rdf-schema#Literal"/>
            </owl:Restriction>
        </rdfs:subClassOf>
        <rdfs:subClassOf>
            <owl:Restriction>
                <owl:onProperty rdf:resource="http://stix.mitre.org/stixCommon#confidence.timestampPrecision"/>
                <owl:someValuesFrom rdf:resource="http://www.w3.org/2000/01/rdf-schema#Literal"/>
            </owl:Restriction>
        </rdfs:subClassOf>
        <rdfs:subClassOf>
            <owl:Restriction>
                <owl:onProperty rdf:resource="http://stix.mitre.org/stixCommon#confidence.value"/>
                <owl:someValuesFrom rdf:resource="http://www.w3.org/2000/01/rdf-schema#Literal"/>
            </owl:Restriction>
        </rdfs:subClassOf>
        <rdfs:subClassOf>
            <owl:Restriction>
                <owl:onProperty rdf:resource="http://stix.mitre.org/stixCommon#relationshipScope"/>
                <owl:someValuesFrom rdf:resource="http://www.w3.org/2000/01/rdf-schema#Literal"/>
            </owl:Restriction>
        </rdfs:subClassOf>
        <rdfs:subClassOf>
            <owl:Restriction>
                <owl:onProperty rdf:resource="http://stix.mitre.org/stixCommon#relationshipType"/>
                <owl:someValuesFrom rdf:resource="http://www.w3.org/2000/01/rdf-schema#Literal"/>
            </owl:Restriction>
        </rdfs:subClassOf>
        <rdfs:comment>Characterizes a relationship to an Incident. 

The IncidentRelationship class is designed to support its use in representing the relationship attributes as an nary-relationship that can be associated with relationship between a subject STIX construct and a STIX Incident through the use of the rdf:subject, rdf:predicate, and rdf:object properties.  The IncidentRelationship class inherits from the RelationshipStatement class but is extended with the relatedCampaign property that references an instance of the IncidentBase class or one of its subclasses.

The IncidentRelationship class MUST only be used to represent the relationship&apos;s attributes as an nary-relationship.</rdfs:comment>
        <rdfs:isDefinedBy rdf:resource="http://stix.mitre.org/stixCommon"/>
        <rdfs:label>Incident Relationship</rdfs:label>
    </owl:Class>
    


    <!-- http://stix.mitre.org/stixCommon#IndicatorBase -->

    <owl:Class rdf:about="http://stix.mitre.org/stixCommon#IndicatorBase">
        <rdfs:subClassOf>
            <owl:Restriction>
                <owl:onProperty rdf:resource="http://stix.mitre.org/stixCommon#id"/>
                <owl:someValuesFrom rdf:resource="http://www.w3.org/2000/01/rdf-schema#Literal"/>
            </owl:Restriction>
        </rdfs:subClassOf>
        <rdfs:subClassOf>
            <owl:Restriction>
                <owl:onProperty rdf:resource="http://stix.mitre.org/stixCommon#timestamp"/>
                <owl:someValuesFrom rdf:resource="http://www.w3.org/2000/01/rdf-schema#Literal"/>
            </owl:Restriction>
        </rdfs:subClassOf>
        <rdfs:comment>Characterizes a based definition of information for an Indicator. 

The IndicatorBase class is an abstract class, so it MUST be extended via a subclass to express additional activity information. The definition of the base class in the STIX Common ontology minimizes the inter-dependencies between STIX components.  The default and strongly RECOMMENDED subclass to extend the IndicatorBase class is defined in the STIX Indicator ontology.</rdfs:comment>
        <rdfs:isDefinedBy rdf:resource="http://stix.mitre.org/stixCommon"/>
        <rdfs:label>Indicator Base</rdfs:label>
    </owl:Class>
    


    <!-- http://stix.mitre.org/stixCommon#IndicatorRelationship -->

    <owl:Class rdf:about="http://stix.mitre.org/stixCommon#IndicatorRelationship">
        <rdfs:subClassOf rdf:resource="http://stix.mitre.org/stixCommon#RelationshipStatement"/>
        <rdfs:subClassOf>
            <owl:Restriction>
                <owl:onProperty rdf:resource="http://stix.mitre.org/stixCommon#confidence.assertionChain"/>
                <owl:someValuesFrom rdf:resource="http://www.w3.org/2002/07/owl#Thing"/>
            </owl:Restriction>
        </rdfs:subClassOf>
        <rdfs:subClassOf>
            <owl:Restriction>
                <owl:onProperty rdf:resource="http://stix.mitre.org/stixCommon#confidence.source"/>
                <owl:someValuesFrom rdf:resource="http://www.w3.org/2002/07/owl#Thing"/>
            </owl:Restriction>
        </rdfs:subClassOf>
        <rdfs:subClassOf>
            <owl:Restriction>
                <owl:onProperty rdf:resource="http://stix.mitre.org/stixCommon#relatedIndicator"/>
                <owl:someValuesFrom rdf:resource="http://www.w3.org/2002/07/owl#Thing"/>
            </owl:Restriction>
        </rdfs:subClassOf>
        <rdfs:subClassOf>
            <owl:Restriction>
                <owl:onProperty rdf:resource="http://stix.mitre.org/stixCommon#confidence.description"/>
                <owl:someValuesFrom rdf:resource="http://www.w3.org/2000/01/rdf-schema#Literal"/>
            </owl:Restriction>
        </rdfs:subClassOf>
        <rdfs:subClassOf>
            <owl:Restriction>
                <owl:onProperty rdf:resource="http://stix.mitre.org/stixCommon#confidence.timestamp"/>
                <owl:someValuesFrom rdf:resource="http://www.w3.org/2000/01/rdf-schema#Literal"/>
            </owl:Restriction>
        </rdfs:subClassOf>
        <rdfs:subClassOf>
            <owl:Restriction>
                <owl:onProperty rdf:resource="http://stix.mitre.org/stixCommon#confidence.timestampPrecision"/>
                <owl:someValuesFrom rdf:resource="http://www.w3.org/2000/01/rdf-schema#Literal"/>
            </owl:Restriction>
        </rdfs:subClassOf>
        <rdfs:subClassOf>
            <owl:Restriction>
                <owl:onProperty rdf:resource="http://stix.mitre.org/stixCommon#confidence.value"/>
                <owl:someValuesFrom rdf:resource="http://www.w3.org/2000/01/rdf-schema#Literal"/>
            </owl:Restriction>
        </rdfs:subClassOf>
        <rdfs:subClassOf>
            <owl:Restriction>
                <owl:onProperty rdf:resource="http://stix.mitre.org/stixCommon#relationshipScope"/>
                <owl:someValuesFrom rdf:resource="http://www.w3.org/2000/01/rdf-schema#Literal"/>
            </owl:Restriction>
        </rdfs:subClassOf>
        <rdfs:subClassOf>
            <owl:Restriction>
                <owl:onProperty rdf:resource="http://stix.mitre.org/stixCommon#relationshipType"/>
                <owl:someValuesFrom rdf:resource="http://www.w3.org/2000/01/rdf-schema#Literal"/>
            </owl:Restriction>
        </rdfs:subClassOf>
        <rdfs:comment>Characterizes a relationship to an Indicator. 

The IndicatorRelationship class is designed to support its use in representing the relationship attributes as an nary-relationship that can be associated with relationship between a subject STIX construct and a STIX Indicator through the use of the rdf:subject, rdf:predicate, and rdf:object properties.  The IndicatorRelationship class inherits from the RelationshipStatement class but is extended with the relatedIndicator property that references an instance of the IndicatorBase class or one of its subclasses.

The IndicatorRelationship class MUST only be used to represent the relationship&apos;s attributes as an nary-relationship.</rdfs:comment>
        <rdfs:isDefinedBy rdf:resource="http://stix.mitre.org/stixCommon"/>
        <rdfs:label>Indicator Relationship</rdfs:label>
    </owl:Class>
    


    <!-- http://stix.mitre.org/stixCommon#InformationSource -->

    <owl:Class rdf:about="http://stix.mitre.org/stixCommon#InformationSource">
        <rdfs:subClassOf>
            <owl:Restriction>
                <owl:onProperty rdf:resource="http://stix.mitre.org/stixCommon#infoSource.identity"/>
                <owl:someValuesFrom rdf:resource="http://www.w3.org/2002/07/owl#Thing"/>
            </owl:Restriction>
        </rdfs:subClassOf>
        <rdfs:subClassOf>
            <owl:Restriction>
                <owl:onProperty rdf:resource="http://stix.mitre.org/stixCommon#id"/>
                <owl:someValuesFrom rdf:resource="http://www.w3.org/2000/01/rdf-schema#Literal"/>
            </owl:Restriction>
        </rdfs:subClassOf>
        <rdfs:subClassOf>
            <owl:Restriction>
                <owl:onProperty rdf:resource="http://stix.mitre.org/stixCommon#infoSource.description"/>
                <owl:someValuesFrom rdf:resource="http://www.w3.org/2000/01/rdf-schema#Literal"/>
            </owl:Restriction>
        </rdfs:subClassOf>
        <rdfs:comment>Characterizes details about the source of a given data for the given STIX context.</rdfs:comment>
        <rdfs:isDefinedBy rdf:resource="http://stix.mitre.org/stixCommon"/>
        <rdfs:label>Information Source</rdfs:label>
    </owl:Class>
    


    <!-- http://stix.mitre.org/stixCommon#IntendedEffectStatement -->

    <owl:Class rdf:about="http://stix.mitre.org/stixCommon#IntendedEffectStatement">
        <rdfs:subClassOf rdf:resource="http://stix.mitre.org/stixCommon#Statement"/>
        <rdfs:subClassOf>
            <owl:Restriction>
                <owl:onProperty rdf:resource="http://stix.mitre.org/stixCommon#confidence.assertionChain"/>
                <owl:someValuesFrom rdf:resource="http://www.w3.org/2002/07/owl#Thing"/>
            </owl:Restriction>
        </rdfs:subClassOf>
        <rdfs:subClassOf>
            <owl:Restriction>
                <owl:onProperty rdf:resource="http://stix.mitre.org/stixCommon#confidence.source"/>
                <owl:someValuesFrom rdf:resource="http://www.w3.org/2002/07/owl#Thing"/>
            </owl:Restriction>
        </rdfs:subClassOf>
        <rdfs:subClassOf>
            <owl:Restriction>
                <owl:onProperty rdf:resource="http://stix.mitre.org/stixCommon#informationSource"/>
                <owl:someValuesFrom rdf:resource="http://www.w3.org/2002/07/owl#Thing"/>
            </owl:Restriction>
        </rdfs:subClassOf>
        <rdfs:subClassOf>
            <owl:Restriction>
                <owl:onProperty rdf:resource="http://stix.mitre.org/stixCommon#confidence.description"/>
                <owl:someValuesFrom rdf:resource="http://www.w3.org/2000/01/rdf-schema#Literal"/>
            </owl:Restriction>
        </rdfs:subClassOf>
        <rdfs:subClassOf>
            <owl:Restriction>
                <owl:onProperty rdf:resource="http://stix.mitre.org/stixCommon#confidence.timestamp"/>
                <owl:someValuesFrom rdf:resource="http://www.w3.org/2000/01/rdf-schema#Literal"/>
            </owl:Restriction>
        </rdfs:subClassOf>
        <rdfs:subClassOf>
            <owl:Restriction>
                <owl:onProperty rdf:resource="http://stix.mitre.org/stixCommon#confidence.timestampPrecision"/>
                <owl:someValuesFrom rdf:resource="http://www.w3.org/2000/01/rdf-schema#Literal"/>
            </owl:Restriction>
        </rdfs:subClassOf>
        <rdfs:subClassOf>
            <owl:Restriction>
                <owl:onProperty rdf:resource="http://stix.mitre.org/stixCommon#confidence.value"/>
                <owl:someValuesFrom rdf:resource="http://www.w3.org/2000/01/rdf-schema#Literal"/>
            </owl:Restriction>
        </rdfs:subClassOf>
        <rdfs:subClassOf>
            <owl:Restriction>
                <owl:onProperty rdf:resource="http://stix.mitre.org/stixCommon#description"/>
                <owl:someValuesFrom rdf:resource="http://www.w3.org/2000/01/rdf-schema#Literal"/>
            </owl:Restriction>
        </rdfs:subClassOf>
        <rdfs:subClassOf>
            <owl:Restriction>
                <owl:onProperty rdf:resource="http://stix.mitre.org/stixCommon#id"/>
                <owl:someValuesFrom rdf:resource="http://www.w3.org/2000/01/rdf-schema#Literal"/>
            </owl:Restriction>
        </rdfs:subClassOf>
        <rdfs:subClassOf>
            <owl:Restriction>
                <owl:onProperty rdf:resource="http://stix.mitre.org/stixCommon#intendedEffectVaue"/>
                <owl:someValuesFrom rdf:resource="http://www.w3.org/2000/01/rdf-schema#Literal"/>
            </owl:Restriction>
        </rdfs:subClassOf>
        <rdfs:subClassOf>
            <owl:Restriction>
                <owl:onProperty rdf:resource="http://stix.mitre.org/stixCommon#timestamp"/>
                <owl:someValuesFrom rdf:resource="http://www.w3.org/2000/01/rdf-schema#Literal"/>
            </owl:Restriction>
        </rdfs:subClassOf>
        <rdfs:subClassOf>
            <owl:Restriction>
                <owl:onProperty rdf:resource="http://stix.mitre.org/stixCommon#timestampPrecision"/>
                <owl:someValuesFrom rdf:resource="http://www.w3.org/2000/01/rdf-schema#Literal"/>
            </owl:Restriction>
        </rdfs:subClassOf>
        <rdfs:comment>Characterizes a statement about an intended effect.

The IntendedEffectStatement class allows for the expression of a statement, a description of the statement, a confidence in the statement, and the source of the statement.</rdfs:comment>
        <rdfs:isDefinedBy rdf:resource="http://stix.mitre.org/stixCommon"/>
        <rdfs:label>Intended Effect Statement</rdfs:label>
    </owl:Class>
    


    <!-- http://stix.mitre.org/stixCommon#JournalEntry -->

    <owl:Class rdf:about="http://stix.mitre.org/stixCommon#JournalEntry">
        <rdfs:subClassOf>
            <owl:Restriction>
                <owl:onProperty rdf:resource="http://stix.mitre.org/stixCommon#author.Details"/>
                <owl:someValuesFrom rdf:resource="http://www.w3.org/2002/07/owl#Thing"/>
            </owl:Restriction>
        </rdfs:subClassOf>
        <rdfs:subClassOf>
            <owl:Restriction>
                <owl:onProperty rdf:resource="http://stix.mitre.org/stixCommon#author"/>
                <owl:someValuesFrom rdf:resource="http://www.w3.org/2000/01/rdf-schema#Literal"/>
            </owl:Restriction>
        </rdfs:subClassOf>
        <rdfs:subClassOf>
            <owl:Restriction>
                <owl:onProperty rdf:resource="http://stix.mitre.org/stixCommon#description"/>
                <owl:someValuesFrom rdf:resource="http://www.w3.org/2000/01/rdf-schema#Literal"/>
            </owl:Restriction>
        </rdfs:subClassOf>
        <rdfs:subClassOf>
            <owl:Restriction>
                <owl:onProperty rdf:resource="http://stix.mitre.org/stixCommon#id"/>
                <owl:someValuesFrom rdf:resource="http://www.w3.org/2000/01/rdf-schema#Literal"/>
            </owl:Restriction>
        </rdfs:subClassOf>
        <rdfs:comment>Characterizes journal notes for information discovered.</rdfs:comment>
        <rdfs:isDefinedBy rdf:resource="http://stix.mitre.org/stixCommon"/>
        <rdfs:label>Journal Entry</rdfs:label>
    </owl:Class>
    


    <!-- http://stix.mitre.org/stixCommon#KillChain -->

    <owl:Class rdf:about="http://stix.mitre.org/stixCommon#KillChain">
        <rdfs:subClassOf>
            <owl:Restriction>
                <owl:onProperty rdf:resource="http://stix.mitre.org/stixCommon#description"/>
                <owl:someValuesFrom rdf:resource="http://www.w3.org/2000/01/rdf-schema#Literal"/>
            </owl:Restriction>
        </rdfs:subClassOf>
        <rdfs:subClassOf>
            <owl:Restriction>
                <owl:onProperty rdf:resource="http://stix.mitre.org/stixCommon#externalReference"/>
                <owl:someValuesFrom rdf:resource="http://www.w3.org/2000/01/rdf-schema#Literal"/>
            </owl:Restriction>
        </rdfs:subClassOf>
        <rdfs:subClassOf>
            <owl:Restriction>
                <owl:onProperty rdf:resource="http://stix.mitre.org/stixCommon#id"/>
                <owl:someValuesFrom rdf:resource="http://www.w3.org/2000/01/rdf-schema#Literal"/>
            </owl:Restriction>
        </rdfs:subClassOf>
        <rdfs:subClassOf>
            <owl:Restriction>
                <owl:onProperty rdf:resource="http://stix.mitre.org/stixCommon#killChainDefiner"/>
                <owl:someValuesFrom rdf:resource="http://www.w3.org/2000/01/rdf-schema#Literal"/>
            </owl:Restriction>
        </rdfs:subClassOf>
        <rdfs:subClassOf>
            <owl:Restriction>
                <owl:onProperty rdf:resource="http://stix.mitre.org/stixCommon#killChainName"/>
                <owl:someValuesFrom rdf:resource="http://www.w3.org/2000/01/rdf-schema#Literal"/>
            </owl:Restriction>
        </rdfs:subClassOf>
        <rdfs:subClassOf>
            <owl:Restriction>
                <owl:onProperty rdf:resource="http://stix.mitre.org/stixCommon#numberOfPhases"/>
                <owl:someValuesFrom rdf:resource="http://www.w3.org/2000/01/rdf-schema#Literal"/>
            </owl:Restriction>
        </rdfs:subClassOf>
        <rdfs:comment>Characterizes a specific Kill Chain definition for reference within specific TTP entries, Indicators and elsewhere.</rdfs:comment>
        <rdfs:isDefinedBy rdf:resource="http://stix.mitre.org/stixCommon"/>
        <rdfs:label>Kill Chain</rdfs:label>
    </owl:Class>
    


    <!-- http://stix.mitre.org/stixCommon#KillChainPhase -->

    <owl:Class rdf:about="http://stix.mitre.org/stixCommon#KillChainPhase">
        <rdfs:subClassOf>
            <owl:Restriction>
                <owl:onProperty rdf:resource="http://stix.mitre.org/stixCommon#ordinalValue"/>
                <owl:someValuesFrom rdf:resource="http://www.w3.org/2000/01/rdf-schema#Literal"/>
            </owl:Restriction>
        </rdfs:subClassOf>
        <rdfs:subClassOf>
            <owl:Restriction>
                <owl:onProperty rdf:resource="http://stix.mitre.org/stixCommon#phaseDescription"/>
                <owl:someValuesFrom rdf:resource="http://www.w3.org/2000/01/rdf-schema#Literal"/>
            </owl:Restriction>
        </rdfs:subClassOf>
        <rdfs:subClassOf>
            <owl:Restriction>
                <owl:onProperty rdf:resource="http://stix.mitre.org/stixCommon#phaseId"/>
                <owl:someValuesFrom rdf:resource="http://www.w3.org/2000/01/rdf-schema#Literal"/>
            </owl:Restriction>
        </rdfs:subClassOf>
        <rdfs:subClassOf>
            <owl:Restriction>
                <owl:onProperty rdf:resource="http://stix.mitre.org/stixCommon#phaseName"/>
                <owl:someValuesFrom rdf:resource="http://www.w3.org/2000/01/rdf-schema#Literal"/>
            </owl:Restriction>
        </rdfs:subClassOf>
        <rdfs:comment>Characterizes an individual phase within a kill chain definition.</rdfs:comment>
        <rdfs:isDefinedBy rdf:resource="http://stix.mitre.org/stixCommon"/>
        <rdfs:label>Kill Chain Phase</rdfs:label>
    </owl:Class>
    


    <!-- http://stix.mitre.org/stixCommon#LikelyImpactStatement -->

    <owl:Class rdf:about="http://stix.mitre.org/stixCommon#LikelyImpactStatement">
        <rdfs:subClassOf rdf:resource="http://stix.mitre.org/stixCommon#Statement"/>
        <rdfs:subClassOf>
            <owl:Restriction>
                <owl:onProperty rdf:resource="http://stix.mitre.org/stixCommon#confidence.assertionChain"/>
                <owl:someValuesFrom rdf:resource="http://www.w3.org/2002/07/owl#Thing"/>
            </owl:Restriction>
        </rdfs:subClassOf>
        <rdfs:subClassOf>
            <owl:Restriction>
                <owl:onProperty rdf:resource="http://stix.mitre.org/stixCommon#confidence.source"/>
                <owl:someValuesFrom rdf:resource="http://www.w3.org/2002/07/owl#Thing"/>
            </owl:Restriction>
        </rdfs:subClassOf>
        <rdfs:subClassOf>
            <owl:Restriction>
                <owl:onProperty rdf:resource="http://stix.mitre.org/stixCommon#informationSource"/>
                <owl:someValuesFrom rdf:resource="http://www.w3.org/2002/07/owl#Thing"/>
            </owl:Restriction>
        </rdfs:subClassOf>
        <rdfs:subClassOf>
            <owl:Restriction>
                <owl:onProperty rdf:resource="http://stix.mitre.org/stixCommon#confidence.description"/>
                <owl:someValuesFrom rdf:resource="http://www.w3.org/2000/01/rdf-schema#Literal"/>
            </owl:Restriction>
        </rdfs:subClassOf>
        <rdfs:subClassOf>
            <owl:Restriction>
                <owl:onProperty rdf:resource="http://stix.mitre.org/stixCommon#confidence.timestamp"/>
                <owl:someValuesFrom rdf:resource="http://www.w3.org/2000/01/rdf-schema#Literal"/>
            </owl:Restriction>
        </rdfs:subClassOf>
        <rdfs:subClassOf>
            <owl:Restriction>
                <owl:onProperty rdf:resource="http://stix.mitre.org/stixCommon#confidence.timestampPrecision"/>
                <owl:someValuesFrom rdf:resource="http://www.w3.org/2000/01/rdf-schema#Literal"/>
            </owl:Restriction>
        </rdfs:subClassOf>
        <rdfs:subClassOf>
            <owl:Restriction>
                <owl:onProperty rdf:resource="http://stix.mitre.org/stixCommon#confidence.value"/>
                <owl:someValuesFrom rdf:resource="http://www.w3.org/2000/01/rdf-schema#Literal"/>
            </owl:Restriction>
        </rdfs:subClassOf>
        <rdfs:subClassOf>
            <owl:Restriction>
                <owl:onProperty rdf:resource="http://stix.mitre.org/stixCommon#description"/>
                <owl:someValuesFrom rdf:resource="http://www.w3.org/2000/01/rdf-schema#Literal"/>
            </owl:Restriction>
        </rdfs:subClassOf>
        <rdfs:subClassOf>
            <owl:Restriction>
                <owl:onProperty rdf:resource="http://stix.mitre.org/stixCommon#id"/>
                <owl:someValuesFrom rdf:resource="http://www.w3.org/2000/01/rdf-schema#Literal"/>
            </owl:Restriction>
        </rdfs:subClassOf>
        <rdfs:subClassOf>
            <owl:Restriction>
                <owl:onProperty rdf:resource="http://stix.mitre.org/stixCommon#likelyImpactValue"/>
                <owl:someValuesFrom rdf:resource="http://www.w3.org/2000/01/rdf-schema#Literal"/>
            </owl:Restriction>
        </rdfs:subClassOf>
        <rdfs:subClassOf>
            <owl:Restriction>
                <owl:onProperty rdf:resource="http://stix.mitre.org/stixCommon#timestamp"/>
                <owl:someValuesFrom rdf:resource="http://www.w3.org/2000/01/rdf-schema#Literal"/>
            </owl:Restriction>
        </rdfs:subClassOf>
        <rdfs:subClassOf>
            <owl:Restriction>
                <owl:onProperty rdf:resource="http://stix.mitre.org/stixCommon#timestampPrecision"/>
                <owl:someValuesFrom rdf:resource="http://www.w3.org/2000/01/rdf-schema#Literal"/>
            </owl:Restriction>
        </rdfs:subClassOf>
        <rdfs:comment>Characterizes a statement about the likely potential impact within the relevant context if this Indicator were to occur.

The LikelyImpactStatement class allows for the expression of a statement, a description of the statement, a confidence in the statement, and the source of the statement.</rdfs:comment>
        <rdfs:isDefinedBy rdf:resource="http://stix.mitre.org/stixCommon"/>
        <rdfs:label>Likely Impact Statement</rdfs:label>
    </owl:Class>
    


    <!-- http://stix.mitre.org/stixCommon#MotivationStatement -->

    <owl:Class rdf:about="http://stix.mitre.org/stixCommon#MotivationStatement">
        <rdfs:subClassOf rdf:resource="http://stix.mitre.org/stixCommon#Statement"/>
        <rdfs:subClassOf>
            <owl:Restriction>
                <owl:onProperty rdf:resource="http://stix.mitre.org/stixCommon#confidence.assertionChain"/>
                <owl:someValuesFrom rdf:resource="http://www.w3.org/2002/07/owl#Thing"/>
            </owl:Restriction>
        </rdfs:subClassOf>
        <rdfs:subClassOf>
            <owl:Restriction>
                <owl:onProperty rdf:resource="http://stix.mitre.org/stixCommon#confidence.source"/>
                <owl:someValuesFrom rdf:resource="http://www.w3.org/2002/07/owl#Thing"/>
            </owl:Restriction>
        </rdfs:subClassOf>
        <rdfs:subClassOf>
            <owl:Restriction>
                <owl:onProperty rdf:resource="http://stix.mitre.org/stixCommon#informationSource"/>
                <owl:someValuesFrom rdf:resource="http://www.w3.org/2002/07/owl#Thing"/>
            </owl:Restriction>
        </rdfs:subClassOf>
        <rdfs:subClassOf>
            <owl:Restriction>
                <owl:onProperty rdf:resource="http://stix.mitre.org/stixCommon#confidence.description"/>
                <owl:someValuesFrom rdf:resource="http://www.w3.org/2000/01/rdf-schema#Literal"/>
            </owl:Restriction>
        </rdfs:subClassOf>
        <rdfs:subClassOf>
            <owl:Restriction>
                <owl:onProperty rdf:resource="http://stix.mitre.org/stixCommon#confidence.timestamp"/>
                <owl:someValuesFrom rdf:resource="http://www.w3.org/2000/01/rdf-schema#Literal"/>
            </owl:Restriction>
        </rdfs:subClassOf>
        <rdfs:subClassOf>
            <owl:Restriction>
                <owl:onProperty rdf:resource="http://stix.mitre.org/stixCommon#confidence.timestampPrecision"/>
                <owl:someValuesFrom rdf:resource="http://www.w3.org/2000/01/rdf-schema#Literal"/>
            </owl:Restriction>
        </rdfs:subClassOf>
        <rdfs:subClassOf>
            <owl:Restriction>
                <owl:onProperty rdf:resource="http://stix.mitre.org/stixCommon#confidence.value"/>
                <owl:someValuesFrom rdf:resource="http://www.w3.org/2000/01/rdf-schema#Literal"/>
            </owl:Restriction>
        </rdfs:subClassOf>
        <rdfs:subClassOf>
            <owl:Restriction>
                <owl:onProperty rdf:resource="http://stix.mitre.org/stixCommon#description"/>
                <owl:someValuesFrom rdf:resource="http://www.w3.org/2000/01/rdf-schema#Literal"/>
            </owl:Restriction>
        </rdfs:subClassOf>
        <rdfs:subClassOf>
            <owl:Restriction>
                <owl:onProperty rdf:resource="http://stix.mitre.org/stixCommon#id"/>
                <owl:someValuesFrom rdf:resource="http://www.w3.org/2000/01/rdf-schema#Literal"/>
            </owl:Restriction>
        </rdfs:subClassOf>
        <rdfs:subClassOf>
            <owl:Restriction>
                <owl:onProperty rdf:resource="http://stix.mitre.org/stixCommon#motivationValue"/>
                <owl:someValuesFrom rdf:resource="http://www.w3.org/2000/01/rdf-schema#Literal"/>
            </owl:Restriction>
        </rdfs:subClassOf>
        <rdfs:subClassOf>
            <owl:Restriction>
                <owl:onProperty rdf:resource="http://stix.mitre.org/stixCommon#timestamp"/>
                <owl:someValuesFrom rdf:resource="http://www.w3.org/2000/01/rdf-schema#Literal"/>
            </owl:Restriction>
        </rdfs:subClassOf>
        <rdfs:subClassOf>
            <owl:Restriction>
                <owl:onProperty rdf:resource="http://stix.mitre.org/stixCommon#timestampPrecision"/>
                <owl:someValuesFrom rdf:resource="http://www.w3.org/2000/01/rdf-schema#Literal"/>
            </owl:Restriction>
        </rdfs:subClassOf>
        <rdfs:comment>Characterizes a statement about the motivations of a threat actor. 

The MotivationStatement class allows for the expression of a statement, a description of the statement, a confidence in the statement, and the source of the statement.</rdfs:comment>
        <rdfs:isDefinedBy rdf:resource="http://stix.mitre.org/stixCommon"/>
        <rdfs:label>Motivation Statement</rdfs:label>
    </owl:Class>
    


    <!-- http://stix.mitre.org/stixCommon#ObservableRelationship -->

    <owl:Class rdf:about="http://stix.mitre.org/stixCommon#ObservableRelationship">
        <rdfs:subClassOf rdf:resource="http://stix.mitre.org/stixCommon#RelationshipStatement"/>
        <rdfs:subClassOf>
            <owl:Restriction>
                <owl:onProperty rdf:resource="http://stix.mitre.org/stixCommon#confidence.assertionChain"/>
                <owl:someValuesFrom rdf:resource="http://www.w3.org/2002/07/owl#Thing"/>
            </owl:Restriction>
        </rdfs:subClassOf>
        <rdfs:subClassOf>
            <owl:Restriction>
                <owl:onProperty rdf:resource="http://stix.mitre.org/stixCommon#confidence.source"/>
                <owl:someValuesFrom rdf:resource="http://www.w3.org/2002/07/owl#Thing"/>
            </owl:Restriction>
        </rdfs:subClassOf>
        <rdfs:subClassOf>
            <owl:Restriction>
                <owl:onProperty rdf:resource="http://stix.mitre.org/stixCommon#relatedObservable"/>
                <owl:someValuesFrom rdf:resource="http://www.w3.org/2002/07/owl#Thing"/>
            </owl:Restriction>
        </rdfs:subClassOf>
        <rdfs:subClassOf>
            <owl:Restriction>
                <owl:onProperty rdf:resource="http://stix.mitre.org/stixCommon#confidence.description"/>
                <owl:someValuesFrom rdf:resource="http://www.w3.org/2000/01/rdf-schema#Literal"/>
            </owl:Restriction>
        </rdfs:subClassOf>
        <rdfs:subClassOf>
            <owl:Restriction>
                <owl:onProperty rdf:resource="http://stix.mitre.org/stixCommon#confidence.timestamp"/>
                <owl:someValuesFrom rdf:resource="http://www.w3.org/2000/01/rdf-schema#Literal"/>
            </owl:Restriction>
        </rdfs:subClassOf>
        <rdfs:subClassOf>
            <owl:Restriction>
                <owl:onProperty rdf:resource="http://stix.mitre.org/stixCommon#confidence.timestampPrecision"/>
                <owl:someValuesFrom rdf:resource="http://www.w3.org/2000/01/rdf-schema#Literal"/>
            </owl:Restriction>
        </rdfs:subClassOf>
        <rdfs:subClassOf>
            <owl:Restriction>
                <owl:onProperty rdf:resource="http://stix.mitre.org/stixCommon#confidence.value"/>
                <owl:someValuesFrom rdf:resource="http://www.w3.org/2000/01/rdf-schema#Literal"/>
            </owl:Restriction>
        </rdfs:subClassOf>
        <rdfs:subClassOf>
            <owl:Restriction>
                <owl:onProperty rdf:resource="http://stix.mitre.org/stixCommon#relationshipScope"/>
                <owl:someValuesFrom rdf:resource="http://www.w3.org/2000/01/rdf-schema#Literal"/>
            </owl:Restriction>
        </rdfs:subClassOf>
        <rdfs:subClassOf>
            <owl:Restriction>
                <owl:onProperty rdf:resource="http://stix.mitre.org/stixCommon#relationshipType"/>
                <owl:someValuesFrom rdf:resource="http://www.w3.org/2000/01/rdf-schema#Literal"/>
            </owl:Restriction>
        </rdfs:subClassOf>
        <rdfs:comment>Characterizes a relationship to a CybOX Observable.

The ObservableRelationship class is designed to support its use in representing the relationship attributes as an nary-relationship that can be associated with relationship between a subject STIX construct and a CybOX Observable through the use of the rdf:subject, rdf:predicate, and rdf:object properties.  The ObservableRelationship class inherits from the RelationshipStatement class but is extended with the relatedCampaign property that references an instance of the CybOX Observable class.

The ObservableRelationship class MUST only be used to represent the relationship&apos;s attributes as an nary-relationship.</rdfs:comment>
        <rdfs:isDefinedBy rdf:resource="http://stix.mitre.org/stixCommon"/>
        <rdfs:label>Observable Relationship</rdfs:label>
    </owl:Class>
    


    <!-- http://stix.mitre.org/stixCommon#PackageBase -->

    <owl:Class rdf:about="http://stix.mitre.org/stixCommon#PackageBase">
        <rdfs:subClassOf>
            <owl:Restriction>
                <owl:onProperty rdf:resource="http://stix.mitre.org/stixCommon#id"/>
                <owl:someValuesFrom rdf:resource="http://www.w3.org/2000/01/rdf-schema#Literal"/>
            </owl:Restriction>
        </rdfs:subClassOf>
        <rdfs:subClassOf>
            <owl:Restriction>
                <owl:onProperty rdf:resource="http://stix.mitre.org/stixCommon#timestamp"/>
                <owl:someValuesFrom rdf:resource="http://www.w3.org/2000/01/rdf-schema#Literal"/>
            </owl:Restriction>
        </rdfs:subClassOf>
        <rdfs:comment>Characterizes a based definition of information for a Package. 

The PackageBase class is an abstract class, so it MUST be extended via a subclass to express additional activity information. The definition of the base class in the STIX Common ontology minimizes the inter-dependencies between STIX components.  The default and strongly RECOMMENDED subclass to extend the PackageBase class is defined in the STIX Core ontology.</rdfs:comment>
        <rdfs:isDefinedBy rdf:resource="http://stix.mitre.org/stixCommon"/>
        <rdfs:label>Package base</rdfs:label>
    </owl:Class>
    


    <!-- http://stix.mitre.org/stixCommon#PackageRelationship -->

    <owl:Class rdf:about="http://stix.mitre.org/stixCommon#PackageRelationship">
        <rdfs:subClassOf rdf:resource="http://stix.mitre.org/stixCommon#RelationshipStatement"/>
        <rdfs:subClassOf>
            <owl:Restriction>
                <owl:onProperty rdf:resource="http://stix.mitre.org/stixCommon#confidence.assertionChain"/>
                <owl:someValuesFrom rdf:resource="http://www.w3.org/2002/07/owl#Thing"/>
            </owl:Restriction>
        </rdfs:subClassOf>
        <rdfs:subClassOf>
            <owl:Restriction>
                <owl:onProperty rdf:resource="http://stix.mitre.org/stixCommon#confidence.source"/>
                <owl:someValuesFrom rdf:resource="http://www.w3.org/2002/07/owl#Thing"/>
            </owl:Restriction>
        </rdfs:subClassOf>
        <rdfs:subClassOf>
            <owl:Restriction>
                <owl:onProperty rdf:resource="http://stix.mitre.org/stixCommon#relatedPackage"/>
                <owl:someValuesFrom rdf:resource="http://www.w3.org/2002/07/owl#Thing"/>
            </owl:Restriction>
        </rdfs:subClassOf>
        <rdfs:subClassOf>
            <owl:Restriction>
                <owl:onProperty rdf:resource="http://stix.mitre.org/stixCommon#confidence.description"/>
                <owl:someValuesFrom rdf:resource="http://www.w3.org/2000/01/rdf-schema#Literal"/>
            </owl:Restriction>
        </rdfs:subClassOf>
        <rdfs:subClassOf>
            <owl:Restriction>
                <owl:onProperty rdf:resource="http://stix.mitre.org/stixCommon#confidence.timestamp"/>
                <owl:someValuesFrom rdf:resource="http://www.w3.org/2000/01/rdf-schema#Literal"/>
            </owl:Restriction>
        </rdfs:subClassOf>
        <rdfs:subClassOf>
            <owl:Restriction>
                <owl:onProperty rdf:resource="http://stix.mitre.org/stixCommon#confidence.timestampPrecision"/>
                <owl:someValuesFrom rdf:resource="http://www.w3.org/2000/01/rdf-schema#Literal"/>
            </owl:Restriction>
        </rdfs:subClassOf>
        <rdfs:subClassOf>
            <owl:Restriction>
                <owl:onProperty rdf:resource="http://stix.mitre.org/stixCommon#confidence.value"/>
                <owl:someValuesFrom rdf:resource="http://www.w3.org/2000/01/rdf-schema#Literal"/>
            </owl:Restriction>
        </rdfs:subClassOf>
        <rdfs:subClassOf>
            <owl:Restriction>
                <owl:onProperty rdf:resource="http://stix.mitre.org/stixCommon#relationshipScope"/>
                <owl:someValuesFrom rdf:resource="http://www.w3.org/2000/01/rdf-schema#Literal"/>
            </owl:Restriction>
        </rdfs:subClassOf>
        <rdfs:subClassOf>
            <owl:Restriction>
                <owl:onProperty rdf:resource="http://stix.mitre.org/stixCommon#relationshipType"/>
                <owl:someValuesFrom rdf:resource="http://www.w3.org/2000/01/rdf-schema#Literal"/>
            </owl:Restriction>
        </rdfs:subClassOf>
        <rdfs:comment>Characterizes a relationship to a STIX Package. 

The PackageRelationship class is designed to support its use in representing the relationship attributes as an nary-relationship that can be associated with relationship between a subject STIX construct and a STIX Package through the use of the rdf:subject, rdf:predicate, and rdf:object properties.  The PackageRelationship class inherits from the RelationshipStatement class but is extended with the relatedPackage property that references an instance of the PackageBase class or one of its subclasses.

The PackageRelationship class MUST only be used to represent the relationship&apos;s attributes as an nary-relationship.</rdfs:comment>
        <rdfs:isDefinedBy rdf:resource="http://stix.mitre.org/stixCommon"/>
        <rdfs:label>Package Relationship</rdfs:label>
    </owl:Class>
    


    <!-- http://stix.mitre.org/stixCommon#PlanningAndOperationalSupportStatement -->

    <owl:Class rdf:about="http://stix.mitre.org/stixCommon#PlanningAndOperationalSupportStatement">
        <rdfs:subClassOf rdf:resource="http://stix.mitre.org/stixCommon#Statement"/>
        <rdfs:subClassOf>
            <owl:Restriction>
                <owl:onProperty rdf:resource="http://stix.mitre.org/stixCommon#confidence.assertionChain"/>
                <owl:someValuesFrom rdf:resource="http://www.w3.org/2002/07/owl#Thing"/>
            </owl:Restriction>
        </rdfs:subClassOf>
        <rdfs:subClassOf>
            <owl:Restriction>
                <owl:onProperty rdf:resource="http://stix.mitre.org/stixCommon#confidence.source"/>
                <owl:someValuesFrom rdf:resource="http://www.w3.org/2002/07/owl#Thing"/>
            </owl:Restriction>
        </rdfs:subClassOf>
        <rdfs:subClassOf>
            <owl:Restriction>
                <owl:onProperty rdf:resource="http://stix.mitre.org/stixCommon#informationSource"/>
                <owl:someValuesFrom rdf:resource="http://www.w3.org/2002/07/owl#Thing"/>
            </owl:Restriction>
        </rdfs:subClassOf>
        <rdfs:subClassOf>
            <owl:Restriction>
                <owl:onProperty rdf:resource="http://stix.mitre.org/stixCommon#confidence.description"/>
                <owl:someValuesFrom rdf:resource="http://www.w3.org/2000/01/rdf-schema#Literal"/>
            </owl:Restriction>
        </rdfs:subClassOf>
        <rdfs:subClassOf>
            <owl:Restriction>
                <owl:onProperty rdf:resource="http://stix.mitre.org/stixCommon#confidence.timestamp"/>
                <owl:someValuesFrom rdf:resource="http://www.w3.org/2000/01/rdf-schema#Literal"/>
            </owl:Restriction>
        </rdfs:subClassOf>
        <rdfs:subClassOf>
            <owl:Restriction>
                <owl:onProperty rdf:resource="http://stix.mitre.org/stixCommon#confidence.timestampPrecision"/>
                <owl:someValuesFrom rdf:resource="http://www.w3.org/2000/01/rdf-schema#Literal"/>
            </owl:Restriction>
        </rdfs:subClassOf>
        <rdfs:subClassOf>
            <owl:Restriction>
                <owl:onProperty rdf:resource="http://stix.mitre.org/stixCommon#confidence.value"/>
                <owl:someValuesFrom rdf:resource="http://www.w3.org/2000/01/rdf-schema#Literal"/>
            </owl:Restriction>
        </rdfs:subClassOf>
        <rdfs:subClassOf>
            <owl:Restriction>
                <owl:onProperty rdf:resource="http://stix.mitre.org/stixCommon#description"/>
                <owl:someValuesFrom rdf:resource="http://www.w3.org/2000/01/rdf-schema#Literal"/>
            </owl:Restriction>
        </rdfs:subClassOf>
        <rdfs:subClassOf>
            <owl:Restriction>
                <owl:onProperty rdf:resource="http://stix.mitre.org/stixCommon#id"/>
                <owl:someValuesFrom rdf:resource="http://www.w3.org/2000/01/rdf-schema#Literal"/>
            </owl:Restriction>
        </rdfs:subClassOf>
        <rdfs:subClassOf>
            <owl:Restriction>
                <owl:onProperty rdf:resource="http://stix.mitre.org/stixCommon#planningAndOpSupportValue"/>
                <owl:someValuesFrom rdf:resource="http://www.w3.org/2000/01/rdf-schema#Literal"/>
            </owl:Restriction>
        </rdfs:subClassOf>
        <rdfs:subClassOf>
            <owl:Restriction>
                <owl:onProperty rdf:resource="http://stix.mitre.org/stixCommon#timestamp"/>
                <owl:someValuesFrom rdf:resource="http://www.w3.org/2000/01/rdf-schema#Literal"/>
            </owl:Restriction>
        </rdfs:subClassOf>
        <rdfs:subClassOf>
            <owl:Restriction>
                <owl:onProperty rdf:resource="http://stix.mitre.org/stixCommon#timestampPrecision"/>
                <owl:someValuesFrom rdf:resource="http://www.w3.org/2000/01/rdf-schema#Literal"/>
            </owl:Restriction>
        </rdfs:subClassOf>
        <rdfs:comment>Characterizes a statement about the suspected planning and operational support performed by a threat actor.

The PlanningAndOperationalSupportStatement class allows for the expression of a statement, a description of the statement, a confidence in the statement, and the source of the statement.</rdfs:comment>
        <rdfs:isDefinedBy rdf:resource="http://stix.mitre.org/stixCommon"/>
        <rdfs:label>Planning and Operational Support Statement</rdfs:label>
    </owl:Class>
    


    <!-- http://stix.mitre.org/stixCommon#RelationshipStatement -->

    <owl:Class rdf:about="http://stix.mitre.org/stixCommon#RelationshipStatement">
        <rdfs:subClassOf rdf:resource="http://www.w3.org/1999/02/22-rdf-syntax-ns#Statement"/>
        <rdfs:subClassOf>
            <owl:Restriction>
                <owl:onProperty rdf:resource="http://stix.mitre.org/stixCommon#confidence.assertionChain"/>
                <owl:someValuesFrom rdf:resource="http://www.w3.org/2002/07/owl#Thing"/>
            </owl:Restriction>
        </rdfs:subClassOf>
        <rdfs:subClassOf>
            <owl:Restriction>
                <owl:onProperty rdf:resource="http://stix.mitre.org/stixCommon#confidence.source"/>
                <owl:someValuesFrom rdf:resource="http://www.w3.org/2002/07/owl#Thing"/>
            </owl:Restriction>
        </rdfs:subClassOf>
        <rdfs:subClassOf>
            <owl:Restriction>
                <owl:onProperty rdf:resource="http://stix.mitre.org/stixCommon#infoSource.identity"/>
                <owl:someValuesFrom rdf:resource="http://www.w3.org/2002/07/owl#Thing"/>
            </owl:Restriction>
        </rdfs:subClassOf>
        <rdfs:subClassOf>
            <owl:Restriction>
                <owl:onProperty rdf:resource="http://stix.mitre.org/stixCommon#confidence.description"/>
                <owl:someValuesFrom rdf:resource="http://www.w3.org/2000/01/rdf-schema#Literal"/>
            </owl:Restriction>
        </rdfs:subClassOf>
        <rdfs:subClassOf>
            <owl:Restriction>
                <owl:onProperty rdf:resource="http://stix.mitre.org/stixCommon#confidence.timestamp"/>
                <owl:someValuesFrom rdf:resource="http://www.w3.org/2000/01/rdf-schema#Literal"/>
            </owl:Restriction>
        </rdfs:subClassOf>
        <rdfs:subClassOf>
            <owl:Restriction>
                <owl:onProperty rdf:resource="http://stix.mitre.org/stixCommon#confidence.timestampPrecision"/>
                <owl:someValuesFrom rdf:resource="http://www.w3.org/2000/01/rdf-schema#Literal"/>
            </owl:Restriction>
        </rdfs:subClassOf>
        <rdfs:subClassOf>
            <owl:Restriction>
                <owl:onProperty rdf:resource="http://stix.mitre.org/stixCommon#confidence.value"/>
                <owl:someValuesFrom rdf:resource="http://www.w3.org/2000/01/rdf-schema#Literal"/>
            </owl:Restriction>
        </rdfs:subClassOf>
        <rdfs:subClassOf>
            <owl:Restriction>
                <owl:onProperty rdf:resource="http://stix.mitre.org/stixCommon#infoSource.description"/>
                <owl:someValuesFrom rdf:resource="http://www.w3.org/2000/01/rdf-schema#Literal"/>
            </owl:Restriction>
        </rdfs:subClassOf>
        <rdfs:subClassOf>
            <owl:Restriction>
                <owl:onProperty rdf:resource="http://stix.mitre.org/stixCommon#relationshipScope"/>
                <owl:someValuesFrom rdf:resource="http://www.w3.org/2000/01/rdf-schema#Literal"/>
            </owl:Restriction>
        </rdfs:subClassOf>
        <rdfs:subClassOf>
            <owl:Restriction>
                <owl:onProperty rdf:resource="http://stix.mitre.org/stixCommon#relationshipType"/>
                <owl:someValuesFrom rdf:resource="http://www.w3.org/2000/01/rdf-schema#Literal"/>
            </owl:Restriction>
        </rdfs:subClassOf>
        <rdfs:comment>Characterizes the attributes associated with a relationship between a subject STIX construct and another STIX construct.

The definition of the base class in the STIX Common ontology minimizes the inter-dependencies between STIX components and helps to define a consistent structure for relationships that go beyond a simple statement of &quot;construct A is related to construct B&quot;.  Instead, additional properties ofthe relationship can be specified such as the nature of the relationship and the level of confidence in the presence and accuracy of the asserted relationship.

The RelationshipStatement class is designed to support its use in representing the relationship attributes as reified data or as a nary-relationship that can be associated with relationship between a subject STIX construct and another STIX construct through the use of the rdf:subject, rdf:predicate, and rdf:object properties.</rdfs:comment>
        <rdfs:isDefinedBy rdf:resource="http://stix.mitre.org/stixCommon"/>
        <rdfs:label>Relationship Statement</rdfs:label>
    </owl:Class>
    


    <!-- http://stix.mitre.org/stixCommon#ReportBase -->

    <owl:Class rdf:about="http://stix.mitre.org/stixCommon#ReportBase">
        <rdfs:subClassOf>
            <owl:Restriction>
                <owl:onProperty rdf:resource="http://stix.mitre.org/stixCommon#id"/>
                <owl:someValuesFrom rdf:resource="http://www.w3.org/2000/01/rdf-schema#Literal"/>
            </owl:Restriction>
        </rdfs:subClassOf>
        <rdfs:subClassOf>
            <owl:Restriction>
                <owl:onProperty rdf:resource="http://stix.mitre.org/stixCommon#timestamp"/>
                <owl:someValuesFrom rdf:resource="http://www.w3.org/2000/01/rdf-schema#Literal"/>
            </owl:Restriction>
        </rdfs:subClassOf>
        <rdfs:comment>Characterizes a based definition of information for a Report. 

The ReportBase class is an abstract class, so it MUST be extended via a subclass to express additional activity information. The definition of the base class in the STIX Common ontology minimizes the inter-dependencies between STIX components.  The default and strongly RECOMMENDED subclass to extend the ReportBase class is defined in the STIX Report ontology.</rdfs:comment>
        <rdfs:isDefinedBy rdf:resource="http://stix.mitre.org/stixCommon"/>
        <rdfs:label>Report Base</rdfs:label>
    </owl:Class>
    


    <!-- http://stix.mitre.org/stixCommon#SophisticationStatement -->

    <owl:Class rdf:about="http://stix.mitre.org/stixCommon#SophisticationStatement">
        <rdfs:subClassOf rdf:resource="http://stix.mitre.org/stixCommon#Statement"/>
        <rdfs:subClassOf>
            <owl:Restriction>
                <owl:onProperty rdf:resource="http://stix.mitre.org/stixCommon#confidence.assertionChain"/>
                <owl:someValuesFrom rdf:resource="http://www.w3.org/2002/07/owl#Thing"/>
            </owl:Restriction>
        </rdfs:subClassOf>
        <rdfs:subClassOf>
            <owl:Restriction>
                <owl:onProperty rdf:resource="http://stix.mitre.org/stixCommon#confidence.source"/>
                <owl:someValuesFrom rdf:resource="http://www.w3.org/2002/07/owl#Thing"/>
            </owl:Restriction>
        </rdfs:subClassOf>
        <rdfs:subClassOf>
            <owl:Restriction>
                <owl:onProperty rdf:resource="http://stix.mitre.org/stixCommon#informationSource"/>
                <owl:someValuesFrom rdf:resource="http://www.w3.org/2002/07/owl#Thing"/>
            </owl:Restriction>
        </rdfs:subClassOf>
        <rdfs:subClassOf>
            <owl:Restriction>
                <owl:onProperty rdf:resource="http://stix.mitre.org/stixCommon#confidence.description"/>
                <owl:someValuesFrom rdf:resource="http://www.w3.org/2000/01/rdf-schema#Literal"/>
            </owl:Restriction>
        </rdfs:subClassOf>
        <rdfs:subClassOf>
            <owl:Restriction>
                <owl:onProperty rdf:resource="http://stix.mitre.org/stixCommon#confidence.timestamp"/>
                <owl:someValuesFrom rdf:resource="http://www.w3.org/2000/01/rdf-schema#Literal"/>
            </owl:Restriction>
        </rdfs:subClassOf>
        <rdfs:subClassOf>
            <owl:Restriction>
                <owl:onProperty rdf:resource="http://stix.mitre.org/stixCommon#confidence.timestampPrecision"/>
                <owl:someValuesFrom rdf:resource="http://www.w3.org/2000/01/rdf-schema#Literal"/>
            </owl:Restriction>
        </rdfs:subClassOf>
        <rdfs:subClassOf>
            <owl:Restriction>
                <owl:onProperty rdf:resource="http://stix.mitre.org/stixCommon#confidence.value"/>
                <owl:someValuesFrom rdf:resource="http://www.w3.org/2000/01/rdf-schema#Literal"/>
            </owl:Restriction>
        </rdfs:subClassOf>
        <rdfs:subClassOf>
            <owl:Restriction>
                <owl:onProperty rdf:resource="http://stix.mitre.org/stixCommon#description"/>
                <owl:someValuesFrom rdf:resource="http://www.w3.org/2000/01/rdf-schema#Literal"/>
            </owl:Restriction>
        </rdfs:subClassOf>
        <rdfs:subClassOf>
            <owl:Restriction>
                <owl:onProperty rdf:resource="http://stix.mitre.org/stixCommon#id"/>
                <owl:someValuesFrom rdf:resource="http://www.w3.org/2000/01/rdf-schema#Literal"/>
            </owl:Restriction>
        </rdfs:subClassOf>
        <rdfs:subClassOf>
            <owl:Restriction>
                <owl:onProperty rdf:resource="http://stix.mitre.org/stixCommon#sophisticationValue"/>
                <owl:someValuesFrom rdf:resource="http://www.w3.org/2000/01/rdf-schema#Literal"/>
            </owl:Restriction>
        </rdfs:subClassOf>
        <rdfs:subClassOf>
            <owl:Restriction>
                <owl:onProperty rdf:resource="http://stix.mitre.org/stixCommon#timestamp"/>
                <owl:someValuesFrom rdf:resource="http://www.w3.org/2000/01/rdf-schema#Literal"/>
            </owl:Restriction>
        </rdfs:subClassOf>
        <rdfs:subClassOf>
            <owl:Restriction>
                <owl:onProperty rdf:resource="http://stix.mitre.org/stixCommon#timestampPrecision"/>
                <owl:someValuesFrom rdf:resource="http://www.w3.org/2000/01/rdf-schema#Literal"/>
            </owl:Restriction>
        </rdfs:subClassOf>
        <rdfs:comment>Characterizes a statement about the sophistication of a Threat Actor.

The SophisticationStatement class allows for the expression of a statement, a description of the statement, a confidence in the statement, and the source of the statement.</rdfs:comment>
        <rdfs:isDefinedBy rdf:resource="http://stix.mitre.org/stixCommon"/>
        <rdfs:label>Threat Actor Sophistication Statement</rdfs:label>
    </owl:Class>
    


    <!-- http://stix.mitre.org/stixCommon#Statement -->

    <owl:Class rdf:about="http://stix.mitre.org/stixCommon#Statement">
	<rdfs:subClassOf>
            <owl:Restriction>
                <owl:onProperty rdf:resource="http://stix.mitre.org/stixCommon#confidence.assertionChain"/>
                <owl:someValuesFrom rdf:resource="http://www.w3.org/2002/07/owl#Thing"/>
            </owl:Restriction>
        </rdfs:subClassOf>
        <rdfs:subClassOf>
            <owl:Restriction>
                <owl:onProperty rdf:resource="http://stix.mitre.org/stixCommon#confidence.source"/>
                <owl:someValuesFrom rdf:resource="http://www.w3.org/2002/07/owl#Thing"/>
            </owl:Restriction>
        </rdfs:subClassOf>
        <rdfs:subClassOf>
            <owl:Restriction>
                <owl:onProperty rdf:resource="http://stix.mitre.org/stixCommon#informationSource"/>
                <owl:someValuesFrom rdf:resource="http://www.w3.org/2002/07/owl#Thing"/>
            </owl:Restriction>
        </rdfs:subClassOf>
        <rdfs:subClassOf>
            <owl:Restriction>
                <owl:onProperty rdf:resource="http://stix.mitre.org/stixCommon#confidence.description"/>
                <owl:someValuesFrom rdf:resource="http://www.w3.org/2000/01/rdf-schema#Literal"/>
            </owl:Restriction>
        </rdfs:subClassOf>
        <rdfs:subClassOf>
            <owl:Restriction>
                <owl:onProperty rdf:resource="http://stix.mitre.org/stixCommon#confidence.timestamp"/>
                <owl:someValuesFrom rdf:resource="http://www.w3.org/2000/01/rdf-schema#Literal"/>
            </owl:Restriction>
        </rdfs:subClassOf>
        <rdfs:subClassOf>
            <owl:Restriction>
                <owl:onProperty rdf:resource="http://stix.mitre.org/stixCommon#confidence.timestampPrecision"/>
                <owl:someValuesFrom rdf:resource="http://www.w3.org/2000/01/rdf-schema#Literal"/>
            </owl:Restriction>
        </rdfs:subClassOf>
        <rdfs:subClassOf>
            <owl:Restriction>
                <owl:onProperty rdf:resource="http://stix.mitre.org/stixCommon#confidence.value"/>
                <owl:someValuesFrom rdf:resource="http://www.w3.org/2000/01/rdf-schema#Literal"/>
            </owl:Restriction>
        </rdfs:subClassOf>
        <rdfs:subClassOf>
            <owl:Restriction>
                <owl:onProperty rdf:resource="http://stix.mitre.org/stixCommon#description"/>
                <owl:someValuesFrom rdf:resource="http://www.w3.org/2000/01/rdf-schema#Literal"/>
            </owl:Restriction>
        </rdfs:subClassOf>
        <rdfs:subClassOf>
            <owl:Restriction>
                <owl:onProperty rdf:resource="http://stix.mitre.org/stixCommon#id"/>
                <owl:someValuesFrom rdf:resource="http://www.w3.org/2000/01/rdf-schema#Literal"/>
            </owl:Restriction>
        </rdfs:subClassOf>
        <rdfs:subClassOf>
            <owl:Restriction>
                <owl:onProperty rdf:resource="http://stix.mitre.org/stixCommon#statementValue"/>
                <owl:someValuesFrom rdf:resource="http://www.w3.org/2000/01/rdf-schema#Literal"/>
            </owl:Restriction>
        </rdfs:subClassOf>
        <rdfs:subClassOf>
            <owl:Restriction>
                <owl:onProperty rdf:resource="http://stix.mitre.org/stixCommon#timestamp"/>
                <owl:someValuesFrom rdf:resource="http://www.w3.org/2000/01/rdf-schema#Literal"/>
            </owl:Restriction>
        </rdfs:subClassOf>
        <rdfs:subClassOf>
            <owl:Restriction>
                <owl:onProperty rdf:resource="http://stix.mitre.org/stixCommon#timestampPrecision"/>
                <owl:someValuesFrom rdf:resource="http://www.w3.org/2000/01/rdf-schema#Literal"/>
            </owl:Restriction>
        </rdfs:subClassOf>
        <rdfs:comment>Characterizes the expression of a statement with an associated value, description, source, confidence, and timestamp.</rdfs:comment>
        <rdfs:isDefinedBy rdf:resource="http://stix.mitre.org/stixCommon"/>
        <rdfs:label>Statement</rdfs:label>
    </owl:Class>
    


    <!-- http://stix.mitre.org/stixCommon#TTPBase -->

    <owl:Class rdf:about="http://stix.mitre.org/stixCommon#TTPBase">
        <rdfs:subClassOf>
            <owl:Restriction>
                <owl:onProperty rdf:resource="http://stix.mitre.org/stixCommon#id"/>
                <owl:cardinality rdf:datatype="http://www.w3.org/2001/XMLSchema#nonNegativeInteger">1</owl:cardinality>
            </owl:Restriction>
        </rdfs:subClassOf>
        <rdfs:subClassOf>
            <owl:Restriction>
                <owl:onProperty rdf:resource="http://stix.mitre.org/stixCommon#timestamp"/>
                <owl:cardinality rdf:datatype="http://www.w3.org/2001/XMLSchema#nonNegativeInteger">1</owl:cardinality>
            </owl:Restriction>
        </rdfs:subClassOf>
        <rdfs:comment>Characterizes a based definition of information for a TTP. 

The TTPBase class is an abstract class, so it MUST be extended via a subclass to express additional activity information. The definition of the base class in the STIX Common ontology minimizes the inter-dependencies between STIX components.  The default and strongly RECOMMENDED subclass to extend the TTPBase class is defined in the STIX TTP ontology. {@en-US}</rdfs:comment>
        <rdfs:isDefinedBy rdf:resource="http://stix.mitre.org/stixCommon"/>
        <rdfs:label>TTP Base</rdfs:label>
    </owl:Class>
    


    <!-- http://stix.mitre.org/stixCommon#TTPRelationship -->

    <owl:Class rdf:about="http://stix.mitre.org/stixCommon#TTPRelationship">
        <rdfs:subClassOf rdf:resource="http://stix.mitre.org/stixCommon#RelationshipStatement"/>
        <rdfs:subClassOf>
            <owl:Restriction>
                <owl:onProperty rdf:resource="http://stix.mitre.org/stixCommon#confidence.assertionChain"/>
                <owl:someValuesFrom rdf:resource="http://www.w3.org/2002/07/owl#Thing"/>
            </owl:Restriction>
        </rdfs:subClassOf>
        <rdfs:subClassOf>
            <owl:Restriction>
                <owl:onProperty rdf:resource="http://stix.mitre.org/stixCommon#confidence.source"/>
                <owl:someValuesFrom rdf:resource="http://www.w3.org/2002/07/owl#Thing"/>
            </owl:Restriction>
        </rdfs:subClassOf>
        <rdfs:subClassOf>
            <owl:Restriction>
                <owl:onProperty rdf:resource="http://stix.mitre.org/stixCommon#relatedTTP"/>
                <owl:someValuesFrom rdf:resource="http://www.w3.org/2002/07/owl#Thing"/>
            </owl:Restriction>
        </rdfs:subClassOf>
        <rdfs:subClassOf>
            <owl:Restriction>
                <owl:onProperty rdf:resource="http://stix.mitre.org/stixCommon#confidence.description"/>
                <owl:someValuesFrom rdf:resource="http://www.w3.org/2000/01/rdf-schema#Literal"/>
            </owl:Restriction>
        </rdfs:subClassOf>
        <rdfs:subClassOf>
            <owl:Restriction>
                <owl:onProperty rdf:resource="http://stix.mitre.org/stixCommon#confidence.timestamp"/>
                <owl:someValuesFrom rdf:resource="http://www.w3.org/2000/01/rdf-schema#Literal"/>
            </owl:Restriction>
        </rdfs:subClassOf>
        <rdfs:subClassOf>
            <owl:Restriction>
                <owl:onProperty rdf:resource="http://stix.mitre.org/stixCommon#confidence.timestampPrecision"/>
                <owl:someValuesFrom rdf:resource="http://www.w3.org/2000/01/rdf-schema#Literal"/>
            </owl:Restriction>
        </rdfs:subClassOf>
        <rdfs:subClassOf>
            <owl:Restriction>
                <owl:onProperty rdf:resource="http://stix.mitre.org/stixCommon#confidence.value"/>
                <owl:someValuesFrom rdf:resource="http://www.w3.org/2000/01/rdf-schema#Literal"/>
            </owl:Restriction>
        </rdfs:subClassOf>
        <rdfs:subClassOf>
            <owl:Restriction>
                <owl:onProperty rdf:resource="http://stix.mitre.org/stixCommon#relationshipScope"/>
                <owl:someValuesFrom rdf:resource="http://www.w3.org/2000/01/rdf-schema#Literal"/>
            </owl:Restriction>
        </rdfs:subClassOf>
        <rdfs:subClassOf>
            <owl:Restriction>
                <owl:onProperty rdf:resource="http://stix.mitre.org/stixCommon#relationshipType"/>
                <owl:someValuesFrom rdf:resource="http://www.w3.org/2000/01/rdf-schema#Literal"/>
            </owl:Restriction>
        </rdfs:subClassOf>
        <rdfs:comment>Characterizes a relationship to a TTP. 

The TTPRelationship class is designed to support its use in representing the relationship attributes as an nary-relationship that can be associated with relationship between a subject STIX construct and a STIX TTP through the use of the rdf:subject, rdf:predicate, and rdf:object properties.  The TTPRelationship class inherits from the RelationshipStatement class but is extended with the relatedTTP property that references an instance of the TTPBase class or one of its subclasses.

The TTPRelationship class MUST only be used to represent the relationship&apos;s attributes as an nary-relationship.</rdfs:comment>
        <rdfs:isDefinedBy rdf:resource="http://stix.mitre.org/stixCommon"/>
        <rdfs:label>TTP Relationship</rdfs:label>
    </owl:Class>
    


    <!-- http://stix.mitre.org/stixCommon#ThreatActorBase -->

    <owl:Class rdf:about="http://stix.mitre.org/stixCommon#ThreatActorBase">
        <rdfs:subClassOf>
            <owl:Restriction>
                <owl:onProperty rdf:resource="http://stix.mitre.org/stixCommon#id"/>
                <owl:someValuesFrom rdf:resource="http://www.w3.org/2000/01/rdf-schema#Literal"/>
            </owl:Restriction>
        </rdfs:subClassOf>
        <rdfs:subClassOf>
            <owl:Restriction>
                <owl:onProperty rdf:resource="http://stix.mitre.org/stixCommon#timestamp"/>
                <owl:someValuesFrom rdf:resource="http://www.w3.org/2000/01/rdf-schema#Literal"/>
            </owl:Restriction>
        </rdfs:subClassOf>
        <rdfs:comment>Characterizes a based definition of information for a ThreatActor. 

The ThreatActorBase class is an abstract class, so it MUST be extended via a subclass to express additional activity information. The definition of the base class in the STIX Common ontology minimizes the inter-dependencies between STIX components.  The default and strongly RECOMMENDED subclass to extend the ThreatActorBase class is defined in the STIX Threat Actor ontology.</rdfs:comment>
        <rdfs:isDefinedBy rdf:resource="http://stix.mitre.org/stixCommon"/>
        <rdfs:label>Threat Actor Base</rdfs:label>
    </owl:Class>
    


    <!-- http://stix.mitre.org/stixCommon#ThreatActorRelationship -->

    <owl:Class rdf:about="http://stix.mitre.org/stixCommon#ThreatActorRelationship">
        <rdfs:subClassOf rdf:resource="http://stix.mitre.org/stixCommon#RelationshipStatement"/>
        <rdfs:subClassOf>
            <owl:Restriction>
                <owl:onProperty rdf:resource="http://stix.mitre.org/stixCommon#confidence.assertionChain"/>
                <owl:someValuesFrom rdf:resource="http://www.w3.org/2002/07/owl#Thing"/>
            </owl:Restriction>
        </rdfs:subClassOf>
        <rdfs:subClassOf>
            <owl:Restriction>
                <owl:onProperty rdf:resource="http://stix.mitre.org/stixCommon#confidence.source"/>
                <owl:someValuesFrom rdf:resource="http://www.w3.org/2002/07/owl#Thing"/>
            </owl:Restriction>
        </rdfs:subClassOf>
        <rdfs:subClassOf>
            <owl:Restriction>
                <owl:onProperty rdf:resource="http://stix.mitre.org/stixCommon#relatedThreatActor"/>
                <owl:someValuesFrom rdf:resource="http://www.w3.org/2002/07/owl#Thing"/>
            </owl:Restriction>
        </rdfs:subClassOf>
        <rdfs:subClassOf>
            <owl:Restriction>
                <owl:onProperty rdf:resource="http://stix.mitre.org/stixCommon#confidence.description"/>
                <owl:someValuesFrom rdf:resource="http://www.w3.org/2000/01/rdf-schema#Literal"/>
            </owl:Restriction>
        </rdfs:subClassOf>
        <rdfs:subClassOf>
            <owl:Restriction>
                <owl:onProperty rdf:resource="http://stix.mitre.org/stixCommon#confidence.timestamp"/>
                <owl:someValuesFrom rdf:resource="http://www.w3.org/2000/01/rdf-schema#Literal"/>
            </owl:Restriction>
        </rdfs:subClassOf>
        <rdfs:subClassOf>
            <owl:Restriction>
                <owl:onProperty rdf:resource="http://stix.mitre.org/stixCommon#confidence.timestampPrecision"/>
                <owl:someValuesFrom rdf:resource="http://www.w3.org/2000/01/rdf-schema#Literal"/>
            </owl:Restriction>
        </rdfs:subClassOf>
        <rdfs:subClassOf>
            <owl:Restriction>
                <owl:onProperty rdf:resource="http://stix.mitre.org/stixCommon#confidence.value"/>
                <owl:someValuesFrom rdf:resource="http://www.w3.org/2000/01/rdf-schema#Literal"/>
            </owl:Restriction>
        </rdfs:subClassOf>
        <rdfs:subClassOf>
            <owl:Restriction>
                <owl:onProperty rdf:resource="http://stix.mitre.org/stixCommon#relationshipScope"/>
                <owl:someValuesFrom rdf:resource="http://www.w3.org/2000/01/rdf-schema#Literal"/>
            </owl:Restriction>
        </rdfs:subClassOf>
        <rdfs:subClassOf>
            <owl:Restriction>
                <owl:onProperty rdf:resource="http://stix.mitre.org/stixCommon#relationshipType"/>
                <owl:someValuesFrom rdf:resource="http://www.w3.org/2000/01/rdf-schema#Literal"/>
            </owl:Restriction>
        </rdfs:subClassOf>
        <rdfs:comment>Characterizes a relationship to a Threat Actor.

The ThreatActorRelationship class is designed to support its use in representing the relationship attributes as an nary-relationship that can be associated with relationship between a subject STIX construct and a STIX Threat Actor through the use of the rdf:subject, rdf:predicate, and rdf:object properties.  The ThreatActorRelationship class inherits from the RelationshipStatement class but is extended with the relatedThreatActor property that references an instance of the ThreatActorBase class or one of its subclasses.

The ThreatActorRelationship class MUST only be used to represent the relationship&apos;s attributes as an nary-relationship.</rdfs:comment>
        <rdfs:isDefinedBy rdf:resource="http://stix.mitre.org/stixCommon"/>
        <rdfs:label>Threat Actor Relationship</rdfs:label>
    </owl:Class>
    


    <!-- http://stix.mitre.org/stixCommon#ThreatActorTypeStatement -->

    <owl:Class rdf:about="http://stix.mitre.org/stixCommon#ThreatActorTypeStatement">
        <rdfs:subClassOf rdf:resource="http://stix.mitre.org/stixCommon#Statement"/>
        <rdfs:subClassOf>
            <owl:Restriction>
                <owl:onProperty rdf:resource="http://stix.mitre.org/stixCommon#confidence.assertionChain"/>
                <owl:someValuesFrom rdf:resource="http://www.w3.org/2002/07/owl#Thing"/>
            </owl:Restriction>
        </rdfs:subClassOf>
        <rdfs:subClassOf>
            <owl:Restriction>
                <owl:onProperty rdf:resource="http://stix.mitre.org/stixCommon#confidence.source"/>
                <owl:someValuesFrom rdf:resource="http://www.w3.org/2002/07/owl#Thing"/>
            </owl:Restriction>
        </rdfs:subClassOf>
        <rdfs:subClassOf>
            <owl:Restriction>
                <owl:onProperty rdf:resource="http://stix.mitre.org/stixCommon#informationSource"/>
                <owl:someValuesFrom rdf:resource="http://www.w3.org/2002/07/owl#Thing"/>
            </owl:Restriction>
        </rdfs:subClassOf>
        <rdfs:subClassOf>
            <owl:Restriction>
                <owl:onProperty rdf:resource="http://stix.mitre.org/stixCommon#confidence.description"/>
                <owl:someValuesFrom rdf:resource="http://www.w3.org/2000/01/rdf-schema#Literal"/>
            </owl:Restriction>
        </rdfs:subClassOf>
        <rdfs:subClassOf>
            <owl:Restriction>
                <owl:onProperty rdf:resource="http://stix.mitre.org/stixCommon#confidence.timestamp"/>
                <owl:someValuesFrom rdf:resource="http://www.w3.org/2000/01/rdf-schema#Literal"/>
            </owl:Restriction>
        </rdfs:subClassOf>
        <rdfs:subClassOf>
            <owl:Restriction>
                <owl:onProperty rdf:resource="http://stix.mitre.org/stixCommon#confidence.timestampPrecision"/>
                <owl:someValuesFrom rdf:resource="http://www.w3.org/2000/01/rdf-schema#Literal"/>
            </owl:Restriction>
        </rdfs:subClassOf>
        <rdfs:subClassOf>
            <owl:Restriction>
                <owl:onProperty rdf:resource="http://stix.mitre.org/stixCommon#confidence.value"/>
                <owl:someValuesFrom rdf:resource="http://www.w3.org/2000/01/rdf-schema#Literal"/>
            </owl:Restriction>
        </rdfs:subClassOf>
        <rdfs:subClassOf>
            <owl:Restriction>
                <owl:onProperty rdf:resource="http://stix.mitre.org/stixCommon#description"/>
                <owl:someValuesFrom rdf:resource="http://www.w3.org/2000/01/rdf-schema#Literal"/>
            </owl:Restriction>
        </rdfs:subClassOf>
        <rdfs:subClassOf>
            <owl:Restriction>
                <owl:onProperty rdf:resource="http://stix.mitre.org/stixCommon#id"/>
                <owl:someValuesFrom rdf:resource="http://www.w3.org/2000/01/rdf-schema#Literal"/>
            </owl:Restriction>
        </rdfs:subClassOf>
        <rdfs:subClassOf>
            <owl:Restriction>
                <owl:onProperty rdf:resource="http://stix.mitre.org/stixCommon#threatActorTypeValue"/>
                <owl:someValuesFrom rdf:resource="http://www.w3.org/2000/01/rdf-schema#Literal"/>
            </owl:Restriction>
        </rdfs:subClassOf>
        <rdfs:subClassOf>
            <owl:Restriction>
                <owl:onProperty rdf:resource="http://stix.mitre.org/stixCommon#timestamp"/>
                <owl:someValuesFrom rdf:resource="http://www.w3.org/2000/01/rdf-schema#Literal"/>
            </owl:Restriction>
        </rdfs:subClassOf>
        <rdfs:subClassOf>
            <owl:Restriction>
                <owl:onProperty rdf:resource="http://stix.mitre.org/stixCommon#timestampPrecision"/>
                <owl:someValuesFrom rdf:resource="http://www.w3.org/2000/01/rdf-schema#Literal"/>
            </owl:Restriction>
        </rdfs:subClassOf>
        <rdfs:comment>Characterizes a statement about the type(s) of a threat actor.

The ThreatActorTypeStatement class allows for the expression of a statement, a description of the statement, a confidence in the statement, and the source of the statement.</rdfs:comment>
        <rdfs:isDefinedBy rdf:resource="http://stix.mitre.org/stixCommon"/>
        <rdfs:label>Threat Actor Type Statement</rdfs:label>
    </owl:Class>
    


    <!-- http://stix.mitre.org/stixCommon#ToolInformation -->

    <owl:Class rdf:about="http://stix.mitre.org/stixCommon#ToolInformation">
        <rdfs:subClassOf>
            <owl:Restriction>
                <owl:onProperty rdf:resource="http://stix.mitre.org/stixCommon#shortDescription"/>
                <owl:someValuesFrom rdf:resource="http://www.w3.org/2000/01/rdf-schema#Literal"/>
            </owl:Restriction>
        </rdfs:subClassOf>
        <rdfs:subClassOf>
            <owl:Restriction>
                <owl:onProperty rdf:resource="http://stix.mitre.org/stixCommon#title"/>
                <owl:someValuesFrom rdf:resource="http://www.w3.org/2000/01/rdf-schema#Literal"/>
            </owl:Restriction>
        </rdfs:subClassOf>
        <rdfs:comment>Characterizes information about a hardware or software tool.</rdfs:comment>
        <rdfs:isDefinedBy rdf:resource="http://stix.mitre.org/stixCommon"/>
        <rdfs:label>Tool Information</rdfs:label>
    </owl:Class>
    


</rdf:RDF>



<!-- Generated by the OWL API (version 4.2.6.20160910-2108) https://github.com/owlcs/owlapi -->

