<?xml version="1.0"?>
<rdf:RDF xmlns="http://stix.mitre.org/ThreatActor#"
     xml:base="http://stix.mitre.org/ThreatActor"
     xmlns:stixCommon="http://stix.mitre.org/stixCommon#"
     xmlns:ciq_common="http://www.oasis-open.org/ciq_common#"
     xmlns:rdf="http://www.w3.org/1999/02/22-rdf-syntax-ns#"
     xmlns:owl="http://www.w3.org/2002/07/owl#"
     xmlns:xml="http://www.w3.org/XML/1998/namespace"
     xmlns:data_marking="http://data-marking.mitre.org/Data_Marking#"
     xmlns:xsd="http://www.w3.org/2001/XMLSchema#"
     xmlns:wgs84_pos="http://www.w3.org/2003/01/geo/wgs84_pos#"
     xmlns:rdfs="http://www.w3.org/2000/01/rdf-schema#"
     xmlns:ta="http://stix.mitre.org/ThreatActor#"
     xmlns:foaf="http://xmlns.com/foaf/0.1/"
     xmlns:dc="http://purl.org/dc/elements/1.1/">
    <owl:Ontology rdf:about="http://stix.mitre.org/ThreatActor">
        <owl:versionIRI rdf:resource="http://stix.mitre.org/ThreatActor/1.2"/>
        <owl:imports rdf:resource="http://data-marking.mitre.org/Data_Marking"/>
        <owl:imports rdf:resource="http://www.oasis-open.org/ciq_common"/>
        <owl:imports rdf:resource="http://stix.mitre.org/stixCommon"/>
        <owl:versionInfo rdf:datatype="http://www.w3.org/2001/XMLSchema#string">1.2.0-000</owl:versionInfo>
        <rdfs:comment>This ontology provides a vocabulary and representation for the Structured Threat Information eXpression (STIX) Threat Actor.  The Threat Actor ontology provides a characterization of a single STIX Threat Actor.

A STIX Threat Actor conveys information that characterizes or identifies (or both) an adversary. The characterization consists of information like the sophistication of the threat actor, its motivations and desired effects, and historically observed behavior. In the STIX relationship model, threat actors also include information such as observed TTPs, historic (or current) campaigns, and other threat actors that appear associated with this actor.</rdfs:comment>
        <rdfs:label>STIX Threat Actor Ontology</rdfs:label>
    </owl:Ontology>
    


    


    <!-- 
    ///////////////////////////////////////////////////////////////////////////////////////
    //
    // Object Properties
    //
    ///////////////////////////////////////////////////////////////////////////////////////
     -->

    


    <!-- http://stix.mitre.org/ThreatActor#associatedActors -->

    <owl:ObjectProperty rdf:about="http://stix.mitre.org/ThreatActor#associatedActors">
        <rdfs:range rdf:resource="http://stix.mitre.org/stixCommon#ThreatActorBase"/>
        <rdfs:comment>Specifies a reference to one or more Threat Actors asserted to be related with this Threat Actor.</rdfs:comment>
        <rdfs:isDefinedBy rdf:resource="http://stix.mitre.org/ThreatActor"/>
        <rdfs:label>Associated Actors</rdfs:label>
    </owl:ObjectProperty>
    


    <!-- http://stix.mitre.org/ThreatActor#associatedCampaigns -->

    <owl:ObjectProperty rdf:about="http://stix.mitre.org/ThreatActor#associatedCampaigns">
        <rdfs:range rdf:resource="http://stix.mitre.org/stixCommon#CampaignBase"/>
        <rdfs:comment>Specifies a reference to one or more Campaigns attributed to this Threat Actor.</rdfs:comment>
        <rdfs:isDefinedBy rdf:resource="http://stix.mitre.org/ThreatActor"/>
        <rdfs:label>Associated Campaigns</rdfs:label>
    </owl:ObjectProperty>
    


    <!-- http://stix.mitre.org/ThreatActor#confidence -->

    <owl:ObjectProperty rdf:about="http://stix.mitre.org/ThreatActor#confidence">
        <rdfs:range rdf:resource="http://stix.mitre.org/stixCommon#Confidence"/>
        <rdfs:comment>Specifies a reference to a characterization of the level of confidence held in the characterization of this Threat Actor.</rdfs:comment>
        <rdfs:isDefinedBy rdf:resource="http://stix.mitre.org/ThreatActor"/>
        <rdfs:label>Confidence</rdfs:label>
    </owl:ObjectProperty>
    


    <!-- http://stix.mitre.org/ThreatActor#identity -->

    <owl:ObjectProperty rdf:about="http://stix.mitre.org/ThreatActor#identity">
        <rdfs:range>
            <owl:Class>
                <owl:unionOf rdf:parseType="Collection">
                    <rdf:Description rdf:about="http://stix.mitre.org/stixCommon#CIQIdentity"/>
                    <rdf:Description rdf:about="http://www.oasis-open.org/ciq_xpil#Organization"/>
                    <rdf:Description rdf:about="http://www.oasis-open.org/ciq_xpil#Party"/>
                    <rdf:Description rdf:about="http://www.oasis-open.org/ciq_xpil#Person"/>
                </owl:unionOf>
            </owl:Class>
        </rdfs:range>
        <rdfs:comment>Specifies a reference to the identity of this Threat Actor.</rdfs:comment>
        <rdfs:isDefinedBy rdf:resource="http://stix.mitre.org/ThreatActor"/>
        <rdfs:label>Identity</rdfs:label>
    </owl:ObjectProperty>
    


    <!-- http://stix.mitre.org/ThreatActor#intendedEffect -->

    <owl:ObjectProperty rdf:about="http://stix.mitre.org/ThreatActor#intendedEffect">
        <rdfs:range rdf:resource="http://stix.mitre.org/stixCommon#IntendedEffectStatement"/>
        <rdfs:comment>Specifies a reference to the suspected intended effect for this Threat Actor.</rdfs:comment>
        <rdfs:isDefinedBy rdf:resource="http://stix.mitre.org/ThreatActor"/>
        <rdfs:label>Intended Effect</rdfs:label>
    </owl:ObjectProperty>
    


    <!-- http://stix.mitre.org/ThreatActor#motivation -->

    <owl:ObjectProperty rdf:about="http://stix.mitre.org/ThreatActor#motivation">
        <rdfs:range rdf:resource="http://stix.mitre.org/stixCommon#MotivationStatement"/>
        <rdfs:comment>Specifies a reference to a characterization of the motivations of this threat actor.</rdfs:comment>
        <rdfs:isDefinedBy rdf:resource="http://stix.mitre.org/ThreatActor"/>
        <rdfs:label>Motivation</rdfs:label>
    </owl:ObjectProperty>
    


    <!-- http://stix.mitre.org/ThreatActor#observedTTPs -->

    <owl:ObjectProperty rdf:about="http://stix.mitre.org/ThreatActor#observedTTPs">
        <rdfs:range rdf:resource="http://stix.mitre.org/stixCommon#TTPBase"/>
        <rdfs:comment>Specifies the TTPs that this Threat Actor has been observed to leverage.</rdfs:comment>
        <rdfs:isDefinedBy rdf:resource="http://stix.mitre.org/ThreatActor"/>
        <rdfs:label>Observed TTPs</rdfs:label>
    </owl:ObjectProperty>
    


    <!-- http://stix.mitre.org/ThreatActor#planningAndOperationalSupport -->

    <owl:ObjectProperty rdf:about="http://stix.mitre.org/ThreatActor#planningAndOperationalSupport">
        <rdfs:range rdf:resource="http://stix.mitre.org/stixCommon#PlanningAndOperationalSupportStatement"/>
        <rdfs:comment>Specifies a reference to the suspected planning and operational support performed by this threat actor.</rdfs:comment>
        <rdfs:isDefinedBy rdf:resource="http://stix.mitre.org/ThreatActor"/>
        <rdfs:label>Planning and Operational Support</rdfs:label>
    </owl:ObjectProperty>
    


    <!-- http://stix.mitre.org/ThreatActor#sophistication -->

    <owl:ObjectProperty rdf:about="http://stix.mitre.org/ThreatActor#sophistication">
        <rdfs:range rdf:resource="http://stix.mitre.org/stixCommon#SophisticationStatement"/>
        <rdfs:comment>Specifies a reference to a charactization of the sophistication of this Threat Actor.</rdfs:comment>
        <rdfs:isDefinedBy rdf:resource="http://stix.mitre.org/ThreatActor"/>
        <rdfs:label>Sophistication</rdfs:label>
    </owl:ObjectProperty>
    


    <!-- http://stix.mitre.org/ThreatActor#type -->

    <owl:ObjectProperty rdf:about="http://stix.mitre.org/ThreatActor#type">
        <rdfs:range rdf:resource="http://stix.mitre.org/stixCommon#ThreatActorTypeStatement"/>
        <rdfs:comment>Specifies a reference to the type(s) of this threat actor.</rdfs:comment>
        <rdfs:isDefinedBy rdf:resource="http://stix.mitre.org/ThreatActor"/>
        <rdfs:label>Type of Threat Actor</rdfs:label>
    </owl:ObjectProperty>
    


    <!-- 
    ///////////////////////////////////////////////////////////////////////////////////////
    //
    // Classes
    //
    ///////////////////////////////////////////////////////////////////////////////////////
     -->

    


    <!-- http://stix.mitre.org/ThreatActor#ThreatActor -->

    <owl:Class rdf:about="http://stix.mitre.org/ThreatActor#ThreatActor">
        <rdfs:subClassOf rdf:resource="http://stix.mitre.org/stixCommon#ThreatActorBase"/>
        <rdfs:subClassOf>
            <owl:Restriction>
                <owl:onProperty rdf:resource="http://stix.mitre.org/ThreatActor#confidence"/>
                <owl:someValuesFrom rdf:resource="http://www.w3.org/2002/07/owl#Thing"/>
            </owl:Restriction>
        </rdfs:subClassOf>
        <rdfs:subClassOf>
            <owl:Restriction>
                <owl:onProperty rdf:resource="http://stix.mitre.org/ThreatActor#identity"/>
                <owl:someValuesFrom rdf:resource="http://www.w3.org/2002/07/owl#Thing"/>
            </owl:Restriction>
        </rdfs:subClassOf>
        <rdfs:comment>Characterizes a single STIX Threat Actor.

A STIX Threat Actor characterizes a cyber threat actor including their identity, sophistication, presumed intent, historically observed behavior (TTPs), and campaigns or other threat actors they are believed to be associated with.

ThreatActors are characterizations of malicious actors (or adversaries) representing a cyber attack threat including presumed intent and historically observed behavior. In a structured sense, ThreatActors consist of a characterization of identity, suspected motivation, suspected intended effect, historically observed TTP used by the ThreatActor, historical Campaigns believed associated with the ThreatActor, other ThreatActors believed associated with the ThreatActor, handling guidance, confidence in the asserted characterization of the ThreatActor, source of the ThreatActor information, etc.</rdfs:comment>
        <rdfs:isDefinedBy rdf:resource="http://stix.mitre.org/ThreatActor"/>
        <rdfs:label>Threat Actor</rdfs:label>
    </owl:Class>
    

</rdf:RDF>



<!-- Generated by the OWL API (version 4.2.6.20160910-2108) https://github.com/owlcs/owlapi -->

