<?xml version="1.0"?>
<rdf:RDF xmlns="http://nvd.nist.gov/cve#"
     xml:base="http://nvd.nist.gov/cve"
     xmlns:cwe="http://cwe.mitre.org/cwe#"
     xmlns:cve="http://nvd.nist.gov/cve#"
     xmlns:rdf="http://www.w3.org/1999/02/22-rdf-syntax-ns#"
     xmlns:owl="http://www.w3.org/2002/07/owl#"
     xmlns:xml="http://www.w3.org/XML/1998/namespace"
     xmlns:xsd="http://www.w3.org/2001/XMLSchema#"
     xmlns:cpe="http://cpe.mitre.org/cpe#"
     xmlns:scap_core="http://scap.nist.gov/scap_core#"
     xmlns:rdfs="http://www.w3.org/2000/01/rdf-schema#"
     xmlns:cvss="http://nvd.nist.gov/cvss#">
    <owl:Ontology rdf:about="http://nvd.nist.gov/cve">
        <owl:imports rdf:resource="http://cpe.mitre.org/cpe"/>
        <owl:imports rdf:resource="http://scap.nist.gov/patch"/>
        <owl:imports rdf:resource="http://cwe.mitre.org/cwe"/>
        <owl:imports rdf:resource="http://scap.nist.gov/scap_core"/>
        <owl:imports rdf:resource="http://nvd.nist.gov/cvss"/>
        <owl:imports rdf:resource="http://cybox.mitre.org/objects/NetworkProtocol"/>
        <rdfs:comment>This ontology provides a vocabulary and representation for the Common Vulnerability Enumeration (CVE) and Open Source Vulnerability Database (OSVDB) which provides a unified, measurable set of software vulnerability information that is enabling more effective discussion, description, selection, and use of software security tools and services that can find these vulnerabilities in source code and operational systems as well as better understanding and management of software vulnerabilities related to architecture and design. 

Copyright (c) 2014, DaedaFusion, LLC.  All rights reserved.</rdfs:comment>
        <owl:versionInfo rdf:datatype="http://www.w3.org/2001/XMLSchema#string">v1.0.0-000</owl:versionInfo>
        <rdfs:label>Common Vulnerability Enumeration (CVE) and Open Source Vulnerabilty Database (OSVDB) Ontology</rdfs:label>
    </owl:Ontology>
    




    <!-- 
    ///////////////////////////////////////////////////////////////////////////////////////
    //
    // Object Properties
    //
    ///////////////////////////////////////////////////////////////////////////////////////
     -->

    


    <!-- http://nvd.nist.gov/cve#applicableCheck -->

    <owl:ObjectProperty rdf:about="http://nvd.nist.gov/cve#applicableCheck">
        <rdfs:range rdf:resource="http://scap.nist.gov/scap_core#CheckReference"/>
        <rdfs:comment>Specifies the check/test (either OVAL or other) that this particular fix action addresses.  Example, when applying this fix will change the vlue of this test result.</rdfs:comment>
        <rdfs:label>Applicable Check</rdfs:label>
    </owl:ObjectProperty>
    


    <!-- http://nvd.nist.gov/cve#applicableConfiguration -->

    <owl:ObjectProperty rdf:about="http://nvd.nist.gov/cve#applicableConfiguration">
        <rdfs:range rdf:resource="http://cpe.mitre.org/cpe#Platform"/>
        <rdfs:comment>Specifies a reference to an applicable configuration.</rdfs:comment>
        <rdfs:label>Applicable Configuration</rdfs:label>
    </owl:ObjectProperty>
    


    <!-- http://nvd.nist.gov/cve#assessmentCheck -->

    <owl:ObjectProperty rdf:about="http://nvd.nist.gov/cve#assessmentCheck">
        <rdfs:range rdf:resource="http://scap.nist.gov/scap_core#CheckReference"/>
        <rdfs:comment>Specifies zero or more assessment checks used to perform an assesstment of the vulnerability</rdfs:comment>
        <rdfs:label>Assessment Check</rdfs:label>
    </owl:ObjectProperty>
    


    <!-- http://nvd.nist.gov/cve#attackScenario -->

    <owl:ObjectProperty rdf:about="http://nvd.nist.gov/cve#attackScenario">
        <rdfs:range rdf:resource="http://scap.nist.gov/scap_core#Reference"/>
        <rdfs:comment>Specifies a reference to a description of the attack scenario</rdfs:comment>
        <rdfs:label>Attack Scenario</rdfs:label>
    </owl:ObjectProperty>
    


    <!-- http://nvd.nist.gov/cve#configurationRemediation -->

    <owl:ObjectProperty rdf:about="http://nvd.nist.gov/cve#configurationRemediation">
        <rdfs:range rdf:resource="http://nvd.nist.gov/cve#VulnerabilityReference"/>
        <rdfs:comment>Specifies a reference to configuration information that describes how to address the attack mechanism.</rdfs:comment>
        <rdfs:label>Configuration Remediation</rdfs:label>
    </owl:ObjectProperty>
    


    <!-- http://nvd.nist.gov/cve#defintion -->

    <owl:ObjectProperty rdf:about="http://nvd.nist.gov/cve#defintion">
        <rdfs:range rdf:resource="http://scap.nist.gov/scap_core#CheckReference"/>
        <rdfs:comment>Specifies the definition for the tool configuration information.</rdfs:comment>
        <rdfs:label>Definition</rdfs:label>
    </owl:ObjectProperty>
    


    <!-- http://nvd.nist.gov/cve#deprecatedBy -->

    <owl:ObjectProperty rdf:about="http://nvd.nist.gov/cve#deprecatedBy">
        <rdfs:range rdf:resource="http://cpe.mitre.org/cpe#CPE"/>
        <rdfs:comment>Specifies the identifier for zero or more software packages that have deprciated the vulnerable software package.  The identifier is expresses as a Common Platform Enumeration (CPE) name.</rdfs:comment>
        <rdfs:label>Deprecated By</rdfs:label>
    </owl:ObjectProperty>
    


    <!-- http://nvd.nist.gov/cve#fixAction -->

    <owl:ObjectProperty rdf:about="http://nvd.nist.gov/cve#fixAction">
        <rdfs:range rdf:resource="http://nvd.nist.gov/cve#FixAction"/>
        <rdfs:comment>Specifies zero or more actions that can be taken to &quot;fix&quot; or address the vulnerability.</rdfs:comment>
        <rdfs:label>Fix Action</rdfs:label>
    </owl:ObjectProperty>
    


    <!-- http://nvd.nist.gov/cve#fixActionToolConfiguration -->

    <owl:ObjectProperty rdf:about="http://nvd.nist.gov/cve#fixActionToolConfiguration">
        <rdfs:range rdf:resource="http://nvd.nist.gov/cve#ToolConfiguration"/>
        <rdfs:comment>Specifies the configuration information for a tool used in the fix action.</rdfs:comment>
        <rdfs:label>Tool Configuration</rdfs:label>
    </owl:ObjectProperty>
    


    <!-- http://nvd.nist.gov/cve#informationSource -->

    <owl:ObjectProperty rdf:about="http://nvd.nist.gov/cve#informationSource">
        <rdfs:comment>Specifies details about the source of the information.</rdfs:comment>
        <rdfs:isDefinedBy rdf:resource="http://nvd.nist.gov/cve"/>
        <rdfs:label>Information Source</rdfs:label>
    </owl:ObjectProperty>
    


    <!-- http://nvd.nist.gov/cve#nextFixAction -->

    <owl:ObjectProperty rdf:about="http://nvd.nist.gov/cve#nextFixAction">
        <rdfs:range rdf:resource="http://nvd.nist.gov/cve#FixAction"/>
        <rdfs:comment>Specifies the next fix action in the chain.  This typically specifies a dependency fix action.</rdfs:comment>
        <rdfs:label>Next Fix Action</rdfs:label>
    </owl:ObjectProperty>
    


    <!-- http://nvd.nist.gov/cve#patch -->

    <owl:ObjectProperty rdf:about="http://nvd.nist.gov/cve#patch">
        <rdfs:range rdf:resource="http://scap.nist.gov/patch#Patch"/>
        <rdfs:comment>Specifies a patch that addresses the vulnerability</rdfs:comment>
        <rdfs:label>Patch</rdfs:label>
    </owl:ObjectProperty>
    


    <!-- http://nvd.nist.gov/cve#references -->

    <owl:ObjectProperty rdf:about="http://nvd.nist.gov/cve#references">
        <rdfs:range rdf:resource="http://nvd.nist.gov/cve#VulnerabilityReference"/>
        <rdfs:comment>Specifies references associated with the vulnerability</rdfs:comment>
        <rdfs:label>Vulnerability Reference</rdfs:label>
    </owl:ObjectProperty>
    


    <!-- http://nvd.nist.gov/cve#relatedWeakness -->

    <owl:ObjectProperty rdf:about="http://nvd.nist.gov/cve#relatedWeakness">
        <rdfs:range rdf:resource="http://cwe.mitre.org/cwe#Weakness"/>
        <rdfs:comment>Associated Common Weakness (CWE)</rdfs:comment>
        <rdfs:label>Common Weakness Enumeration (CWE) Identifier</rdfs:label>
    </owl:ObjectProperty>
    


    <!-- http://nvd.nist.gov/cve#scanner -->

    <owl:ObjectProperty rdf:about="http://nvd.nist.gov/cve#scanner">
        <rdfs:range rdf:resource="http://nvd.nist.gov/cve#ToolConfiguration"/>
        <rdfs:comment>Specifies a scanner and required configuration that is capable of detecting the referenced vulnerability.  May also be an OVAL defintion.</rdfs:comment>
        <rdfs:label>Scanner</rdfs:label>
    </owl:ObjectProperty>
    


    <!-- http://nvd.nist.gov/cve#softwareUpdate -->

    <owl:ObjectProperty rdf:about="http://nvd.nist.gov/cve#softwareUpdate">
        <rdfs:range rdf:resource="http://cpe.mitre.org/cpe#CPE"/>
        <rdfs:comment>Specifies the identifier for zero or more software update packages.  The software update identifier is expresses as a Common Platform Enumeration (CPE) name.</rdfs:comment>
        <rdfs:label>Software Update</rdfs:label>
    </owl:ObjectProperty>
    


    <!-- http://nvd.nist.gov/cve#technicalDescription -->

    <owl:ObjectProperty rdf:about="http://nvd.nist.gov/cve#technicalDescription">
        <rdfs:range rdf:resource="http://scap.nist.gov/scap_core#Reference"/>
        <rdfs:comment>Specifies a refernce to a technical description of the vulnerability.</rdfs:comment>
        <rdfs:label>Technical Description</rdfs:label>
    </owl:ObjectProperty>
    


    <!-- http://nvd.nist.gov/cve#toolName -->

    <owl:ObjectProperty rdf:about="http://nvd.nist.gov/cve#toolName">
        <rdfs:range rdf:resource="http://cpe.mitre.org/cpe#CPE"/>
        <rdfs:comment></rdfs:comment>
        <rdfs:label>Tool Name</rdfs:label>
    </owl:ObjectProperty>
    


    <!-- http://nvd.nist.gov/cve#vulnerabilities -->

    <owl:ObjectProperty rdf:about="http://nvd.nist.gov/cve#vulnerabilities">
        <rdfs:range rdf:resource="http://nvd.nist.gov/cve#Vulnerability"/>
        <rdfs:comment>Specifies one or more vulnerabilities, represented by their CVE identifier, in the Vulnerability Catalog</rdfs:comment>
        <rdfs:isDefinedBy rdf:resource="http://nvd.nist.gov/cve"/>
        <rdfs:label>Vulnerabilities</rdfs:label>
    </owl:ObjectProperty>
    


    <!-- http://nvd.nist.gov/cve#vulnerabilityImpactScore -->

    <owl:ObjectProperty rdf:about="http://nvd.nist.gov/cve#vulnerabilityImpactScore">
        <rdfs:range rdf:resource="http://nvd.nist.gov/cvss#CVSSImpact"/>
        <rdfs:comment>Specifies a reference to the Vulnerability Impact score</rdfs:comment>
        <rdfs:isDefinedBy rdf:resource="http://nvd.nist.gov/cve"/>
        <rdfs:label>Vulnerability Impact Score</rdfs:label>
    </owl:ObjectProperty>
    


    <!-- http://nvd.nist.gov/cve#vulnerableConfigurations -->

    <owl:ObjectProperty rdf:about="http://nvd.nist.gov/cve#vulnerableConfigurations">
        <rdfs:range rdf:resource="http://cpe.mitre.org/cpe#Platform"/>
        <rdfs:comment>Specifies the configuration in which the vulnerability exists.</rdfs:comment>
        <rdfs:label>Vulnerable Configurations</rdfs:label>
    </owl:ObjectProperty>
    


    <!-- http://nvd.nist.gov/cve#vulnerableProducts -->

    <owl:ObjectProperty rdf:about="http://nvd.nist.gov/cve#vulnerableProducts">
        <rdfs:range rdf:resource="http://cpe.mitre.org/cpe#CPE"/>
        <rdfs:comment>Specifies the products associated with this vulnerability</rdfs:comment>
        <rdfs:label>Vulnerable Products</rdfs:label>
    </owl:ObjectProperty>
    


    <!-- 
    ///////////////////////////////////////////////////////////////////////////////////////
    //
    // Data properties
    //
    ///////////////////////////////////////////////////////////////////////////////////////
     -->

    


    <!-- http://nvd.nist.gov/cve#deprecated -->

    <owl:DatatypeProperty rdf:about="http://nvd.nist.gov/cve#deprecated">
        <rdfs:range rdf:resource="http://www.w3.org/2001/XMLSchema#boolean"/>
        <rdfs:comment>Specifies that the related entity has been deprecated.</rdfs:comment>
        <rdfs:label>Deprecated</rdfs:label>
    </owl:DatatypeProperty>
    


    <!-- http://nvd.nist.gov/cve#description -->

    <owl:DatatypeProperty rdf:about="http://nvd.nist.gov/cve#description">
        <rdfs:range rdf:resource="http://www.w3.org/2001/XMLSchema#string"/>
        <rdfs:comment rdf:datatype="http://www.w3.org/2001/XMLSchema#string">Specifies a short description of the vulnerability.</rdfs:comment>
        <rdfs:label>Description</rdfs:label>
    </owl:DatatypeProperty>
    


    <!-- http://nvd.nist.gov/cve#dictionaryLink -->

    <owl:DatatypeProperty rdf:about="http://nvd.nist.gov/cve#dictionaryLink">
        <rdfs:range rdf:resource="http://www.w3.org/2001/XMLSchema#anyURI"/>
        <rdfs:comment>Specifies an external link to the vulnerability contained at the Common Vulnerability Enumeration (CVE) or the Open Source Vulnerabiity Database (OSVDB) dictionary.  The link should be in the following form:  http://cve.mitre.org/cgi-bin/cvename.cgi?name={vulnerability-id} or http://nvd.nist.gov/nvd.cfm?cvename=CVE-{vulnerability-id} or http://osvdb.org/{vulnerability-id} , where {vulnerability-id) should be the Identifier of the specific vulnerability.</rdfs:comment>
        <rdfs:label>Dictionary Link</rdfs:label>
        <rdfs:seeAlso rdf:datatype="http://www.w3.org/2001/XMLSchema#string"></rdfs:seeAlso>
    </owl:DatatypeProperty>
    


    <!-- http://nvd.nist.gov/cve#disclosureDate -->

    <owl:DatatypeProperty rdf:about="http://nvd.nist.gov/cve#disclosureDate">
        <rdfs:range rdf:resource="http://www.w3.org/2001/XMLSchema#dateTime"/>
        <rdfs:comment>Specifies the date and time the vulnerability was disclosed.</rdfs:comment>
        <rdfs:label>Disclosure Date</rdfs:label>
    </owl:DatatypeProperty>
    


    <!-- http://nvd.nist.gov/cve#discoveryDate -->

    <owl:DatatypeProperty rdf:about="http://nvd.nist.gov/cve#discoveryDate">
        <rdfs:range rdf:resource="http://www.w3.org/2001/XMLSchema#dateTime"/>
        <rdfs:comment>Specifies the date and time the vulnerability was discovered.</rdfs:comment>
        <rdfs:label>Discovery Date</rdfs:label>
    </owl:DatatypeProperty>
    


    <!-- http://nvd.nist.gov/cve#effectiveness -->

    <owl:DatatypeProperty rdf:about="http://nvd.nist.gov/cve#effectiveness">
        <rdfs:range rdf:resource="http://www.w3.org/2001/XMLSchema#string"/>
        <rdfs:comment>Specifies whether the fix action fully avoids the risk associated with the vulnerability or reduces risk to some extent.</rdfs:comment>
        <rdfs:label>Effectiveness</rdfs:label>
    </owl:DatatypeProperty>
    


    <!-- http://nvd.nist.gov/cve#exploitLocation.Dialup -->

    <owl:DatatypeProperty rdf:about="http://nvd.nist.gov/cve#exploitLocation.Dialup">
        <rdfs:range rdf:resource="http://www.w3.org/2001/XMLSchema#boolean"/>
        <rdfs:comment>Specifies that the attack mechanism requires dial-up access.</rdfs:comment>
        <rdfs:label>Associated Exploit Location: Dialup</rdfs:label>
    </owl:DatatypeProperty>
    


    <!-- http://nvd.nist.gov/cve#exploitLocation.PhysicalAccess -->

    <owl:DatatypeProperty rdf:about="http://nvd.nist.gov/cve#exploitLocation.PhysicalAccess">
        <rdfs:range rdf:resource="http://www.w3.org/2001/XMLSchema#boolean"/>
        <rdfs:comment>Specifies that the attack mechanism requires physical access.</rdfs:comment>
        <rdfs:label>Associated Exploit Location: Physical Access</rdfs:label>
    </owl:DatatypeProperty>
    


    <!-- http://nvd.nist.gov/cve#exploitLocation.Unknown -->

    <owl:DatatypeProperty rdf:about="http://nvd.nist.gov/cve#exploitLocation.Unknown">
        <rdfs:range rdf:resource="http://www.w3.org/2001/XMLSchema#boolean"/>
        <rdfs:comment rdf:datatype="http://www.w3.org/2001/XMLSchema#string">Specifies that that the location requirements of the attack mechanism is unknown.</rdfs:comment>
        <rdfs:label>Associated Exploit Location: Unknown</rdfs:label>
    </owl:DatatypeProperty>
    


    <!-- http://nvd.nist.gov/cve#exploitLocation.VoluntarilyInteract -->

    <owl:DatatypeProperty rdf:about="http://nvd.nist.gov/cve#exploitLocation.VoluntarilyInteract">
        <rdfs:range rdf:resource="http://www.w3.org/2001/XMLSchema#boolean"/>
        <rdfs:comment>Specifies that the victim must voluntarily interact with the attack mechanism.</rdfs:comment>
        <rdfs:label>Associated Exploit Location: Voluntarily Interact</rdfs:label>
    </owl:DatatypeProperty>
    


    <!-- http://nvd.nist.gov/cve#exploitPublicationDate -->

    <owl:DatatypeProperty rdf:about="http://nvd.nist.gov/cve#exploitPublicationDate">
        <rdfs:range rdf:resource="http://www.w3.org/2001/XMLSchema#dateTime"/>
        <rdfs:comment>Specifies the date and time when the exploit was first published.</rdfs:comment>
        <rdfs:label>Exploit Publication Date</rdfs:label>
    </owl:DatatypeProperty>
    


    <!-- http://nvd.nist.gov/cve#extendedDescription -->

    <owl:DatatypeProperty rdf:about="http://nvd.nist.gov/cve#extendedDescription">
        <rdfs:range rdf:resource="http://www.w3.org/2001/XMLSchema#string"/>
        <rdfs:comment>Specifies an unstructured text description</rdfs:comment>
        <rdfs:isDefinedBy rdf:resource="http://nvd.nist.gov/cve"/>
        <rdfs:label>Extended Description</rdfs:label>
    </owl:DatatypeProperty>
    


    <!-- http://nvd.nist.gov/cve#externalIdentifier -->

    <owl:DatatypeProperty rdf:about="http://nvd.nist.gov/cve#externalIdentifier">
        <rdfs:range rdf:resource="http://www.w3.org/2001/XMLSchema#string"/>
        <rdfs:comment rdf:datatype="http://www.w3.org/2001/XMLSchema#string">Specifies the external identifier associated with the vulnerability, such as the Common Vulnerability Enumeration (CVE) and Open-Source Vulnerability (OSVDB). 

Common Vulnerability Enumeration (CVE) identifier associated with the vulnerability must follow the CVE identifier pattern of &quot;CVE-yyyy-nnnn&quot; where &apos;yyyy&apos; specifies a 4-digit year and &apos;nnnnn&apos; specifies an numerically incrementing number that resets to 0 when a new year is reached.</rdfs:comment>
        <rdfs:label>External Identifier</rdfs:label>
    </owl:DatatypeProperty>
    


    <!-- http://nvd.nist.gov/cve#fixActionDescription -->

    <owl:DatatypeProperty rdf:about="http://nvd.nist.gov/cve#fixActionDescription">
        <rdfs:range rdf:resource="http://www.w3.org/2001/XMLSchema#string"/>
        <rdfs:comment>Specifies a description of the fix action</rdfs:comment>
        <rdfs:label>Fix Action Description</rdfs:label>
    </owl:DatatypeProperty>
    


    <!-- http://nvd.nist.gov/cve#fixActionId -->

    <owl:DatatypeProperty rdf:about="http://nvd.nist.gov/cve#fixActionId">
        <rdfs:range rdf:resource="http://www.w3.org/2001/XMLSchema#string"/>
        <rdfs:comment>Specifies a unique identifier associated to be associated with the fix action</rdfs:comment>
        <rdfs:label>Fix Action Id</rdfs:label>
    </owl:DatatypeProperty>
    


    <!-- http://nvd.nist.gov/cve#fixActionSource -->

    <owl:DatatypeProperty rdf:about="http://nvd.nist.gov/cve#fixActionSource">
        <rdfs:range rdf:resource="http://www.w3.org/2001/XMLSchema#anyURI"/>
        <rdfs:comment>Specifies the source of the fix item.</rdfs:comment>
        <rdfs:label>Source</rdfs:label>
    </owl:DatatypeProperty>
    


    <!-- http://nvd.nist.gov/cve#fixActionType -->

    <owl:DatatypeProperty rdf:about="http://nvd.nist.gov/cve#fixActionType">
        <rdfs:range rdf:resource="http://www.w3.org/2001/XMLSchema#string"/>
        <rdfs:comment>Specifies the type of the fix action.</rdfs:comment>
        <rdfs:label>Fix Action Type</rdfs:label>
    </owl:DatatypeProperty>
    


    <!-- http://nvd.nist.gov/cve#isKnown -->

    <owl:DatatypeProperty rdf:about="http://nvd.nist.gov/cve#isKnown">
        <rdfs:range rdf:resource="http://www.w3.org/2001/XMLSchema#boolean"/>
        <rdfs:comment>Specifies whether or not the vulnerability is known (i.e., not a 0-day) at the time of characterization.</rdfs:comment>
        <rdfs:isDefinedBy rdf:resource="http://nvd.nist.gov/cve"/>
        <rdfs:label>Is Known</rdfs:label>
    </owl:DatatypeProperty>
    


    <!-- http://nvd.nist.gov/cve#isPubliclyAcknowledged -->

    <owl:DatatypeProperty rdf:about="http://nvd.nist.gov/cve#isPubliclyAcknowledged">
        <rdfs:range rdf:resource="http://www.w3.org/2001/XMLSchema#boolean"/>
        <rdfs:comment>Specifies whether or not the vulnerability is publicly acknowledged by the vendor.</rdfs:comment>
        <rdfs:isDefinedBy rdf:resource="http://nvd.nist.gov/cve"/>
        <rdfs:label>Is Publicly Acknowledged</rdfs:label>
    </owl:DatatypeProperty>
    


    <!-- http://nvd.nist.gov/cve#lastModifiedDate -->

    <owl:DatatypeProperty rdf:about="http://nvd.nist.gov/cve#lastModifiedDate">
        <rdfs:range rdf:resource="http://www.w3.org/2001/XMLSchema#dateTime"/>
        <rdfs:comment>Specifies the date and time vulnerability information was modified.</rdfs:comment>
        <rdfs:label>Last Modified</rdfs:label>
    </owl:DatatypeProperty>
    


    <!-- http://nvd.nist.gov/cve#publishedDate -->

    <owl:DatatypeProperty rdf:about="http://nvd.nist.gov/cve#publishedDate">
        <rdfs:range rdf:resource="http://www.w3.org/2001/XMLSchema#dateTime"/>
        <rdfs:comment>Specifies the date and time the Vulnerability information was published</rdfs:comment>
        <rdfs:label>Published Date</rdfs:label>
    </owl:DatatypeProperty>
    


    <!-- http://nvd.nist.gov/cve#referenceName -->

    <owl:DatatypeProperty rdf:about="http://nvd.nist.gov/cve#referenceName">
        <rdfs:range rdf:resource="http://www.w3.org/2001/XMLSchema#string"/>
        <rdfs:comment>Specifies a piece of human-readable text that provides a meaningful name for the reference</rdfs:comment>
        <rdfs:label>Name</rdfs:label>
    </owl:DatatypeProperty>
    


    <!-- http://nvd.nist.gov/cve#referenceSource -->

    <owl:DatatypeProperty rdf:about="http://nvd.nist.gov/cve#referenceSource">
        <rdfs:range rdf:resource="http://www.w3.org/2001/XMLSchema#string"/>
        <rdfs:comment>Specifies the name of the source of the vulnerability reference</rdfs:comment>
        <rdfs:label>Reference Source Name</rdfs:label>
    </owl:DatatypeProperty>
    


    <!-- http://nvd.nist.gov/cve#referenceType -->

    <owl:DatatypeProperty rdf:about="http://nvd.nist.gov/cve#referenceType">
        <rdfs:range rdf:resource="http://www.w3.org/2001/XMLSchema#string"/>
        <rdfs:comment>Specifies the type of vulnerability reference</rdfs:comment>
        <rdfs:label>Vulnerabilty Reference Type</rdfs:label>
    </owl:DatatypeProperty>
    


    <!-- http://nvd.nist.gov/cve#securityProtection -->

    <owl:DatatypeProperty rdf:about="http://nvd.nist.gov/cve#securityProtection">
        <rdfs:range rdf:resource="http://www.w3.org/2001/XMLSchema#string"/>
        <rdfs:comment>Specifies the type of security protection gain from the attack mechanism</rdfs:comment>
        <rdfs:label>Security Protection</rdfs:label>
    </owl:DatatypeProperty>
    


    <!-- http://nvd.nist.gov/cve#status -->

    <owl:DatatypeProperty rdf:about="http://nvd.nist.gov/cve#status">
        <rdfs:comment>Specifies the status of the vulnerability reporting</rdfs:comment>
        <rdfs:isDefinedBy rdf:resource="http://nvd.nist.gov/cve"/>
        <rdfs:label>Status</rdfs:label>
    </owl:DatatypeProperty>
    


    <!-- http://nvd.nist.gov/cve#title -->

    <owl:DatatypeProperty rdf:about="http://nvd.nist.gov/cve#title">
        <rdfs:range rdf:resource="http://www.w3.org/2001/XMLSchema#string"/>
        <rdfs:comment>Specifies a simple title for the entity</rdfs:comment>
        <rdfs:isDefinedBy rdf:resource="http://nvd.nist.gov/cve"/>
        <rdfs:label>Title</rdfs:label>
    </owl:DatatypeProperty>
    


    <!-- 
    ///////////////////////////////////////////////////////////////////////////////////////
    //
    // Classes
    //
    ///////////////////////////////////////////////////////////////////////////////////////
     -->

    



    <!-- http://nvd.nist.gov/cve#FixAction -->

    <owl:Class rdf:about="http://nvd.nist.gov/cve#FixAction">
        <rdfs:subClassOf>
            <owl:Restriction>
                <owl:onProperty rdf:resource="http://nvd.nist.gov/cve#configurationRemediation"/>
                <owl:someValuesFrom rdf:resource="http://www.w3.org/2002/07/owl#Thing"/>
            </owl:Restriction>
        </rdfs:subClassOf>
        <rdfs:subClassOf>
            <owl:Restriction>
                <owl:onProperty rdf:resource="http://nvd.nist.gov/cve#patch"/>
                <owl:someValuesFrom rdf:resource="http://www.w3.org/2002/07/owl#Thing"/>
            </owl:Restriction>
        </rdfs:subClassOf>
        <rdfs:subClassOf>
            <owl:Restriction>
                <owl:onProperty rdf:resource="http://nvd.nist.gov/cve#effectiveness"/>
                <owl:someValuesFrom rdf:resource="http://www.w3.org/2000/01/rdf-schema#Literal"/>
            </owl:Restriction>
        </rdfs:subClassOf>
        <rdfs:subClassOf>
            <owl:Restriction>
                <owl:onProperty rdf:resource="http://nvd.nist.gov/cve#fixActionDescription"/>
                <owl:someValuesFrom rdf:resource="http://www.w3.org/2000/01/rdf-schema#Literal"/>
            </owl:Restriction>
        </rdfs:subClassOf>
        <rdfs:subClassOf>
            <owl:Restriction>
                <owl:onProperty rdf:resource="http://nvd.nist.gov/cve#fixActionId"/>
                <owl:someValuesFrom rdf:resource="http://www.w3.org/2000/01/rdf-schema#Literal"/>
            </owl:Restriction>
        </rdfs:subClassOf>
        <rdfs:subClassOf>
            <owl:Restriction>
                <owl:onProperty rdf:resource="http://nvd.nist.gov/cve#fixActionSource"/>
                <owl:someValuesFrom rdf:resource="http://www.w3.org/2000/01/rdf-schema#Literal"/>
            </owl:Restriction>
        </rdfs:subClassOf>
        <rdfs:subClassOf>
            <owl:Restriction>
                <owl:onProperty rdf:resource="http://nvd.nist.gov/cve#fixActionType"/>
                <owl:someValuesFrom rdf:resource="http://www.w3.org/2000/01/rdf-schema#Literal"/>
            </owl:Restriction>
        </rdfs:subClassOf>
        <rdfs:comment>Defines a single action to fix or address a vulnerability.  A fix action should only cover a signle patch application, software update, configuration change, or external fix.  Dependencies should be documented by chainging instance of a FixAction together.</rdfs:comment>
        <rdfs:isDefinedBy rdf:resource="http://nvd.nist.gov/cve"/>
        <rdfs:label>Fix Action</rdfs:label>
    </owl:Class>
    


    <!-- http://nvd.nist.gov/cve#ToolConfiguration -->

    <owl:Class rdf:about="http://nvd.nist.gov/cve#ToolConfiguration">
        <rdfs:subClassOf>
            <owl:Restriction>
                <owl:onProperty rdf:resource="http://nvd.nist.gov/cve#toolName"/>
                <owl:someValuesFrom rdf:resource="http://www.w3.org/2002/07/owl#Thing"/>
            </owl:Restriction>
        </rdfs:subClassOf>
        <rdfs:comment>Defines configuration information for tool</rdfs:comment>
        <rdfs:isDefinedBy rdf:resource="http://nvd.nist.gov/cve"/>
        <rdfs:label>Tool Configuration</rdfs:label>
    </owl:Class>
    


    <!-- http://nvd.nist.gov/cve#Vulnerability -->

    <owl:Class rdf:about="http://nvd.nist.gov/cve#Vulnerability">
        <rdfs:subClassOf>
            <owl:Restriction>
                <owl:onProperty rdf:resource="http://nvd.nist.gov/cve#informationSource"/>
                <owl:someValuesFrom rdf:resource="http://www.w3.org/2002/07/owl#Thing"/>
            </owl:Restriction>
        </rdfs:subClassOf>
        <rdfs:subClassOf>
            <owl:Restriction>
                <owl:onProperty rdf:resource="http://nvd.nist.gov/cve#vulnerabilityImpactScore"/>
                <owl:someValuesFrom rdf:resource="http://www.w3.org/2002/07/owl#Thing"/>
            </owl:Restriction>
        </rdfs:subClassOf>
        <rdfs:subClassOf>
            <owl:Restriction>
                <owl:onProperty rdf:resource="http://nvd.nist.gov/cve#description"/>
                <owl:someValuesFrom rdf:resource="http://www.w3.org/2000/01/rdf-schema#Literal"/>
            </owl:Restriction>
        </rdfs:subClassOf>
        <rdfs:subClassOf>
            <owl:Restriction>
                <owl:onProperty rdf:resource="http://nvd.nist.gov/cve#disclosureDate"/>
                <owl:someValuesFrom rdf:resource="http://www.w3.org/2000/01/rdf-schema#Literal"/>
            </owl:Restriction>
        </rdfs:subClassOf>
        <rdfs:subClassOf>
            <owl:Restriction>
                <owl:onProperty rdf:resource="http://nvd.nist.gov/cve#discoveryDate"/>
                <owl:someValuesFrom rdf:resource="http://www.w3.org/2000/01/rdf-schema#Literal"/>
            </owl:Restriction>
        </rdfs:subClassOf>
        <rdfs:subClassOf>
            <owl:Restriction>
                <owl:onProperty rdf:resource="http://nvd.nist.gov/cve#extendedDescription"/>
                <owl:someValuesFrom rdf:resource="http://www.w3.org/2000/01/rdf-schema#Literal"/>
            </owl:Restriction>
        </rdfs:subClassOf>
        <rdfs:subClassOf>
            <owl:Restriction>
                <owl:onProperty rdf:resource="http://nvd.nist.gov/cve#externalIdentifier"/>
                <owl:someValuesFrom rdf:resource="http://www.w3.org/2000/01/rdf-schema#Literal"/>
            </owl:Restriction>
        </rdfs:subClassOf>
        <rdfs:subClassOf>
            <owl:Restriction>
                <owl:onProperty rdf:resource="http://nvd.nist.gov/cve#isKnown"/>
                <owl:someValuesFrom rdf:resource="http://www.w3.org/2000/01/rdf-schema#Literal"/>
            </owl:Restriction>
        </rdfs:subClassOf>
        <rdfs:subClassOf>
            <owl:Restriction>
                <owl:onProperty rdf:resource="http://nvd.nist.gov/cve#isPubliclyAcknowledged"/>
                <owl:someValuesFrom rdf:resource="http://www.w3.org/2000/01/rdf-schema#Literal"/>
            </owl:Restriction>
        </rdfs:subClassOf>
        <rdfs:subClassOf>
            <owl:Restriction>
                <owl:onProperty rdf:resource="http://nvd.nist.gov/cve#lastModifiedDate"/>
                <owl:someValuesFrom rdf:resource="http://www.w3.org/2000/01/rdf-schema#Literal"/>
            </owl:Restriction>
        </rdfs:subClassOf>
        <rdfs:subClassOf>
            <owl:Restriction>
                <owl:onProperty rdf:resource="http://nvd.nist.gov/cve#publishedDate"/>
                <owl:someValuesFrom rdf:resource="http://www.w3.org/2000/01/rdf-schema#Literal"/>
            </owl:Restriction>
        </rdfs:subClassOf>
        <rdfs:subClassOf>
            <owl:Restriction>
                <owl:onProperty rdf:resource="http://nvd.nist.gov/cve#securityProtection"/>
                <owl:someValuesFrom rdf:resource="http://www.w3.org/2000/01/rdf-schema#Literal"/>
            </owl:Restriction>
        </rdfs:subClassOf>
        <rdfs:subClassOf>
            <owl:Restriction>
                <owl:onProperty rdf:resource="http://nvd.nist.gov/cve#status"/>
                <owl:someValuesFrom rdf:resource="http://www.w3.org/2000/01/rdf-schema#Literal"/>
            </owl:Restriction>
        </rdfs:subClassOf>
        <rdfs:subClassOf>
            <owl:Restriction>
                <owl:onProperty rdf:resource="http://nvd.nist.gov/cve#title"/>
                <owl:someValuesFrom rdf:resource="http://www.w3.org/2000/01/rdf-schema#Literal"/>
            </owl:Restriction>
        </rdfs:subClassOf>
        <rdfs:comment>Characterizes a vulnerability</rdfs:comment>
        <rdfs:isDefinedBy rdf:resource="http://nvd.nist.gov/cve"/>
        <rdfs:label>Vulnerability</rdfs:label>
    </owl:Class>
    


    <!-- http://nvd.nist.gov/cve#VulnerabilityCatalog -->

    <owl:Class rdf:about="http://nvd.nist.gov/cve#VulnerabilityCatalog">
        <rdfs:subClassOf rdf:resource="http://scap.nist.gov/scap_core#Catalog"/>
        <rdfs:comment>Characterizes a collection of vulnerabilities, represented by CVE identifier, in a Vulnerability Catalog</rdfs:comment>
        <rdfs:isDefinedBy rdf:resource="http://nvd.nist.gov/cve"/>
        <rdfs:label>Vulnerability Catalog</rdfs:label>
    </owl:Class>
    


    <!-- http://nvd.nist.gov/cve#VulnerabilityReference -->

    <owl:Class rdf:about="http://nvd.nist.gov/cve#VulnerabilityReference">
        <rdfs:subClassOf>
            <owl:Restriction>
                <owl:onProperty rdf:resource="http://nvd.nist.gov/cve#deprecated"/>
                <owl:someValuesFrom rdf:resource="http://www.w3.org/2000/01/rdf-schema#Literal"/>
            </owl:Restriction>
        </rdfs:subClassOf>
        <rdfs:subClassOf>
            <owl:Restriction>
                <owl:onProperty rdf:resource="http://nvd.nist.gov/cve#referenceName"/>
                <owl:someValuesFrom rdf:resource="http://www.w3.org/2000/01/rdf-schema#Literal"/>
            </owl:Restriction>
        </rdfs:subClassOf>
        <rdfs:subClassOf>
            <owl:Restriction>
                <owl:onProperty rdf:resource="http://nvd.nist.gov/cve#referenceSource"/>
                <owl:someValuesFrom rdf:resource="http://www.w3.org/2000/01/rdf-schema#Literal"/>
            </owl:Restriction>
        </rdfs:subClassOf>
        <rdfs:subClassOf>
            <owl:Restriction>
                <owl:onProperty rdf:resource="http://nvd.nist.gov/cve#referenceType"/>
                <owl:someValuesFrom rdf:resource="http://www.w3.org/2000/01/rdf-schema#Literal"/>
            </owl:Restriction>
        </rdfs:subClassOf>
        <rdfs:comment>Specifies a reference associated with a vulnerability</rdfs:comment>
        <rdfs:isDefinedBy rdf:resource="http://nvd.nist.gov/cve"/>
        <rdfs:label>Vulnerabilty Reference</rdfs:label>
    </owl:Class>
    


</rdf:RDF>



<!-- Generated by the OWL API (version 4.2.6.20160910-2108) https://github.com/owlcs/owlapi -->

