<?xml version="1.0"?>
<rdf:RDF xmlns="http://maec.mitre.org/maec_common#"
     xml:base="http://maec.mitre.org/maec_common"
     xmlns:rdf="http://www.w3.org/1999/02/22-rdf-syntax-ns#"
     xmlns:owl="http://www.w3.org/2002/07/owl#"
     xmlns:xml="http://www.w3.org/XML/1998/namespace"
     xmlns:xsd="http://www.w3.org/2001/XMLSchema#"
     xmlns:wgs84_pos="http://www.w3.org/2003/01/geo/wgs84_pos#"
     xmlns:rdfs="http://www.w3.org/2000/01/rdf-schema#"
     xmlns:cyboxCommon="http://cybox.mitre.org/cyboxCommon#"
     xmlns:maecc="http://maec.mitre.org/maec_common#"
     xmlns:foaf="http://xmlns.com/foaf/0.1/"
     xmlns:dc="http://purl.org/dc/elements/1.1/">
    <owl:Ontology rdf:about="http://maec.mitre.org/maec_common">
        <owl:imports rdf:resource="http://cybox.mitre.org/objects/Code"/>
        <owl:imports rdf:resource="http://cybox.mitre.org/objects/URI"/>
        <owl:imports rdf:resource="http://cybox.mitre.org/objects/API"/>
        <owl:imports rdf:resource="http://cybox.mitre.org/cyboxCommon"/>
        <owl:imports rdf:resource="http://www.oasis-open.org/ciq_xpil"/>
        <rdfs:label>Malware Attribute Enumeration and Characterization (MAEC)  Common Ontology</rdfs:label>
        <rdfs:comment>This ontology provides a vocabulary and representation for the  Malware Attribute Enumeration and Characterization (MAEC)  common  types.  

MAEC provides a common mechansim (structure and content) for encoding and communicating high-fidelity information about malware based upon attributes such as behaviors, artifacts, and attack patterns.  The Common ontology provides a vocabulary of common data and object types that are commonly used across the related malware ontologies.

The ontology is based on the MAEC Bundle, Container, and Package schemas maintained by The MITRE Corporation copyright 2012-2014.  The version number of the ontology is kept in sync with the schema in order to more easily relate between the ontology and the corresponding schema version.

Copyright (c) 2014, DaedaFusion, LLC.  All rights reserved.</rdfs:comment>
        <owl:versionInfo rdf:datatype="http://www.w3.org/2001/XMLSchema#string">2.1.0-000</owl:versionInfo>
    </owl:Ontology>
    
    


    <!-- 
    ///////////////////////////////////////////////////////////////////////////////////////
    //
    // Object Properties
    //
    ///////////////////////////////////////////////////////////////////////////////////////
     -->

    


    <!-- http://maec.mitre.org/maec_common#actionReference -->

    <owl:ObjectProperty rdf:about="http://maec.mitre.org/maec_common#actionReference">
        <rdfs:range rdf:resource="http://maec.mitre.org/maec_common#MalwareAction"/>
        <rdfs:comment>Specifies a reference to a single Action that is part of the Action Equivalency</rdfs:comment>
        <rdfs:isDefinedBy rdf:resource="http://maec.mitre.org/maec_common"/>
        <rdfs:label>Action Reference</rdfs:label>
    </owl:ObjectProperty>
    


    <!-- http://maec.mitre.org/maec_common#apiCall -->

    <owl:ObjectProperty rdf:about="http://maec.mitre.org/maec_common#apiCall">
        <rdfs:range rdf:resource="http://cybox.mitre.org/objects/API#API"/>
        <rdfs:comment>Specifies a system-level API call that was used to implement the action. Software must make use of such calls to talk to hardware and perform system-specific functions.</rdfs:comment>
        <rdfs:isDefinedBy rdf:resource="http://maec.mitre.org/maec_common"/>
        <rdfs:label>APIc Call</rdfs:label>
    </owl:ObjectProperty>
    


    <!-- http://maec.mitre.org/maec_common#author -->

    <owl:ObjectProperty rdf:about="http://maec.mitre.org/maec_common#author">
        <rdfs:range>
            <owl:Class>
                <owl:unionOf rdf:parseType="Collection">
                    <rdf:Description rdf:about="http://www.oasis-open.org/ciq_xpil#Organization"/>
                    <rdf:Description rdf:about="http://www.oasis-open.org/ciq_xpil#Person"/>
                </owl:unionOf>
            </owl:Class>
        </rdfs:range>
        <rdfs:comment>Specifies a reference to the author</rdfs:comment>
        <rdfs:isDefinedBy rdf:resource="http://maec.mitre.org/maec_common"/>
        <rdfs:label>Author</rdfs:label>
    </owl:ObjectProperty>
    


    <!-- http://maec.mitre.org/maec_common#code -->

    <owl:ObjectProperty rdf:about="http://maec.mitre.org/maec_common#code">
        <rdfs:range rdf:resource="http://cybox.mitre.org/objects/Code#Code"/>
        <rdfs:comment>Specifies any form of code that was used to implement the action.</rdfs:comment>
        <rdfs:isDefinedBy rdf:resource="http://maec.mitre.org/maec_common"/>
        <rdfs:label>Code</rdfs:label>
    </owl:ObjectProperty>
    


    <!-- http://maec.mitre.org/maec_common#commentText -->

    <owl:ObjectProperty rdf:about="http://maec.mitre.org/maec_common#commentText">
        <rdfs:range>
            <owl:Class>
                <owl:unionOf rdf:parseType="Collection">
                    <rdf:Description rdf:about="http://www.w3.org/2001/XMLSchema#anyURI"/>
                    <rdf:Description rdf:about="http://www.w3.org/2001/XMLSchema#string"/>
                </owl:unionOf>
            </owl:Class>
        </rdfs:range>
    </owl:ObjectProperty>
    


    <!-- http://maec.mitre.org/maec_common#compatiblePlatforms -->

    <owl:ObjectProperty rdf:about="http://maec.mitre.org/maec_common#compatiblePlatforms">
        <rdfs:range>
            <owl:Class>
                <owl:unionOf rdf:parseType="Collection">
                    <rdf:Description rdf:about="http://cpe.mitre.org/cpe#CPE"/>
                    <rdf:Description rdf:about="http://cybox.mitre.org/cyboxCommon#PlatformSpecification"/>
                </owl:unionOf>
            </owl:Class>
        </rdfs:range>
        <rdfs:comment></rdfs:comment>
        <rdfs:isDefinedBy rdf:datatype="http://www.w3.org/2001/XMLSchema#string">&lt;http://maec.mitre.org/maec_bundle&gt;</rdfs:isDefinedBy>
        <rdfs:label>compatible platforms</rdfs:label>
    </owl:ObjectProperty>
    


    <!-- http://maec.mitre.org/maec_common#implementation -->

    <owl:ObjectProperty rdf:about="http://maec.mitre.org/maec_common#implementation">
        <rdfs:range rdf:resource="http://maec.mitre.org/maec_common#ActionImplementation"/>
        <rdfs:comment>Specifies attributes that are relevant to how the Action is implemented in the malware, such as the specific API call that was used.</rdfs:comment>
        <rdfs:isDefinedBy rdf:resource="http://maec.mitre.org/maec_common"/>
        <rdfs:label>Implementation</rdfs:label>
    </owl:ObjectProperty>
    


    <!-- http://maec.mitre.org/maec_common#malwareInstanceObject -->

    <owl:ObjectProperty rdf:about="http://maec.mitre.org/maec_common#malwareInstanceObject">
        <rdfs:range rdf:resource="http://cybox.mitre.org/cybox_core#Object"/>
        <rdfs:comment>Specifies the attributes of the malware instance object (most commonly a file) that is encompassed in the Malware Subject.</rdfs:comment>
        <rdfs:isDefinedBy rdf:resource="http://maec.mitre.org/maec_common"/>
        <rdfs:label>malware instance object</rdfs:label>
    </owl:ObjectProperty>
    


    <!-- http://maec.mitre.org/maec_common#objectReference -->

    <owl:ObjectProperty rdf:about="http://maec.mitre.org/maec_common#objectReference">
        <rdfs:range rdf:resource="http://cybox.mitre.org/cybox_core#Object"/>
        <rdfs:comment>Specifies a reference to a single Object that is part of the Object Equivalency</rdfs:comment>
        <rdfs:isDefinedBy rdf:resource="http://maec.mitre.org/maec_common"/>
        <rdfs:label>Object Reference</rdfs:label>
    </owl:ObjectProperty>
    


    <!-- http://maec.mitre.org/maec_common#source.internetLocation -->

    <owl:ObjectProperty rdf:about="http://maec.mitre.org/maec_common#source.internetLocation">
        <rdfs:range rdf:resource="http://cybox.mitre.org/objects/URI#URI"/>
        <rdfs:comment>Specifies the the Uniform Resource Locator (URL) of the external source, if applicable.</rdfs:comment>
        <rdfs:isDefinedBy rdf:resource="http://maec.mitre.org/maec_common"/>
        <rdfs:label>Internet Location</rdfs:label>
    </owl:ObjectProperty>
    


    <!-- http://maec.mitre.org/maec_common#source.organization -->

    <owl:ObjectProperty rdf:about="http://maec.mitre.org/maec_common#source.organization">
        <rdfs:range rdf:resource="http://www.oasis-open.org/ciq_xpil#Organization"/>
        <rdfs:comment>Specifies a reference to the organization from which teh source originated</rdfs:comment>
        <rdfs:isDefinedBy rdf:resource="http://maec.mitre.org/maec_common"/>
        <rdfs:label>Source Organization</rdfs:label>
    </owl:ObjectProperty>
    


    <!-- http://maec.mitre.org/maec_common#source.person -->

    <owl:ObjectProperty rdf:about="http://maec.mitre.org/maec_common#source.person">
        <rdfs:range rdf:resource="http://www.oasis-open.org/ciq_xpil#Person"/>
        <rdfs:comment>Specifies a reference to the person linked to the source.</rdfs:comment>
        <rdfs:isDefinedBy rdf:resource="http://maec.mitre.org/maec_common"/>
        <rdfs:label>Source Person</rdfs:label>
    </owl:ObjectProperty>
    


    <!-- 
    ///////////////////////////////////////////////////////////////////////////////////////
    //
    // Data properties
    //
    ///////////////////////////////////////////////////////////////////////////////////////
     -->

    


    <!-- http://maec.mitre.org/maec_common#actionImplType -->

    <owl:DatatypeProperty rdf:about="http://maec.mitre.org/maec_common#actionImplType">
        <rdfs:range rdf:resource="http://www.w3.org/2001/XMLSchema#string"/>
        <rdfs:comment>Specifies the type of Action Implementation being characterized in this element.</rdfs:comment>
        <rdfs:isDefinedBy rdf:resource="http://maec.mitre.org/maec_common"/>
        <rdfs:label>Action Implementation Type</rdfs:label>
    </owl:DatatypeProperty>
    


    <!-- http://maec.mitre.org/maec_common#affinityDegree -->

    <owl:DatatypeProperty rdf:about="http://maec.mitre.org/maec_common#affinityDegree">
        <rdfs:range rdf:resource="http://www.w3.org/2001/XMLSchema#string"/>
        <rdfs:comment>Specifies the degree to which the objects in a collection are related.</rdfs:comment>
        <rdfs:isDefinedBy rdf:resource="http://maec.mitre.org/maec_common"/>
        <rdfs:label>Affinity Degree</rdfs:label>
    </owl:DatatypeProperty>
    


    <!-- http://maec.mitre.org/maec_common#affinityType -->

    <owl:DatatypeProperty rdf:about="http://maec.mitre.org/maec_common#affinityType">
        <rdfs:range rdf:resource="http://www.w3.org/2001/XMLSchema#string"/>
        <rdfs:comment>Specifies how the objects in a collection are related.</rdfs:comment>
        <rdfs:isDefinedBy rdf:resource="http://maec.mitre.org/maec_common"/>
        <rdfs:label>Affinity Type</rdfs:label>
    </owl:DatatypeProperty>
    


    <!-- http://maec.mitre.org/maec_common#authorName -->

    <owl:DatatypeProperty rdf:about="http://maec.mitre.org/maec_common#authorName">
        <rdfs:range rdf:resource="http://www.w3.org/2001/XMLSchema#string"/>
        <rdfs:comment>Specifies the name of the author that added the comment.</rdfs:comment>
        <rdfs:isDefinedBy rdf:resource="http://maec.mitre.org/maec_common"/>
        <rdfs:label>Author Name</rdfs:label>
    </owl:DatatypeProperty>
    


    <!-- http://maec.mitre.org/maec_common#collectionDescription -->

    <owl:DatatypeProperty rdf:about="http://maec.mitre.org/maec_common#collectionDescription">
        <rdfs:range rdf:resource="http://www.w3.org/2001/XMLSchema#string"/>
        <rdfs:comment>Specifies a textual description of the collection.</rdfs:comment>
        <rdfs:isDefinedBy rdf:resource="http://maec.mitre.org/maec_common"/>
        <rdfs:label>Description</rdfs:label>
    </owl:DatatypeProperty>
    


    <!-- http://maec.mitre.org/maec_common#collectionName -->

    <owl:DatatypeProperty rdf:about="http://maec.mitre.org/maec_common#collectionName">
        <rdfs:range rdf:resource="http://www.w3.org/2001/XMLSchema#string"/>
        <rdfs:comment>Specifies the name of the collection.</rdfs:comment>
        <rdfs:isDefinedBy rdf:resource="http://maec.mitre.org/maec_common"/>
        <rdfs:label>Name</rdfs:label>
    </owl:DatatypeProperty>
    


    <!-- http://maec.mitre.org/maec_common#commentText -->

    <owl:DatatypeProperty rdf:about="http://maec.mitre.org/maec_common#commentText"/>
    


    <!-- http://maec.mitre.org/maec_common#creationDateTime -->

    <owl:DatatypeProperty rdf:about="http://maec.mitre.org/maec_common#creationDateTime">
        <rdfs:range rdf:resource="http://www.w3.org/2001/XMLSchema#dateTime"/>
        <rdfs:comment>Specifies the date/time the entity was created.</rdfs:comment>
        <rdfs:isDefinedBy rdf:resource="http://maec.mitre.org/maec_common"/>
        <rdfs:label>Creation Date</rdfs:label>
    </owl:DatatypeProperty>
    


    <!-- http://maec.mitre.org/maec_common#id -->

    <owl:DatatypeProperty rdf:about="http://maec.mitre.org/maec_common#id">
        <rdfs:range rdf:resource="http://www.w3.org/2001/XMLSchema#string"/>
        <rdfs:comment>Specifies the unique identifier associated with this entity instance.

The format of the identifier MUST be in the format of [construct-type]-[UUID], where [construct-type] should be associated with the entity&apos;s construct and [UUID] SHOULD correspond to a universally unique identifier.</rdfs:comment>
        <rdfs:isDefinedBy rdf:resource="http://maec.mitre.org/maec_common"/>
        <rdfs:label>ID</rdfs:label>
    </owl:DatatypeProperty>
    


    <!-- http://maec.mitre.org/maec_common#importance -->

    <owl:DatatypeProperty rdf:about="http://maec.mitre.org/maec_common#importance">
        <rdfs:range rdf:resource="http://www.w3.org/2001/XMLSchema#string"/>
        <rdfs:comment>Specifies the relative importance of the entity.</rdfs:comment>
        <rdfs:isDefinedBy rdf:resource="http://maec.mitre.org/maec_common"/>
        <rdfs:label>Importance</rdfs:label>
    </owl:DatatypeProperty>
    


    <!-- http://maec.mitre.org/maec_common#lastUpdateDateTime -->

    <owl:DatatypeProperty rdf:about="http://maec.mitre.org/maec_common#lastUpdateDateTime">
        <rdfs:range rdf:resource="http://www.w3.org/2001/XMLSchema#dateTime"/>
        <rdfs:comment>Specifies the the last date/time the entity was updated</rdfs:comment>
        <rdfs:isDefinedBy rdf:resource="http://maec.mitre.org/maec_common"/>
        <rdfs:label>Last Update</rdfs:label>
    </owl:DatatypeProperty>
    


    <!-- http://maec.mitre.org/maec_common#observationName -->

    <owl:DatatypeProperty rdf:about="http://maec.mitre.org/maec_common#observationName">
        <rdfs:range rdf:resource="http://www.w3.org/2001/XMLSchema#string"/>
        <rdfs:comment>Specifies the name, type, or identifier of an observation, for comments that refer to the observation of particular entities. For example, a comment that refers to a command and control (C2) encryption key could have an observation_name of &quot;C2 Encryption Key&quot;. {@en-US}</rdfs:comment>
        <rdfs:isDefinedBy rdf:resource="http://maec.mitre.org/maec_common"/>
        <rdfs:label>observation name</rdfs:label>
    </owl:DatatypeProperty>
    


    <!-- http://maec.mitre.org/maec_common#source.obtainMethod -->

    <owl:DatatypeProperty rdf:about="http://maec.mitre.org/maec_common#source.obtainMethod">
        <rdfs:range rdf:resource="http://www.w3.org/2001/XMLSchema#string"/>
        <rdfs:comment>Specifys the method used to obtain the data that the Source element refers to.</rdfs:comment>
        <rdfs:isDefinedBy rdf:resource="http://maec.mitre.org/maec_common"/>
        <rdfs:label>Obtain Method</rdfs:label>
    </owl:DatatypeProperty>
    


    <!-- http://maec.mitre.org/maec_common#source.organizationName -->

    <owl:DatatypeProperty rdf:about="http://maec.mitre.org/maec_common#source.organizationName">
        <rdfs:range rdf:resource="http://www.w3.org/2001/XMLSchema#string"/>
        <rdfs:comment>Specifies the name of the organization from which the source originated.</rdfs:comment>
        <rdfs:isDefinedBy rdf:resource="http://maec.mitre.org/maec_common"/>
        <rdfs:label>Organization Name</rdfs:label>
    </owl:DatatypeProperty>
    


    <!-- http://maec.mitre.org/maec_common#source.personName -->

    <owl:DatatypeProperty rdf:about="http://maec.mitre.org/maec_common#source.personName">
        <rdfs:range rdf:resource="http://www.w3.org/2001/XMLSchema#string"/>
        <rdfs:comment>Specifies the name of the person linked to the source.</rdfs:comment>
        <rdfs:isDefinedBy rdf:resource="http://maec.mitre.org/maec_common"/>
        <rdfs:label>Person Name</rdfs:label>
    </owl:DatatypeProperty>
    


    <!-- http://maec.mitre.org/maec_common#source.reference -->

    <owl:DatatypeProperty rdf:about="http://maec.mitre.org/maec_common#source.reference">
        <rdfs:range rdf:resource="http://www.w3.org/2001/XMLSchema#string"/>
        <rdfs:comment>Specifies a reference name or ID for the source.</rdfs:comment>
        <rdfs:isDefinedBy rdf:resource="http://maec.mitre.org/maec_common"/>
        <rdfs:label>Reference</rdfs:label>
    </owl:DatatypeProperty>
    


    <!-- http://maec.mitre.org/maec_common#timestamp -->

    <owl:DatatypeProperty rdf:about="http://maec.mitre.org/maec_common#timestamp">
        <rdfs:range rdf:resource="http://www.w3.org/2001/XMLSchema#dateTime"/>
        <rdfs:comment>Specifies the time and date of an entity</rdfs:comment>
        <rdfs:isDefinedBy rdf:resource="http://maec.mitre.org/maec_common"/>
        <rdfs:label>Timestamp</rdfs:label>
    </owl:DatatypeProperty>
    


    <!-- http://maec.mitre.org/maec_common#toolType -->

    <owl:DatatypeProperty rdf:about="http://maec.mitre.org/maec_common#toolType">
        <rdfs:range rdf:resource="http://www.w3.org/2001/XMLSchema#string"/>
        <rdfs:comment>Specifies the type of the tool leveraged.</rdfs:comment>
        <rdfs:isDefinedBy rdf:resource="http://maec.mitre.org/maec_common"/>
        <rdfs:label>Tool Type</rdfs:label>
    </owl:DatatypeProperty>
    


    <!-- http://maec.mitre.org/maec_common#version -->

    <owl:DatatypeProperty rdf:about="http://maec.mitre.org/maec_common#version">
        <rdfs:range rdf:resource="http://www.w3.org/2001/XMLSchema#string"/>
        <rdfs:comment>Specifies the version of the entity</rdfs:comment>
        <rdfs:isDefinedBy rdf:resource="http://maec.mitre.org/maec_common"/>
        <rdfs:label>Version</rdfs:label>
    </owl:DatatypeProperty>
    


    <!-- 
    ///////////////////////////////////////////////////////////////////////////////////////
    //
    // Classes
    //
    ///////////////////////////////////////////////////////////////////////////////////////
     -->

    


    <!-- http://maec.mitre.org/maec_common#ActionEquivalence -->

    <owl:Class rdf:about="http://maec.mitre.org/maec_common#ActionEquivalence">
        <rdfs:subClassOf>
            <owl:Restriction>
                <owl:onProperty rdf:resource="http://maec.mitre.org/maec_common#actionReference"/>
                <owl:someValuesFrom rdf:resource="http://www.w3.org/2002/07/owl#Thing"/>
            </owl:Restriction>
        </rdfs:subClassOf>
        <rdfs:subClassOf>
            <owl:Restriction>
                <owl:onProperty rdf:resource="http://maec.mitre.org/maec_common#id"/>
                <owl:someValuesFrom rdf:resource="http://www.w3.org/2000/01/rdf-schema#Literal"/>
            </owl:Restriction>
        </rdfs:subClassOf>
        <rdfs:comment>Specifies any Actions that are equivalent to each other, e.g., those that were found for the same Malware Subject when using different analysis tools. It can be used as a way of referencing equivalent actions as a single unit, such as for specifying the Action composition of a Behavior</rdfs:comment>
        <rdfs:isDefinedBy rdf:resource="http://maec.mitre.org/maec_common"/>
        <rdfs:label>Action Equivalence</rdfs:label>
    </owl:Class>
    


    <!-- http://maec.mitre.org/maec_common#ActionImplementation -->

    <owl:Class rdf:about="http://maec.mitre.org/maec_common#ActionImplementation">
        <rdfs:subClassOf>
            <owl:Restriction>
                <owl:onProperty rdf:resource="http://maec.mitre.org/maec_common#apiCall"/>
                <owl:someValuesFrom rdf:resource="http://www.w3.org/2002/07/owl#Thing"/>
            </owl:Restriction>
        </rdfs:subClassOf>
        <rdfs:subClassOf>
            <owl:Restriction>
                <owl:onProperty rdf:resource="http://maec.mitre.org/maec_common#actionImplType"/>
                <owl:someValuesFrom rdf:resource="http://www.w3.org/2000/01/rdf-schema#Literal"/>
            </owl:Restriction>
        </rdfs:subClassOf>
        <rdfs:subClassOf>
            <owl:Restriction>
                <owl:onProperty rdf:resource="http://maec.mitre.org/maec_common#id"/>
                <owl:someValuesFrom rdf:resource="http://www.w3.org/2000/01/rdf-schema#Literal"/>
            </owl:Restriction>
        </rdfs:subClassOf>
        <rdfs:comment>Characterizes an Action Implementations. 

Currently supported are implementations achieved through API function calls and abstractly defined code.</rdfs:comment>
        <rdfs:isDefinedBy rdf:resource="http://maec.mitre.org/maec_common"/>
        <rdfs:label>Action Implementation</rdfs:label>
    </owl:Class>
    


    <!-- http://maec.mitre.org/maec_common#BaseCollection -->

    <owl:Class rdf:about="http://maec.mitre.org/maec_common#BaseCollection">
        <rdfs:subClassOf>
            <owl:Restriction>
                <owl:onProperty rdf:resource="http://maec.mitre.org/maec_common#affinityDegree"/>
                <owl:someValuesFrom rdf:resource="http://www.w3.org/2000/01/rdf-schema#Literal"/>
            </owl:Restriction>
        </rdfs:subClassOf>
        <rdfs:subClassOf>
            <owl:Restriction>
                <owl:onProperty rdf:resource="http://maec.mitre.org/maec_common#affinityType"/>
                <owl:someValuesFrom rdf:resource="http://www.w3.org/2000/01/rdf-schema#Literal"/>
            </owl:Restriction>
        </rdfs:subClassOf>
        <rdfs:subClassOf>
            <owl:Restriction>
                <owl:onProperty rdf:resource="http://maec.mitre.org/maec_common#collectionDescription"/>
                <owl:someValuesFrom rdf:resource="http://www.w3.org/2000/01/rdf-schema#Literal"/>
            </owl:Restriction>
        </rdfs:subClassOf>
        <rdfs:subClassOf>
            <owl:Restriction>
                <owl:onProperty rdf:resource="http://maec.mitre.org/maec_common#collectionName"/>
                <owl:someValuesFrom rdf:resource="http://www.w3.org/2000/01/rdf-schema#Literal"/>
            </owl:Restriction>
        </rdfs:subClassOf>
        <rdfs:subClassOf>
            <owl:Restriction>
                <owl:onProperty rdf:resource="http://maec.mitre.org/maec_common#id"/>
                <owl:someValuesFrom rdf:resource="http://www.w3.org/2000/01/rdf-schema#Literal"/>
            </owl:Restriction>
        </rdfs:subClassOf>
        <rdfs:comment>Characterizes the base type for other Collection types.</rdfs:comment>
        <rdfs:isDefinedBy rdf:resource="http://maec.mitre.org/maec_common"/>
        <rdfs:label>Base Collection</rdfs:label>
    </owl:Class>
    


    <!-- http://maec.mitre.org/maec_common#Comment -->

    <owl:Class rdf:about="http://maec.mitre.org/maec_common#Comment">
        <rdfs:subClassOf>
            <owl:Restriction>
                <owl:onProperty rdf:resource="http://maec.mitre.org/maec_common#author"/>
                <owl:someValuesFrom rdf:resource="http://www.w3.org/2002/07/owl#Thing"/>
            </owl:Restriction>
        </rdfs:subClassOf>
        <rdfs:subClassOf>
            <owl:Restriction>
                <owl:onProperty rdf:resource="http://maec.mitre.org/maec_common#authorName"/>
                <owl:someValuesFrom rdf:resource="http://www.w3.org/2000/01/rdf-schema#Literal"/>
            </owl:Restriction>
        </rdfs:subClassOf>
        <rdfs:subClassOf>
            <owl:Restriction>
                <owl:onProperty rdf:resource="http://maec.mitre.org/maec_common#observationName"/>
                <owl:someValuesFrom rdf:resource="http://www.w3.org/2000/01/rdf-schema#Literal"/>
            </owl:Restriction>
        </rdfs:subClassOf>
        <rdfs:subClassOf>
            <owl:Restriction>
                <owl:onProperty rdf:resource="http://maec.mitre.org/maec_common#timestamp"/>
                <owl:someValuesFrom rdf:resource="http://www.w3.org/2000/01/rdf-schema#Literal"/>
            </owl:Restriction>
        </rdfs:subClassOf>
        <rdfs:comment>Characterizes a comment relating to some field.</rdfs:comment>
        <rdfs:isDefinedBy rdf:resource="http://maec.mitre.org/maec_common"/>
        <rdfs:label>Comment</rdfs:label>
    </owl:Class>
    


    <!-- http://maec.mitre.org/maec_common#MalwareAction -->

    <owl:Class rdf:about="http://maec.mitre.org/maec_common#MalwareAction">
        <rdfs:subClassOf rdf:resource="http://cybox.mitre.org/cybox_core#Action"/>
        <rdfs:subClassOf>
            <owl:Restriction>
                <owl:onProperty rdf:resource="http://maec.mitre.org/maec_common#implementation"/>
                <owl:cardinality  rdf:datatype="http://www.w3.org/2001/XMLSchema#nonNegativeInteger">1</owl:cardinality>
            </owl:Restriction>
        </rdfs:subClassOf>
        <rdfs:subClassOf>
            <owl:Restriction>
                <owl:onProperty rdf:resource="http://maec.mitre.org/maec_common#actionImplType"/>
                <owl:cardinality rdf:datatype="http://www.w3.org/2001/XMLSchema#nonNegativeInteger">1</owl:cardinality>
            </owl:Restriction>
        </rdfs:subClassOf>
        <rdfs:comment>Characterizes actions found or observed in malware.  Actions can be thought of as system state changes and similar operations that represent the fundamental low-level operation of malware. Some examples include the creation of a file, deletion of a registry key, and the sending of some  data on a socket.</rdfs:comment>
        <rdfs:label>Malware Action</rdfs:label>
    </owl:Class>
    


    <!-- http://maec.mitre.org/maec_common#ObjectEquivalence -->

    <owl:Class rdf:about="http://maec.mitre.org/maec_common#ObjectEquivalence">
        <rdfs:subClassOf>
            <owl:Restriction>
                <owl:onProperty rdf:resource="http://maec.mitre.org/maec_common#objectReference"/>
                <owl:someValuesFrom rdf:resource="http://www.w3.org/2002/07/owl#Thing"/>
            </owl:Restriction>
        </rdfs:subClassOf>
        <rdfs:subClassOf>
            <owl:Restriction>
                <owl:onProperty rdf:resource="http://maec.mitre.org/maec_common#id"/>
                <owl:someValuesFrom rdf:resource="http://www.w3.org/2000/01/rdf-schema#Literal"/>
            </owl:Restriction>
        </rdfs:subClassOf>
        <rdfs:comment>Characterizes the Objects that are equivalent to each other, e.g., those that were found for the same Malware Subject when using different analysis tools.</rdfs:comment>
        <rdfs:isDefinedBy rdf:resource="http://maec.mitre.org/maec_common"/>
        <rdfs:label>Object Equivalence</rdfs:label>
    </owl:Class>
    


    <!-- http://maec.mitre.org/maec_common#Source -->

    <owl:Class rdf:about="http://maec.mitre.org/maec_common#Source">
        <rdfs:subClassOf>
            <owl:Restriction>
                <owl:onProperty rdf:resource="http://maec.mitre.org/maec_common#source.internetLocation"/>
                <owl:someValuesFrom rdf:resource="http://www.w3.org/2002/07/owl#Thing"/>
            </owl:Restriction>
        </rdfs:subClassOf>
        <rdfs:subClassOf>
            <owl:Restriction>
                <owl:onProperty rdf:resource="http://maec.mitre.org/maec_common#source.organization"/>
                <owl:someValuesFrom rdf:resource="http://www.w3.org/2002/07/owl#Thing"/>
            </owl:Restriction>
        </rdfs:subClassOf>
        <rdfs:subClassOf>
            <owl:Restriction>
                <owl:onProperty rdf:resource="http://maec.mitre.org/maec_common#source.person"/>
                <owl:someValuesFrom rdf:resource="http://www.w3.org/2002/07/owl#Thing"/>
            </owl:Restriction>
        </rdfs:subClassOf>
        <rdfs:subClassOf>
            <owl:Restriction>
                <owl:onProperty rdf:resource="http://maec.mitre.org/maec_common#id"/>
                <owl:someValuesFrom rdf:resource="http://www.w3.org/2000/01/rdf-schema#Literal"/>
            </owl:Restriction>
        </rdfs:subClassOf>
        <rdfs:subClassOf>
            <owl:Restriction>
                <owl:onProperty rdf:resource="http://maec.mitre.org/maec_common#source.obtainMethod"/>
                <owl:someValuesFrom rdf:resource="http://www.w3.org/2000/01/rdf-schema#Literal"/>
            </owl:Restriction>
        </rdfs:subClassOf>
        <rdfs:subClassOf>
            <owl:Restriction>
                <owl:onProperty rdf:resource="http://maec.mitre.org/maec_common#source.organizationName"/>
                <owl:someValuesFrom rdf:resource="http://www.w3.org/2000/01/rdf-schema#Literal"/>
            </owl:Restriction>
        </rdfs:subClassOf>
        <rdfs:subClassOf>
            <owl:Restriction>
                <owl:onProperty rdf:resource="http://maec.mitre.org/maec_common#source.personName"/>
                <owl:someValuesFrom rdf:resource="http://www.w3.org/2000/01/rdf-schema#Literal"/>
            </owl:Restriction>
        </rdfs:subClassOf>
        <rdfs:subClassOf>
            <owl:Restriction>
                <owl:onProperty rdf:resource="http://maec.mitre.org/maec_common#source.reference"/>
                <owl:someValuesFrom rdf:resource="http://www.w3.org/2000/01/rdf-schema#Literal"/>
            </owl:Restriction>
        </rdfs:subClassOf>
        <rdfs:comment>Specifies information about the internal or external source of the analysis, if applicable.</rdfs:comment>
        <rdfs:isDefinedBy rdf:resource="http://maec.mitre.org/maec_common"/>
        <rdfs:label>Source</rdfs:label>
    </owl:Class>
    


    <!-- http://maec.mitre.org/maec_common#ToolInformation -->

    <owl:Class rdf:about="http://maec.mitre.org/maec_common#ToolInformation">
        <rdfs:subClassOf>
            <owl:Restriction>
                <owl:onProperty rdf:resource="http://maec.mitre.org/maec_common#id"/>
                <owl:someValuesFrom rdf:resource="http://www.w3.org/2000/01/rdf-schema#Literal"/>
            </owl:Restriction>
        </rdfs:subClassOf>
        <rdfs:subClassOf>
            <owl:Restriction>
                <owl:onProperty rdf:resource="http://maec.mitre.org/maec_common#toolType"/>
                <owl:someValuesFrom rdf:resource="http://www.w3.org/2000/01/rdf-schema#Literal"/>
            </owl:Restriction>
        </rdfs:subClassOf>
        <rdfs:comment>Characterizes the properties of a hardware or software tool, including those related to instances of its use.</rdfs:comment>
        <rdfs:isDefinedBy rdf:resource="http://maec.mitre.org/maec_common"/>
        <rdfs:label>Tool</rdfs:label>
    </owl:Class>
    


</rdf:RDF>



<!-- Generated by the OWL API (version 4.2.6.20160910-2108) https://github.com/owlcs/owlapi -->

