<?xml version="1.0"?>
<rdf:RDF xmlns="http://xml/metadatasharing#"
     xml:base="http://xml/metadatasharing"
     xmlns:rdf="http://www.w3.org/1999/02/22-rdf-syntax-ns#"
     xmlns:owl="http://www.w3.org/2002/07/owl#"
     xmlns:xml="http://www.w3.org/XML/1998/namespace"
     xmlns:mmdef="http://xml/metadatasharing#"
     xmlns:xsd="http://www.w3.org/2001/XMLSchema#"
     xmlns:rdfs="http://www.w3.org/2000/01/rdf-schema#">
    <owl:Ontology rdf:about="http://xml/metadatasharing">
        <rdfs:label>Malware Metadata Exchange Format (MMDEF) Metadata Sharing Ontology</rdfs:label>
        <rdfs:comment>This ontology provides a vocabulary and representation for the  Metadata Sharing  component of the Malware Metadata Exchange Format (MMDEF) common  types.  

The Metadata Sharing ontology provides a set of data types for representing prevalence information associated with malicous software.

The ontology is based on the Malware Metadata Exchange Format schemas maintained by the IEEE Standards Assocation copyright 2011-2014.  The version number of the ontology is kept in sync with the schema in order to more easily relate between the ontology and the corresponding schema version.

Copyright (c) 2014, DaedaFusion, LLC.  All rights reserved.</rdfs:comment>
        <owl:versionInfo rdf:datatype="http://www.w3.org/2001/XMLSchema#string">1.2.0-000</owl:versionInfo>
    </owl:Ontology>
    


    <!-- 
    ///////////////////////////////////////////////////////////////////////////////////////
    //
    // Object Properties
    //
    ///////////////////////////////////////////////////////////////////////////////////////
     -->

    


    <!-- http://xml/metadatasharing#fieldData.location -->

    <owl:ObjectProperty rdf:about="http://xml/metadatasharing#fieldData.location">
        <rdfs:range rdf:resource="http://xml/metadatasharing#Location"/>
        <rdfs:comment>Specifies geolocation information for prevalence.</rdfs:comment>
        <rdfs:isDefinedBy rdf:resource="http://xml/metadatasharing"/>
        <rdfs:label>field data.location</rdfs:label>
    </owl:ObjectProperty>
    


    <!-- http://xml/metadatasharing#fieldData.volume -->

    <owl:ObjectProperty rdf:about="http://xml/metadatasharing#fieldData.volume">
        <rdfs:range rdf:resource="http://xml/metadatasharing#Volume"/>
        <rdfs:comment>Specifies a quantitive measurements of prevalence</rdfs:comment>
        <rdfs:isDefinedBy rdf:resource="http://xml/metadatasharing"/>
        <rdfs:label>field data.volume</rdfs:label>
    </owl:ObjectProperty>
    


    <!-- 
    ///////////////////////////////////////////////////////////////////////////////////////
    //
    // Data properties
    //
    ///////////////////////////////////////////////////////////////////////////////////////
     -->

    


    <!-- http://xml/metadatasharing#fieldData.commonality -->

    <owl:DatatypeProperty rdf:about="http://xml/metadatasharing#fieldData.commonality">
        <rdfs:range>
            <rdfs:Datatype>
                <owl:onDatatype rdf:resource="http://www.w3.org/2001/XMLSchema#integer"/>
                <owl:withRestrictions rdf:parseType="Collection">
                    <rdf:Description>
                        <xsd:minInclusive rdf:datatype="http://www.w3.org/2001/XMLSchema#integer">0</xsd:minInclusive>
                    </rdf:Description>
                    <rdf:Description>
                        <xsd:maxInclusive rdf:datatype="http://www.w3.org/2001/XMLSchema#integer">100</xsd:maxInclusive>
                    </rdf:Description>
                </owl:withRestrictions>
            </rdfs:Datatype>
        </rdfs:range>
        <rdfs:comment>Specifies a qualitative measurements of prevalence.  The value must be a number between 0 and 100.</rdfs:comment>
        <rdfs:isDefinedBy rdf:resource="http://xml/metadatasharing"/>
        <rdfs:label>field data.commonality</rdfs:label>
    </owl:DatatypeProperty>
    


    <!-- http://xml/metadatasharing#fieldData.endDateTime -->

    <owl:DatatypeProperty rdf:about="http://xml/metadatasharing#fieldData.endDateTime">
        <rdfs:range rdf:resource="http://www.w3.org/2001/XMLSchema#dateTime"/>
        <rdfs:comment>Specifies the end date of the period over which the prevalence (commonality) and importance is measured.</rdfs:comment>
        <rdfs:isDefinedBy rdf:resource="http://xml/metadatasharing"/>
        <rdfs:label>field data.end date</rdfs:label>
    </owl:DatatypeProperty>
    


    <!-- http://xml/metadatasharing#fieldData.firstSeenDateTime -->

    <owl:DatatypeProperty rdf:about="http://xml/metadatasharing#fieldData.firstSeenDateTime">
        <rdfs:range rdf:resource="http://www.w3.org/2001/XMLSchema#dateTime"/>
        <rdfs:comment>Specifies the date that the object was first seen by the reporting entity.</rdfs:comment>
        <rdfs:isDefinedBy rdf:resource="http://xml/metadatasharing"/>
        <rdfs:label>field data.first seen</rdfs:label>
    </owl:DatatypeProperty>
    


    <!-- http://xml/metadatasharing#fieldData.importance -->

    <owl:DatatypeProperty rdf:about="http://xml/metadatasharing#fieldData.importance">
        <rdfs:range>
            <rdfs:Datatype>
                <owl:onDatatype rdf:resource="http://www.w3.org/2001/XMLSchema#integer"/>
                <owl:withRestrictions rdf:parseType="Collection">
                    <rdf:Description>
                        <xsd:minInclusive rdf:datatype="http://www.w3.org/2001/XMLSchema#integer">0</xsd:minInclusive>
                    </rdf:Description>
                    <rdf:Description>
                        <xsd:maxInclusive rdf:datatype="http://www.w3.org/2001/XMLSchema#integer">100</xsd:maxInclusive>
                    </rdf:Description>
                </owl:withRestrictions>
            </rdfs:Datatype>
        </rdfs:range>
        <rdfs:comment>Specifies a qualitative measurement of risk associated with the object.  The value must be a number between 0 and 100.</rdfs:comment>
        <rdfs:isDefinedBy rdf:resource="http://xml/metadatasharing"/>
        <rdfs:label>field data.importance</rdfs:label>
    </owl:DatatypeProperty>
    


    <!-- http://xml/metadatasharing#fieldData.origin -->

    <owl:DatatypeProperty rdf:about="http://xml/metadatasharing#fieldData.origin">
        <rdfs:range rdf:resource="http://www.w3.org/2001/XMLSchema#string"/>
        <rdfs:comment>Specifies the origins of data associated with the field data.</rdfs:comment>
        <rdfs:isDefinedBy rdf:resource="http://xml/metadatasharing"/>
        <rdfs:label>field data.origin</rdfs:label>
    </owl:DatatypeProperty>
    


    <!-- http://xml/metadatasharing#fieldData.startDateTime -->

    <owl:DatatypeProperty rdf:about="http://xml/metadatasharing#fieldData.startDateTime">
        <rdfs:range rdf:resource="http://www.w3.org/2001/XMLSchema#dateTime"/>
        <rdfs:comment>Specifies the start date of the period over which the prevalence (commonality) and importance is measured.</rdfs:comment>
        <rdfs:isDefinedBy rdf:resource="http://xml/metadatasharing"/>
        <rdfs:label>Start Date</rdfs:label>
    </owl:DatatypeProperty>
    


    <!-- http://xml/metadatasharing#id -->

    <owl:DatatypeProperty rdf:about="http://xml/metadatasharing#id">
        <rdfs:domain rdf:resource="http://xml/metadatasharing#Location"/>
        <rdfs:domain rdf:resource="http://xml/metadatasharing#Volume"/>
        <rdfs:range rdf:resource="http://www.w3.org/2001/XMLSchema#string"/>
        <rdfs:comment>Specifies the unique identifier associated with this entity instance.

An identifier MUST take the format [ns-prefix]:[construct-type]-[UUID], where [ns-prefix] should be the namespace prefix owned/controlled by the producer of the content

The format of the Id must be in the format of [ns-prefix]:construct-type-[UUID], there the [ns-prefix] SHOULD be a namespace prefix bound to a namespace owned/controlled by the producer of the content, and [UUID] SHOULD correspond to a globally unique identifier. {@en-US}</rdfs:comment>
        <rdfs:isDefinedBy rdf:resource="http://xml/metadatasharing"/>
        <rdfs:label>Id</rdfs:label>
    </owl:DatatypeProperty>
    


    <!-- http://xml/metadatasharing#locationType -->

    <owl:DatatypeProperty rdf:about="http://xml/metadatasharing#locationType">
        <rdfs:domain rdf:resource="http://xml/metadatasharing#Location"/>
        <rdfs:range rdf:resource="http://www.w3.org/2001/XMLSchema#string"/>
        <rdfs:comment>Specifies the type of the location</rdfs:comment>
        <rdfs:isDefinedBy rdf:resource="http://xml/metadatasharing"/>
        <rdfs:label>Location Type</rdfs:label>
    </owl:DatatypeProperty>
    


    <!-- http://xml/metadatasharing#locationValue -->

    <owl:DatatypeProperty rdf:about="http://xml/metadatasharing#locationValue">
        <rdfs:domain rdf:resource="http://xml/metadatasharing#Location"/>
        <rdfs:range rdf:resource="http://www.w3.org/2001/XMLSchema#string"/>
        <rdfs:comment>Specifies the location value</rdfs:comment>
        <rdfs:isDefinedBy rdf:resource="http://xml/metadatasharing"/>
        <rdfs:label>Location Value</rdfs:label>
    </owl:DatatypeProperty>
    


    <!-- http://xml/metadatasharing#volumeUnits -->

    <owl:DatatypeProperty rdf:about="http://xml/metadatasharing#volumeUnits">
        <rdfs:domain rdf:resource="http://xml/metadatasharing#Volume"/>
        <rdfs:range rdf:resource="http://www.w3.org/2001/XMLSchema#string"/>
        <rdfs:comment>Specifies the associated units in which the volume is stated.</rdfs:comment>
        <rdfs:isDefinedBy rdf:resource="http://xml/metadatasharing"/>
        <rdfs:label>Volumn Units</rdfs:label>
    </owl:DatatypeProperty>
    


    <!-- http://xml/metadatasharing#volumeValue -->

    <owl:DatatypeProperty rdf:about="http://xml/metadatasharing#volumeValue">
        <rdfs:domain rdf:resource="http://xml/metadatasharing#Volume"/>
        <rdfs:range rdf:resource="http://www.w3.org/2001/XMLSchema#integer"/>
        <rdfs:comment></rdfs:comment>
        <rdfs:isDefinedBy rdf:datatype="http://www.w3.org/2001/XMLSchema#string">&lt;http://maec.mitre.org/maec_bundle&gt;</rdfs:isDefinedBy>
        <rdfs:label>volume value</rdfs:label>
    </owl:DatatypeProperty>
    


    <!-- 
    ///////////////////////////////////////////////////////////////////////////////////////
    //
    // Classes
    //
    ///////////////////////////////////////////////////////////////////////////////////////
     -->

    


    <!-- http://xml/metadatasharing#Location -->

    <owl:Class rdf:about="http://xml/metadatasharing#Location">
        <rdfs:subClassOf>
            <owl:Restriction>
                <owl:onProperty rdf:resource="http://xml/metadatasharing#id"/>
                <owl:cardinality rdf:datatype="http://www.w3.org/2001/XMLSchema#nonNegativeInteger">1</owl:cardinality>
            </owl:Restriction>
        </rdfs:subClassOf>
        <rdfs:subClassOf>
            <owl:Restriction>
                <owl:onProperty rdf:resource="http://xml/metadatasharing#locationType"/>
                <owl:cardinality rdf:datatype="http://www.w3.org/2001/XMLSchema#nonNegativeInteger">1</owl:cardinality>
            </owl:Restriction>
        </rdfs:subClassOf>
        <rdfs:subClassOf>
            <owl:Restriction>
                <owl:onProperty rdf:resource="http://xml/metadatasharing#locationValue"/>
                <owl:cardinality rdf:datatype="http://www.w3.org/2001/XMLSchema#nonNegativeInteger">1</owl:cardinality>
            </owl:Restriction>
        </rdfs:subClassOf>
        <rdfs:comment>Characterizes a location</rdfs:comment>
        <rdfs:isDefinedBy rdf:resource="http://xml/metadatasharing"/>
        <rdfs:label>Location</rdfs:label>
    </owl:Class>
    


    <!-- http://xml/metadatasharing#Volume -->

    <owl:Class rdf:about="http://xml/metadatasharing#Volume">
        <rdfs:subClassOf>
            <owl:Restriction>
                <owl:onProperty rdf:resource="http://xml/metadatasharing#id"/>
                <owl:cardinality rdf:datatype="http://www.w3.org/2001/XMLSchema#nonNegativeInteger">1</owl:cardinality>
            </owl:Restriction>
        </rdfs:subClassOf>
        <rdfs:subClassOf>
            <owl:Restriction>
                <owl:onProperty rdf:resource="http://xml/metadatasharing#volumeUnits"/>
                <owl:cardinality rdf:datatype="http://www.w3.org/2001/XMLSchema#nonNegativeInteger">1</owl:cardinality>
            </owl:Restriction>
        </rdfs:subClassOf>
        <rdfs:subClassOf>
            <owl:Restriction>
                <owl:onProperty rdf:resource="http://xml/metadatasharing#volumeValue"/>
                <owl:cardinality rdf:datatype="http://www.w3.org/2001/XMLSchema#nonNegativeInteger">1</owl:cardinality>
            </owl:Restriction>
        </rdfs:subClassOf>
        <rdfs:comment>Specifies the volume quantity</rdfs:comment>
        <rdfs:isDefinedBy rdf:resource="http://xml/metadatasharing"/>
        <rdfs:label>Volume</rdfs:label>
    </owl:Class>
</rdf:RDF>



<!-- Generated by the OWL API (version 4.2.6.20160910-2108) https://github.com/owlcs/owlapi -->

